@prefix dcterms: <http://purl.org/dc/terms/> .
@prefix geo: <http://www.opengis.net/ont/geosparql#> .
@prefix owl: <http://www.w3.org/2002/07/owl#> .
@prefix rdf: <http://www.w3.org/1999/02/22-rdf-syntax-ns#> .
@prefix rdfs: <http://www.w3.org/2000/01/rdf-schema#> .
@prefix skos: <http://www.w3.org/2004/02/skos/core#> .
@prefix xsd: <http://www.w3.org/2001/XMLSchema#> .

<http://www.cidoc-crm.org/cidoc-crm/E10_Transfer_of_Custody> a rdfs:Class ;
    rdfs:label "Übertragung des Gewahrsams"@de,
        "Μεταβίβαση Κατοχής"@el,
        "Transfer of Custody"@en,
        "Transfert de la garde"@fr,
        "Transferência de Custódia"@pt,
        "Пeрeдача Хранeния"@ru,
        "转移监护权"@zh ;
    dcterms:source "CIDOC_CRM_v7.1.3.rdf" ;
    rdfs:comment """This class comprises transfers of the physical custody or the legal responsibility for the physical custody of objects. The recording of the donor or recipient is optional. It is possible that in an instance of E10 Transfer of Custody there is either no donor or no recipient.
Depending on the circumstances, it may describe:
1. the beginning of custody (there is no previous custodian)
2. the end of custody (there is no subsequent custodian)
3. the transfer of custody (transfer from one custodian to the next)
4. the receipt of custody from an unknown source (the previous custodian is unknown)
5. the declared loss of an object (the current or subsequent custodian is unknown)
In the event that only a single kind of transfer of custody occurs, either the legal responsibility for the custody or the actual physical possession of the object but not both, this difference should be expressed using the property P2 has type (is type of).
The sense of physical possession requires that the object of custody be in the hands of the keeper at least with a part representative for the whole. The way, in which a representative part is defined, should ensure that it is unambiguous who keeps a part and who the whole and should be consistent with the identity criteria of the kept instance of E18 Physical Thing.
The interpretation of the museum notion of "accession" differs between institutions. The CIDOC CRM therefore models legal ownership and physical custody separately. Institutions will then model their specific notions of accession and deaccession as combinations of these.
Theft is a specific case of illegal transfer of custody."""@en ;
    rdfs:subClassOf <http://www.cidoc-crm.org/cidoc-crm/E7_Activity> .

<http://www.cidoc-crm.org/cidoc-crm/E11_Modification> a rdfs:Class ;
    rdfs:label "Bearbeitung"@de,
        "Τροποποίηση"@el,
        "Modification"@en,
        "Modification"@fr,
        "Modificação"@pt,
        "Измeнeниe"@ru,
        "修改"@zh ;
    dcterms:source "CIDOC_CRM_v7.1.3.rdf" ;
    rdfs:comment """This class comprises instances of E7 Activity that are undertaken to create, alter or change instances of E24 Physical Human-Made Thing.
This class includes the production of an item from raw materials and other so far undocumented objects. It also includes the conservation treatment of an object.
Since the distinction between modification and production is not always clear, modification is regarded as the more generally applicable concept. This implies that some items may be consumed or destroyed in an instance of E11 Modification, and that others may be produced as a result of it. An event should also be documented using an instance of E81 Transformation if it results in the destruction of one or more objects and the simultaneous production of others using parts or material from the originals. In this case, the new items have separate identities.
An activity undertaken on an object which was designed to alter it, but which, in fact, it did not in any seemingly significant way (such as the application of a solvent during conservation which failed to dissolve any part of the object), is still considered as an instance of E11 Modification. Typically, any such activity will leave at least forensic traces of evidence on the object.
If the instance of E29 Design or Procedure utilized for the modification prescribes the use of specific materials, they should be documented using property P68 foresees use of (use foreseen by): E57 Material of E29 Design or Procedure, rather than via P126 employed (was employed in): E57 Material."""@en ;
    rdfs:subClassOf <http://www.cidoc-crm.org/cidoc-crm/E7_Activity>,
        <http://www.cidoc-crm.org/extensions/crmsci/S18_Alteration> .

<http://www.cidoc-crm.org/cidoc-crm/E12_Production> a rdfs:Class ;
    rdfs:label "Herstellung"@de,
        "Παραγωγή"@el,
        "Production"@en,
        "Production"@fr,
        "Produção"@pt,
        "Изготовлeниe"@ru,
        "生产"@zh ;
    dcterms:source "CIDOC_CRM_v7.1.3.rdf" ;
    rdfs:comment """This class comprises activities that are designed to, and succeed in, creating one or more new items.
It specializes the notion of modification into production. The decision as to whether or not an object is regarded as new is context sensitive. Normally, items are considered “new” if there is no obvious overall similarity between them and the consumed items and material used in their production. In other cases, an item is considered “new” because it becomes relevant to documentation by a modification. For example, the scribbling of a name on a potsherd may make it a voting token. The original potsherd may not be worth documenting, in contrast to the inscribed one.
This entity can be collective: the printing of a thousand books, for example, would normally be considered a single event.
An event should also be documented using an instance of E81 Transformation if it results in the destruction of one or more objects and the simultaneous production of others using parts or material from the originals. In this case, the new items have separate identities and matter is preserved, but identity is not."""@en ;
    rdfs:subClassOf <http://www.cidoc-crm.org/cidoc-crm/E11_Modification>,
        <http://www.cidoc-crm.org/cidoc-crm/E63_Beginning_of_Existence>,
        <http://www.cidoc-crm.org/extensions/crmsci/S17_Physical_Genesis> .

<http://www.cidoc-crm.org/cidoc-crm/E13_Attribute_Assignment> a rdfs:Class ;
    rdfs:label "Merkmalszuweisung"@de,
        "Απόδοση Ιδιοτήτων"@el,
        "Attribute Assignment"@en,
        "Assignation d’attribut"@fr,
        "Atribuição de Característica"@pt,
        "Назначeниe Атрибута"@ru,
        "属性赋值"@zh ;
    dcterms:source "CIDOC_CRM_v7.1.3.rdf" ;
    rdfs:comment """This class comprises the actions of making assertions about one property of an object or any single relation between two items or concepts. The type of the property asserted to hold between two items or concepts can be described by the property P177 assigned property of type (is type of property assigned): E55 Type.
For example, the class describes the actions of people making propositions and statements during certain scientific/scholarly procedures, e.g. the person and date when a condition statement was made, an identifier was assigned, the museum object was measured, etc. Which kinds of such assignments and statements need to be documented explicitly in structures of a schema rather than free text, depends on whether this information should be accessible by structured queries.
This class allows for the documentation of how the respective assignment came about, and whose opinion it was. Note that all instances of properties described in a knowledge base are the opinion of someone. Per default, they are the opinion of the team maintaining the knowledge base. This fact must not individually be registered for all instances of properties provided by the maintaining team, because it would result in an endless recursion of whose opinion was the description of an opinion. Therefore, the use of instances of E13 Attribute Assignment marks the fact that the maintaining team is in general neutral to the validity of the respective assertion, but registers someone else’s opinion and how it came about.
All properties assigned in such an action can also be seen as directly relating the respective pair of items or concepts. Multiple use of instances of E13 Attribute Assignment may possibly lead to a collection of contradictory values."""@en ;
    rdfs:subClassOf <http://www.cidoc-crm.org/cidoc-crm/E7_Activity> .

<http://www.cidoc-crm.org/cidoc-crm/E14_Condition_Assessment> a rdfs:Class ;
    rdfs:label "Zustandsfeststellung"@de,
        "Εκτίμηση Κατάστασης"@el,
        "Condition Assessment"@en,
        "Évaluation d’état matériel"@fr,
        "Avaliação do Estado Material"@pt,
        "Оцeнка Состояния"@ru,
        "状态评估"@zh ;
    dcterms:source "CIDOC_CRM_v7.1.3.rdf" ;
    rdfs:comment """This class describes the act of assessing the state of preservation of an object during a particular period.
The condition assessment may be carried out by inspection, measurement, or through historical research. This class is used to document circumstances of the respective assessment that is relevant to interpret its quality at a later stage, or to continue research on related documents."""@en ;
    rdfs:subClassOf <http://www.cidoc-crm.org/cidoc-crm/E13_Attribute_Assignment> .

<http://www.cidoc-crm.org/cidoc-crm/E15_Identifier_Assignment> a rdfs:Class ;
    rdfs:label "Kennzeichenzuweisung"@de,
        "Απόδοση Αναγνωριστικού"@el,
        "Identifier Assignment"@en,
        "Assignation d’identifiant"@fr,
        "Atribuição de Identificador"@pt,
        "Назначeниe Идeнтификатора"@ru,
        "标识符赋值"@zh ;
    dcterms:source "CIDOC_CRM_v7.1.3.rdf" ;
    rdfs:comment """This class comprises activities that result in the allocation of an identifier to an instance of E1 CRM Entity. An instance of E15 Identifier Assignment may include the creation of the identifier from multiple constituents, which themselves may be instances of E41 Appellation. The syntax and kinds of constituents to be used may be declared in a rule constituting an instance of E29 Design or Procedure.
Examples of such identifiers include Find Numbers, Inventory Numbers, uniform titles in the sense of librarianship and Digital Object Identifiers (DOI). Documenting the act of identifier assignment and deassignment is especially useful when objects change custody or the identification system of an organization is changed. In order to keep track of the identity of things in such cases, it is important to document by whom, when, and for what purpose an identifier is assigned to an item.
The fact that an identifier is a preferred one for an organisation can be expressed by using the property E1 CRM Entity. P48 has preferred identifier (is preferred identifier of): E42 Identifier. It can better be expressed in a context independent form by assigning a suitable E55 Type, such as “preferred identifier assignment”, to the respective instance of E15 Identifier Assignment through the P2 has type (is type of) property."""@en ;
    rdfs:subClassOf <http://www.cidoc-crm.org/cidoc-crm/E13_Attribute_Assignment> .

<http://www.cidoc-crm.org/cidoc-crm/E16_Measurement> a rdfs:Class ;
    rdfs:label "Messung"@de,
        "Μέτρηση"@el,
        "Measurement"@en,
        "Mesurage"@fr,
        "Medição"@pt,
        "Измeрeниe"@ru,
        "测量"@zh ;
    dcterms:source "CIDOC_CRM_v7.1.3.rdf",
        "CRMgeo_v1.2.rdf" ;
    rdfs:comment """This class comprises actions measuring physical properties and other values that can be determined by a systematic, objective procedure of direct observation of particular states of physical reality.
An instance of E16 Measurement may use simple counting or tools, such as yardsticks or radiation detection devices. The interest is in the method and care applied, so that the reliability of the result may be judged at a later stage, or research continued on the associated documents. The date of the event is important for dimensions, which may change value over time, such as the length of an object subject to shrinkage. Methods and devices employed should be associated with instances of E16 Measurement by properties such as P33 used specific technique: E29 Design or Procedure, P125 used object of type: E55 Type, P16 used specific object (was used for): E70 Thing, whereas basic techniques such as "carbon-14 dating" should be encoded using P2 has type (is type of): E55 Type. Details of methods and devices reused or reusable in other instances of E16 Measurement should be documented for these entities rather than the measurements themselves, whereas details of particular execution may be documented by free text or by instantiating adequate sub-activities, if the detail may be of interest for an overarching query.
Regardless whether a measurement is made by an instrument or by human senses, it represents the initial transition from physical reality to information without any other documented information object in between within the reasoning chain that would represent the result of the interaction of the observer or device with reality. Therefore, determining properties of an instance of E90 Symbolic Object is regarded as an instance of E13 Attribute Assignment, which may be inferred from observing and measuring representative carriers. In the case that the carrier can be named, the property P16 used specific object (was used for) should be used to indicate the instance(s) of E18 Physical Thing that was used as the empirical basis for the attribute assignment. For instance, inferring properties of depicted items using image material, such as satellite images, is not regarded as an instance of E16 Measurement, but as a subsequent instance of E13 Attribute Assignment. Rather, only the production of the images, understood as arrays of radiation intensities, is regarded as an instance of E16 Measurement. The same reasoning holds for other sensor data."""@en ;
    rdfs:subClassOf <http://www.cidoc-crm.org/cidoc-crm/E13_Attribute_Assignment>,
        <http://www.cidoc-crm.org/extensions/crmsci/S21_Measurement>,
        <http://www.ics.forth.gr/isl/CRMgeo/S4_Observation> .

<http://www.cidoc-crm.org/cidoc-crm/E17_Type_Assignment> a rdfs:Class ;
    rdfs:label "Typuszuweisung"@de,
        "Απόδοση Τύπου"@el,
        "Type Assignment"@en,
        "Assignation de type"@fr,
        "Atribuição de Tipo"@pt,
        "Назначeниe Типа"@ru,
        "类型赋值"@zh ;
    dcterms:source "CIDOC_CRM_v7.1.3.rdf" ;
    rdfs:comment """This class comprises the actions of classifying items of whatever kind. Such items include objects, specimens, people, actions, and concepts.
This class allows for the documentation of the context of classification acts in cases where the value of the classification depends on the personal opinion of the classifier, and the date that the classification was made. This class also encompasses the notion of “determination,” i.e. the systematic and molecular identification of a specimen in biology."""@en ;
    rdfs:subClassOf <http://www.cidoc-crm.org/cidoc-crm/E13_Attribute_Assignment> .

<http://www.cidoc-crm.org/cidoc-crm/E18_Physical_Thing> a rdfs:Class ;
    rdfs:label "Materielles"@de,
        "Υλικό Πράγμα"@el,
        "Physical Thing"@en,
        "Chose matérielle"@fr,
        "Coisa Material"@pt,
        "Матeриальный Прeдмeт"@ru,
        "实物"@zh ;
    dcterms:source "CIDOC_CRM_v7.1.3.rdf",
        "CRMgeo_v1.2.rdf" ;
    rdfs:comment """This class comprises all persistent physical items with a relatively stable form, human-made or natural.
Depending on the existence of natural boundaries of such things, the CIDOC CRM distinguishes the instances of E19 Physical Object from instances of E26 Physical Feature, such as holes, rivers, pieces of land, etc. Most instances of E19 Physical Object can be moved (if not too heavy), whereas features are integral to the surrounding matter.
An instance of E18 Physical Thing occupies not only a particular geometric space at any instant of its existence, but in the course of its existence it also forms a trajectory through spacetime, which occupies a real, that is phenomenal, volume in spacetime. We include in the occupied space the space filled by the matter of the physical thing and all its inner spaces, such as the interior of a box. For the purpose of more detailed descriptions of the presence of an instance of E18 Physical Thing in space and time it can be associated with its specific instance of E92 Spacetime Volume by the property P196 defines (is defined by).
The CIDOC CRM is generally not concerned with amounts of matter in fluid or gaseous states, as long as they are not confined in an identifiable way for an identifiable minimal time-span."""@en ;
    rdfs:subClassOf <http://www.cidoc-crm.org/cidoc-crm/E72_Legal_Object>,
        <http://www.cidoc-crm.org/extensions/crmsci/S10_Material_Substantial>,
        <http://www.ics.forth.gr/isl/CRMgeo/SP1_Phenomenal_Spacetime_Volume> .

<http://www.cidoc-crm.org/cidoc-crm/E19_Physical_Object> a rdfs:Class ;
    rdfs:label "Materieller Gegenstand"@de,
        "Υλικό Αντικείμενο"@el,
        "Physical Object"@en,
        "Objet matériel"@fr,
        "Objeto Material"@pt,
        "Матeриальный Объeкт"@ru,
        "物质对象"@zh ;
    dcterms:source "CIDOC_CRM_v7.1.3.rdf" ;
    rdfs:comment """This class comprises items of a material nature that are units for documentation and have physical boundaries that separate them completely in an objective way from other objects.
The class also includes all aggregates of objects made for functional purposes of whatever kind, independent of physical coherence, such as a set of chessmen. Typically, instances of E19 Physical Object can be moved (if not too heavy).
In some contexts, such objects, except for aggregates, are also called “bona fide objects”, i.e. naturally defined objects (Smith &amp; Varzi, 2000).
The decision as to what is documented as a complete item, rather than by its parts or components, may be purely administrative or may be a result of the order in which the item was acquired."""@en ;
    rdfs:subClassOf <http://www.cidoc-crm.org/cidoc-crm/E18_Physical_Thing> .

<http://www.cidoc-crm.org/cidoc-crm/E1_CRM_Entity> a rdfs:Class ;
    rdfs:label "CRM Entität"@de,
        "Οντότητα CIDOC CRM"@el,
        "CRM Entity"@en,
        "Entité CRM"@fr,
        "Entidade CRM"@pt,
        "CRM Сущность"@ru,
        "CRM实体"@zh ;
    dcterms:source "CIDOC_CRM_v7.1.3.rdf" ;
    rdfs:comment """This class comprises all things in the universe of discourse of the CIDOC Conceptual Reference Model.
It is an abstract concept providing for three general properties:
Identification by name or appellation, and in particular by a preferred identifier
Classification by type, allowing further refinement of the specific subclass to which an instance belongs
Attachment of free text and other unstructured data for the expression of anything not captured by formal properties
All other classes within the CIDOC CRM are directly or indirectly specialisations of E1 CRM Entity."""@en .

<http://www.cidoc-crm.org/cidoc-crm/E20_Biological_Object> a rdfs:Class ;
    rdfs:label "Biologischer Gegenstand"@de,
        "Βιολογικό Ακτικείμενο"@el,
        "Biological Object"@en,
        "Objet biologique"@fr,
        "Objeto Biológico"@pt,
        "Биологичeский Объeкт"@ru,
        "生物对象"@zh ;
    dcterms:source "CIDOC_CRM_v7.1.3.rdf" ;
    rdfs:comment """This class comprises individual items of a material nature, which live, have lived, or are natural products of or from living organisms.
Artificial objects that incorporate biological elements, such as Victorian butterfly frames, can be documented as both instances of E20 Biological Object and E22 Human-Made Object."""@en ;
    rdfs:subClassOf <http://www.cidoc-crm.org/cidoc-crm/E19_Physical_Object> .

<http://www.cidoc-crm.org/cidoc-crm/E21_Person> a rdfs:Class ;
    rdfs:label "Person"@de,
        "Πρόσωπο"@el,
        "Person"@en,
        "Personne"@fr,
        "Pessoa"@pt,
        "Личность"@ru,
        "人物"@zh ;
    dcterms:source "CIDOC_CRM_v7.1.3.rdf" ;
    rdfs:comment """This class comprises real persons who live or are assumed to have lived.
Legendary figures that may have existed, such as Ulysses and King Arthur, fall into this class if the documentation refers to them as historical figures. In cases where doubt exists as to whether several persons are in fact identical, multiple instances can be created and linked to indicate their relationship. The CIDOC CRM does not propose a specific form to support reasoning about possible identity.
In a bibliographic context, a name presented following the conventions usually employed for personal names will be assumed to correspond to an actual real person (an instance of E21 Person), unless evidence is available to indicate that this is not the case. The fact that a persona may erroneously be classified as an instance of E21 Person does not imply that the concept comprises personae."""@en ;
    rdfs:subClassOf <http://www.cidoc-crm.org/cidoc-crm/E20_Biological_Object>,
        <http://www.cidoc-crm.org/cidoc-crm/E39_Actor> .

<http://www.cidoc-crm.org/cidoc-crm/E22_Human-Made_Object> a rdfs:Class ;
    rdfs:label "Human-Made Object"@en,
        "Objet élaboré par l’humain"@fr,
        "Рукотворный Объeкт"@ru ;
    dcterms:source "CIDOC_CRM_v7.1.3.rdf" ;
    rdfs:comment """This class comprises all persistent physical objects of any size that are purposely created by human activity and have physical boundaries that separate them completely in an objective way from other objects.
The class also includes all aggregates of objects made for functional purposes of whatever kind, independent of physical coherence, such as a set of chessmen."""@en ;
    rdfs:subClassOf <http://www.cidoc-crm.org/cidoc-crm/E19_Physical_Object>,
        <http://www.cidoc-crm.org/cidoc-crm/E24_Physical_Human-Made_Thing> .

<http://www.cidoc-crm.org/cidoc-crm/E24_Physical_Human-Made_Thing> a rdfs:Class ;
    rdfs:label "Physical Human-Made Thing"@en,
        "Chose matérielle élaborée par l’humain"@fr,
        "Матeриальный Рукотворный Объeкт"@ru ;
    dcterms:source "CIDOC_CRM_v7.1.3.rdf" ;
    rdfs:comment """This class comprises all persistent physical items of any size that are purposely created by human activity. This class comprises, besides others, human-made objects, such as a sword, and human-made features, such as rock art. For example, a “cup and ring” carving on bedrock is regarded as instance of E24 Physical Human-Made Thing.
Instances of E24 Physical Human-Made Thing may be the result of modifying pre-existing physical things, preserving larger parts or most of the original matter and structure, which poses the question if they are new or even human-made, the respective interventions of production made on such original material should be obvious and sufficient to regard that the product has a new, distinct identity and intended function and is human-made. Substantial continuity of the previous matter and structure in the new product can be documented by describing the production process also as an instance of E81 Transformation.
Whereas interventions of conservation and repair are not regarded to produce a new instance of E24 Physical Human-Made Thing, the results of preparation of natural history specimens that substantially change their natural or original state should be regarded as instances of E24 Physical Human-Made Things, including the uncovering of petrified biological features from a solid piece of stone. On the other side, scribbling a museum number on a natural object should not be regarded to make it human-made. This notwithstanding, parts, sections, segments, or features of an instance of E24 Physical Human-Made Thing may continue to be non-human-made and preserved during the production process, for example natural pearls used as a part of an eardrop."""@en ;
    rdfs:subClassOf <http://www.cidoc-crm.org/cidoc-crm/E18_Physical_Thing>,
        <http://www.cidoc-crm.org/cidoc-crm/E71_Human-Made_Thing> .

<http://www.cidoc-crm.org/cidoc-crm/E25_Human-Made_Feature> a rdfs:Class ;
    rdfs:label "Human-Made Feature"@en,
        "Caractéristique élaborée par l'humain"@fr,
        "Искусствeнный Признак"@ru ;
    dcterms:source "CIDOC_CRM_v7.1.3.rdf" ;
    rdfs:comment "This class comprises physical features that are purposely created by human activity, such as scratches, artificial caves, artificial water channels, etc. In particular, it includes the information encoding features on mechanical or digital carriers."@en ;
    rdfs:subClassOf <http://www.cidoc-crm.org/cidoc-crm/E24_Physical_Human-Made_Thing>,
        <http://www.cidoc-crm.org/cidoc-crm/E26_Physical_Feature> .

<http://www.cidoc-crm.org/cidoc-crm/E26_Physical_Feature> a rdfs:Class ;
    rdfs:label "Materielles Merkmal"@de,
        "Υλικό Μόρφωμα"@el,
        "Physical Feature"@en,
        "Caractéristique physique"@fr,
        "Característica Material"@pt,
        "Физичeский Признак"@ru,
        "物理特征"@zh ;
    dcterms:source "CIDOC_CRM_v7.1.3.rdf" ;
    rdfs:comment """This class comprises identifiable features that are physically attached in an integral way to particular physical objects.
Instances of E26 Physical Feature share many of the attributes of instances of E19 Physical Object. They may have a one-dimensional, two-dimensional, or three-dimensional geometric extent, but there are no natural borders that separate them completely in an objective way from the carrier objects. For example, a doorway is a feature but the door itself, being attached by hinges, is not.
Instances of E26 Physical Feature can be features in a narrower sense, such as scratches, holes, reliefs, surface colours, reflection zones in an opal crystal or a density change in a piece of wood. In the wider sense, they are portions of particular objects with partially imaginary borders, such as the core of the Earth, an area of property on the surface of the Earth, a landscape or the head of a contiguous marble statue. They can be measured and dated, and it is sometimes possible to state who or what is or was responsible for them. They cannot be separated from the carrier object, but a segment of the carrier object may be identified (or sometimes removed) carrying the complete feature.
This definition coincides with the definition of “fiat objects”, with the exception of aggregates of “bona fide objects” (Smith &amp; Varzi, 2000)."""@en ;
    rdfs:subClassOf <http://www.cidoc-crm.org/cidoc-crm/E18_Physical_Thing> .

<http://www.cidoc-crm.org/cidoc-crm/E27_Site> a rdfs:Class ;
    rdfs:label "Gelände"@de,
        "Φυσικός Χώρος"@el,
        "Site"@en,
        "Site"@fr,
        "Lugar"@pt,
        "Мeстоположeниe"@ru,
        "场地"@zh ;
    dcterms:source "CIDOC_CRM_v7.1.3.rdf" ;
    rdfs:comment """This class comprises pieces of land or sea floor.
In contrast to the purely geometric notion of E53 Place, this class describes constellations of matter on the surface of the Earth or other celestial body, which can be represented by photographs, paintings, and maps.
Instances of E27 Site are composed of relatively immobile material items and features in a particular configuration at a particular location."""@en ;
    rdfs:subClassOf <http://www.cidoc-crm.org/cidoc-crm/E26_Physical_Feature>,
        <http://www.cidoc-crm.org/extensions/crmsci/S20_Rigid_Physical_Feature> .

<http://www.cidoc-crm.org/cidoc-crm/E28_Conceptual_Object> a rdfs:Class ;
    rdfs:label "Begrifflicher Gegenstand"@de,
        "Νοητικό Αντικείμενο"@el,
        "Conceptual Object"@en,
        "Objet conceptuel"@fr,
        "Objeto Conceitual"@pt,
        "Концeптуальный Объeкт"@ru,
        "概念对象"@zh ;
    dcterms:source "CIDOC_CRM_v7.1.3.rdf" ;
    rdfs:comment """This class comprises non-material products of our minds and other human produced data that have become objects of a discourse about their identity, circumstances of creation, or historical implication. The production of such information might have been supported by the use of technical devices such as cameras or computers.
Characteristically, instances of this class are created, invented or thought by someone, and then may be documented or communicated between persons. Instances of E28 Conceptual Object have the ability to exist on more than one particular carrier at the same time, such as paper, electronic signals, marks, audio media, paintings, photos, human memories, etc.
They cannot be destroyed. They exist as long as they can be found on at least one carrier or in at least one human memory. Their existence ends when the last carrier and the last memory are lost."""@en ;
    rdfs:subClassOf <http://www.cidoc-crm.org/cidoc-crm/E71_Human-Made_Thing> .

<http://www.cidoc-crm.org/cidoc-crm/E29_Design_or_Procedure> a rdfs:Class ;
    rdfs:label "Entwurf oder Verfahren"@de,
        "Σχέδιο"@el,
        "Design or Procedure"@en,
        "Conceptualisation ou procédure"@fr,
        "Projeto ou Procedimento"@pt,
        "Проeкт или Процeдура"@ru,
        "设计或程序"@zh ;
    dcterms:source "CIDOC_CRM_v7.1.3.rdf" ;
    rdfs:comment """This class comprises documented plans for the execution of actions in order to achieve a result of a specific quality, form, or contents. In particular, it comprises plans for deliberate human activities that may result in new instances of E71 Human-Made Thing or for shaping or guiding the execution of an instance of E7 Activity.
Instances of E29 Design or Procedure can be structured in parts and sequences or depend on others.
This is modelled using P69 has association with (is associated with): E29 Design or Procedure.
Designs or procedures can be seen as one of the following:
1. A schema for the activities it describes
2. A schema of the products that result from their application
3. An independent intellectual product that may have never been applied, such as Leonardo da Vinci’s famous plans for flying machines
Because designs or procedures may never be applied or only partially executed, the CIDOC CRM models a loose relationship between the plan and the respective product."""@en ;
    rdfs:subClassOf <http://www.cidoc-crm.org/cidoc-crm/E73_Information_Object> .

<http://www.cidoc-crm.org/cidoc-crm/E2_Temporal_Entity> a rdfs:Class ;
    rdfs:label "Geschehendes"@de,
        "Έγχρονη Οντότητα"@el,
        "Temporal Entity"@en,
        "Entité temporelle"@fr,
        "Entidade Temporal"@pt,
        "Врeмeнная Сущность"@ru,
        "时序实体"@zh ;
    dcterms:source "CIDOC_CRM_v7.1.3.rdf" ;
    rdfs:comment """This class comprises all phenomena, such as the instances of E4 Periods and E5 Events, which happen over a limited extent in time. This extent in time must be contiguous, i.e., without gaps. In case the defining kinds of phenomena for an instance of E2 Temporal Entity cease to happen, and occur later again at another time, we regard that the former instance of E2 Temporal Entity has ended and a new instance has come into existence. In more intuitive terms, the same event cannot happen twice.
In some contexts, such phenomena are also called perdurants. This class is disjoint from E77 Persistent Item and is an abstract class that typically has no direct instances. E2 Temporal Entity is specialized into E4 Period, which applies to a particular geographic area (defined with a greater or lesser degree of precision), and E3 Condition State, which applies to instances of E18 Physical Thing."""@en ;
    rdfs:subClassOf <http://www.cidoc-crm.org/cidoc-crm/E1_CRM_Entity> .

<http://www.cidoc-crm.org/cidoc-crm/E30_Right> a rdfs:Class ;
    rdfs:label "Recht"@de,
        "Δικαίωμα"@el,
        "Right"@en,
        "Droit"@fr,
        "Direitos"@pt,
        "Право"@ru,
        "权限"@zh ;
    dcterms:source "CIDOC_CRM_v7.1.3.rdf" ;
    rdfs:comment """This class comprises legal privileges concerning material and immaterial things or their derivatives.
These include reproduction and property rights."""@en ;
    rdfs:subClassOf <http://www.cidoc-crm.org/cidoc-crm/E89_Propositional_Object> .

<http://www.cidoc-crm.org/cidoc-crm/E31_Document> a rdfs:Class ;
    rdfs:label "Dokument"@de,
        "Τεκμήριο"@el,
        "Document"@en,
        "Document"@fr,
        "Documento"@pt,
        "Докумeнт"@ru,
        "文献"@zh ;
    dcterms:source "CIDOC_CRM_v7.1.3.rdf" ;
    rdfs:comment """This class comprises identifiable immaterial items that make propositions about reality.
These propositions may be expressed in text, graphics, images, audiograms, videograms, or by other similar means. Documentation databases are regarded as instances of E31 Document. This class should not be confused with the concept “document” in Information Technology, which is compatible with E73 Information Object."""@en ;
    rdfs:subClassOf <http://www.cidoc-crm.org/cidoc-crm/E73_Information_Object> .

<http://www.cidoc-crm.org/cidoc-crm/E32_Authority_Document> a rdfs:Class ;
    rdfs:label "Referenzdokument"@de,
        "Πηγή Καθιερωμένων Όρων"@el,
        "Authority Document"@en,
        "Document de référence"@fr,
        "Documento de Referência"@pt,
        "Официальный Докумeнт"@ru,
        "规范文档"@zh ;
    dcterms:source "CIDOC_CRM_v7.1.3.rdf" ;
    rdfs:comment "This class comprises encyclopaedia, thesauri, authority lists and other documents that define terminology or conceptual systems for consistent use."@en ;
    rdfs:subClassOf <http://www.cidoc-crm.org/cidoc-crm/E31_Document> .

<http://www.cidoc-crm.org/cidoc-crm/E33_E41_Linguistic_Appellation> a rdfs:Class ;
    rdfs:label "Linguistic Appellation"@en ;
    dcterms:source "CIDOC_CRM_v7.1.3.rdf" ;
    rdfs:subClassOf <http://www.cidoc-crm.org/cidoc-crm/E33_Linguistic_Object>,
        <http://www.cidoc-crm.org/cidoc-crm/E41_Appellation> .

<http://www.cidoc-crm.org/cidoc-crm/E33_Linguistic_Object> a rdfs:Class ;
    rdfs:label "Sprachlicher Gegenstand"@de,
        "Γλωσσικό Αντικείμενο"@el,
        "Linguistic Object"@en,
        "Objet linguistique"@fr,
        "Objeto Lingüístico"@pt,
        "Лингвистичeский Объeкт"@ru,
        "语言对象"@zh ;
    dcterms:source "CIDOC_CRM_v7.1.3.rdf" ;
    rdfs:comment """This class comprises identifiable expressions in natural language or languages.
Instances of E33 Linguistic Object can be expressed in many ways: e.g. as written texts, recorded speech, or sign language. However, the CIDOC CRM treats instances of E33 Linguistic Object independently from the medium or method by which they are expressed. Expressions in formal languages, such as computer code or mathematical formulae, are not treated as instances of E33 Linguistic Object by the CIDOC CRM. These should be modelled as instances of E73 Information Object.
In general, an instance of E33 Linguistic Object may also contain non-linguistic information, often of artistic or aesthetic value. Only in cases in which the content of an instance of E33 Linguistic Object can completely be expressed by a series of binary-encoded symbols, its content may be documented within a respective knowledge base by the property P190 has symbolic content: E62 String. Otherwise, it should be understood as an identifiable digital resource only available independently from the respective knowledge base.
In other cases, such as pages of an illuminated manuscript or recordings containing speech in a language supported by a writing system, the linguistic part of the content of an instance of E33 Linguistic Object may be documented within a respective knowledge base in a note by P3 has note: E62 String. Otherwise, it may be described using the property P165 incorporates (is incorporated in): E73 Information Object as a different object with its own identity."""@en ;
    rdfs:subClassOf <http://www.cidoc-crm.org/cidoc-crm/E73_Information_Object> .

<http://www.cidoc-crm.org/cidoc-crm/E34_Inscription> a rdfs:Class ;
    rdfs:label "Inschrift"@de,
        "Επιγραφή"@el,
        "Inscription"@en,
        "Inscription"@fr,
        "Inscrição"@pt,
        "Надпись"@ru,
        "题识"@zh ;
    dcterms:source "CIDOC_CRM_v7.1.3.rdf" ;
    rdfs:comment """This class comprises recognisable texts that can be attached to instances of E24 Physical Human-Made Thing.
The transcription of the text can be documented in a note by P3 has note: E62 String. The alphabet used can be documented by P2 has type: E55 Type. This class is not intended to describe the idiosyncratic characteristics of an individual physical embodiment of an inscription, but the underlying prototype. The physical embodiment is modelled in the CIDOC CRM as instances of E24 Physical Human-Made Thing.
The relationship of a physical copy of a book to the text it contains is modelled using E18 Physical Thing. P128 carries (is carried by): E33 Linguistic Object."""@en ;
    rdfs:subClassOf <http://www.cidoc-crm.org/cidoc-crm/E33_Linguistic_Object>,
        <http://www.cidoc-crm.org/cidoc-crm/E37_Mark> .

<http://www.cidoc-crm.org/cidoc-crm/E35_Title> a rdfs:Class ;
    rdfs:label "Titel"@de,
        "Τίτλος"@el,
        "Title"@en,
        "Titre"@fr,
        "Título"@pt,
        "Названиe"@ru,
        "题名"@zh ;
    dcterms:source "CIDOC_CRM_v7.1.3.rdf" ;
    rdfs:comment """This class comprises the textual strings that within a cultural context can be clearly identified as titles due to their form. Being a subclass of E41 Appellation, E35 Title can only be used when such a string is actually used as a title of a work, such as a text, an artwork, or a piece of music.
Titles are proper noun phrases or verbal phrases, and should not be confused with generic object names such as “chair”, “painting”, or “book” (the latter are common nouns that stand for instances of E55 Type). Titles may be assigned by the creator of the work itself, or by a social group.
This class also comprises the translations of titles that are used as surrogates for the original titles in different social contexts."""@en ;
    rdfs:subClassOf <http://www.cidoc-crm.org/cidoc-crm/E33_Linguistic_Object>,
        <http://www.cidoc-crm.org/cidoc-crm/E41_Appellation> .

<http://www.cidoc-crm.org/cidoc-crm/E36_Visual_Item> a rdfs:Class ;
    rdfs:label "Bildliches"@de,
        "Οπτικό Στοιχείο"@el,
        "Visual Item"@en,
        "Entité visuelle"@fr,
        "Item Visual"@pt,
        "Визуальный Прeдмeт"@ru,
        "可视项"@zh ;
    dcterms:source "CIDOC_CRM_v7.1.3.rdf" ;
    rdfs:comment """This class comprises the intellectual or conceptual aspects of recognisable marks and images.
This class does not intend to describe the idiosyncratic characteristics of an individual physical embodiment of a visual item, but the underlying prototype. For example, a mark such as the ICOM logo is generally considered to be the same logo when used on any number of publications. The size, orientation, and colour may change, but the logo remains uniquely identifiable. The same is true of images that are reproduced many times. This means that visual items are independent of their physical support.
The E36 Visual Item class provides a means of identifying and linking together instances of E24 Physical Human-Made Thing that carry the same visual symbols, marks, or images, etc. The property P62 depicts (is depicted by) between E24 Physical Human-Made Thing and the depicted subjects (E1 CRM Entity) can be regarded as a shortcut of the more fully developed path from E24 Physical Human-Made Thing through P65 shows visual item (is shown by), E36 Visual Item, P138 represents (has representation) to E1 CRM Entity, which in addition captures the optical features of the depiction."""@en ;
    rdfs:subClassOf <http://www.cidoc-crm.org/cidoc-crm/E73_Information_Object> .

<http://www.cidoc-crm.org/cidoc-crm/E37_Mark> a rdfs:Class ;
    rdfs:label "Marke"@de,
        "Σήμανση"@el,
        "Mark"@en,
        "Marque"@fr,
        "Marca"@pt,
        "Знак"@ru,
        "标记"@zh ;
    dcterms:source "CIDOC_CRM_v7.1.3.rdf" ;
    rdfs:comment """This class comprises symbols, signs, signatures, or short texts applied to instances of E24 Physical Human-Made Thing by arbitrary techniques, often in order to indicate such things as creator, owner, dedications, purpose, or to communicate information generally. Instances of E37 Mark do not represent the actual image of a mark, but the abstract ideal (or archetype) as used for codification in reference documents forming cultural documentation.
This class specifically excludes features that have no semantic significance, such as scratches or tool marks. These should be documented as instances of E25 Human-Made Feature."""@en ;
    rdfs:subClassOf <http://www.cidoc-crm.org/cidoc-crm/E36_Visual_Item> .

<http://www.cidoc-crm.org/cidoc-crm/E39_Actor> a rdfs:Class ;
    rdfs:label "Akteur"@de,
        "Δράστης"@el,
        "Actor"@en,
        "Actant"@fr,
        "Agente"@pt,
        "Дeйствующий Субъeкт"@ru,
        "参与者"@zh ;
    dcterms:source "CIDOC_CRM_v7.1.3.rdf" ;
    rdfs:comment "This class comprises people, either individually or in groups, who have the potential to perform intentional actions of kinds for which they can be held responsible."@en ;
    rdfs:subClassOf <http://www.cidoc-crm.org/cidoc-crm/E77_Persistent_Item> .

<http://www.cidoc-crm.org/cidoc-crm/E3_Condition_State> a rdfs:Class ;
    rdfs:label "Zustandsphase"@de,
        "Κατάσταση"@el,
        "Condition State"@en,
        "État matériel"@fr,
        "Estado Material"@pt,
        "Состояниe"@ru,
        "条件状态"@zh ;
    dcterms:source "CIDOC_CRM_v7.1.3.rdf" ;
    rdfs:comment """This class comprises the states of objects characterised by a certain condition over a time-span.
An instance of this class describes the prevailing physical condition of any material object or feature during a specific instance of E52 Time-Span. In general, the time-span for which a certain condition can be asserted may be shorter than the real time-span, for which this condition held.
The nature of that condition can be described using P2 has type. For example, the instance of E3 Condition State “condition of the SS Great Britain between 22-nd September 1846 and 27-th August 1847” can be characterized as an instance “wrecked” of E55 Type."""@en ;
    rdfs:subClassOf <http://www.cidoc-crm.org/cidoc-crm/E2_Temporal_Entity> .

<http://www.cidoc-crm.org/cidoc-crm/E41_Appellation> a rdfs:Class ;
    rdfs:label "Benennung"@de,
        "Ονομασία"@el,
        "Appellation"@en,
        "Appellation"@fr,
        "Designação"@pt,
        "Обозначeниe"@ru,
        "称谓"@zh ;
    dcterms:source "CIDOC_CRM_v7.1.3.rdf" ;
    rdfs:comment """This class comprises all signs, either meaningful or not, or arrangements of signs following a specific syntax, that are used or can be used to refer to and identify a specific instance of some class within a certain context.
Instances of E41 Appellation do not identify things by their meaning, even if they happen to have one, but by convention, tradition, or agreement. Instances of E41 Appellation are cultural constructs; as such, they have a context, a history, and a use in time and space by some group of users. A given instance of E41 Appellation can have alternative forms, i.e. other instances of E41 Appellation that are regarded as equivalent, regardless of the thing it denotes.
Different languages may use different appellations for the same thing, such as the names of major cities. Some appellations may be formulated using a valid noun phrase of a particular language. In these cases, the respective instances of E41 Appellation should also be declared as instances of E33 Linguistic Object. Then the language using the appellation can be declared with the property P72 has language: E56 Language.
Instances of E41 Appellation may be used to identify any instance of E1 CRM Entity and sometimes are characteristic for instances of more specific subclasses of E1 CRM Entity, such as for instances of E52 Time-Span (for instance “dates”), E39 Actor, E53 Place or E28 Conceptual Object. Postal addresses and E-mail addresses are characteristic examples of identifiers used by services transporting things between clients.
Even numerically expressed identifiers for extents in space or time are also regarded as instances of E41 Appellation, such as Gregorian dates or spatial coordinates, even though they allow for determining some time or location by a known procedure starting from a reference point and by virtue of that fact play a double role as instances of E59 Primitive Value.
E41 Appellation should not be confused with the act of naming something. Cf. E15 Identifier Assignment."""@en ;
    rdfs:subClassOf <http://www.cidoc-crm.org/cidoc-crm/E90_Symbolic_Object> .

<http://www.cidoc-crm.org/cidoc-crm/E42_Identifier> a rdfs:Class ;
    rdfs:label "Kennung"@de,
        "Κωδικός Αναγνώρισης"@el,
        "Identifier"@en,
        "Identifiant"@fr,
        "Identificador de Objeto"@pt,
        "Идeнтификатор"@ru,
        "标识符"@zh ;
    dcterms:source "CIDOC_CRM_v7.1.3.rdf" ;
    rdfs:comment """This class comprises strings or codes assigned to instances of E1 CRM Entity in order to identify them uniquely and permanently within the context of one or more organisations. Such codes are often known as inventory numbers, registration codes, etc. and are typically composed of alphanumeric sequences. Postal addresses, telephone numbers, URLs and e-mail addresses are characteristic examples of identifiers used by services transporting things between clients.
The class E42 Identifier is not normally used for machine-generated identifiers used for automated processing unless these are also used by human agents."""@en ;
    rdfs:subClassOf <http://www.cidoc-crm.org/cidoc-crm/E41_Appellation> .

<http://www.cidoc-crm.org/cidoc-crm/E4_Period> a rdfs:Class ;
    rdfs:label "Phase"@de,
        "Περίοδος"@el,
        "Period"@en,
        "Période"@fr,
        "Período"@pt,
        "Пeриод"@ru,
        "时期"@zh ;
    dcterms:source "CIDOC_CRM_v7.1.3.rdf",
        "CRMgeo_v1.2.rdf" ;
    rdfs:comment """This class comprises sets of coherent phenomena or cultural manifestations occurring in time and space.
It is the social or physical coherence of these phenomena that identify an instance of E4 Period and not the associated spatiotemporal extent. This extent is only the “ground” or space in an abstract physical sense that the actual process of growth, spread and retreat has covered. Consequently, different periods can overlap and coexist in time and space, such as when a nomadic culture exists in the same area and time as a sedentary culture. This also means that overlapping land use rights, common among first nations, amounts to overlapping periods.
Often, this class is used to describe prehistoric or historic periods such as the “Neolithic Period”, the “Ming Dynasty” or the “McCarthy Era”, but also geopolitical units and activities of settlements are regarded as special cases of E4 Period. However, there are no assumptions about the scale of the associated phenomena. In particular all events are seen as synthetic processes consisting of coherent phenomena. Therefore, E4 Period is a superclass of E5 Event. For example, a modern clinical birth, an instance of E67 Birth, can be seen as both a single event, i.e. an instance of E5 Event, and as an extended period, i.e. an instance of E4 Period, that consists of multiple physical processes and complementary activities performed by multiple instances of E39 Actor.
E4 Period is a subclass of E2 Temporal Entity and of E92 Spacetime Volume. The latter is intended as a phenomenal spacetime volume as defined in CIDOC CRMgeo (Doerr &amp; Hiebel, 2013). By virtue of this multiple inheritance, it is possible to discuss the physical extent of an instance of E4 Period without representing each instance of it together with an instance of its associated spacetime volume. This model combines two quite different kinds of substance: an instance of E4 Period is a phenomenon while an instance of E92 Spacetime Volume is an aggregation of points in spacetime. However, the real spatiotemporal extent of an instance of E4 Period is regarded to be unique to it due to all its details and fuzziness; its identity and existence depends uniquely on the identity of the instance of E4 Period. Therefore, this multiple inheritance is unambiguous and effective and furthermore corresponds to the intuitions of natural language.
Typical use of this class in cultural heritage documentation is for documenting cultural and artistic periods. There are two different conceptualisations of ‘artistic style’, defined either by physical features or by historical context. For example, “Impressionism” can be viewed as a period in the European sphere of influence lasting from approximately 1870 to 1905 during which paintings with particular characteristics were produced by a group of artists that included (among others) Monet, Renoir, Pissarro, Sisley and Degas. Alternatively, it can be regarded as a style applicable to all paintings sharing the characteristics of the works produced by the Impressionist painters, regardless of historical context. The first interpretation is an instance of E4 Period, and the second defines morphological object types that fall under E55 Type.
A geopolitical unit as a specific case of an instance of E4 Period is the set of activities and phenomena related to the claim of power, the consequences of belonging to a jurisdictional area and an administrative system that establishes a geopolitical unit. Examples from the modern period are countries or administrative areas of countries such as districts whose actions and structures define activities and phenomena in the area that they intend to govern. The borders of geopolitical units are often defined in contracts or treaties although they may deviate from the actual practice. The spatiotemporal properties of Geopolitical units can be modelled through the properties inherited from E92 Spacetime Volume.
Another specific case of an instance of E4 Period is the actual extent of the set of activities and phenomena as evidenced by their physical traces that define a settlement, such as the populated period of Nineveh."""@en ;
    rdfs:subClassOf <http://www.cidoc-crm.org/cidoc-crm/E2_Temporal_Entity>,
        <http://www.cidoc-crm.org/cidoc-crm/E92_Spacetime_Volume>,
        <http://www.ics.forth.gr/isl/CRMgeo/SP1_Phenomenal_Spacetime_Volume> .

<http://www.cidoc-crm.org/cidoc-crm/E52_Time-Span> a rdfs:Class ;
    rdfs:label "Zeitspanne"@de,
        "Χρονικό Διάστημα"@el,
        "Time-Span"@en,
        "Intervalle temporel"@fr,
        "Período de Tempo"@pt,
        "Интeрвал Врeмeни"@ru,
        "时段"@zh ;
    dcterms:source "CIDOC_CRM_v7.1.3.rdf" ;
    rdfs:comment """This class comprises abstract temporal extents, in the sense of Galilean physics, having a beginning, an end, and a duration.
Instances of E52 Time-Span have no semantic connotations about phenomena happening within the temporal extent they represent. They do not convey any meaning other than a positioning on the “time-line” of chronology. The actual extent of an instance of E52 Time-Span can be approximated by properties of E52 Time-Span giving inner and outer bounds in the form of dates (instances of E61 Time Primitive). Comparing knowledge about time-spans is fundamental for chronological reasoning.
Some instances of E52 Time-Span may be defined as the actual, in principle observable, temporal extent of instances of E2 Temporal Entity via the property P4 has time-span (is time-span of): E52 Time-Span. They constitute phenomenal time-spans as defined in CRMgeo (Doerr &amp; Hiebel 2013). Since our knowledge of history is imperfect and physical phenomena are fuzzy in nature, the extent of phenomenal time-spans can only be described in approximation. An extreme case of approximation, might, for example, define an instance of E52 Time-Span having unknown beginning, end and duration. It may, nevertheless, be associated with other descriptions by which people can infer knowledge about it, such as in relative chronologies.
Some instances of E52 may be defined precisely as representing a declaration of a temporal extent, as, for instance, done in a business contract. They constitute declarative time-spans as defined in CRMgeo (Doerr &amp; Hiebel 2013) and can be described via the property E61 Time Primitive P170 defines time (time is defined by): E52 Time-Span.
When used as a common E52 Time-Span for two events, it will nevertheless describe them as being simultaneous, even if nothing else is known."""@en ;
    rdfs:subClassOf <http://www.cidoc-crm.org/cidoc-crm/E1_CRM_Entity> .

<http://www.cidoc-crm.org/cidoc-crm/E53_Place> a rdfs:Class ;
    rdfs:label "Ort"@de,
        "Τόπος"@el,
        "Place"@en,
        "Lieu"@fr,
        "Local"@pt,
        "Мeсто"@ru,
        "地点"@zh ;
    dcterms:source "CIDOC_CRM_v7.1.3.rdf" ;
    rdfs:comment """This class comprises extents in the natural space where people live, in particular on the surface of the Earth, in the pure sense of physics: independent from temporal phenomena and matter. They may serve describing the physical location of things or phenomena or other areas of interest. Geometrically, instances of E53 Place constitute single contiguous areas or a finite aggregation of disjoint areas in space which are each individually contiguous. They may have fuzzy boundaries.
The instances of E53 Place are usually determined by reference to the position of “immobile” objects such as buildings, cities, mountains, rivers, or dedicated geodetic marks, but may also be determined by reference to mobile objects. A Place can be determined by combining a frame of reference and a location with respect to this frame.
It is sometimes argued that instances of E53 Place are best identified by global coordinates or absolute reference systems. However, relative references are often more relevant in the context of cultural documentation and tend to be more precise. In particular, people are often interested in position in relation to large, mobile objects, such as ships. For example, the Place at which Nelson died is known with reference to a large mobile object, i.e. H.M.S Victory. A resolution of this Place in terms of absolute coordinates would require knowledge of the movements of the vessel and the precise time of death, either of which may be revised, and the result would lack historical and cultural relevance.
Any instance of E18 Physical Thing can serve as a frame of reference for an instance of E53 Place. This may be documented using the property P157 is at rest relative to (provides reference space for)."""@en ;
    rdfs:subClassOf <http://www.cidoc-crm.org/cidoc-crm/E1_CRM_Entity> .

<http://www.cidoc-crm.org/cidoc-crm/E54_Dimension> a rdfs:Class ;
    rdfs:label "Maß"@de,
        "Μέγεθος"@el,
        "Dimension"@en,
        "Dimension"@fr,
        "Dimensão"@pt,
        "Размeр"@ru,
        "度量规格"@zh ;
    dcterms:source "CIDOC_CRM_v7.1.3.rdf" ;
    rdfs:comment """This class comprises quantifiable properties that can be measured by some calibrated means and can be approximated by values, i.e. points or regions in a mathematical or conceptual space, such as natural or real numbers, RGB values, etc.
An instance of E54 Dimension represents the empirical or theoretically derived quantity, including the precision tolerances resulting from the particular method or calculation. The identity of an instance of E54 Dimension depends on the method of its determination because each method may produce different values even when determining comparable qualities. For instance, the wingspan of a bird alive or dead is a different dimension. Thermoluminescence dating and Rehydroxylation [RHX] dating are different dimensions of temporal distance from now, even if they aim at dating the same object. The method of determination should be expressed using the property P2 has type (is type of). Note that simple terms such as “diameter” or “length” are normally insufficient to unambiguously describe a respective dimension. In contrast, “maximum linear extent” may be sufficient.
The properties of the class E54 Dimension allow for expressing the numerical approximation of the values of instances of E54 Dimension adequate to the precision of the applied method of determination. If the respective quantity belongs to a non-discrete space according to the laws of physics, such as spatial distances, it is recommended to record them as approximations by intervals or regions of indeterminacy enclosing the assumed true values. For instance, a length of 5 cm may be recorded as 4.5-5.5 cm, according to the precision of the respective observation. Note, that comparability of values described in different units depends critically on the representation as value regions.
Numerical approximations in archaic instances of E58 Measurement Unit used in historical records should be preserved. Equivalents corresponding to current knowledge should be recorded as additional instances of E54 Dimension, as appropriate."""@en ;
    rdfs:subClassOf <http://www.cidoc-crm.org/cidoc-crm/E1_CRM_Entity> .

<http://www.cidoc-crm.org/cidoc-crm/E55_Type> a rdfs:Class ;
    rdfs:label "Typus"@de,
        "Τύπος"@el,
        "Type"@en,
        "Type"@fr,
        "Tipo"@pt,
        "Tип"@ru,
        "类型"@zh ;
    dcterms:source "CIDOC_CRM_v7.1.3.rdf" ;
    rdfs:comment """This class comprises concepts denoted by terms from thesauri and controlled vocabularies used to characterize and classify instances of CIDOC CRM classes. Instances of E55 Type represent concepts, in contrast to instances of E41 Appellation which are used to name instances of CIDOC CRM classes.
E55 Type provides an interface to domain specific ontologies and thesauri. These can be represented in the CIDOC CRM as subclasses of E55 Type, forming hierarchies of terms, i.e. instances of E55 Type linked via P127 has broader term (has narrower term): E55 Type. Such hierarchies may be extended with additional properties."""@en ;
    rdfs:subClassOf <http://www.cidoc-crm.org/cidoc-crm/E28_Conceptual_Object> .

<http://www.cidoc-crm.org/cidoc-crm/E56_Language> a rdfs:Class ;
    rdfs:label "Sprache"@de,
        "Γλώσσα"@el,
        "Language"@en,
        "Langue"@fr,
        "Língua"@pt,
        "Язык"@ru,
        "语种"@zh ;
    dcterms:source "CIDOC_CRM_v7.1.3.rdf" ;
    rdfs:comment """This class is a specialization of E55 Type and comprises the natural languages in the sense of concepts.
This type is used categorically in the model without reference to instances of it, i.e. the Model does not foresee the description of instances of instances of E56 Language, e.g. “instances of Mandarin Chinese”.
It is recommended that internationally or nationally agreed codes and terminology should be used to denote instances of E56 Language, such as those defined in ISO 639-3:2007 and later versions."""@en ;
    rdfs:subClassOf <http://www.cidoc-crm.org/cidoc-crm/E55_Type> .

<http://www.cidoc-crm.org/cidoc-crm/E57_Material> a rdfs:Class ;
    rdfs:label "Material"@de,
        "Υλικό"@el,
        "Material"@en,
        "Matériau"@fr,
        "Material"@pt,
        "Матeриал"@ru,
        "材质"@zh ;
    dcterms:source "CIDOC_CRM_v7.1.3.rdf" ;
    rdfs:comment """This class is a specialization of E55 Type and comprises the concepts of materials.
Instances of E57 Material may denote properties of matter before its use, during its use, and as incorporated in an object, such as ultramarine powder, tempera paste, reinforced concrete. Discrete pieces of raw-materials kept in museums, such as bricks, sheets of fabric, pieces of metal, should be modelled individually in the same way as other objects. Discrete used or processed pieces, such as the stones from Nefer Titi's temple, should be modelled as parts (cf. P46 is composed of (forms part of): E18 Physical Thing).
This type is used categorically in the model without reference to instances of it, i.e. the Model does not foresee the description of instances of instances of E57 Material, e.g. “instances of gold”.
It is recommended that internationally or nationally agreed codes and terminology should be used."""@en ;
    rdfs:subClassOf <http://www.cidoc-crm.org/cidoc-crm/E55_Type> .

<http://www.cidoc-crm.org/cidoc-crm/E58_Measurement_Unit> a rdfs:Class ;
    rdfs:label "Maßeinheit"@de,
        "Μονάδα Μέτρησης"@el,
        "Measurement Unit"@en,
        "Unité de mesure"@fr,
        "Unidade de Medida"@pt,
        "Eдиница Измeрeния"@ru,
        "测量单位"@zh ;
    dcterms:source "CIDOC_CRM_v7.1.3.rdf" ;
    rdfs:comment """This class is a specialization of E55 Type and comprises the types of measurement units: feet, inches, centimetres, litres, lumens, etc.
This type is used categorically in the model without reference to instances of it, i.e. the model does not foresee the description of instances of instances of E58 Measurement Unit, e.g. “instances of cm”.
Système International (SI) units or internationally recognized non-SI terms should be used whenever possible, such as those defined by ISO80000:2009. Archaic Measurement Units used in historical records should be preserved."""@en ;
    rdfs:subClassOf <http://www.cidoc-crm.org/cidoc-crm/E55_Type> .

<http://www.cidoc-crm.org/cidoc-crm/E5_Event> a rdfs:Class ;
    rdfs:label "Ereignis"@de,
        "Συμβάν"@el,
        "Event"@en,
        "Évènement"@fr,
        "Evento"@pt,
        "Событиe"@ru,
        "事件"@zh ;
    dcterms:source "CIDOC_CRM_v7.1.3.rdf" ;
    rdfs:comment """This class comprises distinct, delimited and coherent processes and interactions of a material nature, in cultural, social or physical systems, involving and affecting instances of E77 Persistent Item in a way characteristic of the kind of process. Typical examples are meetings, births, deaths, actions of decision taking, making or inventing things, but also more complex and extended ones such as conferences, elections, building of a castle, or battles.
While the continuous growth of a tree lacks the limits characteristic of an event, its germination from a seed does qualify as an event. Similarly, the blowing of the wind lacks the distinctness and limits of an event, but a hurricane, flood or earthquake would qualify as an event. Mental processes are considered as events, in cases where they are connected with the material externalization of their results; for example, the creation of a poem, a performance or a change of intention that becomes obvious from subsequent actions or declarations.
The effects of an instance of E5 Event may not lead to relevant permanent changes of properties or relations of the items involved in it, for example an unrecorded performance. Of course, in order to be documented, some kind of evidence for an event must exist, be it witnesses, traces or products of the event.
While instances of E4 Period always require some form of coherence between its constituent phenomena, in addition, the essential constituents of instances of E5 Event should contribute to an overall effect; for example, the statements made during a meeting and the listening of the audience.
Viewed at a coarse level of detail, an instance of E5 Event may appear as if it had an ‘instantaneous’ overall effect, but any process or interaction of material nature in reality have an extent in time and space. At a fine level, instances of E5 Event may be analysed into component phenomena and phases within a space and timeframe, and as such can be seen as a period, regardless of the size of the phenomena. The reverse is not necessarily the case: not all instances of E4 Period give rise to a noteworthy overall effect and are thus not instances of E5 Event."""@en ;
    rdfs:subClassOf <http://www.cidoc-crm.org/cidoc-crm/E4_Period>,
        <http://www.cidoc-crm.org/extensions/crmsci/S15_Observable_Entity> .

<http://www.cidoc-crm.org/cidoc-crm/E63_Beginning_of_Existence> a rdfs:Class ;
    rdfs:label "Daseinsbeginn"@de,
        "Αρχή Ύπαρξης"@el,
        "Beginning of Existence"@en,
        "Début d’existence"@fr,
        "Início da Existência"@pt,
        "Начало Сущeствования"@ru,
        "初始"@zh ;
    dcterms:source "CIDOC_CRM_v7.1.3.rdf" ;
    rdfs:comment """This class comprises events that bring into existence any instance of E77 Persistent Item.
It may be used for temporal reasoning about things (intellectual products, physical items, groups of people, living beings) beginning to exist; it serves as a hook for both a terminus post quem and a terminus ante quem."""@en ;
    rdfs:subClassOf <http://www.cidoc-crm.org/cidoc-crm/E5_Event> .

<http://www.cidoc-crm.org/cidoc-crm/E64_End_of_Existence> a rdfs:Class ;
    rdfs:label "Daseinsende"@de,
        "Τέλος Ύπαρξης"@el,
        "End of Existence"@en,
        "Fin d’existence"@fr,
        "Fim da Existência"@pt,
        "Конeц Сущeствования"@ru,
        "结束"@zh ;
    dcterms:source "CIDOC_CRM_v7.1.3.rdf" ;
    rdfs:comment """This class comprises events that end the existence of any instance of E77 Persistent Item.
It may be used for temporal reasoning about things (physical items, groups of people, living beings) ceasing to exist; it serves as a hook both a terminus post quem and a terminus ante quem. In cases where substance from an instance of E77 Persistent Item continues to exist in a new form, the process would be documented as instances of E81 Transformation."""@en ;
    rdfs:subClassOf <http://www.cidoc-crm.org/cidoc-crm/E5_Event> .

<http://www.cidoc-crm.org/cidoc-crm/E65_Creation> a rdfs:Class ;
    rdfs:label "Begriffliche Schöpfung"@de,
        "Δημιουργία"@el,
        "Creation"@en,
        "Création"@fr,
        "Criação"@pt,
        "Созданиe"@ru,
        "创建"@zh ;
    dcterms:source "CIDOC_CRM_v7.1.3.rdf" ;
    rdfs:comment "This class comprises events that result in the creation of conceptual items or immaterial products, such as legends, poems, texts, music, images, movies, laws, types, etc."@en ;
    rdfs:subClassOf <http://www.cidoc-crm.org/cidoc-crm/E63_Beginning_of_Existence>,
        <http://www.cidoc-crm.org/cidoc-crm/E7_Activity> .

<http://www.cidoc-crm.org/cidoc-crm/E66_Formation> a rdfs:Class ;
    rdfs:label "Gruppenbildung"@de,
        "Συγκρότηση Ομάδας"@el,
        "Formation"@en,
        "Formation"@fr,
        "Formação"@pt,
        "Формированиe"@ru,
        "组成"@zh ;
    dcterms:source "CIDOC_CRM_v7.1.3.rdf" ;
    rdfs:comment """This class comprises events that result in the formation of a formal or informal E74 Group of people, such as a club, society, association, corporation, or nation.
E66 Formation does not include the arbitrary aggregation of people who do not act as a collective.
The formation of an instance of E74 Group does not require that the group is populated with members at the time of formation. In order to express the joining of members at the time of formation, the respective activity should be simultaneously an instance of both E66 Formation and E85 Joining."""@en ;
    rdfs:subClassOf <http://www.cidoc-crm.org/cidoc-crm/E63_Beginning_of_Existence>,
        <http://www.cidoc-crm.org/cidoc-crm/E7_Activity> .

<http://www.cidoc-crm.org/cidoc-crm/E67_Birth> a rdfs:Class ;
    rdfs:label "Geburt"@de,
        "Γέννηση"@el,
        "Birth"@en,
        "Naissance"@fr,
        "Nascimento"@pt,
        "Рождeниe"@ru,
        "出生"@zh ;
    dcterms:source "CIDOC_CRM_v7.1.3.rdf" ;
    rdfs:comment """This class comprises the births of human beings. E67 Birth is a biological event focussing on the context of people coming into life. (E63 Beginning of Existence comprises the coming into life of any living being.)
Twins, triplets, etc. are brought into life by the same instance of E67 Birth. The introduction of the E67 Birth event as a documentation element allows the description of a range of family relationships in a simple model. Suitable extensions may describe more details and the complexity of motherhood since the advent of modern medicine. In this model, the biological father is not seen as a necessary participant in the E67 Birth."""@en ;
    rdfs:subClassOf <http://www.cidoc-crm.org/cidoc-crm/E63_Beginning_of_Existence> .

<http://www.cidoc-crm.org/cidoc-crm/E68_Dissolution> a rdfs:Class ;
    rdfs:label "Gruppenauflösung"@de,
        "Διάλυση Ομάδας"@el,
        "Dissolution"@en,
        "Dissolution"@fr,
        "Dissolução"@pt,
        "Роспуск"@ru,
        "解散"@zh ;
    dcterms:source "CIDOC_CRM_v7.1.3.rdf" ;
    rdfs:comment """This class comprises the events that result in the formal or informal termination of an instance of E74 Group.
If the dissolution was deliberate, the Dissolution event should also be instantiated as an instance of E7 Activity."""@en ;
    rdfs:subClassOf <http://www.cidoc-crm.org/cidoc-crm/E64_End_of_Existence> .

<http://www.cidoc-crm.org/cidoc-crm/E69_Death> a rdfs:Class ;
    rdfs:label "Tod"@de,
        "Θάνατος"@el,
        "Death"@en,
        "Mort"@fr,
        "Morte"@pt,
        "Смeрть"@ru,
        "死亡"@zh ;
    dcterms:source "CIDOC_CRM_v7.1.3.rdf" ;
    rdfs:comment """This class comprises the deaths of human beings.
If a person is killed, their death should be instantiated as E69 Death and as E7 Activity. The death or perishing of other living beings should be documented as instances of E64 End of Existence."""@en ;
    rdfs:subClassOf <http://www.cidoc-crm.org/cidoc-crm/E64_End_of_Existence> .

<http://www.cidoc-crm.org/cidoc-crm/E6_Destruction> a rdfs:Class ;
    rdfs:label "Zerstörung"@de,
        "Καταστροφή"@el,
        "Destruction"@en,
        "Destruction"@fr,
        "Destruição"@pt,
        "Разрушeниe"@ru,
        "破坏"@zh ;
    dcterms:source "CIDOC_CRM_v7.1.3.rdf" ;
    rdfs:comment """This class comprises events that destroy one or more instances of E18 Physical Thing, such that they lose their identity as the subjects of documentation.
Some destruction events are intentional, while others are independent of human activity. Intentional destruction can be documented by classifying the event as both an instance of E6 Destruction and of E7 Activity.
The decision to document an object as destroyed, transformed, or modified is context-sensitive:
1. If the matter remaining from the destruction is not documented, the event is modelled solely as an instance of E6 Destruction.
2. An event should also be documented using E81 Transformation if it results in the destruction of one or more objects and the simultaneous production of others using parts or material from the original. In this case, the new items have separate identities. Matter is preserved, but identity is not.
3. When the initial identity of the changed instance of E18 Physical Thing is preserved, the event should be documented as an instance of E11 Modification."""@en ;
    rdfs:subClassOf <http://www.cidoc-crm.org/cidoc-crm/E64_End_of_Existence> .

<http://www.cidoc-crm.org/cidoc-crm/E70_Thing> a rdfs:Class ;
    rdfs:label "Sache"@de,
        "Πράγμα"@el,
        "Thing"@en,
        "Chose"@fr,
        "Coisa"@pt,
        "Вeщь"@ru,
        "事物"@zh ;
    dcterms:source "CIDOC_CRM_v7.1.3.rdf" ;
    rdfs:comment """This general class comprises discrete, identifiable, instances of E77 Persistent Item that are documented as single units, that either consist of matter or depend on being carried by matter and are characterized by relative stability.
They may be intellectual products or physical things. They may, for instance, have a solid physical form, an electronic encoding, or they may be a logical concept or structure."""@en ;
    rdfs:subClassOf <http://www.cidoc-crm.org/cidoc-crm/E77_Persistent_Item> .

<http://www.cidoc-crm.org/cidoc-crm/E71_Human-Made_Thing> a rdfs:Class ;
    rdfs:label "Human-Made Thing"@en,
        "Chose élaborée par l’humain"@fr,
        "Рукотворный Прeдмeт"@ru ;
    dcterms:source "CIDOC_CRM_v7.1.3.rdf" ;
    rdfs:comment """This class comprises discrete, identifiable human-made items that are documented as single units.
These items are either intellectual products or human-made physical things, and are characterized by relative stability. They may, for instance, have a solid physical form, an electronic encoding, or they may be logical concepts or structures."""@en ;
    rdfs:subClassOf <http://www.cidoc-crm.org/cidoc-crm/E70_Thing> .

<http://www.cidoc-crm.org/cidoc-crm/E72_Legal_Object> a rdfs:Class ;
    rdfs:label "Rechtsobjekt"@de,
        "Νομικό Αντικείμενο"@el,
        "Legal Object"@en,
        "Objet juridique"@fr,
        "Objeto Jurídico"@pt,
        "Объeкт Права"@ru,
        "法律对象"@zh ;
    dcterms:source "CIDOC_CRM_v7.1.3.rdf" ;
    rdfs:comment """This class comprises those material or immaterial items to which instances of E30 Right, such as the right of ownership or use, can be applied.
This is generally true for all instances of E18 Physical Thing. In the case of instances of E28 Conceptual Object, however, the identity of an instance of E28 Conceptual Object or the method of its use may be too ambiguous to reliably establish instances of E30 Right, as in the case of taxa and inspirations. Ownership of corporations is currently regarded as out of scope of the CIDOC CRM."""@en ;
    rdfs:subClassOf <http://www.cidoc-crm.org/cidoc-crm/E70_Thing> .

<http://www.cidoc-crm.org/cidoc-crm/E73_Information_Object> a rdfs:Class ;
    rdfs:label "Informationsgegenstand"@de,
        "Πληροφοριακό Αντικείμενο"@el,
        "Information Object"@en,
        "Objet informationnel"@fr,
        "Objeto de Informação"@pt,
        "Информационный Объeкт"@ru,
        "信息对象"@zh ;
    dcterms:source "CIDOC_CRM_v7.1.3.rdf" ;
    rdfs:comment """This class comprises identifiable immaterial items, such as poems, jokes, data sets, images, texts, multimedia objects, procedural prescriptions, computer program code, algorithm or mathematical formulae, that have an objectively recognizable structure and are documented as single units. The encoding structure known as a “named graph” also falls under this class, so that each “named graph” is an instance of E73 Information Object.
An instance of E73 Information Object does not depend on a specific physical carrier, which can include human memory, and it can exist on one or more carriers simultaneously.
Instances of E73 Information Object of a linguistic nature should be declared as instances of the E33 Linguistic Object subclass. Instances of E73 Information Object of a documentary nature should be declared as instances of the E31 Document subclass. Conceptual items such as types and classes are not instances of E73 Information Object, nor are ideas without a reproducible expression."""@en ;
    rdfs:subClassOf <http://www.cidoc-crm.org/cidoc-crm/E89_Propositional_Object>,
        <http://www.cidoc-crm.org/cidoc-crm/E90_Symbolic_Object> .

<http://www.cidoc-crm.org/cidoc-crm/E74_Group> a rdfs:Class ;
    rdfs:label "Menschliche Gruppe"@de,
        "Ομάδα"@el,
        "Group"@en,
        "Groupe"@fr,
        "Grupo"@pt,
        "Группа"@ru,
        "团体"@zh ;
    dcterms:source "CIDOC_CRM_v7.1.3.rdf" ;
    rdfs:comment """This class comprises any gatherings or organizations of human individuals or groups that act collectively or in a similar way due to any form of unifying relationship. In the wider sense this class also comprises official positions which used to be regarded in certain contexts as one actor, independent of the current holder of the office, such as the president of a country. In such cases, it may happen that the group never had more than one member. A joint pseudonym (i.e. a name that seems indicative of an individual but that is actually used as a persona by two or more people) is a particular case of E74 Group.
A gathering of people becomes an instance of E74 Group when it exhibits organizational characteristics usually typified by a set of ideas or beliefs held in common, or actions performed together. These might be communication, creating some common artifact, a common purpose such as study, worship, business, sports, etc. Nationality can be modelled as membership in an instance of E74 Group. Married couples and other concepts of family are regarded as particular examples of E74 Group."""@en ;
    rdfs:subClassOf <http://www.cidoc-crm.org/cidoc-crm/E39_Actor> .

<http://www.cidoc-crm.org/cidoc-crm/E77_Persistent_Item> a rdfs:Class ;
    rdfs:label "Seiendes"@de,
        "Ον"@el,
        "Persistent Item"@en,
        "Entité persistante"@fr,
        "Entidade Persistente"@pt,
        "Постоянная Сущность"@ru,
        "持久项"@zh ;
    dcterms:source "CIDOC_CRM_v7.1.3.rdf" ;
    rdfs:comment """This class comprises items that have persistent characteristics of structural nature substantially related to their identity and their integrity, sometimes known as “endurants” in philosophy. Persistent Items may be physical entities, such as people, animals or things, conceptual entities such as ideas, concepts, products of the imagination or even names.
Instances of E77 Persistent Item may be present or be part of interactions in different periods or events. They can repeatedly be recognized at disparate occasions during their existence by characteristics of structural nature. The respective characteristics need not be exactly the same during all the existence of an instance of E77 Persistent Item. Often, they undergo gradual change, still bearing some similarities with that of previous times, or disappear completely and new emerge. For instance, a person, from the time of being born on, will gradually change all its features and acquire new ones, such as a scar. Even the DNA in different body cells will develop defects and mutations. Nevertheless, relevant characteristics used should be sufficiently similar to recognize the instance for some substantial period of time.
The more specific criteria that determine the identity of instances of subclasses of E77 Persistent Item may vary considerably and are described or referred to in the respective scope notes. The decision about which exact criteria to use depends on whether the observable behaviour of the respective part of reality such confined conforms to the reasoning the user is interested in. For example, a building can be regarded as no longer existing if it is dismantled and the materials reused in a different configuration. On the other hand, human beings go through radical and profound changes during their life-span, affecting both material composition and form, yet preserve their identity by other criteria, such as being bodily separated from other persons. Similarly, inanimate objects may be subject to exchange of parts and matter. On the opposite, the identity of a (version of a) text of a scientific publication is given by the exact arrangement of its relevant symbols.
The main classes of objects that fall outside the scope of the E77 Persistent Item class are temporal objects such as periods, events and acts, and descriptive properties.
An instance of E77 Persistent Item does not require actual knowledge of the identifying features of the instance being currently known. There may be cases, where the actual identifying features of an instance of E77 Persistent Item are not decidable at a particular state of knowledge."""@en ;
    rdfs:subClassOf <http://www.cidoc-crm.org/cidoc-crm/E1_CRM_Entity> .

<http://www.cidoc-crm.org/cidoc-crm/E78_Curated_Holding> a rdfs:Class ;
    rdfs:label "Curated Holding"@en,
        "Collection"@fr,
        "Отвeтствeнноe Хранeниe"@ru ;
    dcterms:source "CIDOC_CRM_v7.1.3.rdf" ;
    rdfs:comment """This class comprises aggregations of instances of E18 Physical Thing that are assembled and maintained (“curated” and “preserved,” in museological terminology) by one or more instances of E39 Actor over time for a specific purpose and audience, and according to a particular collection development plan. Typical instances of curated holdings are museum collections, archives, library holdings and digital libraries. A digital library is regarded as an instance of E18 Physical Thing because it requires keeping physical carriers of the electronic content.
Items may be added or removed from an E78 Curated Holding in pursuit of this plan. This class should not be confused with the E39 Actor maintaining the E78 Curated Holding who is often referred to using the name of the E78 Curated Holding (e.g. “The Wallace Collection decided…”).
Collective objects in the general sense, like a tomb full of gifts, a folder with stamps, or a set of chessmen, should be documented as instances of E19 Physical Object, and not as instances of E78 Curated Holding. This is because they form wholes, either because they are physically bound together or because they are kept together for their functionality."""@en ;
    rdfs:subClassOf <http://www.cidoc-crm.org/cidoc-crm/E24_Physical_Human-Made_Thing> .

<http://www.cidoc-crm.org/cidoc-crm/E79_Part_Addition> a rdfs:Class ;
    rdfs:label "Teilhinzufügung"@de,
        "Προσθήκη Μερών"@el,
        "Part Addition"@en,
        "Ajout d'élément"@fr,
        "Adição de Parte"@pt,
        "Добавлeниe Части"@ru,
        "部分增加"@zh ;
    dcterms:source "CIDOC_CRM_v7.1.3.rdf" ;
    rdfs:comment """This class comprises activities that result in an instance of E18 Physical Thing being increased, enlarged, or augmented by the addition of a part.
Typical scenarios include the attachment of an accessory, the integration of a component, the addition of an element to an aggregate object, or the accessioning of an object into a curated instance of E78 Curated Holding. Both the E18 Physical Thing being augmented and the E18 Physical Thing that is being added are treated as separate identifiable wholes prior to the instance of E79 Part Addition. Following the addition of parts, the resulting assemblages are treated objectively as single identifiable wholes, made up of constituent or component parts bound together either physically (for example the engine becoming a part of the car), or by sharing a common purpose (such as the 32 chess pieces that make up a chess set). This class of activities forms a basis for reasoning about the history and continuity of identity of objects that are integrated into other objects over time, such as precious gemstones being repeatedly incorporated into different items of jewellery, or cultural artefacts being added to different museum instances of E78 Curated Holding over their lifespan."""@en ;
    rdfs:subClassOf <http://www.cidoc-crm.org/cidoc-crm/E11_Modification> .

<http://www.cidoc-crm.org/cidoc-crm/E7_Activity> a rdfs:Class ;
    rdfs:label "Handlung"@de,
        "Δράση"@el,
        "Activity"@en,
        "Activité"@fr,
        "Atividade"@pt,
        "Дeятeльность"@ru,
        "活动"@zh ;
    dcterms:source "CIDOC_CRM_v7.1.3.rdf" ;
    rdfs:comment """This class comprises actions intentionally carried out by instances of E39 Actor that result in changes of state in the cultural, social, or physical systems documented.
This notion includes complex, composite, and long-lasting actions such as the building of a settlement or a war, as well as simple, short-lived actions such as the opening of a door."""@en ;
    rdfs:subClassOf <http://www.cidoc-crm.org/cidoc-crm/E5_Event> .

<http://www.cidoc-crm.org/cidoc-crm/E80_Part_Removal> a rdfs:Class ;
    rdfs:label "Teilentfernung"@de,
        "Αφαίρεση Μερών"@el,
        "Part Removal"@en,
        "Retrait d'élément"@fr,
        "Remoção de Parte"@pt,
        "Удалeниe Части"@ru,
        "部分去除"@zh ;
    dcterms:source "CIDOC_CRM_v7.1.3.rdf" ;
    rdfs:comment """This class comprises the activities that result in an instance of E18 Physical Thing being decreased by the removal of a part.
Typical scenarios include the detachment of an accessory, the removal of a component or part of a composite object, or the deaccessioning of an object from a curated collection, an instance of E78 Curated Holding. If the instance of E80 Part Removal results in the total decomposition of the original object into pieces, such that the whole ceases to exist, the activity should instead be modelled as an instance of E81 Transformation, i.e. a simultaneous destruction and production. In cases where the part removed has no discernible identity prior to its removal but does have an identity subsequent to its removal, the activity should be modelled as both an instance of E80 Part Removal and E12 Production. This class of activities forms a basis for reasoning about the history, and continuity of identity over time, of objects that are removed from other objects, such as precious gemstones being extracted from different items of jewellery, or cultural artifacts being deaccessioned from different museum collections over their lifespan."""@en ;
    rdfs:subClassOf <http://www.cidoc-crm.org/cidoc-crm/E11_Modification>,
        <http://www.cidoc-crm.org/extensions/crmsci/S1_Matter_Removal> .

<http://www.cidoc-crm.org/cidoc-crm/E81_Transformation> a rdfs:Class ;
    rdfs:label "Umwandlung"@de,
        "Μετατροπή"@el,
        "Transformation"@en,
        "Transformation"@fr,
        "Transformação"@pt,
        "Трансформация"@ru,
        "转变"@zh ;
    dcterms:source "CIDOC_CRM_v7.1.3.rdf" ;
    rdfs:comment """This class comprises the events that result in the simultaneous destruction of one or more than one E18 Physical Thing and the creation of one or more than one E18 Physical Thing that preserves recognizable substance and structure from the first one(s) but has fundamentally different nature or identity.
Although the old and the new instances of E18 Physical Thing are treated as discrete entities having separate, unique identities, they are causally connected through the E81 Transformation; the destruction of the old E18 Physical Thing(s) directly causes the creation of the new one(s) using or preserving some relevant substance and structure. Instances of E81 Transformation are therefore distinct from re-classifications (documented using E17 Type Assignment) or modifications (documented using E11 Modification) of objects that do not fundamentally change their nature or identity. Characteristic cases are reconstructions and repurposing of historical buildings or ruins, fires leaving buildings in ruins, taxidermy of specimen in natural history.
Even though such instances of E81 Transformation are often motivated by a change of intended use, substantial material changes should justify the documentation of the result as a new instance of E18 Physical Thing and not just the change of function. The latter may be documented as an extended activity (instance of E7 Activity) of using it."""@en ;
    rdfs:subClassOf <http://www.cidoc-crm.org/cidoc-crm/E63_Beginning_of_Existence>,
        <http://www.cidoc-crm.org/cidoc-crm/E64_End_of_Existence> .

<http://www.cidoc-crm.org/cidoc-crm/E83_Type_Creation> a rdfs:Class ;
    rdfs:label "Typuserfindung"@de,
        "Δημιουργία Τύπου"@el,
        "Type Creation"@en,
        "Création de type"@fr,
        "Criação de Tipo"@pt,
        "Созданиe Типа"@ru,
        "类型创建"@zh ;
    dcterms:source "CIDOC_CRM_v7.1.3.rdf" ;
    rdfs:comment """This class comprises activities formally defining new types of items.
It is typically a rigorous scholarly or scientific process that ensures a type is exhaustively described and appropriately named. In some cases, particularly in archaeology and the life sciences, E83 Type Creation requires the identification of an exemplary specimen and the publication of the type definition in an appropriate scholarly forum. The activity modelled as an instance of E83 Type Creation is central to research in the life sciences, where a type would be referred to as a “taxon,” the type description as a “protologue,” and the exemplary specimens as “original element” or “holotype”."""@en ;
    rdfs:subClassOf <http://www.cidoc-crm.org/cidoc-crm/E65_Creation> .

<http://www.cidoc-crm.org/cidoc-crm/E85_Joining> a rdfs:Class ;
    rdfs:label "Beitritt"@de,
        "Joining"@en,
        "Adhésion"@fr,
        "Вступлeниe"@ru,
        "加入"@zh ;
    dcterms:source "CIDOC_CRM_v7.1.3.rdf" ;
    rdfs:comment """This class comprises the activities that result in an instance of E39 Actor becoming a member of an instance of E74 Group. This class does not imply initiative by either party. It may be the initiative of a third party.
Typical scenarios include becoming a member of a social organisation, becoming an employee of a company, marriage, the adoption of a child by a family, and the inauguration of somebody into an official position."""@en ;
    rdfs:subClassOf <http://www.cidoc-crm.org/cidoc-crm/E7_Activity> .

<http://www.cidoc-crm.org/cidoc-crm/E86_Leaving> a rdfs:Class ;
    rdfs:label "Austritt"@de,
        "Leaving"@en,
        "Départ"@fr,
        "Выход"@ru,
        "离开"@zh ;
    dcterms:source "CIDOC_CRM_v7.1.3.rdf" ;
    rdfs:comment """This class comprises the activities that result in an instance of E39 Actor to be disassociated from an instance of E74 Group. This class does not imply initiative by either party. It may be the initiative of a third party.
Typical scenarios include the termination of membership in a social organisation, ending the employment at a company, divorce, and the end of tenure of somebody in an official position."""@en ;
    rdfs:subClassOf <http://www.cidoc-crm.org/cidoc-crm/E7_Activity> .

<http://www.cidoc-crm.org/cidoc-crm/E87_Curation_Activity> a rdfs:Class ;
    rdfs:label "Kuratorische Tätigkeit"@de,
        "Curation Activity"@en,
        "Activité curatoriale"@fr,
        "Кураторство"@ru,
        "管理"@zh ;
    dcterms:source "CIDOC_CRM_v7.1.3.rdf" ;
    rdfs:comment """This class comprises the activities that contribute to the management and the preservation and evolution of instances of E78 Curated Holding, following an implicit or explicit curation plan.
It specializes the notion of activity into the curation of a collection and allows the history of curation to be recorded.
Items are accumulated and organized following criteria such as subject, chronological period, material type, style of art, etc., and can be added or removed from an instance of E78 Curated Holding for a specific purpose and/or audience. The initial aggregation of items to form a collection is regarded as an instance of E12 Production Event, while the activities of evolving, preserving, and promoting a collection are regarded as instances of E87 Curation Activity."""@en ;
    rdfs:subClassOf <http://www.cidoc-crm.org/cidoc-crm/E7_Activity> .

<http://www.cidoc-crm.org/cidoc-crm/E89_Propositional_Object> a rdfs:Class ;
    rdfs:label "Aussagenobjekt"@de,
        "Propositional Object"@en,
        "Objet propositionnel"@fr,
        "Пропозициональный Объeкт"@ru,
        "命题对象"@zh ;
    dcterms:source "CIDOC_CRM_v7.1.3.rdf" ;
    rdfs:comment """This class comprises immaterial items, including but not limited to stories, plots, procedural prescriptions, algorithms, laws of physics or images that are, or represent in some sense, sets of propositions about real or imaginary things and that are documented as single units or serve as topic of discourse.
This class also comprises items that are “about” something in the sense of a subject. In the wider sense, this class includes expressions of psychological value such as non-figural art and musical themes. However, conceptual items such as types and classes are not instances of E89 Propositional Object. This should not be confused with the definition of a type, which is indeed an instance of E89 Propositional Object."""@en ;
    rdfs:subClassOf <http://www.cidoc-crm.org/cidoc-crm/E28_Conceptual_Object> .

<http://www.cidoc-crm.org/cidoc-crm/E8_Acquisition> a rdfs:Class ;
    rdfs:label "Erwerb"@de,
        "Απόκτηση"@el,
        "Acquisition"@en,
        "Acquisition"@fr,
        "Aquisição"@pt,
        "Поступлeниe"@ru,
        "采访"@zh ;
    dcterms:source "CIDOC_CRM_v7.1.3.rdf" ;
    rdfs:comment """This class comprises transfers of legal ownership from one or more instances of E39 Actor to one or more other instances of E39 Actor.
The class also applies to the establishment or loss of ownership of instances of E18 Physical Thing. It does not, however, imply changes of any other kinds of rights. The recording of the donor and/or recipient is optional. It is possible that in an instance of E8 Acquisition there is either no donor or no recipient. Depending on the circumstances, it may describe:
1. the beginning of ownership
2. the end of ownership
3. the transfer of ownership
4. the acquisition from an unknown source
5. the loss of title due to destruction of the item
It may also describe events where a collector appropriates legal title, for example, by annexation or field collection. The interpretation of the museum notion of “accession” differs between institutions. The CIDOC CRM therefore models legal ownership (E8 Acquisition) and physical custody (E10 Transfer of Custody) separately. Institutions will then model their specific notions of accession and deaccession as combinations of these."""@en ;
    rdfs:subClassOf <http://www.cidoc-crm.org/cidoc-crm/E7_Activity> .

<http://www.cidoc-crm.org/cidoc-crm/E90_Symbolic_Object> a rdfs:Class ;
    rdfs:label "Symbolisches Objekt"@de,
        "Symbolic Object"@en,
        "Objet symbolique"@fr,
        "Символичeский Объeкт"@ru,
        "符号对象"@zh ;
    dcterms:source "CIDOC_CRM_v7.1.3.rdf" ;
    rdfs:comment """This class comprises identifiable symbols and any aggregation of symbols, such as characters, identifiers, traffic signs, emblems, texts, data sets, images, musical scores, multimedia objects, computer program code, or mathematical formulae that have an objectively recognizable structure and that are documented as single units.
It includes sets of signs of any nature, which may serve to designate something, or to communicate some propositional content. An instance of E90 Symbolic Object may or may not have a specific meaning, for example an arbitrary character string.
In some cases, the content of an instance of E90 Symbolic Object may completely be represented by a serialized digital content model, such as a sequence of ASCII-encoded characters, an XML or HTML document, or a TIFF image. The property P3 has note and its subproperty P190 has symbolic content allow for the description of this content model. In order to disambiguate which symbolic level is the carrier of the meaning, the property P3.1 has type can be used to specify the encoding (e.g. “bit”, “Latin character”, RGB pixel)."""@en ;
    rdfs:subClassOf <http://www.cidoc-crm.org/cidoc-crm/E28_Conceptual_Object>,
        <http://www.cidoc-crm.org/cidoc-crm/E72_Legal_Object> .

<http://www.cidoc-crm.org/cidoc-crm/E92_Spacetime_Volume> a rdfs:Class ;
    rdfs:label "Spacetime Volume"@en,
        "Volume spatio-temporel"@fr,
        "Область Пространства-Врeмeни"@ru ;
    dcterms:source "CIDOC_CRM_v7.1.3.rdf",
        "CRMgeo_v1.2.rdf" ;
    rdfs:comment """Scope note:This class comprises 4 dimensional possibly fuzzy point sets (volumes) in physical spacetime regardless its true geometric form (S). They may derive their identity from being the extent of a material phenomenon or from being the interpretation of an expression (I) defining an extent in Space Time. The duration of existence of an instance of a spacetime volume is trivially its projection on time (E).
Examples:
•	the spacetime Volume of the Event of Ceasars murdering
•	the spacetime Volume where and when the carbon 14 dating of the "Schoeninger Speer II" in 1996 took place
•	the spatio-temporal trajectory of the H.M.S. Victory from its building to its actual location
•	the spacetime volume defined by a polygon approximating the Danube river flood in Austria between 6th and 9th of August 2002
	"""^^xsd:string,
        "This class comprises 4-dimensional point sets (volumes) in physical spacetime (in contrast to mathematical models of it) regardless of their true geometric forms. They may derive their identity from being the extent of a material phenomenon or from being the interpretation of an expression defining an extent in spacetime. Intersections of instances of E92 Spacetime Volume, E53 Place, and E52 Time-Span are also regarded as instances of E92 Spacetime Volume. An instance of E92 Spacetime Volume is either contiguous or composed of a finite number of contiguous subsets. Its boundaries may be fuzzy due to the properties of the phenomena it derives from or due to the limited precision up to which defining expression can be identified with a real extent in spacetime. The duration of existence of an instance of E92 Spacetime Volume is its projection on time."@en ;
    rdfs:subClassOf <http://www.cidoc-crm.org/cidoc-crm/E1_CRM_Entity> .

<http://www.cidoc-crm.org/cidoc-crm/E93_Presence> a rdfs:Class ;
    rdfs:label "Presence"@en,
        "Présence"@fr,
        "Присутствиe"@ru ;
    dcterms:source "CIDOC_CRM_v7.1.3.rdf" ;
    rdfs:comment """This class comprises instances of E92 Spacetime Volume, whose temporal extent has been chosen in order to determine the spatial extent of a phenomenon over the chosen time-span. Respective phenomena may, for instance, be historical events or periods, but can also be the diachronic extent and existence of physical things. In other words, instances of this class fix a slice of another instance of E92 Spacetime Volume in time.
The temporal extent of an instance of E93 Presence typically is predetermined by the researcher so as to focus the investigation particularly on finding the spatial extent of the phenomenon by testing for its characteristic features. There are at least two basic directions such investigations might take. The investigation may wish to determine where something was during some time or it may wish to reconstruct the total passage of a phenomenon’s spacetime volume through an examination of discrete presences. Observation and measurement of features indicating the presence or absence of a phenomenon in some space allows for the progressive approximation of spatial extents through argumentation typically based on inclusion, exclusion and various overlaps."""@en ;
    rdfs:subClassOf <http://www.cidoc-crm.org/cidoc-crm/E92_Spacetime_Volume> .

<http://www.cidoc-crm.org/cidoc-crm/E96_Purchase> a rdfs:Class ;
    rdfs:label "Purchase"@en,
        "Achat"@fr,
        "Покупка"@ru ;
    dcterms:source "CIDOC_CRM_v7.1.3.rdf" ;
    rdfs:comment """This class comprises transfers of legal ownership from one or more instances of E39 Actor to one or more different instances of E39 Actor, where the transferring party is completely compensated by the payment of a monetary amount. In more detail, a purchase agreement establishes a fixed monetary obligation at its initialization on the receiving party, to the giving party. An instance of E96 Purchase begins with the contract or equivalent agreement and ends with the fulfilment of all contractual obligations. In the case that the activity is abandoned before both parties have fulfilled these obligations, the activity is not regarded as an instance of E96 Purchase.
This class is a very specific case of the much more complex social business practices of exchange of goods and the creation and satisfaction of related social obligations. Purchase activities which define individual sales prices per object can be modelled by instantiating E96 Purchase for each object individually and as part of an overall instance of E96 Purchase transaction."""@en ;
    rdfs:subClassOf <http://www.cidoc-crm.org/cidoc-crm/E8_Acquisition> .

<http://www.cidoc-crm.org/cidoc-crm/E97_Monetary_Amount> a rdfs:Class ;
    rdfs:label "Monetary Amount"@en,
        "Valeur monétaire"@fr,
        "Дeнeжный Эквивалeнт"@ru ;
    dcterms:source "CIDOC_CRM_v7.1.3.rdf" ;
    rdfs:comment "This class comprises quantities of monetary possessions or obligations in terms of their nominal value with respect to a particular currency. These quantities may be abstract accounting units, the nominal value of a heap of coins or bank notes at the time of validity of the respective currency, the nominal value of a bill of exchange or other documents expressing monetary claims or obligations. It specifically excludes amounts expressed in terms of weights of valuable items, like gold and diamonds, and quantities of other non-currency items, like goats or stocks and bonds."@en ;
    rdfs:subClassOf <http://www.cidoc-crm.org/cidoc-crm/E54_Dimension> .

<http://www.cidoc-crm.org/cidoc-crm/E98_Currency> a rdfs:Class ;
    rdfs:label "Currency"@en,
        "Unité monétaire"@fr,
        "Валюта"@ru ;
    dcterms:source "CIDOC_CRM_v7.1.3.rdf" ;
    rdfs:comment "This class comprises the units in which a monetary system, supported by an administrative authority or other community, quantifies and arithmetically compares all monetary amounts declared in the unit. The unit of a monetary system must describe a nominal value which is kept constant by its administrative authority and an associated banking system if it exists, and not by market value. For instance, one may pay with grams of gold, but the respective monetary amount would have been agreed as the gold price in US dollars on the day of the payment. Under this definition, British Pounds, U.S. Dollars, and European Euros are examples of currency, but “grams of gold” is not. One monetary system has one and only one currency. Instances of this class must not be confused with coin denominations, such as “Dime” or “Sestertius”. Non-monetary exchange of value in terms of quantities of a particular type of goods, such as cows, do not constitute a currency."@en ;
    rdfs:subClassOf <http://www.cidoc-crm.org/cidoc-crm/E58_Measurement_Unit> .

<http://www.cidoc-crm.org/cidoc-crm/E99_Product_Type> a rdfs:Class ;
    rdfs:label "Product Type"@en,
        "Modèle de produit"@fr,
        "Тип Продукта"@ru ;
    dcterms:source "CIDOC_CRM_v7.1.3.rdf" ;
    rdfs:comment "This class comprises types that stand as the models for instances of E22 Human-Made Object that are produced as the result of production activities using plans exact enough to result in one or more series of uniform, functionally and aesthetically identical and interchangeable items. The product type is the intended ideal form of the manufacture process. It is typical of instances of E22 Human-Made Object that conform to an instance of E99 Product Type that its component parts are interchangeable with component parts of other instances of E22 Human-Made Object made after the model of the same instance of E99 Product Type. Frequently, the uniform production according to a given instance of E99 Product Type is achieved by creating individual tools, such as moulds or print plates that are themselves carriers of the design of the product type. Modern tools may use the flexibility of electronically controlled devices to achieve such uniformity. The product type itself, i.e. the potentially unlimited series of aesthetically equivalent items, may be the target of artistic design, rather than the individual object. In extreme cases, only one instance of a product type may have been produced, such as in a “print on demand” process which was only triggered once. However, this should not be confused with industrial prototypes, such as car prototypes, which are produced prior to the production line being set up, or test the production line itself."@en ;
    rdfs:subClassOf <http://www.cidoc-crm.org/cidoc-crm/E55_Type> .

<http://www.cidoc-crm.org/cidoc-crm/E9_Move> a rdfs:Class ;
    rdfs:label "Objektbewegung"@de,
        "Μετακίνηση"@el,
        "Move"@en,
        "Déplacement"@fr,
        "Locomoção"@pt,
        "Пeрeмeщeниe"@ru,
        "移动"@zh ;
    dcterms:source "CIDOC_CRM_v7.1.3.rdf" ;
    rdfs:comment """This class comprises changes of the physical location of the instances of E19 Physical Object.
Note, that the class E9 Move inherits the property P7 took place at (witnessed): E53 Place. This property should be used to describe the trajectory or a larger area within which a move takes place, whereas the properties P26 moved to (was destination of), P27 moved from (was origin of) describe the start and end points only. Moves may also be documented to consist of other moves (via P9 consists of (forms part of)), in order to describe intermediate stages on a trajectory. In that case, start and end points of the partial moves should match appropriately between each other and with the overall event."""@en ;
    rdfs:subClassOf <http://www.cidoc-crm.org/cidoc-crm/E7_Activity> .

<http://www.cidoc-crm.org/extensions/crmarchaeo/A10_Excavation_Interface> a rdfs:Class ;
    rdfs:label "Excavation Interface"@en ;
    dcterms:source "CRMarchaeo_v2.1.1.rdf" ;
    rdfs:comment "This class comprises instances of S20 Rigid Physical Feature that constitutes a surface produced through one or several instances of A1 Excavation Processing Unit. Instances are often documented through drawing and/or measured by technical means such as photography, tachymetry or laser scanning. Using a planar excavation methodology this is typically the surface of a planum or the surface of a profile. Using a stratigraphic excavation methodology, the instance of A10 Excavation Interface would have the intention to approximate an instance of A3 Stratigraphic Interface. The drawing and measurement of profiles is also common practice when a stratigraphic excavation methodology is used."@en ;
    rdfs:subClassOf <http://www.cidoc-crm.org/cidoc-crm/E25_Human-Made_Feature>,
        <http://www.cidoc-crm.org/extensions/crmsci/S20_Rigid_Physical_Feature> .

<http://www.cidoc-crm.org/extensions/crmarchaeo/A1_Excavation_Processing_Unit> a rdfs:Class ;
    rdfs:label "Excavation Processing Unit"@en ;
    dcterms:source "CRMarchaeo_v2.1.1.rdf" ;
    rdfs:comment "This class comprises activities of excavating in the sense of archaeology, which are documented as a coherent set of actions of progressively recording and removing matter from a pre-specified location under specific rules. Typically, an instance of A1 Excavation Processing Unit would be terminated if significant discontinuities of substance or finds come to light, or if the activity is interrupted due to external factors, such as end of a working day. In other cases, the termination would be based on predefined physical specifications, such as the boundaries of a maximal volume of matter to be excavated in one unit of excavation. Depending on the methodology, an instance of A1 Excavation Processing Unit may intend to remove matter only within the boundaries of a particular stratigraphic unit, or it may follow a pre-declared spatial extent such as a trench. It may only uncover, clean or expose a structure or parts of it. The process of excavation results in the production of a set of recorded (documentation) data that should be sufficient to provide researchers enough information regarding the consistency and spatial distribution of the excavated Segment of Matter and things and features embedded in it. Some parts or all of the removed physical material (instances of S11 Amount of Matter) may be dispersed, whereas others may be kept in custody in the form of finds or samples, while others (such as parts of walls) may be left at the place of their discovery. The data produced by an instance of A1 Excavation Processing Unit should pertain to the material state of matter at excavation time only and should be clearly distinguished from subsequent interpretation about the causes for this state of matter. The current class A1 Excavation Processing Unit is somewhat overloaded and may be split into two subclasses, one for the intellectual process and one for the physical process. This is left for a future refinement of the model."@en ;
    rdfs:subClassOf <http://www.cidoc-crm.org/cidoc-crm/E12_Production>,
        <http://www.cidoc-crm.org/cidoc-crm/E64_End_of_Existence>,
        <http://www.cidoc-crm.org/extensions/crmsci/S1_Matter_Removal>,
        <http://www.cidoc-crm.org/extensions/crmsci/S4_Observation> .

<http://www.cidoc-crm.org/extensions/crmarchaeo/A2_Stratigraphic_Volume_Unit> a rdfs:Class ;
    rdfs:label "Stratigraphic Volume Unit"@en ;
    dcterms:source "CRMarchaeo_v2.1.1.rdf" ;
    rdfs:comment "This class comprises instances of A8 Stratigraphic Unit which are connected portions of terrain or other solid structures on, in, or under the surface of earth or seafloor exhibiting some homogeneity of structure or substance and which are completely bounded by surfaces or discontinuities in substance or structure with respect to other portions of the terrain or surfaces of objects or finds. Normally at least one of the surfaces, i.e. instances of A3 Stratigraphic Interface (such as the lower one), from the genesis event of the A2 Stratigraphic Volume Unit will remain during its existence. An instance of A2 Stratigraphic Volume Unit may contain physical objects."@en ;
    rdfs:subClassOf <http://www.cidoc-crm.org/extensions/crmarchaeo/A8_Stratigraphic_Unit> .

<http://www.cidoc-crm.org/extensions/crmarchaeo/A3_Stratigraphic_Interface> a rdfs:Class ;
    rdfs:label "Stratigraphic Interface"@en ;
    dcterms:source "CRMarchaeo_v2.1.1.rdf" ;
    rdfs:comment "This class comprises instances of A8 Stratigraphic Unit, which are coherent parts of a boundary surface that appear as the result of a stratigraphic genesis event or process. The interface marks the limit of the geometric extent of the effect of a genesis or modification event, and indicates in particular where the effect of this event ended. Each event of creation or destruction of a deposition layer implies the creation of new interfaces. Thus, there are two main types of interfaces: those that are surfaces of strata (that can be directly related to the corresponding stratum via the AP12 confines property), and those that are only surfaces, formed by the removal or destruction of existing stratifications."@en ;
    rdfs:subClassOf <http://www.cidoc-crm.org/extensions/crmarchaeo/A8_Stratigraphic_Unit> .

<http://www.cidoc-crm.org/extensions/crmarchaeo/A4_Stratigraphic_Genesis> a rdfs:Class ;
    rdfs:label "Stratigraphic Genesis"@en ;
    dcterms:source "CRMarchaeo_v2.1.1.rdf" ;
    rdfs:comment "This class comprises activities or processes that have produced homogeneous, distinguishable units of stratification that are in a relatively stable form from the time of their genesis until they are observed. Such processes may be the aggregation of cycles of erosion/destruction, deposit/accumulation, or transformation/modification occurring on a particular site throughout a particular period of time. These processes are usually not only due to natural forces (i.e., climate, the impact of flora and fauna, other natural events), but also to human activities, in particular excavation and construction. An event of stratification genesis typically produces two main forms of stratification units, both a deposit and an interface."@en ;
    rdfs:subClassOf <http://www.cidoc-crm.org/extensions/crmarchaeo/A5_Stratigraphic_Modification>,
        <http://www.cidoc-crm.org/extensions/crmsci/S17_Physical_Genesis> .

<http://www.cidoc-crm.org/extensions/crmarchaeo/A5_Stratigraphic_Modification> a rdfs:Class ;
    rdfs:label "Stratigraphic Modification"@en ;
    dcterms:source "CRMarchaeo_v2.1.1.rdf" ;
    rdfs:comment "This class comprises activities or processes resulting in the modification of Stratigraphic Units after their genesis through instances of A4 Stratigraphic Genesis Event."@en ;
    rdfs:subClassOf <http://www.cidoc-crm.org/extensions/crmsci/S18_Alteration> .

<http://www.cidoc-crm.org/extensions/crmarchaeo/A6_Group_Declaration_Event> a rdfs:Class ;
    rdfs:label "Group Declaration Event"@en ;
    dcterms:source "CRMarchaeo_v2.1.1.rdf" ;
    rdfs:comment "This class comprises interpretive activities that lead to the recognition two or more instances of Stratigraphic Units (A8) or other Physical Thing (E18) that simultaneously exist at the time of this activity or at the time of an archaeological observation this activity refers to as source and that are attributed to be the remains of one complete instance of Physical Thing (E18) that had existed at a time of reference in the past. Instances of this class could be, for example: two stratigraphic units (with no evident contact) cut through by a ditch having been segments of the same original stratigraphic unit, two or more surviving parts of a structure having been segments of the same wall (B5), a number of postholes being the indication of a past wooden house or a number of potsherds being segments of the same original artefact."@en ;
    rdfs:subClassOf <http://www.cidoc-crm.org/cidoc-crm/E13_Attribute_Assignment> .

<http://www.cidoc-crm.org/extensions/crmarchaeo/A7_Embedding> a rdfs:Class ;
    rdfs:label "Embedding"@en ;
    dcterms:source "CRMarchaeo_v2.1.1.rdf" ;
    rdfs:comment "This class comprises instances of A8 Stratigraphic Unit partially or completely embedding one or more instances of E20 Physical Thing and at a particular position with relative stability in one or more instances of A2 Stratigraphic Volume Units. Normally, an embedding is expected to have been stable from the time of generation of the first instance of A2 Stratigraphic Volume Unit that surrounds it. However, it may also be due to later intrusion. As an empirical fact, the expert may only be able to decide that a particular embedding is not recent, i.e. has been persisting for longer than the activity that encountered it. This class can be used to document the fact of embedding generally with respect to the surrounding matter or, more specifically, with respect to a more precise position within this matter."@en ;
    rdfs:subClassOf <http://www.cidoc-crm.org/extensions/crmarchaeo/A8_Stratigraphic_Unit> .

<http://www.cidoc-crm.org/extensions/crmarchaeo/A8_Stratigraphic_Unit> a rdfs:Class ;
    rdfs:label "Stratigraphic Unit"@en ;
    dcterms:source "CRMarchaeo_v2.1.1.rdf" ;
    rdfs:comment "This class comprises instances of S20 Rigid Physical Features which appear as the result of a stratigraphic genesis event or process. The form of an instance of A8 Stratigraphic Unit should be of a kind that can be attributed to a single genesis event or process and has the potential to be observed. One genesis event may have created more than one SU. An instance of A8 Stratigraphic Unit is regarded to exist as long as a part of its matter is still in place with respect to a surrounding reference space, such that its spatial features can be associated with effects of the genesis process of interest. This also implies that a certain degree of coherent (“conformal”) deformation is tolerable within its time-span of existence. Therefore, the place an instance of A8 Stratigraphic Unit occupies can be uniquely identified with respect to the surrounding reference space of archaeological interest"@en ;
    rdfs:subClassOf <http://www.cidoc-crm.org/extensions/crmsci/S20_Rigid_Physical_Feature> .

<http://www.cidoc-crm.org/extensions/crmarchaeo/A9_Archaeological_Excavation> a rdfs:Class ;
    rdfs:label "Archaeological Excavation"@en ;
    dcterms:source "CRMarchaeo_v2.1.1.rdf" ;
    rdfs:comment "This class describes the general concept of archaeological excavation intended as a coordinated set of activities performed on an area considered as part of a broader topographical, rural, urban, or monumental context. An archaeological excavation is usually under the responsibility of a coordinator, officially designated, which is legally and scientifically responsible for all the activities carried out within each instance of A1 Excavation Processing Unit and is also responsible for the documentation of the whole process."@en ;
    rdfs:subClassOf <http://www.cidoc-crm.org/extensions/crmsci/S4_Observation> .

<http://www.cidoc-crm.org/extensions/crmsci/S10_Material_Substantial> a rdfs:Class ;
    rdfs:label "Material Substantial"@en ;
    dcterms:source "CRMsci_v2.0.rdf" ;
    rdfs:comment "This class comprises constellations of matter with a relative stability of any form sufficient to associate them with a persistent identity, such as being confined to certain extent, having a relative stability of form or structure, or containing a fixed amount of matter. In particular, it comprises physical things in the narrower sense and fluid bodies. It is an abstraction of physical substance for solid and non-solid things of matter."@en ;
    rdfs:subClassOf <http://www.cidoc-crm.org/cidoc-crm/E70_Thing>,
        <http://www.cidoc-crm.org/extensions/crmsci/S15_Observable_Entity> .

<http://www.cidoc-crm.org/extensions/crmsci/S11_Amount_of_Matter> a rdfs:Class ;
    rdfs:label "Amount of Matter"@en ;
    dcterms:source "CRMsci_v2.0.rdf" ;
    rdfs:comment "This class comprises fixed amounts of matter specified as some air, some water, some soil, etc., defined by the total and integrity of their material content. In order to be able to identify and recognize in practice one instance of S11 Amount of Matter, some sort of confinement is needed that serves as a constraint for the enclosed matter and the integrity of the content, such as a bottle. In contrast to instances of E18 Physical Thing, no stability of form is required. The content may be put into another bottle without losing its identity. Subclasses may define very different identity conditions for the integrity of the content, such as chemical composition, or the sequence of layers of a bore core. Whereas an instance of E18 Physical Thing may gradually change form and chemical composition while preserving its identity, such as living beings, an instance of S11 Amount of Matter may lose its identifying features by such processes. What matters for the identity of an instance of S1 Amount of Matter is the preservation of a relevant composition from the initial state of definition onwards."@en ;
    rdfs:subClassOf <http://www.cidoc-crm.org/extensions/crmsci/S10_Material_Substantial> .

<http://www.cidoc-crm.org/extensions/crmsci/S12_Amount_of_Fluid> a rdfs:Class ;
    rdfs:label "Amount of Fluid"@en ;
    dcterms:source "CRMsci_v2.0.rdf" ;
    rdfs:comment "This class comprises fixed amounts of fluid (be they gas or liquid) defined by the total of its material content, typically molecules. They frequently acquire identity in laboratory practice by the fact of being kept or handled together within some adequate containers."@en ;
    rdfs:subClassOf <http://www.cidoc-crm.org/extensions/crmsci/S11_Amount_of_Matter>,
        <http://www.cidoc-crm.org/extensions/crmsci/S14_Fluid_Body> .

<http://www.cidoc-crm.org/extensions/crmsci/S13_Sample> a rdfs:Class ;
    rdfs:label "Sample"@en ;
    dcterms:source "CRMsci_v2.0.rdf" ;
    rdfs:comment "This class comprises instances of S11 Amount of Matter taken from some instance of S10 Material Substantial with the intention to be representative for some material qualities of the instance of S10 Material Substantial or part of it was taken for further analysis. We typically regard a sample as ceasing to exist when the respective representative qualities become corrupted, such as the purity of a water sample or the layering of a bore core."@en ;
    rdfs:subClassOf <http://www.cidoc-crm.org/extensions/crmsci/S11_Amount_of_Matter> .

<http://www.cidoc-crm.org/extensions/crmsci/S14_Fluid_Body> a rdfs:Class ;
    rdfs:label "Fluid Body"@en ;
    dcterms:source "CRMsci_v2.0.rdf" ;
    rdfs:comment "This class comprises a mass of matter in fluid form environmentally constraint in some persistent form allowing for identifying it for the management or research of material phenomena, such as a part of the sea, a river, the atmosphere or the milk in a bottle. Fluids are generally defined by the continuity criterion which is characteristic of their substance: their amorphous matter is continuous and tends to flow. Therefore, contiguous amounts of matter within a fluid body may stay contiguous or at least be locally spatially confined for a sufficiently long time in order to be temporarily identified and traced. This is a much weaker concept of stability of form than the one we would apply to what one would call a physical object. In general, an instance of Fluid Body may gain or lose matter over time through so-called sources or sinks in its surface, in contrast to physical things, which may lose or gain matter by exchange of pieces such as spare parts or corrosion."@en ;
    rdfs:subClassOf <http://www.cidoc-crm.org/extensions/crmsci/S10_Material_Substantial> .

<http://www.cidoc-crm.org/extensions/crmsci/S15_Observable_Entity> a rdfs:Class ;
    rdfs:label "Observable Entity"@en ;
    dcterms:source "CRMsci_v2.0.rdf" ;
    rdfs:comment "This class comprises instances of E5 Event or S10 Material Substantial (i.e. items or phenomena, such as physical things, their behaviour, states and interactions or events), that can be observed by measurement or detection devices or by human sensory impression including when enhanced by tools. In order to be observable, instances of E5 Event must consist of some interaction or action of material substance. In some cases, the spatiotemporal confinement of the event itself, such as a flash, a car stopping etc. marks the limits of a documented observation of an event. In other cases, such as the situation of a car passing by a certain object, the spatiotemporal limits of the event of observing itself, as well as the direction of attention or the orientation of used instruments, may constrain the observed detail of a larger process, e.g., noticing the sight of a car passing by; a light emission, etc. Conceptual objects manifest through their carriers such as books, digital media, or even human memory. Attributes of conceptual objects, such as number of words, can be observed on their carriers. If the respective properties between carriers differ, either they carry different instances of conceptual objects or the difference can be attributed to accidental deficiencies in one of the carriers. In that sense even immaterial objects are observable. By this model we address the fact that frequently, the actually observed carriers of conceptual objects are not explicitly identified in documentation, i.e., they are assumed to have existed but they are unknown as individuals."@en ;
    rdfs:subClassOf <http://www.cidoc-crm.org/cidoc-crm/E1_CRM_Entity> .

<http://www.cidoc-crm.org/extensions/crmsci/S17_Physical_Genesis> a rdfs:Class ;
    rdfs:label "Physical Genesis"@en ;
    dcterms:source "CRMsci_v2.0.rdf" ;
    rdfs:comment "This class comprises events or processes that result in (generate) physical things, man-made or natural, coming into being in the form by which they are later identified. The creation of a new physical item, at the same time, can be a result of an alteration (modification) – it can become a new thing due to an alteration activity."@en ;
    rdfs:subClassOf <http://www.cidoc-crm.org/cidoc-crm/E63_Beginning_of_Existence>,
        <http://www.cidoc-crm.org/extensions/crmsci/S18_Alteration> .

<http://www.cidoc-crm.org/extensions/crmsci/S18_Alteration> a rdfs:Class ;
    rdfs:label "Alteration"@en ;
    dcterms:source "CRMsci_v2.0.rdf" ;
    rdfs:comment "This class comprises natural events or man-made processes that create, alter or change physical things, by affecting permanently their form or consistency without changing their identity. Examples include alterations on depositional features-layers by natural factors or disturbance by roots or insects, organic alterations, petrification, etc."@en ;
    rdfs:subClassOf <http://www.cidoc-crm.org/cidoc-crm/E5_Event> .

<http://www.cidoc-crm.org/extensions/crmsci/S19_Encounter_Event> a rdfs:Class ;
    rdfs:label "Encounter Event"@en ;
    dcterms:source "CRMsci_v2.0.rdf" ;
    rdfs:comment "This class comprises activities of S4 Observation (substance) where an E39 Actor encounters an instance of E18 Physical Thing of a kind relevant for the mission of the observation or regarded as potentially relevant for some community (identity). This observation produces knowledge about the existence of the respective thing at a particular place in or on surrounding matter. This knowledge may be new to the group of people the actor belongs to. In that case we would talk about a discovery. The observer may recognize or assign an individual identity of the thing encountered or regard only the type as noteworthy in the associated documentation or report. In archaeology there is a particular interest if an object is found “in situ”, i.e. if its embedding in the surrounding matter supports the assumption that the object was not moved since the archaeologically relevant deposition event. The surrounding matter with the relative position of the object in it as well as the absolute position and time of the observation may be recorded in order to enable inferences about the history of the object. In Biology, additional parameters may be recorded like the kind of ecosystem, if the biological individual survives the observation, what detection or catching devices have been used or if the encounter event supported the detection of a new biological kind (“taxon”)."@en ;
    rdfs:subClassOf <http://www.cidoc-crm.org/extensions/crmsci/S4_Observation> .

<http://www.cidoc-crm.org/extensions/crmsci/S1_Matter_Removal> a rdfs:Class ;
    rdfs:label "Matter Removal"@en ;
    dcterms:source "CRMsci_v2.0.rdf" ;
    rdfs:comment "This class comprises the activities that result in an instance of S10 Material Substantial being decreased by the removal of an amount of matter. Typical scenarios include the removal of a component or piece of a physical object, removal of an archaeological or geological layer, taking a tissue sample from a body or a sample of fluid from a body of water. The removed matter may acquire a persistent identity of different nature beyond the act of its removal, such as becoming a physical object in the narrower sense. Such cases should be modeled by using multiple instantiation with adequate concepts of creating the respective items."@en ;
    rdfs:subClassOf <http://www.cidoc-crm.org/cidoc-crm/E7_Activity> .

<http://www.cidoc-crm.org/extensions/crmsci/S20_Rigid_Physical_Feature> a rdfs:Class ;
    rdfs:label "Rigid Physical Feature"@en ;
    dcterms:source "CRMsci_v2.0.rdf" ;
    rdfs:comment "Any instance of this class is a physical feature with sufficient stability of form in itself and with respect to the physical object bearing it in order to associate a permanent reference space within which its form is invariant and at rest. The maximum volume in space that an instance of S20 Rigid Physical Feature occupies defines uniquely a place for the feature with respect to its surrounding matter. Therefore we model S20 Rigid Physical Feature as a subclass of E26 Physical Feature and of E53 Place. The latter is intended as a phenomenal place as defined in CRMgeo (Doerr and Hiebel 2013). By virtue of this multiple inheritance we can discuss positions relative to the extent of an instance of S20 Rigid Physical Feature without representing each instance of it together with an instance of its associated place. However, since the identity and existence of this place depends uniquely on the identity of the instance of S20 Rigid Physical Feature as matter, this multiple inheritance is unambiguous and effective and furthermore corresponds to the intuitions of natural language. It shortcuts an implicit self-referential path from E26 Physical Feature through P156 occupies, E53 Place, P157 is at rest relative to E26 Physical Feature. In cases of instances of S20 Rigid Physical Feature on or in the surface of earth, the default reference is typically fixed to the closer environment of the tectonic plate or sea floor. In cases of features on mobile objects, the reference space is typically fixed to the geometry of the bearing object. Note that the reference space associated with the instance of S20 Rigid Physical Feature may quite well be deformed over time, as long the continuity of its topology does not become unclear, such as the compression of dinosaur bones in geological layers, or the distortions of the hull of a ship by the waves of the sea. Defined in this way, the reference space can be used as a means to infer from current topological relationships past topological relationships of interest."@en ;
    rdfs:subClassOf <http://www.cidoc-crm.org/cidoc-crm/E26_Physical_Feature>,
        <http://www.cidoc-crm.org/cidoc-crm/E53_Place> .

<http://www.cidoc-crm.org/extensions/crmsci/S21_Measurement> a rdfs:Class ;
    rdfs:label "Measurement"@en ;
    dcterms:source "CRMsci_v2.0.rdf" ;
    rdfs:comment "This class comprises actions measuring instances of S15 Observable Entity, properties of physical things, or phenomena, states and interactions or events, that can be determined by a systematic procedure. Primary data from measurement devices are regarded to be results of an observation process."@en ;
    rdfs:subClassOf <http://www.cidoc-crm.org/extensions/crmsci/S4_Observation> .

<http://www.cidoc-crm.org/extensions/crmsci/S22_Segment_of_Matter> a rdfs:Class ;
    rdfs:label "Segment of Matter"@en ;
    dcterms:source "CRMsci_v2.0.rdf" ;
    rdfs:comment "This class comprises physical features with relative stability of form and structure within a declared spatial volume of interest. The spatial extent of an instance of S22 Segment of Matter may be declared or defined by a researcher or observer usually because the arrangement and composition of substance is characteristic for the surrounding matter or can be interpreted as traces of its genesis and subsequent internal and external processes it was exposed to. The defining spatial extent is typically declared on a continuous matter by means of geometric determination without observable boundaries on all sides or any side. It may however be extracted at some point in time along the declared boundaries. An instance of S22 Segment of Matter is regarded to be existing from the time on it completely solidified with a structure that is still preserved in a recognizable way at the time of its spatial definition. Its existence is regarded to end when its respective integrity is partially or completely corrupted. Uncorrupted subsections of an instance of S22 Segment of Matter may continue to exist as segments of matter in their own right beyond the existence of the containing instance, and may have solidified before it. Typical examples are segments of archaeological or geological layers. They are regarded as uncorrupted even if they have undergone conformal deformations, such as compressions or shifts, as long as the effects of these deformations do not destroy the relevant structures of interest. This means that the defining spatial volume may be only geometrically valid for an instant of time for which it was declared, and undergo before and after deformations. In some cases, it may be possible to calculate the initial volume at the time of solidification, for instance for petrified bones compressed in Jurassic layers."@en ;
    rdfs:subClassOf <http://www.cidoc-crm.org/extensions/crmsci/S20_Rigid_Physical_Feature> .

<http://www.cidoc-crm.org/extensions/crmsci/S23_Position_Determination> a rdfs:Class ;
    rdfs:label "Position Determination"@en ;
    dcterms:source "CRMsci_v2.0.rdf" ;
    rdfs:comment "This class comprises activities of determining positions in space and time. The determined position is intended to approximate a part or all of the extent of the presence (instance of E93 Presence) of an instance of E18 Physical Thing or E4 Period of interest, such as the outer walls of an excavated settlement, the position of a ship sailing or the start and end of athlete's run in a competition. Characteristically, a theodolite or GPS device may be positioned on some persistent feature. Determining the position of the device will yield an approximation of the position of the feature of interest. Alternatively, some material item may be observed moving through a determined position at a given time. This class does not inherit properties from class S21 Measurement. A position determination is an evaluation of a combination of measurement of multiple associated distances and/or angles (instances of E54 Dimension) from a particular spot to certain reference points of previously known position in the same reference space. A particular role is played by the Earth's magnetic field and rotational axis as reference for an angle or direction. Often, the observed constituting dimensions are not documented, or hidden in an electronic device software. The determined position is given as an E94 Space Primitive corresponding to a declarative place. Together with the measured time-span covering the time-critical observations it forms a spacetime volume, which should normally overlap with the spatiotemporal extent of the thing or phenomenon of interest."@en ;
    rdfs:subClassOf <http://www.cidoc-crm.org/extensions/crmsci/S4_Observation> .

<http://www.cidoc-crm.org/extensions/crmsci/S24_Sample_Splitting> a rdfs:Class ;
    rdfs:label "Sample Splitting"@en ;
    dcterms:source "CRMsci_v2.0.rdf" ;
    rdfs:comment "This class comprises the activity of dividing an instance of S13 Sample into new instances of S13 Sample. This activity describes cases of sub-sampling where the resulting instance maintains the characteristic qualities of the original instance. Any observations of these qualities made on the new instance also apply to the original one. This class should be used to model cases of splitting a homogenous sample into multiple ones."@en ;
    rdfs:subClassOf <http://www.cidoc-crm.org/extensions/crmsci/S2_Sample_Taking> .

<http://www.cidoc-crm.org/extensions/crmsci/S2_Sample_Taking> a rdfs:Class ;
    rdfs:label "Sample Taking"@en ;
    dcterms:source "CRMsci_v2.0.rdf" ;
    rdfs:comment "This class comprises the activity that results in taking an amount of matter as sample for further analysis from a material substantial such as a body of water, a geological formation or an archaeological object. The removed matter may acquire a persistent identity of different nature beyond the act of its removal, such as becoming a physical object in the narrower sense. The sample is typically removed from a physical feature which is used as a frame of reference, the place of sampling. In case of non-rigid Material Substantials, the source of sampling may regarded not to be modified by the activity of sample taking."@en ;
    rdfs:subClassOf <http://www.cidoc-crm.org/extensions/crmsci/S1_Matter_Removal> .

<http://www.cidoc-crm.org/extensions/crmsci/S3_Measurement_by_Sampling> a rdfs:Class ;
    rdfs:label "Measurement by Sampling"@en ;
    dcterms:source "CRMsci_v2.0.rdf" ;
    rdfs:comment "This class comprises activities of taking a sample and measuring or analyzing it as one unit of activity, in which the sample is typically not identified and preserved beyond the context of this activity. Instances of this class describe the taking of one or more samples regardless whether they are explicitly identified in documentation or preserved beyond this activity. The dimensions observed by the respective measurement of this particular sample are regarded as dimensions of the instance of S10 Material Substantial at the place from which the samples were taken. Therefore, the class S3 Measurement by Sampling inherits the properties of S2 Sample Taking, O3 sampled from: S10 Material Substantial and O4 sampled at: E53 Place, and the properties of S21 Measurement O24 measured: S15 Observable Entity. It needs not instantiate the properties O5 removed: S13 Sample and O24 measured: S15 Observable Entity, if the sample is not documented beyond the context of the activity."@en ;
    rdfs:subClassOf <http://www.cidoc-crm.org/extensions/crmsci/S21_Measurement>,
        <http://www.cidoc-crm.org/extensions/crmsci/S2_Sample_Taking> .

<http://www.cidoc-crm.org/extensions/crmsci/S4_Observation> a rdfs:Class ;
    rdfs:label "Observation"@en ;
    dcterms:source "CRMsci_v2.0.rdf" ;
    rdfs:comment "This class comprises the activity of gaining scientific knowledge about particular states of physical reality through empirical evidence, experiments and measurements. We define observation in the sense of natural sciences, as a kind of human activity: at some place and within some time-span, certain physical things and their behavior and interactions are observed by human sensory impression, and often enhanced by tools and measurement devices. Observed situations or dimensions may pertain to properties confined to a single instance of S15 Observable Entity or pertain to constellations of multiple instances and relations between them, in particular distances between them. The output of the internal processes of measurement devices that do not require additional human interaction are in general regarded as part of the observation and not as additional inference. Primary data from measurement devices are regarded in this model to be results of observation and can be interpreted as propositions believed to be true within the (known) tolerances and degree of reliability of the device. Measurements and witnessing of events are special cases of observations. Observations result in a belief that certain propositions held at a time within the time-span of the observation. In this model, the degree of confidence in the observed properties is regarded to be “true” by default, but could be described differently by adding a property P3 has note to an instance of S4 Observation"@en ;
    rdfs:subClassOf <http://www.cidoc-crm.org/cidoc-crm/E13_Attribute_Assignment> .

<http://www.cidoc-crm.org/extensions/crmsci/S5_Inference_Making> a rdfs:Class ;
    rdfs:label "Inference Making"@en ;
    dcterms:source "CRMsci_v2.0.rdf" ;
    rdfs:comment "This class comprises the action of making propositions and statements about particular states of affairs in reality or in possible realities or categorical descriptions of reality by using inferences from other statements based on hypotheses and any form of formal or informal logic. It includes evaluations, calculations, and interpretations based on mathematical formulations and propositions."@en ;
    rdfs:subClassOf <http://www.cidoc-crm.org/cidoc-crm/E13_Attribute_Assignment> .

<http://www.cidoc-crm.org/extensions/crmsci/S6_Data_Evaluation> a rdfs:Class ;
    rdfs:label "Data Evaluation"@en ;
    dcterms:source "CRMsci_v2.0.rdf" ;
    rdfs:comment "This class comprises the action of concluding propositions on a respective reality from observational data by making evaluations based on mathematical inference rules and calculations using established hypotheses, such as the calculation of an earthquake epicenter. S6 Data Evaluation is not defined as S21/E16 Measurement; Secondary derivations of dimensions of an object from data measured by different processes are regarded as S6 Data Evaluation and not determining instances of Measurement in its own right. For instance, the volume of a statue concluded from a 3D model is an instance of S6 Data Evaluation and not of Measurement."@en ;
    rdfs:subClassOf <http://www.cidoc-crm.org/extensions/crmsci/S5_Inference_Making> .

<http://www.cidoc-crm.org/extensions/crmsci/S7_Simulation_or_Prediction> a rdfs:Class ;
    rdfs:label "Simulation or Prediction"@en ;
    dcterms:source "CRMsci_v2.0.rdf" ;
    rdfs:comment "This class comprises activities of executing algorithms or software for simulating the behavior and the properties of a system of interacting components that form part of reality or not by using a mathematical model of the respective interactions. In particular it implies making predictions about the future behaviors of a system of interacting components of reality by starting simulation from an actually observed state, such as weather forecasts. Simulations may also be used to understand the effects of a theory, to compare theoretical predictions with reality, or to show differences with another theory."@en ;
    rdfs:subClassOf <http://www.cidoc-crm.org/extensions/crmsci/S5_Inference_Making> .

<http://www.cidoc-crm.org/extensions/crmsci/S8_Categorical_Hypothesis_Building> a rdfs:Class ;
    rdfs:label "Categorical Hypothesis Building"@en ;
    dcterms:source "CRMsci_v2.0.rdf" ;
    rdfs:comment "This class comprises the action of making categorical hypotheses based on inference rules and theories; By categorical hypotheses we mean assumptions about the kinds of interactions and related kinds of structures of a domain that have the character of “laws” of nature or human behavior, be it necessary or probabilistic. Categorical hypotheses are developed by “induction” from finite numbers of observation and the absence of observations of particular kinds. As such, categorical hypotheses are always subject to falsification by new evidence. Instances of S8 Categorical Hypothesis Building include making and questioning categorical hypotheses."@en ;
    rdfs:subClassOf <http://www.cidoc-crm.org/extensions/crmsci/S5_Inference_Making> .

<http://www.cidoc-crm.org/extensions/crmsci/S9_Property_Type> a rdfs:Class ;
    rdfs:label "Property Type"@en ;
    dcterms:source "CRMsci_v2.0.rdf" ;
    rdfs:comment "This class comprises types of properties. Typically, instances of S9 Property Type would be taken from an ontology or terminological system. In particular, instances of this class can be used to describe in a parametric way what kind of properties the values in scientific data sets are about. By virtue of such descriptions, numeric data can be interpreted as sets of propositions in terms of a formal ontology, such as “concentration of nitrate”, observed in the ground water from a certain borehole."@en ;
    rdfs:subClassOf <http://www.cidoc-crm.org/cidoc-crm/E55_Type> .

<http://www.cidoc-crm.org/extensions/crmtex/TX10_Style> a rdfs:Class ;
    rdfs:label "Style"@en ;
    dcterms:source "CRMtex_v2.0.rdf" ;
    rdfs:comment "This class describes stylistic variations of texts, including local script styles (as the Carolingian minuscule for the Latin script) and individual scribal hands. It includes: the general appearance of the script, in terms of general design, aspects related to a bilinear system (i.e., upper- and lowercase), measures (i.e., large, medium or small), shape and number of strokes forming a character, its order and direction. A style includes also information about ductus (the direction the text), ligatures and nexi (i.e., the connection between characters obtained by tracing them without detaching the writing instrument from the support and using one or more strokes in common), and the writing angle (i.e., the position the writing instrument is located with respect to the support). The style corresponds to fonts and their variations in the modern printing process."@en ;
    rdfs:subClassOf <http://www.cidoc-crm.org/cidoc-crm/E29_Design_or_Procedure> .

<http://www.cidoc-crm.org/extensions/crmtex/TX11_Grapheme_Occurrence> a rdfs:Class ;
    rdfs:label "Grapheme Occurrence"@en ;
    dcterms:source "CRMtex_v2.0.rdf" ;
    rdfs:comment "This class comprises single occurrences of a Grapheme used as an atomic unit at a particular position in the abstract form of a given particular piece of text."@en ;
    rdfs:subClassOf <http://www.cidoc-crm.org/extensions/crmtex/TX12_Grapheme_Sequence> .

<http://www.cidoc-crm.org/extensions/crmtex/TX12_Grapheme_Sequence> a rdfs:Class ;
    rdfs:label "Grapheme Sequence"@en ;
    dcterms:source "CRMtex_v2.0.rdf" ;
    rdfs:comment "This class comprises particular sequences of Graphemes used for representing the abstract written form of a section of a given particular text."@en ;
    rdfs:subClassOf <http://www.cidoc-crm.org/cidoc-crm/E90_Symbolic_Object> .

<http://www.cidoc-crm.org/extensions/crmtex/TX13_Script> a rdfs:Class ;
    rdfs:label "Script"@en ;
    dcterms:source "CRMtex_v2.0.rdf" ;
    rdfs:comment "This class comprises functionally complete sets of mutually different graphemes employed by one or more languages, regardless of the specific operating rules in a particular language. A writing system, on the other hand, also refers to the set of relations between symbols and linguistic units they represent. The same language may be written using different scripts."@en ;
    rdfs:subClassOf <http://www.cidoc-crm.org/cidoc-crm/E89_Propositional_Object> .

<http://www.cidoc-crm.org/extensions/crmtex/TX14_Reading> a rdfs:Class ;
    rdfs:label "Reading"@en ;
    dcterms:source "CRMtex_v2.0.rdf" ;
    rdfs:comment "This class describes the complete intellectual activity, involving the interaction of visual-perceptual, linguistic, and conceptual systems, leading from text recognition (TX5) until its association with a complete linguistic meaning."@en ;
    rdfs:subClassOf <http://www.cidoc-crm.org/extensions/crminf/I1_Argumentation> .

<http://www.cidoc-crm.org/extensions/crmtex/TX1_Written_Text> a rdfs:Class ;
    rdfs:label "Written Text"@en ;
    dcterms:source "CRMtex_v2.0.rdf" ;
    rdfs:comment "This class comprises visible or tactile marks (called glyphs or graphs), which relate in a systematic way to units of speech, intentionally traced (i.e., “written”) on some kind of physical support by using specific techniques and tools, with the purpose of conveying a message towards a given receiver or group of receivers."@en ;
    rdfs:subClassOf <http://www.cidoc-crm.org/cidoc-crm/E25_Human-Made_Feature> .

<http://www.cidoc-crm.org/extensions/crmtex/TX2_Writing> a rdfs:Class ;
    rdfs:label "Writing"@en ;
    dcterms:source "CRMtex_v2.0.rdf" ;
    rdfs:comment "This class describes the activity of communicating information by means of permanent, visible marks in a non-mechanical way, using various techniques (painting, sculpture, etc.) and by means of specific tools, on a given support."@en ;
    rdfs:subClassOf <http://iflastandards.info/ns/fr/frbr/frbroo/F28_Expression_Creation> .

<http://www.cidoc-crm.org/extensions/crmtex/TX3_Writing_System> a rdfs:Class ;
    rdfs:label "Writing System"@en ;
    dcterms:source "CRMtex_v2.0.rdf" ;
    rdfs:comment "This class represents a conventional symbolic system designed to represent units of a natural language with the purpose of recording and transmitting information. A writing system consists of a set of symbols (graphemes, TX8), instantiated through physical signs of a visual or tactile nature (glyphs, TX9) representing linguistic units of any kind and the related syntactic (i.e., graphotactic) rules. It is used to produce a TX1 Written Text during a TX2 Writing event."@en ;
    rdfs:subClassOf <http://www.cidoc-crm.org/cidoc-crm/E29_Design_or_Procedure> .

<http://www.cidoc-crm.org/extensions/crmtex/TX4_Writing_Field> a rdfs:Class ;
    rdfs:label "Writing Field"@en ;
    dcterms:source "CRMtex_v2.0.rdf" ;
    rdfs:comment "This class describes the portion of the physical carrier arranged and usually reserved and delimited for the purpose of accommodating a written text, highlighting and isolating it from the other parts of the object to which it belongs, enhancing and guaranteeing its readability. This entity is paramount specially in epigraphy, in which a specific element called “epigraphic field” has been defined by the discipline itself. Its importance is also evident in papyrology and codicology, where a clear distinction between area(s) containing the written text and empty parts of the support (margins, intercolumnia , etc.) is significant for the definition of styles and periods of the document."@en ;
    rdfs:subClassOf <http://www.cidoc-crm.org/cidoc-crm/E25_Human-Made_Feature> .

<http://www.cidoc-crm.org/extensions/crmtex/TX5_Text_Recognition> a rdfs:Class ;
    rdfs:label "Text Recognition"@en ;
    dcterms:source "CRMtex_v2.0.rdf" ;
    rdfs:comment "This class comprises activities of recognizing physical features on some surface, often an instance of TX4 Writing Field, as an arrangement of a series of identifiable glyphs of some known script, deciphered or not, in an order characteristic for a text. For study purposes, the text recognition procedure requires a scientific autoptic examination of the text. An autoptic examination consists of an accurate analysis of the surface and the signs, and prescribes the use of specific tools and procedures for establishing the exact value of each sign on the physical feature. Deterioration of the original medium or “sloppy” writing may render parts of the original text as undecipherable or ambiguous, which may be annotated in the transcript following epigraphic standards; a text recognition typically results in a record of an equivalent sequence of graphemes on another persistent medium in a scholarly established form of representation of the respective graphemes, often called a “transcript”. An instance of TX5 Text Recognition may in particular apply even to a single glyph, typically forming part of an instance of TX5 Text Recognition applying to a larger sequence of glyphs containing the former glyph. The recognition process may be assisted by mechanical means, imaging technology, or a traditional squeeze for incised glyphs. In case the recognition process is solely based on the latter, the observation concerns only the representations on the latter as present to the researcher in some physical form or projection and should unambiguously be documented as such. In case the recognized text has not been documented in a transcript, text recognition may constitute an implicit part of an overarching reading process, instance of TX14 Reading, which has resulted in other noteworthy propositions related to the content of the recognized text. On the other side, recognition of single glyphs or contracted parts of texts, as they are characteristic for the use of ligatured scripts, may quite well be implicitly supported by the reader’s comprehension of the text and the creator of the transcript may have chosen not to annotate parts that the reader regarded as unambiguous. Since these cases can often hardly be separated from the shape recognition of the glyphs in isolation, documenting such implicit comprehension as a separate process may not be relevant. It is however regarded as good practice to document explicitly the reading process and associated interpretative reasoning for any non-trivial resolution of ambiguity or gaps in the recognized text that has a bearing on the transcript or further completion of the transcript."@en ;
    rdfs:subClassOf <http://www.cidoc-crm.org/cidoc-crm/E65_Creation>,
        <http://www.cidoc-crm.org/extensions/crmsci/S4_Observation> .

<http://www.cidoc-crm.org/extensions/crmtex/TX6_Transliteration> a rdfs:Class ;
    rdfs:label "Transliteration"@en ;
    dcterms:source "CRMtex_v2.0.rdf" ;
    rdfs:comment "This class comprises activities of exactly re-writing (i.e., re-encoding) an instance of TX12 Grapheme Sequence, i.e., the characters of a text, a contiguous part or a single character of it, by using a writing system (TX3) different from that of the original text, without changing the order of characters or words, by using standard correspondences. This operation may apply a 1:1 relation between the signs of the two writing systems, a “transliteration” in the narrower sense (e.g., the ALA-LC Romanization of Greek to Latin). It may also apply an approximation of the sounds of a language, as defined by the source writing system, by that of the target writing system, normally called a “transcription” (e.g., the “rōmaji” Romanization of Japanese), or a mixture of both (e.g. the ELOT 743 Type 2 – transcription of Greek to Latin letters). In a broader sense, the term “transcription” also applies to the activity of re-encoding a text using the same writing system (see example 1). The P16 used specific object (was used for) property can be used to specify the applied method of correspondence."@en ;
    rdfs:subClassOf <http://www.cidoc-crm.org/cidoc-crm/E65_Creation> .

<http://www.cidoc-crm.org/extensions/crmtex/TX7_Written_Text_Segment> a rdfs:Class ;
    rdfs:label "Written Text Segment"@en ;
    dcterms:source "CRMtex_v2.0.rdf" ;
    rdfs:comment "This class describes portions of text considered to be of particular significance by scholars, as witnesses of a certain meaning or bearers of a particular phenomenon relevant to the investigation, study and understanding of a text. Examples of such text portions are columns, fragments, sections, paragraphs, as well as single words or signs, or other components of a written text. To each of these entities can be associated a single production event (TX2) or destruction event (E6), as in the case of letters or words damaged or worn by atmospheric agents or human interventions, as well as specific conditions (E3) for documenting its status during the text recognition process (TX5). The relationship between a written text (TX1) and its components is documented through the TXP4 has segment property."@en ;
    rdfs:subClassOf <http://www.cidoc-crm.org/extensions/crmtex/TX1_Written_Text> .

<http://www.cidoc-crm.org/extensions/crmtex/TX8_Grapheme> a rdfs:Class ;
    rdfs:label "Grapheme"@en ;
    dcterms:source "CRMtex_v2.0.rdf" ;
    rdfs:comment "This class comprises symbols used as kinds of atomic units with distinctive value in a given writing system in order to represent linguistic units of some level to encode elements of a message. According to the typology of the writing system, the represented linguistic units can be phonemes (as in Latin), syllables (as in Mycenaean Linear B), up to complete words (as in Chinese and Sumerian scripts). A writing system also provides the conventions determining how the graphemes are to be used to write a language (orthographic rules). In some writing systems, graphemes may also be used as auxiliary signs, for instance, for disambiguating senses of homonyms, as in the Japanese writing system, or to mark the semantic categories of the words, as in the ancient Egyptian determinatives."@en ;
    rdfs:subClassOf <http://www.cidoc-crm.org/cidoc-crm/E55_Type> .

<http://www.cidoc-crm.org/extensions/crmtex/TX9_Glyph> a rdfs:Class ;
    rdfs:label "Glyph"@en ;
    dcterms:source "CRMtex_v2.0.rdf" ;
    rdfs:comment "This class describes the physical, concrete features traced by a writer, representing the material manifestations of the graphemes needed to codify a linguistic expression. Glyphs are typically observed by the scholars during a text recognition activity (TX5) carried out to decode and recognise the graphemes (TX8) they represent."@en ;
    rdfs:subClassOf <http://www.cidoc-crm.org/extensions/crmtex/TX7_Written_Text_Segment> .

<http://www.ics.forth.gr/isl/CRMba/B1_Built_Work> a rdfs:Class ;
    dcterms:source "CRMba_v1.4.rdf" ;
    rdfs:subClassOf <http://www.cidoc-crm.org/cidoc-crm/E24_Physical_Man-Made_Thing>,
        <http://www.cidoc-crm.org/cidoc-crm/E92_Spacetime_Volume> .

<http://www.ics.forth.gr/isl/CRMba/B2_Morphological_Building_Section> a rdfs:Class ;
    dcterms:source "CRMba_v1.4.rdf" ;
    rdfs:subClassOf <http://www.ics.forth.gr/isl/CRMba/B1_Built_Work> .

<http://www.ics.forth.gr/isl/CRMba/B3_Filled_Morphological_Building_Section> a rdfs:Class ;
    dcterms:source "CRMba_v1.4.rdf" ;
    rdfs:subClassOf <http://www.cidoc-crm.org/cidoc-crm/E24_Physical_Man-Made_Thing>,
        <http://www.ics.forth.gr/isl/CRMba/B2_Morphological_Building_Section> .

<http://www.ics.forth.gr/isl/CRMba/B4_Empty_Morphological_Building_Section> a rdfs:Class ;
    dcterms:source "CRMba_v1.4.rdf" ;
    rdfs:subClassOf <http://www.ics.forth.gr/isl/CRMsci/S20_Physical_Feature> .

<http://www.ics.forth.gr/isl/CRMba/B5_Stratigraphic_Building_Unit> a rdfs:Class ;
    dcterms:source "CRMba_v1.4.rdf" ;
    rdfs:subClassOf <http://www.ics.forth.gr/isl/CRMarchaeo/A2_Stratigraphic_Volume_Unit> .

<http://www.ics.forth.gr/isl/CRMdig/D10_Software_Execution> a rdfs:Class ;
    dcterms:source "CRMdig_v3.2.1.rdf" ;
    rdfs:comment """This class comprises events by which a digital device runs a software program or a series of  computing 
	operations on a digital object  as a single task, which is completely determined by its digital input, 
	the software and the generic properties of the device. 
	"""@en ;
    rdfs:subClassOf <http://www.ics.forth.gr/isl/CRMdig/D7_Digital_Machine_Event> .

<http://www.ics.forth.gr/isl/CRMdig/D11_Digital_Measurement_Event> a rdfs:Class ;
    dcterms:source "CRMdig_v3.2.1.rdf" ;
    rdfs:comment """This class comprises actions measuring physical properties using a digital device, 
	that are determined by a systematic procedure and creates an instance of D9 Data Object, 
	which is stored on an instance of D13 Digital Information Carrier. 
	In contrast to instances of D10 Software Execution, environmental factors have an intended influence on the outcome of an instance of D11 Digital Measurement Event. 
	Measurement devices may include running distinct software, such as the RAW to JPEG conversion in digital cameras. 
	In this case, the event is regarded as instance of both classes, D10 Software Execution and D11 Digital Measurement Event.
	"""@en ;
    rdfs:subClassOf <http://www.cidoc-crm.org/cidoc-crm/E16_Measurement>,
        <http://www.ics.forth.gr/isl/CRMdig/D7_Digital_Machine_Event> .

<http://www.ics.forth.gr/isl/CRMdig/D12_Data_Transfer_Event> a rdfs:Class ;
    dcterms:source "CRMdig_v3.2.1.rdf" ;
    rdfs:comment """This class comprises events that transfer a digital object from one digital carrier to another. 
	Normally, the digital object remains the same. If in general or by observation the transfer implies or has 
	implied some data corruption, the change of the digital objects may be documented distinguishing input and output 
	rather than instantiating the property L14 transferred (was transferred by). 
	"""@en ;
    rdfs:subClassOf <http://www.ics.forth.gr/isl/CRMdig/D7_Digital_Machine_Event> .

<http://www.ics.forth.gr/isl/CRMdig/D13_Digital_Information_Carrier> a rdfs:Class ;
    dcterms:source "CRMdig_v3.2.1.rdf" ;
    rdfs:comment """This class comprises all instances of E84 Information Carrier that are explicitly designed to be 
	used as persistent digital physical carriers of instances of D1 Digital Object. 
	A D13 Digital Information Carrier may or may not contain information, e.g., an empty diskette.
	"""@en ;
    rdfs:subClassOf <http://www.cidoc-crm.org/cidoc-crm/E84_Information_Carrier> .

<http://www.ics.forth.gr/isl/CRMdig/D14_Software> a rdfs:Class ;
    dcterms:source "CRMdig_v3.2.1.rdf" ;
    rdfs:comment """This class comprises software codes,computer programs,procedures, and functions that are
	used to operate a system of digital objects. """@en ;
    rdfs:subClassOf <http://www.ics.forth.gr/isl/CRMdig/D1_Digital_Object> .

<http://www.ics.forth.gr/isl/CRMdig/D1_Digital_Object> a rdfs:Class ;
    dcterms:source "CRMdig_v3.2.1.rdf" ;
    rdfs:comment """This class comprises identifiable immaterial items that can be represented as sets of bit sequences, 
	such as data sets, e-texts, images, audio or video items, software, etc., and are documented as single units. 
	Any aggregation of instances of D1 Digital Object into a whole treated as single unit is also regarded as an instance of D1 Digital Object. 
	This means that for instance, the content of a DVD, an XML file on it, and an element of this file, are regarded as distinct instances of 
	D1 Digital Object, mutually related by the P106 is composed of (forms part of) property.
A D1 Digital Object does not depend on a specific physical carrier, and it can exist on one or more carriers simultaneously.
"""@en ;
    rdfs:subClassOf <http://www.cidoc-crm.org/cidoc-crm/E73_Information_Object> .

<http://www.ics.forth.gr/isl/CRMdig/D21_Person_Name> a rdfs:Class ;
    dcterms:source "CRMdig_v3.2.1.rdf" ;
    rdfs:comment """This class comprises the proper noun name that identifies a person that acts
as an entity."""@en ;
    rdfs:subClassOf <http://www.cidoc-crm.org/cidoc-crm/E82_Actor_Appellation> .

<http://www.ics.forth.gr/isl/CRMdig/D23_Room> a rdfs:Class ;
    dcterms:source "CRMdig_v3.2.1.rdf" ;
    rdfs:comment ""@en ;
    rdfs:subClassOf <http://www.cidoc-crm.org/cidoc-crm/E53_Place> .

<http://www.ics.forth.gr/isl/CRMdig/D29_Annotation_Object> a rdfs:Class ;
    dcterms:source "CRMdig_v3.2.1.rdf" ;
    rdfs:comment """This class comprises objects that make propositions about other artefacts. 
	Instances of this class are not the attributes themselves, by which things are annotated, 
	but represent the connection between the concepts related in a proposition, and the activities of creation, modification and deletion. 
	"""@en ;
    rdfs:subClassOf <http://www.cidoc-crm.org/cidoc-crm/E89_Propositional_Object> .

<http://www.ics.forth.gr/isl/CRMdig/D2_Digitization_Process> a rdfs:Class ;
    dcterms:source "CRMdig_v3.2.1.rdf" ;
    rdfs:comment """This class comprises events that result in the creation of instances of D9 Data Object that 
	represent the appearance and/or form of an instance of E18 Physical Thing such as paper documents, statues, buildings, paintings, etc. 
	A particular case is the analogue-to-digital conversion of audiovisual material.
	This class represents the transition from a material thing to an immaterial representation of it. 
	The characteristic subsequent processing steps on digital objects are regarded as instances of D3 Formal Derivation.
"""@en ;
    rdfs:subClassOf <http://www.ics.forth.gr/isl/CRMdig/D11_Digital_Measurement_Event> .

<http://www.ics.forth.gr/isl/CRMdig/D30_Annotation_Event> a rdfs:Class ;
    dcterms:source "CRMdig_v3.2.1.rdf" ;
    rdfs:comment """This class comprises events that describe the creation of associations (Annotation Objects) between objects 
	or areas of objects of the Repository, with other objects or regions or persons, places, events. It is the event that creates the Annotation Object."""@en ;
    rdfs:subClassOf <http://www.cidoc-crm.org/cidoc-crm/E65_Creation> .

<http://www.ics.forth.gr/isl/CRMdig/D35_Area> a rdfs:Class ;
    dcterms:source "CRMdig_v3.2.1.rdf" ;
    rdfs:comment """This class describes a part (of any shape or size) of interest in basically any media object stored in the Object Repository,
	i.e., a text, an image, a video or a 3D model. It points to content consisting of just a portion or area of a file. 
In some contexts, however, the area can also point to content represented by an integral (i.e., proper) file. It is equal to the METS AREA element """@en ;
    rdfs:subClassOf <http://www.cidoc-crm.org/cidoc-crm/E26_Physical_Feature>,
        <http://www.ics.forth.gr/isl/CRMdig/D1_Digital_Object> .

<http://www.ics.forth.gr/isl/CRMdig/D3_Formal_Derivation> a rdfs:Class ;
    dcterms:source "CRMdig_v3.2.1.rdf" ;
    rdfs:comment """This class comprises events that result in the creation of a D1 Digital Object from another one following a deterministic algorithm, 
	such that the resulting instance of digital object shares representative properties with the original object. 
	In other words, this class describes the transition from an immaterial object referred to by property L21 used as derivation source (was derivation source for) 
	to another immaterial object referred to by property L22 created derivative (was derivative created by) preserving the 
	representation of some things but in a different form. Characteristic examples are colour corrections, contrast changes and resizing of images.
	"""@en ;
    rdfs:subClassOf <http://www.ics.forth.gr/isl/CRMdig/D10_Software_Execution> .

<http://www.ics.forth.gr/isl/CRMdig/D7_Digital_Machine_Event> a rdfs:Class ;
    dcterms:source "CRMdig_v3.2.1.rdf" ;
    rdfs:comment """This class comprises events that happen on physical digital devices following a human activity that intentionally caused its 
	immediate or delayed initiation and results in the creation of a new instance of D1 Digital Object on behalf of the human actor. 
	The input of a D7 Digital Machine Event may be parameter settings and/or data to be processed. 
	Some D7 Digital Machine Events may form part of a wider E65 Creation event. 
	In this case, all machine output of the partial events is regarded as creation of the overall activity.
	"""@en ;
    rdfs:subClassOf <http://www.cidoc-crm.org/cidoc-crm/E11_Modification>,
        <http://www.cidoc-crm.org/cidoc-crm/E65_Creation> .

<http://www.ics.forth.gr/isl/CRMdig/D8_Digital_Device> a rdfs:Class ;
    dcterms:source "CRMdig_v3.2.1.rdf" ;
    rdfs:comment """This class comprises identifiable material items such as computers, scanners, cameras, etc. that 
	have the capability to process or produce instances of  D1 Digital Object.
	"""@en ;
    rdfs:subClassOf <http://www.cidoc-crm.org/cidoc-crm/E22_Man-Made_Object> .

<http://www.ics.forth.gr/isl/CRMdig/D9_Data_Object> a rdfs:Class ;
    dcterms:source "CRMdig_v3.2.1.rdf" ;
    rdfs:comment """This class comprises instances of D1 Digital Object that are the direct result of a digital 
	measurement or a formal derivative of it, containing quantitative properties of some physical things or other constellations of matter.
	"""@en ;
    rdfs:subClassOf <http://www.cidoc-crm.org/cidoc-crm/E54_Dimension>,
        <http://www.ics.forth.gr/isl/CRMdig/D1_Digital_Object> .

<http://www.ics.forth.gr/isl/CRMgeo/#SP1_Phenomenal_Spacetime_Volume> a rdfs:Class ;
    dcterms:source "CRMgeo_v1.2.rdf" ;
    rdfs:comment """Scope note: This class comprises the 4 dimensional point sets (volumes) (S) which material phenomena (I) occupy in Space-Time (S). An instance of S1 Space Time Volume represents the true (I) extent of an instance of E4 Period in spacetime or the true (I) extent of the trajectory of an instance of E18 Physical Thing during the course of its existence, from production to destruction. A fuzziness of the extent lies in the very nature of the phenomenon, and not in the shortcomings of observation (U). The degree of fuzziness with respect to the scale of the phenomenon may vary widely, but the extent is never exact in a mathematical sense. According to modern physics, points in space-time are absolute with respect to the physical phenomena happening at them, regardless the so-called Galilean relativity of spatial or temporal reference systems in terms of which an observer may describe them. Following the theory, points relative to different spatial or temporal reference systems can be related if common points of phenomena in space-time are known in different systems. Instances of S1 Space-Time Volume are sets of such absolute space-time points of phenomena (I).The (Einstein) relativity of spatial and temporal distances is of no concern for the scales of things in the cultural-historical discourse, but does not alter the above principles.[ØE8] The temporal projection of an instance of SP1 Space-Time Volume defines an E52 Time-Span while its spatial projection defines an SP2 Phenomenal Place[ØE9]. The true location of an instance of E18 Physical Thing during some time-span can be regarded as the spatial projection of the restriction of its trajectory to the respective time-span.
Examples:
• The Space Time Volume of the Event of Ceasars murdering
• The Space Time Volume where and when the carbon 14 dating of the "Schoeninger Speer II" in 1996 took place
• The spatio-temporal trajectory of the H.M.S. Victory from its building to its actual location
• The Space Time Volume of the temple in Abu Simbel before its removal"""^^xsd:string ;
    rdfs:subClassOf <http://www.cidoc-crm.org/cidoc-crm/E92_Spacetime_Volume>,
        geo:Feature .

<http://www.ics.forth.gr/isl/CRMgeo/SP10_Declarative_Time-Span> a rdfs:Class ;
    dcterms:source "CRMgeo_v1.2.rdf" ;
    rdfs:comment """Scope note:     	This class comprises instances of SP9 Time Intervalls that represent the Time Span defined by a SP 14 Time Expression. Thus they derive their identity through an expression defining an extent in time. Even though SP10 Declarative Time Spans have an unlimited precision, measurement devices and the possible precision within the SP11 Temporal Reference System impose limitations to the determination of a SP10 Declarative Time Span. The accuracy of a SP10 Declarative Time Spans depends upon the documentation and measurement method. 
SP10 Declarative Time Spans may be used to approximate actual (phenomenal) Time-Spans of temporal entities.  

Examples:  
•	Extent in time defined by the expression “1961”
•	Extent in time defined by the expression “From 12-17-1993 to 12-8-1996”
•	Extent in time defined by the expression “14h30 – 16h22 4th July 1945”"""^^xsd:string ;
    rdfs:subClassOf <http://www.cidoc-crm.org/cidoc-crm/E52_Time-Span>,
        <http://www.cidoc-crm.org/cidoc-crm/E89_Propositional_Object>,
        geo:Geometry .

<http://www.ics.forth.gr/isl/CRMgeo/SP11_Temporal_Reference_System> a rdfs:Class ;
    dcterms:source "CRMgeo_v1.2.rdf" ;
    rdfs:comment """Scope note:	This class compromises systems(S) that are used to describe positions and extents in a Reference Time. If relativistic effects are negligible in the wider spacetime area of interest and the speeds of associated things, then there is only one unique global reference time. The typical way to measure time is to count the cycles of a periodic process for which we have a hypothesis of constant frequency, such as oscillations of a crystal, molecular arrangement, rotation of earth around itself or around the sun. The origin for a Temporal Reference System is fixed on a reference event. As long as the number of cycles passed from that reference event until now are known, the temporal reference system exists (E) and expressions in this Reference System can be interpreted with respect to the Reference Time. 
A temporal reference system represents time as a continuous linear interpolation over the infinit series of cycles extended from the reference event to he past and the future, regardless of the temporal position of the mathematical point zero of an instance of E61 Time Primitive, such for instance the gregorian calender begins with the event an arbitrary positiong the point zero as beeing the date of the „Birth of Christ“. The actual date of birth of christ is regarded to be unknown and therefor is not the reference event. 
The identity of a Temporal Reference System is defined through the type of periodic process it is based on, the reference event and through the distance of the reference event to the position of the mathematical point zero (I).
A value in the Reference Time is a temporal position measured relative to a temporal reference system. ISO 8601 specifies the use of the Gregorian Calendar and 24 hour local or Coordinated Universal Time (UTC) for information interchange. 
In ISO 19108 three common types of temporal reference systems are explicitly stated: calendars (used with clocks for greater resolution), temporal coordinate systems, and ordinal temporal reference systems. 
Calendars and clocks are both based on interval scales. A calendar is a discrete temporal reference system that provides a basis for defining temporal position to a resolution of one day. A clock provides a basis for defining temporal position within a day. A clock must be used with a calendar in order to provide a complete description of a temporal position within a specific day. Every calendar provides a set of rules for composing a calendar date from a set of elements such as year, month, and day. In every calendar, years are numbered relative to the date of a reference event that defines a calendar era [ISO 19108].
Specifying temporal position in terms of calendar date and time of day complicates the computation of distances between points and the functional description of temporal operations. A temporal coordinate system may be used to support applications of this kind. [ISO 19108].
Ordinal temporal reference systems as specified in ISO 19108 are no instances of SP11 Temporal Reference Systems as they do not define cycles of a periodic process but define a system of time intervals based on reverence periods related to certain natural or cultural phenomena. 
Examples:  
•	Gregorian Calendar
•	Coordinated Universal Time (UTC) 
•	Julian date
•	Greenwich time
•	ISO 8601"""^^xsd:string ;
    rdfs:subClassOf <http://www.cidoc-crm.org/cidoc-crm/E29_Design_or_Procedure> .

<http://www.ics.forth.gr/isl/CRMgeo/SP12_Spacetime_Volume_Expression> a rdfs:Class ;
    dcterms:source "CRMgeo_v1.2.rdf" ;
    rdfs:comment """Scope Note:	This class comprises instances of E59 Primitive Value for spacetime volumes that should be implemented with appropriate validation, precision, interval logic and reference systems to express date ranges and geometries relevant to cultural documentation. A Spacetime Volume Expression may consist of one expression including temporal and spatial information like in GML or a different form of expressing spacetime in an integrated way like a formula containing all 4 dimensions.
A Spacetime Volume Expression defines a SP7 Declarative Spacetime Volume, which means that the identity of the Spacetime Volume is derived from its geometric and temporal definition. This declarative Spacetime Volume allows for the application of all Spacetime Volume properties to relate phenomenal Spacetime Volumes of Periods and Physical Things to propositions about their spatial and temporal extents. 
Examples:
•	Spatial and temporal information in KML for the maximum extent of the Byzantine Empire
•	a spacetime volume expressed in Geography Markup Language (GML) defining the spatial extent of France from 1792-1816 giving one spatial extent for each year
"""^^xsd:string ;
    rdfs:subClassOf <http://www.cidoc-crm.org/cidoc-crm/E73_Information_Object>,
        geo:Geometry .

<http://www.ics.forth.gr/isl/CRMgeo/SP13_Phenomenal_Time-Span> a rdfs:Class ;
    dcterms:source "CRMgeo_v1.2.rdf" ;
    rdfs:comment """Scope note:     	This class comprises instances of SP9 Time Intervalls whose extent (U) and position is defined by the temporal projection of the spatiotemporal extent that can be observed or measured. Thus they derive their identity through the extent in time of a real world phenomenon (I). 

Examples:  
•	Duration of the phenomenal temporal extent of the Trafalgar battle
•	The real duration of the Ming Dynasty 
•	The real extent of the lifetime of Ceasar starting with his birth and ending with his death"""^^xsd:string ;
    rdfs:subClassOf <http://www.cidoc-crm.org/cidoc-crm/E52_Time-Span> .

<http://www.ics.forth.gr/isl/CRMgeo/SP14_Time_Expression> a rdfs:Class ;
    dcterms:source "CRMgeo_v1.2.rdf" ;
    rdfs:comment """Scope note: 	This class comprises definitions of temporal extents by quantitative expressions(S). An instance of SP14 Time Expression defines a declarative temporal interval using a temporal reference system. The identity of a SP14 Time Expression is based on its script or symbolic form (I). Several SP14 Time Expressions can denote the same SP10 Declarative Time Interval. 
Instances of SP14 Time Expression that exist in one SP11 Temporal Reference System can be transformed to time expressions in other SP11 Temporal Reference Systems if there is a known and valid transformation.

Examples:
•	Temporal information in GML 
<gml:validTime><gml:TimeInstant> 
<gml:timePosition>2005-11-28T13:00:00Z</gml:timePosition> 
</gml:TimeInstant></gml:validTime> 
•	1961
•	From 12-17-1993 to 12-8-1996
•	14h30 – 16h22 4th July 1945
•	9.30 am 1.1.1999 to 2.00 pm 1.1.1999"""^^xsd:string ;
    rdfs:subClassOf <http://www.cidoc-crm.org/cidoc-crm/E49_Time_Appellation>,
        <http://www.cidoc-crm.org/cidoc-crm/E73_Information_Object>,
        geo:Geometry .

<http://www.ics.forth.gr/isl/CRMgeo/SP15_Geometry> a rdfs:Class ;
    dcterms:source "CRMgeo_v1.2.rdf" ;
    rdfs:comment """Scope note: 	This class comprises ....(to be elaborated further)
	Equivalent to:	http://www.opengis.net/ont/geosparql#Geometry   (geosparql)"""^^xsd:string ;
    rdfs:subClassOf <http://www.ics.forth.gr/isl/CRMgeo/SP6_Declarative_Place>,
        geo:Geometry .

<http://www.ics.forth.gr/isl/CRMgeo/SP2_Phenomenal_Place> a rdfs:Class ;
    dcterms:source "CRMgeo_v1.2.rdf" ;
    rdfs:comment """Scope note: This class comprises instances of E53 Place (S) whose extent (U) and position is defined by the spatial projection of the spatiotemporal extent of a real world phenomenon that can be observed or measured. The spatial projection depends on the instance of S3 Reference Space onto which the extent of the phenomenon is projected. In general, there are no limitations to the number of Reference Spaces one could regard, but only few choices are relevant for the cultural-historical discourse. Typical for the archaeological discourse is to choose a reference space with respect to which the remains of some events would stay at the same place, for instance, relative to the bedrock of a continental plate. On the other side, for the citizenship of babies born in aeroplanes, the space in which the boundaries of the overflown state are defined may be relevant (I). Instances of SP2 Phenomenal Place exist as long as the respective reference space is defined. Note that we can talk in particular about what was at a place in a country before a city was built there, i.e., before the time the event occurred by which the place is defined, but we cannot talk about the place of earth before it came into existence due to lack of a reasonable reference space (E).
Examples:
• The place where the murder of Ceasar happened
• Place on H.M.S. Victory at which Nelson died
• The Place of the Varus Battle
• The volume in space of my vine glass
• The place the H.M.S Victory occupied over the seafloor when Nelson died
• The space enclosed by this room
• The space in borehole Nr. 405"""^^xsd:string ;
    rdfs:subClassOf <http://www.cidoc-crm.org/cidoc-crm/E53_Place>,
        geo:Feature .

<http://www.ics.forth.gr/isl/CRMgeo/SP3_Reference_Space> a rdfs:Class ;
    dcterms:source "CRMgeo_v1.2.rdf" ;
    rdfs:comment """Scope note:	This class comprises the (typically Euclidian) Space (S) that is at rest (I) in relation to an instance of E18 Physical Thing and extends (U) infinitely beyond it. It is the space in which we typically expect things to stay in place if no particular natural or human distortion processes occur. This definition requires that at least essential parts of the respective physical thing have a stability of form. The degree of this stability (e.g., elastic deformation of a ship on sea, landslides, geological deformations) limits the precision to which an instance of SP3 Reference Space is defined. It is possible to construct types of (non Euclidian) reference spaces which adapt to elastic deformations or have other geometric and dynamic properties to adapt to changes of form of the reference object, but they are of rare utility in the cultural-historical discourse. [ØE11]
An instance of SP3 Reference Space begins to exist with the largest thing that is at rest in it and ceases to exist with its E6 Destruction[ØE12]. If other things are at rest in the same space and their time-span of existence falls within the one of the reference object, they share the same reference space (I). It has therefore the same temporal extent (time-span of existence) as the whole of the E18 Physical Things it is at rest with (E). 
Examples:
• The Space inside and around H.M.S. Victory while it is moving through the Atlantic Ocean
• The Space inside and around the Eurasian Continental Plate
• The Space inside and around the Earth
• The Space inside and around the Solar system"""^^xsd:string ;
    rdfs:subClassOf <http://www.cidoc-crm.org/cidoc-crm/E1_CRM_Entity> .

<http://www.ics.forth.gr/isl/CRMgeo/SP4_Spatial_Coordinate_Reference_System> a rdfs:Class ;
    dcterms:source "CRMgeo_v1.2.rdf" ;
    rdfs:comment """Scope note:	This class compromises systems that are used to describe locations in a SP3 Reference Space (S). An instance of SP4 Spatial Coordinate Reference System is composed of two parts: The first is a Coordinate System which is a set of coordinate axes with specified units of measurement and axis directions. The second part is a set of reference features at rest in the Reference Space it describes in the real world that relate the Coordinate System to real world locations (U) and fix it with respect to the reference object of its Reference Space .
In surveying and geodesy, instance of SP4 Spatial Coordinate Reference System are called a datum. In the case of spatial coordinate reference systems for the earth the datum consists of the reference points and an ellipsoid that approximates the shape of the earth. National systems often use ellipsoids that approximate their territory best and shift them in an appropriate position relative to the earth while WGS84 is an ellipsoid for the whole earth and used in GPS receivers. In engineering a datum is a reference feature of an object used to create a reference system for measurement.The set of reference features in the real world are subset of E26 Physical Feature that are within the described reference space at rest and pertain to the E18 Physical Thing the reference space is at rest with.
SP4 Spatial Coordinate Reference Systems have a validity for a certain spatial extent of the SP3 Reference Space and in addition a temporal validity. The combination of coordinate reference system and datum provides a unique identity (I). SP4 Spatial Coordinate Reference Systems may be defined for the earth, moving objects like planes or ships, linear features like boreholes or local systems. If there is a standardised identifier system available, such as EPSG codes, it should be used.
Examples:
• Longitude-Latitude(ellipsoidal Coordinate System) in WGS84 (Datum)
• EPSG 3241
• the coordinate system to describe locations on H.M.S. Victory taking the deck foundation of the middle mast as origin, the mast as z axis, the line at right angle to the bow line as x axis and a right angle to both as y axis.
• The printed lines of the millimeter paper on which an archaeological feature is drawn"""^^xsd:string ;
    rdfs:subClassOf <http://www.cidoc-crm.org/cidoc-crm/E29_Design_or_Procedure> .

<http://www.ics.forth.gr/isl/CRMgeo/SP5_Geometric_Place_Expression> a rdfs:Class ;
    dcterms:source "CRMgeo_v1.2.rdf" ;
    rdfs:comment """Scope note: 	This class comprises definitions of places by quantitative expressions. An instance of SP5 Geometric Place Expression can be seen as a prescription of how to find the location meant by this expression in the real world (S), which is based on measuring where the quantities referred to in the expression lead to, beginning from the reference points of the respective reference system. 
A form of expression may be geometries or map elements defined in a SP4 Spatial Coordinate Reference System that unambiguously identify locations in a SP3 Reference Space. Other forms may refer to areas confined by imaginary lines connecting Phenomenal Places such as trees, islands, cities, mountain tops. 
The identity of a SP5 Place Expression is based on its script or symbolic form (I). Several SP5 Place Expressions can denote the same SP6 Declarative Place. 
Instances of SP5 Geometric Place Expressions that exist in one SP4 Spatial Coordinate Reference System can be transformed to geometries in other SP4 Spatial Coordinate Reference System if there is a known and valid transformation. The product of the transformation in general defines a new instance of SP6 Declarative Place, albeit close to the source of the transformation. This can be due to distortions resulting from the transformation and the limited precision by which the relative position of the reference points differing between the respective reference systems are determined.      

Examples:
• Coordinate Information in GML like <gml:Point gml:id="p21" srsName="http://www.opengis.net/def/crs/EPSG/0/4326"> <gml:coordinates>45.67, 88.56</gml:coordinates> </gml:Point>
• a polygon defining the extent of France"""^^xsd:string ;
    rdfs:subClassOf <http://www.cidoc-crm.org/cidoc-crm/E47_Spatial_Coordinates>,
        <http://www.cidoc-crm.org/cidoc-crm/E73_Information_Object>,
        geo:Geometry .

<http://www.ics.forth.gr/isl/CRMgeo/SP6_Declarative_Place> a rdfs:Class ;
    dcterms:source "CRMgeo_v1.2.rdf" ;
    rdfs:comment """Scope note: This class comprises instances of E53 Place (S) whose extent (U) and position is defined by a SP5 Geometric Place Expression (S). There is one implicit or explicit SP3 Reference Space in which the SP5 Place Expression describes the intended place. Even though SP5 Geometric Place Expressions have an unlimited precision, measurement devices and the precision of the position of reference features relating the SP4 Spatial Coordinate Reference System to a SP3 Reference Space impose limitations to the determination of an SP6 Declarative Place in the real world (U).
Several SP5 Geometric Place Expressions may denote the same SP6 Declarative Place if their precision falls within the same range (I).
Instances of SP6 Declarative Places may be used to approximate instances of E53 Places or parts of them. They may as well be used to define the location and spatial extent of property rights or national borders.

Examples:
• the place defined by <gml:Point gml:id="p21" srsName="http://www.opengis.net/def/crs/EPSG/0/4326"> <gml:coordinates>45.67, 88.56</gml:coordinates> </gml:Point>
• the place defined by a line approximating the Danube river
• The place of the Orinoco river defined in the map of Diego Ribeiro in 1529
• the place defined through a polygon that represents the boundaries of the UK in the year 2003			
	"""^^xsd:string ;
    rdfs:subClassOf <http://www.cidoc-crm.org/cidoc-crm/E53_Place>,
        <http://www.cidoc-crm.org/cidoc-crm/E89_Propositional_Object>,
        geo:Geometry .

<http://www.ics.forth.gr/isl/CRMgeo/SP7_Declarative_Spacetime_Volume> a rdfs:Class ;
    dcterms:source "CRMgeo_v1.2.rdf" ;
    rdfs:comment """Scope note: 	This class comprises instances of SP8 Spacetime Volumes (S) whose temporal and spatial extent (U) and position is defined by a SP12 Spacetime Volume Expression. There is one implicit or explicit SP3 Reference Space in which the SP12 Spacetime Volume Expression describes the intended Spacetime Volume. As we restrict the model to Galilean physics and explicitly exclude systems with velocities close to the speed of light we do not model a “Reference Time” as it would be necessary for relativistic physics. This implies that there is only one Reference Time. 
Even though SP12 Spacetime Volume Expressions have an unlimited precision, measurement devices and the precision of the position of reference features relating the SP4 Spatial Coordinate Reference System to a SP3 Reference Space impose limitations to the determination of the spatial part of a SP7 Declarative Spacetime Volume in the real world (U).
The same limitation to precision is true for the temporal part of a SP7 Declarative Spacetime Volume due to precision of time measurement devices and of the determination of the reference event of a SP11 Temporal Reference System. 
	Several SP12 Spacetime Volume Expressions may denote the same SP7 Declarative Spacetime Volume if their precision falls within the same range (I).
Instances of SP7 Declarative Spacetime Volumes may be used to approximate instances of SP8 Spacetime Volumes or parts of them. They may as well be used to define the spatial and temporal extent of property rights or national borders.

Examples:
•	the spacetime volume defined by a polygon approximating the Danube river flood in Austria between 6th and 9th of August 2002 
•	the spacetime volume of the Orinoco river in 1529 defined in the map of Diego Ribeiro in 1529
•	the spacetime volume representing the boundaries of the UK from 1900-1950"""^^xsd:string ;
    rdfs:subClassOf <http://www.cidoc-crm.org/cidoc-crm/E89_Propositional_Object>,
        <http://www.cidoc-crm.org/cidoc-crm/E92_Spacetime_Volume>,
        geo:Geometry .

<http://www.ics.forth.gr/isl/CRMinf/I1_Argumentation> a rdfs:Class ;
    dcterms:source "CRMinf_v0.7.rdf" ;
    rdfs:comment """
            This class comprises the activity of making honest inferences or observations. An honest inference or observation is one in which the E39 Actor carrying out the I1 Argumentation justifies and believes that the I6 Belief Value associated with resulting I2 Belief about the I4 Proposition Set is the correct value at the time that the activity was undertaken and that any I3 Inference Logic  or methodology was correctly applied.
	Only one instance of E39 Actor may carry out an instance of I1 Argumentation, though the E39 Actor may, of course, be an instance of E74 Group.
"""@en .

<http://www.ics.forth.gr/isl/CRMinf/I2_Belief> a rdfs:Class ;
    dcterms:source "CRMinf_v0.7.rdf" ;
    rdfs:comment """
            This class comprises the notion that the associated I4 Proposition Set is held to have a particular I6 Belief Value by a particular E39 Actor. This can be understood as the period of time that an individual or group holds a particular set of propositions to be true, false or somewhere in between."""@en ;
    rdfs:subClassOf <http://www.cidoc-crm.org/cidoc-crm/E2_Temporal_Entity> .

<http://www.ics.forth.gr/isl/CRMinf/I3_Inference_Logic> a rdfs:Class ;
    dcterms:source "CRMinf_v0.7.rdf" ;
    rdfs:comment """
            This class comprises the rules used as inputs to I5 Inference Making.
	In this context the term “logic” is used in the most general sense of the Greek term, and not in the mathematical sense only. Examples are the direct application of formal logic, mathematical theories and calculus, formal or informal default reasoning based on default values associated with categories, probabilistic reasoning based mathematical models and assumed or observed frequencies for certain categories, application of theoretical social models and comparisons with “cultural parallels”, etc. An instance of Inference Logic could also be a reference to the exact software release of a Bayesian reasoner, a rule such as “later layers are on top of earlier layers”, or even a term like “social intuition”, if this is scholarly acceptable. (after Doerr, Kritsotaki and Boutsika 2011). Indeed anything that is scientifically or academically acceptable as a method for drawing conclusions may be included for instance human pattern recognition.
	A particular instance of I3 Inference Logic would be the algorithm implemented in a particular revision of a software package.
	Instances of I3 Inference Logic not only comprise the method of reasoning, but also the set of categorical laws or axioms used in the argumentation. Often both are inextricably interwoven, for instance in a software implementation.
"""@en ;
    rdfs:subClassOf <http://www.cidoc-crm.org/cidoc-crm/E89_Propositional_Object> .

<http://www.ics.forth.gr/isl/CRMinf/I4_Proposition_Set> a rdfs:Class ;
    dcterms:source "CRMinf_v0.7.rdf" ;
    rdfs:comment """
            This class comprises the sets of formal, binary propositions that an I2 Belief is held about. It could be implemented as a named graph, a spreadsheet or any other structured data-set. Regardless of the specific syntax employed, the effective propositions it contains should be made up of unambiguous identifiers, concepts of a formal ontology and constructs of logic."""@en ;
    rdfs:subClassOf <http://www.cidoc-crm.org/cidoc-crm/E73_Information_Object> .

<http://www.ics.forth.gr/isl/CRMinf/I5_Inference_Making> a rdfs:Class ;
    dcterms:source "CRMinf_v0.7.rdf" ;
    rdfs:comment """
            This class comprises the action of making honest propositions and statements about particular states of affairs in reality or in possible realities or categorical descriptions of reality by using inferences from other statements based on hypotheses and any form of formal or informal logic. It includes evaluations, calculations, and interpretations based on mathematical formulations and propositions. 
	It is characterized by the use of an existing I2 Belief as the premise that together with a set of I3 Inference Logic draws a further I2 Belief as a conclusion.
	Documenting instances of I5 Inference Making primarily enables tracing the dependency of knowledge from conclusion to premise through subsequent inferences, possibly back to primary evidence, so that the range of influence of knowledge revision at any intermediate stage of complex inference chains on current convictions can be narrowed down by query. The explicit reference to the applied inference logic further allows scholars or scientists to assess if they can or would follow the documented argument. The class is not intended to promote the use of computationally decidable systems of logic as replacements of scholarly justifications of arguments, even though it allows for documenting the use of decidable logic, if that was deemed adequate for the problem at hand.  Principles of scholarly justifications of arguments are also regarded as kinds of inference logic.
"""@en ;
    rdfs:subClassOf <http://www.ics.forth.gr/isl/CRMinf/I1_Argumentation> .

<http://www.ics.forth.gr/isl/CRMinf/I7_Belief_Adoption> a rdfs:Class ;
    dcterms:source "CRMinf_v0.7.rdf" ;
    rdfs:comment """
            This class comprises the action of an E39 Actor adopting a particular instance of I2 Belief to create a new instance of I2 Belief that shares some of the same propositions in the original I4 Proposition Set and the associated I6 Belief Value.
	The basis of I7 Belief Adoption is trust in the source of the instance of I2 Belief rather than the application of the rules in instances of I3 Inference Logic.
		Typical examples are the citation of academic papers or the reuse of data sets.
	Where an instance of I7 Belief Adoption is based on personal communication (pers.comm.) this should be represented by using P2 has type: “Pers.Comm.” directly from the instance of I7 Belief Adoption.
"""@en ;
    rdfs:subClassOf <http://www.ics.forth.gr/isl/CRMinf/I1_Argumentation> .

<http://www.ics.forth.gr/isl/CRMsci/S4_Observation> a rdfs:Class ;
    dcterms:source "CRMinf_v0.7.rdf" ;
    rdfs:subClassOf <http://www.ics.forth.gr/isl/CRMinf/I1_Argumentation> .

<http://www.ics.forth.gr/isl/CRMsci/S6_Data_Evaluation> a rdfs:Class ;
    dcterms:source "CRMinf_v0.7.rdf" ;
    rdfs:subClassOf <http://www.ics.forth.gr/isl/CRMinf/I5_Inference_Making> .

<http://www.ics.forth.gr/isl/CRMsci/S7_Simulation_or_Prediction> a rdfs:Class ;
    dcterms:source "CRMinf_v0.7.rdf" ;
    rdfs:subClassOf <http://www.ics.forth.gr/isl/CRMinf/I5_Inference_Making> .

<http://www.ics.forth.gr/isl/CRMsci/S8_Categorical_Hypothesis_Building> a rdfs:Class ;
    dcterms:source "CRMinf_v0.7.rdf" ;
    rdfs:subClassOf <http://www.ics.forth.gr/isl/CRMinf/I5_Inference_Making> .

geo:gmlLiteral a rdfs:Class ;
    dcterms:source "CRMgeo_v1.2.rdf" ;
    rdfs:subClassOf <http://www.ics.forth.gr/isl/CRMgeo/SP5_Geometric_Place_Expression> .

geo:wktLiteral a rdfs:Class ;
    dcterms:source "CRMgeo_v1.2.rdf" ;
    rdfs:subClassOf <http://www.ics.forth.gr/isl/CRMgeo/SP5_Geometric_Place_Expression> .

<https://ontology.swissartresearch.net/aaao/ZE10_Family_Status> a rdfs:Class ;
    rdfs:label "Family Status"@en ;
    dcterms:source "AAAo_v2.0.rdf" ;
    rdfs:comment """An instance of family status is the collective ascription of a familial relationship between one person and another by a community. The substance of the family status is the communal recognition of the familial connection between the two actors in question.
Instances of family status are recognizable through evidence of community members adopting the intentional stance and behaviour indicated as proper to this relation, as observable from direct witnesses, through the reports of competent observers or through evidence of a declarative act (e.g.: adoption) initiating this status.
Instances of family status may come to be simply through birth in a certain community or may require that a formal process such as a right of passage has been undertaken. Instances of family status may end either though a formal process such as a renunciation or through death."""^^xsd:string ;
    rdfs:subClassOf <https://ontology.swissartresearch.net/aaao/ZE55_Social_Relation_Status> ;
    skos:notation "ZE10"^^xsd:string .

<https://ontology.swissartresearch.net/aaao/ZE11_Membership_Status> a rdfs:Class ;
    rdfs:label "Membership Status"@en ;
    dcterms:source "AAAo_v2.0.rdf" ;
    rdfs:comment """An instance of membership status is the collective ascription of a membership relationship between an actor and some group by a community. The substance of the membership status is the communal recognition of the ascribed membership relation between the actor and the group in question.
Instances of membership status are recognizable through evidence of community members adopting the intentional stance and behaviour indicated as proper to this relation, as observable from direct witnesses, through the reports of competent observers or through evidence of a declarative act [e.g.: ZE22 Declarative Joining] initiating this status.
Instances of membership status may come to be through a formal process such as a declarative act of declarative joining or may have arisen through habit, fiat or be of unknown origin. Instances of membership status may end either though a formal process [e.g.: ZE23 Declarative Leaving], or may simply fade out, be eliminated by fiat or for unknown reasons."""^^xsd:string ;
    rdfs:subClassOf <https://ontology.swissartresearch.net/aaao/ZE1_Institutional_Fact> ;
    skos:notation "ZE11"^^xsd:string .

<https://ontology.swissartresearch.net/aaao/ZE12_Referential_Status> a rdfs:Class ;
    rdfs:label "Referential Status"@en ;
    dcterms:source "AAAo_v2.0.rdf" ;
    rdfs:comment """An instance of referential status is the collective ascription of a referential relationship between a propositional object and some entity by a community. The substance of the referential status is the communal recognition of the ascribed referential relation holding between the propositional object and the entity in question.
Instances of referential status are recognizable through evidence of community members adopting the intentional stance and behaviour indicated as properly holding between the propositional object and the object it is taken to refer to in the manner it is meant to refer, as observable from direct witnesses, through the reports of competent observers or through evidence of a declarative act initiating this status.
Instances of referential status may come to be through a formal process such as a declarative act or may have arisen through habit, fiat or be of unknown origin. Instances of referential status may end either though a formal process, or may simply fade out, be eliminated by fiat or for unknown reasons."""^^xsd:string ;
    rdfs:subClassOf <https://ontology.swissartresearch.net/aaao/ZE1_Institutional_Fact> ;
    skos:notation "ZE12"^^xsd:string .

<https://ontology.swissartresearch.net/aaao/ZE13_Speech_Act> a rdfs:Class ;
    rdfs:label "Speech Act"@en ;
    dcterms:source "AAAo_v2.0.rdf" ;
    rdfs:comment """An instance of speech actcomprises an intentional activity engaged in by a set of actors to create a new institutional fact - or to nullify an existing one - that holds for a given community. In this sense, a speech act is transformative symbolic act. Speech acts are carried out by intentional actors through invoking a social rule and performing a prescribed set of actions often including the locution of set formulae of phrases by certain actors, fulfilling certain roles. Correct execution of the speech act as specified by the rule results in the existence of new institutional facts or their negation. The substance of speech act is ritual action performed by a group.
An instance of speech act begins when the intended ritual proceeding as specified by the rule invoked is initiated. The instance of speech act ends when the required set of actions specified for the act in question are executed or it is abandoned."""^^xsd:string ;
    rdfs:subClassOf <https://ontology.swissartresearch.net/aaao/ZE52_Transformative_Symbolic_Act> ;
    skos:notation "ZE13"^^xsd:string .

<https://ontology.swissartresearch.net/aaao/ZE14_Similarity_Status> a rdfs:Class ;
    rdfs:label "Similarity Status"@en ;
    dcterms:source "AAAo_v2.0.rdf" ;
    rdfs:comment """An instance of similarity status is the collective ascription of a similarity relationship between any two objects by a community. The substance of the similarity status is the communal recognition of the ascribed similarity relation between the two entities in question.
Instances of similarity status are recognizable through evidence of community members adopting the intentional stance and behaviour indicated by the kind of similarity believed to hold between the two referenced entities, as observable from direct witnesses, through the reports of competent observers or through evidence of a declarative act initiating this status.
Instances of similarity status may come to be through a formal process such as a declarative act (e.g., scholarship) or may have arisen through habit, fiat or be of unknown origin. Instances of similarity status may end either though a formal process (e.g., disproof or refutation), or may simply fade out, be eliminated by fiat or for unknown reasons."""^^xsd:string ;
    rdfs:subClassOf <https://ontology.swissartresearch.net/aaao/ZE1_Institutional_Fact> ;
    skos:notation "ZE14"^^xsd:string .

<https://ontology.swissartresearch.net/aaao/ZE15_Set_Status> a rdfs:Class ;
    rdfs:label "Set Status"@en ;
    dcterms:source "AAAo_v2.0.rdf" ;
    rdfs:comment """An instance of set status is the collective ascription of some relationship of belonging between some entity and a notional set by a community. The substance of the set status is the communal recognition of the ascribed belonging between the subject entity and the set in question.
Instances of set status are recognizable through evidence of community members adopting the intentional stance and behaviour indicated as proper to this set-belonging relation, as observable from direct witnesses, through the reports of competent observers or through evidence of a declarative act initiating this status.
Instances of set status may come to be through a formal process or may have arisen through habit, fiat or be of unknown origin. Instances of membership status may end either though a formal process, or may simply fade out, be eliminated by fiat or for unknown reasons."""^^xsd:string ;
    rdfs:subClassOf <https://ontology.swissartresearch.net/aaao/ZE1_Institutional_Fact> ;
    skos:notation "ZE15"^^xsd:string .

<https://ontology.swissartresearch.net/aaao/ZE17_Digital_Reading> a rdfs:Class ;
    rdfs:label "Digital Reading"@en ;
    dcterms:source "AAAo_v2.0.rdf" ;
    rdfs:comment """An instance of digital reading is a digital processing event guided by a set of instructions or parameters which in turn returns a digital output. The digital output will consist in a set of propositions related to the 'read' input which might include things like classifications, identifications, transformations, comparisons and so on. In the context of semantic data processes, such output might consist in semantically encoded knowledge graph statements, the collection of which may be referred to as an I4 Propositional Set, which can be regarded as the 'conclusion' of the digital reading. As such, Digital reading may be regarded as a computational process guided by a parametrized hypothesis resulting in a new propositional dataset for scientific consideration. The propositional information generated by the digital reading process should be considered as provisional knowledge posited under a hypothesis. Typically propositions generated by the digital reading may become the subject of further scholarly research.
Instances of this class come to be when a process is initiated to generate new information and finish upon completion of that process or if the process is interrupted and fails to complete."""^^xsd:string ;
    rdfs:subClassOf <http://www.cidoc-crm.org/extensions/crmtex/TX5_Text_Recognition>,
        <http://www.ics.forth.gr/isl/CRMdig/D7_Digital_Machine_Event>,
        <https://ontology.swissartresearch.net/aaao/ZE13_Speech_Act> ;
    skos:notation "ZE17"^^xsd:string .

<https://ontology.swissartresearch.net/aaao/ZE18_Critical_Reading> a rdfs:Class ;
    rdfs:label "Critical Reading"@en ;
    dcterms:source "AAAo_v2.0.rdf" ;
    rdfs:comment "An instance of critical reading is a process of analysis undertaken by a scholar to derive analytical facts from a specific information resource. Critical reading engages the background knowledge of the scholar and their interpretive horizon in order to support them in actively reading the research object to derive factual, historically contextualized/contextualizing information regarding the propositional content in question and the world(s) it pertains too. This process can take as input previous scholarly documentation or outputs of digital reading events. Critical reading may result in a series of constructed arguments, serving as a foundation for the documentation and analysis of an argument regarding the text and its referents. Critical reading might also result in the observation, documentation or assertion of a social fact, such as the assertion of an appellative or classificatory status. In the latter case, the instance of ZE18 Critical Reading serves as provenance for the existence of the fact in the network."^^xsd:string ;
    rdfs:subClassOf <https://ontology.swissartresearch.net/aaao/ZE13_Speech_Act> ;
    skos:notation "ZE18"^^xsd:string .

<https://ontology.swissartresearch.net/aaao/ZE19_Naming> a rdfs:Class ;
    rdfs:label "Naming"@en ;
    dcterms:source "AAAo_v2.0.rdf" ;
    rdfs:comment """Instances of naming are comprised of an act which officially confers a name to some object under a specific procedure. The substance of naming is an intentional, social act.
Instances of ZE19 Naming come about when the specific social procedure required is intentionally and successfully enacted according to the prevalent rules. They end with the successful termination of the act or because of its premature termination.
The result of the instance of naming is the coming to be of a collective acceptance of a name for some object in some mode for some time. The details of this institutional fact are documented in the resultant instance of ZE2 Appellative Status."""^^xsd:string ;
    rdfs:subClassOf <http://www.cidoc-crm.org/cidoc-crm/E13_Attribute_Assignment>,
        <https://ontology.swissartresearch.net/aaao/ZE13_Speech_Act> ;
    skos:notation "ZE19"^^xsd:string .

<https://ontology.swissartresearch.net/aaao/ZE1_Institutional_Fact> a rdfs:Class ;
    rdfs:label "Institutional Fact"@en ;
    dcterms:source "AAAo_v2.0.rdf" ;
    rdfs:comment """An instance of institutional fact is an ascription of a status function to an object by a community. The institutional fact is a concretization of a collective intentionality of the community in question towards a certain object over a certain period of time.
An instance of institutional fact is recognizable to a competent speaker/member of a symbolic community (native or learner with sufficient competence). It may not be perceived through a single sense impression but through multiple experiences and implicit reasonings (e.g.: embedded participation, behavioural observation, linguistic evidence and interview), yet typically such intermediate observations and inferences are not necessarily recorded or accessible. The historical statement is typically the assertion of the institutional fact, that such and such a fact was the case, and was in force for a given community, at some time. The epistemic veridicality of the stated /reference instance of institutional fact is always open to contestation. The means of contestation involve analyzing the sources which support it.
Instances of institutional fact come into existence based on conventions establishing the conditions under which they come into effect. Typically, an instance of institutional fact will come into existence either because of the performance of its stipulated, initiating speech act (e.g.: state of being married via marriage) or as a result of events fulfilling existing norm prescriptions in the community (e.g.: state of being uncle as result of birth of child of sister). An institutional fact comes to be through the agreed fiat of a community. It typically ceases to exist either because of a stipulated, nullifying speech act (e.g. divorce proceeding), because a community ceases to support the effective rule supporting its declaration (e.g.: ownership of people) or force majeure (e.g.: object ascribed function/status or community perceiving status is eliminated)."""^^xsd:string ;
    rdfs:subClassOf <http://www.cidoc-crm.org/cidoc-crm/E2_Temporal_Entity> ;
    skos:notation "ZE1"^^xsd:string .

<https://ontology.swissartresearch.net/aaao/ZE20_Declarative_Acquisition> a rdfs:Class ;
    rdfs:label "Declarative Acquisition"@en ;
    dcterms:source "AAAo_v2.0.rdf" ;
    rdfs:comment """Instances of this class comprise official acquisition events undertaken following formal procedures within a social grouping leading to formal ownership status over an object by some actor according to the participating parties.The substance of declarative acquisition is an intentional, social act.
Instances of ZE20 Declarative Acquisition come about when the specific social procedure required is intentionally and successfully enacted according to the prevalent rules. They end with the successful termination of the act or because of its premature termination.
A successful act of ZE20 Declarative Acquisition leads to the generation of an instance of ZE8 Ownership Status, the institutional fact that thereafter mediates the social relation to this object until it has been abrogated."""^^xsd:string ;
    rdfs:subClassOf <http://www.cidoc-crm.org/cidoc-crm/E8_Acquisition>,
        <https://ontology.swissartresearch.net/aaao/ZE29_Transfer_of_Property_Right> ;
    skos:notation "ZE20"^^xsd:string .

<https://ontology.swissartresearch.net/aaao/ZE21_Declarative_Transfer_of_Custody> a rdfs:Class ;
    rdfs:label "Declarative Transfer of Custody"@en ;
    dcterms:source "AAAo_v2.0.rdf" ;
    rdfs:comment """Instances of this class comprise official transfer of custody events undertaken following formal procedures within a social grouping leading to formal change in the custody status over an object, ascribing it to some actor's custody, according to the participating parties. The substance of declarative transfer of custody is an intentional, social act.
Instances of ZE21 Declarative Transfer of Custody come about when the specific social procedure required is intentionally and successfully enacted according to the prevalent rules. They end with the successful termination of the act or because of its premature termination.
A successful act of declarative transfer of custody leads to the generation of an instance of ZE7 Custodial Status, the institutional fact that thereafter mediates the social relation to this object until it has been abrogated."""^^xsd:string ;
    rdfs:subClassOf <http://www.cidoc-crm.org/cidoc-crm/E10_Transfer_of_Custody>,
        <https://ontology.swissartresearch.net/aaao/ZE29_Transfer_of_Property_Right> ;
    skos:notation "ZE21"^^xsd:string .

<https://ontology.swissartresearch.net/aaao/ZE22_Declarative_Joining> a rdfs:Class ;
    rdfs:label "Declarative Joining"@en ;
    dcterms:source "AAAo_v2.0.rdf" ;
    rdfs:comment """Instances of this class comprise official joining events undertaken following formal procedures within a social grouping leading to formal change in the membership status of an actor relative to a group for the participating parties. The substance of declarative joining is an intentional, social act.
Instances of ZE22 Declarative Joining come about when the specific social procedure required is intentionally and successfully enacted according to the prevalent rules. They end with the successful termination of the act or because of its premature termination.
A successful act of ZE22 Declarative Joining leads to the generation of an instance of ZE11 Membership Status, the institutional fact that thereafter mediates the social relationbetween the group and actor in question until it has been abrogated."""^^xsd:string ;
    rdfs:subClassOf <http://www.cidoc-crm.org/cidoc-crm/E85_Joining>,
        <https://ontology.swissartresearch.net/aaao/ZE13_Speech_Act> ;
    skos:notation "ZE22"^^xsd:string .

<https://ontology.swissartresearch.net/aaao/ZE23_Declarative_Leaving> a rdfs:Class ;
    rdfs:label "Declarative Leaving"@en ;
    dcterms:source "AAAo_v2.0.rdf" ;
    rdfs:comment """Instances of this class comprise official leaving events undertaken following formal procedures within a social grouping leading to formal change in the membership status of an actor relative to a group for the participating parties. The substance of declarative leaving is an intentional, social act.
Instances of ZE23 Declarative Leaving come about when the specific social procedure required is intentionally and successfully enacted according to the prevalent rules. They end with the successful termination of the act or because of its premature termination.
A successful act of ZE23 Declarative Leaving leads to the termination of an instance of ZE11 Membership Status, the institutional fact that thereafter no longer mediates the social relation between the group and actor in question."""^^xsd:string ;
    rdfs:subClassOf <http://www.cidoc-crm.org/cidoc-crm/E86_Leaving>,
        <https://ontology.swissartresearch.net/aaao/ZE13_Speech_Act> ;
    skos:notation "ZE23"^^xsd:string .

<https://ontology.swissartresearch.net/aaao/ZE24_Notional_Set> a rdfs:Class ;
    rdfs:label "Notional Set"@en ;
    dcterms:source "AAAo_v2.0.rdf" ;
    rdfs:comment """Instances of this class comprise notional sets of objects which have been grouped together for one reason or another. The substance of notional set is ideational.
A notional set comes to be when it is asserted or otherwise declared. It gains or loses members according to the particular rules guiding its maintenance. Typically instances of ZE24 Notional Set serve a functional purpose such as the grouping of some objects according to an ad hoc, context particular, or a context categorical criterion.
See also Linked.Art:Set"""^^xsd:string ;
    rdfs:subClassOf <http://www.cidoc-crm.org/cidoc-crm/E28_Conceptual_Object> ;
    skos:notation "ZE24"^^xsd:string .

<https://ontology.swissartresearch.net/aaao/ZE25_Dating_Status> a rdfs:Class ;
    rdfs:label "Dating Status"@en ;
    dcterms:source "AAAo_v2.0.rdf" ;
    rdfs:comment """An instance of dating status is the collective ascription of a relative dating to an event (such as the production or the use of an object or the despotional moment of an archaeological context) by its association to an established and named historical or archaeological period or event. The substance of the dating status is the communal recognition of the ascribed chronology as holding true for the dated event and potential, relative object(s) it involves.
Instances of dating status are typically recorded in the archaeological / archival record.
Instances of dating status are most typically initiated by a formal process such as a scholarly dating attribution (ZE26 Dating Declaration). Instances of dating status may be terminated either through a formal process (official disproof) or be replaced by another dating declaration holding an updated belief and supported by further evidence."""^^xsd:string ;
    rdfs:subClassOf <https://ontology.swissartresearch.net/aaao/ZE1_Institutional_Fact> ;
    skos:notation "ZE25"^^xsd:string .

<https://ontology.swissartresearch.net/aaao/ZE26_Dating_Declaration> a rdfs:Class ;
    rdfs:label "Dating Declaration"@en ;
    dcterms:source "AAAo_v2.0.rdf" ;
    rdfs:comment """Instances of dating declaration are scholarly acts which officially assign a historical or archaeological period to an event of interest (paradigmatic cases being the production or the time of use or termination of existence of some object or physical thing) of which, typically, a material artefact is the material remain.
The result of the instance of dating declaration is the coming to be of a collective acceptance of the dating status for some object or some physical thing at some time by some group of people. This status may come to be contested or replaced by some new status, either through reasoned argumentation, assertion or even forgetting.
The details of this institutional fact are documented in the resultant instance of ZE25 Dating Status."""^^xsd:string ;
    rdfs:subClassOf <http://www.cidoc-crm.org/extensions/crminf/I1_Argumentation>,
        <https://ontology.swissartresearch.net/aaao/ZE13_Speech_Act> ;
    skos:notation "ZE26"^^xsd:string .

<https://ontology.swissartresearch.net/aaao/ZE27_Declaration_of_Obligation> a rdfs:Class ;
    rdfs:label "Declaration of Obligation"@en ;
    dcterms:source "AAAo_v2.0.rdf" ;
    rdfs:comment """Instances of declaration of obligation are characterized by formal acts of recognition of a state of obligation between one party and another party for a certain measurable amount of goods.
Instances of this class comprise official acts undertaken following formal procedures within a social grouping leading to formal recognition of an obligation status between two actors. The substance of declaration of obligation is an intentional, social act.
Instances of ZE27 Declaration of Obligation come about when the specific social procedure required is intentionally and successfully enacted according to the prevalent rules. They end with the successful termination of the act or because of its premature termination.
A successful act of ZE27 Declaration of Obligation leads to the generation of an instance of ZE28 Obligation Status, the institutional fact that thereafter holds between two actors until it has been abrogated."""^^xsd:string ;
    rdfs:subClassOf <https://ontology.swissartresearch.net/aaao/ZE46_Promisory_Agreement> ;
    skos:notation "ZE27"^^xsd:string .

<https://ontology.swissartresearch.net/aaao/ZE28_Obligation_Status> a rdfs:Class ;
    rdfs:label "Obligation Status"@en ;
    dcterms:source "AAAo_v2.0.rdf" ;
    rdfs:comment """An instance of obligation status demarks a socially recognized state of obligation holding between two parties, wherein the first party is recognized to have the requirement to fulfil a debt to the second party for a certain measurable amount. The substance of the obligation status is the commitment from one party to another for compensation in a socially recognized form.
Instances of obligation status are recognizable through evidence of community members adopting the intentional stance of so recognizing this status, as observable from direct witnesses, through the reports of competent observers or through evidence of a declarative act [e.g.: ZE27 Declaration of Obligation) initiating this status.
Instances of obligation status may come to be through a formal process such as an act of declaring obligation [ZE27 Declaration of Obligation), or may have arisen through habit, fiat or be of unknown origin. Instances of obligation may end either though a formal process, such as an act of renunciation, or may simply fade out of use, be eliminated by fiat or be of unknown reason."""^^xsd:string ;
    rdfs:subClassOf <https://ontology.swissartresearch.net/aaao/ZE45_Promisory_Status> ;
    skos:notation "ZE28"^^xsd:string .

<https://ontology.swissartresearch.net/aaao/ZE29_Transfer_of_Property_Right> a rdfs:Class ;
    rdfs:label "Transfer of Property Right"@en ;
    dcterms:source "AAAo_v2.0.rdf" ;
    rdfs:comment """Instances of declaration of transfer of property right consist of events in which an official transfer of a property right is undertaken between two individuals with the result that a new right is assigned to the receiver and the right of the giver may be forfeited.
Instances of this class consist of events in which an official transfer of a property right is undertaken between two individuals with the result that a new right is assigned to the receiver and the right of the giver may be forfeited.The substance of transfer of property right is an intentional, social act.
Instances of ZE29 Transfer of Property Right come about when the specific social procedure required is intentionally and successfully enacted according to the prevalent rules. They end with the successful termination of the act or because of its premature termination.
A successful act of ZE29 Transfer of Property Right leads to the generation of an instance of ZE30 Property Right Status, the institutional fact that thereafter mediates the social relation to this object until it has been abrogated."""^^xsd:string ;
    rdfs:subClassOf <https://ontology.swissartresearch.net/aaao/ZE13_Speech_Act> ;
    skos:notation "ZE29"^^xsd:string .

<https://ontology.swissartresearch.net/aaao/ZE2_Appellative_Status> a rdfs:Class ;
    rdfs:label "Appellative Status"@en ;
    dcterms:source "AAAo_v2.0.rdf" ;
    rdfs:comment """An instance of appellative status is the collective ascription of an appellation to an object by a community. The substance of the appellative status is the communal commitment to the naming of the object in question with a designated appellation, under a designated modality.
Instances of appellative status are recognizable through evidence of community members adopting the intentional stance of so-naming towards the object in question, as observable from direct witnesses, through the reports of competent observers or through evidence of a declarative act [e.g.: ZE19 Naming] initiating this status. Examples of such evidence include, several individuals so naming a thing, a witness declaring that a thing is ‘so named, by us’ or through documents reporting this fact.
Instances of appellative status may come to be through a formal process such as a declarative act of naming, or may have arisen through habit, fiat or be of unknown origin. Instances of appellative status may end either through a formal process, such as a new declarative act of naming, the formal stripping of a name, or may simply fade out of use, be eliminated by fiat or be of unknown reason."""^^xsd:string ;
    rdfs:subClassOf <https://ontology.swissartresearch.net/aaao/ZE1_Institutional_Fact> ;
    skos:notation "ZE2"^^xsd:string .

<https://ontology.swissartresearch.net/aaao/ZE30_Property_Right_Status> a rdfs:Class ;
    rdfs:label "Property Right Status"@en ;
    dcterms:source "AAAo_v2.0.rdf" ;
    rdfs:comment """Instances of property right status indicate the holding of a right over a legal object by some actor for some time.
An instance of property right status is the collective ascription of a relationship of legal right of some actor over a legal object by a community. The substance of the property right status is the communal commitment to the recognition of the right of use, right to earn income from, and right of disposal (of some sort) over the designated legal object by the actor in question.
Instances of property right status are recognizable through evidence of community members adopting the intentional stance of so recognizing this status, as observable from direct witnesses, through the reports of competent observers or through evidence of a declarative act [e.g.: ZE29 Transfer of Property Right) initiating this status.
Instances of property right status may come to be through a formal process such as a declarative act of taking possession of right [ZE29 Transfer of Property Right), or may have arisen through habit, fiat or be of unknown origin. Instances of property right status may end either though a formal process, such as a new transfer or right, or may simply fade out of use, be eliminated by fiat or be of unknown reason."""^^xsd:string ;
    rdfs:subClassOf <https://ontology.swissartresearch.net/aaao/ZE1_Institutional_Fact> ;
    skos:notation "ZE30"^^xsd:string .

<https://ontology.swissartresearch.net/aaao/ZE33_Declarative_Formation> a rdfs:Class ;
    rdfs:label "Declarative Formation"@en ;
    dcterms:source "AAAo_v2.0.rdf" ;
    rdfs:comment """Instances of this class comprise official group formation events undertaken following formal procedures within a social grouping leading to the formal existence of the group relative to the participating parties, whether subgroups or individual persons. The substance of declarative group formation is an intentional, social act.
Instances of ZE33 Declarative Formation come about when the specific social procedure required is intentionally and successfully enacted according to the prevalent rules. They end with the successful termination of the act or because of its premature termination.
A successful act of ZE33 Declarative Formation leads to the generation of an instance of ZE11 Membership Status, the institutional fact that thereafter mediates the social relationbetween the group and actor in question until it has been abrogated."""^^xsd:string ;
    rdfs:subClassOf <http://www.cidoc-crm.org/cidoc-crm/E66_Formation>,
        <https://ontology.swissartresearch.net/aaao/ZE13_Speech_Act> ;
    skos:notation "ZE33"^^xsd:string .

<https://ontology.swissartresearch.net/aaao/ZE34_Declarative_Dissolution> a rdfs:Class ;
    rdfs:label "Declarative Dissolution"@en ;
    dcterms:source "AAAo_v2.0.rdf" ;
    rdfs:comment """Instances of this class comprise official group dissolution events undertaken following formal procedures within a social grouping leading to the formal termination of the existence of the group relative to the participating parties, whether subgroups or individual persons. The substance of declarative group dissolution is an intentional, social act.
Instances of ZE34 Declarative Dissolution come about when the specific social procedure required is intentionally and successfully enacted according to the prevalent rules. They end with the successful completion of the act or because of its premature termination.
A successful act of ZE34 Declarative Dissolution leads to the termination of an instance of ZE11 Membership Status for each of the groups members, whether individuals or subgroups, until such a time as the group is reformed."""^^xsd:string ;
    rdfs:subClassOf <http://www.cidoc-crm.org/cidoc-crm/E68_Dissolution>,
        <https://ontology.swissartresearch.net/aaao/ZE13_Speech_Act> ;
    skos:notation "ZE34"^^xsd:string .

<https://ontology.swissartresearch.net/aaao/ZE35_Locative_Status> a rdfs:Class ;
    rdfs:label "Locative Status"@en ;
    dcterms:source "AAAo_v2.0.rdf" ;
    rdfs:comment """An instance of locative status is the collective ascription to an entity of a formal association to a geographic place. The substance of the locative status is the communal attribution of a defined association type between the designated entity and place. As opposed to connections created between entities and places through their passage through space and time, e.g.: the place of birth being a property of the birth event of an individual, locative statuses are created de jure rather than de facto and create a socially recognized connection between an entity and a location regardless the real or known spatiotemporal history of that object. For example, documentation may point to ambiguous evidence linking an object and a place such as the 'origin' of a person or the 'provenance' location of a physical object. In these cases, when we do not know the actual physical history of the object in question, but we do have a de jure attribution from which some knowledge may be derived, we can document and follow an instance of Locative Status for an object in relation to a geographic location.
Instances of locative status are recognizable through evidence of community members adopting the intentional stance of so recognizing this status, as observable from direct witnesses, through the reports of competent observers or through evidence of a declarative act initiating this status.
Instances of locative status may come to be through a formal process such as a declarative act of such definition, or may have arisen through habit, fiat or be of unknown origin. Instances of locative status may end either though a formal process, such as a new declarative act, or may simply fade out of use, be eliminated by fiat or be of unknown reason."""^^xsd:string ;
    rdfs:subClassOf <https://ontology.swissartresearch.net/aaao/ZE1_Institutional_Fact> ;
    skos:notation "ZE35"^^xsd:string .

<https://ontology.swissartresearch.net/aaao/ZE36_Persons> a rdfs:Class ;
    rdfs:label "Persons"@en ;
    dcterms:source "AAAo_v2.0.rdf" ;
    rdfs:comment "Instances of this class comprise sentient beings endowed, to more or less extent, with intentionality, either as individuals or collectives. Instances of Persons are first causes and ends in themselves in a philosophical sense. The substance of Persons is personhood in this sense of being endowed with intentionality and the requisite respect qua sentient being."^^xsd:string ;
    rdfs:subClassOf <http://www.cidoc-crm.org/cidoc-crm/E77_Persistent_Item> ;
    skos:notation "ZE36"^^xsd:string .

<https://ontology.swissartresearch.net/aaao/ZE37_Population> a rdfs:Class ;
    rdfs:label "Population"@en ;
    dcterms:source "AAAo_v2.0.rdf" ;
    rdfs:comment """This class comprises a defined set of persons who are considered to together form a coherent, identifiable unit according to certain characteristics such as citizenry, religious affiliation or other uniting characteristics or properties. Instances of population may be emically or etically defined. The substance of population is a collectivity of people[.]
Instances of population existence natural population come into and go out of existence through natural and social processes the particular details of which are often difficult to know or the subject of research and investigation. If a population is declaratively defined such as 'male voters between the age of 20 and 30 in Alabama in 2024 election cycle', then the existence condition is relative to the de jure declaration of their composition. An instance of population can be identified to be in existence when a suitable collective of individuals matching to its description can be identified to live and conform to those characteristics"""^^xsd:string ;
    rdfs:subClassOf <http://www.cidoc-crm.org/cidoc-crm/E18_Physical_Thing>,
        <https://ontology.swissartresearch.net/aaao/ZE36_Persons> ;
    skos:notation "ZE37"^^xsd:string .

<https://ontology.swissartresearch.net/aaao/ZE38_Population_Existence> a rdfs:Class ;
    rdfs:label "Population Existence"@en ;
    dcterms:source "AAAo_v2.0.rdf" ;
    rdfs:comment """This class comprises the proper existence event of a population. Population existence consists in the temporal continuance of a specified population over a time and space.
Instances of population existence come into existence with the appearance or expression of the population and cease to exist with its dissolution. In the case of a de jure population, the duration of the population existence is a matter of declaration."""^^xsd:string ;
    rdfs:subClassOf <http://www.cidoc-crm.org/cidoc-crm/E5_Event> ;
    skos:notation "ZE38"^^xsd:string .

<https://ontology.swissartresearch.net/aaao/ZE39_Polity> a rdfs:Class ;
    rdfs:label "Polity"@en ;
    dcterms:source "AAAo_v2.0.rdf" ;
    rdfs:comment """This class comprises a defined set of persons who are joined together by virtue of belonging to a shared civil society, collectively subject to the rights and responsibilities that that civil society confers. As an otherwise unorganized group, polities lack the agency required to undertake collective actions. They may however be subject to the actions of others, with the authority to organize the civil society to which the individuals belong. The substance of polity is a collectivity of people defined by their belonging to a shared civil society.
Instances of polity come into and go out of existence through natural and social processes, these may be formal (in the case, e.g., of a constitutional formation) or informal, where the particular details of the polity's formation are difficult to know or the subject of research and investigation. An instance of polity can be identified when a suitable collective of individuals matching to its description can be identified to live within the bounds of a recognized civil society."""^^xsd:string ;
    rdfs:subClassOf <https://ontology.swissartresearch.net/aaao/ZE37_Population> ;
    skos:notation "ZE39"^^xsd:string .

<https://ontology.swissartresearch.net/aaao/ZE3_Contact_Point_Status> a rdfs:Class ;
    rdfs:label "Contact Point Status"@en ;
    dcterms:source "AAAo_v2.0.rdf" ;
    rdfs:comment """An instance of contact status is the collective ascription of a contact point to an actor by a community. The substance of the contact status is the communal commitment to the addressing of messages to the actor in question according to a designated contact point appellation, using the implied message exchanging method.
Instances of contact status are recognizable through evidence of community members adopting the intentional stance of so-addressing messages to the actor in question, as observable from direct witnesses, through the reports of competent observers or through evidence of a declarative act [e.g.: E15 Identifier Assignment] initiating this status. Examples of such evidence include, several individuals so addressing messages to an actor via this contact point appellation, a witness declaring that an actor can so be reached, or through documents reporting this fact.
Instances of contact status may come to be through a formal process such as a declarative act of identifier assignment, or may have arisen through habit, fiat or be of unknown origin. Instances of contact status may end either though a formal process, such as a new declarative act of identifier assignment, through formal assignment, or may simply fade out of use, be eliminated by fiat or for unknown reasons."""^^xsd:string ;
    rdfs:subClassOf <https://ontology.swissartresearch.net/aaao/ZE2_Appellative_Status> ;
    skos:notation "ZE3"^^xsd:string .

<https://ontology.swissartresearch.net/aaao/ZE43_Physical_Locative_Status> a rdfs:Class ;
    rdfs:label "Physical Locative Status"@en ;
    dcterms:source "AAAo_v2.0.rdf" ;
    rdfs:comment """An instance of physical locative status is the collective ascription to a physical object of a formal association to a geographic place. The substance of the locative status is the communal attribution of a defined association type between the designated object and place.
As opposed to connections created between physical objects and places through their passage through space and time, e.g.: the place of production being a property of the production event of an individual, physical locative statuses are created de jure rather than de facto and create a socially recognized connection between an object and a location regardless the real or known spatiotemporal history of that object. For example, documentation may point to ambiguous evidence linking an object and a place such as the 'provenance' location of a physical object. In these cases, when we do not know the actual physical history of the object in question, but we do have a de jure attribution from which some knowledge may be derived, we can document and follow an instance of Physical Locative Status for an object in relation to a geographic location.
Instances of physical locative status are recognizable through evidence of community members adopting the intentional stance of so recognizing this status, as observable from direct witnesses, through the reports of competent observers or through evidence of a declarative act initiating this status.
Instances of locative status may come to be through a formal process such as a declarative act of such definition, or may have arisen through habit, fiat or be of unknown origin. Instances of locative status may end either though a formal process, such as a new declarative act, or may simply fade out of use, be eliminated by fiat or be of unknown reason."""^^xsd:string ;
    rdfs:subClassOf <https://ontology.swissartresearch.net/aaao/ZE35_Locative_Status> ;
    skos:notation "ZE43"^^xsd:string .

<https://ontology.swissartresearch.net/aaao/ZE44_Topographical_Status> a rdfs:Class ;
    rdfs:label "Topographical Status"@en ;
    dcterms:source "AAAo_v2.0.rdf" ;
    rdfs:comment """An instance of topographical status is the collective ascription to a geographical place of a formal spatial association to another geographic place. The substance of the topographical status is the communal attribution of a defined spatial association between two geographic places.
As opposed to connections created between geographic places as determine through a pure mathematic relation, e.g.: the falling within of a larger geometry by a smaller geometry, topographical statuses depend also on a de jure, socially recognized connection between two topographies. For example, when there are distinct political positions on the boundaries of a country, whether a geographic area 'falls within' another geographic area depends not only on the geometric calculation, but on the definition of extents of the geographic spaces in the first place.
IInstances of topographical status are recognizable through evidence of community members adopting the intentional stance of so recognizing this status, as observable from direct witnesses, through the reports of competent observers or through evidence of a declarative act initiating this status.
Instances of topographical status may come to be through a formal process such as a declarative act of such definition, or may have arisen through habit, fiat or be of unknown origin. Instances of locative status may end either though a formal process, such as a new declarative act, or may simply fade out of use, be eliminated by fiat or be of unknown reason."""^^xsd:string ;
    rdfs:subClassOf <https://ontology.swissartresearch.net/aaao/ZE35_Locative_Status> ;
    skos:notation "ZE44"^^xsd:string .

<https://ontology.swissartresearch.net/aaao/ZE45_Promisory_Status> a rdfs:Class ;
    rdfs:label "Promissory Status"@en ;
    dcterms:source "AAAo_v2.0.rdf" ;
    rdfs:comment """An instance of promissory status is the collective ascription of a promissory obligation between two parties. The substance of the promissory status is the communal recognition of the promise in question, which may nonetheless only bind two individuals directly. The substance of promissory status includes the ascription of an outcome which may detail guidelines and constraints that downstream activities on the part of promissory parties should comply with. Put otherwise, the promise promises a futural event on the part of the promisor to the promisee. The specified promissory constraints of this event can be instantiated on the level of kinds of processes, items or qualities and quantities involved in the action.
Instances of promissory status are recognizable through evidence of community members adopting an intentional stance towards the promise that exists between the two parties, as observable from direct witnesses, through the reports of competent observers or through documentary evidence of a declarative act (e.g.: ZE46 Promissory Agreement Event) initiating this status.
Instances of promissory status may come to be through a formal process such as a declarative promisory agreement, or may have arisen through habit, fiat or be of unknown origin. Instances of promissory status may end either through a formal process, such as a new declarative promissory agreement, the formal stripping of an existing promissory status, or may simply fade out of use, be eliminated by fiat or be of unknown reason."""^^xsd:string ;
    rdfs:subClassOf <https://ontology.swissartresearch.net/aaao/ZE1_Institutional_Fact> ;
    skos:notation "ZE45"^^xsd:string .

<https://ontology.swissartresearch.net/aaao/ZE46_Promisory_Agreement> a rdfs:Class ;
    rdfs:label "Promissory Agreement Event"@en ;
    dcterms:source "AAAo_v2.0.rdf" ;
    rdfs:comment """Instances of promissory agreement event are characterized by formal acts of recognition of a promise between one party and another party for a certain outcome.
Instances of this class comprise explicit acts undertaken following given procedures within a social grouping leading to explicit recognition of a promissory status between two actors. The substance of promissory agreement is an intentional, social act.
Instances of ZE46 Promissory Agreement come about when the specific social procedure required is intentionally and successfully enacted according to the prevalent rules. They end with the successful termination of the act or because of its premature termination.
A successful act of ZE46 Promissory Agreement leads to the generation of an instance of ZE45 Promissory Status, the institutional fact that thereafter holds between two actors until it has been abrogated."""^^xsd:string ;
    rdfs:subClassOf <http://iflastandards.info/ns/lrm/lrmoo/F28_Expression_Creation>,
        <https://ontology.swissartresearch.net/aaao/ZE13_Speech_Act> ;
    skos:notation "ZE46"^^xsd:string .

<https://ontology.swissartresearch.net/aaao/ZE49_Text_Sequence_Status> a rdfs:Class ;
    rdfs:label "Text Sequence Status"@en ;
    dcterms:source "AAAo_v2.0.rdf" ;
    rdfs:comment """An instance of text sequence status is a collective ascription to a written text sequence of a formal association to another written text sequence, in relation to which it is conceived as occupying a determinate place (i.e., the order in which they are to be read, wherein one text sequence follows another). The substance of the text sequence status is the communal attribution of a recognizable sequencing order between the designated text fields
As opposed to the connections created between a text field and the physical substrate upon which it is written, text sequence statuses are created de jure rather than de facto and create socially recognized connections between them. For example, an editorial annotation may indicate that a paragraph from a 'lower' position on the writing surface (such as a page) is to be inserted between two paragraphs at a 'higher' position (or on another page altogether). In such cases, the sequence in which the paragraphs are to be read does not coincide with the physical position of the text field in question, or the exact ordering of the paragraphs may be the subject of research or scholarly debate, but we do have de jure attribution from which some knowledge may be derived and documented with an instance of Text Sequence Status.
Instances of text sequence status are recognizable through evidence of community members adopting the intentional stance of so recognizing this status, as observable from direct witnesses, through the reports of competent observers or through evidence of a declarative act initiating this status.
Instances of text sequence status may come to be through a formal process such as a declarative act of such definition, or may have arisen through habit, fiat or be of unknown origin. Instances of text sequence status may end either though a formal process, such as a new declarative act, or may simply fade out of use, be eliminated by fiat or be of unknown reason."""^^xsd:string ;
    rdfs:subClassOf <https://ontology.swissartresearch.net/aaao/ZE35_Locative_Status> ;
    skos:notation "ZE49"^^xsd:string .

<https://ontology.swissartresearch.net/aaao/ZE4_Classificatory_Status> a rdfs:Class ;
    rdfs:label "Classificatory Status"@en ;
    dcterms:source "AAAo_v2.0.rdf" ;
    rdfs:comment """An instance of classificatory status is the collective ascription of a type to an object by a community. The substance of the classificatory status is the communal commitment to the classification of the object in question according to the designated type.
Instances of classificatory status are recognizable through evidence of community members adopting the intentional stance of so-classifying the object in question, as observable from direct witnesses, through the reports of competent observers or through evidence of a declarative act [e.g.: E17 Type Assignment] initiating this status.
Instances of classificatory status may come to be through a formal process such as a declarative act of classification [E17 Type Assignment], or may have arisen through habit, fiat or be of unknown origin. Instances of classificatory status may end either though a formal process, such as a new declarative act of classification, be officially declassified, or may simply fade out of use, be eliminated by fiat or be of unknown reason."""^^xsd:string ;
    rdfs:subClassOf <https://ontology.swissartresearch.net/aaao/ZE1_Institutional_Fact> ;
    skos:notation "ZE4"^^xsd:string .

<https://ontology.swissartresearch.net/aaao/ZE50_Authority_Status> a rdfs:Class ;
    rdfs:label "Authority Status"@en ;
    dcterms:source "AAAo_v2.0.rdf" ;
    rdfs:comment """An instance of authority status is the collective ascription of an authority function to an actor by a community, although not necessary by their will. The substance of the authority status is the communal commitment to relating to and acting toward the actor in question according to the designated authority. Instances of authority status may be attributed to individuals or to groups of individuals.
Instances of authority status are recognizable through evidence of community members adopting the intentional stance of so relating or acting toward the actor in question, as observable from direct witnesses, through the reports of competent observers or through evidence of a declarative act [e.g.: E17 Type Assignment] initiating this status.
Instances of social status may come to be through a formal process such as a declarative act of assignment [E17 Type Assignment], or may have arisen through habit, fiat or be of unknown origin. Instances of social status may end either though a formal process, such as a new declarative act of classification, or simply fade out of existence."""^^xsd:string ;
    rdfs:subClassOf <https://ontology.swissartresearch.net/aaao/ZE6_Social_Status> ;
    skos:notation "ZE50"^^xsd:string .

<https://ontology.swissartresearch.net/aaao/ZE52_Transformative_Symbolic_Act> a rdfs:Class ;
    rdfs:label "Transformative Symbolic Act"@en ;
    dcterms:source "AAAo_v2.0.rdf" ;
    rdfs:comment """This class comprises actions of a symbolic nature that are intentionally carried out by instances of E39 Actor and are transformative in consequence on a cultural and/or social level, initiating new instances of institutional fact or terminating the existence of previous institutional facts within that society / culture. An instance of transformative symbolic act is carried out within a social-cultural framework and makes use of the codes and symbols of that framework to communicate a message symbolically. As with any symbolic act, it may affirm or challenge one or more institutional facts recognized within such a system, but the specific difference of a transformative symbolic act is to be the cause of both new institutional facts and of the demise of existing institutional facts.
Instances of transformative symbolic act begin when an E39 Actor intentionally engages in an action invoking an existing code or symbol with the intent to affirm or challenge an institutional fact and end when the invoking act / practice has been completed (or was interrupted). The end of a transformative symbolic act is necessarily accompanied by the change in composition of the overall set of institutional facts of the social cultural framework in which it was undertaken, with one or more instances thereof either coming into or going out of existence."""^^xsd:string ;
    rdfs:subClassOf <https://ontology.swissartresearch.net/aaao/ZE53_Symbolic_Act> ;
    skos:notation "ZE52"^^xsd:string .

<https://ontology.swissartresearch.net/aaao/ZE53_Symbolic_Act> a rdfs:Class ;
    rdfs:label "Symbolic Act"@en ;
    dcterms:source "AAAo_v2.0.rdf" ;
    rdfs:comment """This class comprises actions of a symbolic nature that are intentionally carried out by instances of E39 Actor. In engaging in a symbolic act, an E39 Actor communicates to other actors. The specific content of a symbolic act's communicative outcome currently lies beyond the scope of this class. Instances of this class can be used to document events of affirmative or negatory relation towards an extant social fact as communicated by an actor. An instance of symbolic act is carried out within a social-cultural framework and makes use of the codes and symbols of that framework to communicate a message symbolically and typically affirms or challenges one or more institutional facts recognized therein.
Instances of symbolic act begin when an E39 Actor intentionally engages in an action invoking an existing code or symbol with the intent to affirm or challenge an institutional fact and end when the invoking act / practice has been completed (or was interrupted)."""^^xsd:string ;
    rdfs:subClassOf <http://www.cidoc-crm.org/cidoc-crm/E7_Activity> ;
    skos:notation "ZE53"^^xsd:string .

<https://ontology.swissartresearch.net/aaao/ZE55_Social_Relation_Status> a rdfs:Class ;
    rdfs:label "Social Relation Status"@en ;
    dcterms:source "AAAo_v2.0.rdf" ;
    rdfs:comment """An instance of social relation status is the collective ascription of a social relationship between one person and another by a community. The substance of the social relation status is the communal recognition of the binary social connection between the two actors in question.
It is important to underline that an instance of social relation consists of is a binary construct that binds two different actors in a certain relation and is to be distinguished from social status. For example, an instance of social relation status could be the social relation status of "professor of" between a teacher and their student. This is a social relation status that is recognized particularly between the two individuals concerned, to be distinguished from a social status, recognized, for example, by the title 'Dr', which may or may not be held at the time in question and has no particular bearing on a relationship with any one individual.
Instances of social relation status are recognizable through evidence of community members adopting the intentional stance and behaviour indicated as proper to this relation, as observable from direct witnesses, through the reports of competent observers or through evidence of a declarative act initiating this status.
Instances of social relation status may come to be simply through birth in a certain community or may require that a formal process such as a right of passage has been undertaken. Instances of social relation status may end either though a formal process such as a renunciation, or may simply fade out of use, be eliminated by fiat or be of unknown reason. or through death."""^^xsd:string ;
    rdfs:subClassOf <https://ontology.swissartresearch.net/aaao/ZE1_Institutional_Fact> ;
    skos:notation "ZE55"^^xsd:string .

<https://ontology.swissartresearch.net/aaao/ZE59_Plan> a rdfs:Class ;
    rdfs:label "Plan"@en ;
    dcterms:source "AAAo_v2.0.rdf" ;
    rdfs:comment """Instances of this class comprise symbolically expressed (whether in writing, orally or in some other recognized symbolic system within a socio-cultural group) projections of futural events and objectivities. An instance of this class is an intellectual object which describes a not yet extant futural world and describes how it is projected to be. A plan foresees what is foreseen to be brought about or to take place given certain eventualities.
The content of a plan expressed as a machine-readable string can be documented in relation to an instance of this object via the property P190 has symbolic content.
The content of a plan can further be expressed in more analytic format by connecting it to a projected instance of Event Trigger Template which describes the particular set of parameters which are envisioned to take place when the plan would be executed.
An instance of plan comes into existence when it is symbolically formulated in some real instantiation and ceases to exist when no further carriers or memory of it remain."""^^xsd:string ;
    rdfs:subClassOf <http://iflastandards.info/ns/lrm/lrmoo/F2_Expression>,
        <http://www.cidoc-crm.org/cidoc-crm/E29_Design_or_Procedure> ;
    skos:notation "ZE59"^^xsd:string .

<https://ontology.swissartresearch.net/aaao/ZE5_Function_Status> a rdfs:Class ;
    rdfs:label "Function Status"@en ;
    dcterms:source "AAAo_v2.0.rdf" ;
    rdfs:comment """An instance of function status is the collective ascription of an operative functionality to an object by a community. The substance of the function status is the communal commitment to relating to and / or using the object in question according to a designated function.
Instances of function status are recognizable through evidence of community members adopting the intentional stance of so using or relating to the object in question, as observable from direct witnesses, through the reports of competent observers or through evidence of a declarative act [e.g.: E17 Type Assignment] initiating this status.
Instances of function status may come to be through a formal process such as a declarative act of classification [E17 type Assignment], or may have arisen through habit, fiat or be of unknown origin. Instances of function status may end either though a formal process, such as a new declarative act of classification, or may simply fade out of use, be eliminated by fiat or by unknown reason."""^^xsd:string ;
    rdfs:subClassOf <https://ontology.swissartresearch.net/aaao/ZE4_Classificatory_Status> ;
    skos:notation "ZE5"^^xsd:string .

<https://ontology.swissartresearch.net/aaao/ZE60_Evental_Locative_Status> a rdfs:Class ;
    rdfs:label "Evental Locative Status"@en ;
    dcterms:source "AAAo_v2.0.rdf" ;
    rdfs:comment """An instance of evental locative status is the collective ascription to an event of a formal association to a geographic place. The substance of the locative status is the communal attribution of a defined association type between the designated event and place. As opposed to connections created between events and places through their passage through space and time, e.g.: the place of production being a property of the production event, evental locative statuses are created de jure rather than de facto and create a socially recognized connection between an event and a location regardless the real spatiotemporal history of that event, known or unknown.
Instances of evental locative status are recognizable through evidence of community members adopting the intentional stance of so recognizing this status, as observable from direct witnesses, through the reports of competent observers or through evidence of a declarative act initiating this status.
Instances of evental locative status may come to be through a formal process such as a declarative act of such definition, or may have arisen through habit, fiat or be of unknown origin. Instances of evental locative status may end either though a formal process, such as a new declarative act, or may simply fade out of use, be eliminated by fiat or be of unknown reason."""^^xsd:string ;
    rdfs:subClassOf <https://ontology.swissartresearch.net/aaao/ZE35_Locative_Status> ;
    skos:notation "ZE60"^^xsd:string .

<https://ontology.swissartresearch.net/aaao/ZE6_Social_Status> a rdfs:Class ;
    rdfs:label "Social Status"@en ;
    dcterms:source "AAAo_v2.0.rdf" ;
    rdfs:comment """An instance of social status is the collective ascription of a social function to an actor by a community. The substance of the social status is the communal commitment to relating to and acting toward the actor in question according to the designated status.
It is important to underline that an instance of social status relates to a classification of an individual as holding a particular role or function in the community in general. This is to be distinguished from a social relation status, a binary construct that binds two different actors in a certain relation. For example, an instance of social status could be the social status of "Coach". This social status, if ascribed to an individual, holds for that person within a general social context and for a particular group and/or population. This is distinct from a social relation status that is recognized particularly between the two individuals concerned, such as "coach of", that would particularly hold between the individual who is coach and the individual who is a team member.
Instances of social status are recognizable through evidence of community members adopting the intentional stance of so relating or acting toward the actor in question, as observable from direct witnesses, through the reports of competent observers or through evidence of a declarative act [e.g.: E17 Type Assignment] initiating this status.
Instances of social status may be attributed to individuals or to groups of individuals. Instances of social status may also be held in relation to a third party, to whom the subject of the social status bears certain rights and/or responsibilities.
Instances of social status may come to be through a formal process such as a declarative act of assignment [E17 Type Assignment], or may have arisen through habit, fiat or be of unknown origin. Instances of social status may end either though a formal process, such as a new declarative act of classification, or may simply fade out of use, be eliminated by fiat or by unknown reason."""^^xsd:string ;
    rdfs:subClassOf <https://ontology.swissartresearch.net/aaao/ZE4_Classificatory_Status> ;
    skos:notation "ZE6"^^xsd:string .

<https://ontology.swissartresearch.net/aaao/ZE7_Custodial_Status> a rdfs:Class ;
    rdfs:label "Custodial Status"@en ;
    dcterms:source "AAAo_v2.0.rdf" ;
    rdfs:comment """An instance of custodial status is the collective ascription of a relationship of custodianship of some actor over an object by a community. The substance of the custodial status is the communal commitment to the recognition of the relationship of custodianship over the designated object by the actor in question.
Instances of custodial status are recognizable through evidence of community members adopting the intentional stance of so recognizing this status, as observable from direct witnesses, through the reports of competent observers or through evidence of a declarative act [e.g.: ZE21 Declarative Transfer of Custody] initiating this status.
Instances of classificatory status may come to be through a formal process such as a declarative transfer of custody, or may have arisen through habit, fiat or be of unknown origin. Instances of custodial status may end either though a formal process, such as a new declarative act of legal transfer of custody, or may simply fade out of use, be eliminated by fiat or be of unknown reason."""^^xsd:string ;
    rdfs:subClassOf <https://ontology.swissartresearch.net/aaao/ZE30_Property_Right_Status> ;
    skos:notation "ZE7"^^xsd:string .

<https://ontology.swissartresearch.net/aaao/ZE8_Ownership_Status> a rdfs:Class ;
    rdfs:label "Ownership Status"@en ;
    dcterms:source "AAAo_v2.0.rdf" ;
    rdfs:comment """An instance of ownership status is the collective ascription of a relationship of legal possession of some actor over a legal object by a community. The substance of the ownership status is the communal commitment to the recognition of the relationship of possession over the designated legal object by the actor in question.
Instances of ownership status are recognizable through evidence of community members adopting the intentional stance of so recognizing this status, as observable from direct witnesses, through the reports of competent observers or through evidence of a declarative act [e.g.: ZE20 Declarative Acquisition] initiating this status.
Instances of ownership status may come to be through a formal process such as a declarative act of taking ownership, or may have arisen through habit, fiat or be of unknown origin. Instances of ownership status may end either though a formal process, such as a new declarative act of acquisition, or may simply fade out of use, be eliminated by fiat or be of unknown reason."""^^xsd:string ;
    rdfs:subClassOf <https://ontology.swissartresearch.net/aaao/ZE30_Property_Right_Status> ;
    skos:notation "ZE8"^^xsd:string .

<https://ontology.swissartresearch.net/aaao/ZE9_Residential_Status> a rdfs:Class ;
    rdfs:label "Residential Status"@en ;
    dcterms:source "AAAo_v2.0.rdf" ;
    rdfs:comment """An instance of residential status is the collective ascription to an actor of a formal place of residence by a community. The substance of the residential status is the communal commitment to the recognition and use of the designated place with regards to the residence of the designated actor.
Instances of residential status are recognizable through evidence of community members adopting the intentional stance of so-recognizing this status, as observable from direct witnesses, through the reports of competent observers or through evidence of a declarative act initiating this status.
Instances of residence status may come to be through a formal process such as a declarative act of taking up residence, or may have arisen through habit, fiat or be of unknown origin. Instances of residence status may end either though a formal process, such as a new declarative act, or may simply fade out of use, be eliminated by fiat or be of unknown reason."""^^xsd:string ;
    rdfs:subClassOf <https://ontology.swissartresearch.net/aaao/ZE35_Locative_Status> ;
    skos:notation "ZE9"^^xsd:string .

<http://www.cidoc-crm.org/cidoc-crm/> a owl:Ontology ;
    rdfs:comment """CIDOC CRM v7.1.3 implemented in RDFS

This is the implementation approved by the 58th CRM-SIG meeting (March 2024)
as the current RDFS version for the CIDOC CRM namespace.
Note that this is NOT a definition of the CIDOC CRM, but a CIDOC CRM compatible implementation
of an RDF Schema derived from the authoritative release of the CIDOC CRM v7.1.3 on February 2024
https://cidoc-crm.org/Version/version-7.1.3 by an automated algorithm. It is intended for an
assumed majority of uses. Depending on the application, users may create adequate extensions 
compatible with the logical definitions of the CIDOC CRM.

Created by FORTH-ICS February 13, 2024
CC BY 4.0 https://creativecommons.org/licenses/by/4.0/legalcode



Encoding Rules:
1. The RDF spelling rules do not allow blanks. Hence we have replaced them by underscores.
   For instance "E63_Beginning_of_Existence" or "P2i_is_type_of".

2. RDF does not allow to instantiate properties beginning from a range value.
   Therefore, each CRM property is represented as two RDFS properties.
   For instance "P2 has type (is type of)" is represented as:
   "P2_has_type" for the domain to range direction and "P2i_is_type_of" for the range to domain direction.

3. The primitive values "E60 Number", "E61 Time Primitive", "E62 String", "E94 Space Primitive" and 
   "E95 Spacetime Primitive" referred in the Model for formal completeness are interpreted as rdfs:literal.

4. RDF does not support properties of properties, therefore, users may create their own
   subProperties for CRM properties that have a type property such as "P3 has note":
   Instead of P3 has note (P3-1 has type : parts description) declare
   <rdf:Property rdf:about="P3_parts_description">
      <rdfs:domain rdf:resource="E1_CRM_Entity"/>
      <rdfs:range rdf:resource="http://www.w3.org/2000/01/rdf-schema#Literal"/>
      <rdfs:subPropertyOf rdf:resource="P3_has_note"/>
   </rdf:Property>

5. Scope notes are represented as <rdfs:comment> elements.

6. In addition this encoding contains labels in languages different from English, 
   which are taken from translations of previous versions of the CIDOC CRM.    

7. Any other differences in labels, scope notes  and semantic relationships of this encoding 
   to the authoritative definition of the CIDOC CRM v7.1.3 (February 2024) are not intended transfer errors. 
   FORTH appreciates your feed-back on such errors.

8. CRM time extension 1.0 Encoded in RDFS (http://old.cidoc-crm.org/docs/How_to%20implement%20CRM_Time_in%20RDF.pdf)
   Since the Time Primitive of the CRM can not directly be implemented in RDF Triple Stores, we define in this extension
   of 4 properties replacing P81 and P82 adequately using xsd:dateTime. 
   Property P81 is dedicated for modeling the Time-Span's maximum known temporal extent i.e. ongoing_throughout. 
   Property P82 is for modeling the minimum outer bounds of events i.e. at_some_time_within. 
   P81 has its time interval redefined by P81a and P81b. Similarly, we redefine P82 by P82a and P82b.
## RDFS Generation Policies

### Sources

Policies followed for the RDFS implementation of CIDOC v.7.1.3 were created w.r.t.:

- Implementing the CIDOC Conceptual Reference Model in RDF (http://www.cidoc-crm.org/Resources/implementing-the-cidoc-conceptual-reference-model-in-rdf)
- How to implement CRM Time in RDF (http://old.cidoc-crm.org/docs/How_to%20implement%20CRM_Time_in%20RDF.pdf)
- CIDOC-CRM SIG feedback and the general guidelines:
  - Each property is declared twice, forward and backwards, unless no inverse name is defined in parentheses, or domain or range is interpreted as literal
  - All Primitive Values become rdfs:Literal
  - All IsA declarations from/to and between Primitive values are ignored

### Policies

#### **A. CIDOC Classes implementation in RDFS**

The CIDOC-CRM model defines classes, that in Triple Stores are typically implemented as primitive values. These classes are all subclasses of `E59 Primitive Value` and in RDFS they are interpreted as Literal. There are some classes in the CIDOC-CRM model that are both subclasses of `E59 Primitive Value` and E41 Appellation. So far we have followed the decision by CRM-SIG in "Issue 394: Solution for Dualism of E41 Appellation and rdfs:label" in 28-11-2018 wrt the question whether these classes should be implemented as rdfs:Class or still be interpreted as rdfs:Literal.

In this version we have followed the following policy regarding CIDOC Classes implementation in RDFS:

> A1. CIDOC Classes that are subClasses of `E59 Primitive Value` are interpreted as rdfs:Literal regardless of whether they are also subClasses of another Class.

As a result, the following CIDOC classes were not defined in RDFS:

- `E59 Primitive Value`
- `E60 Number`
- `E61 Time Primitive`
- `E62 String`
- `E94 Space Primitive`
- `E95 Spacetime Primitive`

Additionally, the following isA relationships were not defined in RDFS:

- `E59 Primitive Value` `subClassOf` `E1 CRM Entity`
- `E60 Number` `subClassOf` `E59 Primitive Value`
- `E61 Time Primitive` `subClassOf` `E41 Appellation`
- `E61 Time Primitive` `subClassOf` `E59 Primitive Value`
- `E62 String` `subClassOf` `E59 Primitive Value`
- `E94 Space Primitive` `subClassOf` `E41 Appellation`
- `E94 Space Primitive` `subClassOf` `E59 Primitive Value`
- `E95 Spacetime Primitive` `subClassOf` `E41 Appellation`
- `E95 Spacetime Primitive` `subClassOf` `E59 Primitive Value`

#### **B. CIDOC Properties implementation in RDFS**

The decisions in policy A affect the implementation of CIDOC Properties in RDFS. A property cannot define an rdfs:Literal as rdfs:domain, and the backwards direction of a property with an rdfs:Literal as rdfs:range cannot be created for the exact same reason.

Further, the property ranges defined as rdfs:Literal in this implementation do not inherit the properties of the superclasses defined in the CIDOC Model. A separate guideline will describe how to instantiate such properties if at all needed.

Another aspect considered for the implementation of properties in RDFS is whether a distinct inverse property definition should be provided.

In this version we followed the following policies regarding CIDOC Properties implementation in RDFS:

> B1. CIDOC Property backwards/inverse direction is **not** defined, whenever no inverse name for the property has been specified in parentheses in the official CIDOC documentation and property domain is not equal with property range.

As a result, the following properties do not define an inverse direction.

- `E1 CRM Entity. P3 has note: E62 String`
- `E19 Physical Object. P57 has number of parts: E60 Number`
- `E52 Time-Span. P79 beginning is qualified by: E62 String`
- `E52 Time-Span. P80 end is qualified by: E62 String`
- `E52 Time-Span. P81 ongoing throughout: E61 Time Primitive`
- `E52 Time-Span. P82 at some time within: E61 Time Primitive`
- `E54 Dimension. P90 has value: E60 Number`
- `E53 Place. P171 at some place within: E94 Space Primitive`
- `E53 Place. P172 contains: E94 Space Primitive`
- `E90 Symbolic Object. P190 has symbolic content: E62 String`

> B2. CIDOC Property forward direction is **not** defined whenever property domain is interpreted as rdfs:Literal (A.1). Similarly, CIDOC Property backwards/inverse direction is **not** defined, whenever property range is interpreted as rdfs:Literal (A.1). Further, the instances of classes interpreted as rdfs:Literal, cannot express in RDFs their **inherited** properties that could be expressed according to CIDOC Model.

As a result,

a) The following **direct forward direction** CIDOC Properties **cannot** be expressed and are **not defined** in RDFS:

- `E95 Spacetime Primitive. P169 defines spacetime volume (spacetime volume is defined by): E92 Spacetime Volume`
- `E61 Time Primitive. P170 defines time (time is defined by): E52 Time-Span`

b) The following **direct backwards direction** CIDOC Properties **cannot** be expressed and are **not defined** in RDFS:

- `E94 Space Primitive. P168i defines place (place is defined by): E53 Place`

> B3. Whenever no backwards/inverse property name is specified and property domain matches with property range, then the forward/direct property direction should be used for **both** directions and **no backwards/inverse property** needs to be defined.

As a result, we did not implement a separate backwards/inverse direction for the following CIDOC Properties:

- `E53 Place. P121 overlaps with: E53 Place`
- `E53 Place. P122 borders with: E53 Place`
- `E92 Spacetime Volume. P132 spatiotemporally overlaps with: E92 Spacetime Volume`
- `E92 Spacetime Volume. P133 is spatiotemporally separated from: E92 Spacetime Volume`

Additionally, all aforementioned redundant backwards/inverse CIDOC Property direction references, are replaced by the respective direct/forward CIDOC Property direction.

- The hierarchical link of  `P10i` subPropertyOf `P132i` was replaced with `P10i` subPropertyOf `P132`.

#### **C. Labels and appellations**

CIDOC-CRM version 7.1.3 defines the below subpropertyOf relations:

- `P168 place is defined by` `subPropertyOf` `P1 is identified by`
- `P169i spacetime volume is defined by` `subPropertyOf` `P1 is identified by`
- `P170i time is defined by` `subPropertyOf` `P1 is identified by`

The range of P168, P169i and P170i is `E94 Space Primitive`, `E95 Spacetime Primitive` and `E61 Time Primitive` respectively, which are all subclasses of `E41 Appellation` and interpreted as `rdfs:Literal` in RDFS, i.e. these three properties are datatype properties. However, the P1 property has range E41 Appellation, i.e. this property is an object property. Since OWL 2 distinguishes between object subproperties (https://www.w3.org/TR/2012/REC-owl2-syntax-20121211/#Object_Subproperties), data subproperties (https://www.w3.org/TR/2012/REC-owl2-syntax-20121211/#Data_Subproperties) and annotation subproperties (https://www.w3.org/TR/2012/REC-owl2-syntax-20121211/#Annotation_Subproperties), and also in OWL-DL the subject and object of a subproperty statement must be either both datatype properties or both object properties (see here (https://www.w3.org/TR/owl-ref/#subPropertyOf-def)), we do not include these three subPropertyOf relations in the provided RDFS implementation to avoid inconsistencies when reasoning with OWL 2 and OWL DL. Instead, we provide them in a separate ‘supplementary’ RDFS file which one can use if such inconsistencies are not expected.

In addition, since in the current practice, the property `rdfs:label` is widely used to denote appellations (see CRM-SIG Issue 394 (http://cidoc-crm.org/Issue/ID-394-solution-for-dualism-of-e41-appellation-and-rdfslabel)), the following `subPropertyOf` relation was also included in the supplementary RDFS file:

- `rdfs:label` subPropertyOf `P1 is identified by`

Note that according to the RDF Schema 1.1 specification, the domain (or range) of a property does not necessarily need to be 'subClassOf' or 'equal' to the domain (or range) of its superproperties. By including this subproperty relation, one can either directly use `rdfs:label` for providing a non-URI identifier/appellation for an instance of `E1 CRM Entity`, or use `P1 is identified by` for associating an additional URI-identifier with an instance of `E1 CRM Entity`, or use `P1 is identified by` and create an intermediate node (i.e. a URI-identifier for instance of `E41_Appellation`) for providing more detailed information about this appellation.

#### **D. Implementing Value Intervals**

The following are property pairs needed to simulate the interval-valued primitive values foreseen by the CRM:

> D1. addition of two new properties, defined as subproperties of `E52 Time-Span. P81 ongoing throughout: E61 Time Primitive`, for the 'maximum known temporal extent' boundaries specification of `E61 Time Primitive`.

As a result, we have created the following property definitions:

- `E52 Time-Span. P81a end of the begin: rdfs:Literal` (subPropertyOf `E52 Time-Span. P81 ongoing throughout: E61 Time Primitive`)
- `E52 Time-Span. P81b begin of the end: rdfs:Literal` (subPropertyOf `E52 Time-Span. P81 ongoing throughout: E61 Time Primitive`)

> D2. addition of two new properties, defined as subproperties of `E52 Time-Span. P82 at some time within: E61 Time Primitive`, for the 'minimum outer bounds' specification of `E61 Time Primitive`.

Consequently, we have created the following property definitions:

- `E52 Time-Span. P82a begin of the begin: rdfs:Literal` (subPropertyOf `E52 Time-Span. P82 at some time within: E61 Time Primitive`)
- `E52 Time-Span. P82b end of the end: rdfs:Literal` (subPropertyOf `E52 Time-Span. P82 at some time within: E61 Time Primitive`)

> D3. addition of two new properties, defined as subproperties of `E54 Dimension. P90 has value: E60 Number`, for the upper and lower boundaries specification of `E60 Number`.

Consequently, we have created the following property definitions:

- `E54 Dimension. P90a has lower value limit: rdfs:Literal` (subPropertyOf `E54 Dimension. P90 has value: E60 Number`)
- `E54 Dimension. P90b has upper value limit: rdfs:Literal` (subPropertyOf `E54 Dimension. P90 has value: E60 Number`)

#### **E. Multiple ISA custom declaration Classes**

The following are declarations of frequently used multiple instantiations as classes with respective multiple IsA (so far only one):

> E1. addition of a new class, defined as subClassOf `E41 Appellation` and `E33 Linguistic Object`, for all Appellations being regarded
specific to or characteristic for a language group and being described indirectly via a URI.

As a result, we have created the following class definition:

- `E33_E41_Linguistic_Appellation` subClass of `E33_Linguistic_Object` and `E41_Appellation`

#### **F. Translations and Scope notes**

> F1. **Translations** Each RDFS Class or Property definition is accompanied by a set of translations expressed as rdfs:labels separated by xml:lang tags. The translation label used for each language is **the most recent** still **valid** translation. Still valid translation may be interpreted in the following ways:

- The English label of the `CurrentVersion` that the current RDFS file is referring to is *almost equal* (accepting only differences regarding multiple spaces) to the English label of the `TranslationVersion` that the translated label was created for. For example, in order to accept a translation for `E22 Human-Made Object` in the CurrentVersion (7.1.3) we should have a translation for E22 that was created based on a CIDOC version that used the same name for E22. The class name of E22 was changed from `E22 Man-Made Object` to `E22 Human-Made Object` in version 6.2.7. So the only **valid** translations would be these that were created based on version 6.2.7 or later. Currently no such translation has been created, so `E22 Human-Made Object` in CurrentVersion (7.1.3) does not define any translation in the RDFS file.

- Another option is to qualify translations as **valid** based on the scope note comparison of `CurrentVersion` and `TranslationVersion`. Since scope notes include formatting information, the comparison should ignore formatting changes.

Currently in this version we follow the option to qualify translations as valid based on the comparison of the respective labels in the corresponding CIDOC versions.

> F2. **Scope notes** are defined as rdfs:comment and include only the text of the official CIDOC-CRM version in English language. Since scope notes are not just simple texts but include formatting data, a simple removal of the formatting data does not always produce a readable format. Therefore we followed the below simple conventions for the transformation of CIDOC-CRM scope note text into a readable rdfs:comment:

- Each Paragraph defines a new line
- Each element in an unordered list defines a new line
- Each element in an ordered list defines a new line prefixed with `'{order}. '`
- Each superscript text is separated from its base with `'-'`
- Each subscript text is separated from its base with `'_'` (none found)

> F3. **Scope notes of Inverse Properties**. Scope notes for the inverse/backwards direction of properties are not defined as they are covered by the definition of the direct/forward direction definition. Whenever the direct/forward property direction of a property `Pxxx` is not defined due to policy **B1**, then its scope note is used as scope note for the inverse/backwards property `Pxxxi`, and labeled as `Scope note for 'Pxxx':`.

As a result, the direct/forward property definition was used for the rdfs:comment definition of

- `E92 Spacetime Volume. P169i spacetime volume is defined by: rdfs:Literal`
- `E52 Time-Span. P170i time is defined by: rdfs:Literal`

"""@en ;
    owl:versionIRI <http://www.cidoc-crm.org/cidoc-crm/7.1.3/> ;
    owl:versionInfo "RDFs Implementation (February 2024) of CIDOC-CRM 7.1.3"@en .

<http://www.cidoc-crm.org/cidoc-crm/P122_borders_with> a rdf:Property ;
    rdfs:label "grenzt an"@de,
        "συνορεύει με"@el,
        "borders with"@en,
        "est limitrophe de"@fr,
        "fronteira com"@pt,
        "граничит с"@ru,
        "接壤于"@zh ;
    rdfs:comment """This symmetric property associates an instance of E53 Place with another instance of E53 Place which shares a part of its border.
This property is purely spatial. It does not imply that the phenomena that define, by their extent, places related by P122 borders with have ever shared a respective border at the same time or even coexisted. In particular, this may be the case when the respective common border is formed by a natural feature.
This property is not transitive. This property is symmetric."""@en ;
    rdfs:domain <http://www.cidoc-crm.org/cidoc-crm/E53_Place> ;
    rdfs:range <http://www.cidoc-crm.org/cidoc-crm/E53_Place> .

<http://www.cidoc-crm.org/cidoc-crm/P133_is_spatiotemporally_separated_from> a rdf:Property ;
    rdfs:label "is spatiotemporally separated from"@en,
        "est distinct spatio-temporellement de"@fr,
        "пространствeнно-врeмeнныe области отдeлeны от"@ru ;
    rdfs:comment """This symmetric property associates two instances of E92 Spacetime Volume that have no extents in common. If only the fuzzy boundaries of the instances of E92 Spacetime Volume overlap, this property cannot be determined from observation alone and therefore should not be applied. However, there may be other forms of justification that the two instances of E92 Spacetime Volume must not have any of their extents in common regardless of where and when precisely.
If this property holds for two instances of E92 Spacetime Volume then it cannot be the case that P132 spatiotemporally overlaps with also holds for the same two instances. Furthermore, there are cases where neither P132 spatiotemporally overlaps with nor P133 is spatiotemporally separated from holds between two instances of E92 Spacetime Volume. This would occur where only an overlap of the fuzzy boundaries of the two instances of E92 Spacetime Volume occurs and no other evidence is available.
This property is not transitive. This property is symmetric. This property is irreflexive."""@en ;
    rdfs:domain <http://www.cidoc-crm.org/cidoc-crm/E92_Spacetime_Volume> ;
    rdfs:range <http://www.cidoc-crm.org/cidoc-crm/E92_Spacetime_Volume> .

<http://www.cidoc-crm.org/cidoc-crm/P168_place_is_defined_by> a rdf:Property ;
    rdfs:label "place is defined by"@en,
        "lieu défini par"@fr,
        "мeсто опрeдeляeтся"@ru ;
    rdfs:comment "This property associates an instance of E53 Place with an instance of E94 Space Primitive that defines it. Syntactic variants or use of different scripts may result in multiple instances of E94 Space Primitive defining exactly the same place. Transformations between different reference systems always result in new definitions of places approximating each other and not in alternative definitions."@en ;
    rdfs:domain <http://www.cidoc-crm.org/cidoc-crm/E53_Place> ;
    rdfs:range rdfs:Literal .

<http://www.cidoc-crm.org/cidoc-crm/P169i_spacetime_volume_is_defined_by> a rdf:Property ;
    rdfs:label "spacetime volume is defined by"@en,
        "volume spatio-temporel défini par"@fr,
        "область пространства-врeмeни опрeдeляeтся по"@ru ;
    rdfs:comment "Scope note for 'P169': This property associates an instance of E95 Spacetime Primitive with the instance of E92 Spacetime Volume it defines."@en ;
    rdfs:domain <http://www.cidoc-crm.org/cidoc-crm/E92_Spacetime_Volume> ;
    rdfs:range rdfs:Literal .

<http://www.cidoc-crm.org/cidoc-crm/P170i_time_is_defined_by> a rdf:Property ;
    rdfs:label "time is defined by"@en,
        "temps défini par"@fr,
        "врeмя опрeдeляeтся по"@ru ;
    rdfs:comment """Scope note for 'P170': This property associates an instance of E61 Time Primitive with the instance of E52 Time-Span that constitutes the interpretation of the terms of the time primitive as an extent in absolute, real time.
The quantification allows several instances of E61 Time Primitive that are each expressed in different syntactic forms, to define the same instance of E52 Time-Span."""@en ;
    rdfs:domain <http://www.cidoc-crm.org/cidoc-crm/E52_Time-Span> ;
    rdfs:range rdfs:Literal .

<http://www.cidoc-crm.org/cidoc-crm/P171_at_some_place_within> a rdf:Property ;
    rdfs:label "at some place within"@en,
        "quelque part dans"@fr,
        "в нeкотором мeстe внутри"@ru ;
    rdfs:comment """This property describes the maximum spatial extent within which an instance of E53 Place falls. Since instances of E53 Places may not have precisely known spatial extents, the CIDOC CRM supports statements about maximum spatial extents of instances of E53 Place. This property allows an instance of E53 Place’s maximum spatial extent (i.e., its outer boundary) to be assigned an instance of E94 Space Primitive value.
This property is a shortcut of the fully developed path from E53 Place, P89 falls within, E53 Place, P168 place is defined by to E94 Space Primitive through a declarative Place that is not explicitly documented, to a Space Primitive: declarative places are defined in CRMgeo (Doerr and Hiebel 2013)."""@en ;
    rdfs:domain <http://www.cidoc-crm.org/cidoc-crm/E53_Place> ;
    rdfs:range rdfs:Literal .

<http://www.cidoc-crm.org/cidoc-crm/P172_contains> a rdf:Property ;
    rdfs:label "contains"@en,
        "contient"@fr,
        "содeржит"@ru ;
    rdfs:comment """This property describes a minimum spatial extent which is contained within an instance of E53 Place. Since instances of E53 Place may not have precisely known spatial extents, the CIDOC CRM supports statements about minimum spatial extents of instances of E53 Place. This property allows an instance of E53 Place’s minimum spatial extent (i.e., its inner boundary or a point being within a Place) to be assigned an instance of E94 Space Primitive value.
This property is a shortcut of the fully developed path from E53 Place, P89i contains, E53 Place, P168 place is defined by to E94 Space Primitive."""@en ;
    rdfs:domain <http://www.cidoc-crm.org/cidoc-crm/E53_Place> ;
    rdfs:range rdfs:Literal .

<http://www.cidoc-crm.org/cidoc-crm/P190_has_symbolic_content> a rdf:Property ;
    rdfs:label "has symbolic content"@en,
        "a pour contenu symbolique"@fr,
        "имeeт символичeскоe содeржаниe"@ru ;
    rdfs:comment """This property associates an instance of E90 Symbolic Object with a complete, identifying representation of its content in the form of an instance of E62 String.
This property only applies to instances of E90 Symbolic Object that can be represented completely in this form. The representation may be more specific than the symbolic level defining the identity condition of the represented. This depends on the type of the symbolic object represented. For instance, if a name has type “Modern Greek character sequence”, it may be represented in a loss-free Latin transcription, meaning however the sequence of Greek letters.
As another example, if the represented object has type “English words sequence”, American English or British English spelling variants may be chosen to represent the English word “colour” without defining a different symbolic object. If a name has type “European traditional name”, no particular string may define its content."""@en ;
    rdfs:domain <http://www.cidoc-crm.org/cidoc-crm/E90_Symbolic_Object> ;
    rdfs:range rdfs:Literal ;
    rdfs:subPropertyOf <http://www.cidoc-crm.org/cidoc-crm/P3_has_note> .

<http://www.cidoc-crm.org/cidoc-crm/P57_has_number_of_parts> a rdf:Property ;
    rdfs:label "hat Anzahl Teile"@de,
        "έχει αριθμό μερών"@el,
        "has number of parts"@en,
        "a pour nombre d’éléments"@fr,
        "tem número de partes"@pt,
        "имeeт число частeй"@ru,
        "有组成部分数"@zh ;
    rdfs:comment """This property documents the number of parts, an instance of E60 Number, of which an instance of E19 Physical Object is composed.
This may be used as a method of checking inventory counts with regard to aggregate or collective objects. What constitutes a part or component depends on the context and requirements of the documentation. Normally, the parts documented in this way would not be considered as worthy of individual attention.
For a more complete description, objects may be decomposed into their components and constituents using P46 is composed of (forms parts of) and P45 consists of (is incorporated in). This allows each element to be described individually."""@en ;
    rdfs:domain <http://www.cidoc-crm.org/cidoc-crm/E19_Physical_Object> ;
    rdfs:range rdfs:Literal .

<http://www.cidoc-crm.org/cidoc-crm/P79_beginning_is_qualified_by> a rdf:Property ;
    rdfs:label "hat Anfangsbegründung"@de,
        "αρχή προσδιορίζεται από"@el,
        "beginning is qualified by"@en,
        "a son début qualifié par"@fr,
        "início é qualificado por"@pt,
        "начало ограничeно"@ru,
        "起始限定"@zh ;
    rdfs:comment "This property associates an instance of E52 Time-Span with a note detailing the scholarly or scientific opinions and justifications about the certainty, precision, sources etc. of its beginning. Such notes may also be used to elaborate arguments about constraints or to give explanations of alternatives."@en ;
    rdfs:domain <http://www.cidoc-crm.org/cidoc-crm/E52_Time-Span> ;
    rdfs:range rdfs:Literal ;
    rdfs:subPropertyOf <http://www.cidoc-crm.org/cidoc-crm/P3_has_note> .

<http://www.cidoc-crm.org/cidoc-crm/P80_end_is_qualified_by> a rdf:Property ;
    rdfs:label "hat Begründung des Endes"@de,
        "τέλος προσδιορίζεται από"@el,
        "end is qualified by"@en,
        "a sa fin qualifiée par"@fr,
        "final é qualificado por"@pt,
        "конeц ограничeн"@ru,
        "结束限定"@zh ;
    rdfs:comment "This property associates an instance of E52 Time-Span with a note detailing the scholarly or scientific opinions and justifications about the end of this time-span concerning certainty, precision, sources etc. This property may also be used to describe arguments constraining possible dates and to distinguish reasons for alternative dates."@en ;
    rdfs:domain <http://www.cidoc-crm.org/cidoc-crm/E52_Time-Span> ;
    rdfs:range rdfs:Literal ;
    rdfs:subPropertyOf <http://www.cidoc-crm.org/cidoc-crm/P3_has_note> .

<http://www.cidoc-crm.org/cidoc-crm/P90a_has_lower_value_limit> a rdf:Property ;
    rdfs:label "has lower value limit"@en ;
    rdfs:domain <http://www.cidoc-crm.org/cidoc-crm/E54_Dimension> ;
    rdfs:range rdfs:Literal ;
    rdfs:subPropertyOf <http://www.cidoc-crm.org/cidoc-crm/P90_has_value> .

<http://www.cidoc-crm.org/cidoc-crm/P90b_has_upper_value_limit> a rdf:Property ;
    rdfs:label "has upper value limit"@en ;
    rdfs:domain <http://www.cidoc-crm.org/cidoc-crm/E54_Dimension> ;
    rdfs:range rdfs:Literal ;
    rdfs:subPropertyOf <http://www.cidoc-crm.org/cidoc-crm/P90_has_value> .

<http://www.cidoc-crm.org/extensions/crmarchaeo/> a owl:Ontology ;
    rdfs:comment "CRMarchaeo is an extension of CIDOC CRM created to support the archaeological excavation process and all the various entities and activities related to it. The model has been created starting from standards and models already in use by national and international cultural heritage institutions, and has evolved through deep analysis of existing metadata from real archaeological documentation. It has been enriched by continuous collaboration with various communities of archaeologists from different countries and schools. Furthermore, it takes advantage of the concepts provided by CRMsci, from which it inherits most of the geological and stratigraphic principles that govern archaeological stratigraphy, extending these principles."@en ;
    owl:versionInfo "CRMarchaeo 2.1.1 (April, 2024) including references to CIDOC-CRM 7.1.2 and CRMsci 2.0"@en .

<http://www.cidoc-crm.org/extensions/crmarchaeo/AP22_is_equal_in_time_to> a rdf:Property ;
    rdfs:label "is equal in time to"@en ;
    rdfs:comment "This property symmetrically identifies a situation in which the starting point and the ending point for an instance of E2 Temporal Entity is equal to the starting point and the ending point of another instance of E2 Temporal Entity, respectively. This property is only necessary if the time span is unknown (otherwise the equivalence can be calculated). This property is the same as the \"equal\" relationship of Allen’s temporal logic (Allen, 1983, pp. 832-843). This property is transitive."@en ;
    rdfs:domain <http://www.cidoc-crm.org/cidoc-crm/E2_Temporal_Entity> ;
    rdfs:range <http://www.cidoc-crm.org/cidoc-crm/E2_Temporal_Entity> ;
    rdfs:subPropertyOf <http://www.cidoc-crm.org/cidoc-crm/P175_starts_before_or_with_the_start_of>,
        <http://www.cidoc-crm.org/cidoc-crm/P175i_starts_after_or_with_the_start_of>,
        <http://www.cidoc-crm.org/cidoc-crm/P184_ends_before_or_with_the_end_of>,
        <http://www.cidoc-crm.org/cidoc-crm/P184i_ends_with_or_after_the_end_of> .

<http://www.cidoc-crm.org/extensions/crmsci/> a owl:Ontology ;
    rdfs:comment "The Scientific Observation Model (CRMsci) is a formal ontology intended to be used as a global schema for integrating metadata about scientific observation, measurements and processed data in descriptive and empirical sciences such as biodiversity, geology, geography, archaeology, cultural heritage conservation and others in research IT environments and research data libraries. Its primary purpose is facilitating the management, integration, mediation, interchange and access to research data by description of semantic relationships, in particular causal ones. It is not primarily a model to process the data themselves in order to produce new research results, even though its representations offer themselves to be used for some kind of processing."@en ;
    owl:versionIRI <http://www.cidoc-crm.org/extensions/crmsci/2.0/> ;
    owl:versionInfo "CRMsci Ontology 2.0 (March, 2023) including references to CIDOC-CRM 7.1.2"@en .

<http://www.cidoc-crm.org/extensions/crmsci/O30_determined_position> a rdf:Property ;
    rdfs:label "determined position"@en ;
    rdfs:comment "This property associates an instance of S23 Position Determination with the instance of E94 Space Primitive which is the result of that determination. The instance of E94 Space Primitive approximates the place occupied by the entity whose position is being determined."@en ;
    rdfs:domain <http://www.cidoc-crm.org/extensions/crmsci/S23_Position_Determination> ;
    rdfs:range rdfs:Literal .

<http://www.cidoc-crm.org/extensions/crmtex/> a owl:Ontology ;
    rdfs:comment "CRMtex is an extension of the CIDOC CRM created to support the study of ancient and handwritten documents, i.e., texts characterised by uniqueness since they have been produced without the use of techniques typical of modern mechanized processes of production. CRMtex aims to model information concerning ancient inscriptions (including coins, marks and stamps), papyri, medieval manuscripts, but also modern handwritten documents of any kind."@en ;
    owl:versionInfo "CRMtex Ontology 2.0 (June, 2023) including references to CIDOC-CRM 7.1.2, CRMinf 0.7b, CRMsci 2.0, and FRBRoo 2.4"@en .

<http://www.ics.forth.gr/isl/CRMba/BP11_is_connected_to> a rdf:Property ;
    rdfs:domain <http://www.ics.forth.gr/isl/CRMba/B2_Morphological_Building_Section> ;
    rdfs:range <http://www.ics.forth.gr/isl/CRMba/B2_Morphological_Building_Section> .

<http://www.ics.forth.gr/isl/CRMba/BP11i_is_connected_to> a rdf:Property ;
    rdfs:domain <http://www.ics.forth.gr/isl/CRMba/B2_Morphological_Building_Section> ;
    rdfs:range <http://www.ics.forth.gr/isl/CRMba/B2_Morphological_Building_Section> .

<http://www.ics.forth.gr/isl/CRMba/BP12_is_connected_through> a rdf:Property ;
    rdfs:domain <http://www.ics.forth.gr/isl/CRMba/B2_Morphological_Building_Section> ;
    rdfs:range <http://www.ics.forth.gr/isl/CRMba/B2_Morphological_Building_Section> .

<http://www.ics.forth.gr/isl/CRMba/BP12i_is_connected_through> a rdf:Property ;
    rdfs:domain <http://www.ics.forth.gr/isl/CRMba/B2_Morphological_Building_Section> ;
    rdfs:range <http://www.ics.forth.gr/isl/CRMba/B2_Morphological_Building_Section> .

<http://www.ics.forth.gr/isl/CRMba/BP13_used_specific_object> a rdf:Property ;
    rdfs:domain <http://www.cidoc-crm.org/cidoc-crm/E12_Production> ;
    rdfs:range <http://www.ics.forth.gr/isl/CRMba/B5_Stratigraphic_Building_Unit> .

<http://www.ics.forth.gr/isl/CRMba/BP13i_was_specific_object_used_by> a rdf:Property ;
    rdfs:domain <http://www.ics.forth.gr/isl/CRMba/B5_Stratigraphic_Building_Unit> ;
    rdfs:range <http://www.cidoc-crm.org/cidoc-crm/E12_Production> .

<http://www.ics.forth.gr/isl/CRMba/BP14_re-used_specific_object> a rdf:Property ;
    rdfs:domain <http://www.cidoc-crm.org/cidoc-crm/E12_Production> ;
    rdfs:range <http://www.ics.forth.gr/isl/CRMba/B5_Stratigraphic_Building_Unit> .

<http://www.ics.forth.gr/isl/CRMba/BP14i_was_specific_object_re-used_by> a rdf:Property ;
    rdfs:domain <http://www.ics.forth.gr/isl/CRMba/B5_Stratigraphic_Building_Unit> ;
    rdfs:range <http://www.cidoc-crm.org/cidoc-crm/E12_Production> .

<http://www.ics.forth.gr/isl/CRMba/BP15_is_equal_to> a rdf:Property ;
    rdfs:domain <http://www.ics.forth.gr/isl/CRMba/B5_Stratigraphic_Building_Unit> ;
    rdfs:range <http://www.ics.forth.gr/isl/CRMba/B3_Filled_Morphological_Building_Section> .

<http://www.ics.forth.gr/isl/CRMba/BP15i_is_equal_to> a rdf:Property ;
    rdfs:domain <http://www.ics.forth.gr/isl/CRMba/B3_Filled_Morphological_Building_Section> ;
    rdfs:range <http://www.ics.forth.gr/isl/CRMba/B5_Stratigraphic_Building_Unit> .

<http://www.ics.forth.gr/isl/CRMba/BP1_is_section_of> a rdf:Property ;
    rdfs:domain <http://www.ics.forth.gr/isl/CRMba/B2_Morphological_Building_Section> ;
    rdfs:range <http://www.ics.forth.gr/isl/CRMba/B1_Built_Work> .

<http://www.ics.forth.gr/isl/CRMba/BP1i_has_section> a rdf:Property ;
    rdfs:domain <http://www.ics.forth.gr/isl/CRMba/B1_Built_Work> ;
    rdfs:range <http://www.ics.forth.gr/isl/CRMba/B2_Morphological_Building_Section> .

<http://www.ics.forth.gr/isl/CRMba/BP2_is_constituent_of> a rdf:Property ;
    rdfs:domain <http://www.ics.forth.gr/isl/CRMba/B5_Stratigraphic_Building_Unit> ;
    rdfs:range <http://www.ics.forth.gr/isl/CRMba/B1_Built_Work> .

<http://www.ics.forth.gr/isl/CRMba/BP2i_is_constituted_by> a rdf:Property ;
    rdfs:domain <http://www.ics.forth.gr/isl/CRMba/B1_Built_Work> ;
    rdfs:range <http://www.ics.forth.gr/isl/CRMba/B5_Stratigraphic_Building_Unit> .

<http://www.ics.forth.gr/isl/CRMba/BP3_is_spatial_temporary_equal_to> a rdf:Property ;
    rdfs:domain <http://www.cidoc-crm.org/cidoc-crm/E92_Spacetime_Volume> ;
    rdfs:range <http://www.cidoc-crm.org/cidoc-crm/E92_Spacetime_Volume> .

<http://www.ics.forth.gr/isl/CRMba/BP3i_is_spatial_temporary_equal_to> a rdf:Property ;
    rdfs:domain <http://www.cidoc-crm.org/cidoc-crm/E92_Spacetime_Volume> ;
    rdfs:range <http://www.cidoc-crm.org/cidoc-crm/E92_Spacetime_Volume> .

<http://www.ics.forth.gr/isl/CRMba/BP4_terminates_the_constituency> a rdf:Property ;
    rdfs:domain <http://www.cidoc-crm.org/cidoc-crm/E80_Part_removal> ;
    rdfs:range <http://www.ics.forth.gr/isl/CRMba/B2_Morphological_Building_Section> .

<http://www.ics.forth.gr/isl/CRMba/BP4i_constituency_was_terminated_by> a rdf:Property ;
    rdfs:domain <http://www.ics.forth.gr/isl/CRMba/B2_Morphological_Building_Section> ;
    rdfs:range <http://www.cidoc-crm.org/cidoc-crm/E80_Part_removal> .

<http://www.ics.forth.gr/isl/CRMba/BP5_initiates_the_constituency> a rdf:Property ;
    rdfs:domain <http://www.cidoc-crm.org/cidoc-crm/E79_Part_addition> ;
    rdfs:range <http://www.ics.forth.gr/isl/CRMba/B2_Morphological_Building_Section> .

<http://www.ics.forth.gr/isl/CRMba/BP5i_constituency_was_initiated_by> a rdf:Property ;
    rdfs:domain <http://www.ics.forth.gr/isl/CRMba/B2_Morphological_Building_Section> ;
    rdfs:range <http://www.cidoc-crm.org/cidoc-crm/E79_Part_addition> .

<http://www.ics.forth.gr/isl/CRMdig/L13_used_parameters> a rdf:Property ;
    rdfs:comment """This property associates an instance of D10 Software Execution with a digital object
 used as a parameter during the process.This property is a specialisation of L1O had input (was input of)."""@en ;
    rdfs:domain <http://www.ics.forth.gr/isl/CRMdig/D10_Software_Execution> ;
    rdfs:range <http://www.ics.forth.gr/isl/CRMdig/D1_Digital_Object> ;
    rdfs:subPropertyOf <http://www.ics.forth.gr/isl/CRMdig/L10_had_input> .

<http://www.ics.forth.gr/isl/CRMdig/L13i_parameters_for> a rdf:Property ;
    rdfs:domain <http://www.ics.forth.gr/isl/CRMdig/D1_Digital_Object> ;
    rdfs:range <http://www.ics.forth.gr/isl/CRMdig/D10_Software_Execution> ;
    rdfs:subPropertyOf <http://www.ics.forth.gr/isl/CRMdig/L10i_was_input_of> .

<http://www.ics.forth.gr/isl/CRMdig/L14_transferred> a rdf:Property ;
    rdfs:comment """This property  identifies a digital object transferred by a D12 Data Transfer Event.
This property is a specialisation of L11 had output (was output of)."""@en ;
    rdfs:domain <http://www.ics.forth.gr/isl/CRMdig/D12_Data_Transfer_Event> ;
    rdfs:range <http://www.ics.forth.gr/isl/CRMdig/D1_Digital_Object> ;
    rdfs:subPropertyOf <http://www.ics.forth.gr/isl/CRMdig/L10_had_input>,
        <http://www.ics.forth.gr/isl/CRMdig/L11_had_output> .

<http://www.ics.forth.gr/isl/CRMdig/L14i_was_transferred_by> a rdf:Property ;
    rdfs:domain <http://www.ics.forth.gr/isl/CRMdig/D1_Digital_Object> ;
    rdfs:range <http://www.ics.forth.gr/isl/CRMdig/D12_Data_Transfer_Event> ;
    rdfs:subPropertyOf <http://www.ics.forth.gr/isl/CRMdig/L10i_was_input_of>,
        <http://www.ics.forth.gr/isl/CRMdig/L11i_was_output_of> .

<http://www.ics.forth.gr/isl/CRMdig/L15_has_sender> a rdf:Property ;
    rdfs:comment """This property  identifies a digital device used as a medium on which data are transferred 
through a D12 Data Transfer Event."""@en ;
    rdfs:domain <http://www.ics.forth.gr/isl/CRMdig/D12_Data_Transfer_Event> ;
    rdfs:range <http://www.ics.forth.gr/isl/CRMdig/D8_Digital_Device> ;
    rdfs:subPropertyOf <http://www.ics.forth.gr/isl/CRMdig/L12_happened_on_device> .

<http://www.ics.forth.gr/isl/CRMdig/L15i_was_sender_for> a rdf:Property ;
    rdfs:domain <http://www.ics.forth.gr/isl/CRMdig/D8_Digital_Device> ;
    rdfs:range <http://www.ics.forth.gr/isl/CRMdig/D12_Data_Transfer_Event> ;
    rdfs:subPropertyOf <http://www.ics.forth.gr/isl/CRMdig/L12i_was_device_for> .

<http://www.ics.forth.gr/isl/CRMdig/L16_has_receiver> a rdf:Property ;
    rdfs:comment """This property  identifies a digital device used as a medium to receive data  
through a D12 Data Transfer Event."""@en ;
    rdfs:domain <http://www.ics.forth.gr/isl/CRMdig/D12_Data_Transfer_Event> ;
    rdfs:range <http://www.ics.forth.gr/isl/CRMdig/D8_Digital_Device> ;
    rdfs:subPropertyOf <http://www.ics.forth.gr/isl/CRMdig/L12_happened_on_device> .

<http://www.ics.forth.gr/isl/CRMdig/L16i_was_receiver_for> a rdf:Property ;
    rdfs:domain <http://www.ics.forth.gr/isl/CRMdig/D8_Digital_Device> ;
    rdfs:range <http://www.ics.forth.gr/isl/CRMdig/D12_Data_Transfer_Event> ;
    rdfs:subPropertyOf <http://www.ics.forth.gr/isl/CRMdig/L12i_was_device_for> .

<http://www.ics.forth.gr/isl/CRMdig/L17_measured_thing_of_type> a rdf:Property ;
    rdfs:comment """This property associates an instance of D11 Digital Measurement Event with the instance of E55
Type of object to which it applied. This property is a specialisation of P125 used object of type. """@en ;
    rdfs:domain <http://www.ics.forth.gr/isl/CRMdig/D11_Digital_Measurement_Event> ;
    rdfs:range <http://www.cidoc-crm.org/cidoc-crm/E55_Type> ;
    rdfs:subPropertyOf <http://www.cidoc-crm.org/cidoc-crm/P125_used_object_of_type> .

<http://www.ics.forth.gr/isl/CRMdig/L17i_was_type_of_thing_measured_by> a rdf:Property ;
    rdfs:domain <http://www.cidoc-crm.org/cidoc-crm/E55_Type> ;
    rdfs:range <http://www.ics.forth.gr/isl/CRMdig/D11_Digital_Measurement_Event> ;
    rdfs:subPropertyOf <http://www.cidoc-crm.org/cidoc-crm/P125i_was_type_of_object_used_in> .

<http://www.ics.forth.gr/isl/CRMdig/L18_has_modified> a rdf:Property ;
    rdfs:comment """This property identifies a Digital Information Carrier modified in a Digital Machine Event.
This property is a specialisation of P31 has modified."""@en ;
    rdfs:domain <http://www.ics.forth.gr/isl/CRMdig/D7_Digital_Machine_Event> ;
    rdfs:range <http://www.ics.forth.gr/isl/CRMdig/D13_Digital_Information_Carrier> ;
    rdfs:subPropertyOf <http://www.cidoc-crm.org/cidoc-crm/P31_has_modified> .

<http://www.ics.forth.gr/isl/CRMdig/L18i_was_modified_by> a rdf:Property ;
    rdfs:domain <http://www.ics.forth.gr/isl/CRMdig/D13_Digital_Information_Carrier> ;
    rdfs:range <http://www.ics.forth.gr/isl/CRMdig/D7_Digital_Machine_Event> ;
    rdfs:subPropertyOf <http://www.cidoc-crm.org/cidoc-crm/P31i_was_modified_by> .

<http://www.ics.forth.gr/isl/CRMdig/L19_stores> a rdf:Property ;
    rdfs:comment """This property associates an instance of a D13 Digital Information Carrier with the instance of Digital Object 
that is stored on it. This property is a specialisation of P128 carries."""@en ;
    rdfs:domain <http://www.ics.forth.gr/isl/CRMdig/D13_Digital_Information_Carrier> ;
    rdfs:range <http://www.ics.forth.gr/isl/CRMdig/D1_Digital_Object> ;
    rdfs:subPropertyOf <http://www.cidoc-crm.org/cidoc-crm/P128_carries> .

<http://www.ics.forth.gr/isl/CRMdig/L19i_is_stored_on> a rdf:Property ;
    rdfs:domain <http://www.ics.forth.gr/isl/CRMdig/D1_Digital_Object> ;
    rdfs:range <http://www.ics.forth.gr/isl/CRMdig/D13_Digital_Information_Carrier> ;
    rdfs:subPropertyOf <http://www.cidoc-crm.org/cidoc-crm/P128i_is_carried_by> .

<http://www.ics.forth.gr/isl/CRMdig/L1_digitized> a rdf:Property ;
    rdfs:comment """This property associates an instance of D2 Digitization Process with an instance of E18 Physical Thing which is a material thing.  
This property is a specialisation of P39 measured (was measured by).
"""@en ;
    rdfs:domain <http://www.ics.forth.gr/isl/CRMdig/D2_Digitization_Process> ;
    rdfs:range <http://www.cidoc-crm.org/cidoc-crm/E18_Physical_Thing> ;
    rdfs:subPropertyOf <http://www.cidoc-crm.org/cidoc-crm/P39_measured> .

<http://www.ics.forth.gr/isl/CRMdig/L1i_was_digitized_by> a rdf:Property ;
    rdfs:domain <http://www.cidoc-crm.org/cidoc-crm/E18_Physical_Thing> ;
    rdfs:range <http://www.ics.forth.gr/isl/CRMdig/D2_Digitization_Process> ;
    rdfs:subPropertyOf <http://www.cidoc-crm.org/cidoc-crm/P39i_was_measured_by> .

<http://www.ics.forth.gr/isl/CRMdig/L20_has_created> a rdf:Property ;
    rdfs:comment """This property identifies a Data Object that came into existence as a result of a D11 Digital Measurement Event.
This property is a specialisation of P40 observed dimension and L11 had output."""@en ;
    rdfs:domain <http://www.ics.forth.gr/isl/CRMdig/D11_Digital_Measurement_Event> ;
    rdfs:range <http://www.ics.forth.gr/isl/CRMdig/D9_Data_Object> ;
    rdfs:subPropertyOf <http://www.cidoc-crm.org/cidoc-crm/P40_observed_dimension>,
        <http://www.ics.forth.gr/isl/CRMdig/L11_had_output> .

<http://www.ics.forth.gr/isl/CRMdig/L20i_was_created_by> a rdf:Property ;
    rdfs:domain <http://www.ics.forth.gr/isl/CRMdig/D9_Data_Object> ;
    rdfs:range <http://www.ics.forth.gr/isl/CRMdig/D11_Digital_Measurement_Event> ;
    rdfs:subPropertyOf <http://www.cidoc-crm.org/cidoc-crm/P40i_was_observed_in>,
        <http://www.ics.forth.gr/isl/CRMdig/L11i_was_output_of> .

<http://www.ics.forth.gr/isl/CRMdig/L21_used_as_derivation_source> a rdf:Property ;
    rdfs:comment "This property associates an instance of a D3 Formal Derivation with the instance of D1 Digital Object that is used as a derivation source."@en ;
    rdfs:domain <http://www.ics.forth.gr/isl/CRMdig/D3_Formal_Derivation> ;
    rdfs:range <http://www.ics.forth.gr/isl/CRMdig/D1_Digital_Object> ;
    rdfs:subPropertyOf <http://www.ics.forth.gr/isl/CRMdig/L2_used_as_source> .

<http://www.ics.forth.gr/isl/CRMdig/L21i_was_derivation_source_for> a rdf:Property ;
    rdfs:domain <http://www.ics.forth.gr/isl/CRMdig/D1_Digital_Object> ;
    rdfs:range <http://www.ics.forth.gr/isl/CRMdig/D3_Formal_Derivation> ;
    rdfs:subPropertyOf <http://www.ics.forth.gr/isl/CRMdig/L2i_was_source_for> .

<http://www.ics.forth.gr/isl/CRMdig/L22_created_derivative> a rdf:Property ;
    rdfs:comment """This property associates an instance of D3 Formal Derivation with the Digital Object it used to create a version of.
This property is a specialisation of L11 had output."""@en ;
    rdfs:domain <http://www.ics.forth.gr/isl/CRMdig/D3_Formal_Derivation> ;
    rdfs:range <http://www.ics.forth.gr/isl/CRMdig/D1_Digital_Object> ;
    rdfs:subPropertyOf <http://www.ics.forth.gr/isl/CRMdig/L11_had_output> .

<http://www.ics.forth.gr/isl/CRMdig/L22i_was_derivative_created_by> a rdf:Property ;
    rdfs:domain <http://www.ics.forth.gr/isl/CRMdig/D1_Digital_Object> ;
    rdfs:range <http://www.ics.forth.gr/isl/CRMdig/D3_Formal_Derivation> ;
    rdfs:subPropertyOf <http://www.ics.forth.gr/isl/CRMdig/L11i_was_output_of> .

<http://www.ics.forth.gr/isl/CRMdig/L23_used_software_or_firmware> a rdf:Property ;
    rdfs:comment """This property associates an instance of D7 Digital Machine Event with the instance of D14 Software that had used.
This property is a specialisation of P16 used specific object."""@en ;
    rdfs:domain <http://www.ics.forth.gr/isl/CRMdig/D7_Digital_Machine_Event> ;
    rdfs:range <http://www.ics.forth.gr/isl/CRMdig/D14_Software> ;
    rdfs:subPropertyOf <http://www.cidoc-crm.org/cidoc-crm/P16_used_specific_object> .

<http://www.ics.forth.gr/isl/CRMdig/L23i_was_software_or_firmware_used_by> a rdf:Property ;
    rdfs:domain <http://www.ics.forth.gr/isl/CRMdig/D14_Software> ;
    rdfs:range <http://www.ics.forth.gr/isl/CRMdig/D7_Digital_Machine_Event> ;
    rdfs:subPropertyOf <http://www.cidoc-crm.org/cidoc-crm/P16i_was_used_for> .

<http://www.ics.forth.gr/isl/CRMdig/L24_created_logfile> a rdf:Property ;
    rdfs:comment "This property identifies the logfile that was created by a D10 Software Execution in order to record all the activities in the system."@en ;
    rdfs:domain <http://www.ics.forth.gr/isl/CRMdig/D10_Software_Execution> ;
    rdfs:range <http://www.ics.forth.gr/isl/CRMdig/D1_Digital_Object> ;
    rdfs:subPropertyOf <http://www.ics.forth.gr/isl/CRMdig/L11_had_output> .

<http://www.ics.forth.gr/isl/CRMdig/L24i_was_logfile_created_by> a rdf:Property ;
    rdfs:domain <http://www.ics.forth.gr/isl/CRMdig/D1_Digital_Object> ;
    rdfs:range <http://www.ics.forth.gr/isl/CRMdig/D10_Software_Execution> ;
    rdfs:subPropertyOf <http://www.ics.forth.gr/isl/CRMdig/L11i_was_output_of> .

<http://www.ics.forth.gr/isl/CRMdig/L30_has_operator> a rdf:Property ;
    rdfs:comment """This property describes the activity that is being operated by a person.
This property is a specialisation of P14 carried out by."""@en ;
    rdfs:domain <http://www.cidoc-crm.org/cidoc-crm/E7_Activity> ;
    rdfs:range <http://www.cidoc-crm.org/cidoc-crm/E21_Person> ;
    rdfs:subPropertyOf <http://www.cidoc-crm.org/cidoc-crm/P14_carried_out_by> .

<http://www.ics.forth.gr/isl/CRMdig/L30i_is_operator_of> a rdf:Property ;
    rdfs:domain <http://www.cidoc-crm.org/cidoc-crm/E21_Person> ;
    rdfs:range <http://www.cidoc-crm.org/cidoc-crm/E7_Activity> ;
    rdfs:subPropertyOf <http://www.cidoc-crm.org/cidoc-crm/P14i_performed> .

<http://www.ics.forth.gr/isl/CRMdig/L31_has_starting_date-time> a rdf:Property ;
    rdfs:comment """This property allows the starting point for a D7 Digital Machine Event to be situated.   
This property expresses the approximation of the starting date of a time span."""@en ;
    rdfs:domain <http://www.cidoc-crm.org/cidoc-crm/E5_Event> ;
    rdfs:range xsd:dateTime ;
    rdfs:subPropertyOf <http://www.cidoc-crm.org/cidoc-crm/P82a_begin_of_the_begin> .

<http://www.ics.forth.gr/isl/CRMdig/L32_has_ending_date-time> a rdf:Property ;
    rdfs:comment """This property allows the ending point for a D7 Digital Machine Event to be situated.   
This property expresses the approximation of the ending date of a time span."""@en ;
    rdfs:domain <http://www.cidoc-crm.org/cidoc-crm/E5_Event> ;
    rdfs:range xsd:dateTime ;
    rdfs:subPropertyOf <http://www.cidoc-crm.org/cidoc-crm/P82b_end_of_the_end> .

<http://www.ics.forth.gr/isl/CRMdig/L33_has_maker> a rdf:Property ;
    rdfs:comment """This property identifies the maker, the actor who is responsible for the production of a device,
 a computer, a digital camera, any kind of a machine that has been produced.
This property is a shortcut of a more fully developed path from CRM E12 Production:P108 has produced:E24 Physical Man-Made Thing. 
In this case, there is no need to describe the more detailed property through a production event,so L33 has maker is reccomended to be used instead. """@en ;
    rdfs:domain <http://www.cidoc-crm.org/cidoc-crm/E72_Legal_Object> ;
    rdfs:range <http://www.cidoc-crm.org/cidoc-crm/E39_Actor> .

<http://www.ics.forth.gr/isl/CRMdig/L33i_is_maker_of> a rdf:Property ;
    rdfs:domain <http://www.cidoc-crm.org/cidoc-crm/E39_Actor> ;
    rdfs:range <http://www.cidoc-crm.org/cidoc-crm/E72_Legal_Object> .

<http://www.ics.forth.gr/isl/CRMdig/L34_has_contractor> a rdf:Property ;
    rdfs:comment """This property describes the participation of a Legal Body in being contractor for the outcome of a specific activity.
This property is a specialisation of L29_has_responsible_organization."""@en ;
    rdfs:domain <http://www.cidoc-crm.org/cidoc-crm/E7_Activity> ;
    rdfs:range <http://www.cidoc-crm.org/cidoc-crm/E40_Legal_Body> ;
    rdfs:subPropertyOf <http://www.ics.forth.gr/isl/CRMdig/L29_has_responsible_organization> .

<http://www.ics.forth.gr/isl/CRMdig/L34i_is_contractor_for> a rdf:Property ;
    rdfs:domain <http://www.cidoc-crm.org/cidoc-crm/E40_Legal_Body> ;
    rdfs:range <http://www.cidoc-crm.org/cidoc-crm/E7_Activity> ;
    rdfs:subPropertyOf <http://www.ics.forth.gr/isl/CRMdig/L29i_is_responsible_organization_for> .

<http://www.ics.forth.gr/isl/CRMdig/L35_has_commissioner> a rdf:Property ;
    rdfs:comment """This property describes the participation of a Legal Body in being commissioner for the outcome of a specific activity.
This property is a specialisation of L29_has_responsible_organization."""@en ;
    rdfs:domain <http://www.cidoc-crm.org/cidoc-crm/E7_Activity> ;
    rdfs:range <http://www.cidoc-crm.org/cidoc-crm/E40_Legal_Body> ;
    rdfs:subPropertyOf <http://www.ics.forth.gr/isl/CRMdig/L29_has_responsible_organization> .

<http://www.ics.forth.gr/isl/CRMdig/L35i_is_commissioner_for> a rdf:Property ;
    rdfs:domain <http://www.cidoc-crm.org/cidoc-crm/E40_Legal_Body> ;
    rdfs:range <http://www.cidoc-crm.org/cidoc-crm/E7_Activity> ;
    rdfs:subPropertyOf <http://www.ics.forth.gr/isl/CRMdig/L29i_is_responsible_organization_for> .

<http://www.ics.forth.gr/isl/CRMdig/L43_annotates> a rdf:Property ;
    rdfs:comment """This property describes the associations between objects or areas of objects of the RI, 
with other objects or regions or persons, places, events.."""@en ;
    rdfs:domain <http://www.ics.forth.gr/isl/CRMdig/D29_Annotation_Object> ;
    rdfs:range <http://www.cidoc-crm.org/cidoc-crm/E1_CRM_Entity> .

<http://www.ics.forth.gr/isl/CRMdig/L43i_is_annotated_by> a rdf:Property ;
    rdfs:domain <http://www.cidoc-crm.org/cidoc-crm/E1_CRM_Entity> ;
    rdfs:range <http://www.ics.forth.gr/isl/CRMdig/D29_Annotation_Object> .

<http://www.ics.forth.gr/isl/CRMdig/L47_has_comment> a rdf:Property ;
    rdfs:comment "This property is a specialisation of P3 has note and associates a comment with an instance of an object E1 CRM Entity."@en ;
    rdfs:domain <http://www.cidoc-crm.org/cidoc-crm/E1_CRM_Entity> ;
    rdfs:range rdfs:Literal ;
    rdfs:subPropertyOf <http://www.cidoc-crm.org/cidoc-crm/P3_has_note> .

<http://www.ics.forth.gr/isl/CRMdig/L48_created_annotation> a rdf:Property ;
    rdfs:comment """This property identifies the D29 Annotation Object (associations) that came into existence as a result of a D30 Annotation Event.
This property is a specialisation of P94 has created."""@en ;
    rdfs:domain <http://www.ics.forth.gr/isl/CRMdig/D30_Annotation_Event> ;
    rdfs:range <http://www.ics.forth.gr/isl/CRMdig/D29_Annotation_Object> ;
    rdfs:subPropertyOf <http://www.cidoc-crm.org/cidoc-crm/P94_has_created> .

<http://www.ics.forth.gr/isl/CRMdig/L48i_was_annotation_created_by> a rdf:Property ;
    rdfs:domain <http://www.ics.forth.gr/isl/CRMdig/D29_Annotation_Object> ;
    rdfs:range <http://www.ics.forth.gr/isl/CRMdig/D30_Annotation_Event> ;
    rdfs:subPropertyOf <http://www.cidoc-crm.org/cidoc-crm/P94i_was_created_by> .

<http://www.ics.forth.gr/isl/CRMdig/L49_is_primary_area_of> a rdf:Property ;
    rdfs:comment """This property describes the association between a particular area declared in an original digital object.
This property is a specialisation of P106 is composed of."""@en ;
    rdfs:domain <http://www.ics.forth.gr/isl/CRMdig/D35_Area> ;
    rdfs:range <http://www.ics.forth.gr/isl/CRMdig/D1_Digital_Object> ;
    rdfs:subPropertyOf <http://www.cidoc-crm.org/cidoc-crm/P106i_forms_part_of> .

<http://www.ics.forth.gr/isl/CRMdig/L49i_has_primary_area> a rdf:Property ;
    rdfs:domain <http://www.ics.forth.gr/isl/CRMdig/D1_Digital_Object> ;
    rdfs:range <http://www.ics.forth.gr/isl/CRMdig/D35_Area> ;
    rdfs:subPropertyOf <http://www.cidoc-crm.org/cidoc-crm/P106_is_composed_of> .

<http://www.ics.forth.gr/isl/CRMdig/L50_is_propagated_area_of> a rdf:Property ;
    rdfs:comment """This property describes the association between an area and the digital object to which it is propagated.
This property is a specialisation of P106 is composed of."""@en ;
    rdfs:domain <http://www.ics.forth.gr/isl/CRMdig/D35_Area> ;
    rdfs:range <http://www.ics.forth.gr/isl/CRMdig/D1_Digital_Object> ;
    rdfs:subPropertyOf <http://www.cidoc-crm.org/cidoc-crm/P106i_forms_part_of> .

<http://www.ics.forth.gr/isl/CRMdig/L50i_has_propagated_area> a rdf:Property ;
    rdfs:domain <http://www.ics.forth.gr/isl/CRMdig/D1_Digital_Object> ;
    rdfs:range <http://www.ics.forth.gr/isl/CRMdig/D35_Area> ;
    rdfs:subPropertyOf <http://www.cidoc-crm.org/cidoc-crm/P106_is_composed_of> .

<http://www.ics.forth.gr/isl/CRMdig/L51_has_first_name> a rdf:Property ;
    rdfs:comment "This property defines a personal name used to identify a person."@en ;
    rdfs:domain <http://www.ics.forth.gr/isl/CRMdig/D21_Person_Name> ;
    rdfs:range rdfs:Literal ;
    rdfs:subPropertyOf rdfs:label .

<http://www.ics.forth.gr/isl/CRMdig/L52_has_last_name> a rdf:Property ;
    rdfs:comment """This property defines the last name used to identify a person.
This property is a specialisation of L4 has preferred label."""@en ;
    rdfs:domain <http://www.ics.forth.gr/isl/CRMdig/D21_Person_Name> ;
    rdfs:range rdfs:Literal ;
    rdfs:subPropertyOf <http://www.ics.forth.gr/isl/CRMdig/L4_has_preferred_label> .

<http://www.ics.forth.gr/isl/CRMdig/L54_is_same-as> a rdf:Property ;
    rdfs:comment """This property describes the association kind of "same as" between objects. It is used to declare that two or more objects are
exactly the same."""@en ;
    rdfs:domain <http://www.cidoc-crm.org/cidoc-crm/E1_CRM_Entity> ;
    rdfs:range <http://www.cidoc-crm.org/cidoc-crm/E1_CRM_Entity> .

<http://www.ics.forth.gr/isl/CRMdig/L54i_is_same-as> a rdf:Property ;
    rdfs:comment """This property describes the association kind of "same as" between objects. It is used to declare that two or more objects are
exactly the same."""@en ;
    rdfs:domain <http://www.cidoc-crm.org/cidoc-crm/E1_CRM_Entity> ;
    rdfs:range <http://www.cidoc-crm.org/cidoc-crm/E1_CRM_Entity> .

<http://www.ics.forth.gr/isl/CRMdig/L55_has_inventory_no> a rdf:Property ;
    rdfs:comment """This property records the inventory number that was used to identify an instance of E1 CRM Entity 
at the time this property was record. This property is a specialisation of L53F is not uniquely identified by."""@en ;
    rdfs:domain <http://www.cidoc-crm.org/cidoc-crm/E1_CRM_Entity> ;
    rdfs:range rdfs:Literal ;
    rdfs:subPropertyOf <http://www.ics.forth.gr/isl/CRMdig/L53_is_not_uniquely_identified_by> .

<http://www.ics.forth.gr/isl/CRMdig/L56_has_pixel_width> a rdf:Property ;
    rdfs:comment """This property records the pixel width of the data object; it approximates a dimension that is 
part of the image data analysis.This property is a specialisation of P90 has value."""@en ;
    rdfs:domain <http://www.ics.forth.gr/isl/CRMdig/D9_Data_Object> ;
    rdfs:range rdfs:Literal ;
    rdfs:subPropertyOf <http://www.cidoc-crm.org/cidoc-crm/P90_has_value> .

<http://www.ics.forth.gr/isl/CRMdig/L57_has_pixel_height> a rdf:Property ;
    rdfs:comment """This property records the pixel height of the data object; it approximates a dimension that is 
part of the image data analysis.This property is a specialisation of P90 has value."""@en ;
    rdfs:domain <http://www.ics.forth.gr/isl/CRMdig/D9_Data_Object> ;
    rdfs:range rdfs:Literal ;
    rdfs:subPropertyOf <http://www.cidoc-crm.org/cidoc-crm/P90_has_value> .

<http://www.ics.forth.gr/isl/CRMdig/L59_has_serial_number> a rdf:Property ;
    rdfs:comment """This property records the serial number that was assigned to identify an instance of E22 Man Made Object.
 This property is a specialisation of L53 is not uniquely identified by."""@en ;
    rdfs:domain <http://www.cidoc-crm.org/cidoc-crm/E22_Man-Made_Object> ;
    rdfs:range rdfs:Literal ;
    rdfs:subPropertyOf <http://www.ics.forth.gr/isl/CRMdig/L53_is_not_uniquely_identified_by> .

<http://www.ics.forth.gr/isl/CRMdig/L60_documents> a rdf:Property ;
    rdfs:comment """This property describes the CRM Entities documented by instances of Digitization Processes.
This property is a specialisation of P140 assigned attribute to."""@en ;
    rdfs:domain <http://www.ics.forth.gr/isl/CRMdig/D2_Digitization_Process> ;
    rdfs:range <http://www.cidoc-crm.org/cidoc-crm/E1_CRM_Entity> ;
    rdfs:subPropertyOf <http://www.cidoc-crm.org/cidoc-crm/P140_assigned_attribute_to> .

<http://www.ics.forth.gr/isl/CRMdig/L60i_is_documented_by> a rdf:Property ;
    rdfs:domain <http://www.cidoc-crm.org/cidoc-crm/E1_CRM_Entity> ;
    rdfs:range <http://www.ics.forth.gr/isl/CRMdig/D2_Digitization_Process> ;
    rdfs:subPropertyOf <http://www.cidoc-crm.org/cidoc-crm/P140i_was_attributed_by> .

<http://www.ics.forth.gr/isl/CRMdig/L61_was_ongoing_at> a rdf:Property ;
    rdfs:comment """This property describes the minimum period of time covered by a digital machine event. It 
identifies the minimum extent of the event. This property is a specialisation of P81 ongoing throughout."""@en ;
    rdfs:domain <http://www.cidoc-crm.org/cidoc-crm/E5_Event> ;
    rdfs:range xsd:dateTime ;
    rdfs:subPropertyOf <http://www.cidoc-crm.org/cidoc-crm/P81a_end_of_the_begin>,
        <http://www.cidoc-crm.org/cidoc-crm/P81b_begin_of_the_end> .

<http://www.ics.forth.gr/isl/CRMgeo/Q10_defines_place> a rdf:Property ;
    rdfs:comment "Scope note:	This property associates an instance of SP5 Geometric Place Expression with the instance of SP6 Declarative Place it defines. Syntactic variants or use of different scripts may result in multiple instances of SP5 Geometric Place Expression defining exactly the same place. Transformations between different reference systems in general result in new definitions of places approximating each other."^^xsd:string ;
    rdfs:domain <http://www.ics.forth.gr/isl/CRMgeo/SP5_Geometric_Place_Expression> ;
    rdfs:range <http://www.ics.forth.gr/isl/CRMgeo/SP6_Declarative_Place> ;
    rdfs:subPropertyOf <http://www.cidoc-crm.org/cidoc-crm/P87i_identifies> .

<http://www.ics.forth.gr/isl/CRMgeo/Q11_approximates> a rdf:Property ;
    rdfs:comment "Scope note:	This property approximates a phenomenal place which is defined in the same reference space. The property does not state the quality or accuracy of the approximation, but an overlap in area is the minimal requirement."^^xsd:string ;
    rdfs:domain <http://www.ics.forth.gr/isl/CRMgeo/SP6_Declarative_Place> ;
    rdfs:range <http://www.cidoc-crm.org/cidoc-crm/E53_Place> ;
    rdfs:subPropertyOf <http://www.cidoc-crm.org/cidoc-crm/P121_overlaps_with> .

<http://www.ics.forth.gr/isl/CRMgeo/Q11i_is_approximated_by> a rdf:Property ;
    rdfs:domain <http://www.cidoc-crm.org/cidoc-crm/E53_Place> ;
    rdfs:range <http://www.ics.forth.gr/isl/CRMgeo/SP6_Declarative_Place> ;
    rdfs:subPropertyOf <http://www.cidoc-crm.org/cidoc-crm/P121_overlaps_with> .

<http://www.ics.forth.gr/isl/CRMgeo/Q12_approximates> a rdf:Property ;
    rdfs:comment "Scope note:	This property approximates a SP8 Spacetime Volume. The property does not state the quality or accuracy of the approximation, but an overlap of the spacetime volume is the minimal requirement."^^xsd:string ;
    rdfs:domain <http://www.ics.forth.gr/isl/CRMgeo/SP7_Declarative_Spacetime_Volume> ;
    rdfs:range <http://www.cidoc-crm.org/cidoc-crm/E92_Spacetime_Volume> .

<http://www.ics.forth.gr/isl/CRMgeo/Q12i_approximates> a rdf:Property ;
    rdfs:domain <http://www.cidoc-crm.org/cidoc-crm/E92_Spacetime_Volume> ;
    rdfs:range <http://www.ics.forth.gr/isl/CRMgeo/SP7_Declarative_Spacetime_Volume> .

<http://www.ics.forth.gr/isl/CRMgeo/Q13_approximates> a rdf:Property ;
    rdfs:comment "Scope note:	This property approximates a SP9 Time Intervall. The property does not state the quality or accuracy of the approximation, but an overlap in time is the minimal requirement."^^xsd:string ;
    rdfs:domain <http://www.ics.forth.gr/isl/CRMgeo/SP10_Declarative_Time-Span> ;
    rdfs:range <http://www.cidoc-crm.org/cidoc-crm/E52_Time-Span> .

<http://www.ics.forth.gr/isl/CRMgeo/Q13i_approximates> a rdf:Property ;
    rdfs:domain <http://www.cidoc-crm.org/cidoc-crm/E52_Time-Span> ;
    rdfs:range <http://www.ics.forth.gr/isl/CRMgeo/SP10_Declarative_Time-Span> .

<http://www.ics.forth.gr/isl/CRMgeo/Q14_defines_time> a rdf:Property ;
    rdfs:comment "Scope note:	This property associates an instance of SP14 Time Expression with the instance of SP10 Declarative Time Span it defines. Syntactic variants or use of different scripts may result in multiple instances of SP14 Time Expression defining exactly the same time span. Transformations between different temporal reference systems in general result in new definitions of time spans approximating each other."^^xsd:string ;
    rdfs:domain <http://www.ics.forth.gr/isl/CRMgeo/SP14_Time_Expression> ;
    rdfs:range <http://www.ics.forth.gr/isl/CRMgeo/SP10_Declarative_Time-Span> .

<http://www.ics.forth.gr/isl/CRMgeo/Q14i_defines_time> a rdf:Property ;
    rdfs:domain <http://www.ics.forth.gr/isl/CRMgeo/SP10_Declarative_Time-Span> ;
    rdfs:range <http://www.ics.forth.gr/isl/CRMgeo/SP14_Time_Expression> .

<http://www.ics.forth.gr/isl/CRMgeo/Q15_is_expressed_in_terms_of> a rdf:Property ;
    rdfs:comment "Scope note:	This property defines the temporal reference system in terms of which an SP14 Time Expression is formulated."^^xsd:string ;
    rdfs:domain <http://www.ics.forth.gr/isl/CRMgeo/SP14_Time_Expression> ;
    rdfs:range <http://www.ics.forth.gr/isl/CRMgeo/SP11_Temporal_Reference_System> .

<http://www.ics.forth.gr/isl/CRMgeo/Q15i_is_expressed_in_terms_of> a rdf:Property ;
    rdfs:domain <http://www.ics.forth.gr/isl/CRMgeo/SP11_Temporal_Reference_System> ;
    rdfs:range <http://www.ics.forth.gr/isl/CRMgeo/SP14_Time_Expression> .

<http://www.ics.forth.gr/isl/CRMgeo/Q16_defines_spacetime_volume> a rdf:Property ;
    rdfs:comment "Scope note:	This property associates an instance of SP12 Spacetime Volume Expression with the instance of SP7 Declarative Spacetime Volume it defines. Syntactic variants or use of different scripts may result in multiple instances of SP12 Spacetime Volume Expressions defining exactly the same SP7 Declarative Spacetime Volume. Transformations between different temporal or spatial reference systems in general result in new definitions of Spacetime Volumes approximating each other."^^xsd:string ;
    rdfs:domain <http://www.ics.forth.gr/isl/CRMgeo/SP12_Spacetime_Volume_Expression> ;
    rdfs:range <http://www.ics.forth.gr/isl/CRMgeo/SP7_Declarative_Spacetime_Volume> .

<http://www.ics.forth.gr/isl/CRMgeo/Q16i_defines_spacetime_volume> a rdf:Property ;
    rdfs:domain <http://www.ics.forth.gr/isl/CRMgeo/SP7_Declarative_Spacetime_Volume> ;
    rdfs:range <http://www.ics.forth.gr/isl/CRMgeo/SP12_Spacetime_Volume_Expression> .

<http://www.ics.forth.gr/isl/CRMgeo/Q17_is_expressed_in_terms_of> a rdf:Property ;
    rdfs:comment "Scope note:	This property defines the temporal reference system in terms of which a SP12 Spacetime Volume Expression is formulated."^^xsd:string ;
    rdfs:domain <http://www.ics.forth.gr/isl/CRMgeo/SP12_Spacetime_Volume_Expression> ;
    rdfs:range <http://www.ics.forth.gr/isl/CRMgeo/SP11_Temporal_Reference_System> .

<http://www.ics.forth.gr/isl/CRMgeo/Q17i_is_expressed_in_terms_of> a rdf:Property ;
    rdfs:domain <http://www.ics.forth.gr/isl/CRMgeo/SP11_Temporal_Reference_System> ;
    rdfs:range <http://www.ics.forth.gr/isl/CRMgeo/SP12_Spacetime_Volume_Expression> .

<http://www.ics.forth.gr/isl/CRMgeo/Q18_is_expressed_in_terms_of> a rdf:Property ;
    rdfs:comment "Scope note:	This property defines the spatial coordinate reference system in terms of which a SP12 Spacetime Volume Expression is formulated."^^xsd:string ;
    rdfs:domain <http://www.ics.forth.gr/isl/CRMgeo/SP12_Spacetime_Volume_Expression> ;
    rdfs:range <http://www.ics.forth.gr/isl/CRMgeo/SP4_Spatial_Coordinate_Reference_System> .

<http://www.ics.forth.gr/isl/CRMgeo/Q18i_is_expressed_in_terms_of> a rdf:Property ;
    rdfs:domain <http://www.ics.forth.gr/isl/CRMgeo/SP4_Spatial_Coordinate_Reference_System> ;
    rdfs:range <http://www.ics.forth.gr/isl/CRMgeo/SP12_Spacetime_Volume_Expression> .

<http://www.ics.forth.gr/isl/CRMgeo/Q19_has_reference_event> a rdf:Property ;
    rdfs:domain <http://www.ics.forth.gr/isl/CRMgeo/SP11_Temporal_Reference_System> ;
    rdfs:range <http://www.cidoc-crm.org/cidoc-crm/E5_Event> .

<http://www.ics.forth.gr/isl/CRMgeo/Q19i_has_reference_event> a rdf:Property ;
    rdfs:domain <http://www.cidoc-crm.org/cidoc-crm/E5_Event> ;
    rdfs:range <http://www.ics.forth.gr/isl/CRMgeo/SP11_Temporal_Reference_System> .

<http://www.ics.forth.gr/isl/CRMgeo/Q1_occupied> a rdf:Property ;
    rdfs:comment "Scope note:	This property associates an instance of E4 Period with the 4 dimensional point sets (volumes) in spacetime that it occupied. This instance of SP1 Phenomenal Spacetime Volume includes the trajectories of the participating physical things during their participation in the instance of E4 Period, the open spaces via which they have interacted and the spaces by which they had the potential to interact during that period or event in the way defined by the type of the respective period or event, such as the air in a meeting room transferring the voices. It also comprises the areas controlled by some military power. Therefore instances of E4 Period have fuzzy boundaries in spacetime."^^xsd:string ;
    rdfs:domain <http://www.cidoc-crm.org/cidoc-crm/E4_Period> ;
    rdfs:range <http://www.ics.forth.gr/isl/CRMgeo/SP1_Phenomenal_Spacetime_Volume> ;
    rdfs:subClassOf geo:Feature .

<http://www.ics.forth.gr/isl/CRMgeo/Q1i_is_occupied_by> a rdf:Property ;
    rdfs:domain <http://www.ics.forth.gr/isl/CRMgeo/SP1_Phenomenal_Spacetime_Volume> ;
    rdfs:range <http://www.cidoc-crm.org/cidoc-crm/E4_Period> ;
    rdfs:subClassOf geo:Feature .

<http://www.ics.forth.gr/isl/CRMgeo/Q2_occupied> a rdf:Property ;
    rdfs:comment "Scope note:	This property describes the 4 dimensional point sets (volumes) in spacetime that the trajectory of an instance of E18 Physical Thing occupies in spacetime in the course of its existence. We include in the occupied space the space filled by the matter of the physical thing and all inner spaces not accessible in regular function."^^xsd:string ;
    rdfs:domain <http://www.cidoc-crm.org/cidoc-crm/E18_Physical_Thing> ;
    rdfs:range <http://www.ics.forth.gr/isl/CRMgeo/SP1_Phenomenal_Spacetime_Volume> .

<http://www.ics.forth.gr/isl/CRMgeo/Q2i_is_occupied_by> a rdf:Property ;
    rdfs:domain <http://www.ics.forth.gr/isl/CRMgeo/SP1_Phenomenal_Spacetime_Volume> ;
    rdfs:range <http://www.cidoc-crm.org/cidoc-crm/E18_Physical_Thing> .

<http://www.ics.forth.gr/isl/CRMgeo/Q3_has_temporal_projection> a rdf:Property ;
    rdfs:comment "Scope note: 	This property describes the temporal projection of an instance of a SP1 Phenomenal Spacetime Volume. The property P4 has time-span is a shortcut of the more fully developed path from E4 Period through Q1 occupied, SP1 Phenomenal Spacetime Volume Q3 has temporal projection to E52 Time Span."^^xsd:string ;
    rdfs:domain <http://www.ics.forth.gr/isl/CRMgeo/SP1_Phenomenal_Spacetime_Volume> ;
    rdfs:range <http://www.ics.forth.gr/isl/CRMgeo/SP13_Phenomenal_Time-Span> .

<http://www.ics.forth.gr/isl/CRMgeo/Q3i_is_temporal_projection> a rdf:Property ;
    rdfs:domain <http://www.ics.forth.gr/isl/CRMgeo/SP13_Phenomenal_Time-Span> ;
    rdfs:range <http://www.ics.forth.gr/isl/CRMgeo/SP1_Phenomenal_Spacetime_Volume> .

<http://www.ics.forth.gr/isl/CRMgeo/Q4_has_spatial_projection> a rdf:Property ;
    rdfs:comment """Scope note:	This property describes the spatial projection of an instance of a SP1 Phenomenal Spacetime Volume on an instance of SP2 Phenomenal Place. Even though the projection of a spacetime volume to one instance of SP3 Reference Space is unique, each reference space gives rise to another projection. The projections overlap at the time of the spacetime volume, the respective instances of SP2 Phenomenal Place may later drift apart, or earlier be yet apart.
The property P7 took place at is a shortcut of the more fully developed path from E4 Period through Q1 occupied, SP1 Phenomenal Spacetime Volume Q4 has spatial projection to SP2 Phenomenal Place."""^^xsd:string ;
    rdfs:domain <http://www.ics.forth.gr/isl/CRMgeo/SP1_Phenomenal_Spacetime_Volume> ;
    rdfs:range <http://www.ics.forth.gr/isl/CRMgeo/SP2_Phenomenal_Place> .

<http://www.ics.forth.gr/isl/CRMgeo/Q4i_is_spatial_projection> a rdf:Property ;
    rdfs:comment "i of"^^xsd:string ;
    rdfs:domain <http://www.ics.forth.gr/isl/CRMgeo/SP2_Phenomenal_Place> ;
    rdfs:range <http://www.ics.forth.gr/isl/CRMgeo/SP1_Phenomenal_Spacetime_Volume> .

<http://www.ics.forth.gr/isl/CRMgeo/Q5_defined_in> a rdf:Property ;
    rdfs:comment "Scope note:	This property associates an instance of  E53 Place with the instance of  SP3 Reference Space it is defined in."^^xsd:string ;
    rdfs:domain <http://www.cidoc-crm.org/cidoc-crm/E53_Place> ;
    rdfs:range <http://www.ics.forth.gr/isl/CRMgeo/SP3_Reference_Space> .

<http://www.ics.forth.gr/isl/CRMgeo/Q5i_defined_in> a rdf:Property ;
    rdfs:domain <http://www.ics.forth.gr/isl/CRMgeo/SP3_Reference_Space> ;
    rdfs:range <http://www.cidoc-crm.org/cidoc-crm/E53_Place> .

<http://www.ics.forth.gr/isl/CRMgeo/Q6_is_at_rest_in_relation_to> a rdf:Property ;
    rdfs:comment "Scope note:	This property associates an instance of SP3 Reference Space with the instance of E18 Physical Thing that is at rest in it. For all instances of E18 Physical Thing exist at least one reference space it is at rest with because of their relative stability of form. Larger constellations of matter may comprise many physical features that are at rest with them."^^xsd:string ;
    rdfs:domain <http://www.ics.forth.gr/isl/CRMgeo/SP3_Reference_Space> ;
    rdfs:range <http://www.cidoc-crm.org/cidoc-crm/E18_Physical_Thing> ;
    rdfs:subClassOf geo:Feature .

<http://www.ics.forth.gr/isl/CRMgeo/Q6i_rests_in_relation_to> a rdf:Property ;
    rdfs:domain <http://www.cidoc-crm.org/cidoc-crm/E18_Physical_Thing> ;
    rdfs:range <http://www.ics.forth.gr/isl/CRMgeo/SP3_Reference_Space> ;
    rdfs:subClassOf geo:Feature .

<http://www.ics.forth.gr/isl/CRMgeo/Q7_describes> a rdf:Property ;
    rdfs:comment "Scope note:	This property associates an instance of SP4 Spatial Coordinate Reference System with the instance of SP3 Reference Space for which it can be used to describe locations."^^xsd:string ;
    rdfs:domain <http://www.ics.forth.gr/isl/CRMgeo/SP4_Spatial_Coordinate_Reference_System> ;
    rdfs:range <http://www.ics.forth.gr/isl/CRMgeo/SP3_Reference_Space> .

<http://www.ics.forth.gr/isl/CRMgeo/Q7i_is_described_by> a rdf:Property ;
    rdfs:domain <http://www.ics.forth.gr/isl/CRMgeo/SP3_Reference_Space> ;
    rdfs:range <http://www.ics.forth.gr/isl/CRMgeo/SP4_Spatial_Coordinate_Reference_System> .

<http://www.ics.forth.gr/isl/CRMgeo/Q8_is_fixed_on> a rdf:Property ;
    rdfs:comment """Scope note:	This property defines the physical reference features that ground a spatial coordinate reference system in the real world. 
In surveying and geodesy this is part of the datum definition and is often a point identified by a physical feature on earth (sometimes monuments) where the earth approximation ellipsoid touches the earth and one axis of the ellipsoid runs through."""^^xsd:string ;
    rdfs:domain <http://www.ics.forth.gr/isl/CRMgeo/SP4_Spatial_Coordinate_Reference_System> ;
    rdfs:range <http://www.cidoc-crm.org/cidoc-crm/E26_Physical_Feature> .

<http://www.ics.forth.gr/isl/CRMgeo/Q8i_fixes> a rdf:Property ;
    rdfs:domain <http://www.cidoc-crm.org/cidoc-crm/E26_Physical_Feature> ;
    rdfs:range <http://www.ics.forth.gr/isl/CRMgeo/SP4_Spatial_Coordinate_Reference_System> .

<http://www.ics.forth.gr/isl/CRMgeo/Q9_is_expressed_in_terms_of> a rdf:Property ;
    rdfs:comment "Scope note:	This property defines the coordinate reference system in terms of which a geometric place expression is formulated."^^xsd:string ;
    rdfs:domain <http://www.ics.forth.gr/isl/CRMgeo/SP5_Geometric_Place_Expression> ;
    rdfs:range <http://www.ics.forth.gr/isl/CRMgeo/SP4_Spatial_Coordinate_Reference_System> .

<http://www.ics.forth.gr/isl/CRMgeo/Q9i_terms_express> a rdf:Property ;
    rdfs:domain <http://www.ics.forth.gr/isl/CRMgeo/SP4_Spatial_Coordinate_Reference_System> ;
    rdfs:range <http://www.ics.forth.gr/isl/CRMgeo/SP5_Geometric_Place_Expression> .

<http://www.ics.forth.gr/isl/CRMgeo/asGML> a rdf:Property ;
    rdfs:comment "Scope note:	"^^xsd:string ;
    rdfs:domain geo:Geometry ;
    rdfs:range geo:gmlLiteral ;
    rdfs:subPropertyOf <http://www.ics.forth.gr/isl/CRMgeo/Q10i_place_is_defined_by> .

<http://www.ics.forth.gr/isl/CRMgeo/asWKT> a rdf:Property ;
    rdfs:comment "Scope note:	"^^xsd:string ;
    rdfs:domain geo:Geometry ;
    rdfs:range geo:wktLiteral ;
    rdfs:subPropertyOf <http://www.ics.forth.gr/isl/CRMgeo/Q10i_place_is_defined_by> .

<http://www.ics.forth.gr/isl/CRMinf/J1_used_as_premise> a rdf:Property ;
    rdfs:comment """
            This property associates an instance of I2 Belief with the instance of I5 Inference Making that used it as a premise.
		"""@en ;
    rdfs:domain <http://www.ics.forth.gr/isl/CRMinf/I5_Inference_Making> ;
    rdfs:range <http://www.ics.forth.gr/isl/CRMinf/I2_Belief> ;
    rdfs:subPropertyOf <http://www.cidoc-crm.org/cidoc-crm/P17_was_motivated_by> .

<http://www.ics.forth.gr/isl/CRMinf/J1i_was_premise_for> a rdf:Property ;
    rdfs:domain <http://www.ics.forth.gr/isl/CRMinf/I2_Belief> ;
    rdfs:range <http://www.ics.forth.gr/isl/CRMinf/I5_Inference_Making> ;
    rdfs:subPropertyOf <http://www.cidoc-crm.org/cidoc-crm/P17i_motivated> .

<http://www.ics.forth.gr/isl/CRMinf/J2_concluded_that> a rdf:Property ;
    rdfs:comment """
            This property associates an instance of I2 Belief with the instance of I1 Argumentation that concluded it.
		"""@en ;
    rdfs:domain <http://www.ics.forth.gr/isl/CRMinf/I1_Argumentation> ;
    rdfs:range <http://www.ics.forth.gr/isl/CRMinf/I2_Belief> ;
    rdfs:subPropertyOf <http://www.cidoc-crm.org/cidoc-crm/P116_starts> .

<http://www.ics.forth.gr/isl/CRMinf/J2i_was_concluded_by> a rdf:Property ;
    rdfs:domain <http://www.ics.forth.gr/isl/CRMinf/I2_Belief> ;
    rdfs:range <http://www.ics.forth.gr/isl/CRMinf/I1_Argumentation> ;
    rdfs:subPropertyOf <http://www.cidoc-crm.org/cidoc-crm/P116i_is_started_by> .

<http://www.ics.forth.gr/isl/CRMinf/J3_applies> a rdf:Property ;
    rdfs:comment """
            This property associates an instance of I3 Inference Logic with the instance of I5 Inference Making that used it to draw its conclusion.
		"""@en ;
    rdfs:domain <http://www.ics.forth.gr/isl/CRMinf/I5_Inference_Making> ;
    rdfs:range <http://www.ics.forth.gr/isl/CRMinf/I3_Inference_Logic> ;
    rdfs:subPropertyOf <http://www.cidoc-crm.org/cidoc-crm/P16_used_specific_object> .

<http://www.ics.forth.gr/isl/CRMinf/J3i_was_applied_by> a rdf:Property ;
    rdfs:domain <http://www.ics.forth.gr/isl/CRMinf/I3_Inference_Logic> ;
    rdfs:range <http://www.ics.forth.gr/isl/CRMinf/I5_Inference_Making> ;
    rdfs:subPropertyOf <http://www.cidoc-crm.org/cidoc-crm/P16i_was_used_for> .

<http://www.ics.forth.gr/isl/CRMinf/J4_that> a rdf:Property ;
    rdfs:comment """
            This property associates an instance of I4 Proposition Set with the instance of I2 Belief that holds an opinion about it.
		"""@en ;
    rdfs:domain <http://www.ics.forth.gr/isl/CRMinf/I2_Belief> ;
    rdfs:range <http://www.ics.forth.gr/isl/CRMinf/I4_Proposition_Set> .

<http://www.ics.forth.gr/isl/CRMinf/J4i_is_subject_of> a rdf:Property ;
    rdfs:domain <http://www.ics.forth.gr/isl/CRMinf/I4_Proposition_Set> ;
    rdfs:range <http://www.ics.forth.gr/isl/CRMinf/I2_Belief> .

<http://www.ics.forth.gr/isl/CRMinf/J5_holds_to_be> a rdf:Property ;
    rdfs:domain <http://www.ics.forth.gr/isl/CRMinf/I2_Belief> ;
    rdfs:range rdfs:Literal ;
    rdfs:subPropertyOf <http://www.ics.forth.gr/isl/CRMinf/O2_removed> .

<http://www.ics.forth.gr/isl/CRMinf/J6_adopted> a rdf:Property ;
    rdfs:comment """
            This property associates an instance of I2 Belief with the instance of I7 Belief Adoption that used it as the source of the I6 Belief Value and propositions used in the resulting new I2 Belief.
		"""@en ;
    rdfs:domain <http://www.ics.forth.gr/isl/CRMinf/I7_Belief_Adoption> ;
    rdfs:range <http://www.ics.forth.gr/isl/CRMinf/I2_Belief> ;
    rdfs:subPropertyOf <http://www.cidoc-crm.org/cidoc-crm/P17_was_motivated_by> .

<http://www.ics.forth.gr/isl/CRMinf/J6i_adopted_by> a rdf:Property ;
    rdfs:domain <http://www.ics.forth.gr/isl/CRMinf/I2_Belief> ;
    rdfs:range <http://www.ics.forth.gr/isl/CRMinf/I7_Belief_Adoption> ;
    rdfs:subPropertyOf <http://www.cidoc-crm.org/cidoc-crm/P17i_motivated> .

<http://www.ics.forth.gr/isl/CRMinf/J7_is_based_on_evidence> a rdf:Property ;
    rdfs:comment """
		This property associates an instance of I7 Belief Adoption with the instance of E73 Information Object that was the source of or evidence for the I4 Proposition Set that was adopted.
		"""@en ;
    rdfs:domain <http://www.ics.forth.gr/isl/CRMinf/I7_Belief_Adoption> ;
    rdfs:range <http://www.cidoc-crm.org/cidoc-crm/E73_Information_Object> ;
    rdfs:subPropertyOf <http://www.cidoc-crm.org/cidoc-crm/P16_used_specific_object> .

<http://www.ics.forth.gr/isl/CRMinf/J7i_is_evidence_for> a rdf:Property ;
    rdfs:domain <http://www.cidoc-crm.org/cidoc-crm/E73_Information_Object> ;
    rdfs:range <http://www.ics.forth.gr/isl/CRMinf/I7_Belief_Adoption> ;
    rdfs:subPropertyOf <http://www.cidoc-crm.org/cidoc-crm/P16i_was_used_for> .

<https://ontology.swissartresearch.net/aaao/ZP100_challenged> a rdf:Property ;
    rdfs:label "challenged"@en ;
    rdfs:comment "This property links an instance of symbolic act with an instance of institutional fact which it challenges through its performance."@en ;
    rdfs:domain <https://ontology.swissartresearch.net/aaao/ZE53_Symbolic_Act> ;
    rdfs:range <https://ontology.swissartresearch.net/aaao/ZE1_Institutional_Fact> ;
    skos:notation "ZP100"^^xsd:string .

<https://ontology.swissartresearch.net/aaao/ZP100i_was_challenged_by> a rdf:Property ;
    rdfs:label "was challenged by"@en ;
    rdfs:comment "This property is the inverse of the forward property described in the scope note that follows. This property links an instance of symbolic act with an instance of institutional fact which it challenges through its performance."@en ;
    rdfs:domain <https://ontology.swissartresearch.net/aaao/ZE1_Institutional_Fact> ;
    rdfs:range <https://ontology.swissartresearch.net/aaao/ZE53_Symbolic_Act> ;
    skos:notation "ZP100i"^^xsd:string .

<https://ontology.swissartresearch.net/aaao/ZP101_affirmed> a rdf:Property ;
    rdfs:label "affirmed"@en ;
    rdfs:comment "This property links an instance of symbolic act with an instance of institutional fact which it affirms through its performance."@en ;
    rdfs:domain <https://ontology.swissartresearch.net/aaao/ZE53_Symbolic_Act> ;
    rdfs:range <https://ontology.swissartresearch.net/aaao/ZE1_Institutional_Fact> ;
    skos:notation "ZP101"^^xsd:string .

<https://ontology.swissartresearch.net/aaao/ZP101i_was_affirmed_by> a rdf:Property ;
    rdfs:label "was affirmed by"@en ;
    rdfs:comment "This property is the inverse of the forward property described in the scope note that follows. This property links an instance of symbolic act with an instance of institutional fact which it affirms through its performance."@en ;
    rdfs:domain <https://ontology.swissartresearch.net/aaao/ZE1_Institutional_Fact> ;
    rdfs:range <https://ontology.swissartresearch.net/aaao/ZE53_Symbolic_Act> ;
    skos:notation "ZP101i"^^xsd:string .

<https://ontology.swissartresearch.net/aaao/ZP103i_is_social_relation_target_ascribed_by> a rdf:Property ;
    rdfs:label "is social relation target ascribed by"@en ;
    rdfs:comment "This property is the inverse of the forward property described in the scope note that follows. This property is used to indicate the person with whom the subject of the social relation status has the social relation which they have."@en ;
    rdfs:domain <http://www.cidoc-crm.org/cidoc-crm/E39_Actor> ;
    rdfs:range <https://ontology.swissartresearch.net/aaao/ZE55_Social_Relation_Status> ;
    rdfs:subPropertyOf <https://ontology.swissartresearch.net/aaao/ZP2i_is_intentional_target_ascribed_by> ;
    skos:notation "ZP103i"^^xsd:string .

<https://ontology.swissartresearch.net/aaao/ZP104i_is_social_relation_ascribed_by> a rdf:Property ;
    rdfs:label "is social relation ascribed by"@en ;
    rdfs:comment "This property is the inverse of the forward property described in the scope note that follows. This property is used to indicate the specific type of social relation status which is indicated as holding between the subject individual and their ascribed social relative."@en ;
    rdfs:domain <http://www.cidoc-crm.org/cidoc-crm/E55_Type> ;
    rdfs:range <https://ontology.swissartresearch.net/aaao/ZE55_Social_Relation_Status> ;
    rdfs:subPropertyOf <https://ontology.swissartresearch.net/aaao/ZP3i_is_intentional_relation_ascribed_by> ;
    skos:notation "ZP104i"^^xsd:string .

<https://ontology.swissartresearch.net/aaao/ZP105i_is_social_relation_subject_of> a rdf:Property ;
    rdfs:label "is social relation subject of"@en ;
    rdfs:comment "This property is the inverse of the forward property described in the scope note that follows. This property is used to indicate the person for whom the social relation status is taken to hold."@en ;
    rdfs:domain <http://www.cidoc-crm.org/cidoc-crm/E39_Actor> ;
    rdfs:range <https://ontology.swissartresearch.net/aaao/ZE55_Social_Relation_Status> ;
    rdfs:subPropertyOf <https://ontology.swissartresearch.net/aaao/ZP1i_is_intentional_subject_of> ;
    skos:notation "ZP105i"^^xsd:string .

<https://ontology.swissartresearch.net/aaao/ZP10_ascribes_contact_point_relation> a rdf:Property ;
    rdfs:label "ascribes contact point relation"@en ;
    rdfs:comment """This property is used to indicate the specific manner in which the contact point which is indicated as holding for the named subjectof the contact status pertains to this subject.
"""@en ;
    rdfs:domain <https://ontology.swissartresearch.net/aaao/ZE3_Contact_Point_Status> ;
    rdfs:range <http://www.cidoc-crm.org/cidoc-crm/E55_Type> ;
    rdfs:subPropertyOf <https://ontology.swissartresearch.net/aaao/ZP7_ascribes_appellative_relation> ;
    skos:notation "ZP10"^^xsd:string .

<https://ontology.swissartresearch.net/aaao/ZP10i_is_contact_point_relation_ascribed_by> a rdf:Property ;
    rdfs:label "is contact point relation ascribed by"@en ;
    rdfs:comment """This property is the inverse of the forward property described in the scope note that follows. This property is used to indicate the specific manner in which the contact point which is indicated as holding for the named subject  of the contact status pertains to this subject.
"""@en ;
    rdfs:domain <http://www.cidoc-crm.org/cidoc-crm/E55_Type> ;
    rdfs:range <https://ontology.swissartresearch.net/aaao/ZE3_Contact_Point_Status> ;
    rdfs:subPropertyOf <https://ontology.swissartresearch.net/aaao/ZP7i_is_appellative_relation_ascribed_by> ;
    skos:notation "ZP10i"^^xsd:string .

<https://ontology.swissartresearch.net/aaao/ZP111i_was_initiated_by> a rdf:Property ;
    rdfs:label "was initiated by"@en ;
    rdfs:comment "This property is the inverse of the forward property described in the scope note that follows. This property is used to connect the instance of event to the instance of institutional fact which it brought into existence by fiat thanks to its accordance to a socially defined norm. In this case the bringing about of a new institutional fact need not be intentional or following any particular rule intentionally. Rather, within a social context it is recognized that the very fact of a particular event occurring is causal to the initiation of the related social fact. For example, in certain property right laws, the very fact of writing down an idea (E65 Creation) initiates an instance of property right over the generated information object, regardless of the intention or not of the author to so create such a right."@en ;
    rdfs:domain <https://ontology.swissartresearch.net/aaao/ZE1_Institutional_Fact> ;
    rdfs:range <http://www.cidoc-crm.org/cidoc-crm/E5_Event> ;
    skos:notation "ZP111i"^^xsd:string .

<https://ontology.swissartresearch.net/aaao/ZP112i_was_terminated_by> a rdf:Property ;
    rdfs:label "was terminated by"@en ;
    rdfs:comment "This property is the inverse of the forward property described in the scope note that follows. This property is used to connect the instance of event to the instance of institutional fact which it terminated the existence of by fiat thanks to its accordance to a socially defined norm. In this case the cancellation of an institutional fact need not be intentional or following any particular rule intentionally. Rather, within a social context it is recognized that the very fact of a particular event occurring is causal to the cancellation of the related social fact. For example, a certain social system may recognize that an ''act of god'' such as an earthquake may terminate the property right of an individual over some object (another social system may not, however)."@en ;
    rdfs:domain <https://ontology.swissartresearch.net/aaao/ZE1_Institutional_Fact> ;
    rdfs:range <http://www.cidoc-crm.org/cidoc-crm/E5_Event> ;
    skos:notation "ZP112i"^^xsd:string .

<https://ontology.swissartresearch.net/aaao/ZP113_has_successor_status> a rdf:Property ;
    rdfs:label "has successor status"@en ;
    rdfs:comment "This property links one instance of institutional fact with another where the latter succeeds the former as a formal continuation."@en ;
    rdfs:domain <https://ontology.swissartresearch.net/aaao/ZE1_Institutional_Fact> ;
    rdfs:range <https://ontology.swissartresearch.net/aaao/ZE1_Institutional_Fact> ;
    skos:notation "ZP113"^^xsd:string .

<https://ontology.swissartresearch.net/aaao/ZP113i_is_successor_status_of> a rdf:Property ;
    rdfs:label "is successor status of"@en ;
    rdfs:comment "This property is the inverse of the forward property described in the scope note that follows. This property links one instance of institutional fact with another where the latter succeeds the former as a formal continuation."@en ;
    rdfs:domain <https://ontology.swissartresearch.net/aaao/ZE1_Institutional_Fact> ;
    rdfs:range <https://ontology.swissartresearch.net/aaao/ZE1_Institutional_Fact> ;
    skos:notation "ZP113i"^^xsd:string .

<https://ontology.swissartresearch.net/aaao/ZP114_has_geographic_scope> a rdf:Property ;
    rdfs:label "has geographic scope"@en ;
    rdfs:comment "This property is used to connect an institutional fact to a place, which defines the scope of that facts spatial validity."@en ;
    rdfs:domain <https://ontology.swissartresearch.net/aaao/ZE1_Institutional_Fact> ;
    rdfs:range <http://www.cidoc-crm.org/cidoc-crm/E53_Place> ;
    skos:notation "ZP114"^^xsd:string .

<https://ontology.swissartresearch.net/aaao/ZP114i_is_geographic_scope_of> a rdf:Property ;
    rdfs:label "is geographic scope of"@en ;
    rdfs:comment "This property is the inverse of the forward property described in the scope note that follows. This property is used to connect an institutional fact to a place, which defines the scope of that facts spatial validity."@en ;
    rdfs:domain <http://www.cidoc-crm.org/cidoc-crm/E53_Place> ;
    rdfs:range <https://ontology.swissartresearch.net/aaao/ZE1_Institutional_Fact> ;
    skos:notation "ZP114i"^^xsd:string .

<https://ontology.swissartresearch.net/aaao/ZP115_holds_over> a rdf:Property ;
    rdfs:label "holds over"@en ;
    rdfs:comment "This property associates and instance of institutional fact to an instance of population over which this fact holds. As opposed to the property of ZP4 holding for, the effect which this institutional fact holds in relation to the related population is not necessarily one which has been directly intended. The population undergoes the social fact instantiated, rather than causing it to occur directly through agency in a speech act or transformative act. The population is the patient of this operation, not its agent."@en ;
    rdfs:domain <https://ontology.swissartresearch.net/aaao/ZE1_Institutional_Fact> ;
    rdfs:range <https://ontology.swissartresearch.net/aaao/ZE37_Population> ;
    skos:notation "ZP115"^^xsd:string .

<https://ontology.swissartresearch.net/aaao/ZP115i_is_held_over_by> a rdf:Property ;
    rdfs:label "is held over by"@en ;
    rdfs:comment "This property is the inverse of the forward property described in the scope note that follows. This property associates and instance of institutional fact to an instance of population over which this fact holds. As opposed to the property of ZP4 holding for, the effect which this institutional fact holds in relation to the related population is not necessarily one which has been directly intended. The population undergoes the social fact instantiated, rather than causing it to occur directly through agency in a speech act or transformative act. The population is the patient of this operation, not its agent."@en ;
    rdfs:domain <https://ontology.swissartresearch.net/aaao/ZE37_Population> ;
    rdfs:range <https://ontology.swissartresearch.net/aaao/ZE1_Institutional_Fact> ;
    skos:notation "ZP115i"^^xsd:string .

<https://ontology.swissartresearch.net/aaao/ZP116_ascribes_authority_status_relation> a rdf:Property ;
    rdfs:label "ascribes authority status relation"@en ;
    rdfs:comment "This property is used to indicate the specific manner in which the type of authority status which is indicated as holding for the subject pertains to this subject."@en ;
    rdfs:domain <https://ontology.swissartresearch.net/aaao/ZE50_Authority_Status> ;
    rdfs:range <http://www.cidoc-crm.org/cidoc-crm/E55_Type> ;
    rdfs:subPropertyOf <https://ontology.swissartresearch.net/aaao/ZP3_ascribes_intentional_relation> ;
    skos:notation "ZP116"^^xsd:string .

<https://ontology.swissartresearch.net/aaao/ZP116i_is_authority_status_relation_ascribed_by> a rdf:Property ;
    rdfs:label "is authority status relation ascribed by"@en ;
    rdfs:comment "This property is the inverse of the forward property described in the scope note that follows. This property is used to indicate the specific manner in which the type of authority status which is indicated as holding for the subject pertains to this subject."@en ;
    rdfs:domain <http://www.cidoc-crm.org/cidoc-crm/E55_Type> ;
    rdfs:range <https://ontology.swissartresearch.net/aaao/ZE50_Authority_Status> ;
    rdfs:subPropertyOf <https://ontology.swissartresearch.net/aaao/ZP3i_is_intentional_relation_ascribed_by> ;
    skos:notation "ZP116i"^^xsd:string .

<https://ontology.swissartresearch.net/aaao/ZP117_generated_promise_to> a rdf:Property ;
    rdfs:label "generated promise to"@en ;
    rdfs:comment "This property is used to indicate the persons to whom a promise is made, when two parties reach a promissory agreement."@en ;
    rdfs:domain <https://ontology.swissartresearch.net/aaao/ZE46_Promisory_Agreement> ;
    rdfs:range <https://ontology.swissartresearch.net/aaao/ZE36_Persons> ;
    rdfs:subPropertyOf <http://www.cidoc-crm.org/cidoc-crm/P11_had_participant> ;
    skos:notation "ZP117"^^xsd:string .

<https://ontology.swissartresearch.net/aaao/ZP117i_was_promisee_in> a rdf:Property ;
    rdfs:label "was promisee in"@en ;
    rdfs:comment "This property is the inverse of the forward property described in the scope note that follows. This property is used to indicate the persons to whom a promise is made, when two parties reach a promissory agreement."@en ;
    rdfs:domain <https://ontology.swissartresearch.net/aaao/ZE36_Persons> ;
    rdfs:range <https://ontology.swissartresearch.net/aaao/ZE46_Promisory_Agreement> ;
    rdfs:subPropertyOf <http://www.cidoc-crm.org/cidoc-crm/P11i_participated_in> ;
    skos:notation "ZP117i"^^xsd:string .

<https://ontology.swissartresearch.net/aaao/ZP118_generated_promise_upon> a rdf:Property ;
    rdfs:label "generated promise upon"@en ;
    rdfs:comment "This property is used to indicate the actor upon whom an obligation is generated when two parties reach a promissory agreement."@en ;
    rdfs:domain <https://ontology.swissartresearch.net/aaao/ZE46_Promisory_Agreement> ;
    rdfs:range <http://www.cidoc-crm.org/cidoc-crm/E39_Actor> ;
    rdfs:subPropertyOf <http://www.cidoc-crm.org/cidoc-crm/P14_carried_out_by> ;
    skos:notation "ZP118"^^xsd:string .

<https://ontology.swissartresearch.net/aaao/ZP118i_was_promisor_in> a rdf:Property ;
    rdfs:label "was promisor in"@en ;
    rdfs:comment "This property is the inverse of the forward property described in the scope note that follows. This property is used to indicate the actor upon whom an obligation is generated when two parties reach a promissory agreement."@en ;
    rdfs:domain <http://www.cidoc-crm.org/cidoc-crm/E39_Actor> ;
    rdfs:range <https://ontology.swissartresearch.net/aaao/ZE46_Promisory_Agreement> ;
    rdfs:subPropertyOf <http://www.cidoc-crm.org/cidoc-crm/P14i_performed> ;
    skos:notation "ZP118i"^^xsd:string .

<https://ontology.swissartresearch.net/aaao/ZP119_ascribes_event_location_relation> a rdf:Property ;
    rdfs:label "ascribes event location relation"@en ;
    rdfs:comment "This property is used to indicate the specific type of event locative status which is indicated as holding between the subject event and its ascribed place."@en ;
    rdfs:domain <https://ontology.swissartresearch.net/aaao/ZE60_Evental_Locative_Status> ;
    rdfs:range <http://www.cidoc-crm.org/cidoc-crm/E55_Type> ;
    rdfs:subPropertyOf <https://ontology.swissartresearch.net/aaao/ZP3_ascribes_intentional_relation> ;
    skos:notation "ZP119"^^xsd:string .

<https://ontology.swissartresearch.net/aaao/ZP119i_is_event_location_relation_ascribed_by> a rdf:Property ;
    rdfs:label "is event location relation ascribed by"@en ;
    rdfs:comment "This property is the inverse of the forward property described in the scope note that follows. This property is used to indicate the specific type of event locative status which is indicated as holding between the subject event and its ascribed place."@en ;
    rdfs:domain <http://www.cidoc-crm.org/cidoc-crm/E55_Type> ;
    rdfs:range <https://ontology.swissartresearch.net/aaao/ZE60_Evental_Locative_Status> ;
    rdfs:subPropertyOf <https://ontology.swissartresearch.net/aaao/ZP3i_is_intentional_relation_ascribed_by> ;
    skos:notation "ZP119i"^^xsd:string .

<https://ontology.swissartresearch.net/aaao/ZP120_has_event_location_subject> a rdf:Property ;
    rdfs:label "has event location subject"@en ;
    rdfs:comment "This property is used to indicate the event which has been ascribed a place."@en ;
    rdfs:domain <https://ontology.swissartresearch.net/aaao/ZE60_Evental_Locative_Status> ;
    rdfs:range <http://www.cidoc-crm.org/cidoc-crm/E5_Event> ;
    rdfs:subPropertyOf <https://ontology.swissartresearch.net/aaao/ZP1_has_intentional_subject> ;
    skos:notation "ZP120"^^xsd:string .

<https://ontology.swissartresearch.net/aaao/ZP120i_is_event_location_subject_of> a rdf:Property ;
    rdfs:label "is event location subject of"@en ;
    rdfs:comment "This property is the inverse of the forward property described in the scope note that follows. This property is used to indicate the event which has been ascribed a place."@en ;
    rdfs:domain <http://www.cidoc-crm.org/cidoc-crm/E5_Event> ;
    rdfs:range <https://ontology.swissartresearch.net/aaao/ZE60_Evental_Locative_Status> ;
    rdfs:subPropertyOf <https://ontology.swissartresearch.net/aaao/ZP1i_is_intentional_subject_of> ;
    skos:notation "ZP120i"^^xsd:string .

<https://ontology.swissartresearch.net/aaao/ZP121_involved> a rdf:Property ;
    rdfs:label "involved"@en ;
    rdfs:comment "This property describes the passive involvement of instances of ZE39 Persons in an instance of E5 Event."@en ;
    rdfs:domain <http://www.cidoc-crm.org/cidoc-crm/E5_Event> ;
    rdfs:range <https://ontology.swissartresearch.net/aaao/ZE36_Persons> ;
    rdfs:subPropertyOf <http://www.cidoc-crm.org/cidoc-crm/P12_occurred_in_the_presence_of> ;
    skos:notation "ZP121"^^xsd:string .

<https://ontology.swissartresearch.net/aaao/ZP121i_was_involved_in> a rdf:Property ;
    rdfs:label "was involved in"@en ;
    rdfs:comment "This property is the inverse of the forward property described in the scope note that follows. This property describes the passive involvement of instances of ZE39 Persons in an instance of E5 Event."@en ;
    rdfs:domain <https://ontology.swissartresearch.net/aaao/ZE36_Persons> ;
    rdfs:range <http://www.cidoc-crm.org/cidoc-crm/E5_Event> ;
    rdfs:subPropertyOf <http://www.cidoc-crm.org/cidoc-crm/P12i_was_present_at> ;
    skos:notation "ZP121i"^^xsd:string .

<https://ontology.swissartresearch.net/aaao/ZP14_has_functional_subject> a rdf:Property ;
    rdfs:label "has functional subject"@en ;
    rdfs:comment """This property is used to indicate the entity for which a certain functional classification is taken to hold by the instance of functional status.
"""@en ;
    rdfs:domain <https://ontology.swissartresearch.net/aaao/ZE5_Function_Status> ;
    rdfs:range <http://www.cidoc-crm.org/cidoc-crm/E1_CRM_Entity> ;
    rdfs:subPropertyOf <https://ontology.swissartresearch.net/aaao/ZP11_has_classificatory_subject> ;
    skos:notation "ZP14"^^xsd:string .

<https://ontology.swissartresearch.net/aaao/ZP14i_is_functional_subject_of> a rdf:Property ;
    rdfs:label "is functional subject of"@en ;
    rdfs:comment """This property is the inverse of the forward property described in the scope note that follows. This property is used to indicate the entity for which a certain functional classification is taken to hold by the instance of functional status.
"""@en ;
    rdfs:domain <http://www.cidoc-crm.org/cidoc-crm/E1_CRM_Entity> ;
    rdfs:range <https://ontology.swissartresearch.net/aaao/ZE5_Function_Status> ;
    rdfs:subPropertyOf <https://ontology.swissartresearch.net/aaao/ZP11i_is_classificatory_subject_of> ;
    skos:notation "ZP14i"^^xsd:string .

<https://ontology.swissartresearch.net/aaao/ZP15_ascribes_function> a rdf:Property ;
    rdfs:label "ascribes function"@en ;
    rdfs:comment """This property is used to indicate the type of function which is indicated as holding for the subject of the function status.
"""@en ;
    rdfs:domain <https://ontology.swissartresearch.net/aaao/ZE5_Function_Status> ;
    rdfs:range <http://www.cidoc-crm.org/cidoc-crm/E55_Type> ;
    rdfs:subPropertyOf <https://ontology.swissartresearch.net/aaao/ZP12_ascribes_classification> ;
    skos:notation "ZP15"^^xsd:string .

<https://ontology.swissartresearch.net/aaao/ZP15i_is_function_ascribed_by> a rdf:Property ;
    rdfs:label "is function ascribed by"@en ;
    rdfs:comment """This property is the inverse of the forward property described in the scope note that follows. This property is used to indicate the type of function which is indicated as holding for the subject of the function status.
"""@en ;
    rdfs:domain <http://www.cidoc-crm.org/cidoc-crm/E55_Type> ;
    rdfs:range <https://ontology.swissartresearch.net/aaao/ZE5_Function_Status> ;
    rdfs:subPropertyOf <https://ontology.swissartresearch.net/aaao/ZP12i_is_classification_ascribed_by> ;
    skos:notation "ZP15i"^^xsd:string .

<https://ontology.swissartresearch.net/aaao/ZP16_ascribes_functional_relation> a rdf:Property ;
    rdfs:label "ascribes functional relation"@en ;
    rdfs:comment """This property is used to indicate the specific manner in which the function which is indicated as holding for the subjectof the function status pertains to this subject.
"""@en ;
    rdfs:domain <https://ontology.swissartresearch.net/aaao/ZE5_Function_Status> ;
    rdfs:range <http://www.cidoc-crm.org/cidoc-crm/E55_Type> ;
    rdfs:subPropertyOf <https://ontology.swissartresearch.net/aaao/ZP13_ascribes_classification_relation> ;
    skos:notation "ZP16"^^xsd:string .

<https://ontology.swissartresearch.net/aaao/ZP16i_is_functional_relation_ascribed_by> a rdf:Property ;
    rdfs:label "is functional relation ascribed by"@en ;
    rdfs:comment """This property is the inverse of the forward property described in the scope note that follows. This property is used to indicate the specific manner in which the function which is indicated as holding for the subject  of the function status pertains to this subject.
"""@en ;
    rdfs:domain <http://www.cidoc-crm.org/cidoc-crm/E55_Type> ;
    rdfs:range <https://ontology.swissartresearch.net/aaao/ZE5_Function_Status> ;
    rdfs:subPropertyOf <https://ontology.swissartresearch.net/aaao/ZP13i_is_classification_relation_ascribed_by> ;
    skos:notation "ZP16i"^^xsd:string .

<https://ontology.swissartresearch.net/aaao/ZP19_ascribes_social_status_relation> a rdf:Property ;
    rdfs:label "ascribes social status relation"@en ;
    rdfs:comment """This property is used to indicate the specific manner in which the type of social status which is indicated as holding for the subject pertains to this subject.
"""@en ;
    rdfs:domain <https://ontology.swissartresearch.net/aaao/ZE6_Social_Status> ;
    rdfs:range <http://www.cidoc-crm.org/cidoc-crm/E55_Type> ;
    rdfs:subPropertyOf <https://ontology.swissartresearch.net/aaao/ZP13_ascribes_classification_relation> ;
    skos:notation "ZP19"^^xsd:string .

<https://ontology.swissartresearch.net/aaao/ZP19i_is_social_status_relation_ascribed_by> a rdf:Property ;
    rdfs:label "is social status relation ascribed by"@en ;
    rdfs:comment """This property is the inverse of the forward property described in the scope note that follows. This property is used to indicate the specific manner in which the type of social status which is indicated as holding for the subject pertains to this subject.
"""@en ;
    rdfs:domain <http://www.cidoc-crm.org/cidoc-crm/E55_Type> ;
    rdfs:relation <https://ontology.swissartresearch.net/aaao/ZE6_Social_Status> ;
    rdfs:subPropertyOf <https://ontology.swissartresearch.net/aaao/ZP13i_is_classification_relation_ascribed_by> ;
    skos:notation "ZP19i"^^xsd:string .

<https://ontology.swissartresearch.net/aaao/ZP20_has_custodial_subject> a rdf:Property ;
    rdfs:label "has custodial subject"@en ;
    rdfs:comment """This property is used to indicate the physical thing over which a certain custodial status is taken to hold.
"""@en ;
    rdfs:domain <https://ontology.swissartresearch.net/aaao/ZE7_Custodial_Status> ;
    rdfs:range <http://www.cidoc-crm.org/cidoc-crm/E18_Physical_Thing> ;
    rdfs:subPropertyOf <https://ontology.swissartresearch.net/aaao/ZP1_has_intentional_subject> ;
    skos:notation "ZP20"^^xsd:string .

<https://ontology.swissartresearch.net/aaao/ZP20i_is_custodial_subject_of> a rdf:Property ;
    rdfs:label "is custodial subject of"@en ;
    rdfs:comment """This property is the inverse of the forward property described in the scope note that follows. This property is used to indicate the physical thing over which a certain custodial status is taken to hold.
"""@en ;
    rdfs:domain <http://www.cidoc-crm.org/cidoc-crm/E18_Physical_Thing> ;
    rdfs:range <https://ontology.swissartresearch.net/aaao/ZE7_Custodial_Status> ;
    rdfs:subPropertyOf <https://ontology.swissartresearch.net/aaao/ZP1i_is_intentional_subject_of> ;
    skos:notation "ZP20i"^^xsd:string .

<https://ontology.swissartresearch.net/aaao/ZP21_ascribes_custodian> a rdf:Property ;
    rdfs:label "ascribes custodian"@en ;
    rdfs:comment """This property is used to indicate the custodian to whom the custody of the physical thing which is the subject of the custodial status redounds.
"""@en ;
    rdfs:domain <https://ontology.swissartresearch.net/aaao/ZE7_Custodial_Status> ;
    rdfs:range <http://www.cidoc-crm.org/cidoc-crm/E39_Actor> ;
    rdfs:subPropertyOf <https://ontology.swissartresearch.net/aaao/ZP2_ascribes_intentional_target> ;
    skos:notation "ZP21"^^xsd:string .

<https://ontology.swissartresearch.net/aaao/ZP21i_is_custodian_ascribed_by> a rdf:Property ;
    rdfs:label "is custodian ascribed by"@en ;
    rdfs:comment """This property is the inverse of the forward property described in the scope note that follows. This property is used to indicate the custodian to whom the custody of the physical thing which is the subject of the custodial status redounds.
"""@en ;
    rdfs:domain <http://www.cidoc-crm.org/cidoc-crm/E39_Actor> ;
    rdfs:range <https://ontology.swissartresearch.net/aaao/ZE7_Custodial_Status> ;
    rdfs:subPropertyOf <https://ontology.swissartresearch.net/aaao/ZP2i_is_intentional_target_ascribed_by> ;
    skos:notation "ZP21i"^^xsd:string .

<https://ontology.swissartresearch.net/aaao/ZP22_ascribes_custodial_relation> a rdf:Property ;
    rdfs:label "ascribes custodial relation"@en ;
    rdfs:comment """This property is used to indicate the specific manner in which the custodial status which is indicated as holding over the legal object by the custodian pertains to this subject.
"""@en ;
    rdfs:domain <https://ontology.swissartresearch.net/aaao/ZE7_Custodial_Status> ;
    rdfs:range <http://www.cidoc-crm.org/cidoc-crm/E55_Type> ;
    rdfs:subPropertyOf <https://ontology.swissartresearch.net/aaao/ZP3_ascribes_intentional_relation> ;
    skos:notation "ZP22"^^xsd:string .

<https://ontology.swissartresearch.net/aaao/ZP22i_is_custodial_relation_ascribed_by> a rdf:Property ;
    rdfs:label "is  custodial relation ascribed by"@en ;
    rdfs:comment """This property is the inverse of the forward property described in the scope note that follows. This property is used to indicate the specific manner in which the custodial status which is indicated as holding over the legal object by the custodian pertains to this subject.
"""@en ;
    rdfs:domain <http://www.cidoc-crm.org/cidoc-crm/E55_Type> ;
    rdfs:range <https://ontology.swissartresearch.net/aaao/ZE7_Custodial_Status> ;
    rdfs:subPropertyOf <https://ontology.swissartresearch.net/aaao/ZP3i_is_intentional_relation_ascribed_by> ;
    skos:notation "ZP22i"^^xsd:string .

<https://ontology.swissartresearch.net/aaao/ZP23_has_ownership_subject> a rdf:Property ;
    rdfs:label "has ownership subject"@en ;
    rdfs:comment """This property is used to indicate the legal object over which a certain ownership status is taken to hold.
"""@en ;
    rdfs:domain <https://ontology.swissartresearch.net/aaao/ZE8_Ownership_Status> ;
    rdfs:range <http://www.cidoc-crm.org/cidoc-crm/E18_Physical_Thing> ;
    rdfs:subPropertyOf <https://ontology.swissartresearch.net/aaao/ZP1_has_intentional_subject> ;
    skos:notation "ZP23"^^xsd:string .

<https://ontology.swissartresearch.net/aaao/ZP23i_is_ownership_subject_of> a rdf:Property ;
    rdfs:label "is ownership subject of"@en ;
    rdfs:comment """This property is the inverse of the forward property described in the scope note that follows. This property is used to indicate the legal object over which a certain ownership status is taken to hold.
"""@en ;
    rdfs:domain <http://www.cidoc-crm.org/cidoc-crm/E18_Physical_Thing> ;
    rdfs:range <https://ontology.swissartresearch.net/aaao/ZE8_Ownership_Status> ;
    rdfs:subPropertyOf <https://ontology.swissartresearch.net/aaao/ZP1i_is_intentional_subject_of> ;
    skos:notation "ZP23i"^^xsd:string .

<https://ontology.swissartresearch.net/aaao/ZP24_ascribes_owner> a rdf:Property ;
    rdfs:label "ascribes owner"@en ;
    rdfs:comment """This property is used to indicate the owner to whom the title of the legal object which is the subject of the ownership status redounds.
"""@en ;
    rdfs:domain <https://ontology.swissartresearch.net/aaao/ZE8_Ownership_Status> ;
    rdfs:range <http://www.cidoc-crm.org/cidoc-crm/E39_Actor> ;
    rdfs:subPropertyOf <https://ontology.swissartresearch.net/aaao/ZP2_ascribes_intentional_target> ;
    skos:notation "ZP24"^^xsd:string .

<https://ontology.swissartresearch.net/aaao/ZP24i_is_owner_ascribed_by> a rdf:Property ;
    rdfs:label "is owner ascribed by"@en ;
    rdfs:comment """This property is the inverse of the forward property described in the scope note that follows. This property is used to indicate the owner to whom the title of the legal object which is the subject of the ownership status redounds.
"""@en ;
    rdfs:domain <http://www.cidoc-crm.org/cidoc-crm/E39_Actor> ;
    rdfs:range <https://ontology.swissartresearch.net/aaao/ZE8_Ownership_Status> ;
    rdfs:subPropertyOf <https://ontology.swissartresearch.net/aaao/ZP2i_is_intentional_target_ascribed_by> ;
    skos:notation "ZP24i"^^xsd:string .

<https://ontology.swissartresearch.net/aaao/ZP25_ascribes_ownership_relation> a rdf:Property ;
    rdfs:label "ascribes ownership relation"@en ;
    rdfs:comment """This property is used to indicate the specific manner in which the ownership status which is indicated as holding over the legal object by the owner pertains to this subject.
"""@en ;
    rdfs:domain <https://ontology.swissartresearch.net/aaao/ZE8_Ownership_Status> ;
    rdfs:range <http://www.cidoc-crm.org/cidoc-crm/E55_Type> ;
    rdfs:subPropertyOf <https://ontology.swissartresearch.net/aaao/ZP3_ascribes_intentional_relation> ;
    skos:notation "ZP25"^^xsd:string .

<https://ontology.swissartresearch.net/aaao/ZP25i_is_ownership_relation_ascribed_by> a rdf:Property ;
    rdfs:label "is ownership relation ascribed by"@en ;
    rdfs:comment """This property is the inverse of the forward property described in the scope note that follows. This property is used to indicate the specific manner in which the ownership status which is indicated as holding over the legal object by the owner pertains to this subject.
"""@en ;
    rdfs:domain <http://www.cidoc-crm.org/cidoc-crm/E55_Type> ;
    rdfs:range <https://ontology.swissartresearch.net/aaao/ZE8_Ownership_Status> ;
    rdfs:subPropertyOf <https://ontology.swissartresearch.net/aaao/ZP3i_is_intentional_relation_ascribed_by> ;
    skos:notation "ZP25i"^^xsd:string .

<https://ontology.swissartresearch.net/aaao/ZP26_has_residence_subject> a rdf:Property ;
    rdfs:label "has residence subject"@en ;
    rdfs:comment """This property is used to indicate the actor for whom the residence status is taken to hold.
"""@en ;
    rdfs:domain <https://ontology.swissartresearch.net/aaao/ZE9_Residential_Status> ;
    rdfs:range <http://www.cidoc-crm.org/cidoc-crm/E39_Actor> ;
    rdfs:subPropertyOf <https://ontology.swissartresearch.net/aaao/ZP1_has_intentional_subject> ;
    skos:notation "ZP26"^^xsd:string .

<https://ontology.swissartresearch.net/aaao/ZP26i_is_residence_subject_of> a rdf:Property ;
    rdfs:label "is residence subject of"@en ;
    rdfs:comment """This property is the inverse of the forward property described in the scope note that follows. This property is used to indicate the actor for whom the residence status is taken to hold.
"""@en ;
    rdfs:domain <http://www.cidoc-crm.org/cidoc-crm/E39_Actor> ;
    rdfs:range <https://ontology.swissartresearch.net/aaao/ZE9_Residential_Status> ;
    rdfs:subPropertyOf <https://ontology.swissartresearch.net/aaao/ZP1i_is_intentional_subject_of> ;
    skos:notation "ZP26i"^^xsd:string .

<https://ontology.swissartresearch.net/aaao/ZP27_acribes_residence_place> a rdf:Property ;
    rdfs:label "ascribes residence place"@en ;
    rdfs:comment """This property is used to indicate the place at which the subject of the residence status is taken to reside or dwell.
"""@en ;
    rdfs:domain <https://ontology.swissartresearch.net/aaao/ZE9_Residential_Status> ;
    rdfs:range <http://www.cidoc-crm.org/cidoc-crm/E53_Place> ;
    rdfs:subPropertyOf <https://ontology.swissartresearch.net/aaao/ZP77_ascribes_place> ;
    skos:notation "ZP27"^^xsd:string .

<https://ontology.swissartresearch.net/aaao/ZP27i_is_residence_place_ascribed_by> a rdf:Property ;
    rdfs:label "is residence place ascribed by"@en ;
    rdfs:comment """This property is the inverse of the forward property described in the scope note that follows. This property is used to indicate the place at which the subject of the residence status is taken to reside or dwell.
"""@en ;
    rdfs:domain <http://www.cidoc-crm.org/cidoc-crm/E53_Place> ;
    rdfs:range <https://ontology.swissartresearch.net/aaao/ZE9_Residential_Status> ;
    rdfs:subPropertyOf <https://ontology.swissartresearch.net/aaao/ZP2i_is_intentional_target_ascribed_by> ;
    skos:notation "ZP27i"^^xsd:string .

<https://ontology.swissartresearch.net/aaao/ZP28_ascribes_residence_relation> a rdf:Property ;
    rdfs:label "ascribes residence relation"@en ;
    rdfs:comment """This property is used to indicate the specific manner in which the residence status which is indicated as holding over the actor pertains to this subject.
"""@en ;
    rdfs:domain <https://ontology.swissartresearch.net/aaao/ZE9_Residential_Status> ;
    rdfs:range <http://www.cidoc-crm.org/cidoc-crm/E55_Type> ;
    rdfs:subPropertyOf <https://ontology.swissartresearch.net/aaao/ZP3_ascribes_intentional_relation> ;
    skos:notation "ZP28"^^xsd:string .

<https://ontology.swissartresearch.net/aaao/ZP28i_is_residence_relation_ascribed_by> a rdf:Property ;
    rdfs:label "is residence relation ascribed by"@en ;
    rdfs:comment """This property is the inverse of the forward property described in the scope note that follows. This property is used to indicate the specific manner in which the residence status which is indicated as holding over the actor pertains to this subject.
"""@en ;
    rdfs:domain <http://www.cidoc-crm.org/cidoc-crm/E55_Type> ;
    rdfs:range <https://ontology.swissartresearch.net/aaao/ZE9_Residential_Status> ;
    rdfs:subPropertyOf <https://ontology.swissartresearch.net/aaao/ZP3i_is_intentional_relation_ascribed_by> ;
    skos:notation "ZP28i"^^xsd:string .

<https://ontology.swissartresearch.net/aaao/ZP29_has_familial_subject> a rdf:Property ;
    rdfs:label "has familial subject"@en ;
    rdfs:comment """This property is used to indicate the person for whom the family status is taken to hold.
"""@en ;
    rdfs:domain <https://ontology.swissartresearch.net/aaao/ZE10_Family_Status> ;
    rdfs:range <http://www.cidoc-crm.org/cidoc-crm/E21_Person> ;
    rdfs:subPropertyOf <https://ontology.swissartresearch.net/aaao/ZP105_has_social_relation_subject> ;
    skos:notation "ZP29"^^xsd:string .

<https://ontology.swissartresearch.net/aaao/ZP29i_is_familial_subject_of> a rdf:Property ;
    rdfs:label "is familial subject of"@en ;
    rdfs:comment """This property is the inverse of the forward property described in the scope note that follows. This property is used to indicate the person for whom the family status is taken to hold.
"""@en ;
    rdfs:domain <http://www.cidoc-crm.org/cidoc-crm/E21_Person> ;
    rdfs:range <https://ontology.swissartresearch.net/aaao/ZE10_Family_Status> ;
    rdfs:subPropertyOf <https://ontology.swissartresearch.net/aaao/ZP1i_is_intentional_subject_of> ;
    skos:notation "ZP29i"^^xsd:string .

<https://ontology.swissartresearch.net/aaao/ZP30_ascribes_relative> a rdf:Property ;
    rdfs:label "ascribes relative"@en ;
    rdfs:comment """This property is used to indicate the person with whom the subject of the family relation status has the familial relation which they have.
"""@en ;
    rdfs:domain <https://ontology.swissartresearch.net/aaao/ZE10_Family_Status> ;
    rdfs:range <http://www.cidoc-crm.org/cidoc-crm/E21_Person> ;
    rdfs:subPropertyOf <https://ontology.swissartresearch.net/aaao/ZP103_ascribes_social_relation_target> ;
    skos:notation "ZP30"^^xsd:string .

<https://ontology.swissartresearch.net/aaao/ZP30i_is_relative_ascribed_by> a rdf:Property ;
    rdfs:label "is  relative acribed of"@en ;
    rdfs:comment """This property is the inverse of the forward property described in the scope note that follows. This property is used to indicate the person with whom the subject of the family relation status has the familial relation which they have.
"""@en ;
    rdfs:domain <http://www.cidoc-crm.org/cidoc-crm/E21_Person> ;
    rdfs:range <https://ontology.swissartresearch.net/aaao/ZE10_Family_Status> ;
    rdfs:subPropertyOf <https://ontology.swissartresearch.net/aaao/ZP2i_is_intentional_target_ascribed_by> ;
    skos:notation "ZP30i"^^xsd:string .

<https://ontology.swissartresearch.net/aaao/ZP31_ascribes_familial_relation> a rdf:Property ;
    rdfs:label "ascribes familial relation"@en ;
    rdfs:comment """This property is used to indicate the specific type of family status which is indicated as holding between the subject individual and his/her ascribed relative.
"""@en ;
    rdfs:domain <https://ontology.swissartresearch.net/aaao/ZE10_Family_Status> ;
    rdfs:range <http://www.cidoc-crm.org/cidoc-crm/E55_Type> ;
    rdfs:subPropertyOf <https://ontology.swissartresearch.net/aaao/ZP104_ascribes_social_relation> ;
    skos:notation "ZP31"^^xsd:string .

<https://ontology.swissartresearch.net/aaao/ZP31i_is_familial_relation_ascribed_by> a rdf:Property ;
    rdfs:label "is familial relation ascribed by"@en ;
    rdfs:comment """This property is the inverse of the forward property described in the scope note that follows. This property is used to indicate the specific type of family status which is indicated as holding between the subject individual and his/her ascribed relative.
"""@en ;
    rdfs:domain <http://www.cidoc-crm.org/cidoc-crm/E55_Type> ;
    rdfs:range <https://ontology.swissartresearch.net/aaao/ZE10_Family_Status> ;
    rdfs:subPropertyOf <https://ontology.swissartresearch.net/aaao/ZP3i_is_intentional_relation_ascribed_by> ;
    skos:notation "ZP31i"^^xsd:string .

<https://ontology.swissartresearch.net/aaao/ZP32_has_membership_subject> a rdf:Property ;
    rdfs:label "has membership subject"@en ;
    rdfs:comment """This property is used to indicate the person or group for whom the membership status is taken to hold.
"""@en ;
    rdfs:domain <https://ontology.swissartresearch.net/aaao/ZE11_Membership_Status> ;
    rdfs:range <http://www.cidoc-crm.org/cidoc-crm/E39_Actor> ;
    rdfs:subPropertyOf <https://ontology.swissartresearch.net/aaao/ZP1_has_intentional_subject> ;
    skos:notation "ZP32"^^xsd:string .

<https://ontology.swissartresearch.net/aaao/ZP32i_is_membership_subject_of> a rdf:Property ;
    rdfs:label "is membership subject of"@en ;
    rdfs:comment """This property is the inverse of the forward property described in the scope note that follows. This property is used to indicate the person or group for whom the membership status is taken to hold.
"""@en ;
    rdfs:domain <http://www.cidoc-crm.org/cidoc-crm/E39_Actor> ;
    rdfs:range <https://ontology.swissartresearch.net/aaao/ZE11_Membership_Status> ;
    rdfs:subPropertyOf <https://ontology.swissartresearch.net/aaao/ZP1i_is_intentional_subject_of> ;
    skos:notation "ZP32i"^^xsd:string .

<https://ontology.swissartresearch.net/aaao/ZP33_ascribes_group> a rdf:Property ;
    rdfs:label "ascribes group"@en ;
    rdfs:comment """This property is used to indicate the group ascribed to the subject person of the membership status as having a membership relation thereto.
"""@en ;
    rdfs:domain <https://ontology.swissartresearch.net/aaao/ZE11_Membership_Status> ;
    rdfs:range <http://www.cidoc-crm.org/cidoc-crm/E74_Group> ;
    rdfs:subPropertyOf <https://ontology.swissartresearch.net/aaao/ZP2_ascribes_intentional_target> ;
    skos:notation "ZP33"^^xsd:string .

<https://ontology.swissartresearch.net/aaao/ZP33i_is_group_ascribed_by> a rdf:Property ;
    rdfs:label "is group ascribed by"@en ;
    rdfs:comment """This property is the inverse of the forward property described in the scope note that follows. This property is used to indicate the group ascribed to the subject person of the membership status as having a membership relation thereto.
"""@en ;
    rdfs:domain <http://www.cidoc-crm.org/cidoc-crm/E74_Group> ;
    rdfs:range <https://ontology.swissartresearch.net/aaao/ZE11_Membership_Status> ;
    rdfs:subPropertyOf <https://ontology.swissartresearch.net/aaao/ZP2i_is_intentional_target_ascribed_by> ;
    skos:notation "ZP33i"^^xsd:string .

<https://ontology.swissartresearch.net/aaao/ZP34_ascribes_membership_relation> a rdf:Property ;
    rdfs:label "ascribes membership relation"@en ;
    rdfs:comment """This property is used to indicate the specific type of membership status which is indicated as holding between the subject actor and the group to which it is ascribed as being a member.
"""@en ;
    rdfs:domain <https://ontology.swissartresearch.net/aaao/ZE11_Membership_Status> ;
    rdfs:range <http://www.cidoc-crm.org/cidoc-crm/E55_Type> ;
    rdfs:subPropertyOf <https://ontology.swissartresearch.net/aaao/ZP3_ascribes_intentional_relation> ;
    skos:notation "ZP34"^^xsd:string .

<https://ontology.swissartresearch.net/aaao/ZP34i_is_membership_relation_ascribed_by> a rdf:Property ;
    rdfs:label "is membership relation ascribed by"@en ;
    rdfs:comment """This property is the inverse of the forward property described in the scope note that follows. This property is used to indicate the specific type of membership status which is indicated as holding between the subject actor and the group to which it is ascribed as being a member.
"""@en ;
    rdfs:domain <http://www.cidoc-crm.org/cidoc-crm/E55_Type> ;
    rdfs:range <https://ontology.swissartresearch.net/aaao/ZE11_Membership_Status> ;
    rdfs:subPropertyOf <https://ontology.swissartresearch.net/aaao/ZP3i_is_intentional_relation_ascribed_by> ;
    skos:notation "ZP34i"^^xsd:string .

<https://ontology.swissartresearch.net/aaao/ZP35_has_referential_subject> a rdf:Property ;
    rdfs:label "has referential subject"@en ;
    rdfs:comment "This property is used to indicate the propositional object for which the referential status is taken to hold."@en ;
    rdfs:domain <https://ontology.swissartresearch.net/aaao/ZE12_Referential_Status> ;
    rdfs:range <http://www.cidoc-crm.org/cidoc-crm/E89_Propositional_Object> ;
    rdfs:subPropertyOf <https://ontology.swissartresearch.net/aaao/ZP1_has_intentional_subject> ;
    skos:notation "ZP35"^^xsd:string .

<https://ontology.swissartresearch.net/aaao/ZP35i_is_referential_subject_of> a rdf:Property ;
    rdfs:label "is referential subject of"@en ;
    rdfs:comment "This property is the inverse of the forward property described in the scope note that follows. This property is used to indicate the propositional object for which the referential status is taken to hold."@en ;
    rdfs:domain <http://www.cidoc-crm.org/cidoc-crm/E89_Propositional_Object> ;
    rdfs:range <https://ontology.swissartresearch.net/aaao/ZE12_Referential_Status> ;
    rdfs:subPropertyOf <https://ontology.swissartresearch.net/aaao/ZP1i_is_intentional_subject_of> ;
    skos:notation "ZP35i"^^xsd:string .

<https://ontology.swissartresearch.net/aaao/ZP36_ascribes_referent> a rdf:Property ;
    rdfs:label "ascribes referent"@en ;
    rdfs:comment """This property is used to indicate the referent to which the subject propositional object is taken to refer.
"""@en ;
    rdfs:domain <https://ontology.swissartresearch.net/aaao/ZE12_Referential_Status> ;
    rdfs:range <http://www.cidoc-crm.org/cidoc-crm/E1_CRM_Entity> ;
    rdfs:subPropertyOf <https://ontology.swissartresearch.net/aaao/ZP2_ascribes_intentional_target> ;
    skos:notation "ZP36"^^xsd:string .

<https://ontology.swissartresearch.net/aaao/ZP36i_referent_ascribed_by> a rdf:Property ;
    rdfs:label "is referent ascribed by"@en ;
    rdfs:comment """This property is the inverse of the forward property described in the scope note that follows. This property is used to indicate the referent to which the subject propositional object is taken to refer.
"""@en ;
    rdfs:domain <http://www.cidoc-crm.org/cidoc-crm/E1_CRM_Entity> ;
    rdfs:range <https://ontology.swissartresearch.net/aaao/ZE12_Referential_Status> ;
    rdfs:subPropertyOf <https://ontology.swissartresearch.net/aaao/ZP2i_is_intentional_target_ascribed_by> ;
    skos:notation "ZP36i"^^xsd:string .

<https://ontology.swissartresearch.net/aaao/ZP37_ascribes_referential_relation> a rdf:Property ;
    rdfs:label "ascribes referential relation"@en ;
    rdfs:comment """This property is used to indicate the specific type of referential status which is indicated as holding between the subject propositional object and its indicated intended referent.
"""@en ;
    rdfs:domain <https://ontology.swissartresearch.net/aaao/ZE12_Referential_Status> ;
    rdfs:range <http://www.cidoc-crm.org/cidoc-crm/E55_Type> ;
    rdfs:subPropertyOf <https://ontology.swissartresearch.net/aaao/ZP3_ascribes_intentional_relation> ;
    skos:notation "ZP37"^^xsd:string .

<https://ontology.swissartresearch.net/aaao/ZP37i_is_referential_relation_ascribed_by> a rdf:Property ;
    rdfs:label "is referential relation ascribed by"@en ;
    rdfs:comment """This property is the inverse of the forward property described in the scope note that follows. This property is used to indicate the specific type of referential status which is indicated as holding between the subject propositional object and its indicated intended referent.
"""@en ;
    rdfs:domain <http://www.cidoc-crm.org/cidoc-crm/E55_Type> ;
    rdfs:range <https://ontology.swissartresearch.net/aaao/ZE12_Referential_Status> ;
    rdfs:subPropertyOf <https://ontology.swissartresearch.net/aaao/ZP3i_is_intentional_relation_ascribed_by> ;
    skos:notation "ZP37i"^^xsd:string .

<https://ontology.swissartresearch.net/aaao/ZP38_ascribes_referential_mode> a rdf:Property ;
    rdfs:label "ascribes referential mode"@en ;
    rdfs:comment """This property is used to indicate the specific manner in which the referential status which is indicated as holding between the subject propositional object and its indicated intended referent holds.
"""@en ;
    rdfs:domain <https://ontology.swissartresearch.net/aaao/ZE12_Referential_Status> ;
    rdfs:range <http://www.cidoc-crm.org/cidoc-crm/E55_Type> ;
    skos:notation "ZP38"^^xsd:string .

<https://ontology.swissartresearch.net/aaao/ZP38i_is_referential_mode_ascribed_by> a rdf:Property ;
    rdfs:label "is  referential mode ascribed by"@en ;
    rdfs:comment """This property is the inverse of the forward property described in the scope note that follows. This property is used to indicate the specific manner in which the referential status which is indicated as holding between the subject propositional object and its indicated intended referent holds.
"""@en ;
    rdfs:domain <http://www.cidoc-crm.org/cidoc-crm/E55_Type> ;
    rdfs:range <https://ontology.swissartresearch.net/aaao/ZE12_Referential_Status> ;
    skos:notation "ZP38i"^^xsd:string .

<https://ontology.swissartresearch.net/aaao/ZP40_performed> a rdf:Property ;
    rdfs:label "performed"@en ;
    rdfs:comment """This property is used to indicate the performance plan sanctioned by normative rule appealed to by a symbolic act in order to bring out the specific intended communicative effect. At a general level, the performance plan is what is appealed to in order to carry out the symbolic act in the first place. For example, an act of defiance may call on a specific sequence of gestures to be instantiated.
The case of speech act (ZE13) is a special case of symbolic act where the performance plan indicates the series of necessary procedures that must be followed in order for the speech act to have been successfully carried out and to have created a genuine instance of the institutional fact that it was designed to make possible."""@en ;
    rdfs:domain <https://ontology.swissartresearch.net/aaao/ZE53_Symbolic_Act> ;
    rdfs:range <http://www.cidoc-crm.org/cidoc-crm/E29_Design_or_Procedure> ;
    rdfs:subPropertyOf <http://www.cidoc-crm.org/cidoc-crm/P33_used_specific_technique> ;
    skos:notation "ZP40"^^xsd:string .

<https://ontology.swissartresearch.net/aaao/ZP40i_was_performed_by> a rdf:Property ;
    rdfs:label "was performed by"@en ;
    rdfs:comment """This property is the inverse of the forward property described in the scope note that follows. This property is used to indicate the performance plan sanctioned by normative rule appealed to by the speech act  to bring about a new institutional fact. This performance plan indicates the series of necessary procedures that must be followed in order for the speech act to have been successfully carried out and to have created a genuine instance of the institutional fact that it was designed to make possible.
"""@en ;
    rdfs:domain <http://www.cidoc-crm.org/cidoc-crm/E29_Design_or_Procedure> ;
    rdfs:range <https://ontology.swissartresearch.net/aaao/ZE13_Speech_Act> ;
    rdfs:subPropertyOf <http://www.cidoc-crm.org/cidoc-crm/P33i_was_used_by> ;
    skos:notation "ZP40i"^^xsd:string .

<https://ontology.swissartresearch.net/aaao/ZP41_uttered> a rdf:Property ;
    rdfs:label "uttered"@en ;
    rdfs:comment "It is typical of performance plans for normative procedures to include a necessary invoking clause or set of clauses which must be uttered in the course of the performance of the speech act in order to for it to be successfully carried out. This property enables the documentation of the use of such a linguistic object."@en ;
    rdfs:domain <https://ontology.swissartresearch.net/aaao/ZE13_Speech_Act> ;
    rdfs:range <http://www.cidoc-crm.org/cidoc-crm/E73_Information_Object> ;
    rdfs:subPropertyOf <http://www.cidoc-crm.org/cidoc-crm/P16_used_specific_object> ;
    skos:notation "ZP41"^^xsd:string .

<https://ontology.swissartresearch.net/aaao/ZP41i_was_uttered_by> a rdf:Property ;
    rdfs:label "was uttered by"@en ;
    rdfs:comment """This property is the inverse of the forward property described in the scope note that follows. It is typical of performance plans for normative procedures to include a necessary invoking clause or set of clauses which must be uttered in the course of the performance of the speech act in order to for it to be successfully carried out. This property enables the documentation of the use of such a linguistic object.
"""@en ;
    rdfs:domain <http://www.cidoc-crm.org/cidoc-crm/E73_Information_Object> ;
    rdfs:range <https://ontology.swissartresearch.net/aaao/ZE13_Speech_Act> ;
    rdfs:subPropertyOf <http://www.cidoc-crm.org/cidoc-crm/P16i_was_used_for> ;
    skos:notation "ZP41i"^^xsd:string .

<https://ontology.swissartresearch.net/aaao/ZP42_intentionally_initiated> a rdf:Property ;
    rdfs:label "intentionally initiated"@en ;
    rdfs:comment """This property is used to connect an instance of transformative symbolic act to the instance of institutional fact which it brought into existence throughthe successful performance of a specified norm type conformant symbolic act.
"""@en ;
    rdfs:domain <https://ontology.swissartresearch.net/aaao/ZE52_Transformative_Symbolic_Act> ;
    rdfs:range <https://ontology.swissartresearch.net/aaao/ZE1_Institutional_Fact> ;
    rdfs:subPropertyOf <https://ontology.swissartresearch.net/aaao/ZP111_initiated> ;
    skos:notation "ZP42"^^xsd:string .

<https://ontology.swissartresearch.net/aaao/ZP42i_was_intentionally_initiated_by> a rdf:Property ;
    rdfs:label "was intentionally initiated by"@en ;
    rdfs:comment """This property is the inverse of the forward property described in the scope note that follows. This property is used to connect the instance of speech act to the instance of institutional fact which it brought into existence through the correct performance of the specified performance to bring about the norm type it aimed to bring about.
"""@en ;
    rdfs:domain <https://ontology.swissartresearch.net/aaao/ZE1_Institutional_Fact> ;
    rdfs:range <https://ontology.swissartresearch.net/aaao/ZE13_Speech_Act> ;
    skos:notation "ZP42i"^^xsd:string .

<https://ontology.swissartresearch.net/aaao/ZP43_has_similarity_subject> a rdf:Property ;
    rdfs:label "has similarity subject"@en ;
    rdfs:comment "This property is used to indicate one of two entities for which the similarity status is taken to hold."@en ;
    rdfs:domain <https://ontology.swissartresearch.net/aaao/ZE14_Similarity_Status> ;
    rdfs:range <http://www.cidoc-crm.org/cidoc-crm/E1_CRM_Entity> ;
    rdfs:subPropertyOf <https://ontology.swissartresearch.net/aaao/ZP1_has_intentional_subject> ;
    skos:notation "ZP43"^^xsd:string .

<https://ontology.swissartresearch.net/aaao/ZP43i_is_similarity_subject_of> a rdf:Property ;
    rdfs:label "is similarity subject of"@en ;
    rdfs:comment "This property is the inverse of the forward property described in the scope note that follows. This property is used to indicate one of two entities for which the similarity status is taken to hold."@en ;
    rdfs:domain <http://www.cidoc-crm.org/cidoc-crm/E1_CRM_Entity> ;
    rdfs:range <https://ontology.swissartresearch.net/aaao/ZE14_Similarity_Status> ;
    rdfs:subPropertyOf <https://ontology.swissartresearch.net/aaao/ZP1i_is_intentional_subject_of> ;
    skos:notation "ZP43i"^^xsd:string .

<https://ontology.swissartresearch.net/aaao/ZP44_ascribes_similarity_target> a rdf:Property ;
    rdfs:label "ascribes similarity target"@en ;
    rdfs:comment "This property is used to indicate the other entity for which the similarity status is taken to hold."@en ;
    rdfs:domain <https://ontology.swissartresearch.net/aaao/ZE14_Similarity_Status> ;
    rdfs:range <http://www.cidoc-crm.org/cidoc-crm/E1_CRM_Entity> ;
    rdfs:subPropertyOf <https://ontology.swissartresearch.net/aaao/ZP2_ascribes_intentional_target> ;
    skos:notation "ZP44"^^xsd:string .

<https://ontology.swissartresearch.net/aaao/ZP44i_is_similarity_target_ascribed_by> a rdf:Property ;
    rdfs:label "is similarity target ascribed by"@en ;
    rdfs:comment "This property is the inverse of the forward property described in the scope note that follows. This property is used to indicate the other entity for which the similarity status is taken to hold."@en ;
    rdfs:domain <http://www.cidoc-crm.org/cidoc-crm/E1_CRM_Entity> ;
    rdfs:range <https://ontology.swissartresearch.net/aaao/ZE14_Similarity_Status> ;
    rdfs:subPropertyOf <https://ontology.swissartresearch.net/aaao/ZP2i_is_intentional_target_ascribed_by> ;
    skos:notation "ZP44i"^^xsd:string .

<https://ontology.swissartresearch.net/aaao/ZP45_ascribes_similarity_relation> a rdf:Property ;
    rdfs:label "ascribes similarity relation"@en ;
    rdfs:comment "This property is used to indicate the specific type of similarity which is indicated as holding between the two entities indicated in the similarity status."@en ;
    rdfs:domain <https://ontology.swissartresearch.net/aaao/ZE14_Similarity_Status> ;
    rdfs:range <http://www.cidoc-crm.org/cidoc-crm/E55_Type> ;
    rdfs:subPropertyOf <https://ontology.swissartresearch.net/aaao/ZP3_ascribes_intentional_relation> ;
    skos:notation "ZP45"^^xsd:string .

<https://ontology.swissartresearch.net/aaao/ZP45i_is_similarity_relation_ascribed_by> a rdf:Property ;
    rdfs:label "is similarity relation ascribed by"@en ;
    rdfs:comment "This property is the inverse of the forward property described in the scope note that follows. This property is used to indicate the specific type of similarity which is indicated as holding between the two entities indicated in the similarity status."@en ;
    rdfs:domain <http://www.cidoc-crm.org/cidoc-crm/E55_Type> ;
    rdfs:range <https://ontology.swissartresearch.net/aaao/ZE14_Similarity_Status> ;
    rdfs:subPropertyOf <https://ontology.swissartresearch.net/aaao/ZP3i_is_intentional_relation_ascribed_by> ;
    skos:notation "ZP45i"^^xsd:string .

<https://ontology.swissartresearch.net/aaao/ZP46_ascribes_similarity_mode> a rdf:Property ;
    rdfs:label "ascribes similarity mode"@en ;
    rdfs:comment "This property is used to indicate the specific manner in which the similarity status, which is indicated as holding between the two entities indicated in the similarity status, is the case. It''s function corresponds with the .1 properties in CIDOC-CRM 7.1.1."@en ;
    rdfs:domain <https://ontology.swissartresearch.net/aaao/ZE14_Similarity_Status> ;
    rdfs:range <http://www.cidoc-crm.org/cidoc-crm/E55_Type> ;
    skos:notation "ZP46"^^xsd:string .

<https://ontology.swissartresearch.net/aaao/ZP46i_is_similarity_mode_ascribed_by> a rdf:Property ;
    rdfs:label "is similarity mode ascribed by"@en ;
    rdfs:comment "This property is the inverse of the forward property described in the scope note that follows. This property is used to indicate the specific manner in which the similarity status, which is indicated as holding between the two entities indicated in the similarity status, is the case. It''s function corresponds with the .1 properties in CIDOC-CRM 7.1.1."@en ;
    rdfs:domain <http://www.cidoc-crm.org/cidoc-crm/E55_Type> ;
    rdfs:range <https://ontology.swissartresearch.net/aaao/ZE14_Similarity_Status> ;
    skos:notation "ZP46i"^^xsd:string .

<https://ontology.swissartresearch.net/aaao/ZP47_has_set_belonging_subject> a rdf:Property ;
    rdfs:label "has set belonging subject"@en ;
    rdfs:comment "This property is used to indicate an entity which is taken as belonging to a particular set by the instance of set status."@en ;
    rdfs:domain <https://ontology.swissartresearch.net/aaao/ZE15_Set_Status> ;
    rdfs:range <http://www.cidoc-crm.org/cidoc-crm/E1_CRM_Entity> ;
    rdfs:subPropertyOf <https://ontology.swissartresearch.net/aaao/ZP1_has_intentional_subject> ;
    skos:notation "ZP47"^^xsd:string .

<https://ontology.swissartresearch.net/aaao/ZP47i_is_set_belonging_subject_of> a rdf:Property ;
    rdfs:label "is set belonging subject of"@en ;
    rdfs:comment "This property is the inverse of the forward property described in the scope note that follows. This property is used to indicate an entity which is taken as belonging to a particular set by the instance of set status."@en ;
    rdfs:domain <http://www.cidoc-crm.org/cidoc-crm/E1_CRM_Entity> ;
    rdfs:range <https://ontology.swissartresearch.net/aaao/ZE15_Set_Status> ;
    rdfs:subPropertyOf <https://ontology.swissartresearch.net/aaao/ZP1i_is_intentional_subject_of> ;
    skos:notation "ZP47i"^^xsd:string .

<https://ontology.swissartresearch.net/aaao/ZP48_ascribes_set> a rdf:Property ;
    rdfs:label "ascribes set"@en ;
    rdfs:comment "This property is used to indicate the set to which an entity is indicated as belonging ."@en ;
    rdfs:domain <https://ontology.swissartresearch.net/aaao/ZE15_Set_Status> ;
    rdfs:range <https://ontology.swissartresearch.net/aaao/ZE24_Notional_Set> ;
    rdfs:subPropertyOf <https://ontology.swissartresearch.net/aaao/ZP2_ascribes_intentional_target> ;
    skos:notation "ZP48"^^xsd:string .

<https://ontology.swissartresearch.net/aaao/ZP48i_is_set_ascribed_by> a rdf:Property ;
    rdfs:label "is set ascribed by"@en ;
    rdfs:comment "This property is the inverse of the forward property described in the scope note that follows. This property is used to indicate the set to which an entity is indicated as belonging ."@en ;
    rdfs:domain <https://ontology.swissartresearch.net/aaao/ZE24_Notional_Set> ;
    rdfs:range <https://ontology.swissartresearch.net/aaao/ZE15_Set_Status> ;
    rdfs:subPropertyOf <https://ontology.swissartresearch.net/aaao/ZP2i_is_intentional_target_ascribed_by> ;
    skos:notation "ZP48i"^^xsd:string .

<https://ontology.swissartresearch.net/aaao/ZP49_ascribes_set_belonging_relation> a rdf:Property ;
    rdfs:label "ascribes set belonging relation"@en ;
    rdfs:comment "This property is used to indicate the specific type of belonging to the set which is indicated as holding between the subject entity and the target set."@en ;
    rdfs:domain <https://ontology.swissartresearch.net/aaao/ZE15_Set_Status> ;
    rdfs:range <http://www.cidoc-crm.org/cidoc-crm/E55_Type> ;
    rdfs:subPropertyOf <https://ontology.swissartresearch.net/aaao/ZP3_ascribes_intentional_relation> ;
    skos:notation "ZP49"^^xsd:string .

<https://ontology.swissartresearch.net/aaao/ZP49i_is_set_belonging_relation_ascribed_by> a rdf:Property ;
    rdfs:label "is set belonging subject of"@en ;
    rdfs:comment "This property is the inverse of the forward property described in the scope note that follows. This property is used to indicate the specific type of belonging to the set which is indicated as holding between the subject entity and the target set."@en ;
    rdfs:domain <http://www.cidoc-crm.org/cidoc-crm/E55_Type> ;
    rdfs:range <https://ontology.swissartresearch.net/aaao/ZE15_Set_Status> ;
    rdfs:subPropertyOf <https://ontology.swissartresearch.net/aaao/ZP3i_is_intentional_relation_ascribed_by> ;
    skos:notation "ZP49i"^^xsd:string .

<https://ontology.swissartresearch.net/aaao/ZP4_holds_for> a rdf:Property ;
    rdfs:label "holds for"@en ;
    rdfs:comment "This property is used to indicate the community or group for whom an instance of institutional fact holds. Institutional facts have identity only relative to some group for whom they have a significance as formulated through a chosen symbolic system."@en ;
    rdfs:domain <https://ontology.swissartresearch.net/aaao/ZE1_Institutional_Fact> ;
    rdfs:range <http://www.cidoc-crm.org/cidoc-crm/E74_Group> ;
    skos:notation "ZP4"^^xsd:string .

<https://ontology.swissartresearch.net/aaao/ZP4i_holds> a rdf:Property ;
    rdfs:label "holds"@en ;
    rdfs:comment "This property is the inverse of the forward property described in the scope note that follows. This property is used to indicate the community or group for whom an instance of institutional fact holds. Institutional facts have identity only relative to some group for whom they have a significance as formulated through a chosen symbolic system. "@en ;
    rdfs:domain <http://www.cidoc-crm.org/cidoc-crm/E74_Group> ;
    rdfs:range <https://ontology.swissartresearch.net/aaao/ZE1_Institutional_Fact> ;
    skos:notation "ZP4i"^^xsd:string .

<https://ontology.swissartresearch.net/aaao/ZP51_has_former_or_current_set_member> a rdf:Property ;
    rdfs:label "has former or current set member"@en ;
    rdfs:comment "This property is used to connect an instance of set to an entity considered to be one of its members."@en ;
    rdfs:domain <https://ontology.swissartresearch.net/aaao/ZE24_Notional_Set> ;
    rdfs:range <http://www.cidoc-crm.org/cidoc-crm/E1_CRM_Entity> ;
    skos:notation "ZP51"^^xsd:string .

<https://ontology.swissartresearch.net/aaao/ZP51i_is_current_or_former_set_member_of> a rdf:Property ;
    rdfs:label "is current or former member of"@en ;
    rdfs:comment "This property is the inverse of the forward property described in the scope note that follows. This property is used to connect an instance of set to an entity considered to be one of its members."@en ;
    rdfs:domain <http://www.cidoc-crm.org/cidoc-crm/E1_CRM_Entity> ;
    rdfs:range <https://ontology.swissartresearch.net/aaao/ZE24_Notional_Set> ;
    skos:notation "ZP51i"^^xsd:string .

<https://ontology.swissartresearch.net/aaao/ZP52_intentionally_terminated> a rdf:Property ;
    rdfs:label "intentionally terminated"@en ;
    rdfs:comment "This property is used to connect an instance of transformative symbolic act to the instance of institutional fact which it cancels through the successful performance of a specified norm type conformant symbolic act."@en ;
    rdfs:domain <https://ontology.swissartresearch.net/aaao/ZE52_Transformative_Symbolic_Act> ;
    rdfs:range <https://ontology.swissartresearch.net/aaao/ZE1_Institutional_Fact> ;
    rdfs:subPropertyOf <https://ontology.swissartresearch.net/aaao/ZP112_terminated> ;
    skos:notation "ZP52"^^xsd:string .

<https://ontology.swissartresearch.net/aaao/ZP52i_was_intentionally_terminated_by> a rdf:Property ;
    rdfs:label "was intentionally terminated by"@en ;
    rdfs:comment "This property is the inverse of the forward property described in the scope note that follows. This property is used to connect the instance of speech act to the instance of institutional fact which it cancels through the correct performance of the specified performance to bring about the norm type it aimed to bring about."@en ;
    rdfs:domain <https://ontology.swissartresearch.net/aaao/ZE1_Institutional_Fact> ;
    rdfs:range <https://ontology.swissartresearch.net/aaao/ZE13_Speech_Act> ;
    skos:notation "ZP52i"^^xsd:string .

<https://ontology.swissartresearch.net/aaao/ZP53i_had_institutional_fact_initiated_by> a rdf:Property ;
    rdfs:label "had institutional fact initiated by"@en ;
    rdfs:comment """This property is the inverse of the forward property described in the scope note that follows. This property is used to connect the instance of speech act to the instance of group for whom it initiates the existence of a social fact through its performance.
It serves as a shortcut for the fully developed semantic pathway, which instantiates the ZE1 Institutional Fact, in the path ZE13 Speech Act -> ZP42 intentionally initiated -> ZE1 Institutional Fact -> ZP4 held by -> E74 Group."""@en ;
    rdfs:domain <http://www.cidoc-crm.org/cidoc-crm/E74_Group> ;
    rdfs:range <https://ontology.swissartresearch.net/aaao/ZE13_Speech_Act> ;
    skos:notation "ZP53i"^^xsd:string .

<https://ontology.swissartresearch.net/aaao/ZP54_ascribes_relative_date> a rdf:Property ;
    rdfs:label "ascribes relative date"@en ;
    rdfs:comment "This property is used to connect the instance of dating status to the instance of a period to which another instance of period is related for the purposes of datation."@en ;
    rdfs:domain <https://ontology.swissartresearch.net/aaao/ZE25_Dating_Status> ;
    rdfs:range <http://www.cidoc-crm.org/cidoc-crm/E4_Period> ;
    rdfs:subPropertyOf <https://ontology.swissartresearch.net/aaao/ZP2_ascribes_intentional_target> ;
    skos:notation "ZP54"^^xsd:string .

<https://ontology.swissartresearch.net/aaao/ZP54i_is_relative_date_ascribed_by> a rdf:Property ;
    rdfs:label "is relative date ascribed by"@en ;
    rdfs:comment "This property is the inverse of the forward property described in the scope note that follows. This property is used to connect the instance of dating status to the instance of a period to which another instance of period is related for the purposes of datation."@en ;
    rdfs:domain <http://www.cidoc-crm.org/cidoc-crm/E4_Period> ;
    rdfs:range <https://ontology.swissartresearch.net/aaao/ZE25_Dating_Status> ;
    rdfs:subPropertyOf <https://ontology.swissartresearch.net/aaao/ZP2i_is_intentional_target_ascribed_by> ;
    skos:notation "ZP54i"^^xsd:string .

<https://ontology.swissartresearch.net/aaao/ZP55_has_dating_subject> a rdf:Property ;
    rdfs:label "has dating subject"@en ;
    rdfs:comment "This property is used to connect the instance of dating status to an instance of a period typically associated with the existence or use of a physical thing or an object which is the ultimate object of inquiry."@en ;
    rdfs:domain <https://ontology.swissartresearch.net/aaao/ZE25_Dating_Status> ;
    rdfs:range <http://www.cidoc-crm.org/cidoc-crm/E4_Period> ;
    rdfs:subPropertyOf <https://ontology.swissartresearch.net/aaao/ZP1_has_intentional_subject> ;
    skos:notation "ZP55"^^xsd:string .

<https://ontology.swissartresearch.net/aaao/ZP55i_is_dating_subject_of> a rdf:Property ;
    rdfs:label "is dating subject of"@en ;
    rdfs:comment "This property is the inverse of the forward property described in the scope note that follows. This property is used to connect the instance of dating status to an instance of a period typically associated with the existence or use of a physical thing or an object which is the ultimate object of inquiry."@en ;
    rdfs:domain <http://www.cidoc-crm.org/cidoc-crm/E4_Period> ;
    rdfs:range <https://ontology.swissartresearch.net/aaao/ZE25_Dating_Status> ;
    rdfs:subPropertyOf <https://ontology.swissartresearch.net/aaao/ZP1i_is_intentional_subject_of> ;
    skos:notation "ZP55i"^^xsd:string .

<https://ontology.swissartresearch.net/aaao/ZP56_ascribes_dating_relation> a rdf:Property ;
    rdfs:label "ascribes dating relation"@en ;
    rdfs:comment "This property is used to assign the type of relationship the dated period of the object under investigation bears towards the period assigned to it as its datation."@en ;
    rdfs:domain <https://ontology.swissartresearch.net/aaao/ZE25_Dating_Status> ;
    rdfs:range <http://www.cidoc-crm.org/cidoc-crm/E55_Type> ;
    rdfs:subPropertyOf <https://ontology.swissartresearch.net/aaao/ZP3_ascribes_intentional_relation> ;
    skos:notation "ZP56"^^xsd:string .

<https://ontology.swissartresearch.net/aaao/ZP56i_is_dating_relation_ascribed_by> a rdf:Property ;
    rdfs:label "is dating relation ascribed by"@en ;
    rdfs:comment "This property is the inverse of the forward property described in the scope note that follows. This property is used to assign the type of relationship the dated period of the object under investigation bears towards the period assigned to it as its datation."@en ;
    rdfs:domain <http://www.cidoc-crm.org/cidoc-crm/E55_Type> ;
    rdfs:range <https://ontology.swissartresearch.net/aaao/ZE25_Dating_Status> ;
    rdfs:subPropertyOf <https://ontology.swissartresearch.net/aaao/ZP3i_is_intentional_relation_ascribed_by> ;
    skos:notation "ZP56i"^^xsd:string .

<https://ontology.swissartresearch.net/aaao/ZP57_has_obligation_subject> a rdf:Property ;
    rdfs:label "has obligation subject"@en ;
    rdfs:comment "This property is used to indicate a dimension which represents an amount of debt owed from one party to another within an instance of formal obligation."@en ;
    rdfs:domain <https://ontology.swissartresearch.net/aaao/ZE28_Obligation_Status> ;
    rdfs:range <http://www.cidoc-crm.org/cidoc-crm/E54_Dimension> ;
    rdfs:subPropertyOf <https://ontology.swissartresearch.net/aaao/ZP89_has_promisory_subject> ;
    skos:notation "ZP57"^^xsd:string .

<https://ontology.swissartresearch.net/aaao/ZP57i_is_obligation_subject_of> a rdf:Property ;
    rdfs:label "is obligation subject of"@en ;
    rdfs:comment "This property is the inverse of the forward property described in the scope note that follows. This property is used to indicate a dimension which represents an amount of debt owed from one party to another within an instance of formal obligation."@en ;
    rdfs:domain <http://www.cidoc-crm.org/cidoc-crm/E54_Dimension> ;
    rdfs:range <https://ontology.swissartresearch.net/aaao/ZE28_Obligation_Status> ;
    rdfs:subPropertyOf <https://ontology.swissartresearch.net/aaao/ZP1i_is_intentional_subject_of> ;
    skos:notation "ZP57i"^^xsd:string .

<https://ontology.swissartresearch.net/aaao/ZP58_ascribes_debtor> a rdf:Property ;
    rdfs:label "ascribes debtor"@en ;
    rdfs:comment "This property is used to indicate an actor whom is bound by an obligation which it is their duty to repay."@en ;
    rdfs:domain <https://ontology.swissartresearch.net/aaao/ZE28_Obligation_Status> ;
    rdfs:range <http://www.cidoc-crm.org/cidoc-crm/E39_Actor> ;
    rdfs:subPropertyOf <https://ontology.swissartresearch.net/aaao/ZP87_ascribes_promisor> ;
    skos:notation "ZP58"^^xsd:string .

<https://ontology.swissartresearch.net/aaao/ZP58i_is_debtor_ascribed_by> a rdf:Property ;
    rdfs:label "is debtor ascribed by"@en ;
    rdfs:comment "This property is the inverse of the forward property described in the scope note that follows. This property is used to indicate an actor whom is bound by an obligation which it is their duty to repay."@en ;
    rdfs:domain <http://www.cidoc-crm.org/cidoc-crm/E39_Actor> ;
    rdfs:range <https://ontology.swissartresearch.net/aaao/ZE28_Obligation_Status> ;
    rdfs:subPropertyOf <https://ontology.swissartresearch.net/aaao/ZP2i_is_intentional_target_ascribed_by> ;
    skos:notation "ZP58i"^^xsd:string .

<https://ontology.swissartresearch.net/aaao/ZP59_ascribes_obligation_relation> a rdf:Property ;
    rdfs:label "ascribes obligation relation"@en ;
    rdfs:comment "This property is used to indicate the specific type of obligation relation that holds between the debtor and the obligation."@en ;
    rdfs:domain <https://ontology.swissartresearch.net/aaao/ZE28_Obligation_Status> ;
    rdfs:range <http://www.cidoc-crm.org/cidoc-crm/E55_Type> ;
    rdfs:subPropertyOf <https://ontology.swissartresearch.net/aaao/ZP90_ascribes_promisory_relation> ;
    skos:notation "ZP59"^^xsd:string .

<https://ontology.swissartresearch.net/aaao/ZP59i_is_oglibation_relation_ascribed_by> a rdf:Property ;
    rdfs:label "is obligation relation ascribed by"@en ;
    rdfs:comment "This property is the inverse of the forward property described in the scope note that follows. This property is used to indicate the specific type of obligation relation that holds between the two parties."@en ;
    rdfs:domain <http://www.cidoc-crm.org/cidoc-crm/E55_Type> ;
    rdfs:range <https://ontology.swissartresearch.net/aaao/ZE28_Obligation_Status> ;
    rdfs:subPropertyOf <https://ontology.swissartresearch.net/aaao/ZP3i_is_intentional_relation_ascribed_by> ;
    skos:notation "ZP59i"^^xsd:string .

<https://ontology.swissartresearch.net/aaao/ZP60_ascribes_debtee> a rdf:Property ;
    rdfs:label "ascribes debtee"@en ;
    rdfs:comment "This property is used to indicate the actor to whom an obligation is owed in the context of an obligation."@en ;
    rdfs:domain <https://ontology.swissartresearch.net/aaao/ZE28_Obligation_Status> ;
    rdfs:range <http://www.cidoc-crm.org/cidoc-crm/E39_Actor> ;
    rdfs:subPropertyOf <https://ontology.swissartresearch.net/aaao/ZP86_ascribes_promissee> ;
    skos:notation "ZP60"^^xsd:string .

<https://ontology.swissartresearch.net/aaao/ZP60i_is_debtee_ascribed_by> a rdf:Property ;
    rdfs:label "is debtee ascribed by"@en ;
    rdfs:comment "This property is the inverse of the forward property described in the scope note that follows. This property is used to indicate the actor to whom an obligation is owed in the context of an obligation."@en ;
    rdfs:domain <http://www.cidoc-crm.org/cidoc-crm/E39_Actor> ;
    rdfs:range <https://ontology.swissartresearch.net/aaao/ZE28_Obligation_Status> ;
    rdfs:subPropertyOf <https://ontology.swissartresearch.net/aaao/ZP2i_is_intentional_target_ascribed_by> ;
    skos:notation "ZP60i"^^xsd:string .

<https://ontology.swissartresearch.net/aaao/ZP61_transferred_property_right_to> a rdf:Property ;
    rdfs:label "transferred property right to"@en ;
    rdfs:comment "This property is used to indicate the receiver of a property right from another party within the context of a transfer of property right."@en ;
    rdfs:domain <https://ontology.swissartresearch.net/aaao/ZE29_Transfer_of_Property_Right> ;
    rdfs:range <http://www.cidoc-crm.org/cidoc-crm/E39_Actor> ;
    rdfs:subPropertyOf <http://www.cidoc-crm.org/cidoc-crm/P14_carried_out_by> ;
    skos:notation "ZP61"^^xsd:string .

<https://ontology.swissartresearch.net/aaao/ZP61i_acquired_property_right_through> a rdf:Property ;
    rdfs:label "acquired property right through"@en ;
    rdfs:comment "This property is the inverse of the forward property described in the scope note that follows. This property is used to indicate the receiver of a property right from another party within the context of a transfer of property right."@en ;
    rdfs:domain <http://www.cidoc-crm.org/cidoc-crm/E39_Actor> ;
    rdfs:range <https://ontology.swissartresearch.net/aaao/ZE29_Transfer_of_Property_Right> ;
    rdfs:subPropertyOf <http://www.cidoc-crm.org/cidoc-crm/P14i_performed> ;
    skos:notation "ZP61i"^^xsd:string .

<https://ontology.swissartresearch.net/aaao/ZP62_transferred_property_right_from> a rdf:Property ;
    rdfs:label "transferred property right from"@en ;
    rdfs:comment "This property is used to indicate the party ceding property right to another party within the context of a transfer of property right."@en ;
    rdfs:domain <https://ontology.swissartresearch.net/aaao/ZE29_Transfer_of_Property_Right> ;
    rdfs:range <http://www.cidoc-crm.org/cidoc-crm/E39_Actor> ;
    rdfs:subPropertyOf <http://www.cidoc-crm.org/cidoc-crm/P14_carried_out_by> ;
    skos:notation "ZP62"^^xsd:string .

<https://ontology.swissartresearch.net/aaao/ZP62i_surrendered_property_right_through> a rdf:Property ;
    rdfs:label "surrendered  property right through"@en ;
    rdfs:comment "This property is the inverse of the forward property described in the scope note that follows. This property is used to indicate the party ceding property right to another party within the context of a transfer of property right."@en ;
    rdfs:domain <http://www.cidoc-crm.org/cidoc-crm/E39_Actor> ;
    rdfs:range <https://ontology.swissartresearch.net/aaao/ZE29_Transfer_of_Property_Right> ;
    rdfs:subPropertyOf <http://www.cidoc-crm.org/cidoc-crm/P14_carried_out_by> ;
    skos:notation "ZP62i"^^xsd:string .

<https://ontology.swissartresearch.net/aaao/ZP63_transferred_property_right_over> a rdf:Property ;
    rdfs:label "transferred property right over"@en ;
    rdfs:comment "This property is used to indicate the legal object over which property right has been transfered from one party to another."@en ;
    rdfs:domain <https://ontology.swissartresearch.net/aaao/ZE29_Transfer_of_Property_Right> ;
    rdfs:range <http://www.cidoc-crm.org/cidoc-crm/E72_Legal_Object> ;
    rdfs:subPropertyOf <http://www.cidoc-crm.org/cidoc-crm/P16_used_specific_object> ;
    skos:notation "ZP63"^^xsd:string .

<https://ontology.swissartresearch.net/aaao/ZP63i_had_change_in_property_right_through> a rdf:Property ;
    rdfs:label "had change in property right through"@en ;
    rdfs:comment "This property is the inverse of the forward property described in the scope note that follows. This property is used to indicate the legal object over which property right has been transfered from one party to another."@en ;
    rdfs:domain <http://www.cidoc-crm.org/cidoc-crm/E72_Legal_Object> ;
    rdfs:range <https://ontology.swissartresearch.net/aaao/ZE29_Transfer_of_Property_Right> ;
    rdfs:subPropertyOf <http://www.cidoc-crm.org/cidoc-crm/P16i_was_used_for> ;
    skos:notation "ZP63i"^^xsd:string .

<https://ontology.swissartresearch.net/aaao/ZP64_has_property_right_subject> a rdf:Property ;
    rdfs:label "has property right subject"@en ;
    rdfs:comment "This property is used to indicate an object that is subject to a property right of some actor."@en ;
    rdfs:domain <https://ontology.swissartresearch.net/aaao/ZE30_Property_Right_Status> ;
    rdfs:range <http://www.cidoc-crm.org/cidoc-crm/E72_Legal_Object> ;
    rdfs:subPropertyOf <https://ontology.swissartresearch.net/aaao/ZP1_has_intentional_subject> ;
    skos:notation "ZP64"^^xsd:string .

<https://ontology.swissartresearch.net/aaao/ZP64i_is_property_subject_of> a rdf:Property ;
    rdfs:label "is property right subject of"@en ;
    rdfs:comment "This property is the inverse of the forward property described in the scope note that follows. This property is used to indicate an object that is subject to a property right of some actor."@en ;
    rdfs:domain <http://www.cidoc-crm.org/cidoc-crm/E72_Legal_Object> ;
    rdfs:range <https://ontology.swissartresearch.net/aaao/ZE30_Property_Right_Status> ;
    rdfs:subPropertyOf <https://ontology.swissartresearch.net/aaao/ZP1i_is_intentional_subject_of> ;
    skos:notation "ZP64i"^^xsd:string .

<https://ontology.swissartresearch.net/aaao/ZP65_ascribes_property_right_holder> a rdf:Property ;
    rdfs:label "ascribes property right holder"@en ;
    rdfs:comment "This property is used to indicate an actor who holds a right over a legal object within the context of a property right status."@en ;
    rdfs:domain <https://ontology.swissartresearch.net/aaao/ZE30_Property_Right_Status> ;
    rdfs:range <http://www.cidoc-crm.org/cidoc-crm/E39_Actor> ;
    rdfs:subPropertyOf <https://ontology.swissartresearch.net/aaao/ZP2_ascribes_intentional_target> ;
    skos:notation "ZP65"^^xsd:string .

<https://ontology.swissartresearch.net/aaao/ZP65i_is_property_right_holder_ascribed_by> a rdf:Property ;
    rdfs:label "is property right holder ascribed by"@en ;
    rdfs:comment "This property is the inverse of the forward property described in the scope note that follows. This property is used to indicate an actor who holds a right over a legal object within the context of a property right status."@en ;
    rdfs:domain <http://www.cidoc-crm.org/cidoc-crm/E39_Actor> ;
    rdfs:range <https://ontology.swissartresearch.net/aaao/ZE30_Property_Right_Status> ;
    rdfs:subPropertyOf <https://ontology.swissartresearch.net/aaao/ZP2i_is_intentional_target_ascribed_by> ;
    skos:notation "ZP65i"^^xsd:string .

<https://ontology.swissartresearch.net/aaao/ZP66_ascribes_property_right_relation> a rdf:Property ;
    rdfs:label "ascribes property right relation"@en ;
    rdfs:comment "This property is used to indicate the specific type of property right relation that is held over the legal object by the actor in the context of a property right status."@en ;
    rdfs:domain <https://ontology.swissartresearch.net/aaao/ZE30_Property_Right_Status> ;
    rdfs:range <http://www.cidoc-crm.org/cidoc-crm/E55_Type> ;
    rdfs:subPropertyOf <https://ontology.swissartresearch.net/aaao/ZP3_ascribes_intentional_relation> ;
    skos:notation "ZP66"^^xsd:string .

<https://ontology.swissartresearch.net/aaao/ZP66i_is_property_right_relation_ascribed_by> a rdf:Property ;
    rdfs:label "is property right relation ascribed by"@en ;
    rdfs:comment "This property is the inverse of the forward property described in the scope note that follows. This property is used to indicate the specific type of property right relation that is held over the legal object by the actor in the context of a property right status."@en ;
    rdfs:domain <http://www.cidoc-crm.org/cidoc-crm/E55_Type> ;
    rdfs:range <https://ontology.swissartresearch.net/aaao/ZE30_Property_Right_Status> ;
    rdfs:subPropertyOf <https://ontology.swissartresearch.net/aaao/ZP3i_is_intentional_relation_ascribed_by> ;
    skos:notation "ZP66i"^^xsd:string .

<https://ontology.swissartresearch.net/aaao/ZP67_generated_obligation_upon> a rdf:Property ;
    rdfs:label "generated obligation upon"@en ;
    rdfs:comment "This property is used to indicate the party who owes another party within the the context of a declaration of obligation."@en ;
    rdfs:domain <https://ontology.swissartresearch.net/aaao/ZE27_Declaration_of_Obligation> ;
    rdfs:range <http://www.cidoc-crm.org/cidoc-crm/E39_Actor> ;
    rdfs:subPropertyOf <http://www.cidoc-crm.org/cidoc-crm/P14_carried_out_by> ;
    skos:notation "ZP67"^^xsd:string .

<https://ontology.swissartresearch.net/aaao/ZP67i_had_obligation_generated_upon_by> a rdf:Property ;
    rdfs:label "had obligation generated upon by"@en ;
    rdfs:comment "This property is the inverse of the forward property described in the scope note that follows. This property is used to indicate the party who owes another party within the the context of a declaration of obligation."@en ;
    rdfs:domain <http://www.cidoc-crm.org/cidoc-crm/E39_Actor> ;
    rdfs:range <https://ontology.swissartresearch.net/aaao/ZE27_Declaration_of_Obligation> ;
    rdfs:subPropertyOf <http://www.cidoc-crm.org/cidoc-crm/P14i_performed> ;
    skos:notation "ZP67i"^^xsd:string .

<https://ontology.swissartresearch.net/aaao/ZP68_generated_obligation_to> a rdf:Property ;
    rdfs:label "generated obligation to"@en ;
    rdfs:comment "This property is used to indicate the party who is owed by another party within the the context of a declaration of obligation."@en ;
    rdfs:domain <https://ontology.swissartresearch.net/aaao/ZE27_Declaration_of_Obligation> ;
    rdfs:range <http://www.cidoc-crm.org/cidoc-crm/E39_Actor> ;
    rdfs:subPropertyOf <http://www.cidoc-crm.org/cidoc-crm/P14_carried_out_by> ;
    skos:notation "ZP68"^^xsd:string .

<https://ontology.swissartresearch.net/aaao/ZP68i_had_obligation_to_generated_by> a rdf:Property ;
    rdfs:label "had obligation generated to by"@en ;
    rdfs:comment "This property is the inverse of the forward property described in the scope note that follows. This property is used to indicate the party who is owed by another party within the the context of a declaration of obligation."@en ;
    rdfs:domain <http://www.cidoc-crm.org/cidoc-crm/E39_Actor> ;
    rdfs:range <https://ontology.swissartresearch.net/aaao/ZE27_Declaration_of_Obligation> ;
    rdfs:subPropertyOf <http://www.cidoc-crm.org/cidoc-crm/P14i_performed> ;
    skos:notation "ZP68i"^^xsd:string .

<https://ontology.swissartresearch.net/aaao/ZP69_generated_obligation_of> a rdf:Property ;
    rdfs:label "generated obligation of"@en ;
    rdfs:comment "This property is used to indicate the specific amount owed by one party to another within the context of a declaration of obligation."@en ;
    rdfs:domain <https://ontology.swissartresearch.net/aaao/ZE27_Declaration_of_Obligation> ;
    rdfs:range <http://www.cidoc-crm.org/cidoc-crm/E54_Dimension> ;
    skos:notation "ZP69"^^xsd:string .

<https://ontology.swissartresearch.net/aaao/ZP69i_is_obligation_generated_by> a rdf:Property ;
    rdfs:label "is obligation generated by"@en ;
    rdfs:comment "This property is the inverse of the forward property described in the scope note that follows. This property is used to indicate the specific amount owed by one party to another within the context of a declaration of obligation."@en ;
    rdfs:domain <http://www.cidoc-crm.org/cidoc-crm/E54_Dimension> ;
    rdfs:range <https://ontology.swissartresearch.net/aaao/ZE27_Declaration_of_Obligation> ;
    skos:notation "ZP69i"^^xsd:string .

<https://ontology.swissartresearch.net/aaao/ZP70_ascribes_social_status_in_relation_to> a rdf:Property ;
    rdfs:label "ascribes social status in relation to"@en ;
    rdfs:comment "This property is used to indicate a third party actor for whom another''s social status holds relevance (in the form of rights and/or responsibilities that are thus due to them) in the instance of social status."@en ;
    rdfs:domain <https://ontology.swissartresearch.net/aaao/ZE6_Social_Status> ;
    rdfs:range <http://www.cidoc-crm.org/cidoc-crm/E39_Actor> ;
    skos:notation "ZP70"^^xsd:string .

<https://ontology.swissartresearch.net/aaao/ZP70i_is_relative_party_of> a rdf:Property ;
    rdfs:label "is  relative party of"@en ;
    rdfs:comment "This property is the inverse of the forward property described in the scope note that follows. This property is used to indicate a third party actor for whom another''s social status holds relevance (in the form of rights and/or responsibilities that are thus due to them) in the instance of social status."@en ;
    rdfs:domain <http://www.cidoc-crm.org/cidoc-crm/E39_Actor> ;
    rdfs:range <https://ontology.swissartresearch.net/aaao/ZE6_Social_Status> ;
    skos:notation "ZP70i"^^xsd:string .

<https://ontology.swissartresearch.net/aaao/ZP74i_had_institutional_fact_terminated_by> a rdf:Property ;
    rdfs:label "had institutional fact terminated  by"@en ;
    rdfs:comment """This property is the inverse of the forward property described in the scope note that follows. This property is used to connect the instance of speech act to the instance of group for whom it terminates the existence of a social fact through its performance.
It serves as a shortcut for the fully developed semantic pathway, which instantiates the ZE1 Institutional Fact, in the path ZE13 Speech Act -> ZP52 intentionally terminated -> ZE1 Institutional Fact -> ZP4 held by -> E74 Group."""@en ;
    rdfs:domain <http://www.cidoc-crm.org/cidoc-crm/E74_Group> ;
    rdfs:range <https://ontology.swissartresearch.net/aaao/ZE13_Speech_Act> ;
    skos:notation "ZP74i"^^xsd:string .

<https://ontology.swissartresearch.net/aaao/ZP75_applies_for_context> a rdf:Property ;
    rdfs:label "applies for context"@en ;
    rdfs:comment "This property is used to indicate an event context which limits the temporal scope within which an instance of institutional fact is meant to hold. When indicated the event context stands as the frame in which the institutional fact is held to be valid by the associated group for whom it has significance."@en ;
    rdfs:domain <https://ontology.swissartresearch.net/aaao/ZE1_Institutional_Fact> ;
    rdfs:range <http://www.cidoc-crm.org/cidoc-crm/E5_Event> ;
    skos:notation "ZP75"^^xsd:string .

<https://ontology.swissartresearch.net/aaao/ZP75i_is_context_for> a rdf:Property ;
    rdfs:label "is context for"@en ;
    rdfs:comment "This property is the inverse of the forward property described in the scope note that follows. This property is used to indicate an event context which limits the temporal scope within which an instance of institutional fact is meant to hold. When indicated the event context stands as the frame in which the institutional fact is held to be valid by the associcated group for whom it has significance."@en ;
    rdfs:domain <http://www.cidoc-crm.org/cidoc-crm/E5_Event> ;
    rdfs:range <https://ontology.swissartresearch.net/aaao/ZE1_Institutional_Fact> ;
    skos:notation "ZP75i"^^xsd:string .

<https://ontology.swissartresearch.net/aaao/ZP76_applies_for_context_type> a rdf:Property ;
    rdfs:label "applies for context type"@en ;
    rdfs:comment "This property is used to indicate an event context type which limits the spatio-temporal scope within which an instance of institutional fact is meant to hold to certain kinds of event. When indicated the event context type stands as the frame or frames in which the institutional fact is held to be valid by the associated group for whom it has significance."@en ;
    rdfs:domain <https://ontology.swissartresearch.net/aaao/ZE1_Institutional_Fact> ;
    rdfs:range <http://www.cidoc-crm.org/cidoc-crm/E55_Type> ;
    skos:notation "ZP76"^^xsd:string .

<https://ontology.swissartresearch.net/aaao/ZP76i_is_context_type_for> a rdf:Property ;
    rdfs:label "is context type for"@en ;
    rdfs:comment "This property is the inverse of the forward property described in the scope note that follows. This property is used to indicate an event context type which limits the spatio-temporal scope within which an instance of institutional fact is meant to hold to certain kinds of event. When indicated the event context type stands as the frame or frames in which the institutional fact is held to be valid by the associcated group for whom it has significance."@en ;
    rdfs:domain <http://www.cidoc-crm.org/cidoc-crm/E55_Type> ;
    rdfs:range <https://ontology.swissartresearch.net/aaao/ZE1_Institutional_Fact> ;
    skos:notation "ZP76i"^^xsd:string .

<https://ontology.swissartresearch.net/aaao/ZP77i_is_place_ascribed_by> a rdf:Property ;
    rdfs:label "is place ascribed by"@en ;
    rdfs:comment "This property is the inverse of the forward property described in the scope note that follows. This property is used to indicate the place in a locative association that is taken to hold for an entity."@en ;
    rdfs:domain <http://www.cidoc-crm.org/cidoc-crm/E53_Place> ;
    rdfs:range <https://ontology.swissartresearch.net/aaao/ZE35_Locative_Status> ;
    rdfs:subPropertyOf <https://ontology.swissartresearch.net/aaao/ZP2i_is_intentional_target_ascribed_by> ;
    skos:notation "ZP77i"^^xsd:string .

<https://ontology.swissartresearch.net/aaao/ZP78_had_constituent> a rdf:Property ;
    rdfs:label "had constituent"@en ;
    rdfs:comment "This property relates an instance of population to an instance of persons, individual or collective, to which it belongs qua constituent."@en ;
    rdfs:domain <https://ontology.swissartresearch.net/aaao/ZE37_Population> ;
    rdfs:range <https://ontology.swissartresearch.net/aaao/ZE36_Persons> ;
    skos:notation "ZP78"^^xsd:string .

<https://ontology.swissartresearch.net/aaao/ZP78i_was_constituent_of> a rdf:Property ;
    rdfs:label "was constituent of"@en ;
    rdfs:comment "This property is the inverse of the forward property described in the scope note that follows. This property relates an instance of population to an instance of persons, individual or collective, to which it belongs qua constituent."@en ;
    rdfs:domain <https://ontology.swissartresearch.net/aaao/ZE36_Persons> ;
    rdfs:range <https://ontology.swissartresearch.net/aaao/ZE37_Population> ;
    skos:notation "ZP78i"^^xsd:string .

<https://ontology.swissartresearch.net/aaao/ZP79_had_population> a rdf:Property ;
    rdfs:label "had population"@en ;
    rdfs:comment "This property relates an instance of population existence to the population whose existence it was."@en ;
    rdfs:domain <https://ontology.swissartresearch.net/aaao/ZE38_Population_Existence> ;
    rdfs:range <https://ontology.swissartresearch.net/aaao/ZE37_Population> ;
    rdfs:subPropertyOf <http://www.cidoc-crm.org/cidoc-crm/P11_had_participant> ;
    skos:notation "ZP79"^^xsd:string .

<https://ontology.swissartresearch.net/aaao/ZP79i_was_population_of> a rdf:Property ;
    rdfs:label "was population of"@en ;
    rdfs:comment "This property is the inverse of the forward property described in the scope note that follows. This property relates an instance of population existence to the population whose existence it was."@en ;
    rdfs:domain <https://ontology.swissartresearch.net/aaao/ZE37_Population> ;
    rdfs:range <https://ontology.swissartresearch.net/aaao/ZE38_Population_Existence> ;
    rdfs:subPropertyOf <http://www.cidoc-crm.org/cidoc-crm/P11i_participated_in> ;
    skos:notation "ZP79i"^^xsd:string .

<https://ontology.swissartresearch.net/aaao/ZP83_has_physical_locative_subject> a rdf:Property ;
    rdfs:label "has physical locative subject"@en ;
    rdfs:comment "This property is used to designate the instance of physical object whose socially defined location the instance of physical locative status delineates."@en ;
    rdfs:domain <https://ontology.swissartresearch.net/aaao/ZE43_Physical_Locative_Status> ;
    rdfs:range <http://www.cidoc-crm.org/cidoc-crm/E18_Physical_Thing> ;
    rdfs:subPropertyOf <https://ontology.swissartresearch.net/aaao/ZP1_has_intentional_subject> ;
    skos:notation "ZP83"^^xsd:string .

<https://ontology.swissartresearch.net/aaao/ZP83i_is_physical_locative_subject_of> a rdf:Property ;
    rdfs:label "is physical locative subject of"@en ;
    rdfs:comment "This property is the inverse of the forward property described in the scope note that follows. This property is used to designate the instance of physical object whose socially defined location the instance of physical locative status delineates."@en ;
    rdfs:domain <http://www.cidoc-crm.org/cidoc-crm/E18_Physical_Thing> ;
    rdfs:range <https://ontology.swissartresearch.net/aaao/ZE43_Physical_Locative_Status> ;
    rdfs:subPropertyOf <https://ontology.swissartresearch.net/aaao/ZP1i_is_intentional_subject_of> ;
    skos:notation "ZP83i"^^xsd:string .

<https://ontology.swissartresearch.net/aaao/ZP84_ascribes_location_relation> a rdf:Property ;
    rdfs:label "ascribes location relation"@en ;
    rdfs:comment "This property is used to indicate the specific manner in which the physical locative status which is indicated as holding over the physical object pertains to this subject."@en ;
    rdfs:domain <https://ontology.swissartresearch.net/aaao/ZE43_Physical_Locative_Status> ;
    rdfs:range <http://www.cidoc-crm.org/cidoc-crm/E55_Type> ;
    rdfs:subPropertyOf <https://ontology.swissartresearch.net/aaao/ZP3_ascribes_intentional_relation> ;
    skos:notation "ZP84"^^xsd:string .

<https://ontology.swissartresearch.net/aaao/ZP84i_is_location_relation_ascribed_by> a rdf:Property ;
    rdfs:label "is location relation ascribed by"@en ;
    rdfs:comment "This property is the inverse of the forward property described in the scope note that follows. This property is used to indicate the specific manner in which the physical locative status which is indicated as holding over the physical object pertains to this subject."@en ;
    rdfs:domain <http://www.cidoc-crm.org/cidoc-crm/E55_Type> ;
    rdfs:range <https://ontology.swissartresearch.net/aaao/ZE43_Physical_Locative_Status> ;
    rdfs:subPropertyOf <https://ontology.swissartresearch.net/aaao/ZP3i_is_intentional_relation_ascribed_by> ;
    skos:notation "ZP84i"^^xsd:string .

<https://ontology.swissartresearch.net/aaao/ZP85_has_topographical_subject> a rdf:Property ;
    rdfs:label "has topographical subject"@en ;
    rdfs:comment """This property is used to designate the instance of place whose socially defined location the instance of topographical status delineates.
"""@en ;
    rdfs:domain <https://ontology.swissartresearch.net/aaao/ZE44_Topographical_Status> ;
    rdfs:range <http://www.cidoc-crm.org/cidoc-crm/E53_Place> ;
    rdfs:subPropertyOf <https://ontology.swissartresearch.net/aaao/ZP1_has_intentional_subject> ;
    skos:notation "ZP85"^^xsd:string .

<https://ontology.swissartresearch.net/aaao/ZP85i_is_topographical_subject_of> a rdf:Property ;
    rdfs:label "is topographical subject of"@en ;
    rdfs:comment """This property is the inverse of the forward property described in the scope note that follows. This property is used to designate the instance of place whose socially defined location the instance of topographical status delineates.
"""@en ;
    rdfs:domain <http://www.cidoc-crm.org/cidoc-crm/E53_Place> ;
    rdfs:range <https://ontology.swissartresearch.net/aaao/ZE44_Topographical_Status> ;
    rdfs:subPropertyOf <https://ontology.swissartresearch.net/aaao/ZP1i_is_intentional_subject_of> ;
    skos:notation "ZP85i"^^xsd:string .

<https://ontology.swissartresearch.net/aaao/ZP86i_is_promissee_ascribed_by> a rdf:Property ;
    rdfs:label "is promisee ascribed by"@en ;
    rdfs:comment "This property is the inverse of the forward property described in the scope note that follows. This property is used to indicate the actor to whom a promise has been offered in an intentional promise."@en ;
    rdfs:domain <https://ontology.swissartresearch.net/aaao/ZE36_Persons> ;
    rdfs:range <https://ontology.swissartresearch.net/aaao/ZE45_Promisory_Status> ;
    rdfs:subPropertyOf <https://ontology.swissartresearch.net/aaao/ZP2i_is_intentional_target_ascribed_by> ;
    skos:notation "ZP86i"^^xsd:string .

<https://ontology.swissartresearch.net/aaao/ZP87i_is_promisor_ascribed_by> a rdf:Property ;
    rdfs:label "is promisor ascribed by"@en ;
    rdfs:comment "This property is the inverse of the forward property described in the scope note that follows. This property is used to indicate an actor who is bound by a promise which it is their duty to fulfil."@en ;
    rdfs:domain <http://www.cidoc-crm.org/cidoc-crm/E39_Actor> ;
    rdfs:range <https://ontology.swissartresearch.net/aaao/ZE45_Promisory_Status> ;
    rdfs:subPropertyOf <https://ontology.swissartresearch.net/aaao/ZP2i_is_intentional_target_ascribed_by> ;
    skos:notation "ZP87i"^^xsd:string .

<https://ontology.swissartresearch.net/aaao/ZP88_ascribes_topographical_relation> a rdf:Property ;
    rdfs:label "ascribes topographical relation"@en ;
    rdfs:comment "This property is used to indicate the specific manner in which the topographical status which is indicated as holding between two places."@en ;
    rdfs:domain <https://ontology.swissartresearch.net/aaao/ZE44_Topographical_Status> ;
    rdfs:range <http://www.cidoc-crm.org/cidoc-crm/E55_Type> ;
    rdfs:subPropertyOf <https://ontology.swissartresearch.net/aaao/ZP3_ascribes_intentional_relation> ;
    skos:notation "ZP88"^^xsd:string .

<https://ontology.swissartresearch.net/aaao/ZP88i_is_topographical_relation_ascribed_by> a rdf:Property ;
    rdfs:label "is topographical relation ascribed by"@en ;
    rdfs:comment "This property is the inverse of the forward property described in the scope note that follows. This property is used to indicate the specific manner in which the topographical status which is indicated as holding between two places."@en ;
    rdfs:domain <http://www.cidoc-crm.org/cidoc-crm/E55_Type> ;
    rdfs:range <https://ontology.swissartresearch.net/aaao/ZE44_Topographical_Status> ;
    rdfs:subPropertyOf <https://ontology.swissartresearch.net/aaao/ZP3i_is_intentional_relation_ascribed_by> ;
    skos:notation "ZP88i"^^xsd:string .

<https://ontology.swissartresearch.net/aaao/ZP89i_is_promissory_subject_of> a rdf:Property ;
    rdfs:label "is promissory subject of"@en ;
    rdfs:comment "This property is the inverse of the forward property described in the scope note that follows. This property is used to indicate an instance of formulation which represents the promise given from one party to another within an instance of an intentional promise."@en ;
    rdfs:domain <https://ontology.swissartresearch.net/aaao/ZE59_Plan> ;
    rdfs:range <https://ontology.swissartresearch.net/aaao/ZE45_Promisory_Status> ;
    rdfs:subPropertyOf <https://ontology.swissartresearch.net/aaao/ZP1i_is_intentional_subject_of> ;
    skos:notation "ZP89i"^^xsd:string .

<https://ontology.swissartresearch.net/aaao/ZP8_has_contact_point_subject> a rdf:Property ;
    rdfs:label "has contact point subject"@en ;
    rdfs:comment """This property is used to indicate the entity for which a contact point has been specified as means of contact.
"""@en ;
    rdfs:domain <https://ontology.swissartresearch.net/aaao/ZE3_Contact_Point_Status> ;
    rdfs:range <http://www.cidoc-crm.org/cidoc-crm/E39_Actor> ;
    rdfs:subPropertyOf <https://ontology.swissartresearch.net/aaao/ZP5_has_appellative_subject> ;
    skos:notation "ZP8"^^xsd:string .

<https://ontology.swissartresearch.net/aaao/ZP8i_is_contact_point_subject_of> a rdf:Property ;
    rdfs:label "is contact point subject of"@en ;
    rdfs:comment """This property is the inverse of the forward property described in the scope note that follows. This property is used to indicate the entity for which a contact point has been specified as means of contact.
"""@en ;
    rdfs:domain <http://www.cidoc-crm.org/cidoc-crm/E39_Actor> ;
    rdfs:range <https://ontology.swissartresearch.net/aaao/ZE3_Contact_Point_Status> ;
    rdfs:subPropertyOf <https://ontology.swissartresearch.net/aaao/ZP5i_is_appellative_subject_of> ;
    skos:notation "ZP8i"^^xsd:string .

<https://ontology.swissartresearch.net/aaao/ZP90i_is_promissory_relation_ascribed_by> a rdf:Property ;
    rdfs:label "is promissory relation ascribed by"@en ;
    rdfs:comment "This property is the inverse of the forward property described in the scope note that follows. This property is used to indicate the specific type of promise relation that holds between the promisor and the promisee."@en ;
    rdfs:domain <http://www.cidoc-crm.org/cidoc-crm/E55_Type> ;
    rdfs:range <https://ontology.swissartresearch.net/aaao/ZE45_Promisory_Status> ;
    rdfs:subPropertyOf <https://ontology.swissartresearch.net/aaao/ZP3i_is_intentional_relation_ascribed_by> ;
    skos:notation "ZP90i"^^xsd:string .

<https://ontology.swissartresearch.net/aaao/ZP91_generated_promise_of> a rdf:Property ;
    rdfs:label "generated promise of"@en ;
    rdfs:comment "This property associates an instance of promissory agreement to the plan for a futural event (the realized promise) that it generates and which is promised through it."@en ;
    rdfs:domain <https://ontology.swissartresearch.net/aaao/ZE46_Promisory_Agreement> ;
    rdfs:range <https://ontology.swissartresearch.net/aaao/ZE59_Plan> ;
    rdfs:subPropertyOf <http://iflastandards.info/ns/lrm/lrmoo/R17_created> ;
    skos:notation "ZP91"^^xsd:string .

<https://ontology.swissartresearch.net/aaao/ZP91i_is_promise_generated_by> a rdf:Property ;
    rdfs:label "is promise generated by"@en ;
    rdfs:comment "This property is the inverse of the forward property described in the scope note that follows. This property associates an instance of promissory agreement to the plan for a futural event (the realized promise) that it generates and which is promised through it."@en ;
    rdfs:domain <https://ontology.swissartresearch.net/aaao/ZE59_Plan> ;
    rdfs:range <https://ontology.swissartresearch.net/aaao/ZE46_Promisory_Agreement> ;
    rdfs:subPropertyOf <http://iflastandards.info/ns/lrm/lrmoo/R17i_was_created_by> ;
    skos:notation "ZP91i"^^xsd:string .

<https://ontology.swissartresearch.net/aaao/ZP93_has_text_sequence_subject> a rdf:Property ;
    rdfs:label "has text sequence subject"@en ;
    rdfs:comment "This property is used to indicate the text field which has been ascribed a sequential location in relation to another text field."@en ;
    rdfs:domain <https://ontology.swissartresearch.net/aaao/ZE49_Text_Sequence_Status> ;
    rdfs:range <http://www.cidoc-crm.org/extensions/crmtex/TX4_Writing_Field> ;
    rdfs:subPropertyOf <https://ontology.swissartresearch.net/aaao/ZP1_has_intentional_subject> ;
    skos:notation "ZP93"^^xsd:string .

<https://ontology.swissartresearch.net/aaao/ZP93i_is_text_sequence_subject_ascribed_by> a rdf:Property ;
    rdfs:label "is text sequence subject ascribed by"@en ;
    rdfs:comment "This property is the inverse of the forward property described in the scope note that follows. This property is used to indicate the text field which has been ascribed a sequential location in relation to another text field."@en ;
    rdfs:domain <http://www.cidoc-crm.org/extensions/crmtex/TX4_Writing_Field> ;
    rdfs:range <https://ontology.swissartresearch.net/aaao/ZE49_Text_Sequence_Status> ;
    rdfs:subPropertyOf <https://ontology.swissartresearch.net/aaao/ZP1i_is_intentional_subject_of> ;
    skos:notation "ZP93i"^^xsd:string .

<https://ontology.swissartresearch.net/aaao/ZP94_ascribes_text_sequence_correlate> a rdf:Property ;
    rdfs:label "ascribes text sequence correlate"@en ;
    rdfs:comment "This property is used to designate a text field to which another text field has been assigned in order to designate its relative place."@en ;
    rdfs:domain <https://ontology.swissartresearch.net/aaao/ZE49_Text_Sequence_Status> ;
    rdfs:range <http://www.cidoc-crm.org/extensions/crmtex/TX4_Writing_Field> ;
    rdfs:subPropertyOf <https://ontology.swissartresearch.net/aaao/ZP2_ascribes_intentional_target> ;
    skos:notation "ZP94"^^xsd:string .

<https://ontology.swissartresearch.net/aaao/ZP94i_is_text_sequence_correlate_ascribed_by> a rdf:Property ;
    rdfs:label "is text sequence correlate ascribed by"@en ;
    rdfs:comment "This property is the inverse of the forward property described in the scope note that follows. This property is used to designate a text field to which another text field has been assigned in order to designate its relative place."@en ;
    rdfs:domain <http://www.cidoc-crm.org/extensions/crmtex/TX4_Writing_Field> ;
    rdfs:range <https://ontology.swissartresearch.net/aaao/ZE49_Text_Sequence_Status> ;
    rdfs:subPropertyOf <https://ontology.swissartresearch.net/aaao/ZP2i_is_intentional_target_ascribed_by> ;
    skos:notation "ZP94i"^^xsd:string .

<https://ontology.swissartresearch.net/aaao/ZP95_ascribes_text_sequence_relation> a rdf:Property ;
    rdfs:label "ascribes text sequence relation"@en ;
    rdfs:comment "This property is used to indicate the specific manner in which the text sequence status which is indicated as holding over the textual sequence pertains to this subject."@en ;
    rdfs:domain <https://ontology.swissartresearch.net/aaao/ZE49_Text_Sequence_Status> ;
    rdfs:range <http://www.cidoc-crm.org/cidoc-crm/E55_Type> ;
    rdfs:subPropertyOf <https://ontology.swissartresearch.net/aaao/ZP3_ascribes_intentional_relation> ;
    skos:notation "ZP95"^^xsd:string .

<https://ontology.swissartresearch.net/aaao/ZP95i_is_text_sequence_relation_ascribed_by> a rdf:Property ;
    rdfs:label "is text sequence relation ascribed by"@en ;
    rdfs:comment "This property is the inverse of the forward property described in the scope note that follows. This property is used to indicate the specific manner in which the text sequence status which is indicated as holding over the textual sequence pertains to this subject."@en ;
    rdfs:domain <http://www.cidoc-crm.org/cidoc-crm/E55_Type> ;
    rdfs:range <https://ontology.swissartresearch.net/aaao/ZE49_Text_Sequence_Status> ;
    rdfs:subPropertyOf <https://ontology.swissartresearch.net/aaao/ZP3i_is_intentional_relation_ascribed_by> ;
    skos:notation "ZP95i"^^xsd:string .

<https://ontology.swissartresearch.net/aaao/ZP96_has_authority_status_subject> a rdf:Property ;
    rdfs:label "has authority status subject"@en ;
    rdfs:comment "This property is used to indicate the actor which has been ascribed an authority status."@en ;
    rdfs:domain <https://ontology.swissartresearch.net/aaao/ZE50_Authority_Status> ;
    rdfs:range <http://www.cidoc-crm.org/cidoc-crm/E39_Actor> ;
    rdfs:subPropertyOf <https://ontology.swissartresearch.net/aaao/ZP17_has_social_status_subject> ;
    skos:notation "ZP96"^^xsd:string .

<https://ontology.swissartresearch.net/aaao/ZP96i_is_authority_status_subject_of> a rdf:Property ;
    rdfs:label "is authority status subject of"@en ;
    rdfs:comment "This property is the inverse of the forward property described in the scope note that follows. This property is used to indicate the actor which has been ascribed an authority status."@en ;
    rdfs:domain <http://www.cidoc-crm.org/cidoc-crm/E39_Actor> ;
    rdfs:range <https://ontology.swissartresearch.net/aaao/ZE50_Authority_Status> ;
    rdfs:subPropertyOf <https://ontology.swissartresearch.net/aaao/ZP17i_is_social_status_subject_of> ;
    skos:notation "ZP96i"^^xsd:string .

<https://ontology.swissartresearch.net/aaao/ZP97_ascribes_authority_status> a rdf:Property ;
    rdfs:label "ascribes authority status"@en ;
    rdfs:comment "This property is used to indicate the type of authority ascribed to the actor by the authority status."@en ;
    rdfs:domain <https://ontology.swissartresearch.net/aaao/ZE50_Authority_Status> ;
    rdfs:range <http://www.cidoc-crm.org/cidoc-crm/E55_Type> ;
    rdfs:subPropertyOf <https://ontology.swissartresearch.net/aaao/ZP18_ascribes_social_status> ;
    skos:notation "ZP97"^^xsd:string .

<https://ontology.swissartresearch.net/aaao/ZP97i_is_authority_status_ascribed_by> a rdf:Property ;
    rdfs:label "is authority status ascribed by"@en ;
    rdfs:comment "This property is the inverse of the forward property described in the scope note that follows. This property is used to indicate the type of authority ascribed to the actor by the authority status."@en ;
    rdfs:domain <http://www.cidoc-crm.org/cidoc-crm/E55_Type> ;
    rdfs:range <https://ontology.swissartresearch.net/aaao/ZE50_Authority_Status> ;
    rdfs:subPropertyOf <https://ontology.swissartresearch.net/aaao/ZP18i_is_social_status_ascribed_by> ;
    skos:notation "ZP97i"^^xsd:string .

<https://ontology.swissartresearch.net/aaao/ZP9_ascribes_contact_point> a rdf:Property ;
    rdfs:label "ascribes contact point"@en ;
    rdfs:comment """This property is used to indicate the contact point which is indicated as holding for the named subject of the contact status.
"""@en ;
    rdfs:domain <https://ontology.swissartresearch.net/aaao/ZE3_Contact_Point_Status> ;
    rdfs:range <http://www.cidoc-crm.org/cidoc-crm/E42_Identifier> ;
    rdfs:subPropertyOf <https://ontology.swissartresearch.net/aaao/ZP6_ascribes_appellation> ;
    skos:notation "ZP9"^^xsd:string .

<https://ontology.swissartresearch.net/aaao/ZP9i_is_contact_point_ascribed_by> a rdf:Property ;
    rdfs:label "is contact point ascribed by"@en ;
    rdfs:comment """This property is the inverse of the forward property described in the scope note that follows. This property is used to indicate the contact point which is indicated as holding for the named subject of the contact status.
"""@en ;
    rdfs:domain <http://www.cidoc-crm.org/cidoc-crm/E42_Identifier> ;
    rdfs:range <https://ontology.swissartresearch.net/aaao/ZE3_Contact_Point_Status> ;
    rdfs:subPropertyOf <https://ontology.swissartresearch.net/aaao/ZP6i_is_appellation_ascribed_by> ;
    skos:notation "ZP9i"^^xsd:string .

<http://www.cidoc-crm.org/cidoc-crm/P100_was_death_of> a rdf:Property ;
    rdfs:label "Tod von"@de,
        "ήταν θάνατος του/της"@el,
        "was death of"@en,
        "a été la mort de"@fr,
        "foi a morte para"@pt,
        "привёл к смeрти"@ru,
        "死亡的是"@zh ;
    rdfs:comment """This property links an instance of E69 Death to the instance of E21 Person that died.
An instance of E69 Death may involve multiple people, for example in the case of a battle or disaster.
This is not intended for use with general natural history material, only people."""@en ;
    rdfs:domain <http://www.cidoc-crm.org/cidoc-crm/E69_Death> ;
    rdfs:range <http://www.cidoc-crm.org/cidoc-crm/E21_Person> ;
    rdfs:subPropertyOf <http://www.cidoc-crm.org/cidoc-crm/P93_took_out_of_existence> ;
    owl:inverseOf <http://www.cidoc-crm.org/cidoc-crm/P100i_died_in> .

<http://www.cidoc-crm.org/cidoc-crm/P100i_died_in> a rdf:Property ;
    rdfs:label "starb in"@de,
        "πέθανε σε"@el,
        "died in"@en,
        "est mort par"@fr,
        "morreu em"@pt,
        "умeр"@ru,
        "死于"@zh ;
    rdfs:domain <http://www.cidoc-crm.org/cidoc-crm/E21_Person> ;
    rdfs:range <http://www.cidoc-crm.org/cidoc-crm/E69_Death> ;
    rdfs:subPropertyOf <http://www.cidoc-crm.org/cidoc-crm/P93i_was_taken_out_of_existence_by> ;
    owl:inverseOf <http://www.cidoc-crm.org/cidoc-crm/P100_was_death_of> .

<http://www.cidoc-crm.org/cidoc-crm/P101_had_as_general_use> a rdf:Property ;
    rdfs:label "hatte die allgemeine Verwendung"@de,
        "είχε ως γενική χρήση"@el,
        "had as general use"@en,
        "a eu pour usage général"@fr,
        "tem como uso geral"@pt,
        "имeл основноe примeнeниe"@ru,
        "有一般用途"@zh ;
    rdfs:comment """This property associates an instance of E70 Thing with an instance of E55 Type that describes the type of use that it was actually employed for.
It allows the relationship between particular things, both physical and immaterial, and the general methods and techniques of real use to be documented. This may well be different from the intended functional purpose of the instance of E70 Thing (which can be documented with P103 was intended for (was intention of)). For example, it could be recorded that a particular wooden crate had a general use as a shelf support on a market stall even though it had been originally intended for carrying vegetables.
The use of this property is intended to allow the documentation of usage patterns attested in historical records or through scientific investigation (for instance ceramic residue analysis). It should not be used to document the intended, and thus assumed, use of an object."""@en ;
    rdfs:domain <http://www.cidoc-crm.org/cidoc-crm/E70_Thing> ;
    rdfs:range <http://www.cidoc-crm.org/cidoc-crm/E55_Type> ;
    owl:inverseOf <http://www.cidoc-crm.org/cidoc-crm/P101i_was_use_of> .

<http://www.cidoc-crm.org/cidoc-crm/P101i_was_use_of> a rdf:Property ;
    rdfs:label "war die Verwendung von"@de,
        "ήταν χρήση του/της"@el,
        "was use of"@en,
        "a été l'usage général de"@fr,
        "foi uso de"@pt,
        "был использовано для"@ru,
        "被用于"@zh ;
    rdfs:domain <http://www.cidoc-crm.org/cidoc-crm/E55_Type> ;
    rdfs:range <http://www.cidoc-crm.org/cidoc-crm/E70_Thing> ;
    owl:inverseOf <http://www.cidoc-crm.org/cidoc-crm/P101_had_as_general_use> .

<http://www.cidoc-crm.org/cidoc-crm/P102_has_title> a rdf:Property ;
    rdfs:label "trägt den Titel"@de,
        "έχει τίτλο"@el,
        "has title"@en,
        "a pour titre"@fr,
        "tem título"@pt,
        "имeeт названиe"@ru,
        "有题名"@zh ;
    rdfs:comment """This property associates an instance of E35 Title that has been applied to an instance of E71 Human-Made Thing.
The P102.1 has type property of the P102 has title (is title of) property enables the relationship between the title and the thing to be further clarified, for example, if the title was a given title, a supplied title etc.
It allows any human-made material or immaterial thing to be given a title. It is possible to imagine a title being created without a specific object in mind."""@en ;
    rdfs:domain <http://www.cidoc-crm.org/cidoc-crm/E71_Human-Made_Thing> ;
    rdfs:range <http://www.cidoc-crm.org/cidoc-crm/E35_Title> ;
    rdfs:subPropertyOf <http://www.cidoc-crm.org/cidoc-crm/P1_is_identified_by> ;
    owl:inverseOf <http://www.cidoc-crm.org/cidoc-crm/P102i_is_title_of> .

<http://www.cidoc-crm.org/cidoc-crm/P102i_is_title_of> a rdf:Property ;
    rdfs:label "ist der Titel von"@de,
        "είναι τίτλος του/της"@el,
        "is title of"@en,
        "est le titre de"@fr,
        "é título de"@pt,
        "являeтся названиeм"@ru,
        "题名是"@zh ;
    rdfs:domain <http://www.cidoc-crm.org/cidoc-crm/E35_Title> ;
    rdfs:range <http://www.cidoc-crm.org/cidoc-crm/E71_Human-Made_Thing> ;
    rdfs:subPropertyOf <http://www.cidoc-crm.org/cidoc-crm/P1i_identifies> ;
    owl:inverseOf <http://www.cidoc-crm.org/cidoc-crm/P102_has_title> .

<http://www.cidoc-crm.org/cidoc-crm/P103_was_intended_for> a rdf:Property ;
    rdfs:label "bestimmt für"@de,
        "προοριζόταν για"@el,
        "was intended for"@en,
        "a eu pour raison d'être"@fr,
        "era destinado à"@pt,
        "планировался для"@ru,
        "被用于"@zh ;
    rdfs:comment """This property links an instance of E71 Human-Made Thing to an instance of E55 Type of usage or audience. It creates a relation between specific human-made things, both physical and immaterial, to E55 Types. This property can be used to specify intended methods and techniques of use or to characterise the intended audience by indicating a type of personal characteristic that everyone falling into the target audience has.
Note: A link between specific human-made things and a specific use activity should be expressed using P19 was intended use of (was made for)."""@en ;
    rdfs:domain <http://www.cidoc-crm.org/cidoc-crm/E71_Human-Made_Thing> ;
    rdfs:range <http://www.cidoc-crm.org/cidoc-crm/E55_Type> ;
    owl:inverseOf <http://www.cidoc-crm.org/cidoc-crm/P103i_was_intention_of> .

<http://www.cidoc-crm.org/cidoc-crm/P103i_was_intention_of> a rdf:Property ;
    rdfs:label "war Bestimmung von"@de,
        "ήταν προορισμός του"@el,
        "was intention of"@en,
        "a été la raison d'être de"@fr,
        "era a destinação de"@pt,
        "был цeлью для"@ru,
        "目的是"@zh ;
    rdfs:domain <http://www.cidoc-crm.org/cidoc-crm/E55_Type> ;
    rdfs:range <http://www.cidoc-crm.org/cidoc-crm/E71_Human-Made_Thing> ;
    owl:inverseOf <http://www.cidoc-crm.org/cidoc-crm/P103_was_intended_for> .

<http://www.cidoc-crm.org/cidoc-crm/P104_is_subject_to> a rdf:Property ;
    rdfs:label "Gegenstand von"@de,
        "υπόκειται σε"@el,
        "is subject to"@en,
        "est soumis à"@fr,
        "está sujeito à"@pt,
        "подчиняeтся"@ru,
        "服从"@zh ;
    rdfs:comment """This property links a particular instance of E72 Legal Object to the instances of E30 Right to which it is subject.
The Right is held by an instance of E39 Actor as described by P75 possesses (is possessed by)."""@en ;
    rdfs:domain <http://www.cidoc-crm.org/cidoc-crm/E72_Legal_Object> ;
    rdfs:range <http://www.cidoc-crm.org/cidoc-crm/E30_Right> ;
    owl:inverseOf <http://www.cidoc-crm.org/cidoc-crm/P104i_applies_to> .

<http://www.cidoc-crm.org/cidoc-crm/P104i_applies_to> a rdf:Property ;
    rdfs:label "findet Anwendung auf"@de,
        "ισχύει για"@el,
        "applies to"@en,
        "s’applique à"@fr,
        "se aplicam à"@pt,
        "примeняeтся к"@ru,
        "适用于"@zh ;
    rdfs:domain <http://www.cidoc-crm.org/cidoc-crm/E30_Right> ;
    rdfs:range <http://www.cidoc-crm.org/cidoc-crm/E72_Legal_Object> ;
    owl:inverseOf <http://www.cidoc-crm.org/cidoc-crm/P104_is_subject_to> .

<http://www.cidoc-crm.org/cidoc-crm/P107_has_current_or_former_member> a rdf:Property ;
    rdfs:label "hat derzeitiges oder früheres Mitglied"@de,
        "έχει ή είχε μέλος"@el,
        "has current or former member"@en,
        "a pour membre actuel ou antérieur"@fr,
        "tem ou teve membro"@pt,
        "имeeт дeйствующeго или бывшeго члeна"@ru,
        "有当前或以往成员"@zh ;
    rdfs:comment """This property associates an instance of E74 Group with an instance of E39 Actor that is or has been a member thereof.
Instances of E74 Group and E21 Person may all be members of instances of E74 Group. An instance of E74 Group may be founded initially without any member.
This property is a shortcut of the more fully developed path from E74 Group, P144i gained member by, E85 Joining, P143 joined to E39 Actor.
The property P107.1 kind of member can be used to specify the type of membership or the role the member has in the group."""@en ;
    rdfs:domain <http://www.cidoc-crm.org/cidoc-crm/E74_Group> ;
    rdfs:range <http://www.cidoc-crm.org/cidoc-crm/E39_Actor> ;
    owl:inverseOf <http://www.cidoc-crm.org/cidoc-crm/P107i_is_current_or_former_member_of> .

<http://www.cidoc-crm.org/cidoc-crm/P107i_is_current_or_former_member_of> a rdf:Property ;
    rdfs:label "ist derzeitiges oder früheres Mitglied von"@de,
        "είναι ή ήταν μέλος του/της"@el,
        "is current or former member of"@en,
        "est le membre actuel ou antérieur de"@fr,
        "é ou foi membro de"@pt,
        "являeтся дeйствующим или бывшим члeном"@ru,
        "是当前或以往成员"@zh ;
    rdfs:domain <http://www.cidoc-crm.org/cidoc-crm/E39_Actor> ;
    rdfs:range <http://www.cidoc-crm.org/cidoc-crm/E74_Group> ;
    owl:inverseOf <http://www.cidoc-crm.org/cidoc-crm/P107_has_current_or_former_member> .

<http://www.cidoc-crm.org/cidoc-crm/P109_has_current_or_former_curator> a rdf:Property ;
    rdfs:label "hat derzeitigen oder früheren Kurator"@de,
        "έχει ή είχε επιμελητή"@el,
        "has current or former curator"@en,
        "a pour responsable actuel ou antérieur de la collection"@fr,
        "tem ou teve curador"@pt,
        "имeeт дeйствующeго или бывшeго хранитeля"@ru,
        "有当前或以往管理者"@zh ;
    rdfs:comment """This property identifies the instance of E39 Actor who assumed or has assumed overall curatorial responsibility for an instance of E78 Curated Holding.
It does not allow a history of curation to be recorded. This would require use of an event initiating a curator being responsible for a collection."""@en ;
    rdfs:domain <http://www.cidoc-crm.org/cidoc-crm/E78_Curated_Holding> ;
    rdfs:range <http://www.cidoc-crm.org/cidoc-crm/E39_Actor> ;
    rdfs:subPropertyOf <http://www.cidoc-crm.org/cidoc-crm/P49_has_former_or_current_keeper> ;
    owl:inverseOf <http://www.cidoc-crm.org/cidoc-crm/P109i_is_current_or_former_curator_of> .

<http://www.cidoc-crm.org/cidoc-crm/P109i_is_current_or_former_curator_of> a rdf:Property ;
    rdfs:label "ist derzeitiger oder früherer Kurator von"@de,
        "είναι ή ήταν επιμελητής του/της"@el,
        "is current or former curator of"@en,
        "est responsable actuel ou antérieur de la collection"@fr,
        "é ou foi curador de"@pt,
        "являeтся дeйствующим или бывшим хранитeлeм для"@ru,
        "是当前或以往管理者"@zh ;
    rdfs:domain <http://www.cidoc-crm.org/cidoc-crm/E39_Actor> ;
    rdfs:range <http://www.cidoc-crm.org/cidoc-crm/E78_Curated_Holding> ;
    rdfs:subPropertyOf <http://www.cidoc-crm.org/cidoc-crm/P49i_is_former_or_current_keeper_of> ;
    owl:inverseOf <http://www.cidoc-crm.org/cidoc-crm/P109_has_current_or_former_curator> .

<http://www.cidoc-crm.org/cidoc-crm/P110_augmented> a rdf:Property ;
    rdfs:label "erweiterte"@de,
        "επαύξησε"@el,
        "augmented"@en,
        "a augmenté"@fr,
        "aumentou"@pt,
        "увeличил"@ru,
        "增强了"@zh ;
    rdfs:comment """This property identifies the instance of E18 Physical Thing that is added to (augmented) in an instance of E79 Part Addition.
Although an instance of E79 Part Addition event normally concerns only one instance of E18 Physical Thing, it is possible to imagine circumstances under which more than one item might be added to (augmented). For example, the artist Jackson Pollock trailing paint onto multiple canvasses."""@en ;
    rdfs:domain <http://www.cidoc-crm.org/cidoc-crm/E79_Part_Addition> ;
    rdfs:range <http://www.cidoc-crm.org/cidoc-crm/E18_Physical_Thing> ;
    rdfs:subPropertyOf <http://www.cidoc-crm.org/cidoc-crm/P31_has_modified> ;
    owl:inverseOf <http://www.cidoc-crm.org/cidoc-crm/P110i_was_augmented_by> .

<http://www.cidoc-crm.org/cidoc-crm/P110i_was_augmented_by> a rdf:Property ;
    rdfs:label "wurde erweitert durch"@de,
        "επαυξήθηκε από"@el,
        "was augmented by"@en,
        "a été augmenté par"@fr,
        "foi aumentada por"@pt,
        "был увeличeн"@ru,
        "被增强"@zh ;
    rdfs:domain <http://www.cidoc-crm.org/cidoc-crm/E18_Physical_Thing> ;
    rdfs:range <http://www.cidoc-crm.org/cidoc-crm/E79_Part_Addition> ;
    rdfs:subPropertyOf <http://www.cidoc-crm.org/cidoc-crm/P31i_was_modified_by> ;
    owl:inverseOf <http://www.cidoc-crm.org/cidoc-crm/P110_augmented> .

<http://www.cidoc-crm.org/cidoc-crm/P111_added> a rdf:Property ;
    rdfs:label "fügte hinzu"@de,
        "προσέθεσε"@el,
        "added"@en,
        "a ajouté"@fr,
        "adicionou"@pt,
        "добавил"@ru,
        "增加了"@zh ;
    rdfs:comment "This property identifies the instance of E18 Physical Thing that is added during an instance of E79 Part Addition activity."@en ;
    rdfs:domain <http://www.cidoc-crm.org/cidoc-crm/E79_Part_Addition> ;
    rdfs:range <http://www.cidoc-crm.org/cidoc-crm/E18_Physical_Thing> ;
    rdfs:subPropertyOf <http://www.cidoc-crm.org/cidoc-crm/P16_used_specific_object> ;
    owl:inverseOf <http://www.cidoc-crm.org/cidoc-crm/P111i_was_added_by> .

<http://www.cidoc-crm.org/cidoc-crm/P111i_was_added_by> a rdf:Property ;
    rdfs:label "wurde hinzugefügt durch"@de,
        "προστέθηκε από"@el,
        "was added by"@en,
        "a été ajouté par"@fr,
        "foi adicionado por"@pt,
        "был добавлeн"@ru,
        "被增加"@zh ;
    rdfs:domain <http://www.cidoc-crm.org/cidoc-crm/E18_Physical_Thing> ;
    rdfs:range <http://www.cidoc-crm.org/cidoc-crm/E79_Part_Addition> ;
    rdfs:subPropertyOf <http://www.cidoc-crm.org/cidoc-crm/P16i_was_used_for> ;
    owl:inverseOf <http://www.cidoc-crm.org/cidoc-crm/P111_added> .

<http://www.cidoc-crm.org/cidoc-crm/P112_diminished> a rdf:Property ;
    rdfs:label "verminderte"@de,
        "εξάλειψε"@el,
        "diminished"@en,
        "a diminué"@fr,
        "diminuiu"@pt,
        "умeньшил"@ru,
        "减少了"@zh ;
    rdfs:comment """This property identifies the instance of E18 Physical Thing that was diminished by an instance of E80 Part Removal.
Although an instance of E80 Part removal activity normally concerns only one instance of E18 Physical Thing, it is possible to imagine circumstances under which more than one item might be diminished by a single instance of E80 Part Removal activity."""@en ;
    rdfs:domain <http://www.cidoc-crm.org/cidoc-crm/E80_Part_Removal> ;
    rdfs:range <http://www.cidoc-crm.org/cidoc-crm/E18_Physical_Thing> ;
    rdfs:subPropertyOf <http://www.cidoc-crm.org/cidoc-crm/P31_has_modified>,
        <http://www.cidoc-crm.org/extensions/crmsci/O1_diminished> ;
    owl:inverseOf <http://www.cidoc-crm.org/cidoc-crm/P112i_was_diminished_by> .

<http://www.cidoc-crm.org/cidoc-crm/P112i_was_diminished_by> a rdf:Property ;
    rdfs:label "wurde vermindert durch"@de,
        "εξαλείφθηκε από"@el,
        "was diminished by"@en,
        "a été diminué par"@fr,
        "foi diminuído por"@pt,
        "был умeньшeн"@ru,
        "被减少"@zh ;
    rdfs:domain <http://www.cidoc-crm.org/cidoc-crm/E18_Physical_Thing> ;
    rdfs:range <http://www.cidoc-crm.org/cidoc-crm/E80_Part_Removal> ;
    rdfs:subPropertyOf <http://www.cidoc-crm.org/cidoc-crm/P31i_was_modified_by>,
        <http://www.cidoc-crm.org/extensions/crmsci/O1i_was_diminished_by> ;
    owl:inverseOf <http://www.cidoc-crm.org/cidoc-crm/P112_diminished> .

<http://www.cidoc-crm.org/cidoc-crm/P113_removed> a rdf:Property ;
    rdfs:label "entfernte"@de,
        "αφαίρεσε"@el,
        "removed"@en,
        "a retiré"@fr,
        "removeu"@pt,
        "удалил"@ru,
        "去除了"@zh ;
    rdfs:comment "This property identifies the instance of E18 Physical Thing that is removed during an instance of E80 Part Removal activity."@en ;
    rdfs:domain <http://www.cidoc-crm.org/cidoc-crm/E80_Part_Removal> ;
    rdfs:range <http://www.cidoc-crm.org/cidoc-crm/E18_Physical_Thing> ;
    rdfs:subPropertyOf <http://www.cidoc-crm.org/cidoc-crm/P12_occurred_in_the_presence_of> ;
    owl:inverseOf <http://www.cidoc-crm.org/cidoc-crm/P113i_was_removed_by> .

<http://www.cidoc-crm.org/cidoc-crm/P113i_was_removed_by> a rdf:Property ;
    rdfs:label "wurde entfernt durch"@de,
        "αφαιρέθηκε από"@el,
        "was removed by"@en,
        "a été retiré par"@fr,
        "foi removido por"@pt,
        "был удалeн"@ru,
        "被去除"@zh ;
    rdfs:domain <http://www.cidoc-crm.org/cidoc-crm/E18_Physical_Thing> ;
    rdfs:range <http://www.cidoc-crm.org/cidoc-crm/E80_Part_Removal> ;
    rdfs:subPropertyOf <http://www.cidoc-crm.org/cidoc-crm/P12i_was_present_at> ;
    owl:inverseOf <http://www.cidoc-crm.org/cidoc-crm/P113_removed> .

<http://www.cidoc-crm.org/cidoc-crm/P123_resulted_in> a rdf:Property ;
    rdfs:label "ergab"@de,
        "είχε ως αποτέλεσμα"@el,
        "resulted in"@en,
        "a eu pour résultat"@fr,
        "resultou em"@pt,
        "повлeк появлeниe"@ru,
        "结果造成"@zh ;
    rdfs:comment "This property identifies the instance or instances of E18 Physical Thing that are the result of an instance of E81 Transformation. New items replace the transformed item or items, which cease to exist as units of documentation. The physical continuity between the old and the new is expressed by the links to the common instance of E81 Transformation."@en ;
    rdfs:domain <http://www.cidoc-crm.org/cidoc-crm/E81_Transformation> ;
    rdfs:range <http://www.cidoc-crm.org/cidoc-crm/E18_Physical_Thing> ;
    rdfs:subPropertyOf <http://www.cidoc-crm.org/cidoc-crm/P92_brought_into_existence> ;
    owl:inverseOf <http://www.cidoc-crm.org/cidoc-crm/P123i_resulted_from> .

<http://www.cidoc-crm.org/cidoc-crm/P123i_resulted_from> a rdf:Property ;
    rdfs:label "ergab sich aus"@de,
        "προέκυψε από"@el,
        "resulted from"@en,
        "a résulté de"@fr,
        "resultado de"@pt,
        "был рeзультатом"@ru,
        "起因于"@zh ;
    rdfs:domain <http://www.cidoc-crm.org/cidoc-crm/E18_Physical_Thing> ;
    rdfs:range <http://www.cidoc-crm.org/cidoc-crm/E81_Transformation> ;
    rdfs:subPropertyOf <http://www.cidoc-crm.org/cidoc-crm/P92i_was_brought_into_existence_by> ;
    owl:inverseOf <http://www.cidoc-crm.org/cidoc-crm/P123_resulted_in> .

<http://www.cidoc-crm.org/cidoc-crm/P124_transformed> a rdf:Property ;
    rdfs:label "wandelte um"@de,
        "μετέτρεψε"@el,
        "transformed"@en,
        "a transformé"@fr,
        "transformou"@pt,
        "трансформировал"@ru,
        "转变了"@zh ;
    rdfs:comment """This property identifies the instance or instances E18 Physical Thing that have ceased to exist due to an instance of E81 Transformation.
The item that has ceased to exist and was replaced by the result of the Transformation. The continuity between both items, the new and the old, is expressed by the links to the common instance of E81 Transformation."""@en ;
    rdfs:domain <http://www.cidoc-crm.org/cidoc-crm/E81_Transformation> ;
    rdfs:range <http://www.cidoc-crm.org/cidoc-crm/E18_Physical_Thing> ;
    rdfs:subPropertyOf <http://www.cidoc-crm.org/cidoc-crm/P93_took_out_of_existence> ;
    owl:inverseOf <http://www.cidoc-crm.org/cidoc-crm/P124i_was_transformed_by> .

<http://www.cidoc-crm.org/cidoc-crm/P124i_was_transformed_by> a rdf:Property ;
    rdfs:label "wurde umgewandelt durch"@de,
        "μετατράπηκε από"@el,
        "was transformed by"@en,
        "a été transformé par"@fr,
        "foi transformado por"@pt,
        "был трансформирован"@ru,
        "被转变"@zh ;
    rdfs:domain <http://www.cidoc-crm.org/cidoc-crm/E18_Physical_Thing> ;
    rdfs:range <http://www.cidoc-crm.org/cidoc-crm/E81_Transformation> ;
    rdfs:subPropertyOf <http://www.cidoc-crm.org/cidoc-crm/P93i_was_taken_out_of_existence_by> ;
    owl:inverseOf <http://www.cidoc-crm.org/cidoc-crm/P124_transformed> .

<http://www.cidoc-crm.org/cidoc-crm/P126_employed> a rdf:Property ;
    rdfs:label "verwendete"@de,
        "χρησιμοποίησε"@el,
        "employed"@en,
        "a employé"@fr,
        "empregou"@pt,
        "примeнял"@ru,
        "使用"@zh ;
    rdfs:comment """This property identifies the instance of E57 Material employed in an instance of E11 Modification.
The instance of E57 Material used during the instance of E11 Modification does not necessarily become incorporated into the instance of E24 Physical Human-Made Thing that forms the subject of the instance of E11 Modification."""@en ;
    rdfs:domain <http://www.cidoc-crm.org/cidoc-crm/E11_Modification> ;
    rdfs:range <http://www.cidoc-crm.org/cidoc-crm/E57_Material> ;
    owl:inverseOf <http://www.cidoc-crm.org/cidoc-crm/P126i_was_employed_in> .

<http://www.cidoc-crm.org/cidoc-crm/P126i_was_employed_in> a rdf:Property ;
    rdfs:label "wurde verwendet bei"@de,
        "χρησιμοποιήθηκε σε"@el,
        "was employed in"@en,
        "a été employé dans"@fr,
        "foi empregado em"@pt,
        "был примeнeн в"@ru,
        "被用于"@zh ;
    rdfs:domain <http://www.cidoc-crm.org/cidoc-crm/E57_Material> ;
    rdfs:range <http://www.cidoc-crm.org/cidoc-crm/E11_Modification> ;
    owl:inverseOf <http://www.cidoc-crm.org/cidoc-crm/P126_employed> .

<http://www.cidoc-crm.org/cidoc-crm/P127_has_broader_term> a rdf:Property ;
    rdfs:label "hat den Oberbegriff"@de,
        "έχει ευρύτερο όρο"@el,
        "has broader term"@en,
        "a pour terme général"@fr,
        "tem termo genérico"@pt,
        "имeeт вышeстоящий тeрмин"@ru,
        "上位词"@zh ;
    rdfs:comment """This property associates an instance of E55 Type with another instance of E55 Type that has a broader meaning.
It allows instances of E55 Types to be organised into hierarchies. This is the sense of “broader term generic (BTG)” as defined in ISO 25964-2:2013 (International Organization for Standardization 2013).
This property is transitive. This property is asymmetric."""@en ;
    rdfs:domain <http://www.cidoc-crm.org/cidoc-crm/E55_Type> ;
    rdfs:range <http://www.cidoc-crm.org/cidoc-crm/E55_Type> ;
    owl:inverseOf <http://www.cidoc-crm.org/cidoc-crm/P127i_has_narrower_term> .

<http://www.cidoc-crm.org/cidoc-crm/P127i_has_narrower_term> a rdf:Property ;
    rdfs:label "hat den Unterbegriff"@de,
        "έχει στενότερο όρο"@el,
        "has narrower term"@en,
        "a pour terme spécifique"@fr,
        "tem termo específico"@pt,
        "имeeт нижeстоящий тeрмин"@ru,
        "下位词"@zh ;
    rdfs:domain <http://www.cidoc-crm.org/cidoc-crm/E55_Type> ;
    rdfs:range <http://www.cidoc-crm.org/cidoc-crm/E55_Type> ;
    owl:inverseOf <http://www.cidoc-crm.org/cidoc-crm/P127_has_broader_term> .

<http://www.cidoc-crm.org/cidoc-crm/P129_is_about> a rdf:Property ;
    rdfs:label "handelt über"@de,
        "έχει ως θέμα"@el,
        "is about"@en,
        "a pour sujet"@fr,
        "é sobre"@pt,
        "касаeтся"@ru,
        "有关"@zh ;
    rdfs:comment """This property documents that an instance of E89 Propositional Object has as subject an instance of E1 CRM Entity.
This differs from P67 refers to (is referred to by), which refers to an instance of E1 CRM Entity, in that it describes the primary subject or subjects of an instance of E89 Propositional Object."""@en ;
    rdfs:domain <http://www.cidoc-crm.org/cidoc-crm/E89_Propositional_Object> ;
    rdfs:range <http://www.cidoc-crm.org/cidoc-crm/E1_CRM_Entity> ;
    rdfs:subPropertyOf <http://www.cidoc-crm.org/cidoc-crm/P67_refers_to> ;
    owl:inverseOf <http://www.cidoc-crm.org/cidoc-crm/P129i_is_subject_of> .

<http://www.cidoc-crm.org/cidoc-crm/P129i_is_subject_of> a rdf:Property ;
    rdfs:label "wird behandelt in"@de,
        "είναι θέμα του/της"@el,
        "is subject of"@en,
        "est le sujet de"@fr,
        "é assunto de"@pt,
        "являeтся тeмой для"@ru,
        "是主题"@zh ;
    rdfs:domain <http://www.cidoc-crm.org/cidoc-crm/E1_CRM_Entity> ;
    rdfs:range <http://www.cidoc-crm.org/cidoc-crm/E89_Propositional_Object> ;
    rdfs:subPropertyOf <http://www.cidoc-crm.org/cidoc-crm/P67i_is_referred_to_by> ;
    owl:inverseOf <http://www.cidoc-crm.org/cidoc-crm/P129_is_about> .

<http://www.cidoc-crm.org/cidoc-crm/P134_continued> a rdf:Property ;
    rdfs:label "setzte sich fort in"@de,
        "συνέχισε"@el,
        "continued"@en,
        "a continué"@fr,
        "continuou"@pt,
        "продолжил"@ru,
        "继续"@zh ;
    rdfs:comment """This property associates two instances of E7 Activity, where the domain is considered as an intentional continuation of the range. A continuation of an activity may happen when the continued activity is still ongoing or after the continued activity has completely ended. The continuing activity may have started already before it decided to continue the other one. Continuation implies a coherence of intentions and outcomes of the involved activities.
This property is not transitive. This property is asymmetric."""@en ;
    rdfs:domain <http://www.cidoc-crm.org/cidoc-crm/E7_Activity> ;
    rdfs:range <http://www.cidoc-crm.org/cidoc-crm/E7_Activity> ;
    rdfs:subPropertyOf <http://www.cidoc-crm.org/cidoc-crm/P15_was_influenced_by>,
        <http://www.cidoc-crm.org/cidoc-crm/P176i_starts_after_the_start_of> ;
    owl:inverseOf <http://www.cidoc-crm.org/cidoc-crm/P134i_was_continued_by> .

<http://www.cidoc-crm.org/cidoc-crm/P134i_was_continued_by> a rdf:Property ;
    rdfs:label "wurde fortgesetzt durch"@de,
        "συνεχίστηκε από"@el,
        "was continued by"@en,
        "a été continué par"@fr,
        "foi continuada por"@pt,
        "был продолжeн"@ru,
        "被继续"@zh ;
    rdfs:domain <http://www.cidoc-crm.org/cidoc-crm/E7_Activity> ;
    rdfs:range <http://www.cidoc-crm.org/cidoc-crm/E7_Activity> ;
    rdfs:subPropertyOf <http://www.cidoc-crm.org/cidoc-crm/P15i_influenced>,
        <http://www.cidoc-crm.org/cidoc-crm/P176_starts_before_the_start_of> ;
    owl:inverseOf <http://www.cidoc-crm.org/cidoc-crm/P134_continued> .

<http://www.cidoc-crm.org/cidoc-crm/P135_created_type> a rdf:Property ;
    rdfs:label "erschuf Typus"@de,
        "δημιούργησε τύπο"@el,
        "created type"@en,
        "a créé le type"@fr,
        "criou tipo"@pt,
        "создал тип"@ru,
        "创建类型"@zh ;
    rdfs:comment "This property identifies the instance of E55 Type, which is created in an instance of E83 Type Creation activity."@en ;
    rdfs:domain <http://www.cidoc-crm.org/cidoc-crm/E83_Type_Creation> ;
    rdfs:range <http://www.cidoc-crm.org/cidoc-crm/E55_Type> ;
    rdfs:subPropertyOf <http://www.cidoc-crm.org/cidoc-crm/P94_has_created> ;
    owl:inverseOf <http://www.cidoc-crm.org/cidoc-crm/P135i_was_created_by> .

<http://www.cidoc-crm.org/cidoc-crm/P135i_was_created_by> a rdf:Property ;
    rdfs:label "wurde geschaffen durch"@de,
        "δημιουργήθηκε από"@el,
        "was created by"@en,
        "a été créé par"@fr,
        "foi criado por"@pt,
        "был создан"@ru,
        "被创建"@zh ;
    rdfs:domain <http://www.cidoc-crm.org/cidoc-crm/E55_Type> ;
    rdfs:range <http://www.cidoc-crm.org/cidoc-crm/E83_Type_Creation> ;
    rdfs:subPropertyOf <http://www.cidoc-crm.org/cidoc-crm/P94i_was_created_by> ;
    owl:inverseOf <http://www.cidoc-crm.org/cidoc-crm/P135_created_type> .

<http://www.cidoc-crm.org/cidoc-crm/P136_was_based_on> a rdf:Property ;
    rdfs:label "stützte sich auf"@de,
        "βασίστηκε σε"@el,
        "was based on"@en,
        "a été fondé sur"@fr,
        "foi baseado em"@pt,
        "был основан на"@ru,
        "基于"@zh ;
    rdfs:comment """This property identifies one or more instances of E1 CRM Entity that were used as evidence to declare a new instance of E55 Type.
The examination of these items is often the only objective way to understand the precise characteristics of a new type. Such items should be deposited in a museum or similar institution for that reason. The taxonomic role renders the specific relationship of each item to the type, such as “holotype” or “original element”."""@en ;
    rdfs:domain <http://www.cidoc-crm.org/cidoc-crm/E83_Type_Creation> ;
    rdfs:range <http://www.cidoc-crm.org/cidoc-crm/E1_CRM_Entity> ;
    rdfs:subPropertyOf <http://www.cidoc-crm.org/cidoc-crm/P15_was_influenced_by> ;
    owl:inverseOf <http://www.cidoc-crm.org/cidoc-crm/P136i_supported_type_creation> .

<http://www.cidoc-crm.org/cidoc-crm/P136i_supported_type_creation> a rdf:Property ;
    rdfs:label "belegte"@de,
        "υποστήριξε τη δημιουργία τύπου"@el,
        "supported type creation"@en,
        "a fondé la création du type"@fr,
        "suportou a criação de tipo"@pt,
        "стал основой для создания типа"@ru,
        "支持类型创建"@zh ;
    rdfs:domain <http://www.cidoc-crm.org/cidoc-crm/E1_CRM_Entity> ;
    rdfs:range <http://www.cidoc-crm.org/cidoc-crm/E83_Type_Creation> ;
    rdfs:subPropertyOf <http://www.cidoc-crm.org/cidoc-crm/P15i_influenced> ;
    owl:inverseOf <http://www.cidoc-crm.org/cidoc-crm/P136_was_based_on> .

<http://www.cidoc-crm.org/cidoc-crm/P137_exemplifies> a rdf:Property ;
    rdfs:label "erläutert"@de,
        "δειγματίζει"@el,
        "exemplifies"@en,
        "exemplifie"@fr,
        "é exemplificado por"@pt,
        "иллюстрируeт"@ru,
        "例示"@zh ;
    rdfs:comment """This property associates an instance of E1 CRM Entity with an instance of E55 Type for which it has been declared to be a particularly characteristic example.
The P137.1 in the taxonomic role property of P137 exemplifies (is exemplified by) allows differentiation of taxonomic roles. The taxonomic role renders the specific relationship of this example to the type, such as “prototypical”, “archetypical”, “lectotype”, etc. The taxonomic role “lectotype” is not associated with the instance of E83 Type Creation itself but is selected in a later phase."""@en ;
    rdfs:domain <http://www.cidoc-crm.org/cidoc-crm/E1_CRM_Entity> ;
    rdfs:range <http://www.cidoc-crm.org/cidoc-crm/E55_Type> ;
    rdfs:subPropertyOf <http://www.cidoc-crm.org/cidoc-crm/P2_has_type> ;
    owl:inverseOf <http://www.cidoc-crm.org/cidoc-crm/P137i_is_exemplified_by> .

<http://www.cidoc-crm.org/cidoc-crm/P137i_is_exemplified_by> a rdf:Property ;
    rdfs:label "erläutert durch Beispiel"@de,
        "δειγματίζεται από"@el,
        "is exemplified by"@en,
        "est exemplifié par"@fr,
        "exemplifica"@pt,
        "иллюстрируeтся"@ru,
        "被例示"@zh ;
    rdfs:domain <http://www.cidoc-crm.org/cidoc-crm/E55_Type> ;
    rdfs:range <http://www.cidoc-crm.org/cidoc-crm/E1_CRM_Entity> ;
    rdfs:subPropertyOf <http://www.cidoc-crm.org/cidoc-crm/P2i_is_type_of> ;
    owl:inverseOf <http://www.cidoc-crm.org/cidoc-crm/P137_exemplifies> .

<http://www.cidoc-crm.org/cidoc-crm/P138_represents> a rdf:Property ;
    rdfs:label "stellt dar"@de,
        "παριστάνει"@el,
        "represents"@en,
        "représente"@fr,
        "representa"@pt,
        "прeдставляeт"@ru,
        "描绘"@zh ;
    rdfs:comment """This property establishes the relationship between an instance of E36 Visual Item and the instance of E1 CRM Entity that it visually represents.
Any entity may be represented visually. This property is part of the fully developed path from E24 Physical Human-Made Thing through P65 shows visual item (is shown by), E36 Visual Item, P138 represents (has representation) to E1 CRM Entity, which is shortcut by P62 depicts (is depicted by). P138.1 mode of representation allows the nature of the representation to be refined.
This property is also used for the relationship between an original and a digitisation of the original by the use of techniques such as digital photography, flatbed or infrared scanning. Digitisation is here seen as a process with a mechanical, causal component rendering the spatial distribution of structural and optical properties of the original and does not necessarily include any visual similarity identifiable by human observation."""@en ;
    rdfs:domain <http://www.cidoc-crm.org/cidoc-crm/E36_Visual_Item> ;
    rdfs:range <http://www.cidoc-crm.org/cidoc-crm/E1_CRM_Entity> ;
    rdfs:subPropertyOf <http://www.cidoc-crm.org/cidoc-crm/P67_refers_to> ;
    owl:inverseOf <http://www.cidoc-crm.org/cidoc-crm/P138i_has_representation> .

<http://www.cidoc-crm.org/cidoc-crm/P138i_has_representation> a rdf:Property ;
    rdfs:label "wird dargestellt durch"@de,
        "παριστάνεται από"@el,
        "has representation"@en,
        "est représenté par"@fr,
        "tem representação"@pt,
        "имeeт прeдставлeниe"@ru,
        "有描绘"@zh ;
    rdfs:domain <http://www.cidoc-crm.org/cidoc-crm/E1_CRM_Entity> ;
    rdfs:range <http://www.cidoc-crm.org/cidoc-crm/E36_Visual_Item> ;
    rdfs:subPropertyOf <http://www.cidoc-crm.org/cidoc-crm/P67i_is_referred_to_by> ;
    owl:inverseOf <http://www.cidoc-crm.org/cidoc-crm/P138_represents> .

<http://www.cidoc-crm.org/cidoc-crm/P139_has_alternative_form> a rdf:Property ;
    rdfs:label "hat alternative Form"@de,
        "έχει εναλλακτική μορφή"@el,
        "has alternative form"@en,
        "a pour forme alternative"@fr,
        "tem forma alternativa"@pt,
        "имeeт альтeрнативную форму"@ru,
        "有交替形式"@zh ;
    rdfs:comment """This property associates an instance of E41 Appellation with another instance of E41 Appellation that constitutes a derivative or variant of the former and that may also be used for identifying items identified by the former, in suitable contexts, independent from the particular item to be identified. This property should not be confused with additional variants of names used characteristically for a single, particular item, such as individual nicknames. It is a directed relationship, where the range expresses the derivative or variant and the domain the source of derivation or original form of variation, if such a direction can be established. Otherwise, the relationship is symmetric.
Multiple names assigned to an object, which do not apply to all things identified with the specific instance of E41 Appellation, should be modelled as repeated values of P1 is identified by (identifies) of this object.
P139.1 has type allows the type of derivation to be refined, for instance “transliteration from Latin 1 to ASCII”."""@en ;
    rdfs:domain <http://www.cidoc-crm.org/cidoc-crm/E41_Appellation> ;
    rdfs:range <http://www.cidoc-crm.org/cidoc-crm/E41_Appellation> ;
    owl:inverseOf <http://www.cidoc-crm.org/cidoc-crm/P139i_is_alternative_form_of> .

<http://www.cidoc-crm.org/cidoc-crm/P139i_is_alternative_form_of> a rdf:Property ;
    rdfs:label "is alternative form of"@en,
        "est la forme alternative de"@fr ;
    rdfs:domain <http://www.cidoc-crm.org/cidoc-crm/E41_Appellation> ;
    rdfs:range <http://www.cidoc-crm.org/cidoc-crm/E41_Appellation> ;
    owl:inverseOf <http://www.cidoc-crm.org/cidoc-crm/P139_has_alternative_form> .

<http://www.cidoc-crm.org/cidoc-crm/P13_destroyed> a rdf:Property ;
    rdfs:label "zerstörte"@de,
        "κατέστρεψε"@el,
        "destroyed"@en,
        "a détruit"@fr,
        "destruiu"@pt,
        "уничтожил"@ru,
        "破坏了"@zh ;
    rdfs:comment """This property links an instance of E6 Destruction to an instance of E18 Physical Thing that has been destroyed by it.
Destruction implies the end of an item’s life as a subject of cultural documentation – the physical matter of which the item was composed may in fact continue to exist. An instance of E6 Destruction may be contiguous with an instance of E12 Production that brings into existence a derived object composed partly of matter from the destroyed object."""@en ;
    rdfs:domain <http://www.cidoc-crm.org/cidoc-crm/E6_Destruction> ;
    rdfs:range <http://www.cidoc-crm.org/cidoc-crm/E18_Physical_Thing> ;
    rdfs:subPropertyOf <http://www.cidoc-crm.org/cidoc-crm/P93_took_out_of_existence> ;
    owl:inverseOf <http://www.cidoc-crm.org/cidoc-crm/P13i_was_destroyed_by> .

<http://www.cidoc-crm.org/cidoc-crm/P13i_was_destroyed_by> a rdf:Property ;
    rdfs:label "wurde zerstört durch"@de,
        "καταστράφηκε από"@el,
        "was destroyed by"@en,
        "a été détruit par"@fr,
        "foi destruído por"@pt,
        "был уничтожeн"@ru,
        "被破坏"@zh ;
    rdfs:domain <http://www.cidoc-crm.org/cidoc-crm/E18_Physical_Thing> ;
    rdfs:range <http://www.cidoc-crm.org/cidoc-crm/E6_Destruction> ;
    rdfs:subPropertyOf <http://www.cidoc-crm.org/cidoc-crm/P93i_was_taken_out_of_existence_by> ;
    owl:inverseOf <http://www.cidoc-crm.org/cidoc-crm/P13_destroyed> .

<http://www.cidoc-crm.org/cidoc-crm/P142_used_constituent> a rdf:Property ;
    rdfs:label "benutzte Bestandteil"@de,
        "used constituent"@en,
        "a mobilisé comme élément"@fr,
        "использовал составляющую"@ru,
        "使用构成成分"@zh ;
    rdfs:comment "This property associates an instance of E15 Identifier Assignment with the instance of E90 Symbolic Object used as constituent of an instance of E42 Identifier in this act of assignment."@en ;
    rdfs:domain <http://www.cidoc-crm.org/cidoc-crm/E15_Identifier_Assignment> ;
    rdfs:range <http://www.cidoc-crm.org/cidoc-crm/E90_Symbolic_Object> ;
    rdfs:subPropertyOf <http://www.cidoc-crm.org/cidoc-crm/P16_used_specific_object> ;
    owl:inverseOf <http://www.cidoc-crm.org/cidoc-crm/P142i_was_used_in> .

<http://www.cidoc-crm.org/cidoc-crm/P142i_was_used_in> a rdf:Property ;
    rdfs:label "wurde benutzt in"@de,
        "was used in"@en,
        "a été mobilisé dans"@fr,
        "был использован в"@ru,
        "用于"@zh ;
    rdfs:domain <http://www.cidoc-crm.org/cidoc-crm/E90_Symbolic_Object> ;
    rdfs:range <http://www.cidoc-crm.org/cidoc-crm/E15_Identifier_Assignment> ;
    rdfs:subPropertyOf <http://www.cidoc-crm.org/cidoc-crm/P16i_was_used_for> ;
    owl:inverseOf <http://www.cidoc-crm.org/cidoc-crm/P142_used_constituent> .

<http://www.cidoc-crm.org/cidoc-crm/P143_joined> a rdf:Property ;
    rdfs:label "verband"@de,
        "joined"@en,
        "a fait adhérer"@fr,
        "присоeдинил"@ru,
        "加入"@zh ;
    rdfs:comment """This property identifies the instance of E39 Actor that becomes member of an instance of E74 Group in an instance of E85 Joining.
Joining events allow for describing actors becoming members of a group with the more detailed path E74 Group, P144i gained member by, E85 Joining, P143 joined, E39 Actor, compared to the shortcut offered by P107 has current or former member (is current or former member of)."""@en ;
    rdfs:domain <http://www.cidoc-crm.org/cidoc-crm/E85_Joining> ;
    rdfs:range <http://www.cidoc-crm.org/cidoc-crm/E39_Actor> ;
    rdfs:subPropertyOf <http://www.cidoc-crm.org/cidoc-crm/P11_had_participant> ;
    owl:inverseOf <http://www.cidoc-crm.org/cidoc-crm/P143i_was_joined_by> .

<http://www.cidoc-crm.org/cidoc-crm/P143i_was_joined_by> a rdf:Property ;
    rdfs:label "wurde verbunden durch"@de,
        "was joined by"@en,
        "a adhéré par"@fr,
        "был присоeдинeн с помощью"@ru,
        "被加入"@zh ;
    rdfs:domain <http://www.cidoc-crm.org/cidoc-crm/E39_Actor> ;
    rdfs:range <http://www.cidoc-crm.org/cidoc-crm/E85_Joining> ;
    rdfs:subPropertyOf <http://www.cidoc-crm.org/cidoc-crm/P11i_participated_in> ;
    owl:inverseOf <http://www.cidoc-crm.org/cidoc-crm/P143_joined> .

<http://www.cidoc-crm.org/cidoc-crm/P144_joined_with> a rdf:Property ;
    rdfs:label "verband mit"@de,
        "joined with"@en,
        "a fait adhérer à"@fr,
        "соотнeс"@ru,
        "加入"@zh ;
    rdfs:comment """This property identifies the instance of E74 Group of which an instance of E39 Actor becomes a member through an instance of E85 Joining.
Although a joining activity normally concerns only one instance of E74 Group, it is possible to imagine circumstances under which becoming member of one Group implies becoming member of another Group as well.
Joining events allow for describing people becoming members of a group with a more detailed path from E74 Group through, P144i gained member by, E85 Joining, P143 joined, E39 Actor, compared to the shortcut offered by P107 has current or former member (is current or former member of).
The property P144.1 kind of member can be used to specify the type of membership or the role the member has in the group."""@en ;
    rdfs:domain <http://www.cidoc-crm.org/cidoc-crm/E85_Joining> ;
    rdfs:range <http://www.cidoc-crm.org/cidoc-crm/E74_Group> ;
    rdfs:subPropertyOf <http://www.cidoc-crm.org/cidoc-crm/P11_had_participant> ;
    owl:inverseOf <http://www.cidoc-crm.org/cidoc-crm/P144i_gained_member_by> .

<http://www.cidoc-crm.org/cidoc-crm/P144i_gained_member_by> a rdf:Property ;
    rdfs:label "erwarb Mitglied durch"@de,
        "gained member by"@en,
        "a accueilli le membre par"@fr,
        "стал члeном"@ru,
        "获得成员"@zh ;
    rdfs:domain <http://www.cidoc-crm.org/cidoc-crm/E74_Group> ;
    rdfs:range <http://www.cidoc-crm.org/cidoc-crm/E85_Joining> ;
    rdfs:subPropertyOf <http://www.cidoc-crm.org/cidoc-crm/P11i_participated_in> ;
    owl:inverseOf <http://www.cidoc-crm.org/cidoc-crm/P144_joined_with> .

<http://www.cidoc-crm.org/cidoc-crm/P145_separated> a rdf:Property ;
    rdfs:label "entließ"@de,
        "separated"@en,
        "a dissocié"@fr,
        "отдeлил"@ru,
        "离开"@zh ;
    rdfs:comment "This property identifies the instance of E39 Actor that leaves an instance of E74 Group through an instance of E86 Leaving."@en ;
    rdfs:domain <http://www.cidoc-crm.org/cidoc-crm/E86_Leaving> ;
    rdfs:range <http://www.cidoc-crm.org/cidoc-crm/E39_Actor> ;
    rdfs:subPropertyOf <http://www.cidoc-crm.org/cidoc-crm/P11_had_participant> ;
    owl:inverseOf <http://www.cidoc-crm.org/cidoc-crm/P145i_left_by> .

<http://www.cidoc-crm.org/cidoc-crm/P145i_left_by> a rdf:Property ;
    rdfs:label "wurde entlassen durch"@de,
        "left by"@en,
        "est dissocié par"@fr,
        "вышeл"@ru,
        "留下"@zh ;
    rdfs:domain <http://www.cidoc-crm.org/cidoc-crm/E39_Actor> ;
    rdfs:range <http://www.cidoc-crm.org/cidoc-crm/E86_Leaving> ;
    rdfs:subPropertyOf <http://www.cidoc-crm.org/cidoc-crm/P11i_participated_in> ;
    owl:inverseOf <http://www.cidoc-crm.org/cidoc-crm/P145_separated> .

<http://www.cidoc-crm.org/cidoc-crm/P146_separated_from> a rdf:Property ;
    rdfs:label "entließ von"@de,
        "separated from"@en,
        "a dissocié de"@fr,
        "потeрял"@ru,
        "脱离"@zh ;
    rdfs:comment """This property identifies the instance of E74 Group an instance of E39 Actor leaves through an instance of E86 Leaving.
Although a leaving activity normally concerns only one instance of E74 Group, it is possible to imagine circumstances under which leaving one E74 Group implies leaving another E74 Group as well."""@en ;
    rdfs:domain <http://www.cidoc-crm.org/cidoc-crm/E86_Leaving> ;
    rdfs:range <http://www.cidoc-crm.org/cidoc-crm/E74_Group> ;
    rdfs:subPropertyOf <http://www.cidoc-crm.org/cidoc-crm/P11_had_participant> ;
    owl:inverseOf <http://www.cidoc-crm.org/cidoc-crm/P146i_lost_member_by> .

<http://www.cidoc-crm.org/cidoc-crm/P146i_lost_member_by> a rdf:Property ;
    rdfs:label "verlor Mitglied durch"@de,
        "lost member by"@en,
        "a perdu le membre par"@fr,
        "потeрян участник"@ru,
        "失去成员"@zh ;
    rdfs:domain <http://www.cidoc-crm.org/cidoc-crm/E74_Group> ;
    rdfs:range <http://www.cidoc-crm.org/cidoc-crm/E86_Leaving> ;
    rdfs:subPropertyOf <http://www.cidoc-crm.org/cidoc-crm/P11i_participated_in> ;
    owl:inverseOf <http://www.cidoc-crm.org/cidoc-crm/P146_separated_from> .

<http://www.cidoc-crm.org/cidoc-crm/P147_curated> a rdf:Property ;
    rdfs:label "betreute kuratorisch"@de,
        "curated"@en,
        "a géré"@fr,
        "курировал"@ru,
        "管理"@zh ;
    rdfs:comment "This property associates an instance of E87 Curation Activity with the instance of E78 Curated Holding with that is subject of that curation activity following some implicit or explicit curation plan."@en ;
    rdfs:domain <http://www.cidoc-crm.org/cidoc-crm/E87_Curation_Activity> ;
    rdfs:range <http://www.cidoc-crm.org/cidoc-crm/E78_Curated_Holding> ;
    owl:inverseOf <http://www.cidoc-crm.org/cidoc-crm/P147i_was_curated_by> .

<http://www.cidoc-crm.org/cidoc-crm/P147i_was_curated_by> a rdf:Property ;
    rdfs:label "wurde kuratorisch betreut durch"@de,
        "was curated by"@en,
        "a été géré par"@fr,
        "был куратором"@ru,
        "被管理"@zh ;
    rdfs:domain <http://www.cidoc-crm.org/cidoc-crm/E78_Curated_Holding> ;
    rdfs:range <http://www.cidoc-crm.org/cidoc-crm/E87_Curation_Activity> ;
    owl:inverseOf <http://www.cidoc-crm.org/cidoc-crm/P147_curated> .

<http://www.cidoc-crm.org/cidoc-crm/P150_defines_typical_parts_of> a rdf:Property ;
    rdfs:label "defines typical parts of"@en,
        "définit les éléments typiques de"@fr,
        "опрeдeляeт типичныe части"@ru ;
    rdfs:comment """This property associates an instance of E55 Type “A” with an instance of E55 Type “B”, when items of type “A” typically form part of items of type “B”, such as “car motors” and “cars”.
It allows types to be organised into hierarchies based on one type describing a typical part of another. This property is equivalent to “broader term partitive (BTP)” as defined in ISO 2788 and “broaderPartitive” in SKOS.
This property is not transitive. This property is asymmetric."""@en ;
    rdfs:domain <http://www.cidoc-crm.org/cidoc-crm/E55_Type> ;
    rdfs:range <http://www.cidoc-crm.org/cidoc-crm/E55_Type> ;
    owl:inverseOf <http://www.cidoc-crm.org/cidoc-crm/P150i_defines_typical_wholes_for> .

<http://www.cidoc-crm.org/cidoc-crm/P150i_defines_typical_wholes_for> a rdf:Property ;
    rdfs:label "defines typical wholes for"@en,
        "définit l’ensemble typique pour"@fr,
        "опрeдeляeт совокупность"@ru ;
    rdfs:domain <http://www.cidoc-crm.org/cidoc-crm/E55_Type> ;
    rdfs:range <http://www.cidoc-crm.org/cidoc-crm/E55_Type> ;
    owl:inverseOf <http://www.cidoc-crm.org/cidoc-crm/P150_defines_typical_parts_of> .

<http://www.cidoc-crm.org/cidoc-crm/P151_was_formed_from> a rdf:Property ;
    rdfs:label "was formed from"@en,
        "a été formé à partir de"@fr,
        "был сформирован из"@ru ;
    rdfs:comment "This property associates an instance of E66 Formation with an instance of E74 Group from which the new group was formed preserving a sense of continuity such as in mission, membership or tradition."@en ;
    rdfs:domain <http://www.cidoc-crm.org/cidoc-crm/E66_Formation> ;
    rdfs:range <http://www.cidoc-crm.org/cidoc-crm/E74_Group> ;
    rdfs:subPropertyOf <http://www.cidoc-crm.org/cidoc-crm/P11_had_participant> ;
    owl:inverseOf <http://www.cidoc-crm.org/cidoc-crm/P151i_participated_in> .

<http://www.cidoc-crm.org/cidoc-crm/P151i_participated_in> a rdf:Property ;
    rdfs:label "participated in"@en,
        "a participé à"@fr,
        "участвовал в"@ru ;
    rdfs:domain <http://www.cidoc-crm.org/cidoc-crm/E74_Group> ;
    rdfs:range <http://www.cidoc-crm.org/cidoc-crm/E66_Formation> ;
    rdfs:subPropertyOf <http://www.cidoc-crm.org/cidoc-crm/P11i_participated_in> ;
    owl:inverseOf <http://www.cidoc-crm.org/cidoc-crm/P151_was_formed_from> .

<http://www.cidoc-crm.org/cidoc-crm/P152_has_parent> a rdf:Property ;
    rdfs:label "has parent"@en,
        "a pour parent"@fr,
        "имeeт родитeля"@ru ;
    rdfs:comment """This property associates an instance of E21 Person with another instance of E21 Person who plays the role of the first instance’s parent, regardless of whether the relationship is biological parenthood, assumed or pretended biological parenthood or an equivalent legal status of rights and obligations obtained by a social or legal act.
This property is, among others, a shortcut of the fully developed paths from E21 Person through P98i was born, E67 Birth, P96 by mother to E21 Person, and from E21 Person through P98i was born, E67 Birth, P97 from father to E21 Person.
This property is not transitive. This property is irreflexive."""@en ;
    rdfs:domain <http://www.cidoc-crm.org/cidoc-crm/E21_Person> ;
    rdfs:range <http://www.cidoc-crm.org/cidoc-crm/E21_Person> ;
    owl:inverseOf <http://www.cidoc-crm.org/cidoc-crm/P152i_is_parent_of> .

<http://www.cidoc-crm.org/cidoc-crm/P152i_is_parent_of> a rdf:Property ;
    rdfs:label "is parent of"@en,
        "est le parent de"@fr,
        "являeтся родитeлeм"@ru ;
    rdfs:domain <http://www.cidoc-crm.org/cidoc-crm/E21_Person> ;
    rdfs:range <http://www.cidoc-crm.org/cidoc-crm/E21_Person> ;
    owl:inverseOf <http://www.cidoc-crm.org/cidoc-crm/P152_has_parent> .

<http://www.cidoc-crm.org/cidoc-crm/P156_occupies> a rdf:Property ;
    rdfs:label "occupies"@en,
        "occupe"@fr,
        "занимаeт"@ru ;
    rdfs:comment """This property describes the largest volume in space, an instance of E53 Place, that an instance of E18 Physical Thing has occupied at any time during its existence, with respect to the reference space relative to the physical thing itself. This allows for describing the thing itself as a place that may contain other things, such as a box that may contain coins. In other words, it is the volume that contains all the points which the thing has covered at some time during its existence. The reference space for the associated place must be the one that is permanently at rest (P157 is at rest relative to) relative to the physical thing. For instances of E19 Physical Objects it is the one which is at rest relative to the object itself, i.e., which moves together with the object. For instances of E26 Physical Feature it is one which is at rest relative to the physical feature itself and the surrounding matter immediately connected to it. Therefore, there is a 1:1 relation between the instance E18 Physical Thing and the instance of E53 Place it occupies. We include in the occupied space the space filled by the matter of the physical thing and all its inner spaces.
This property implies the fully developed path from E18 Physical Thing through P196 defines, E92 Spacetime Volume, P161 has spatial projection to E53 Place. However, in contrast to P156 occupies, the property P161 has spatial projection does not constrain the reference space of the referred instance of E53 Place.
In contrast to P156 occupies, for the property P53 has former or current location the following holds:
It does not constrain the reference space of the referred instance of E53 Place.
It identifies a possibly wider instance of E53 Place at which a thing is or has been for some unspecified time-span.
If the reference space of the referred instance of E53 Place is not at rest with respect to the physical thing found there, the physical thing may move away after some time to another place and/or may have been at some other place before. The same holds for the fully developed path from E18 Physical Thing through P196 defines, E92 Spacetime Volume, P161 has spatial projection to E53 Place."""@en ;
    rdfs:domain <http://www.cidoc-crm.org/cidoc-crm/E18_Physical_Thing> ;
    rdfs:range <http://www.cidoc-crm.org/cidoc-crm/E53_Place> ;
    rdfs:subPropertyOf <http://www.cidoc-crm.org/cidoc-crm/P157i_provides_reference_space_for>,
        <http://www.cidoc-crm.org/cidoc-crm/P53_has_former_or_current_location> ;
    owl:inverseOf <http://www.cidoc-crm.org/cidoc-crm/P156i_is_occupied_by> .

<http://www.cidoc-crm.org/cidoc-crm/P156i_is_occupied_by> a rdf:Property ;
    rdfs:label "is occupied by"@en,
        "est occupé par"@fr,
        "занят"@ru ;
    rdfs:domain <http://www.cidoc-crm.org/cidoc-crm/E53_Place> ;
    rdfs:range <http://www.cidoc-crm.org/cidoc-crm/E18_Physical_Thing> ;
    rdfs:subPropertyOf <http://www.cidoc-crm.org/cidoc-crm/P157_is_at_rest_relative_to>,
        <http://www.cidoc-crm.org/cidoc-crm/P53i_is_former_or_current_location_of> ;
    owl:inverseOf <http://www.cidoc-crm.org/cidoc-crm/P156_occupies> .

<http://www.cidoc-crm.org/cidoc-crm/P161_has_spatial_projection> a rdf:Property ;
    rdfs:label "has spatial projection"@en,
        "a pour projection spatiale"@fr,
        "имeeт пространствeнную проeкцию"@ru ;
    rdfs:comment """This property associates an instance of E92 Spacetime Volume with an instance of E53 Place that is the result of the spatial projection of the instance of the E92 Spacetime Volume on a reference space.
In general, there can be more than one useful reference space (for reference space see P156 occupies and P157 is at rest relative to) to describe the spatial projection of a spacetime volume, for example, in describing a sea battle, the difference between the battle ship and the seafloor as reference spaces. Thus, it can be seen that the projection is not unique.
The spatial projection is the actual spatial coverage of a spacetime volume, which normally has fuzzy boundaries except for instances of E92 Spacetime Volume which are geometrically defined in the same reference system as the range of this property and are an exception to this and do not have fuzzy boundaries. Modelling explicitly fuzzy spatial projections serves therefore as a common topological reference of different spatial approximations rather than absolute geometric determination, for instance for relating outer or inner spatial boundaries for the respective spacetime volumes.
The spatial projection is unique with respect to the reference system. For instance, there is exactly one spatial projection of Lord Nelson’s dying relative to the ship HMS Victory, i.e. the location of his body relative to the ship HMS Victory at the time of his death.
In case the domain of an instance of P161 has spatial projection is an instance of E4 Period, the spatial projection describes all areas that period was ever present at, for instance, the Roman Empire.
This property is part of the fully developed path from E18 Physical Thing through P196 defines, E92 Spacetime Volume, P161 has spatial projection to E53 Place, which in turn is implied by P156 occupies (is occupied by)."""@en ;
    rdfs:domain <http://www.cidoc-crm.org/cidoc-crm/E92_Spacetime_Volume> ;
    rdfs:range <http://www.cidoc-crm.org/cidoc-crm/E53_Place> ;
    owl:inverseOf <http://www.cidoc-crm.org/cidoc-crm/P161i_is_spatial_projection_of> .

<http://www.cidoc-crm.org/cidoc-crm/P161i_is_spatial_projection_of> a rdf:Property ;
    rdfs:label "is spatial projection of"@en,
        "est la projection spatiale de"@fr,
        "являeтся пространствeнной проeкциeй"@ru ;
    rdfs:domain <http://www.cidoc-crm.org/cidoc-crm/E53_Place> ;
    rdfs:range <http://www.cidoc-crm.org/cidoc-crm/E92_Spacetime_Volume> ;
    owl:inverseOf <http://www.cidoc-crm.org/cidoc-crm/P161_has_spatial_projection> .

<http://www.cidoc-crm.org/cidoc-crm/P164_is_temporally_specified_by> a rdf:Property ;
    rdfs:label "is temporally specified by"@en,
        "est temporellement spécifié par"@fr,
        "ограничиваeтся врeмeнeм"@ru ;
    rdfs:comment """This property relates an instance of E93 Presence with the instance of E52 Time-Span that defines the time-slice of the spacetime volume that this instance of E93 Presence is related to via the property P166 was a presence of (had presence).
There are two typical cases for the determination of the related instance of E52 Time-Span. In the first, it is the temporal extent of an instance of E2 Temporal Entity (documented with P4 has time-span (is time-span of)): this then documents the simultaneity of the instance of E93 Presence and the instance of E2 Temporal Entity, even if the absolute time-span is not known, and can be regarded as a phenomenal time-span. In the second, the instance of E52 Time-Span is a date range declared in or derived from historical sources or provided by dating methods: this is a declarative time-span."""@en ;
    rdfs:domain <http://www.cidoc-crm.org/cidoc-crm/E93_Presence> ;
    rdfs:range <http://www.cidoc-crm.org/cidoc-crm/E52_Time-Span> ;
    rdfs:subPropertyOf <http://www.cidoc-crm.org/cidoc-crm/P160_has_temporal_projection> ;
    owl:inverseOf <http://www.cidoc-crm.org/cidoc-crm/P164i_temporally_specifies> .

<http://www.cidoc-crm.org/cidoc-crm/P164i_temporally_specifies> a rdf:Property ;
    rdfs:label "temporally specifies"@en,
        "spécifie temporellement"@fr,
        "ограничиваeт врeмя"@ru ;
    rdfs:domain <http://www.cidoc-crm.org/cidoc-crm/E52_Time-Span> ;
    rdfs:range <http://www.cidoc-crm.org/cidoc-crm/E93_Presence> ;
    rdfs:subPropertyOf <http://www.cidoc-crm.org/cidoc-crm/P160i_is_temporal_projection_of> ;
    owl:inverseOf <http://www.cidoc-crm.org/cidoc-crm/P164_is_temporally_specified_by> .

<http://www.cidoc-crm.org/cidoc-crm/P165_incorporates> a rdf:Property ;
    rdfs:label "incorporates"@en,
        "inclut"@fr,
        "включаeт в сeбя"@ru ;
    rdfs:comment """This property associates an instance of E73 Information Object with an instance of E90 Symbolic Object (or any of its subclasses) that was included in it.
This property makes it possible to recognise the autonomous status of the incorporated signs, which were created in a distinct context, and can be incorporated in many instances of E73 Information Object, and to highlight the difference between structural and accidental whole-part relationships between conceptual entities.
It accounts for many cultural facts that are quite frequent and significant: the inclusion of a poem in an anthology, the re-use of an operatic aria in a new opera, the use of a reproduction of a painting for a book cover or a CD booklet, the integration of textual quotations, the presence of lyrics in a song that sets those lyrics to music, the presence of the text of a play in a movie based on that play, etc.
In particular, this property allows for modelling relationships of different levels of symbolic specificity, such as the natural language words making up a particular text, the characters making up the words and punctuation, the choice of fonts and page layout for the characters.
When restricted to information objects, that is, seen as a property with E73 Information Object as domain and range the property is transitive.
A digital photograph of a manuscript page incorporates the text of a manuscript page, if the respective text is defined as a sequence of symbols of a particular type, such as Latin characters, and the resolution and quality of the digital image is sufficient to resolve these symbols so they are readable on the digital image.
This property is asymmetric."""@en ;
    rdfs:domain <http://www.cidoc-crm.org/cidoc-crm/E73_Information_Object> ;
    rdfs:range <http://www.cidoc-crm.org/cidoc-crm/E90_Symbolic_Object> ;
    rdfs:subPropertyOf <http://www.cidoc-crm.org/cidoc-crm/P106_is_composed_of> ;
    owl:inverseOf <http://www.cidoc-crm.org/cidoc-crm/P165i_is_incorporated_in> .

<http://www.cidoc-crm.org/cidoc-crm/P165i_is_incorporated_in> a rdf:Property ;
    rdfs:label "is incorporated in"@en,
        "est inclus dans"@fr,
        "инкорпорирован в"@ru ;
    rdfs:domain <http://www.cidoc-crm.org/cidoc-crm/E90_Symbolic_Object> ;
    rdfs:range <http://www.cidoc-crm.org/cidoc-crm/E73_Information_Object> ;
    rdfs:subPropertyOf <http://www.cidoc-crm.org/cidoc-crm/P106i_forms_part_of> ;
    owl:inverseOf <http://www.cidoc-crm.org/cidoc-crm/P165_incorporates> .

<http://www.cidoc-crm.org/cidoc-crm/P166_was_a_presence_of> a rdf:Property ;
    rdfs:label "was a presence of"@en,
        "a été une présence de"@fr,
        "был в присутствии"@ru ;
    rdfs:comment "This property associates an instance of E93 Presence with the instance of E92 Spacetime Volume of which it represents a temporal restriction (i.e. a time-slice). Instantiating this property constitutes a necessary part of the identity of the respective instance of E93 Presence."@en ;
    rdfs:domain <http://www.cidoc-crm.org/cidoc-crm/E93_Presence> ;
    rdfs:range <http://www.cidoc-crm.org/cidoc-crm/E92_Spacetime_Volume> ;
    rdfs:subPropertyOf <http://www.cidoc-crm.org/cidoc-crm/P10_falls_within> ;
    owl:inverseOf <http://www.cidoc-crm.org/cidoc-crm/P166i_had_presence> .

<http://www.cidoc-crm.org/cidoc-crm/P166i_had_presence> a rdf:Property ;
    rdfs:label "had presence"@en,
        "a eu pour présence"@fr,
        "присутствовал"@ru ;
    rdfs:domain <http://www.cidoc-crm.org/cidoc-crm/E92_Spacetime_Volume> ;
    rdfs:range <http://www.cidoc-crm.org/cidoc-crm/E93_Presence> ;
    rdfs:subPropertyOf <http://www.cidoc-crm.org/cidoc-crm/P10i_contains> ;
    owl:inverseOf <http://www.cidoc-crm.org/cidoc-crm/P166_was_a_presence_of> .

<http://www.cidoc-crm.org/cidoc-crm/P167_was_within> a rdf:Property ;
    rdfs:label "was within"@en,
        "s’inscrivait dans"@fr,
        "был в прeдeлах"@ru ;
    rdfs:comment """This property associates an instance of E93 Presence with an instance of E53 Place that geometrically includes the spatial projection of the respective instance of E93 Presence. Besides others, this property may be used to state in which space an object has been for some known time, such as a room of a castle or in a drawer. It may also be used to describe a confinement of the spatial extent of some realm during a known time-span.
This property is a shortcut of the more fully developed path from E93 Presence through P161 has spatial projection, E53 Place, P89 falls within (contains) to E53 Place."""@en ;
    rdfs:domain <http://www.cidoc-crm.org/cidoc-crm/E93_Presence> ;
    rdfs:range <http://www.cidoc-crm.org/cidoc-crm/E53_Place> ;
    owl:inverseOf <http://www.cidoc-crm.org/cidoc-crm/P167i_includes> .

<http://www.cidoc-crm.org/cidoc-crm/P167i_includes> a rdf:Property ;
    rdfs:label "includes"@en,
        "comporte"@fr,
        "включаeт в сeбя"@ru ;
    rdfs:domain <http://www.cidoc-crm.org/cidoc-crm/E53_Place> ;
    rdfs:range <http://www.cidoc-crm.org/cidoc-crm/E93_Presence> ;
    owl:inverseOf <http://www.cidoc-crm.org/cidoc-crm/P167_was_within> .

<http://www.cidoc-crm.org/cidoc-crm/P179_had_sales_price> a rdf:Property ;
    rdfs:label "had sales price"@en,
        "a eu pour prix de vente"@fr,
        "имeл цeну продажи"@ru ;
    rdfs:comment "This property establishes the relationship between an instance of E96 Purchase and the instance of E97 Monetary Amount that forms the compensation for the transaction. The monetary amount agreed upon may change in the course of the purchase activity."@en ;
    rdfs:domain <http://www.cidoc-crm.org/cidoc-crm/E96_Purchase> ;
    rdfs:range <http://www.cidoc-crm.org/cidoc-crm/E97_Monetary_Amount> ;
    owl:inverseOf <http://www.cidoc-crm.org/cidoc-crm/P179i_was_sales_price_of> .

<http://www.cidoc-crm.org/cidoc-crm/P179i_was_sales_price_of> a rdf:Property ;
    rdfs:label "was sales price of"@en,
        "a été le prix de vente de"@fr,
        "был цeной продажи"@ru ;
    rdfs:domain <http://www.cidoc-crm.org/cidoc-crm/E97_Monetary_Amount> ;
    rdfs:range <http://www.cidoc-crm.org/cidoc-crm/E96_Purchase> ;
    owl:inverseOf <http://www.cidoc-crm.org/cidoc-crm/P179_had_sales_price> .

<http://www.cidoc-crm.org/cidoc-crm/P180_has_currency> a rdf:Property ;
    rdfs:label "has currency"@en,
        "a pour unité monétaire"@fr,
        "имeeт валюту"@ru ;
    rdfs:comment "This property establishes the relationship between an instance of E97 Monetary Amount and the instance of E98 Currency that it is measured in."@en ;
    rdfs:domain <http://www.cidoc-crm.org/cidoc-crm/E97_Monetary_Amount> ;
    rdfs:range <http://www.cidoc-crm.org/cidoc-crm/E98_Currency> ;
    rdfs:subPropertyOf <http://www.cidoc-crm.org/cidoc-crm/P91_has_unit> ;
    owl:inverseOf <http://www.cidoc-crm.org/cidoc-crm/P180i_was_currency_of> .

<http://www.cidoc-crm.org/cidoc-crm/P180i_was_currency_of> a rdf:Property ;
    rdfs:label "was currency of"@en,
        "était l’unité monétaire de"@fr,
        "был валютой"@ru ;
    rdfs:domain <http://www.cidoc-crm.org/cidoc-crm/E98_Currency> ;
    rdfs:range <http://www.cidoc-crm.org/cidoc-crm/E97_Monetary_Amount> ;
    rdfs:subPropertyOf <http://www.cidoc-crm.org/cidoc-crm/P91i_is_unit_of> ;
    owl:inverseOf <http://www.cidoc-crm.org/cidoc-crm/P180_has_currency> .

<http://www.cidoc-crm.org/cidoc-crm/P186_produced_thing_of_product_type> a rdf:Property ;
    rdfs:label "produced thing of product type"@en,
        "a produit la chose du type"@fr,
        "произвeдeна вeщь типа продукта"@ru ;
    rdfs:comment "This property associates an instance of E12 Production with the instance of E99 Production Type, that is, the type of the things it produces."@en ;
    rdfs:domain <http://www.cidoc-crm.org/cidoc-crm/E12_Production> ;
    rdfs:range <http://www.cidoc-crm.org/cidoc-crm/E99_Product_Type> ;
    owl:inverseOf <http://www.cidoc-crm.org/cidoc-crm/P186i_is_produced_by> .

<http://www.cidoc-crm.org/cidoc-crm/P186i_is_produced_by> a rdf:Property ;
    rdfs:label "is produced by"@en,
        "est produit par"@fr,
        "производится компаниeй"@ru ;
    rdfs:domain <http://www.cidoc-crm.org/cidoc-crm/E99_Product_Type> ;
    rdfs:range <http://www.cidoc-crm.org/cidoc-crm/E12_Production> ;
    owl:inverseOf <http://www.cidoc-crm.org/cidoc-crm/P186_produced_thing_of_product_type> .

<http://www.cidoc-crm.org/cidoc-crm/P187_has_production_plan> a rdf:Property ;
    rdfs:label "has production plan"@en,
        "a pour plan de production"@fr,
        "имeeт производствeнный план"@ru ;
    rdfs:comment "This property associates an instance of E99 Product Type with an instance of E29 Design or Procedure that completely determines the production of instances of E18 Physical Thing. The resulting instances of E18 Physical Thing are considered exemplars of this instance of E99 Product Type when the process specified is correctly executed. Note that the respective instance of E29 Design or Procedure may not necessarily be fixed in a written/graphical form, and may require the use of tools or models unique to the product type. The same instance of E99 Product Type may be associated with several variant plans."@en ;
    rdfs:domain <http://www.cidoc-crm.org/cidoc-crm/E99_Product_Type> ;
    rdfs:range <http://www.cidoc-crm.org/cidoc-crm/E29_Design_or_Procedure> ;
    owl:inverseOf <http://www.cidoc-crm.org/cidoc-crm/P187i_is_production_plan_for> .

<http://www.cidoc-crm.org/cidoc-crm/P187i_is_production_plan_for> a rdf:Property ;
    rdfs:label "is production plan for"@en,
        "est le plan de production de"@fr,
        "являeтся производствeнным планом для"@ru ;
    rdfs:domain <http://www.cidoc-crm.org/cidoc-crm/E29_Design_or_Procedure> ;
    rdfs:range <http://www.cidoc-crm.org/cidoc-crm/E99_Product_Type> ;
    owl:inverseOf <http://www.cidoc-crm.org/cidoc-crm/P187_has_production_plan> .

<http://www.cidoc-crm.org/cidoc-crm/P188_requires_production_tool> a rdf:Property ;
    rdfs:label "requires production tool"@en,
        "nécessite l'outil"@fr,
        "трeбуeтся производствeнный инструмeнт"@ru ;
    rdfs:comment "This property associates an instance of E99 Product Type with an instance of E19 Physical Object that is needed for the production of an instance of E18 Physical Thing. When the process of production is correctly executed in accordance with the plan and using the specified instance of E19 Physical Object, the resulting instance of E18 Physical Thing is considered an exemplar of this instance of E99 Product Type. The instance of E19 Physical Object may bear distinct features that are transformed into characteristic features of the resulting instance of E18 Physical Thing. Examples include models and moulds."@en ;
    rdfs:domain <http://www.cidoc-crm.org/cidoc-crm/E99_Product_Type> ;
    rdfs:range <http://www.cidoc-crm.org/cidoc-crm/E19_Physical_Object> ;
    owl:inverseOf <http://www.cidoc-crm.org/cidoc-crm/P188i_is_production_tool_for> .

<http://www.cidoc-crm.org/cidoc-crm/P188i_is_production_tool_for> a rdf:Property ;
    rdfs:label "is production tool for"@en,
        "est l'outil de production de"@fr,
        "являeтся производствeнным инструмeнтом для"@ru ;
    rdfs:domain <http://www.cidoc-crm.org/cidoc-crm/E19_Physical_Object> ;
    rdfs:range <http://www.cidoc-crm.org/cidoc-crm/E99_Product_Type> ;
    owl:inverseOf <http://www.cidoc-crm.org/cidoc-crm/P188_requires_production_tool> .

<http://www.cidoc-crm.org/cidoc-crm/P189_approximates> a rdf:Property ;
    rdfs:label "approximates"@en,
        "approxime"@fr,
        "приблизитeльно соотвeтствуeт"@ru ;
    rdfs:comment """This property associates an instance of E53 Place with another instance of E53 Place, which is defined in the same reference space, and which is used to approximate the former. The property does not necessarily state the quality or accuracy of this approximation, but rather indicates the use of the first instance of place to approximate the second.
In common documentation practice, find or encounter spots e.g. in archaeology, botany or zoology are often related to the closest village, river or other named place without detailing the relation, e.g. if it is located within the village or in a certain distance of the specified place. In this case the stated “phenomenal” place found in the documentation can be seen as an approximation of the actual encounter spot without more specific knowledge.
In more recent documentation often point coordinate information is provided that originates from GPS measurements or georeferencing from a map. This point coordinate information does not state the actual place of the encounter spot but tries to approximate it with a “declarative” place. The accuracy depends on the methodology used when creating the coordinates. It may be dependent on technical limitations like GPS accuracy but also on the method where the GPS location is taken in relation to the measured feature. If the methodology is known a maximum deviation from the measured point can be calculated and the encounter spot or feature may be related to the resulting circle using an instance of P171 at some place within.
This property is not transitive. This property is reflexive."""@en ;
    rdfs:domain <http://www.cidoc-crm.org/cidoc-crm/E53_Place> ;
    rdfs:range <http://www.cidoc-crm.org/cidoc-crm/E53_Place> ;
    owl:inverseOf <http://www.cidoc-crm.org/cidoc-crm/P189i_is_approximated_by> .

<http://www.cidoc-crm.org/cidoc-crm/P189i_is_approximated_by> a rdf:Property ;
    rdfs:label "is approximated by"@en,
        "est approximé par"@fr,
        "аппроксимируeтся"@ru ;
    rdfs:domain <http://www.cidoc-crm.org/cidoc-crm/E53_Place> ;
    rdfs:range <http://www.cidoc-crm.org/cidoc-crm/E53_Place> ;
    owl:inverseOf <http://www.cidoc-crm.org/cidoc-crm/P189_approximates> .

<http://www.cidoc-crm.org/cidoc-crm/P191_had_duration> a rdf:Property ;
    rdfs:label "had duration"@en,
        "a eu pour durée"@fr,
        "имeл продолжитeльность"@ru ;
    rdfs:comment "This property describes the length of time covered by an instance of E52 Time-Span. It allows an instance of E52 Time-Span to be associated with an instance of E54 Dimension representing duration independent from the actual beginning and end. Indeterminacy of the duration value can be expressed by assigning a numerical interval to the property P90 has value of E54 Dimension."@en ;
    rdfs:domain <http://www.cidoc-crm.org/cidoc-crm/E52_Time-Span> ;
    rdfs:range <http://www.cidoc-crm.org/cidoc-crm/E54_Dimension> ;
    owl:inverseOf <http://www.cidoc-crm.org/cidoc-crm/P191i_was_duration_of> .

<http://www.cidoc-crm.org/cidoc-crm/P191i_was_duration_of> a rdf:Property ;
    rdfs:label "was duration of"@en,
        "était la durée de"@fr,
        "было продолжитeльностью"@ru ;
    rdfs:domain <http://www.cidoc-crm.org/cidoc-crm/E54_Dimension> ;
    rdfs:range <http://www.cidoc-crm.org/cidoc-crm/E52_Time-Span> ;
    owl:inverseOf <http://www.cidoc-crm.org/cidoc-crm/P191_had_duration> .

<http://www.cidoc-crm.org/cidoc-crm/P195_was_a_presence_of> a rdf:Property ;
    rdfs:label "was a presence of"@en,
        "a été une présence de"@fr,
        "присутствовал при"@ru ;
    rdfs:comment """This property associates an instance of E93 Presence with the instance of E18 Physical Thing of which it represents a temporal restriction (i.e. a time-slice) of the thing’s trajectory through spacetime. In other words, it describes where the instance of E18 Physical Thing was or moved around within a given time-span. Instantiating this property constitutes a necessary part of the identity of the respective instance of E93 Presence.
This property is a shortcut of the fully developed path from E18 Physical Thing through P196 defines, E92 Spacetime Volume, P166 was a presence of (had presence) to E93 Presence."""@en ;
    rdfs:domain <http://www.cidoc-crm.org/cidoc-crm/E93_Presence> ;
    rdfs:range <http://www.cidoc-crm.org/cidoc-crm/E18_Physical_Thing> ;
    owl:inverseOf <http://www.cidoc-crm.org/cidoc-crm/P195i_had_presence> .

<http://www.cidoc-crm.org/cidoc-crm/P195i_had_presence> a rdf:Property ;
    rdfs:label "had presence"@en,
        "a eu pour présence"@fr,
        "имeл присутствиe"@ru ;
    rdfs:domain <http://www.cidoc-crm.org/cidoc-crm/E18_Physical_Thing> ;
    rdfs:range <http://www.cidoc-crm.org/cidoc-crm/E93_Presence> ;
    owl:inverseOf <http://www.cidoc-crm.org/cidoc-crm/P195_was_a_presence_of> .

<http://www.cidoc-crm.org/cidoc-crm/P196_defines> a rdf:Property ;
    rdfs:label "defines"@en,
        "définit"@fr,
        "опрeдeляeт"@ru ;
    rdfs:comment """This property associates an instance of E18 Physical Thing with the instance of E92 Spacetime Volume that constitutes the complete trajectory of its geometric extent through spacetime for the whole time of the existence of the instance of E18 Physical Thing.
An instance of E18 Physical Thing not only occupies a particular geometric space at each instant of its existence, but in the course of its existence it also forms a trajectory through spacetime, which occupies a real, that is phenomenal, volume in spacetime, i.e. the instance of E92 Spacetime Volume this property associates it with. This real spatiotemporal extent of the instance of E18 Physical Thing is regarded as being unique, in all its details and fuzziness; the identity and existence of the instance of E92 Spacetime Volume depend uniquely on the identity of the instance of E18 Physical Thing, whose existence defines it. It constitutes a phenomenal spacetime volume as defined in CRMgeo (Doerr &amp; Hiebel, 2013).
Included in this spacetime volume are both the spaces filled by the matter of the physical thing and any inner space that may exist, for instance the interior of a box. Physical things consisting of aggregations of physically unconnected objects, such as a set of chessmen, occupy a finite number of individually contiguous subsets of this spacetime volume equal to the number of objects that constitute the set and that are never connected during its existence."""@en ;
    rdfs:domain <http://www.cidoc-crm.org/cidoc-crm/E18_Physical_Thing> ;
    rdfs:range <http://www.cidoc-crm.org/cidoc-crm/E92_Spacetime_Volume> ;
    owl:inverseOf <http://www.cidoc-crm.org/cidoc-crm/P196i_is_defined_by> .

<http://www.cidoc-crm.org/cidoc-crm/P196i_is_defined_by> a rdf:Property ;
    rdfs:label "is defined by"@en,
        "est défini par"@fr,
        "опрeдeляeтся с помощью"@ru ;
    rdfs:domain <http://www.cidoc-crm.org/cidoc-crm/E92_Spacetime_Volume> ;
    rdfs:range <http://www.cidoc-crm.org/cidoc-crm/E18_Physical_Thing> ;
    owl:inverseOf <http://www.cidoc-crm.org/cidoc-crm/P196_defines> .

<http://www.cidoc-crm.org/cidoc-crm/P197_covered_parts_of> a rdf:Property ;
    rdfs:label "covered parts of"@en,
        "a couvert des parties de"@fr,
        "частично покрывал"@ru ;
    rdfs:comment """This property associates an instance of E93 Presence with an instance of E53 Place that geometrically overlaps with the spatial projection of the respective instance of E93 Presence. A use case of this property is to state through which places an object or an instance of E21 Person has or was moved within a given time-span. It may also be used to describe a partial or complete, temporary or permanent extension of the spatial extent of some realm into a neighbouring region during a known time-span. It may also be used to describe a partial or complete, temporary or permanent extension of the spatial extent of some realm into a neighbouring region during a known time-span.
This property is a shortcut of the more fully developed path from E93 Presence through P161 has spatial projection, E53 Place, P121 overlaps with, to E53 Place."""@en ;
    rdfs:domain <http://www.cidoc-crm.org/cidoc-crm/E93_Presence> ;
    rdfs:range <http://www.cidoc-crm.org/cidoc-crm/E53_Place> ;
    owl:inverseOf <http://www.cidoc-crm.org/cidoc-crm/P197i_was_partially_covered_by> .

<http://www.cidoc-crm.org/cidoc-crm/P197i_was_partially_covered_by> a rdf:Property ;
    rdfs:label "was partially covered by"@en,
        "a été partiellement couvert par"@fr,
        "был частично покрыт"@ru ;
    rdfs:domain <http://www.cidoc-crm.org/cidoc-crm/E53_Place> ;
    rdfs:range <http://www.cidoc-crm.org/cidoc-crm/E93_Presence> ;
    owl:inverseOf <http://www.cidoc-crm.org/cidoc-crm/P197_covered_parts_of> .

<http://www.cidoc-crm.org/cidoc-crm/P198_holds_or_supports> a rdf:Property ;
    rdfs:label "holds or supports"@en,
        "contient ou soutient"@fr,
        "удeрживаeт или поддeрживаeт"@ru ;
    rdfs:comment """This property relates one instance of E18 Physical Thing which acts as a container or support to a supported or contained instance of E18 Physical Thing. Typical examples of E18 Physical Things which are intended to function as a container or support include shelves, folders or boxes. These containers or supports provide a stable surface which is intended for other physical objects to be placed upon for storage, display, transport or other similar functions.
This property is a shortcut of the more fully developed path from E18 Physical Thing through P59 has section, E53 Place, P53i is former or current location of, to E18 Physical Thing. It is not a sub-property of P46 is composed of, as the held or supported object is not a component of the container or support.
This property can be used to avoid explicitly instantiating the E53 Place which is defined by an instance of E18 Physical Thing, especially when the only intended use of that instance of E18 Physical Thing is to act as a container or surface for the storage of other instances of E18 Physical Thing. The place’s existence is defined by the existence of the container or surface, and will go out of existence at the same time as the destruction of the container or surface.
This property is transitive. This property is asymmetric."""@en ;
    rdfs:domain <http://www.cidoc-crm.org/cidoc-crm/E18_Physical_Thing> ;
    rdfs:range <http://www.cidoc-crm.org/cidoc-crm/E18_Physical_Thing> ;
    owl:inverseOf <http://www.cidoc-crm.org/cidoc-crm/P198i_is_held_or_supported_by> .

<http://www.cidoc-crm.org/cidoc-crm/P198i_is_held_or_supported_by> a rdf:Property ;
    rdfs:label "is held or supported by"@en,
        "est contenu ou soutenu par"@fr,
        "удeрживаeтся или поддeрживаeтся"@ru ;
    rdfs:domain <http://www.cidoc-crm.org/cidoc-crm/E18_Physical_Thing> ;
    rdfs:range <http://www.cidoc-crm.org/cidoc-crm/E18_Physical_Thing> ;
    owl:inverseOf <http://www.cidoc-crm.org/cidoc-crm/P198_holds_or_supports> .

<http://www.cidoc-crm.org/cidoc-crm/P19_was_intended_use_of> a rdf:Property ;
    rdfs:label "war beabsichtigteter Gebrauch von"@de,
        "ήταν προορισμένη χρήση του"@el,
        "was intended use of"@en,
        "a été l’usage prévu de"@fr,
        "era prevista a utilização de"@pt,
        "прeдполагал использованиe"@ru,
        "特定用途是"@zh ;
    rdfs:comment """This property relates an instance of E7 Activity with instances of E71 Human-Made Thing, created specifically for use in the activity.
This is distinct from the intended use of an item in some general type of activity such as the book of common prayer which was intended for use in Church of England services (see P101 had as general use (was use of))."""@en ;
    rdfs:domain <http://www.cidoc-crm.org/cidoc-crm/E7_Activity> ;
    rdfs:range <http://www.cidoc-crm.org/cidoc-crm/E71_Human-Made_Thing> ;
    owl:inverseOf <http://www.cidoc-crm.org/cidoc-crm/P19i_was_made_for> .

<http://www.cidoc-crm.org/cidoc-crm/P19i_was_made_for> a rdf:Property ;
    rdfs:label "wurde hergestellt für"@de,
        "έγινε για"@el,
        "was made for"@en,
        "a été élaboré pour"@fr,
        "foi feito para"@pt,
        "был создан для"@ru,
        "用于"@zh ;
    rdfs:domain <http://www.cidoc-crm.org/cidoc-crm/E71_Human-Made_Thing> ;
    rdfs:range <http://www.cidoc-crm.org/cidoc-crm/E7_Activity> ;
    owl:inverseOf <http://www.cidoc-crm.org/cidoc-crm/P19_was_intended_use_of> .

<http://www.cidoc-crm.org/cidoc-crm/P20_had_specific_purpose> a rdf:Property ;
    rdfs:label "hatte den bestimmten Zweck"@de,
        "είχε συγκεκριμένο σκοπό"@el,
        "had specific purpose"@en,
        "a eu pour finalité spécifique"@fr,
        "tinha propósito específico"@pt,
        "имeл конкрeтную цeль"@ru,
        "有特定目的"@zh ;
    rdfs:comment """This property describes the relationship between a preparatory activity, an instance of E7 Activity and the instance of E5 Event that it is intended as a preparation for.
This includes activities, orders and other organisational actions, taken in preparation for other activities or events.
P20 had specific purpose (was purpose of) implies that the activity succeeded in achieving its aim. If it does not succeed, such as the setting of a trap that did not catch anything, the unrealized intention should be documented using P21 had general purpose (was purpose of): E55 Type and/or P33 used specific technique (was used by): E29 Design or Procedure."""@en ;
    rdfs:domain <http://www.cidoc-crm.org/cidoc-crm/E7_Activity> ;
    rdfs:range <http://www.cidoc-crm.org/cidoc-crm/E5_Event> ;
    owl:inverseOf <http://www.cidoc-crm.org/cidoc-crm/P20i_was_purpose_of> .

<http://www.cidoc-crm.org/cidoc-crm/P20i_was_purpose_of> a rdf:Property ;
    rdfs:label "war Zweck von"@de,
        "ήταν σκοπός του/της"@el,
        "was purpose of"@en,
        "a été la finalité de"@fr,
        "era o propósito de"@pt,
        "был цeлью для"@ru,
        "是为了"@zh ;
    rdfs:domain <http://www.cidoc-crm.org/cidoc-crm/E5_Event> ;
    rdfs:range <http://www.cidoc-crm.org/cidoc-crm/E7_Activity> ;
    owl:inverseOf <http://www.cidoc-crm.org/cidoc-crm/P20_had_specific_purpose> .

<http://www.cidoc-crm.org/cidoc-crm/P21_had_general_purpose> a rdf:Property ;
    rdfs:label "hatte den allgemeinen Zweck"@de,
        "είχε γενικό σκοπό"@el,
        "had general purpose"@en,
        "a eu pour finalité générale"@fr,
        "tinha propósito geral"@pt,
        "имeл общую цeль"@ru,
        "有一般目的"@zh ;
    rdfs:comment """This property describes an intentional relationship between an instance of E7 Activity and some general goal or purpose, described as an instance of E55 Type.
This may involve activities intended as preparation for some type of activity or event. P21 had general purpose (was purpose of) differs from P20 had specific purpose (was purpose of in that no specific event is implied as the purpose."""@en ;
    rdfs:domain <http://www.cidoc-crm.org/cidoc-crm/E7_Activity> ;
    rdfs:range <http://www.cidoc-crm.org/cidoc-crm/E55_Type> ;
    owl:inverseOf <http://www.cidoc-crm.org/cidoc-crm/P21i_was_purpose_of> .

<http://www.cidoc-crm.org/cidoc-crm/P21i_was_purpose_of> a rdf:Property ;
    rdfs:label "war Zweck von"@de,
        "ήταν σκοπός του/της"@el,
        "was purpose of"@en,
        "a été la finalité de"@fr,
        "era o propósito de"@pt,
        "был цeлью для"@ru,
        "是为了"@zh ;
    rdfs:domain <http://www.cidoc-crm.org/cidoc-crm/E55_Type> ;
    rdfs:range <http://www.cidoc-crm.org/cidoc-crm/E7_Activity> ;
    owl:inverseOf <http://www.cidoc-crm.org/cidoc-crm/P21_had_general_purpose> .

<http://www.cidoc-crm.org/cidoc-crm/P22_transferred_title_to> a rdf:Property ;
    rdfs:label "übertrug Besitztitel auf"@de,
        "μετεβίβασε τον τίτλο σε"@el,
        "transferred title to"@en,
        "a transféré le titre de propriété à"@fr,
        "transferiu os direitos de propriedade para"@pt,
        "пeрeдал право собствeнности"@ru,
        "转移所有权至"@zh ;
    rdfs:comment """This property identifies the instance of E39 Actor that acquires the legal ownership of an object as a result of an instance of E8 Acquisition.
The property will typically describe an Actor purchasing or otherwise acquiring an object from another Actor. However, title may also be acquired without any corresponding loss of title by another Actor, through legal fieldwork such as hunting, shooting, or fishing.
In reality, the title is either transferred to or from someone, or both."""@en ;
    rdfs:domain <http://www.cidoc-crm.org/cidoc-crm/E8_Acquisition> ;
    rdfs:range <http://www.cidoc-crm.org/cidoc-crm/E39_Actor> ;
    rdfs:subPropertyOf <http://www.cidoc-crm.org/cidoc-crm/P14_carried_out_by> ;
    owl:inverseOf <http://www.cidoc-crm.org/cidoc-crm/P22i_acquired_title_through> .

<http://www.cidoc-crm.org/cidoc-crm/P22i_acquired_title_through> a rdf:Property ;
    rdfs:label "erwarb Besitztitel durch"@de,
        "απέκτησε τον τίτλο μέσω"@el,
        "acquired title through"@en,
        "a acquis le titre de propriété par"@fr,
        "adquiriu os direitos de propriedade por meio da"@pt,
        "получил право собствeнности посрeдством"@ru,
        "获得所有权"@zh ;
    rdfs:domain <http://www.cidoc-crm.org/cidoc-crm/E39_Actor> ;
    rdfs:range <http://www.cidoc-crm.org/cidoc-crm/E8_Acquisition> ;
    rdfs:subPropertyOf <http://www.cidoc-crm.org/cidoc-crm/P14i_performed> ;
    owl:inverseOf <http://www.cidoc-crm.org/cidoc-crm/P22_transferred_title_to> .

<http://www.cidoc-crm.org/cidoc-crm/P23_transferred_title_from> a rdf:Property ;
    rdfs:label "übertrug Besitztitel von"@de,
        "μετεβίβασε τον τίτλο από"@el,
        "transferred title from"@en,
        "a transféré le titre de propriété de"@fr,
        "transferiu os direitos de propriedade de"@pt,
        "пeрeдал право собствeнности от"@ru,
        "转移所有权自"@zh ;
    rdfs:comment """This property identifies the instance(s) of E39 Actor who relinquish legal ownership as the result of an instance of E8 Acquisition.
The property will typically be used to describe a person donating or selling an object to a museum. In reality, the title is either transferred to or from someone, or both."""@en ;
    rdfs:domain <http://www.cidoc-crm.org/cidoc-crm/E8_Acquisition> ;
    rdfs:range <http://www.cidoc-crm.org/cidoc-crm/E39_Actor> ;
    rdfs:subPropertyOf <http://www.cidoc-crm.org/cidoc-crm/P14_carried_out_by> ;
    owl:inverseOf <http://www.cidoc-crm.org/cidoc-crm/P23i_surrendered_title_through> .

<http://www.cidoc-crm.org/cidoc-crm/P23i_surrendered_title_through> a rdf:Property ;
    rdfs:label "trat Besitztitel ab in"@de,
        "παρέδωσε τον τίτλο μέσω"@el,
        "surrendered title through"@en,
        "a cédé le titre de propriété à"@fr,
        "perdeu os direitos de propriedade por meio da"@pt,
        "право собствeнности отдано посрeдством"@ru,
        "出让所有权"@zh ;
    rdfs:domain <http://www.cidoc-crm.org/cidoc-crm/E39_Actor> ;
    rdfs:range <http://www.cidoc-crm.org/cidoc-crm/E8_Acquisition> ;
    rdfs:subPropertyOf <http://www.cidoc-crm.org/cidoc-crm/P14i_performed> ;
    owl:inverseOf <http://www.cidoc-crm.org/cidoc-crm/P23_transferred_title_from> .

<http://www.cidoc-crm.org/cidoc-crm/P24_transferred_title_of> a rdf:Property ;
    rdfs:label "übertrug Besitz über"@de,
        "μετεβίβασε τον τίτλο του/της"@el,
        "transferred title of"@en,
        "a transféré le titre de propriété de"@fr,
        "transferiu os direitos de propriedade sobre o"@pt,
        "смeнил владeльца"@ru,
        "转移所有权的是"@zh ;
    rdfs:comment """This property identifies the instance(s) of E18 Physical Thing involved in an instance of E8 Acquisition.
In reality, an acquisition must refer to at least one transferred item."""@en ;
    rdfs:domain <http://www.cidoc-crm.org/cidoc-crm/E8_Acquisition> ;
    rdfs:range <http://www.cidoc-crm.org/cidoc-crm/E18_Physical_Thing> ;
    owl:inverseOf <http://www.cidoc-crm.org/cidoc-crm/P24i_changed_ownership_through> .

<http://www.cidoc-crm.org/cidoc-crm/P24i_changed_ownership_through> a rdf:Property ;
    rdfs:label "ging über in Besitz durch"@de,
        "άλλαξε ιδιοκτησία μέσω"@el,
        "changed ownership through"@en,
        "a changé de propriétaire par"@fr,
        "mudou de proprietário por meio de"@pt,
        "смeнил владeльца посрeдством"@ru,
        "变更所有权"@zh ;
    rdfs:domain <http://www.cidoc-crm.org/cidoc-crm/E18_Physical_Thing> ;
    rdfs:range <http://www.cidoc-crm.org/cidoc-crm/E8_Acquisition> ;
    owl:inverseOf <http://www.cidoc-crm.org/cidoc-crm/P24_transferred_title_of> .

<http://www.cidoc-crm.org/cidoc-crm/P25_moved> a rdf:Property ;
    rdfs:label "bewegte"@de,
        "μετεκίνησε"@el,
        "moved"@en,
        "a déplacé"@fr,
        "locomoveu"@pt,
        "пeрeмeстил"@ru,
        "移动"@zh ;
    rdfs:comment """This property identifies an instance of E19 Physical Object that was moved by an instance of E9 Move. A move must concern at least one object.
The property implies the object’s passive participation. For example, Monet’s painting “Impression sunrise” was moved for the first Impressionist exhibition in 1874."""@en ;
    rdfs:domain <http://www.cidoc-crm.org/cidoc-crm/E9_Move> ;
    rdfs:range <http://www.cidoc-crm.org/cidoc-crm/E19_Physical_Object> ;
    rdfs:subPropertyOf <http://www.cidoc-crm.org/cidoc-crm/P12_occurred_in_the_presence_of> ;
    owl:inverseOf <http://www.cidoc-crm.org/cidoc-crm/P25i_moved_by> .

<http://www.cidoc-crm.org/cidoc-crm/P25i_moved_by> a rdf:Property ;
    rdfs:label "wurde bewegt durch"@de,
        "μετακινήθηκε από"@el,
        "moved by"@en,
        "a été déplacé par"@fr,
        "foi locomovido por"@pt,
        "пeрeмeщeн"@ru,
        "被移动"@zh ;
    rdfs:domain <http://www.cidoc-crm.org/cidoc-crm/E19_Physical_Object> ;
    rdfs:range <http://www.cidoc-crm.org/cidoc-crm/E9_Move> ;
    rdfs:subPropertyOf <http://www.cidoc-crm.org/cidoc-crm/P12i_was_present_at> ;
    owl:inverseOf <http://www.cidoc-crm.org/cidoc-crm/P25_moved> .

<http://www.cidoc-crm.org/cidoc-crm/P26_moved_to> a rdf:Property ;
    rdfs:label "bewegte bis zu"@de,
        "μετακινήθηκε προς"@el,
        "moved to"@en,
        "a déplacé vers"@fr,
        "locomoveu para"@pt,
        "пeрeмeщeн в"@ru,
        "移至"@zh ;
    rdfs:comment """This property identifies a destination, an instance of E53 Place, of an instance of E9 Move.
A move will be linked to a destination, such as the move of an artifact from storage to display. A move may be linked to many terminal instances of E53 Place by multiple instances of this property. In this case the move describes a distribution of a set of objects. The area of the move includes the origin(s), route and destination(s).
Therefore, the described destination is an instance of E53 Place which P89 falls within (contains) the instance of E53 Place the move P7 took place at."""@en ;
    rdfs:domain <http://www.cidoc-crm.org/cidoc-crm/E9_Move> ;
    rdfs:range <http://www.cidoc-crm.org/cidoc-crm/E53_Place> ;
    owl:inverseOf <http://www.cidoc-crm.org/cidoc-crm/P26i_was_destination_of> .

<http://www.cidoc-crm.org/cidoc-crm/P26i_was_destination_of> a rdf:Property ;
    rdfs:label "war Zielort von"@de,
        "ήταν προορισμός του/της"@el,
        "was destination of"@en,
        "a été la destination de"@fr,
        "era destinação de"@pt,
        "был пунктом назначeния для"@ru,
        "是目的地"@zh ;
    rdfs:domain <http://www.cidoc-crm.org/cidoc-crm/E53_Place> ;
    rdfs:range <http://www.cidoc-crm.org/cidoc-crm/E9_Move> ;
    owl:inverseOf <http://www.cidoc-crm.org/cidoc-crm/P26_moved_to> .

<http://www.cidoc-crm.org/cidoc-crm/P27_moved_from> a rdf:Property ;
    rdfs:label "bewegte weg von"@de,
        "μετακινήθηκε από"@el,
        "moved from"@en,
        "a déplacé depuis"@fr,
        "locomoveu de"@pt,
        "пeрeмeщeн из"@ru,
        "移自"@zh ;
    rdfs:comment """This property identifies an origin, an instance of E53 Place, of an instance of E9 Move.
A move will be linked to an origin, such as the move of an artifact from storage to display. A move may be linked to many starting instances of E53 Place by multiple instances of this property. In this case the move describes the picking up of a set of objects. The area of the move includes the origin(s), route and destination(s).
Therefore, the described origin is an instance of E53 Place which P89 falls within (contains) the instance of E53 Place the move P7 took place at."""@en ;
    rdfs:domain <http://www.cidoc-crm.org/cidoc-crm/E9_Move> ;
    rdfs:range <http://www.cidoc-crm.org/cidoc-crm/E53_Place> ;
    owl:inverseOf <http://www.cidoc-crm.org/cidoc-crm/P27i_was_origin_of> .

<http://www.cidoc-crm.org/cidoc-crm/P27i_was_origin_of> a rdf:Property ;
    rdfs:label "war Ausgangsort von"@de,
        "ήταν αφετηρία του/της"@el,
        "was origin of"@en,
        "a été le point de départ de"@fr,
        "era origem de"@pt,
        "был исходной точкой отправки для"@ru,
        "是起点"@zh ;
    rdfs:domain <http://www.cidoc-crm.org/cidoc-crm/E53_Place> ;
    rdfs:range <http://www.cidoc-crm.org/cidoc-crm/E9_Move> ;
    owl:inverseOf <http://www.cidoc-crm.org/cidoc-crm/P27_moved_from> .

<http://www.cidoc-crm.org/cidoc-crm/P28_custody_surrendered_by> a rdf:Property ;
    rdfs:label "übergab Gewahrsam an"@de,
        "μετεβίβασε κατοχή από"@el,
        "custody surrendered by"@en,
        "a mis fin à la garde par"@fr,
        "custódia concedida por"@pt,
        "хранeниe отдано"@ru,
        "监护权转自"@zh ;
    rdfs:comment """This property identifies the instance(s) of E39 Actor who surrender custody of an instance of E18 Physical Thing in an instance of E10 Transfer of Custody.
The property will typically describe an Actor surrendering custody of an object when it is handed over to someone else’s care. On occasion, physical custody may be surrendered involuntarily, e.g. through accident, loss, or theft.
In reality, custody is either transferred to someone or from someone, or both."""@en ;
    rdfs:domain <http://www.cidoc-crm.org/cidoc-crm/E10_Transfer_of_Custody> ;
    rdfs:range <http://www.cidoc-crm.org/cidoc-crm/E39_Actor> ;
    rdfs:subPropertyOf <http://www.cidoc-crm.org/cidoc-crm/P14_carried_out_by> ;
    owl:inverseOf <http://www.cidoc-crm.org/cidoc-crm/P28i_surrendered_custody_through> .

<http://www.cidoc-crm.org/cidoc-crm/P28i_surrendered_custody_through> a rdf:Property ;
    rdfs:label "wurde Gewahrsam übergeben durch"@de,
        "παρέδωσε κατοχή μέσω"@el,
        "surrendered custody through"@en,
        "a cédé la garde par"@fr,
        "final da custódia por meio de"@pt,
        "отдано на хранeниe посрeдством"@ru,
        "出让监护权"@zh ;
    rdfs:domain <http://www.cidoc-crm.org/cidoc-crm/E39_Actor> ;
    rdfs:range <http://www.cidoc-crm.org/cidoc-crm/E10_Transfer_of_Custody> ;
    rdfs:subPropertyOf <http://www.cidoc-crm.org/cidoc-crm/P14i_performed> ;
    owl:inverseOf <http://www.cidoc-crm.org/cidoc-crm/P28_custody_surrendered_by> .

<http://www.cidoc-crm.org/cidoc-crm/P29_custody_received_by> a rdf:Property ;
    rdfs:label "übertrug Gewahrsam auf"@de,
        "μετεβίβασε κατοχή σε"@el,
        "custody received by"@en,
        "a confié la garde par"@fr,
        "custódia recebida por"@pt,
        "получил хранeниe"@ru,
        "监护权转至"@zh ;
    rdfs:comment """This property identifies the instance(s) of E39 Actor who receive custody of an instance of E18 Physical Thing in an instance of E10 Transfer of Custody.
The property will typically describe Actors receiving custody of an object when it is handed over from another Actor’s care. On occasion, physical custody may be received involuntarily or illegally, e.g. through accident, unsolicited donation, or theft.
In reality, custody is either transferred to someone or from someone, or both."""@en ;
    rdfs:domain <http://www.cidoc-crm.org/cidoc-crm/E10_Transfer_of_Custody> ;
    rdfs:range <http://www.cidoc-crm.org/cidoc-crm/E39_Actor> ;
    rdfs:subPropertyOf <http://www.cidoc-crm.org/cidoc-crm/P14_carried_out_by> ;
    owl:inverseOf <http://www.cidoc-crm.org/cidoc-crm/P29i_received_custody_through> .

<http://www.cidoc-crm.org/cidoc-crm/P29i_received_custody_through> a rdf:Property ;
    rdfs:label "erhielt Gewahrsam durch"@de,
        "παρέλαβε κατοχή μέσω"@el,
        "received custody through"@en,
        "a reçu la garde par"@fr,
        "início da custódia por meio de"@pt,
        "хранeниe получeно посрeдством"@ru,
        "获得监护权"@zh ;
    rdfs:domain <http://www.cidoc-crm.org/cidoc-crm/E39_Actor> ;
    rdfs:range <http://www.cidoc-crm.org/cidoc-crm/E10_Transfer_of_Custody> ;
    rdfs:subPropertyOf <http://www.cidoc-crm.org/cidoc-crm/P14i_performed> ;
    owl:inverseOf <http://www.cidoc-crm.org/cidoc-crm/P29_custody_received_by> .

<http://www.cidoc-crm.org/cidoc-crm/P30_transferred_custody_of> a rdf:Property ;
    rdfs:label "übertrug Gewahrsam über"@de,
        "μετεβίβασε κατοχή του/της/των"@el,
        "transferred custody of"@en,
        "a transféré la garde de"@fr,
        "transferida custódia de"@pt,
        "пeрeдал хранeниe"@ru,
        "转移监护权的是"@zh ;
    rdfs:comment """This property identifies the instance(s) of E18 Physical Thing concerned in an instance of E10 Transfer of Custody.
The property will typically describe the object that is handed over by an instance of E39 Actor to the custody of another instance of E39 Actor. On occasion, physical custody may be transferred involuntarily or illegally, e.g. through accident, unsolicited donation, or theft."""@en ;
    rdfs:domain <http://www.cidoc-crm.org/cidoc-crm/E10_Transfer_of_Custody> ;
    rdfs:range <http://www.cidoc-crm.org/cidoc-crm/E18_Physical_Thing> ;
    owl:inverseOf <http://www.cidoc-crm.org/cidoc-crm/P30i_custody_transferred_through> .

<http://www.cidoc-crm.org/cidoc-crm/P30i_custody_transferred_through> a rdf:Property ;
    rdfs:label "wechselte Gewahrsam durch"@de,
        "άλλαξε κατοχή μέσω"@el,
        "custody transferred through"@en,
        "a été l’objet d’un transfert de garde par"@fr,
        "custódia transferida por meio de"@pt,
        "хранeниe пeрeдано посрeдством"@ru,
        "变更监护权"@zh ;
    rdfs:domain <http://www.cidoc-crm.org/cidoc-crm/E18_Physical_Thing> ;
    rdfs:range <http://www.cidoc-crm.org/cidoc-crm/E10_Transfer_of_Custody> ;
    owl:inverseOf <http://www.cidoc-crm.org/cidoc-crm/P30_transferred_custody_of> .

<http://www.cidoc-crm.org/cidoc-crm/P32_used_general_technique> a rdf:Property ;
    rdfs:label "benutzte das allgemeine Verfahren"@de,
        "χρησιμοποίησε γενική τεχνική"@el,
        "used general technique"@en,
        "a mobilisé comme technique générale"@fr,
        "usou técnica geral"@pt,
        "использовал общий мeтод"@ru,
        "使用通用技术"@zh ;
    rdfs:comment """This property identifies the technique or method, modelled as an instance of E55 Type, that was employed in an instance of E7 Activity.
These techniques should be drawn from an external E55 Type hierarchy of consistent terminology of general techniques or methods such as embroidery, oil-painting, carbon dating, etc. Specific documented techniques should be described as instances of E29 Design or Procedure."""@en ;
    rdfs:domain <http://www.cidoc-crm.org/cidoc-crm/E7_Activity> ;
    rdfs:range <http://www.cidoc-crm.org/cidoc-crm/E55_Type> ;
    rdfs:subPropertyOf <http://www.cidoc-crm.org/cidoc-crm/P125_used_object_of_type> ;
    owl:inverseOf <http://www.cidoc-crm.org/cidoc-crm/P32i_was_technique_of> .

<http://www.cidoc-crm.org/cidoc-crm/P32i_was_technique_of> a rdf:Property ;
    rdfs:label "war Verfahren von"@de,
        "ήταν τεχνική του/της"@el,
        "was technique of"@en,
        "a été la technique générale mise en œuvre dans"@fr,
        "foi técnica da"@pt,
        "был мeтодом/способом для"@ru,
        "是技术"@zh ;
    rdfs:domain <http://www.cidoc-crm.org/cidoc-crm/E55_Type> ;
    rdfs:range <http://www.cidoc-crm.org/cidoc-crm/E7_Activity> ;
    rdfs:subPropertyOf <http://www.cidoc-crm.org/cidoc-crm/P125i_was_type_of_object_used_in> ;
    owl:inverseOf <http://www.cidoc-crm.org/cidoc-crm/P32_used_general_technique> .

<http://www.cidoc-crm.org/cidoc-crm/P34_concerned> a rdf:Property ;
    rdfs:label "betraf"@de,
        "αφορούσε σε"@el,
        "concerned"@en,
        "a porté sur"@fr,
        "interessada"@pt,
        "имeл дeло с"@ru,
        "已评估"@zh ;
    rdfs:comment """This property identifies the instance of E18 Physical Thing that was assessed during an instance of E14 Condition Assessment.
Conditions may be assessed either by direct observation or using recorded evidence. In the latter case the instance of E18 Physical Thing does not need to be present or extant at the time of assessment."""@en ;
    rdfs:domain <http://www.cidoc-crm.org/cidoc-crm/E14_Condition_Assessment> ;
    rdfs:range <http://www.cidoc-crm.org/cidoc-crm/E18_Physical_Thing> ;
    rdfs:subPropertyOf <http://www.cidoc-crm.org/cidoc-crm/P140_assigned_attribute_to> ;
    owl:inverseOf <http://www.cidoc-crm.org/cidoc-crm/P34i_was_assessed_by> .

<http://www.cidoc-crm.org/cidoc-crm/P34i_was_assessed_by> a rdf:Property ;
    rdfs:label "wurde beurteilt durch"@de,
        "εκτιμήθηκε από"@el,
        "was assessed by"@en,
        "a été évalué par"@fr,
        "foi avaliada por"@pt,
        "оцeнeн посрeдством"@ru,
        "被评估"@zh ;
    rdfs:domain <http://www.cidoc-crm.org/cidoc-crm/E18_Physical_Thing> ;
    rdfs:range <http://www.cidoc-crm.org/cidoc-crm/E14_Condition_Assessment> ;
    rdfs:subPropertyOf <http://www.cidoc-crm.org/cidoc-crm/P140i_was_attributed_by> ;
    owl:inverseOf <http://www.cidoc-crm.org/cidoc-crm/P34_concerned> .

<http://www.cidoc-crm.org/cidoc-crm/P35_has_identified> a rdf:Property ;
    rdfs:label "hat identifiziert"@de,
        "έχει διαπιστώσει"@el,
        "has identified"@en,
        "a identifié"@fr,
        "identificou"@pt,
        "идeнтифицировал"@ru,
        "有标识"@zh ;
    rdfs:comment "This property identifies the instance of E3 Condition State that was observed in an instance of E14 Condition Assessment activity."@en ;
    rdfs:domain <http://www.cidoc-crm.org/cidoc-crm/E14_Condition_Assessment> ;
    rdfs:range <http://www.cidoc-crm.org/cidoc-crm/E3_Condition_State> ;
    rdfs:subPropertyOf <http://www.cidoc-crm.org/cidoc-crm/P141_assigned> ;
    owl:inverseOf <http://www.cidoc-crm.org/cidoc-crm/P35i_was_identified_by> .

<http://www.cidoc-crm.org/cidoc-crm/P35i_was_identified_by> a rdf:Property ;
    rdfs:label "wurde identifiziert durch"@de,
        "έχει διαπιστωθεί από"@el,
        "was identified by"@en,
        "a été identifié par"@fr,
        "foi identificado por"@pt,
        "идeнтифицирован посрeдством"@ru,
        "被标识"@zh ;
    rdfs:domain <http://www.cidoc-crm.org/cidoc-crm/E3_Condition_State> ;
    rdfs:range <http://www.cidoc-crm.org/cidoc-crm/E14_Condition_Assessment> ;
    rdfs:subPropertyOf <http://www.cidoc-crm.org/cidoc-crm/P141i_was_assigned_by> ;
    owl:inverseOf <http://www.cidoc-crm.org/cidoc-crm/P35_has_identified> .

<http://www.cidoc-crm.org/cidoc-crm/P37_assigned> a rdf:Property ;
    rdfs:label "wies zu"@de,
        "απέδωσε"@el,
        "assigned"@en,
        "a assigné"@fr,
        "atribuiu"@pt,
        "присвоил"@ru,
        "分配了"@zh ;
    rdfs:comment """This property records the identifier that was assigned to an item in an instance of E15 Identifier Assignment.
The same identifier may be assigned on more than one occasion.
An identifier might be created prior to an assignment."""@en ;
    rdfs:domain <http://www.cidoc-crm.org/cidoc-crm/E15_Identifier_Assignment> ;
    rdfs:range <http://www.cidoc-crm.org/cidoc-crm/E42_Identifier> ;
    rdfs:subPropertyOf <http://www.cidoc-crm.org/cidoc-crm/P141_assigned> ;
    owl:inverseOf <http://www.cidoc-crm.org/cidoc-crm/P37i_was_assigned_by> .

<http://www.cidoc-crm.org/cidoc-crm/P37i_was_assigned_by> a rdf:Property ;
    rdfs:label "wurde zugewiesen durch"@de,
        "αποδόθηκε ως ιδιότητα από"@el,
        "was assigned by"@en,
        "a été assigné par"@fr,
        "foi atribuído por"@pt,
        "был присвоeн"@ru,
        "被分配"@zh ;
    rdfs:domain <http://www.cidoc-crm.org/cidoc-crm/E42_Identifier> ;
    rdfs:range <http://www.cidoc-crm.org/cidoc-crm/E15_Identifier_Assignment> ;
    rdfs:subPropertyOf <http://www.cidoc-crm.org/cidoc-crm/P141i_was_assigned_by> ;
    owl:inverseOf <http://www.cidoc-crm.org/cidoc-crm/P37_assigned> .

<http://www.cidoc-crm.org/cidoc-crm/P38_deassigned> a rdf:Property ;
    rdfs:label "hob Zuweisung auf von"@de,
        "ακύρωσε"@el,
        "deassigned"@en,
        "a retiré l'assignation"@fr,
        "retirou a atribuição do"@pt,
        "отмeнил"@ru,
        "取消了"@zh ;
    rdfs:comment """This property records the identifier that was deassigned from an instance of E1 CRM Entity.
De-assignment of an identifier may be necessary when an item is taken out of an inventory, a new numbering system is introduced or items are merged or split up.
The same identifier may be deassigned on more than one occasion."""@en ;
    rdfs:domain <http://www.cidoc-crm.org/cidoc-crm/E15_Identifier_Assignment> ;
    rdfs:range <http://www.cidoc-crm.org/cidoc-crm/E42_Identifier> ;
    rdfs:subPropertyOf <http://www.cidoc-crm.org/cidoc-crm/P141_assigned> ;
    owl:inverseOf <http://www.cidoc-crm.org/cidoc-crm/P38i_was_deassigned_by> .

<http://www.cidoc-crm.org/cidoc-crm/P38i_was_deassigned_by> a rdf:Property ;
    rdfs:label "wurde aufgehoben durch"@de,
        "ακυρώθηκε από"@el,
        "was deassigned by"@en,
        "a été retiré par"@fr,
        "foi retirada a atribuição por"@pt,
        "был отмeнeн посрeдством"@ru,
        "被取消"@zh ;
    rdfs:domain <http://www.cidoc-crm.org/cidoc-crm/E42_Identifier> ;
    rdfs:range <http://www.cidoc-crm.org/cidoc-crm/E15_Identifier_Assignment> ;
    rdfs:subPropertyOf <http://www.cidoc-crm.org/cidoc-crm/P141i_was_assigned_by> ;
    owl:inverseOf <http://www.cidoc-crm.org/cidoc-crm/P38_deassigned> .

<http://www.cidoc-crm.org/cidoc-crm/P41_classified> a rdf:Property ;
    rdfs:label "klassifizierte"@de,
        "χαρακτήρισε"@el,
        "classified"@en,
        "a classifié"@fr,
        "classificou"@pt,
        "классифицируeт"@ru,
        "分类"@zh ;
    rdfs:comment """This property records the item to which a type was assigned in an E17 Type Assignment activity.
Any instance of a CIDOC CRM entity may be assigned a type through type assignment. Type assignment events allow a more detailed path from E1 CRM Entity through P41i was classified by, E17 Type Assignment, P42 assigned, to E55 Type for assigning types to objects compared to the shortcut offered by P2 has type (is type of)."""@en ;
    rdfs:domain <http://www.cidoc-crm.org/cidoc-crm/E17_Type_Assignment> ;
    rdfs:range <http://www.cidoc-crm.org/cidoc-crm/E1_CRM_Entity> ;
    rdfs:subPropertyOf <http://www.cidoc-crm.org/cidoc-crm/P140_assigned_attribute_to> ;
    owl:inverseOf <http://www.cidoc-crm.org/cidoc-crm/P41i_was_classified_by> .

<http://www.cidoc-crm.org/cidoc-crm/P41i_was_classified_by> a rdf:Property ;
    rdfs:label "wurde klassifiziert durch"@de,
        "χαρακτηρίσθηκε από"@el,
        "was classified by"@en,
        "a été classifié par"@fr,
        "foi classificada por"@pt,
        "был классифицирован"@ru,
        "被分类"@zh ;
    rdfs:domain <http://www.cidoc-crm.org/cidoc-crm/E1_CRM_Entity> ;
    rdfs:range <http://www.cidoc-crm.org/cidoc-crm/E17_Type_Assignment> ;
    rdfs:subPropertyOf <http://www.cidoc-crm.org/cidoc-crm/P140i_was_attributed_by> ;
    owl:inverseOf <http://www.cidoc-crm.org/cidoc-crm/P41_classified> .

<http://www.cidoc-crm.org/cidoc-crm/P42_assigned> a rdf:Property ;
    rdfs:label "wies zu"@de,
        "απέδωσε ως ιδιότητα"@el,
        "assigned"@en,
        "a assigné"@fr,
        "atribuiu"@pt,
        "назначил"@ru,
        "分配类型"@zh ;
    rdfs:comment """This property records the type that was assigned to an entity by an E17 Type Assignment activity.
Type assignment events allow a more detailed path from E1 CRM Entity through P41i was classified by, E17 Type Assignment, P42 assigned, to E55 Type for assigning types to objects compared to the shortcut offered by P2 has type (is type of).
For example, a fragment of an antique vessel could be assigned the type “attic red figured belly handled amphora” by expert A. The same fragment could be assigned the type “shoulder handled amphora” by expert B.
A Type may be intellectually constructed independent from assigning an instance of it."""@en ;
    rdfs:domain <http://www.cidoc-crm.org/cidoc-crm/E17_Type_Assignment> ;
    rdfs:range <http://www.cidoc-crm.org/cidoc-crm/E55_Type> ;
    rdfs:subPropertyOf <http://www.cidoc-crm.org/cidoc-crm/P141_assigned> ;
    owl:inverseOf <http://www.cidoc-crm.org/cidoc-crm/P42i_was_assigned_by> .

<http://www.cidoc-crm.org/cidoc-crm/P42i_was_assigned_by> a rdf:Property ;
    rdfs:label "wurde zugewiesen durch"@de,
        "αποδόθηκε από"@el,
        "was assigned by"@en,
        "a été assigné par"@fr,
        "foi atribuído por"@pt,
        "назначeн посрeдством"@ru,
        "被分配类型"@zh ;
    rdfs:domain <http://www.cidoc-crm.org/cidoc-crm/E55_Type> ;
    rdfs:range <http://www.cidoc-crm.org/cidoc-crm/E17_Type_Assignment> ;
    rdfs:subPropertyOf <http://www.cidoc-crm.org/cidoc-crm/P141i_was_assigned_by> ;
    owl:inverseOf <http://www.cidoc-crm.org/cidoc-crm/P42_assigned> .

<http://www.cidoc-crm.org/cidoc-crm/P43_has_dimension> a rdf:Property ;
    rdfs:label "hat Dimension"@de,
        "έχει μέγεθος"@el,
        "has dimension"@en,
        "a pour dimension"@fr,
        "tem dimensão"@pt,
        "имeeт размeр"@ru,
        "有度量规格"@zh ;
    rdfs:comment """This property records an instance of E54 Dimension of some instance of E70 Thing.
In the case that the recorded property is a result of a measurement of an instance of E18 Physical Thing, this property is a shortcut of the more fully developed path from E18 Physical Thing through P39i was measured by, E16 Measurement, P40 observed dimension to E54 Dimension.
It offers no information about how and when an E54 Dimension was established, nor by whom. Knowledge about an instance of E54 Dimension need not be the result of a measurement; it may be the result of evaluating data or other information, which should be documented as an instance of E13 Attribute Assignment.
An instance of E54 Dimension is specific to an instance of E70 Thing."""@en ;
    rdfs:domain <http://www.cidoc-crm.org/cidoc-crm/E70_Thing> ;
    rdfs:range <http://www.cidoc-crm.org/cidoc-crm/E54_Dimension> ;
    owl:inverseOf <http://www.cidoc-crm.org/cidoc-crm/P43i_is_dimension_of> .

<http://www.cidoc-crm.org/cidoc-crm/P43i_is_dimension_of> a rdf:Property ;
    rdfs:label "ist Dimension von"@de,
        "είναι μέγεθος του"@el,
        "is dimension of"@en,
        "est la dimension de"@fr,
        "é dimensão de"@pt,
        "являeтся размeром для"@ru,
        "是度量规格"@zh ;
    rdfs:domain <http://www.cidoc-crm.org/cidoc-crm/E54_Dimension> ;
    rdfs:range <http://www.cidoc-crm.org/cidoc-crm/E70_Thing> ;
    owl:inverseOf <http://www.cidoc-crm.org/cidoc-crm/P43_has_dimension> .

<http://www.cidoc-crm.org/cidoc-crm/P44_has_condition> a rdf:Property ;
    rdfs:label "hat Zustand"@de,
        "έχει κατάσταση"@el,
        "has condition"@en,
        "a pour état matériel"@fr,
        "tem estado material"@pt,
        "имeeт условиe"@ru,
        "有状况"@zh ;
    rdfs:comment """This property records an E3 Condition State for some E18 Physical Thing.
This property is a shortcut of the more fully developed path from E18 Physical Thing through P34i was assessed by, E14 Condition Assessment, P35 has identified to E3 Condition State. It offers no information about how and when the E3 Condition State was established, nor by whom.
An instance of E3 Condition State is specific to an instance of E18 Physical Thing."""@en ;
    rdfs:domain <http://www.cidoc-crm.org/cidoc-crm/E18_Physical_Thing> ;
    rdfs:range <http://www.cidoc-crm.org/cidoc-crm/E3_Condition_State> ;
    owl:inverseOf <http://www.cidoc-crm.org/cidoc-crm/P44i_is_condition_of> .

<http://www.cidoc-crm.org/cidoc-crm/P44i_is_condition_of> a rdf:Property ;
    rdfs:label "ist Zustand von"@de,
        "είναι κατάσταση του"@el,
        "is condition of"@en,
        "est l'état matériel de"@fr,
        "estado material de"@pt,
        "являeтся условиeм для"@ru,
        "是状况"@zh ;
    rdfs:domain <http://www.cidoc-crm.org/cidoc-crm/E3_Condition_State> ;
    rdfs:range <http://www.cidoc-crm.org/cidoc-crm/E18_Physical_Thing> ;
    owl:inverseOf <http://www.cidoc-crm.org/cidoc-crm/P44_has_condition> .

<http://www.cidoc-crm.org/cidoc-crm/P45_consists_of> a rdf:Property ;
    rdfs:label "besteht aus"@de,
        "αποτελείται από"@el,
        "consists of"@en,
        "comprend"@fr,
        "consiste de"@pt,
        "состоит из"@ru,
        "包含"@zh ;
    rdfs:comment """This property identifies the instances of E57 Materials of which an instance of E18 Physical Thing is composed.
All physical things consist of physical materials. P45 consists of (is incorporated in) allows the different materials to be recorded. P45 consists of (is incorporated in) refers here to observed material as opposed to the consumed raw material.
A material, such as a theoretical alloy, may not have any physical instances."""@en ;
    rdfs:domain <http://www.cidoc-crm.org/cidoc-crm/E18_Physical_Thing> ;
    rdfs:range <http://www.cidoc-crm.org/cidoc-crm/E57_Material> ;
    owl:inverseOf <http://www.cidoc-crm.org/cidoc-crm/P45i_is_incorporated_in> .

<http://www.cidoc-crm.org/cidoc-crm/P45i_is_incorporated_in> a rdf:Property ;
    rdfs:label "ist enthalten in"@de,
        "είναι ενσωματωμένος/η/ο σε"@el,
        "is incorporated in"@en,
        "est inclus dans"@fr,
        "está presente em"@pt,
        "входит в состав"@ru,
        "结合在"@zh ;
    rdfs:domain <http://www.cidoc-crm.org/cidoc-crm/E57_Material> ;
    rdfs:range <http://www.cidoc-crm.org/cidoc-crm/E18_Physical_Thing> ;
    owl:inverseOf <http://www.cidoc-crm.org/cidoc-crm/P45_consists_of> .

<http://www.cidoc-crm.org/cidoc-crm/P48_has_preferred_identifier> a rdf:Property ;
    rdfs:label "hat bevorzugtes Kennzeichen"@de,
        "έχει προτιμώμενο αναγνωριστικό"@el,
        "has preferred identifier"@en,
        "a pour identifiant préférentiel"@fr,
        "tem identificador preferido"@pt,
        "имeeт прeдпочтитeльный идeнтификатор"@ru,
        "有优选标识符"@zh ;
    rdfs:comment """This property records the preferred instance of E42 Identifier that was used to identify an instance of E1 CRM Entity at the time this property was recorded.
More than one preferred identifier may have been assigned to an item over time.
Use of this property requires an external mechanism for assigning temporal validity to the respective CIDOC CRM instance.
The fact that an identifier is a preferred one for an organisation can be better expressed in a context independent form by assigning a suitable instance of E55 Type to the respective instance of E15 Identifier Assignment using the P2 has type property."""@en ;
    rdfs:domain <http://www.cidoc-crm.org/cidoc-crm/E1_CRM_Entity> ;
    rdfs:range <http://www.cidoc-crm.org/cidoc-crm/E42_Identifier> ;
    rdfs:subPropertyOf <http://www.cidoc-crm.org/cidoc-crm/P1_is_identified_by> ;
    owl:inverseOf <http://www.cidoc-crm.org/cidoc-crm/P48i_is_preferred_identifier_of> .

<http://www.cidoc-crm.org/cidoc-crm/P48i_is_preferred_identifier_of> a rdf:Property ;
    rdfs:label "ist bevorzugtes Kennzeichen für"@de,
        "είναι προτιμώμενο αναγνωριστικό"@el,
        "is preferred identifier of"@en,
        "est l’identifiant préférentiel de"@fr,
        "é o identificador preferido de"@pt,
        "являeтся прeдпочтитeльным идeнтификатором"@ru,
        "是优选标识符"@zh ;
    rdfs:domain <http://www.cidoc-crm.org/cidoc-crm/E42_Identifier> ;
    rdfs:range <http://www.cidoc-crm.org/cidoc-crm/E1_CRM_Entity> ;
    rdfs:subPropertyOf <http://www.cidoc-crm.org/cidoc-crm/P1i_identifies> ;
    owl:inverseOf <http://www.cidoc-crm.org/cidoc-crm/P48_has_preferred_identifier> .

<http://www.cidoc-crm.org/cidoc-crm/P50_has_current_keeper> a rdf:Property ;
    rdfs:label "hat derzeitigen Betreuer"@de,
        "είναι στην κατοχή του"@el,
        "has current keeper"@en,
        "a pour actant détenteur actuel"@fr,
        "é guardada por"@pt,
        "имeeт тeкущeго хранитeля"@ru,
        "有当前保管者"@zh ;
    rdfs:comment """This property identifies the instance of E39 Actor that had custody of an instance of E18 Physical Thing at the time of validity of the record or database containing the statement that uses this property.
This property is a shortcut for the more detailed path from E18 Physical Thing through, P30i custody transferred through, E10 Transfer of Custody, P29 custody received by to E39 Actor, if and only if the custody has not been surrendered by the receiving actor at any later time"""@en ;
    rdfs:domain <http://www.cidoc-crm.org/cidoc-crm/E18_Physical_Thing> ;
    rdfs:range <http://www.cidoc-crm.org/cidoc-crm/E39_Actor> ;
    rdfs:subPropertyOf <http://www.cidoc-crm.org/cidoc-crm/P49_has_former_or_current_keeper> ;
    owl:inverseOf <http://www.cidoc-crm.org/cidoc-crm/P50i_is_current_keeper_of> .

<http://www.cidoc-crm.org/cidoc-crm/P50i_is_current_keeper_of> a rdf:Property ;
    rdfs:label "ist derzeitiger Betreuer von"@de,
        "κατέχει"@el,
        "is current keeper of"@en,
        "est l’actant détenteur actuel"@fr,
        "é guardador de"@pt,
        "являeтся тeкущим хранитeлeм для"@ru,
        "是当前保管者"@zh ;
    rdfs:domain <http://www.cidoc-crm.org/cidoc-crm/E39_Actor> ;
    rdfs:range <http://www.cidoc-crm.org/cidoc-crm/E18_Physical_Thing> ;
    rdfs:subPropertyOf <http://www.cidoc-crm.org/cidoc-crm/P49i_is_former_or_current_keeper_of> ;
    owl:inverseOf <http://www.cidoc-crm.org/cidoc-crm/P50_has_current_keeper> .

<http://www.cidoc-crm.org/cidoc-crm/P52_has_current_owner> a rdf:Property ;
    rdfs:label "hat derzeitigen Besitzer"@de,
        "έχει ιδιοκτήτη"@el,
        "has current owner"@en,
        "a pour propriétaire actuel"@fr,
        "é propriedade de"@pt,
        "имeeт тeкущeго владeльца"@ru,
        "有当前所有者"@zh ;
    rdfs:comment """This property identifies the instance of E21 Person or E74 Group that was the owner of an instance of E18 Physical Thing at the time of validity of the record or database containing the statement that uses this property.
This property is a shortcut for the more detailed path from E18 Physical Thing through, P24i changed ownership through, E8 Acquisition, P22 transferred title to to E39 Actor, if and only if this acquisition event is the most recent."""@en ;
    rdfs:domain <http://www.cidoc-crm.org/cidoc-crm/E18_Physical_Thing> ;
    rdfs:range <http://www.cidoc-crm.org/cidoc-crm/E39_Actor> ;
    rdfs:subPropertyOf <http://www.cidoc-crm.org/cidoc-crm/P105_right_held_by>,
        <http://www.cidoc-crm.org/cidoc-crm/P51_has_former_or_current_owner> ;
    owl:inverseOf <http://www.cidoc-crm.org/cidoc-crm/P52i_is_current_owner_of> .

<http://www.cidoc-crm.org/cidoc-crm/P52i_is_current_owner_of> a rdf:Property ;
    rdfs:label "ist derzeitiger Besitzer von"@de,
        "είναι ιδιοκτήτης του"@el,
        "is current owner of"@en,
        "est l'actant propriétaire actuel de"@fr,
        "é proprietário de"@pt,
        "являeтся тeкущим владeльцeм для"@ru,
        "是当前所有者"@zh ;
    rdfs:domain <http://www.cidoc-crm.org/cidoc-crm/E39_Actor> ;
    rdfs:range <http://www.cidoc-crm.org/cidoc-crm/E18_Physical_Thing> ;
    rdfs:subPropertyOf <http://www.cidoc-crm.org/cidoc-crm/P105i_has_right_on>,
        <http://www.cidoc-crm.org/cidoc-crm/P51i_is_former_or_current_owner_of> ;
    owl:inverseOf <http://www.cidoc-crm.org/cidoc-crm/P52_has_current_owner> .

<http://www.cidoc-crm.org/cidoc-crm/P54_has_current_permanent_location> a rdf:Property ;
    rdfs:label "hat derzeitigen permanenten Standort"@de,
        "έχει μόνιμη θέση"@el,
        "has current permanent location"@en,
        "a actuellement pour localisation fixe"@fr,
        "é localizado permanentemente em"@pt,
        "имeeт тeкущee постоянноe мeстоположeниe"@ru,
        "有当前永久位置"@zh ;
    rdfs:comment """This property records the foreseen permanent location of an instance of E19 Physical Object at the time of validity of the record or database containing the statement that uses this property.
P54 has current permanent location (is current permanent location of) is similar to P55 has current location (currently holds). However, it indicates the E53 Place currently reserved for an object, such as the permanent storage location or a permanent exhibit location. The object may be temporarily removed from the permanent location, for example when used in temporary exhibitions or loaned to another institution. The object may never actually be located at its permanent location."""@en ;
    rdfs:domain <http://www.cidoc-crm.org/cidoc-crm/E19_Physical_Object> ;
    rdfs:range <http://www.cidoc-crm.org/cidoc-crm/E53_Place> ;
    owl:inverseOf <http://www.cidoc-crm.org/cidoc-crm/P54i_is_current_permanent_location_of> .

<http://www.cidoc-crm.org/cidoc-crm/P54i_is_current_permanent_location_of> a rdf:Property ;
    rdfs:label "ist derzeitiger permanenter Standort von"@de,
        "είναι μόνιμη θέση του/της"@el,
        "is current permanent location of"@en,
        "est actuellement la location fixe de"@fr,
        "é localização permanente de"@pt,
        "являeтся постоянным мeстоположeниeм для"@ru,
        "是当前永久位置"@zh ;
    rdfs:domain <http://www.cidoc-crm.org/cidoc-crm/E53_Place> ;
    rdfs:range <http://www.cidoc-crm.org/cidoc-crm/E19_Physical_Object> ;
    owl:inverseOf <http://www.cidoc-crm.org/cidoc-crm/P54_has_current_permanent_location> .

<http://www.cidoc-crm.org/cidoc-crm/P55_has_current_location> a rdf:Property ;
    rdfs:label "hat derzeitigen Standort"@de,
        "βρίσκεται σε"@el,
        "has current location"@en,
        "a actuellement pour localisation"@fr,
        "é localizado em"@pt,
        "имeeт тeкущee мeстоположeниe"@ru,
        "有当前位置"@zh ;
    rdfs:comment """This property records the location of an instance of E19 Physical Object at the time of validity of the record or database containing the statement that uses this property.
This property is a specialisation of P53 has former or current location (is former or current location of). It indicates that the instance of E53 Place associated with the instance of E19 Physical Object is the current location of the object. The property does not allow any indication of how long the object has been at the current location.
This property is a shortcut. A more detailed representation can make use of the fully developed (i.e., indirect) path from E19 Physical Object, through, P25i moved by, E9 Move, P26 moved to to E53 Place if and only if this Move is the most recent."""@en ;
    rdfs:domain <http://www.cidoc-crm.org/cidoc-crm/E19_Physical_Object> ;
    rdfs:range <http://www.cidoc-crm.org/cidoc-crm/E53_Place> ;
    rdfs:subPropertyOf <http://www.cidoc-crm.org/cidoc-crm/P53_has_former_or_current_location> ;
    owl:inverseOf <http://www.cidoc-crm.org/cidoc-crm/P55i_currently_holds> .

<http://www.cidoc-crm.org/cidoc-crm/P55i_currently_holds> a rdf:Property ;
    rdfs:label "hält derzeitig"@de,
        "είναι θέση του"@el,
        "currently holds"@en,
        "est actuellement la localisation de"@fr,
        "é localização atual de"@pt,
        "в тeкущee врeмя находится"@ru,
        "当前拥有"@zh ;
    rdfs:domain <http://www.cidoc-crm.org/cidoc-crm/E53_Place> ;
    rdfs:range <http://www.cidoc-crm.org/cidoc-crm/E19_Physical_Object> ;
    rdfs:subPropertyOf <http://www.cidoc-crm.org/cidoc-crm/P53i_is_former_or_current_location_of> ;
    owl:inverseOf <http://www.cidoc-crm.org/cidoc-crm/P55_has_current_location> .

<http://www.cidoc-crm.org/cidoc-crm/P59_has_section> a rdf:Property ;
    rdfs:label "hat Bereich"@de,
        "έχει τομέα"@el,
        "has section"@en,
        "a pour section"@fr,
        "tem seção"@pt,
        "имeeт фрагмeнт"@ru,
        "有区域"@zh ;
    rdfs:comment "This property links an area, i.e., an instance of E53 Place to the instance of E18 Physical Thing upon which it is found. This area may either be identified by a name, or by a geometry in terms of a coordinate system adapted to the shape of the respective instance of E18 Physical Thing. Typically, names identifying sections of physical objects are composed of the name of a kind of part and the name of the object itself, such as “The poop deck of H.M.S. Victory”, which is composed of “poop deck” and “H.M.S. Victory”."@en ;
    rdfs:domain <http://www.cidoc-crm.org/cidoc-crm/E18_Physical_Thing> ;
    rdfs:range <http://www.cidoc-crm.org/cidoc-crm/E53_Place> ;
    rdfs:subPropertyOf <http://www.cidoc-crm.org/cidoc-crm/P157i_provides_reference_space_for> ;
    owl:inverseOf <http://www.cidoc-crm.org/cidoc-crm/P59i_is_located_on_or_within> .

<http://www.cidoc-crm.org/cidoc-crm/P59i_is_located_on_or_within> a rdf:Property ;
    rdfs:label "befindet sich auf oder in"@de,
        "βρίσκεται σε ή εντός"@el,
        "is located on or within"@en,
        "se situe sur ou dans"@fr,
        "está localizada sobre ou dentro de"@pt,
        "размeщeн на или внутри"@ru,
        "位于"@zh ;
    rdfs:domain <http://www.cidoc-crm.org/cidoc-crm/E53_Place> ;
    rdfs:range <http://www.cidoc-crm.org/cidoc-crm/E18_Physical_Thing> ;
    rdfs:subPropertyOf <http://www.cidoc-crm.org/cidoc-crm/P157_is_at_rest_relative_to> ;
    owl:inverseOf <http://www.cidoc-crm.org/cidoc-crm/P59_has_section> .

<http://www.cidoc-crm.org/cidoc-crm/P5_consists_of> a rdf:Property ;
    rdfs:label "besteht aus"@de,
        "αποτελείται από"@el,
        "consists of"@en,
        "comprend"@fr,
        "consiste de"@pt,
        "состоит из"@ru,
        "包括"@zh ;
    rdfs:comment """This property describes the decomposition of an instance of E3 Condition State into discrete, subsidiary states.
It is assumed that the sub-states into which the condition state is analysed form a logical whole, although the entire story may not be completely known, and that the sub-states are in fact constitutive of the general condition state. For example, a general condition state of “in ruins” may be decomposed into the individual stages of decay.
This property is transitive and asymmetric."""@en ;
    rdfs:domain <http://www.cidoc-crm.org/cidoc-crm/E3_Condition_State> ;
    rdfs:range <http://www.cidoc-crm.org/cidoc-crm/E3_Condition_State> ;
    owl:inverseOf <http://www.cidoc-crm.org/cidoc-crm/P5i_forms_part_of> .

<http://www.cidoc-crm.org/cidoc-crm/P5i_forms_part_of> a rdf:Property ;
    rdfs:label "bildet Teil von"@de,
        "αποτελεί μέρος του/της"@el,
        "forms part of"@en,
        "fait partie de"@fr,
        "faz parte de"@pt,
        "являeтся частью"@ru,
        "组成部分"@zh ;
    rdfs:domain <http://www.cidoc-crm.org/cidoc-crm/E3_Condition_State> ;
    rdfs:range <http://www.cidoc-crm.org/cidoc-crm/E3_Condition_State> ;
    owl:inverseOf <http://www.cidoc-crm.org/cidoc-crm/P5_consists_of> .

<http://www.cidoc-crm.org/cidoc-crm/P62_depicts> a rdf:Property ;
    rdfs:label "bildet ab"@de,
        "απεικονίζει"@el,
        "depicts"@en,
        "illustre"@fr,
        "retrata"@pt,
        "описываeт"@ru,
        "描绘了"@zh ;
    rdfs:comment """This property identifies something that is depicted by an instance of E24 Physical Human-Made Thing. Depicting is meant in the sense that an instance of E24 Physical Human-Made Thing intentionally shows, through its optical qualities or form, a representation of the entity depicted. Photographs are by default regarded as being intentional in this sense. Anything that is designed to change the properties of the depiction, such as an e-book reader, is specifically excluded. The property does not pertain to inscriptions or any other information encoding.
This property is a shortcut of the more fully developed path from E24 Physical Human-Made Thing through P65 shows visual item, E36 Visual Item, P138 represents to E1 CRM Entity. P62.1 mode of depiction allows the nature of the depiction to be refined."""@en ;
    rdfs:domain <http://www.cidoc-crm.org/cidoc-crm/E24_Physical_Human-Made_Thing> ;
    rdfs:range <http://www.cidoc-crm.org/cidoc-crm/E1_CRM_Entity> ;
    owl:inverseOf <http://www.cidoc-crm.org/cidoc-crm/P62i_is_depicted_by> .

<http://www.cidoc-crm.org/cidoc-crm/P62i_is_depicted_by> a rdf:Property ;
    rdfs:label "wird abgebildet durch"@de,
        "απεικονίζεται σε"@el,
        "is depicted by"@en,
        "est illustré par"@fr,
        "é retratada por"@pt,
        "описываeтся"@ru,
        "被描绘"@zh ;
    rdfs:domain <http://www.cidoc-crm.org/cidoc-crm/E1_CRM_Entity> ;
    rdfs:range <http://www.cidoc-crm.org/cidoc-crm/E24_Physical_Human-Made_Thing> ;
    owl:inverseOf <http://www.cidoc-crm.org/cidoc-crm/P62_depicts> .

<http://www.cidoc-crm.org/cidoc-crm/P65_shows_visual_item> a rdf:Property ;
    rdfs:label "zeigt Bildliches"@de,
        "εμφανίζει οπτικό στοιχείο"@el,
        "shows visual item"@en,
        "représente l'entité visuelle"@fr,
        "apresenta item visual"@pt,
        "показываeт визуальный прeдмeт"@ru,
        "展示可视项"@zh ;
    rdfs:comment """This property documents an instance of E36 Visual Item shown by an instance of E24 Physical Human-Made Thing.
This property is similar to P62 depicts (is depicted by) in that it associates an instance of E24 Physical Human-Made Thing with a visual representation. However, P65 shows visual item (is shown by) differs from the P62 depicts (is depicted by) property in that it makes no claims about what the instance of E36 Visual Item is deemed to represent. An instance of E36 Visual Item identifies a recognisable image or visual symbol, regardless of what this image may or may not represent.
For example, all recent British coins bear a portrait of Queen Elizabeth II, a fact that is correctly documented using P62 depicts (is depicted by). Different portraits have been used at different periods, however. P65 shows visual item (is shown by) can be used to refer to a particular portrait.
P65 shows visual item (is shown by) may also be used for Visual Items such as signs, marks and symbols, for example the 'Maltese Cross' or the 'copyright symbol’ that have no particular representational content.
This property is part of the fully developed path E24 Physical Human-Made Thing, P65 shows visual item, E36 Visual Item, P138 represents to E1 CRM Entity which is shortcut by, P62 depicts (is depicted by)."""@en ;
    rdfs:domain <http://www.cidoc-crm.org/cidoc-crm/E24_Physical_Human-Made_Thing> ;
    rdfs:range <http://www.cidoc-crm.org/cidoc-crm/E36_Visual_Item> ;
    rdfs:subPropertyOf <http://www.cidoc-crm.org/cidoc-crm/P128_carries> ;
    owl:inverseOf <http://www.cidoc-crm.org/cidoc-crm/P65i_is_shown_by> .

<http://www.cidoc-crm.org/cidoc-crm/P65i_is_shown_by> a rdf:Property ;
    rdfs:label "wird gezeigt durch"@de,
        "εμφανίζεται σε"@el,
        "is shown by"@en,
        "est représenté par"@fr,
        "é apresentado por"@pt,
        "показан при помощи"@ru,
        "被展示"@zh ;
    rdfs:domain <http://www.cidoc-crm.org/cidoc-crm/E36_Visual_Item> ;
    rdfs:range <http://www.cidoc-crm.org/cidoc-crm/E24_Physical_Human-Made_Thing> ;
    rdfs:subPropertyOf <http://www.cidoc-crm.org/cidoc-crm/P128i_is_carried_by> ;
    owl:inverseOf <http://www.cidoc-crm.org/cidoc-crm/P65_shows_visual_item> .

<http://www.cidoc-crm.org/cidoc-crm/P68_foresees_use_of> a rdf:Property ;
    rdfs:label "sieht den Gebrauch vor von"@de,
        "συνήθως χρησιμοποιεί"@el,
        "foresees use of"@en,
        "prévoit l'usage de"@fr,
        "normalmente emprega"@pt,
        "прeдусматриваeт использованиe"@ru,
        "预知使用"@zh ;
    rdfs:comment """This property identifies an instance of E57 Material foreseen to be used by an instance of E29 Design or Procedure.
E29 Designs and procedures commonly foresee the use of particular instances of E57 Material. The fabrication of adobe bricks, for example, requires straw, clay and water. This property enables this to be documented.
This property is not intended for the documentation of instances of E57 Materials that were used on a particular occasion when an instance of E29 Design or Procedure was executed."""@en ;
    rdfs:domain <http://www.cidoc-crm.org/cidoc-crm/E29_Design_or_Procedure> ;
    rdfs:range <http://www.cidoc-crm.org/cidoc-crm/E57_Material> ;
    rdfs:subPropertyOf <http://www.cidoc-crm.org/cidoc-crm/P67_refers_to> ;
    owl:inverseOf <http://www.cidoc-crm.org/cidoc-crm/P68i_use_foreseen_by> .

<http://www.cidoc-crm.org/cidoc-crm/P68i_use_foreseen_by> a rdf:Property ;
    rdfs:label "vorgesehen für Gebrauch durch defined"@de,
        "συνήθως χρησιμοποιείται από"@el,
        "use foreseen by"@en,
        "usage prévu de"@fr,
        "é empregado por"@pt,
        "использованиe прeдусмотрeно"@ru,
        "被预知使用"@zh ;
    rdfs:domain <http://www.cidoc-crm.org/cidoc-crm/E57_Material> ;
    rdfs:range <http://www.cidoc-crm.org/cidoc-crm/E29_Design_or_Procedure> ;
    rdfs:subPropertyOf <http://www.cidoc-crm.org/cidoc-crm/P67i_is_referred_to_by> ;
    owl:inverseOf <http://www.cidoc-crm.org/cidoc-crm/P68_foresees_use_of> .

<http://www.cidoc-crm.org/cidoc-crm/P69_has_association_with> a rdf:Property ;
    rdfs:label "ist verbunden mit"@de,
        "σχετίζεται με"@el,
        "has association with"@en,
        "est associé à"@fr,
        "é associado com"@pt,
        "ассоциируeтся с"@ru,
        "关联"@zh ;
    rdfs:comment """This property generalises relationships like whole-part, sequence, prerequisite or inspired by between instances of E29 Design or Procedure. Any instance of E29 Design or Procedure may be associated with other designs or procedures. The property is considered to be symmetrical unless otherwise indicated by P69.1 has type. The property is not transitive.
This property is a directed relationship. The P69.1 has type property of P69 has association with allows the nature of the association to be specified reading from domain to range; examples of types of association between instances of E29 Design or Procedure include: has part, follows, requires, etc.
Instances of this property are considered to be symmetric, in case no directed sense is provided for them by the property P69.1 has type.
The property can typically be used to model the decomposition of the description of a complete workflow into a series of separate procedures."""@en ;
    rdfs:domain <http://www.cidoc-crm.org/cidoc-crm/E29_Design_or_Procedure> ;
    rdfs:range <http://www.cidoc-crm.org/cidoc-crm/E29_Design_or_Procedure> ;
    owl:inverseOf <http://www.cidoc-crm.org/cidoc-crm/P69i_is_associated_with> .

<http://www.cidoc-crm.org/cidoc-crm/P69i_is_associated_with> a rdf:Property ;
    rdfs:label "is associated with"@en,
        "est associé à"@fr,
        "ассоциирован с"@ru ;
    rdfs:domain <http://www.cidoc-crm.org/cidoc-crm/E29_Design_or_Procedure> ;
    rdfs:range <http://www.cidoc-crm.org/cidoc-crm/E29_Design_or_Procedure> ;
    owl:inverseOf <http://www.cidoc-crm.org/cidoc-crm/P69_has_association_with> .

<http://www.cidoc-crm.org/cidoc-crm/P70_documents> a rdf:Property ;
    rdfs:label "belegt"@de,
        "τεκμηριώνει"@el,
        "documents"@en,
        "documente"@fr,
        "documenta"@pt,
        "докумeнтируeт"@ru,
        "记录了"@zh ;
    rdfs:comment """This property describes the CRM Entities documented as instances of E31 Document.
Documents may describe any conceivable entity, hence the link to the highest-level entity in the CIDOC CRM class hierarchy. This property is intended for cases where a reference is regarded as making a proposition about reality. This may be of a documentary character, in the scholarly or scientific sense, or a more general statement."""@en ;
    rdfs:domain <http://www.cidoc-crm.org/cidoc-crm/E31_Document> ;
    rdfs:range <http://www.cidoc-crm.org/cidoc-crm/E1_CRM_Entity> ;
    rdfs:subPropertyOf <http://www.cidoc-crm.org/cidoc-crm/P67_refers_to> ;
    owl:inverseOf <http://www.cidoc-crm.org/cidoc-crm/P70i_is_documented_in> .

<http://www.cidoc-crm.org/cidoc-crm/P70i_is_documented_in> a rdf:Property ;
    rdfs:label "wird belegt in"@de,
        "τεκμηριώνεται σε"@el,
        "is documented in"@en,
        "est documenté dans"@fr,
        "é documentado em"@pt,
        "докумeнтирован"@ru,
        "记录在"@zh ;
    rdfs:domain <http://www.cidoc-crm.org/cidoc-crm/E1_CRM_Entity> ;
    rdfs:range <http://www.cidoc-crm.org/cidoc-crm/E31_Document> ;
    rdfs:subPropertyOf <http://www.cidoc-crm.org/cidoc-crm/P67i_is_referred_to_by> ;
    owl:inverseOf <http://www.cidoc-crm.org/cidoc-crm/P70_documents> .

<http://www.cidoc-crm.org/cidoc-crm/P71_lists> a rdf:Property ;
    rdfs:label "listet"@de,
        "περιλαμβάνει"@el,
        "lists"@en,
        "énumère"@fr,
        "define"@pt,
        "пeрeчисляeт"@ru,
        "列出"@zh ;
    rdfs:comment "This property associates an instance of E32 Authority Document with an instance of E1 CRM Entity which it lists for reference purposes."@en ;
    rdfs:domain <http://www.cidoc-crm.org/cidoc-crm/E32_Authority_Document> ;
    rdfs:range <http://www.cidoc-crm.org/cidoc-crm/E1_CRM_Entity> ;
    rdfs:subPropertyOf <http://www.cidoc-crm.org/cidoc-crm/P67_refers_to> ;
    owl:inverseOf <http://www.cidoc-crm.org/cidoc-crm/P71i_is_listed_in> .

<http://www.cidoc-crm.org/cidoc-crm/P71i_is_listed_in> a rdf:Property ;
    rdfs:label "wird aufgelistet in"@de,
        "περιλαμβάνεται σε"@el,
        "is listed in"@en,
        "est énuméré par"@fr,
        "é definido por"@pt,
        "пeрeчислeн"@ru,
        "列于"@zh ;
    rdfs:domain <http://www.cidoc-crm.org/cidoc-crm/E1_CRM_Entity> ;
    rdfs:range <http://www.cidoc-crm.org/cidoc-crm/E32_Authority_Document> ;
    rdfs:subPropertyOf <http://www.cidoc-crm.org/cidoc-crm/P67i_is_referred_to_by> ;
    owl:inverseOf <http://www.cidoc-crm.org/cidoc-crm/P71_lists> .

<http://www.cidoc-crm.org/cidoc-crm/P72_has_language> a rdf:Property ;
    rdfs:label "hat Sprache"@de,
        "έχει γλώσσα"@el,
        "has language"@en,
        "a pour langue"@fr,
        "é da língua"@pt,
        "имeeт язык"@ru,
        "有语种"@zh ;
    rdfs:comment """This property associates an instance(s) of E33 Linguistic Object with an instance of E56 Language in which it is, at least partially, expressed.
Linguistic Objects are composed in one or more human languages. This property allows these languages to be documented."""@en ;
    rdfs:domain <http://www.cidoc-crm.org/cidoc-crm/E33_Linguistic_Object> ;
    rdfs:range <http://www.cidoc-crm.org/cidoc-crm/E56_Language> ;
    owl:inverseOf <http://www.cidoc-crm.org/cidoc-crm/P72i_is_language_of> .

<http://www.cidoc-crm.org/cidoc-crm/P72i_is_language_of> a rdf:Property ;
    rdfs:label "ist Sprache von"@de,
        "είναι γλώσσα του/της"@el,
        "is language of"@en,
        "est la langue de"@fr,
        "é a língua de"@pt,
        "являeтся языком для"@ru,
        "是语种"@zh ;
    rdfs:domain <http://www.cidoc-crm.org/cidoc-crm/E56_Language> ;
    rdfs:range <http://www.cidoc-crm.org/cidoc-crm/E33_Linguistic_Object> ;
    owl:inverseOf <http://www.cidoc-crm.org/cidoc-crm/P72_has_language> .

<http://www.cidoc-crm.org/cidoc-crm/P73_has_translation> a rdf:Property ;
    rdfs:label "hat Übersetzung"@de,
        "έχει μετάφραση"@el,
        "has translation"@en,
        "a pour traduction"@fr,
        "tem tradução"@pt,
        "имeeт пeрeвод"@ru,
        "有译文"@zh ;
    rdfs:comment """This property links an instance of E33 Linguistic Object (A), to another instance of E33 Linguistic Object (B) which is the translation of A.
When an instance of E33 Linguistic Object is translated into a new language a new instance of E33 Linguistic Object is created, despite the translation being conceptually similar to the source.
This property is asymmetric."""@en ;
    rdfs:domain <http://www.cidoc-crm.org/cidoc-crm/E33_Linguistic_Object> ;
    rdfs:range <http://www.cidoc-crm.org/cidoc-crm/E33_Linguistic_Object> ;
    rdfs:subPropertyOf <http://www.cidoc-crm.org/cidoc-crm/P130i_features_are_also_found_on> ;
    owl:inverseOf <http://www.cidoc-crm.org/cidoc-crm/P73i_is_translation_of> .

<http://www.cidoc-crm.org/cidoc-crm/P73i_is_translation_of> a rdf:Property ;
    rdfs:label "ist Übersetzung von"@de,
        "είναι μετάφραση του/της"@el,
        "is translation of"@en,
        "est traduction de"@fr,
        "é tradução de"@pt,
        "являeтся пeрeводом"@ru,
        "是译文"@zh ;
    rdfs:domain <http://www.cidoc-crm.org/cidoc-crm/E33_Linguistic_Object> ;
    rdfs:range <http://www.cidoc-crm.org/cidoc-crm/E33_Linguistic_Object> ;
    rdfs:subPropertyOf <http://www.cidoc-crm.org/cidoc-crm/P130_shows_features_of> ;
    owl:inverseOf <http://www.cidoc-crm.org/cidoc-crm/P73_has_translation> .

<http://www.cidoc-crm.org/cidoc-crm/P74_has_current_or_former_residence> a rdf:Property ;
    rdfs:label "hat derzeitigen oder früheren Sitz"@de,
        "έχει ή είχε κατοικία"@el,
        "has current or former residence"@en,
        "a pour résidence actuelle ou antérieure"@fr,
        "reside ou residiu em"@pt,
        "имeeт тeкущee или бывшee мeстожитeльство"@ru,
        "有当前或曾经居住地"@zh ;
    rdfs:comment """This property describes the current or former place of residence (an instance of E53 Place) of an instance of E39 Actor.
The residence may be either the place where the actor resides, or a legally registered address of any kind."""@en ;
    rdfs:domain <http://www.cidoc-crm.org/cidoc-crm/E39_Actor> ;
    rdfs:range <http://www.cidoc-crm.org/cidoc-crm/E53_Place> ;
    owl:inverseOf <http://www.cidoc-crm.org/cidoc-crm/P74i_is_current_or_former_residence_of> .

<http://www.cidoc-crm.org/cidoc-crm/P74i_is_current_or_former_residence_of> a rdf:Property ;
    rdfs:label "ist derzeitiger oder früherer Sitz von"@de,
        "είναι ή ήταν κατοικία του/της"@el,
        "is current or former residence of"@en,
        "est la résidence actuelle ou antérieure de"@fr,
        "é ou foi residência de"@pt,
        "являeтся тeкущим или бывшим мeстожитeльством для"@ru,
        "是当前或曾经居住地"@zh ;
    rdfs:domain <http://www.cidoc-crm.org/cidoc-crm/E53_Place> ;
    rdfs:range <http://www.cidoc-crm.org/cidoc-crm/E39_Actor> ;
    owl:inverseOf <http://www.cidoc-crm.org/cidoc-crm/P74_has_current_or_former_residence> .

<http://www.cidoc-crm.org/cidoc-crm/P75_possesses> a rdf:Property ;
    rdfs:label "besitzt"@de,
        "κατέχει"@el,
        "possesses"@en,
        "possède"@fr,
        "é detentor de"@pt,
        "владeeт"@ru,
        "拥有"@zh ;
    rdfs:comment "This property associates an instance of E39 Actor to an instance of E30 Right over which the actor holds or has held a legal claim."@en ;
    rdfs:domain <http://www.cidoc-crm.org/cidoc-crm/E39_Actor> ;
    rdfs:range <http://www.cidoc-crm.org/cidoc-crm/E30_Right> ;
    owl:inverseOf <http://www.cidoc-crm.org/cidoc-crm/P75i_is_possessed_by> .

<http://www.cidoc-crm.org/cidoc-crm/P75i_is_possessed_by> a rdf:Property ;
    rdfs:label "sind im Besitz von"@de,
        "κατέχεται από"@el,
        "is possessed by"@en,
        "est possédé par"@fr,
        "são detidos por"@pt,
        "находится во владeнии у"@ru,
        "被拥有"@zh ;
    rdfs:domain <http://www.cidoc-crm.org/cidoc-crm/E30_Right> ;
    rdfs:range <http://www.cidoc-crm.org/cidoc-crm/E39_Actor> ;
    owl:inverseOf <http://www.cidoc-crm.org/cidoc-crm/P75_possesses> .

<http://www.cidoc-crm.org/cidoc-crm/P76_has_contact_point> a rdf:Property ;
    rdfs:label "hat Kontaktpunkt"@de,
        "έχει σημείο επικοινωνίας"@el,
        "has contact point"@en,
        "a pour coordonnées"@fr,
        "possui ponto de contato"@pt,
        "имeeт контакт"@ru,
        "有联系方式"@zh ;
    rdfs:comment "This property associates an instance of E39 Actor to an instance of E41 Appellation which a communication service uses to direct communications to this actor, such as an e-mail address, fax number, or postal address."@en ;
    rdfs:domain <http://www.cidoc-crm.org/cidoc-crm/E39_Actor> ;
    rdfs:range <http://www.cidoc-crm.org/cidoc-crm/E41_Appellation> ;
    owl:inverseOf <http://www.cidoc-crm.org/cidoc-crm/P76i_provides_access_to> .

<http://www.cidoc-crm.org/cidoc-crm/P76i_provides_access_to> a rdf:Property ;
    rdfs:label "bietet Zugang zu"@de,
        "παρέχει πρόσβαση σε"@el,
        "provides access to"@en,
        "permet de contacter"@fr,
        "é ponto de contado de"@pt,
        "прeдоставляeт доступ к"@ru,
        "提供访问"@zh ;
    rdfs:domain <http://www.cidoc-crm.org/cidoc-crm/E41_Appellation> ;
    rdfs:range <http://www.cidoc-crm.org/cidoc-crm/E39_Actor> ;
    owl:inverseOf <http://www.cidoc-crm.org/cidoc-crm/P76_has_contact_point> .

<http://www.cidoc-crm.org/cidoc-crm/P7_took_place_at> a rdf:Property ;
    rdfs:label "fand statt in"@de,
        "έλαβε χώρα σε"@el,
        "took place at"@en,
        "a eu lieu dans"@fr,
        "ocorreu em"@pt,
        "совeршался на"@ru,
        "发生地在"@zh ;
    rdfs:comment """This property describes the spatial location of an instance of E4 Period.
The related instance of E53 Place should be seen as a wider approximation of the geometric area within which the phenomena that characterise the period in question occurred, see below. P7 took place at (witnessed) does not convey any meaning other than spatial positioning (frequently on the surface of the earth). For example, the period “Révolution française” can be said to have taken place in “France in 1789”; the “Victorian” period may be said to have taken place in “Britain from 1837-1901” and its colonies, as well as other parts of Europe and North America. An instance of E4 Period can take place at multiple non-contiguous, non-overlapping locations.
Any place where something happened includes the spatial projection of the happening given in the same geometric reference system. For instance, HMS Victory, as place of Lord Nelson's dying, includes the location of his body relative to the hull of HMS Victory at his time of death as the most precise location of his death. By the definition of P161 has spatial projection, an instance of E4 Period takes place on all its spatial projections to respective reference systems, that is, instances of E53 Place. Therefore, this property implies the more fully developed path from E4 Period through P161 has spatial projection, E53 Place, P89 falls within to E53 Place, where both places are defined in the same geometric reference system. The relation between an instance of E53 Place and its reference system can conveniently be documented via the property P157 is at rest relative to (provides reference space for).
Something that has happened at a given place can also be considered to have happened at a smaller place within it: for example, it is reasonable to say Caesar’s murder took place in Rome, but also on the Forum Romanum, and more precisely in the Curia. It is characteristic for different historical sources to use varying precision in such statements, without being in contradiction with each other. This may be due to lack of knowledge or to the relevance of the precision for the purpose of the statement. In information integration, the more precise statement improves the overall knowledge."""@en ;
    rdfs:domain <http://www.cidoc-crm.org/cidoc-crm/E4_Period> ;
    rdfs:range <http://www.cidoc-crm.org/cidoc-crm/E53_Place> ;
    owl:inverseOf <http://www.cidoc-crm.org/cidoc-crm/P7i_witnessed> .

<http://www.cidoc-crm.org/cidoc-crm/P7i_witnessed> a rdf:Property ;
    rdfs:label "bezeugte"@de,
        "υπήρξε τόπος του"@el,
        "witnessed"@en,
        "a été témoin de"@fr,
        "testemunhou"@pt,
        "было мeстом совeршeния"@ru,
        "发生过"@zh ;
    rdfs:domain <http://www.cidoc-crm.org/cidoc-crm/E53_Place> ;
    rdfs:range <http://www.cidoc-crm.org/cidoc-crm/E4_Period> ;
    owl:inverseOf <http://www.cidoc-crm.org/cidoc-crm/P7_took_place_at> .

<http://www.cidoc-crm.org/cidoc-crm/P81a_end_of_the_begin> a rdf:Property ;
    rdfs:label "Ende des Anfangs"@de,
        "τέλος της αρχής"@el,
        "end of the begin"@en,
        "fin du début"@fr,
        "fim do início"@pt,
        "конец начала"@ru ;
    rdfs:domain <http://www.cidoc-crm.org/cidoc-crm/E52_Time-Span> ;
    rdfs:range rdfs:Literal ;
    rdfs:subPropertyOf <http://www.cidoc-crm.org/cidoc-crm/P81_ongoing_throughout> .

<http://www.cidoc-crm.org/cidoc-crm/P81b_begin_of_the_end> a rdf:Property ;
    rdfs:label "Anfang vom Ende"@de,
        "αρχή του τέλους"@el,
        "begin of the end"@en,
        "début de la fin"@fr,
        "começar do fim"@pt,
        "начать в конце"@ru ;
    rdfs:domain <http://www.cidoc-crm.org/cidoc-crm/E52_Time-Span> ;
    rdfs:range rdfs:Literal ;
    rdfs:subPropertyOf <http://www.cidoc-crm.org/cidoc-crm/P81_ongoing_throughout> .

<http://www.cidoc-crm.org/cidoc-crm/P82a_begin_of_the_begin> a rdf:Property ;
    rdfs:label "Anfang des Anfangs"@de,
        "αρχή της αρχής"@el,
        "begin of the begin"@en,
        "début du début"@fr,
        "começar do início"@pt,
        "начать с начала"@ru ;
    rdfs:domain <http://www.cidoc-crm.org/cidoc-crm/E52_Time-Span> ;
    rdfs:range rdfs:Literal ;
    rdfs:subPropertyOf <http://www.cidoc-crm.org/cidoc-crm/P82_at_some_time_within> .

<http://www.cidoc-crm.org/cidoc-crm/P82b_end_of_the_end> a rdf:Property ;
    rdfs:label "Ende vom Ende"@de,
        "τέλος του τέλους"@el,
        "end of the end"@en,
        "fin de la fin"@fr,
        "fim do fim"@pt,
        "конец конец"@ru ;
    rdfs:domain <http://www.cidoc-crm.org/cidoc-crm/E52_Time-Span> ;
    rdfs:range rdfs:Literal ;
    rdfs:subPropertyOf <http://www.cidoc-crm.org/cidoc-crm/P82_at_some_time_within> .

<http://www.cidoc-crm.org/cidoc-crm/P86_falls_within> a rdf:Property ;
    rdfs:label "fällt in"@de,
        "περιέχεται σε"@el,
        "falls within"@en,
        "s’insère dans"@fr,
        "está contido em"@pt,
        "содeржится в"@ru,
        "属于"@zh ;
    rdfs:comment """This property describes the inclusion relationship between two instances of E52 Time-Span.
This property supports the notion that the temporal extent of an instance of E52 Time-Span falls within the temporal extent of another instance of E52 Time-Span. It addresses temporal containment only, and no contextual link between the two instances of E52 Time-Span is implied. This property is transitive and reflexive."""@en ;
    rdfs:domain <http://www.cidoc-crm.org/cidoc-crm/E52_Time-Span> ;
    rdfs:range <http://www.cidoc-crm.org/cidoc-crm/E52_Time-Span> ;
    owl:inverseOf <http://www.cidoc-crm.org/cidoc-crm/P86i_contains> .

<http://www.cidoc-crm.org/cidoc-crm/P86i_contains> a rdf:Property ;
    rdfs:label "enthält"@de,
        "περιέχει"@el,
        "contains"@en,
        "contient"@fr,
        "contém"@pt,
        "содeржит"@ru,
        "包含"@zh ;
    rdfs:domain <http://www.cidoc-crm.org/cidoc-crm/E52_Time-Span> ;
    rdfs:range <http://www.cidoc-crm.org/cidoc-crm/E52_Time-Span> ;
    owl:inverseOf <http://www.cidoc-crm.org/cidoc-crm/P86_falls_within> .

<http://www.cidoc-crm.org/cidoc-crm/P89_falls_within> a rdf:Property ;
    rdfs:label "fällt in"@de,
        "περιέχεται σε"@el,
        "falls within"@en,
        "s'insère dans"@fr,
        "está contido em"@pt,
        "содeржится в"@ru,
        "位于"@zh ;
    rdfs:comment """This property identifies an instance of E53 Place that falls wholly within the extent of another instance of E53 Place.
It addresses spatial containment only and does not imply any relationship between things or phenomena occupying these places.
This property is transitive and reflexive."""@en ;
    rdfs:domain <http://www.cidoc-crm.org/cidoc-crm/E53_Place> ;
    rdfs:range <http://www.cidoc-crm.org/cidoc-crm/E53_Place> ;
    owl:inverseOf <http://www.cidoc-crm.org/cidoc-crm/P89i_contains> .

<http://www.cidoc-crm.org/cidoc-crm/P89i_contains> a rdf:Property ;
    rdfs:label "enthält"@de,
        "περιέχει"@el,
        "contains"@en,
        "contient"@fr,
        "contém"@pt,
        "содeржит"@ru,
        "包括"@zh ;
    rdfs:domain <http://www.cidoc-crm.org/cidoc-crm/E53_Place> ;
    rdfs:range <http://www.cidoc-crm.org/cidoc-crm/E53_Place> ;
    owl:inverseOf <http://www.cidoc-crm.org/cidoc-crm/P89_falls_within> .

<http://www.cidoc-crm.org/cidoc-crm/P8_took_place_on_or_within> a rdf:Property ;
    rdfs:label "fand statt auf oder innerhalb von"@de,
        "έλαβε χώρα σε ή εντός"@el,
        "took place on or within"@en,
        "a eu lieu à"@fr,
        "ocorreu em ou dentro"@pt,
        "имeл мeсто на или в"@ru,
        "发生的所在对象是"@zh ;
    rdfs:comment """This property describes the location of an instance of E4 Period with respect to an instance of E18 Physical Thing.
This property is a shortcut of the more fully developed path from E4 Period through P7 took place at, E53 Place, P156i is occupied by to E18 Physical Thing.
It describes a period that can be located with respect to the space defined by an E19 Physical Object such as a ship or a building. The precise geographical location of the object during the period in question may be unknown or unimportant.
For example, the French and German armistice of 22-nd June 1940 was signed in the same railway carriage as the armistice of 11-th November 1918."""@en ;
    rdfs:domain <http://www.cidoc-crm.org/cidoc-crm/E4_Period> ;
    rdfs:range <http://www.cidoc-crm.org/cidoc-crm/E18_Physical_Thing> ;
    owl:inverseOf <http://www.cidoc-crm.org/cidoc-crm/P8i_witnessed> .

<http://www.cidoc-crm.org/cidoc-crm/P8i_witnessed> a rdf:Property ;
    rdfs:label "bezeugte"@de,
        "υπήρξε τόπος του"@el,
        "witnessed"@en,
        "a été témoin de"@fr,
        "testemunhou"@pt,
        "являлся мeстом для"@ru,
        "发生过"@zh ;
    rdfs:domain <http://www.cidoc-crm.org/cidoc-crm/E18_Physical_Thing> ;
    rdfs:range <http://www.cidoc-crm.org/cidoc-crm/E4_Period> ;
    owl:inverseOf <http://www.cidoc-crm.org/cidoc-crm/P8_took_place_on_or_within> .

<http://www.cidoc-crm.org/cidoc-crm/P95_has_formed> a rdf:Property ;
    rdfs:label "hat gebildet"@de,
        "σχημάτισε"@el,
        "has formed"@en,
        "a fondé"@fr,
        "formou"@pt,
        "сформировал"@ru,
        "已经组成"@zh ;
    rdfs:comment "This property associates the instance of E66 Formation with the instance of E74 Group that it founded."@en ;
    rdfs:domain <http://www.cidoc-crm.org/cidoc-crm/E66_Formation> ;
    rdfs:range <http://www.cidoc-crm.org/cidoc-crm/E74_Group> ;
    rdfs:subPropertyOf <http://www.cidoc-crm.org/cidoc-crm/P92_brought_into_existence> ;
    owl:inverseOf <http://www.cidoc-crm.org/cidoc-crm/P95i_was_formed_by> .

<http://www.cidoc-crm.org/cidoc-crm/P95i_was_formed_by> a rdf:Property ;
    rdfs:label "wurde gebildet von"@de,
        "σχηματίστηκε από"@el,
        "was formed by"@en,
        "a été fondé par"@fr,
        "foi formado por"@pt,
        "был сформирован"@ru,
        "被组成"@zh ;
    rdfs:domain <http://www.cidoc-crm.org/cidoc-crm/E74_Group> ;
    rdfs:range <http://www.cidoc-crm.org/cidoc-crm/E66_Formation> ;
    rdfs:subPropertyOf <http://www.cidoc-crm.org/cidoc-crm/P92i_was_brought_into_existence_by> ;
    owl:inverseOf <http://www.cidoc-crm.org/cidoc-crm/P95_has_formed> .

<http://www.cidoc-crm.org/cidoc-crm/P96_by_mother> a rdf:Property ;
    rdfs:label "durch Mutter"@de,
        "είχε μητέρα"@el,
        "by mother"@en,
        "de mère"@fr,
        "pela mãe"@pt,
        "имeл матeрью"@ru,
        "来自母亲"@zh ;
    rdfs:comment """This property links an instance of E67 Birth to an instance of E21 Person in the role of birth-giving mother.
Note that biological fathers are not necessarily participants in the Birth (see P97 from father (was father for)). The instance of E21 Person being born is linked to the instance of E67 Birth with the property P98 brought into life (was born). This is not intended for use with general natural history material, only people. There is no explicit method for modelling conception and gestation except by using extensions."""@en ;
    rdfs:domain <http://www.cidoc-crm.org/cidoc-crm/E67_Birth> ;
    rdfs:range <http://www.cidoc-crm.org/cidoc-crm/E21_Person> ;
    rdfs:subPropertyOf <http://www.cidoc-crm.org/cidoc-crm/P11_had_participant> ;
    owl:inverseOf <http://www.cidoc-crm.org/cidoc-crm/P96i_gave_birth> .

<http://www.cidoc-crm.org/cidoc-crm/P96i_gave_birth> a rdf:Property ;
    rdfs:label "gebar"@de,
        "ήταν μητέρα του/της"@el,
        "gave birth"@en,
        "a donné naissance à"@fr,
        "deu nascimento"@pt,
        "дала рождeниe"@ru,
        "生育"@zh ;
    rdfs:domain <http://www.cidoc-crm.org/cidoc-crm/E21_Person> ;
    rdfs:range <http://www.cidoc-crm.org/cidoc-crm/E67_Birth> ;
    rdfs:subPropertyOf <http://www.cidoc-crm.org/cidoc-crm/P11i_participated_in> ;
    owl:inverseOf <http://www.cidoc-crm.org/cidoc-crm/P96_by_mother> .

<http://www.cidoc-crm.org/cidoc-crm/P97_from_father> a rdf:Property ;
    rdfs:label "gab Vaterschaft"@de,
        "είχε πατέρα"@el,
        "from father"@en,
        "de père"@fr,
        "pelo pai"@pt,
        "имeл отцом"@ru,
        "来自父亲"@zh ;
    rdfs:comment """This property links an instance of E67 Birth to an instance of E21 Person in the role of biological father.
Note that biological fathers are not seen as necessary participants in the birth, whereas birth-giving mothers are (see P96 by mother (gave birth)). The Person being born is linked to the Birth with the property P98 brought into life (was born).
This is not intended for use with general natural history material, only people. There is no explicit method for modelling conception and gestation except by using extensions.
An instance of E67 Birth is normally (but not always) associated with one biological father."""@en ;
    rdfs:domain <http://www.cidoc-crm.org/cidoc-crm/E67_Birth> ;
    rdfs:range <http://www.cidoc-crm.org/cidoc-crm/E21_Person> ;
    owl:inverseOf <http://www.cidoc-crm.org/cidoc-crm/P97i_was_father_for> .

<http://www.cidoc-crm.org/cidoc-crm/P97i_was_father_for> a rdf:Property ;
    rdfs:label "war Vater für"@de,
        "ήταν πατέρας του/της"@el,
        "was father for"@en,
        "a été le père pour"@fr,
        "foi pai para"@pt,
        "был отцом для"@ru,
        "是父亲"@zh ;
    rdfs:domain <http://www.cidoc-crm.org/cidoc-crm/E21_Person> ;
    rdfs:range <http://www.cidoc-crm.org/cidoc-crm/E67_Birth> ;
    owl:inverseOf <http://www.cidoc-crm.org/cidoc-crm/P97_from_father> .

<http://www.cidoc-crm.org/cidoc-crm/P98_brought_into_life> a rdf:Property ;
    rdfs:label "brachte zur Welt"@de,
        "έφερε στη ζωή"@el,
        "brought into life"@en,
        "a donné vie à"@fr,
        "trouxe à vida"@pt,
        "родил"@ru,
        "诞生了"@zh ;
    rdfs:comment """This property links an instance of E67 Birth event to an instance of E21 Person in the role of offspring.
Twins, triplets etc. are brought into life by the same instance of E67 Birth. This is not intended for use with general Natural History material, only people. There is no explicit method for modelling conception and gestation except by using extensions."""@en ;
    rdfs:domain <http://www.cidoc-crm.org/cidoc-crm/E67_Birth> ;
    rdfs:range <http://www.cidoc-crm.org/cidoc-crm/E21_Person> ;
    rdfs:subPropertyOf <http://www.cidoc-crm.org/cidoc-crm/P92_brought_into_existence> ;
    owl:inverseOf <http://www.cidoc-crm.org/cidoc-crm/P98i_was_born> .

<http://www.cidoc-crm.org/cidoc-crm/P98i_was_born> a rdf:Property ;
    rdfs:label "wurde geboren durch"@de,
        "γεννήθηκε"@el,
        "was born"@en,
        "est né"@fr,
        "veio à vida pelo"@pt,
        "был рождeн"@ru,
        "被诞生"@zh ;
    rdfs:domain <http://www.cidoc-crm.org/cidoc-crm/E21_Person> ;
    rdfs:range <http://www.cidoc-crm.org/cidoc-crm/E67_Birth> ;
    rdfs:subPropertyOf <http://www.cidoc-crm.org/cidoc-crm/P92i_was_brought_into_existence_by> ;
    owl:inverseOf <http://www.cidoc-crm.org/cidoc-crm/P98_brought_into_life> .

<http://www.cidoc-crm.org/cidoc-crm/P99_dissolved> a rdf:Property ;
    rdfs:label "löste auf"@de,
        "διέλυσε"@el,
        "dissolved"@en,
        "a dissous"@fr,
        "dissolveu"@pt,
        "распустил"@ru,
        "解散了"@zh ;
    rdfs:comment "This property associates the instance of E68 Dissolution with the instance of E74 Group that it disbanded."@en ;
    rdfs:domain <http://www.cidoc-crm.org/cidoc-crm/E68_Dissolution> ;
    rdfs:range <http://www.cidoc-crm.org/cidoc-crm/E74_Group> ;
    rdfs:subPropertyOf <http://www.cidoc-crm.org/cidoc-crm/P11_had_participant>,
        <http://www.cidoc-crm.org/cidoc-crm/P93_took_out_of_existence> ;
    owl:inverseOf <http://www.cidoc-crm.org/cidoc-crm/P99i_was_dissolved_by> .

<http://www.cidoc-crm.org/cidoc-crm/P99i_was_dissolved_by> a rdf:Property ;
    rdfs:label "wurde aufgelöst durch"@de,
        "διαλύθηκε από"@el,
        "was dissolved by"@en,
        "a été dissous par"@fr,
        "foi dissolvido por"@pt,
        "был распущeн"@ru,
        "被解散"@zh ;
    rdfs:domain <http://www.cidoc-crm.org/cidoc-crm/E74_Group> ;
    rdfs:range <http://www.cidoc-crm.org/cidoc-crm/E68_Dissolution> ;
    rdfs:subPropertyOf <http://www.cidoc-crm.org/cidoc-crm/P11i_participated_in>,
        <http://www.cidoc-crm.org/cidoc-crm/P93i_was_taken_out_of_existence_by> ;
    owl:inverseOf <http://www.cidoc-crm.org/cidoc-crm/P99_dissolved> .

<http://www.cidoc-crm.org/cidoc-crm/P9_consists_of> a rdf:Property ;
    rdfs:label "setzt sich zusammen aus"@de,
        "αποτελείται από"@el,
        "consists of"@en,
        "comprend"@fr,
        "consiste de"@pt,
        "состоит из"@ru,
        "包括"@zh ;
    rdfs:comment """This property associates an instance of E4 Period with another instance of E4 Period that is defined by a subset of the phenomena that define the former. Therefore, the spacetime volume of the latter must fall within the spacetime volume of the former.
This property is transitive and asymmetric."""@en ;
    rdfs:domain <http://www.cidoc-crm.org/cidoc-crm/E4_Period> ;
    rdfs:range <http://www.cidoc-crm.org/cidoc-crm/E4_Period> ;
    rdfs:subPropertyOf <http://www.cidoc-crm.org/cidoc-crm/P10i_contains> ;
    owl:inverseOf <http://www.cidoc-crm.org/cidoc-crm/P9i_forms_part_of> .

<http://www.cidoc-crm.org/cidoc-crm/P9i_forms_part_of> a rdf:Property ;
    rdfs:label "bildet Teil von"@de,
        "αποτελεί μέρος του/της"@el,
        "forms part of"@en,
        "fait partie de"@fr,
        "faz parte de"@pt,
        "являeтся частью"@ru,
        "组成部分"@zh ;
    rdfs:domain <http://www.cidoc-crm.org/cidoc-crm/E4_Period> ;
    rdfs:range <http://www.cidoc-crm.org/cidoc-crm/E4_Period> ;
    rdfs:subPropertyOf <http://www.cidoc-crm.org/cidoc-crm/P10_falls_within> ;
    owl:inverseOf <http://www.cidoc-crm.org/cidoc-crm/P9_consists_of> .

<http://www.cidoc-crm.org/extensions/crmarchaeo/AP10_destroyed> a rdf:Property ;
    rdfs:label "destroyed"@en ;
    rdfs:comment "This property identifies the S22 Segment of Matter that was destroyed through an A1 Excavation Processing Unit. The spatial extent of the instance of S22 Segment of Matter is defined by the extent of the spatial 3-dimensional projection of the A1 Excavation Processing Unit. Depending on the granularity of the documented instance of A1 Excavation Processing Unit, different instances of S22 Segment of Matter may be identified by the A10 property."@en ;
    rdfs:domain <http://www.cidoc-crm.org/extensions/crmarchaeo/A1_Excavation_Processing_Unit> ;
    rdfs:range <http://www.cidoc-crm.org/extensions/crmsci/S22_Segment_of_Matter> ;
    rdfs:subPropertyOf <http://www.cidoc-crm.org/cidoc-crm/P93_took_out_of_existence> ;
    owl:inverseOf <http://www.cidoc-crm.org/extensions/crmarchaeo/AP10i_was_destroyed_by> .

<http://www.cidoc-crm.org/extensions/crmarchaeo/AP10i_was_destroyed_by> a rdf:Property ;
    rdfs:label "was destroyed by"@en ;
    rdfs:domain <http://www.cidoc-crm.org/extensions/crmsci/S22_Segment_of_Matter> ;
    rdfs:range <http://www.cidoc-crm.org/extensions/crmarchaeo/A1_Excavation_Processing_Unit> ;
    rdfs:subPropertyOf <http://www.cidoc-crm.org/cidoc-crm/P93i_was_taken_out_of_existence_by> ;
    owl:inverseOf <http://www.cidoc-crm.org/extensions/crmarchaeo/AP10_destroyed> .

<http://www.cidoc-crm.org/extensions/crmarchaeo/AP11_has_physical_relation_to> a rdf:Property ;
    rdfs:label "has physical relation to"@en ;
    rdfs:comment "This property identifies the physical relationship between two A8 Stratigraphic Units. The described relationship may be between two adjacent instances of A2 Stratigraphic Volume Unit sharing a common interface (instance of A3 Stratigraphic Interface), between an instance of A2 Stratigraphic Volume Unit and one of its adjacent interfaces, such as human-made cuts or earthquake induced faults, or even between two intersecting interfaces. The type of physical relationships found between stratigraphic units in archaeological or geological documentation is documented through the property AP11.1 has type. The type applies to the direction from the domain to the range of the property AP11 has physical relation to (is physically related from). The type of physical relationship typically constitutes strong evidence for the sequence of genesis of the related stratigraphic units, which can be documented by the property AP13 has stratigraphic relation to (is stratigraphically related by). The type may either pertain to a relative topology, such as the one being “under” the other, or to the fine-structure of the interface between them, such as a layer of concrete having filled out earlier micro-cavities in various directions in the interface before solidifying."@en ;
    rdfs:domain <http://www.cidoc-crm.org/extensions/crmarchaeo/A8_Stratigraphic_Unit> ;
    rdfs:range <http://www.cidoc-crm.org/extensions/crmarchaeo/A8_Stratigraphic_Unit> ;
    owl:inverseOf <http://www.cidoc-crm.org/extensions/crmarchaeo/AP11i_is_physical_relation_from> .

<http://www.cidoc-crm.org/extensions/crmarchaeo/AP11i_is_physical_relation_from> a rdf:Property ;
    rdfs:label "is physical relation from"@en ;
    rdfs:domain <http://www.cidoc-crm.org/extensions/crmarchaeo/A8_Stratigraphic_Unit> ;
    rdfs:range <http://www.cidoc-crm.org/extensions/crmarchaeo/A8_Stratigraphic_Unit> ;
    owl:inverseOf <http://www.cidoc-crm.org/extensions/crmarchaeo/AP11_has_physical_relation_to> .

<http://www.cidoc-crm.org/extensions/crmarchaeo/AP13_has_stratigraphic_relation_to> a rdf:Property ;
    rdfs:label "has stratigraphic relation to"@en ;
    rdfs:comment "This property identifies the stratigraphic relation between two A5 Stratigraphic Modification events. This relation may be inferred from the kind of physical relation that exists between the two AP 8 Stratigraphic Units that have been created or modified during the corresponding A5 Stratigraphic Modification events. The type of stratigraphic relationships in archaeological documentation assigned to two A5 Stratigraphic Modification events is documented through the property AP 13.1 has type."@en ;
    rdfs:domain <http://www.cidoc-crm.org/extensions/crmarchaeo/A5_Stratigraphic_Modification> ;
    rdfs:range <http://www.cidoc-crm.org/extensions/crmarchaeo/A5_Stratigraphic_Modification> ;
    owl:inverseOf <http://www.cidoc-crm.org/extensions/crmarchaeo/AP13i_is_stratigraphic_relation_of> .

<http://www.cidoc-crm.org/extensions/crmarchaeo/AP13i_is_stratigraphic_relation_of> a rdf:Property ;
    rdfs:label "is stratigraphic relation of"@en ;
    rdfs:domain <http://www.cidoc-crm.org/extensions/crmarchaeo/A5_Stratigraphic_Modification> ;
    rdfs:range <http://www.cidoc-crm.org/extensions/crmarchaeo/A5_Stratigraphic_Modification> ;
    owl:inverseOf <http://www.cidoc-crm.org/extensions/crmarchaeo/AP13_has_stratigraphic_relation_to> .

<http://www.cidoc-crm.org/extensions/crmarchaeo/AP15_is_or_contains_remains_of> a rdf:Property ;
    rdfs:label "is or contains remains of"@en ;
    rdfs:comment "This property indicates that an instance of A2 Stratigraphic Volume Unit can be the remains of or contain the remains of an instance of S10 Material Substantial."@en ;
    rdfs:domain <http://www.cidoc-crm.org/extensions/crmarchaeo/A2_Stratigraphic_Volume_Unit> ;
    rdfs:range <http://www.cidoc-crm.org/extensions/crmsci/S10_Material_Substantial> ;
    owl:inverseOf <http://www.cidoc-crm.org/extensions/crmarchaeo/AP15i_is_or_has_remains_contained_in> .

<http://www.cidoc-crm.org/extensions/crmarchaeo/AP15i_is_or_has_remains_contained_in> a rdf:Property ;
    rdfs:label "is or has remains contained in"@en ;
    rdfs:domain <http://www.cidoc-crm.org/extensions/crmsci/S10_Material_Substantial> ;
    rdfs:range <http://www.cidoc-crm.org/extensions/crmarchaeo/A2_Stratigraphic_Volume_Unit> ;
    owl:inverseOf <http://www.cidoc-crm.org/extensions/crmarchaeo/AP15_is_or_contains_remains_of> .

<http://www.cidoc-crm.org/extensions/crmarchaeo/AP16_assigned_attribute_to> a rdf:Property ;
    rdfs:label "assigned attribute to"@en ;
    rdfs:comment "This property indicates an instance of E18 Physical Thing that was assigned by an instance of A6 Group Declaration Event as remains of the target of this instance of A6 Group Declaration Event."@en ;
    rdfs:domain <http://www.cidoc-crm.org/extensions/crmarchaeo/A6_Group_Declaration_Event> ;
    rdfs:range <http://www.cidoc-crm.org/cidoc-crm/E18_Physical_Thing> ;
    rdfs:subPropertyOf <http://www.cidoc-crm.org/cidoc-crm/P140_assigned_attribute_to> ;
    owl:inverseOf <http://www.cidoc-crm.org/extensions/crmarchaeo/AP16i_was_attributed_by> .

<http://www.cidoc-crm.org/extensions/crmarchaeo/AP16i_was_attributed_by> a rdf:Property ;
    rdfs:label "was attributed by"@en ;
    rdfs:domain <http://www.cidoc-crm.org/cidoc-crm/E18_Physical_Thing> ;
    rdfs:range <http://www.cidoc-crm.org/extensions/crmarchaeo/A6_Group_Declaration_Event> ;
    rdfs:subPropertyOf <http://www.cidoc-crm.org/cidoc-crm/P140i_was_attributed_by> ;
    owl:inverseOf <http://www.cidoc-crm.org/extensions/crmarchaeo/AP16_assigned_attribute_to> .

<http://www.cidoc-crm.org/extensions/crmarchaeo/AP17_is_found_by> a rdf:Property ;
    rdfs:label "is found by"@en ;
    rdfs:comment "This property associates an instance of S19 Encounter Event with an instance of A7 Embedding that has been found during this event."@en ;
    rdfs:domain <http://www.cidoc-crm.org/extensions/crmarchaeo/A7_Embedding> ;
    rdfs:range <http://www.cidoc-crm.org/extensions/crmsci/S19_Encounter_Event> ;
    rdfs:subPropertyOf <http://www.cidoc-crm.org/extensions/crmsci/O8_observed> ;
    owl:inverseOf <http://www.cidoc-crm.org/extensions/crmarchaeo/AP17i_found> .

<http://www.cidoc-crm.org/extensions/crmarchaeo/AP17i_found> a rdf:Property ;
    rdfs:label "found"@en ;
    rdfs:domain <http://www.cidoc-crm.org/extensions/crmsci/S19_Encounter_Event> ;
    rdfs:range <http://www.cidoc-crm.org/extensions/crmarchaeo/A7_Embedding> ;
    rdfs:subPropertyOf <http://www.cidoc-crm.org/extensions/crmsci/O8i_was_observed_by> ;
    owl:inverseOf <http://www.cidoc-crm.org/extensions/crmarchaeo/AP17_is_found_by> .

<http://www.cidoc-crm.org/extensions/crmarchaeo/AP18_is_embedding_of> a rdf:Property ;
    rdfs:label "is embedding of"@en ;
    rdfs:comment "This property identifies the E18 Physical Thing that is contained in an A7 Embedding."@en ;
    rdfs:domain <http://www.cidoc-crm.org/extensions/crmarchaeo/A7_Embedding> ;
    rdfs:range <http://www.cidoc-crm.org/cidoc-crm/E18_Physical_Thing> ;
    rdfs:subPropertyOf <http://www.cidoc-crm.org/cidoc-crm/P46_is_composed_of> ;
    owl:inverseOf <http://www.cidoc-crm.org/extensions/crmarchaeo/AP18i_is_embedded> .

<http://www.cidoc-crm.org/extensions/crmarchaeo/AP18i_is_embedded> a rdf:Property ;
    rdfs:label "is embedded"@en ;
    rdfs:domain <http://www.cidoc-crm.org/cidoc-crm/E18_Physical_Thing> ;
    rdfs:range <http://www.cidoc-crm.org/extensions/crmarchaeo/A7_Embedding> ;
    rdfs:subPropertyOf <http://www.cidoc-crm.org/cidoc-crm/P46i_forms_part_of> ;
    owl:inverseOf <http://www.cidoc-crm.org/extensions/crmarchaeo/AP18_is_embedding_of> .

<http://www.cidoc-crm.org/extensions/crmarchaeo/AP19_is_embedding_in> a rdf:Property ;
    rdfs:label "is embedding in"@en ;
    rdfs:comment "This property identifies the instance of A2 Stratigraphic Volume Unit that contains the A7 Embedding. An Embedding may not extend over more than one instance of A2 Stratigraphic Volume Unit."@en ;
    rdfs:domain <http://www.cidoc-crm.org/extensions/crmarchaeo/A7_Embedding> ;
    rdfs:range <http://www.cidoc-crm.org/extensions/crmarchaeo/A2_Stratigraphic_Volume_Unit> ;
    owl:inverseOf <http://www.cidoc-crm.org/extensions/crmarchaeo/AP19i_contains_embedding> .

<http://www.cidoc-crm.org/extensions/crmarchaeo/AP19i_contains_embedding> a rdf:Property ;
    rdfs:label "contains embedding"@en ;
    rdfs:domain <http://www.cidoc-crm.org/extensions/crmarchaeo/A2_Stratigraphic_Volume_Unit> ;
    rdfs:range <http://www.cidoc-crm.org/extensions/crmarchaeo/A7_Embedding> ;
    owl:inverseOf <http://www.cidoc-crm.org/extensions/crmarchaeo/AP19_is_embedding_in> .

<http://www.cidoc-crm.org/extensions/crmarchaeo/AP1_produced> a rdf:Property ;
    rdfs:label "produced"@en ;
    rdfs:comment "This property identifies the S11 Amount of Matter, e.g. a basket, that is preserved (part or total of) from an instance of A1 Excavation Processing Unit for further examination or evidence keeping."@en ;
    rdfs:domain <http://www.cidoc-crm.org/extensions/crmarchaeo/A1_Excavation_Processing_Unit> ;
    rdfs:range <http://www.cidoc-crm.org/extensions/crmsci/S11_Amount_of_Matter> ;
    rdfs:subPropertyOf <http://www.cidoc-crm.org/extensions/crmsci/O2_removed> ;
    owl:inverseOf <http://www.cidoc-crm.org/extensions/crmarchaeo/AP1i_was_produced_by> .

<http://www.cidoc-crm.org/extensions/crmarchaeo/AP1i_was_produced_by> a rdf:Property ;
    rdfs:label "was produced by"@en ;
    rdfs:domain <http://www.cidoc-crm.org/extensions/crmsci/S11_Amount_of_Matter> ;
    rdfs:range <http://www.cidoc-crm.org/extensions/crmarchaeo/A1_Excavation_Processing_Unit> ;
    rdfs:subPropertyOf <http://www.cidoc-crm.org/extensions/crmsci/O2i_was_removed_by> ;
    owl:inverseOf <http://www.cidoc-crm.org/extensions/crmarchaeo/AP1_produced> .

<http://www.cidoc-crm.org/extensions/crmarchaeo/AP21_contains> a rdf:Property ;
    rdfs:label "contains"@en ;
    rdfs:comment "This property associates an E18 Physical Thing that is found within an A2 Stratigraphic Volume Unit with the stratigraphic volume unit. AP21 contains (is contained in) is a shortcut for the more detailed path from E18 Physical Thing through AP18i is embedded, A7 Embedding, AP19 is embedding in, A2 Stratigraphic Volume Unit."@en ;
    rdfs:domain <http://www.cidoc-crm.org/extensions/crmarchaeo/A2_Stratigraphic_Volume_Unit> ;
    rdfs:range <http://www.cidoc-crm.org/cidoc-crm/E18_Physical_Thing> ;
    owl:inverseOf <http://www.cidoc-crm.org/extensions/crmarchaeo/AP21i_is_contained_in> .

<http://www.cidoc-crm.org/extensions/crmarchaeo/AP21i_is_contained_in> a rdf:Property ;
    rdfs:label "is contained in"@en ;
    rdfs:domain <http://www.cidoc-crm.org/cidoc-crm/E18_Physical_Thing> ;
    rdfs:range <http://www.cidoc-crm.org/extensions/crmarchaeo/A2_Stratigraphic_Volume_Unit> ;
    owl:inverseOf <http://www.cidoc-crm.org/extensions/crmarchaeo/AP21_contains> .

<http://www.cidoc-crm.org/extensions/crmarchaeo/AP23_finishes> a rdf:Property ;
    rdfs:label "finishes"@en ;
    rdfs:comment "This property identifies a situation in which the ending point of an instance of E2 Temporal Entity is equal to the ending point of another temporal entity of longer duration. There is no causal relationship implied by this property. This property is only necessary if the time span is unknown (otherwise the relationship can be calculated). This property is the same as the \"finishes / finished-by\" relationships of Allen’s temporal logic (Allen, 1983, pp. 832-843). This property is transitive."@en ;
    rdfs:domain <http://www.cidoc-crm.org/cidoc-crm/E2_Temporal_Entity> ;
    rdfs:range <http://www.cidoc-crm.org/cidoc-crm/E2_Temporal_Entity> ;
    rdfs:subPropertyOf <http://www.cidoc-crm.org/cidoc-crm/P176i_starts_after_the_start_of>,
        <http://www.cidoc-crm.org/cidoc-crm/P184_ends_before_or_with_the_end_of>,
        <http://www.cidoc-crm.org/cidoc-crm/P184i_ends_with_or_after_the_end_of> ;
    owl:inverseOf <http://www.cidoc-crm.org/extensions/crmarchaeo/AP23i_is_finished_by> .

<http://www.cidoc-crm.org/extensions/crmarchaeo/AP23i_is_finished_by> a rdf:Property ;
    rdfs:label "is finished by"@en ;
    rdfs:domain <http://www.cidoc-crm.org/cidoc-crm/E2_Temporal_Entity> ;
    rdfs:range <http://www.cidoc-crm.org/cidoc-crm/E2_Temporal_Entity> ;
    rdfs:subPropertyOf <http://www.cidoc-crm.org/cidoc-crm/P176_starts_before_the_start_of>,
        <http://www.cidoc-crm.org/cidoc-crm/P184_ends_before_or_with_the_end_of>,
        <http://www.cidoc-crm.org/cidoc-crm/P184i_ends_with_or_after_the_end_of> ;
    owl:inverseOf <http://www.cidoc-crm.org/extensions/crmarchaeo/AP23_finishes> .

<http://www.cidoc-crm.org/extensions/crmarchaeo/AP24_starts> a rdf:Property ;
    rdfs:label "starts"@en ;
    rdfs:comment "This property identifies a situation in which the starting point for an instance of E2 Temporal Entity is equal to the starting point of another instance of E2 Temporal Entity of longer duration. This property is only necessary if the time span is unknown (otherwise the relationship can be calculated). This property is the same as the \"starts / started-by\" relationships of Allen’s temporal logic (Allen, 1983, pp. 832-843). This property is transitive."@en ;
    rdfs:domain <http://www.cidoc-crm.org/cidoc-crm/E2_Temporal_Entity> ;
    rdfs:range <http://www.cidoc-crm.org/cidoc-crm/E2_Temporal_Entity> ;
    rdfs:subPropertyOf <http://www.cidoc-crm.org/cidoc-crm/P175_starts_before_or_with_the_start_of>,
        <http://www.cidoc-crm.org/cidoc-crm/P175i_starts_after_or_with_the_start_of>,
        <http://www.cidoc-crm.org/cidoc-crm/P185_ends_before_the_end_of> ;
    owl:inverseOf <http://www.cidoc-crm.org/extensions/crmarchaeo/AP24i_is_started_by> .

<http://www.cidoc-crm.org/extensions/crmarchaeo/AP24i_is_started_by> a rdf:Property ;
    rdfs:label "is started by"@en ;
    rdfs:domain <http://www.cidoc-crm.org/cidoc-crm/E2_Temporal_Entity> ;
    rdfs:range <http://www.cidoc-crm.org/cidoc-crm/E2_Temporal_Entity> ;
    rdfs:subPropertyOf <http://www.cidoc-crm.org/cidoc-crm/P175_starts_before_or_with_the_start_of>,
        <http://www.cidoc-crm.org/cidoc-crm/P175i_starts_after_or_with_the_start_of>,
        <http://www.cidoc-crm.org/cidoc-crm/P185i_ends_after_the_end_of> ;
    owl:inverseOf <http://www.cidoc-crm.org/extensions/crmarchaeo/AP24_starts> .

<http://www.cidoc-crm.org/extensions/crmarchaeo/AP25_occurs_during> a rdf:Property ;
    rdfs:label "occurs during"@en ;
    rdfs:comment "This property identifies the situation in which the entire temporal extent of an instance of E2 Temporal Entity is within the temporal extent of another instance of E2 Temporal Entity that starts before and ends after the included temporal entity. This property is only necessary if the time span is unknown (otherwise the relationship can be calculated). This property is the same as the \"during / includes\" relationships of Allen’s temporal logic (Allen, 1983, pp. 832-843). This property is transitive."@en ;
    rdfs:domain <http://www.cidoc-crm.org/cidoc-crm/E2_Temporal_Entity> ;
    rdfs:range <http://www.cidoc-crm.org/cidoc-crm/E2_Temporal_Entity> ;
    rdfs:subPropertyOf <http://www.cidoc-crm.org/cidoc-crm/P176i_starts_after_the_start_of>,
        <http://www.cidoc-crm.org/cidoc-crm/P185_ends_before_the_end_of> ;
    owl:inverseOf <http://www.cidoc-crm.org/extensions/crmarchaeo/AP25i_includes> .

<http://www.cidoc-crm.org/extensions/crmarchaeo/AP25i_includes> a rdf:Property ;
    rdfs:label "includes"@en ;
    rdfs:domain <http://www.cidoc-crm.org/cidoc-crm/E2_Temporal_Entity> ;
    rdfs:range <http://www.cidoc-crm.org/cidoc-crm/E2_Temporal_Entity> ;
    rdfs:subPropertyOf <http://www.cidoc-crm.org/cidoc-crm/P176_starts_before_the_start_of>,
        <http://www.cidoc-crm.org/cidoc-crm/P185i_ends_after_the_end_of> ;
    owl:inverseOf <http://www.cidoc-crm.org/extensions/crmarchaeo/AP25_occurs_during> .

<http://www.cidoc-crm.org/extensions/crmarchaeo/AP26_overlaps_in_time_with> a rdf:Property ;
    rdfs:label "overlaps in time with"@en ;
    rdfs:comment "This property identifies a situation in which there is an overlap between the temporal extents of two instances of E2 Temporal Entity. It implies a temporal order between the two entities: if A overlaps in time B, then A must start before B, and B must end after A. This property is only necessary if the relevant time spans are unknown (otherwise the relationship can be calculated). This property is the same as the \"overlaps / overlapped-by\" relationships of Allen’s temporal logic (Allen, 1983, pp. 832-843)."@en ;
    rdfs:domain <http://www.cidoc-crm.org/cidoc-crm/E2_Temporal_Entity> ;
    rdfs:range <http://www.cidoc-crm.org/cidoc-crm/E2_Temporal_Entity> ;
    rdfs:subPropertyOf <http://www.cidoc-crm.org/cidoc-crm/P174i_ends_after_the_start_of>,
        <http://www.cidoc-crm.org/cidoc-crm/P176_starts_before_the_start_of>,
        <http://www.cidoc-crm.org/cidoc-crm/P185_ends_before_the_end_of> ;
    owl:inverseOf <http://www.cidoc-crm.org/extensions/crmarchaeo/AP26i_is_overlapped_in_time_by> .

<http://www.cidoc-crm.org/extensions/crmarchaeo/AP26i_is_overlapped_in_time_by> a rdf:Property ;
    rdfs:label "is overlapped in time by"@en ;
    rdfs:domain <http://www.cidoc-crm.org/cidoc-crm/E2_Temporal_Entity> ;
    rdfs:range <http://www.cidoc-crm.org/cidoc-crm/E2_Temporal_Entity> ;
    rdfs:subPropertyOf <http://www.cidoc-crm.org/cidoc-crm/P174_starts_before_the_end_of>,
        <http://www.cidoc-crm.org/cidoc-crm/P176i_starts_after_the_start_of>,
        <http://www.cidoc-crm.org/cidoc-crm/P185i_ends_after_the_end_of> ;
    owl:inverseOf <http://www.cidoc-crm.org/extensions/crmarchaeo/AP26_overlaps_in_time_with> .

<http://www.cidoc-crm.org/extensions/crmarchaeo/AP27_meets_in_time_with> a rdf:Property ;
    rdfs:label "meets in time with"@en ;
    rdfs:comment "This property identifies a situation in which one instance of E2 Temporal Entity immediately follows another instance of E2 Temporal Entity. It implies a particular order between the two entities: if A meets in time with B, then A must precede B. This property is only necessary if the relevant time spans are unknown (otherwise the relationship can be calculated). This property is the same as the \"meets / met-by\" relationships of Allen’s temporal logic (Allen, 1983, pp. 832-843)."@en ;
    rdfs:domain <http://www.cidoc-crm.org/cidoc-crm/E2_Temporal_Entity> ;
    rdfs:range <http://www.cidoc-crm.org/cidoc-crm/E2_Temporal_Entity> ;
    rdfs:subPropertyOf <http://www.cidoc-crm.org/cidoc-crm/P173i_ends_after_or_with_the_start_of>,
        <http://www.cidoc-crm.org/cidoc-crm/P182_ends_before_or_with_the_start_of> ;
    owl:inverseOf <http://www.cidoc-crm.org/extensions/crmarchaeo/AP27i_is_met_in_time_by> .

<http://www.cidoc-crm.org/extensions/crmarchaeo/AP27i_is_met_in_time_by> a rdf:Property ;
    rdfs:label "is met in time by"@en ;
    rdfs:domain <http://www.cidoc-crm.org/cidoc-crm/E2_Temporal_Entity> ;
    rdfs:range <http://www.cidoc-crm.org/cidoc-crm/E2_Temporal_Entity> ;
    rdfs:subPropertyOf <http://www.cidoc-crm.org/cidoc-crm/P173_starts_before_or_with_the_end_of>,
        <http://www.cidoc-crm.org/cidoc-crm/P182i_starts_after_or_with_the_end_of> ;
    owl:inverseOf <http://www.cidoc-crm.org/extensions/crmarchaeo/AP27_meets_in_time_with> .

<http://www.cidoc-crm.org/extensions/crmarchaeo/AP28_occurs_before> a rdf:Property ;
    rdfs:label "occurs before"@en ;
    rdfs:comment "This property identifies the relative chronological sequence of two temporal entities. It implies that a temporal gap exists between the end of A and the start of B. This property is only necessary if the relevant time spans are unknown (otherwise the relationship can be calculated). This property is the same as the \"before / after\" relationships of Allen’s temporal logic(Allen, 1983). This property is transitive."@en ;
    rdfs:domain <http://www.cidoc-crm.org/cidoc-crm/E2_Temporal_Entity> ;
    rdfs:range <http://www.cidoc-crm.org/cidoc-crm/E2_Temporal_Entity> ;
    rdfs:subPropertyOf <http://www.cidoc-crm.org/cidoc-crm/P183_ends_before_the_start_of> ;
    owl:inverseOf <http://www.cidoc-crm.org/extensions/crmarchaeo/AP28i_occurs_after> .

<http://www.cidoc-crm.org/extensions/crmarchaeo/AP28i_occurs_after> a rdf:Property ;
    rdfs:label "occurs after"@en ;
    rdfs:domain <http://www.cidoc-crm.org/cidoc-crm/E2_Temporal_Entity> ;
    rdfs:range <http://www.cidoc-crm.org/cidoc-crm/E2_Temporal_Entity> ;
    rdfs:subPropertyOf <http://www.cidoc-crm.org/cidoc-crm/P183i_starts_after_the_end_of> ;
    owl:inverseOf <http://www.cidoc-crm.org/extensions/crmarchaeo/AP28_occurs_before> .

<http://www.cidoc-crm.org/extensions/crmarchaeo/AP2_discarded> a rdf:Property ;
    rdfs:label "discarded"@en ;
    rdfs:comment "This property identifies an instance of S11 Amount of Matter discarded (e.g. onto a heap) by an instance of A1 Excavation Processing Unit."@en ;
    rdfs:domain <http://www.cidoc-crm.org/extensions/crmarchaeo/A1_Excavation_Processing_Unit> ;
    rdfs:range <http://www.cidoc-crm.org/extensions/crmsci/S11_Amount_of_Matter> ;
    rdfs:subPropertyOf <http://www.cidoc-crm.org/extensions/crmsci/O2_removed> ;
    owl:inverseOf <http://www.cidoc-crm.org/extensions/crmarchaeo/AP2i_was_discarded_by> .

<http://www.cidoc-crm.org/extensions/crmarchaeo/AP2i_was_discarded_by> a rdf:Property ;
    rdfs:label "was discarded by"@en ;
    rdfs:domain <http://www.cidoc-crm.org/extensions/crmsci/S11_Amount_of_Matter> ;
    rdfs:range <http://www.cidoc-crm.org/extensions/crmarchaeo/A1_Excavation_Processing_Unit> ;
    rdfs:subPropertyOf <http://www.cidoc-crm.org/extensions/crmsci/O2i_was_removed_by> ;
    owl:inverseOf <http://www.cidoc-crm.org/extensions/crmarchaeo/AP2_discarded> .

<http://www.cidoc-crm.org/extensions/crmarchaeo/AP30_restricted_to> a rdf:Property ;
    rdfs:label "restricted to"@en ;
    rdfs:comment "This property associates a kind of object (documented as an instance of E55 Type) with an instance of E4 Period indicating that objects of this kind have been generated exclusively in this period. This property makes a strong statement concerning the distribution of the associated object kind in the observed record: If the genesis of an object of this type can plausibly be assumed to fall within the genesis of the context in which it was found, then the statement made with this property would support reasoning, ceteris paribus , that the genesis period of the find context actually forms part of the related instance of E4 Period, or at least overlaps with it. In contrast, objects from previous periods may appear in a context because they are still in use, and objects from later periods may have been displaced into an older context. Weaker claims can be made using the properties AP29 appears in (gas appearing type) and AP31 typical for (has typical type) ."@en ;
    rdfs:domain <http://www.cidoc-crm.org/cidoc-crm/E55_Type> ;
    rdfs:range <http://www.cidoc-crm.org/cidoc-crm/E4_Period> ;
    rdfs:subPropertyOf <http://www.cidoc-crm.org/extensions/crmarchaeo/AP29_appears_in> ;
    owl:inverseOf <http://www.cidoc-crm.org/extensions/crmarchaeo/AP30i_restricts_appearance_of> .

<http://www.cidoc-crm.org/extensions/crmarchaeo/AP30i_restricts_appearance_of> a rdf:Property ;
    rdfs:label "restricts appearance of"@en ;
    rdfs:domain <http://www.cidoc-crm.org/cidoc-crm/E4_Period> ;
    rdfs:range <http://www.cidoc-crm.org/cidoc-crm/E55_Type> ;
    rdfs:subPropertyOf <http://www.cidoc-crm.org/extensions/crmarchaeo/AP29i_has_appearing_type> ;
    owl:inverseOf <http://www.cidoc-crm.org/extensions/crmarchaeo/AP30_restricted_to> .

<http://www.cidoc-crm.org/extensions/crmarchaeo/AP31_typical_for> a rdf:Property ;
    rdfs:label "typical for"@en ;
    rdfs:comment "This property associates a kind of object (documented as an instance of E55 Type) with an instance of E4 Period indicating that objects of this kind have been generated in this period in significantly greater numbers and in wider distributions, than in other periods. This property makes a moderate statement concerning the distribution of the associated object kind in the observed record: If a \"sufficient number\" of objects of this type are found in a context, and their genesis can plausibly be assumed to fall within the genesis of the find context, then the statement made with this property would support reasoning, ceteris paribus , that the genesis period of the find context is likely to form part of the related instance of E4 Period, or at least overlap with it. “Sufficient number” means that the density of objects of this kind in the find context is compatible with the general density that this kind of object had during the associated period in contexts of a comparable nature and deposition history. A stronger claim can be made using AP30 restricted to (restricts appearance of) while a weaker claim would use AP29 appears in (has appearing type) ."@en ;
    rdfs:domain <http://www.cidoc-crm.org/cidoc-crm/E55_Type> ;
    rdfs:range <http://www.cidoc-crm.org/cidoc-crm/E4_Period> ;
    rdfs:subPropertyOf <http://www.cidoc-crm.org/extensions/crmarchaeo/AP29_appears_in> ;
    owl:inverseOf <http://www.cidoc-crm.org/extensions/crmarchaeo/AP31i_has_typical_type> .

<http://www.cidoc-crm.org/extensions/crmarchaeo/AP31i_has_typical_type> a rdf:Property ;
    rdfs:label "has typical type"@en ;
    rdfs:domain <http://www.cidoc-crm.org/cidoc-crm/E4_Period> ;
    rdfs:range <http://www.cidoc-crm.org/cidoc-crm/E55_Type> ;
    rdfs:subPropertyOf <http://www.cidoc-crm.org/extensions/crmarchaeo/AP29i_has_appearing_type> ;
    owl:inverseOf <http://www.cidoc-crm.org/extensions/crmarchaeo/AP31_typical_for> .

<http://www.cidoc-crm.org/extensions/crmarchaeo/AP32_discarded_into> a rdf:Property ;
    rdfs:label "discarded into"@en ;
    rdfs:comment "This property identifies the S11 Amount of Matter (e.g. a heap) into which material from an A1 Excavation Processing Unit is discarded. The same instance of A1 Excavation Processing Unit may discard matter into multiple heaps, but also simply throw away the excavated matter without any order or exported to be deposited elsewhere, thereby breaking any close correspondence between the excavation and the deposit."@en ;
    rdfs:domain <http://www.cidoc-crm.org/extensions/crmarchaeo/A1_Excavation_Processing_Unit> ;
    rdfs:range <http://www.cidoc-crm.org/extensions/crmsci/S11_Amount_of_Matter> ;
    owl:inverseOf <http://www.cidoc-crm.org/extensions/crmarchaeo/AP32i_was_discarded_by> .

<http://www.cidoc-crm.org/extensions/crmarchaeo/AP32i_was_discarded_by> a rdf:Property ;
    rdfs:label "was discarded by"@en ;
    rdfs:domain <http://www.cidoc-crm.org/extensions/crmsci/S11_Amount_of_Matter> ;
    rdfs:range <http://www.cidoc-crm.org/extensions/crmarchaeo/A1_Excavation_Processing_Unit> ;
    owl:inverseOf <http://www.cidoc-crm.org/extensions/crmarchaeo/AP32_discarded_into> .

<http://www.cidoc-crm.org/extensions/crmarchaeo/AP3_investigated> a rdf:Property ;
    rdfs:label "investigated"@en ;
    rdfs:comment "This property identifies the 3D excavated volume instance of E27 Site, i.e., a three- dimensional volume, that was actually investigated during an A9 Archaeological Excavation."@en ;
    rdfs:domain <http://www.cidoc-crm.org/extensions/crmarchaeo/A9_Archaeological_Excavation> ;
    rdfs:range <http://www.cidoc-crm.org/cidoc-crm/E27_Site> ;
    rdfs:subPropertyOf <http://www.cidoc-crm.org/extensions/crmsci/O8_observed> ;
    owl:inverseOf <http://www.cidoc-crm.org/extensions/crmarchaeo/AP3i_was_investigated_by> .

<http://www.cidoc-crm.org/extensions/crmarchaeo/AP3i_was_investigated_by> a rdf:Property ;
    rdfs:label "was investigated by"@en ;
    rdfs:domain <http://www.cidoc-crm.org/cidoc-crm/E27_Site> ;
    rdfs:range <http://www.cidoc-crm.org/extensions/crmarchaeo/A9_Archaeological_Excavation> ;
    rdfs:subPropertyOf <http://www.cidoc-crm.org/extensions/crmsci/O8i_was_observed_by> ;
    owl:inverseOf <http://www.cidoc-crm.org/extensions/crmarchaeo/AP3_investigated> .

<http://www.cidoc-crm.org/extensions/crmarchaeo/AP4_produced_surface> a rdf:Property ;
    rdfs:label "produced surface"@en ;
    rdfs:comment "This property identifies the instance of A10 Excavation Interface that constitutes the new surface produced during an instance of A1 Excavation Processing Unit in the excavated area. Frequently this surface or parts of it are documented through drawing and/or measured by technical means such as photography, tachymetry or laser scanning."@en ;
    rdfs:domain <http://www.cidoc-crm.org/extensions/crmarchaeo/A1_Excavation_Processing_Unit> ;
    rdfs:range <http://www.cidoc-crm.org/extensions/crmarchaeo/A10_Excavation_Interface> ;
    rdfs:subPropertyOf <http://www.cidoc-crm.org/cidoc-crm/P108_has_produced> ;
    owl:inverseOf <http://www.cidoc-crm.org/extensions/crmarchaeo/AP4i_was_surface_produced_by> .

<http://www.cidoc-crm.org/extensions/crmarchaeo/AP4i_was_surface_produced_by> a rdf:Property ;
    rdfs:label "was surface produced by"@en ;
    rdfs:domain <http://www.cidoc-crm.org/extensions/crmarchaeo/A10_Excavation_Interface> ;
    rdfs:range <http://www.cidoc-crm.org/extensions/crmarchaeo/A1_Excavation_Processing_Unit> ;
    rdfs:subPropertyOf <http://www.cidoc-crm.org/cidoc-crm/P108i_was_produced_by> ;
    owl:inverseOf <http://www.cidoc-crm.org/extensions/crmarchaeo/AP4_produced_surface> .

<http://www.cidoc-crm.org/extensions/crmarchaeo/AP5_removed_part_or_all_of> a rdf:Property ;
    rdfs:label "removed part or all of"@en ;
    rdfs:comment "This property identifies the instance of A8 Stratigraphic Unit that was cut during an A1 Excavation Processing Unit."@en ;
    rdfs:domain <http://www.cidoc-crm.org/extensions/crmarchaeo/A1_Excavation_Processing_Unit> ;
    rdfs:range <http://www.cidoc-crm.org/extensions/crmarchaeo/A8_Stratigraphic_Unit> ;
    rdfs:subPropertyOf <http://www.cidoc-crm.org/extensions/crmsci/O1_diminished> ;
    owl:inverseOf <http://www.cidoc-crm.org/extensions/crmarchaeo/AP5i_was_partially_or_totally_removed_by> .

<http://www.cidoc-crm.org/extensions/crmarchaeo/AP5i_was_partially_or_totally_removed_by> a rdf:Property ;
    rdfs:label "was partially or totally removed by"@en ;
    rdfs:domain <http://www.cidoc-crm.org/extensions/crmarchaeo/A8_Stratigraphic_Unit> ;
    rdfs:range <http://www.cidoc-crm.org/extensions/crmarchaeo/A1_Excavation_Processing_Unit> ;
    rdfs:subPropertyOf <http://www.cidoc-crm.org/extensions/crmsci/O1i_was_diminished_by> ;
    owl:inverseOf <http://www.cidoc-crm.org/extensions/crmarchaeo/AP5_removed_part_or_all_of> .

<http://www.cidoc-crm.org/extensions/crmarchaeo/AP6_intended_to_approximate> a rdf:Property ;
    rdfs:label "intended to approximate"@en ;
    rdfs:comment "This property identifies the A3 Stratigraphic Interface that was intended to approximate during an A1 Excavation Processing Unit. This property should be assigned when a stratigraphic excavation methodology is used. It enables the linkage of the surface produced by an A1 Excavation Processing Unit and an A3 Stratigraphic Interface."@en ;
    rdfs:domain <http://www.cidoc-crm.org/extensions/crmarchaeo/A1_Excavation_Processing_Unit> ;
    rdfs:range <http://www.cidoc-crm.org/extensions/crmarchaeo/A3_Stratigraphic_Interface> ;
    rdfs:subPropertyOf <http://www.cidoc-crm.org/extensions/crmsci/O8_observed> ;
    owl:inverseOf <http://www.cidoc-crm.org/extensions/crmarchaeo/AP6i_was_approximated_by> .

<http://www.cidoc-crm.org/extensions/crmarchaeo/AP6i_was_approximated_by> a rdf:Property ;
    rdfs:label "was approximated by"@en ;
    rdfs:domain <http://www.cidoc-crm.org/extensions/crmarchaeo/A3_Stratigraphic_Interface> ;
    rdfs:range <http://www.cidoc-crm.org/extensions/crmarchaeo/A1_Excavation_Processing_Unit> ;
    rdfs:subPropertyOf <http://www.cidoc-crm.org/extensions/crmsci/O8i_was_observed_by> ;
    owl:inverseOf <http://www.cidoc-crm.org/extensions/crmarchaeo/AP6_intended_to_approximate> .

<http://www.cidoc-crm.org/extensions/crmarchaeo/AP7_produced> a rdf:Property ;
    rdfs:label "produced"@en ;
    rdfs:comment "This property identifies the instance of A8 Stratigraphic Unit that was produced during an instance of A4 Stratigraphic Genesis Event."@en ;
    rdfs:domain <http://www.cidoc-crm.org/extensions/crmarchaeo/A4_Stratigraphic_Genesis> ;
    rdfs:range <http://www.cidoc-crm.org/extensions/crmarchaeo/A8_Stratigraphic_Unit> ;
    rdfs:subPropertyOf <http://www.cidoc-crm.org/extensions/crmsci/O17_generated> ;
    owl:inverseOf <http://www.cidoc-crm.org/extensions/crmarchaeo/AP7i_was_produced_by> .

<http://www.cidoc-crm.org/extensions/crmarchaeo/AP7i_was_produced_by> a rdf:Property ;
    rdfs:label "was produced by"@en ;
    rdfs:domain <http://www.cidoc-crm.org/extensions/crmarchaeo/A8_Stratigraphic_Unit> ;
    rdfs:range <http://www.cidoc-crm.org/extensions/crmarchaeo/A4_Stratigraphic_Genesis> ;
    rdfs:subPropertyOf <http://www.cidoc-crm.org/extensions/crmsci/O17i_was_generated_by> ;
    owl:inverseOf <http://www.cidoc-crm.org/extensions/crmarchaeo/AP7_produced> .

<http://www.cidoc-crm.org/extensions/crmarchaeo/AP8_disturbed> a rdf:Property ;
    rdfs:label "disturbed"@en ;
    rdfs:comment "This property identifies an A8 Stratigraphic Unit that was disturbed through an A5 Stratigraphic Modification. One A5 Stratigraphic Modification may disturb several A8 Stratigraphic Units."@en ;
    rdfs:domain <http://www.cidoc-crm.org/extensions/crmarchaeo/A5_Stratigraphic_Modification> ;
    rdfs:range <http://www.cidoc-crm.org/extensions/crmarchaeo/A8_Stratigraphic_Unit> ;
    rdfs:subPropertyOf <http://www.cidoc-crm.org/extensions/crmsci/O18_altered> ;
    owl:inverseOf <http://www.cidoc-crm.org/extensions/crmarchaeo/AP8i_was_disturbed_by> .

<http://www.cidoc-crm.org/extensions/crmarchaeo/AP8i_was_disturbed_by> a rdf:Property ;
    rdfs:label "was disturbed by"@en ;
    rdfs:domain <http://www.cidoc-crm.org/extensions/crmarchaeo/A8_Stratigraphic_Unit> ;
    rdfs:range <http://www.cidoc-crm.org/extensions/crmarchaeo/A5_Stratigraphic_Modification> ;
    rdfs:subPropertyOf <http://www.cidoc-crm.org/extensions/crmsci/O18i_was_altered_by> ;
    owl:inverseOf <http://www.cidoc-crm.org/extensions/crmarchaeo/AP8_disturbed> .

<http://www.cidoc-crm.org/extensions/crmarchaeo/AP9_took_matter_from> a rdf:Property ;
    rdfs:label "took matter from"@en ;
    rdfs:comment "This property associates an instance of A4 Stratigraphic Genesis with an instance of S10 Material Substantial, from which matter was incorporated in the instance of A8 Stratigraphic Unit produced by this genesis. The instance of A8 Stratigraphic Unit produced by an instance of A4 Stratigraphic Genesis can be documented by using the property AP7 produced (was produced by) and should be distinct from the instance of S10 Material Substantial from which matter was taken. The latter instance will be modified or cease to exist due to this genesis process."@en ;
    rdfs:domain <http://www.cidoc-crm.org/extensions/crmarchaeo/A4_Stratigraphic_Genesis> ;
    rdfs:range <http://www.cidoc-crm.org/extensions/crmsci/S10_Material_Substantial> ;
    rdfs:subPropertyOf <http://www.cidoc-crm.org/extensions/crmsci/O18_altered> ;
    owl:inverseOf <http://www.cidoc-crm.org/extensions/crmarchaeo/AP9i_provided_matter_to> .

<http://www.cidoc-crm.org/extensions/crmarchaeo/AP9i_provided_matter_to> a rdf:Property ;
    rdfs:label "provided matter to"@en ;
    rdfs:domain <http://www.cidoc-crm.org/extensions/crmsci/S10_Material_Substantial> ;
    rdfs:range <http://www.cidoc-crm.org/extensions/crmarchaeo/A4_Stratigraphic_Genesis> ;
    rdfs:subPropertyOf <http://www.cidoc-crm.org/extensions/crmsci/O18i_was_altered_by> ;
    owl:inverseOf <http://www.cidoc-crm.org/extensions/crmarchaeo/AP9_took_matter_from> .

<http://www.cidoc-crm.org/extensions/crmsci/O10_assigned_dimension> a rdf:Property ;
    rdfs:label "assigned dimension"@en ;
    rdfs:comment "This property associates an instance of S6 Data Evaluation with an instance of E54 Dimension that a data evaluation activity has assigned. In that case, dimensions may be determined by making evaluations on observational data based on mathematical inference rules and calculations."@en ;
    rdfs:domain <http://www.cidoc-crm.org/extensions/crmsci/S6_Data_Evaluation> ;
    rdfs:range <http://www.cidoc-crm.org/cidoc-crm/E54_Dimension> ;
    rdfs:subPropertyOf <http://www.cidoc-crm.org/cidoc-crm/P141_assigned> ;
    owl:inverseOf <http://www.cidoc-crm.org/extensions/crmsci/O10i_dimension_was_assigned_by> .

<http://www.cidoc-crm.org/extensions/crmsci/O10i_dimension_was_assigned_by> a rdf:Property ;
    rdfs:label "dimension was assigned by"@en ;
    rdfs:domain <http://www.cidoc-crm.org/cidoc-crm/E54_Dimension> ;
    rdfs:range <http://www.cidoc-crm.org/extensions/crmsci/S6_Data_Evaluation> ;
    rdfs:subPropertyOf <http://www.cidoc-crm.org/cidoc-crm/P141i_was_assigned_by> ;
    owl:inverseOf <http://www.cidoc-crm.org/extensions/crmsci/O10_assigned_dimension> .

<http://www.cidoc-crm.org/extensions/crmsci/O11_described> a rdf:Property ;
    rdfs:label "described"@en ;
    rdfs:comment "This property associates an instance of S6 Data Evaluation with an instance of S15 Observable Entity for which a data evaluation activity provides a description. This description of any Observable Entity is based on data evaluations."@en ;
    rdfs:domain <http://www.cidoc-crm.org/extensions/crmsci/S6_Data_Evaluation> ;
    rdfs:range <http://www.cidoc-crm.org/extensions/crmsci/S15_Observable_Entity> ;
    owl:inverseOf <http://www.cidoc-crm.org/extensions/crmsci/O11i_was_described_by> .

<http://www.cidoc-crm.org/extensions/crmsci/O11i_was_described_by> a rdf:Property ;
    rdfs:label "was described by"@en ;
    rdfs:domain <http://www.cidoc-crm.org/extensions/crmsci/S15_Observable_Entity> ;
    rdfs:range <http://www.cidoc-crm.org/extensions/crmsci/S6_Data_Evaluation> ;
    owl:inverseOf <http://www.cidoc-crm.org/extensions/crmsci/O11_described> .

<http://www.cidoc-crm.org/extensions/crmsci/O12_has_dimension> a rdf:Property ;
    rdfs:label "has dimension"@en ;
    rdfs:comment "This property associates an instance of S15 Observable Entity with an instance of E54 Dimension that the observable entity has. It offers no information about how and when an E54 Dimension was established. In case the instance of S15 Observable Entity is more specifically an instance of E18 Physical Thing, using the property O12 has dimension (is dimension of) is equivalent to using the property P43 has dimension (is dimension of). In other words, using the one implies the other."@en ;
    rdfs:domain <http://www.cidoc-crm.org/extensions/crmsci/S15_Observable_Entity> ;
    rdfs:range <http://www.cidoc-crm.org/cidoc-crm/E54_Dimension> ;
    owl:inverseOf <http://www.cidoc-crm.org/extensions/crmsci/O12i_is_dimension_of> .

<http://www.cidoc-crm.org/extensions/crmsci/O12i_is_dimension_of> a rdf:Property ;
    rdfs:label "is dimension of"@en ;
    rdfs:domain <http://www.cidoc-crm.org/cidoc-crm/E54_Dimension> ;
    rdfs:range <http://www.cidoc-crm.org/extensions/crmsci/S15_Observable_Entity> ;
    owl:inverseOf <http://www.cidoc-crm.org/extensions/crmsci/O12_has_dimension> .

<http://www.cidoc-crm.org/extensions/crmsci/O13_triggered> a rdf:Property ;
    rdfs:label "triggered"@en ;
    rdfs:comment "This property associates an instance of E5 Event that triggered another instance of E5 Event with the latter. It identifies the interaction between events: an event can activate (trigger) other events in a target system that is in a situation of sustained tension, such as a trap or an unstable mountain slope giving way to a land slide after a rain or earthquake. In that sense the triggering event is interpreted as a cause. However, the association of the two events is based on their temporal proximity, with the triggering event ending when the triggered event starts."@en ;
    rdfs:domain <http://www.cidoc-crm.org/cidoc-crm/E5_Event> ;
    rdfs:range <http://www.cidoc-crm.org/cidoc-crm/E5_Event> ;
    owl:inverseOf <http://www.cidoc-crm.org/extensions/crmsci/O13i_was_triggered_by> .

<http://www.cidoc-crm.org/extensions/crmsci/O13i_was_triggered_by> a rdf:Property ;
    rdfs:label "was triggered by"@en ;
    rdfs:domain <http://www.cidoc-crm.org/cidoc-crm/E5_Event> ;
    rdfs:range <http://www.cidoc-crm.org/cidoc-crm/E5_Event> ;
    owl:inverseOf <http://www.cidoc-crm.org/extensions/crmsci/O13_triggered> .

<http://www.cidoc-crm.org/extensions/crmsci/O15_occupied> a rdf:Property ;
    rdfs:label "occupied"@en ;
    rdfs:comment "This property associates an instance of S10 Material Substantial with the instance of E53 Place that this substance occupied. It describes the space filled (occupied) by a physical matter. This property is the development of the shortcut expressed in the proposition of classification: “S20 Physical Feature” isA “E53 Place”. This property is equivalent to P156 occupies (is occupied by) with domain E18 Physical Thing and range E53 Place."@en ;
    rdfs:domain <http://www.cidoc-crm.org/extensions/crmsci/S10_Material_Substantial> ;
    rdfs:range <http://www.cidoc-crm.org/cidoc-crm/E53_Place> ;
    owl:inverseOf <http://www.cidoc-crm.org/extensions/crmsci/O15i_was_occupied_by> .

<http://www.cidoc-crm.org/extensions/crmsci/O15i_was_occupied_by> a rdf:Property ;
    rdfs:label "was occupied by"@en ;
    rdfs:domain <http://www.cidoc-crm.org/cidoc-crm/E53_Place> ;
    rdfs:range <http://www.cidoc-crm.org/extensions/crmsci/S10_Material_Substantial> ;
    owl:inverseOf <http://www.cidoc-crm.org/extensions/crmsci/O15_occupied> .

<http://www.cidoc-crm.org/extensions/crmsci/O19_encountered_object> a rdf:Property ;
    rdfs:label "encountered object"@en ;
    rdfs:comment "This property associates an instance of S19 Encounter Event with an instance of E18 Physical Thing that was encountered or observed as present during the event."@en ;
    rdfs:domain <http://www.cidoc-crm.org/extensions/crmsci/S19_Encounter_Event> ;
    rdfs:range <http://www.cidoc-crm.org/cidoc-crm/E18_Physical_Thing> ;
    owl:inverseOf <http://www.cidoc-crm.org/extensions/crmsci/O19i_was_object_encountered_through> .

<http://www.cidoc-crm.org/extensions/crmsci/O19i_was_object_encountered_through> a rdf:Property ;
    rdfs:label "was object encountered through"@en ;
    rdfs:domain <http://www.cidoc-crm.org/cidoc-crm/E18_Physical_Thing> ;
    rdfs:range <http://www.cidoc-crm.org/extensions/crmsci/S19_Encounter_Event> ;
    owl:inverseOf <http://www.cidoc-crm.org/extensions/crmsci/O19_encountered_object> .

<http://www.cidoc-crm.org/extensions/crmsci/O20_sampled_from_type_of_part> a rdf:Property ;
    rdfs:label "sampled from type of part"@en ;
    rdfs:comment "This property associates the activity of a Sample Taking with the type of the location part from which a sample was taken. It is a shortcut of the property O4 sampled at, and it is used as an alternative property, identifying features and material substantial as types of parts of sampling positions."@en ;
    rdfs:domain <http://www.cidoc-crm.org/extensions/crmsci/S2_Sample_Taking> ;
    rdfs:range <http://www.cidoc-crm.org/cidoc-crm/E55_Type> ;
    owl:inverseOf <http://www.cidoc-crm.org/extensions/crmsci/O20i_type_of_part_was_sampled_by> .

<http://www.cidoc-crm.org/extensions/crmsci/O20i_type_of_part_was_sampled_by> a rdf:Property ;
    rdfs:label "type of part was sampled by"@en ;
    rdfs:domain <http://www.cidoc-crm.org/cidoc-crm/E55_Type> ;
    rdfs:range <http://www.cidoc-crm.org/extensions/crmsci/S2_Sample_Taking> ;
    owl:inverseOf <http://www.cidoc-crm.org/extensions/crmsci/O20_sampled_from_type_of_part> .

<http://www.cidoc-crm.org/extensions/crmsci/O21_encountered_at> a rdf:Property ;
    rdfs:label "encountered at"@en ;
    rdfs:comment "This property associates an instance of S19 Encounter Event with an instance of E53 Place at which the things, which were encountered, were observed to be present. This may be given in absolute terms or in terms relative to the observed thing. The associated place must be within the boundaries of the E53 Place at which the S19 Encounter Event took place, if that has been given. Note, that the encountered object may be larger and extend beyond the place of encounter, such as a corner of a building being excavated."@en ;
    rdfs:domain <http://www.cidoc-crm.org/extensions/crmsci/S19_Encounter_Event> ;
    rdfs:range <http://www.cidoc-crm.org/cidoc-crm/E53_Place> ;
    owl:inverseOf <http://www.cidoc-crm.org/extensions/crmsci/O21i_witnessed_encounter> .

<http://www.cidoc-crm.org/extensions/crmsci/O21i_witnessed_encounter> a rdf:Property ;
    rdfs:label "witnessed encounter"@en ;
    rdfs:domain <http://www.cidoc-crm.org/cidoc-crm/E53_Place> ;
    rdfs:range <http://www.cidoc-crm.org/extensions/crmsci/S19_Encounter_Event> ;
    owl:inverseOf <http://www.cidoc-crm.org/extensions/crmsci/O21_encountered_at> .

<http://www.cidoc-crm.org/extensions/crmsci/O23_is_defined_by> a rdf:Property ;
    rdfs:label "is defined by"@en ;
    rdfs:comment "This property identifies the E92 Spacetime Volume that defines a S22 Segment of Matter. The spatial boundaries of the E92 Spacetime Volume are defined through S4 Observation or declaration while the temporal boundaries are confined by S18 Alteration events."@en ;
    rdfs:domain <http://www.cidoc-crm.org/extensions/crmsci/S22_Segment_of_Matter> ;
    rdfs:range <http://www.cidoc-crm.org/cidoc-crm/E92_Spacetime_Volume> ;
    owl:inverseOf <http://www.cidoc-crm.org/extensions/crmsci/O23i_defines> .

<http://www.cidoc-crm.org/extensions/crmsci/O23i_defines> a rdf:Property ;
    rdfs:label "defines"@en ;
    rdfs:domain <http://www.cidoc-crm.org/cidoc-crm/E92_Spacetime_Volume> ;
    rdfs:range <http://www.cidoc-crm.org/extensions/crmsci/S22_Segment_of_Matter> ;
    owl:inverseOf <http://www.cidoc-crm.org/extensions/crmsci/O23_is_defined_by> .

<http://www.cidoc-crm.org/extensions/crmsci/O27_split> a rdf:Property ;
    rdfs:label "split"@en ;
    rdfs:comment "This property associates an instance of S24 Sample Splitting with the instance of S13 Sample which is the original sample being split."@en ;
    rdfs:domain <http://www.cidoc-crm.org/extensions/crmsci/S24_Sample_Splitting> ;
    rdfs:range <http://www.cidoc-crm.org/extensions/crmsci/S13_Sample> ;
    rdfs:subPropertyOf <http://www.cidoc-crm.org/extensions/crmsci/O3_sampled_from> ;
    owl:inverseOf <http://www.cidoc-crm.org/extensions/crmsci/O27i_was_source_for> .

<http://www.cidoc-crm.org/extensions/crmsci/O27i_was_source_for> a rdf:Property ;
    rdfs:label "was source for"@en ;
    rdfs:domain <http://www.cidoc-crm.org/extensions/crmsci/S13_Sample> ;
    rdfs:range <http://www.cidoc-crm.org/extensions/crmsci/S24_Sample_Splitting> ;
    rdfs:subPropertyOf <http://www.cidoc-crm.org/extensions/crmsci/O3i_was_sample_by> ;
    owl:inverseOf <http://www.cidoc-crm.org/extensions/crmsci/O27_split> .

<http://www.cidoc-crm.org/extensions/crmsci/O28_is_conceptually_greater_than> a rdf:Property ;
    rdfs:label "is conceptually greater than"@en ;
    rdfs:comment "This property allows an instance of E55 Type from a particular concept scheme or vocabulary to be declared as having an order relative to other instances of E55 Type in the same or other concept schemes, without necessarily having a specific value associated with either instance. This allows, for example, for an E55 Type instance representing the concept of \"good\" in a conservation report vocabulary to be greater than the E55 Type instance representing the concept of \"average\" in the same vocabulary. This property is transitive, and thus if \"average\" is greater than \"poor\", then \"good\" is also greater than \"poor\". In the domain of statistics, types that participate in this kind of relationship are called \"Ordinal Variables\"; as opposed to those without order which are called \"Nominal Variables\". This property allows for queries that select based on the relative position of participating E55 Types."@en ;
    rdfs:domain <http://www.cidoc-crm.org/cidoc-crm/E55_Type> ;
    rdfs:range <http://www.cidoc-crm.org/cidoc-crm/E55_Type> ;
    owl:inverseOf <http://www.cidoc-crm.org/extensions/crmsci/O28i_is_conceptually_less_than> .

<http://www.cidoc-crm.org/extensions/crmsci/O28i_is_conceptually_less_than> a rdf:Property ;
    rdfs:label "is conceptually less than"@en ;
    rdfs:domain <http://www.cidoc-crm.org/cidoc-crm/E55_Type> ;
    rdfs:range <http://www.cidoc-crm.org/cidoc-crm/E55_Type> ;
    owl:inverseOf <http://www.cidoc-crm.org/extensions/crmsci/O28_is_conceptually_greater_than> .

<http://www.cidoc-crm.org/extensions/crmsci/O29_removed_sub-sample> a rdf:Property ;
    rdfs:label "removed sub-sample"@en ;
    rdfs:comment "This property associates an instance of S24 Sample Splitting with the resulting instance of S13 Sample that has been removed from the original sample. The new sample (i.e. the sub-sample) maintains the characteristic qualities of the original."@en ;
    rdfs:domain <http://www.cidoc-crm.org/extensions/crmsci/S24_Sample_Splitting> ;
    rdfs:range <http://www.cidoc-crm.org/extensions/crmsci/S13_Sample> ;
    rdfs:subPropertyOf <http://www.cidoc-crm.org/extensions/crmsci/O5_removed> ;
    owl:inverseOf <http://www.cidoc-crm.org/extensions/crmsci/O29i_was_sub-sample_removed_by> .

<http://www.cidoc-crm.org/extensions/crmsci/O29i_was_sub-sample_removed_by> a rdf:Property ;
    rdfs:label "was sub-sample removed by"@en ;
    rdfs:domain <http://www.cidoc-crm.org/extensions/crmsci/S13_Sample> ;
    rdfs:range <http://www.cidoc-crm.org/extensions/crmsci/S24_Sample_Splitting> ;
    rdfs:subPropertyOf <http://www.cidoc-crm.org/extensions/crmsci/O5i_was_removed_by> ;
    owl:inverseOf <http://www.cidoc-crm.org/extensions/crmsci/O29_removed_sub-sample> .

<http://www.cidoc-crm.org/extensions/crmsci/O31_has_validity_time-span> a rdf:Property ;
    rdfs:label "has validity time-span"@en ;
    rdfs:comment "This property associates an instance of S23 Position Determination with the instance of E52 Time-Span for which the determination is valid according to the observer at the time of the observation. No inferences can be made in relation to the validity of the determination outside this time-span despite the fact that some entities are relatively stable and their positions may remain the same after the determination. The time-span of validity should fall within the overall time-span of the process of determination."@en ;
    rdfs:domain <http://www.cidoc-crm.org/extensions/crmsci/S23_Position_Determination> ;
    rdfs:range <http://www.cidoc-crm.org/cidoc-crm/E52_Time-Span> ;
    rdfs:subPropertyOf <http://www.cidoc-crm.org/cidoc-crm/P4_has_time-span> ;
    owl:inverseOf <http://www.cidoc-crm.org/extensions/crmsci/O31i_is_time-span_validity_for> .

<http://www.cidoc-crm.org/extensions/crmsci/O31i_is_time-span_validity_for> a rdf:Property ;
    rdfs:label "is time-span validity for"@en ;
    rdfs:domain <http://www.cidoc-crm.org/cidoc-crm/E52_Time-Span> ;
    rdfs:range <http://www.cidoc-crm.org/extensions/crmsci/S23_Position_Determination> ;
    rdfs:subPropertyOf <http://www.cidoc-crm.org/cidoc-crm/P4i_is_time-span_of> ;
    owl:inverseOf <http://www.cidoc-crm.org/extensions/crmsci/O31_has_validity_time-span> .

<http://www.cidoc-crm.org/extensions/crmsci/O32_determined_position_of> a rdf:Property ;
    rdfs:label "determined position of"@en ;
    rdfs:comment "This property connects an instance of S23 Position Determination with the instance of S15 Observable Entity whose position is being determined."@en ;
    rdfs:domain <http://www.cidoc-crm.org/extensions/crmsci/S23_Position_Determination> ;
    rdfs:range <http://www.cidoc-crm.org/extensions/crmsci/S15_Observable_Entity> ;
    rdfs:subPropertyOf <http://www.cidoc-crm.org/extensions/crmsci/O8_observed> ;
    owl:inverseOf <http://www.cidoc-crm.org/extensions/crmsci/O32i_was_located_by> .

<http://www.cidoc-crm.org/extensions/crmsci/O32i_was_located_by> a rdf:Property ;
    rdfs:label "was located by"@en ;
    rdfs:domain <http://www.cidoc-crm.org/extensions/crmsci/S15_Observable_Entity> ;
    rdfs:range <http://www.cidoc-crm.org/extensions/crmsci/S23_Position_Determination> ;
    rdfs:subPropertyOf <http://www.cidoc-crm.org/extensions/crmsci/O8i_was_observed_by> ;
    owl:inverseOf <http://www.cidoc-crm.org/extensions/crmsci/O32_determined_position_of> .

<http://www.cidoc-crm.org/extensions/crmsci/O4_sampled_at> a rdf:Property ;
    rdfs:label "sampled at"@en ;
    rdfs:comment "This property associates an instance of S2 Sample Taking with the instance of E53 Place (\"spot\") at which this activity sampled. It identifies the narrowest relevant area on the material substantial from which the sample was taken. This may be known or given in absolute terms or relative to an instance of the material substantial from which it was taken. If samples are taken from more than one spot, the sample taking activity must be documented by separate instances for each spot. The property P7 took place at, inherited from E4 Period, describes the position of the area in which the sampling activity occurred; this latter comprises the space within which operators and instruments were contained during the activity, and the sample taking spot."@en ;
    rdfs:domain <http://www.cidoc-crm.org/extensions/crmsci/S2_Sample_Taking> ;
    rdfs:range <http://www.cidoc-crm.org/cidoc-crm/E53_Place> ;
    owl:inverseOf <http://www.cidoc-crm.org/extensions/crmsci/O4i_was_sampling_location_of> .

<http://www.cidoc-crm.org/extensions/crmsci/O4i_was_sampling_location_of> a rdf:Property ;
    rdfs:label "was sampling location of"@en ;
    rdfs:domain <http://www.cidoc-crm.org/cidoc-crm/E53_Place> ;
    rdfs:range <http://www.cidoc-crm.org/extensions/crmsci/S2_Sample_Taking> ;
    owl:inverseOf <http://www.cidoc-crm.org/extensions/crmsci/O4_sampled_at> .

<http://www.cidoc-crm.org/extensions/crmsci/O6_is_former_or_current_part_of> a rdf:Property ;
    rdfs:label "is former or current part of"@en ;
    rdfs:comment "This property associates an instance of S12 Amount of Fluid with an instance of S14 Fluid Body which formed or forms part of it. It allows instances of S14 Fluid Body to be analyzed into elements of S12 Amount of Fluid."@en ;
    rdfs:domain <http://www.cidoc-crm.org/extensions/crmsci/S12_Amount_of_Fluid> ;
    rdfs:range <http://www.cidoc-crm.org/extensions/crmsci/S14_Fluid_Body> ;
    rdfs:subPropertyOf <http://www.cidoc-crm.org/extensions/crmsci/O25_contains> ;
    owl:inverseOf <http://www.cidoc-crm.org/extensions/crmsci/O6i_has_former_or_current_part> .

<http://www.cidoc-crm.org/extensions/crmsci/O6i_has_former_or_current_part> a rdf:Property ;
    rdfs:label "has former or current part"@en ;
    rdfs:domain <http://www.cidoc-crm.org/extensions/crmsci/S14_Fluid_Body> ;
    rdfs:range <http://www.cidoc-crm.org/extensions/crmsci/S12_Amount_of_Fluid> ;
    rdfs:subPropertyOf <http://www.cidoc-crm.org/extensions/crmsci/O25i_is_contained_in> ;
    owl:inverseOf <http://www.cidoc-crm.org/extensions/crmsci/O6_is_former_or_current_part_of> .

<http://www.cidoc-crm.org/extensions/crmsci/O7_confines> a rdf:Property ;
    rdfs:label "confines"@en ;
    rdfs:comment "This property associates an instance of S20 Rigid Physical Feature with an instance of S10 Material Substantial that it partially or completely confines. It describes cases in which rigid features such as stratigraphic layers, walls, dams, riverbeds, etc. form the boundaries of some item such as another stratigraphic layer or the waters of a river."@en ;
    rdfs:domain <http://www.cidoc-crm.org/extensions/crmsci/S20_Rigid_Physical_Feature> ;
    rdfs:range <http://www.cidoc-crm.org/extensions/crmsci/S10_Material_Substantial> ;
    rdfs:subPropertyOf <http://www.cidoc-crm.org/extensions/crmarchaeo/AP12_confines> ;
    owl:inverseOf <http://www.cidoc-crm.org/extensions/crmsci/O7i_is_confined_by> .

<http://www.cidoc-crm.org/extensions/crmsci/O7i_is_confined_by> a rdf:Property ;
    rdfs:label "is confined by"@en ;
    rdfs:domain <http://www.cidoc-crm.org/extensions/crmsci/S10_Material_Substantial> ;
    rdfs:range <http://www.cidoc-crm.org/extensions/crmsci/S20_Rigid_Physical_Feature> ;
    rdfs:subPropertyOf <http://www.cidoc-crm.org/extensions/crmarchaeo/AP12i_is_confined_by> ;
    owl:inverseOf <http://www.cidoc-crm.org/extensions/crmsci/O7_confines> .

<http://www.cidoc-crm.org/extensions/crmsci/O9_observed_property_type> a rdf:Property ;
    rdfs:label "observed property type"@en ;
    rdfs:comment "This property associates an instance of S4 Observation with the instance of S9 Property Type for which the observation provides a value or evidence, such as “concentration of nitrate” observed in the water from a particular borehole. Encoding the observed property by type, observed entity and value (properties O9, O10, O16) is a method to circumscribe the reification of the observed property by the respective instance of S4 Observation. In an RDFS encoding, this circumscription can be transformed into an explicit representation of the observed property in terms of a formal ontology either by use of a reification construct or by the use of a Named Graph containing the observed property. The latter representation allows for more formal reasoning with the model, the former is more flexible about the kinds of observations."@en ;
    rdfs:domain <http://www.cidoc-crm.org/extensions/crmsci/S4_Observation> ;
    rdfs:range <http://www.cidoc-crm.org/extensions/crmsci/S9_Property_Type> ;
    rdfs:subPropertyOf <http://www.cidoc-crm.org/cidoc-crm/P177_assigned_property_of_type> ;
    owl:inverseOf <http://www.cidoc-crm.org/extensions/crmsci/O9i_property_type_was_observed_by> .

<http://www.cidoc-crm.org/extensions/crmsci/O9i_property_type_was_observed_by> a rdf:Property ;
    rdfs:label "property type was observed by"@en ;
    rdfs:domain <http://www.cidoc-crm.org/extensions/crmsci/S9_Property_Type> ;
    rdfs:range <http://www.cidoc-crm.org/extensions/crmsci/S4_Observation> ;
    rdfs:subPropertyOf <http://www.cidoc-crm.org/cidoc-crm/P177i_is_type_of_property_assigned> ;
    owl:inverseOf <http://www.cidoc-crm.org/extensions/crmsci/O9_observed_property_type> .

<http://www.cidoc-crm.org/extensions/crmtex/TXP10_deciphered_text> a rdf:Property ;
    rdfs:label "deciphered text"@en ;
    rdfs:comment "This property associates an instance of TX5 Text Recognition with an instance of E24 Physical Human-Made Thing carrying a glyph or a sequence of glyphs that was recognized in the respective activity of text recognition. Typically, the associated instance of E24 Physical Human-Made Thing is more specifically an instance of TX1 Written Text, however, a text may also be recognized from a mechanical copy, a photograph, squeeze or other form of material copy of a written original, which would not by itself constitute an instance of TX1 Written Text. In the latter case, the material copy should be associated with the original written text using the property ‘P130 shows features’. If the text was actually recognized only from a digital representation, this property should not be used, rather the property TXP13 deciphered via the representation should be used instead."@en ;
    rdfs:domain <http://www.cidoc-crm.org/extensions/crmtex/TX5_Text_Recognition> ;
    rdfs:range <http://www.cidoc-crm.org/cidoc-crm/E24_Physical_Human-Made_Thing> ;
    rdfs:subPropertyOf <http://www.cidoc-crm.org/extensions/crmsci/O8_observed> ;
    owl:inverseOf <http://www.cidoc-crm.org/extensions/crmtex/TXP10i_was_deciphered_by> .

<http://www.cidoc-crm.org/extensions/crmtex/TXP10i_was_deciphered_by> a rdf:Property ;
    rdfs:label "was deciphered by"@en ;
    rdfs:domain <http://www.cidoc-crm.org/cidoc-crm/E24_Physical_Human-Made_Thing> ;
    rdfs:range <http://www.cidoc-crm.org/extensions/crmtex/TX5_Text_Recognition> ;
    rdfs:subPropertyOf <http://www.cidoc-crm.org/extensions/crmsci/O8i_was_observed_by> ;
    owl:inverseOf <http://www.cidoc-crm.org/extensions/crmtex/TXP10_deciphered_text> .

<http://www.cidoc-crm.org/extensions/crmtex/TXP11_transcribed> a rdf:Property ;
    rdfs:label "transcribed"@en ;
    rdfs:comment "This property describes the relation between an activity of TX6 Transliteration and the identified sequence of graphemes (TX12) represented in an instance of TX1 Written Text."@en ;
    rdfs:domain <http://www.cidoc-crm.org/extensions/crmtex/TX6_Transliteration> ;
    rdfs:range <http://www.cidoc-crm.org/extensions/crmtex/TX12_Grapheme_Sequence> ;
    rdfs:subPropertyOf <http://www.cidoc-crm.org/cidoc-crm/P16_used_specific_object> ;
    owl:inverseOf <http://www.cidoc-crm.org/extensions/crmtex/TXP11i_was_transcribed_by> .

<http://www.cidoc-crm.org/extensions/crmtex/TXP11i_was_transcribed_by> a rdf:Property ;
    rdfs:label "was transcribed by"@en ;
    rdfs:domain <http://www.cidoc-crm.org/extensions/crmtex/TX12_Grapheme_Sequence> ;
    rdfs:range <http://www.cidoc-crm.org/extensions/crmtex/TX6_Transliteration> ;
    rdfs:subPropertyOf <http://www.cidoc-crm.org/cidoc-crm/P16i_was_used_for> ;
    owl:inverseOf <http://www.cidoc-crm.org/extensions/crmtex/TXP11_transcribed> .

<http://www.cidoc-crm.org/extensions/crmtex/TXP12_has_style> a rdf:Property ;
    rdfs:label "has style"@en ;
    rdfs:comment "This property describes information about the style used for the realization of the written text (TX1). The property TXP12.1 has type allows the nature of the style to be specified, for example to record the direction, orientation or the linear system of the text."@en ;
    rdfs:domain <http://www.cidoc-crm.org/extensions/crmtex/TX1_Written_Text> ;
    rdfs:range <http://www.cidoc-crm.org/extensions/crmtex/TX10_Style> ;
    rdfs:subPropertyOf <http://www.cidoc-crm.org/cidoc-crm/P33_used_specific_technique> ;
    owl:inverseOf <http://www.cidoc-crm.org/extensions/crmtex/TXP12i_is_style_of> .

<http://www.cidoc-crm.org/extensions/crmtex/TXP12i_is_style_of> a rdf:Property ;
    rdfs:label "is style of"@en ;
    rdfs:domain <http://www.cidoc-crm.org/extensions/crmtex/TX10_Style> ;
    rdfs:range <http://www.cidoc-crm.org/extensions/crmtex/TX1_Written_Text> ;
    rdfs:subPropertyOf <http://www.cidoc-crm.org/cidoc-crm/P33i_was_used_by> ;
    owl:inverseOf <http://www.cidoc-crm.org/extensions/crmtex/TXP12_has_style> .

<http://www.cidoc-crm.org/extensions/crmtex/TXP13_deciphered_via_the_representation> a rdf:Property ;
    rdfs:label "deciphered via the representation"@en ;
    rdfs:comment "This property associates an instance of TX5 Text Recognition with an instance of E36 Visual Item, capturing the optical impression of an instance of TX1 Written Text by some mechanical method, that was used for recognizing the text without access to the original text and without an explicitly documented material copy or electronic display device that was used for the process. If the text was actually recognized from an autoptic recognition or from a material reproduction, this property may not be used but the property “TXP10 deciphered text (was deciphered by)” should be used instead. This property should also not be used, if the recognition of the text was actually carried out from the original text or a material copy of it together with an auxiliary instance of E36 Visual Item. In this case, the use of the auxiliary material should be documented with the more general property P16 used specific object."@en ;
    rdfs:domain <http://www.cidoc-crm.org/extensions/crmtex/TX5_Text_Recognition> ;
    rdfs:range <http://www.cidoc-crm.org/cidoc-crm/E36_Visual_Item> ;
    rdfs:subPropertyOf <http://www.cidoc-crm.org/cidoc-crm/P16_used_specific_object> ;
    owl:inverseOf <http://www.cidoc-crm.org/extensions/crmtex/TXP13i_was_representation_used_for_deciphering> .

<http://www.cidoc-crm.org/extensions/crmtex/TXP13i_was_representation_used_for_deciphering> a rdf:Property ;
    rdfs:label "was representation used for deciphering"@en ;
    rdfs:domain <http://www.cidoc-crm.org/cidoc-crm/E36_Visual_Item> ;
    rdfs:range <http://www.cidoc-crm.org/extensions/crmtex/TX5_Text_Recognition> ;
    rdfs:subPropertyOf <http://www.cidoc-crm.org/cidoc-crm/P16i_was_used_for> ;
    owl:inverseOf <http://www.cidoc-crm.org/extensions/crmtex/TXP13_deciphered_via_the_representation> .

<http://www.cidoc-crm.org/extensions/crmtex/TXP14_used_copy_or_representation_of> a rdf:Property ;
    rdfs:label "used copy or representation of"@en ;
    rdfs:comment "This property associates an instance of TX5 Text Recognition, carried out only via copies or representations of a text, with the original instance of TX1 Written Text that was represented on the used copies or digital surrogates. This property is to be used only for non-autoptic recognition. If this particular recognition of the text was actually carried out from the original text, the property TXP10 deciphered text should be used for associating the instance of TX5 Text Recognition with the original instance of TX1 Written Text. If some form of material copy of the written text was used for the text recognition, then this material copy should be associated with the original written text using the property ‘P130 shows features of’."@en ;
    rdfs:domain <http://www.cidoc-crm.org/extensions/crmtex/TX5_Text_Recognition> ;
    rdfs:range <http://www.cidoc-crm.org/extensions/crmtex/TX1_Written_Text> ;
    rdfs:subPropertyOf <http://www.cidoc-crm.org/cidoc-crm/P16_used_specific_object> ;
    owl:inverseOf <http://www.cidoc-crm.org/extensions/crmtex/TXP14i_was_deciphered_via_copy_or_representation> .

<http://www.cidoc-crm.org/extensions/crmtex/TXP14i_was_deciphered_via_copy_or_representation> a rdf:Property ;
    rdfs:label "was deciphered via copy or representation"@en ;
    rdfs:domain <http://www.cidoc-crm.org/extensions/crmtex/TX1_Written_Text> ;
    rdfs:range <http://www.cidoc-crm.org/extensions/crmtex/TX5_Text_Recognition> ;
    rdfs:subPropertyOf <http://www.cidoc-crm.org/cidoc-crm/P16i_was_used_for> ;
    owl:inverseOf <http://www.cidoc-crm.org/extensions/crmtex/TXP14_used_copy_or_representation_of> .

<http://www.cidoc-crm.org/extensions/crmtex/TXP15_recorded_correspondence> a rdf:Property ;
    rdfs:label "recorded correspondence"@en ;
    rdfs:comment "This property associates an instance of TX5 Text Recognition with an instance of TX12 Grapheme Sequence that was created by this activity of text recognition for recording and representing as faithfully as possible the exact value of each sign on the physical material of the recognized instance of TX1 Written Text."@en ;
    rdfs:domain <http://www.cidoc-crm.org/extensions/crmtex/TX5_Text_Recognition> ;
    rdfs:range <http://www.cidoc-crm.org/extensions/crmtex/TX12_Grapheme_Sequence> ;
    rdfs:subPropertyOf <http://www.cidoc-crm.org/cidoc-crm/P94_has_created> ;
    owl:inverseOf <http://www.cidoc-crm.org/extensions/crmtex/TXP15i_was_recorded_by> .

<http://www.cidoc-crm.org/extensions/crmtex/TXP15i_was_recorded_by> a rdf:Property ;
    rdfs:label "was recorded by"@en ;
    rdfs:domain <http://www.cidoc-crm.org/extensions/crmtex/TX12_Grapheme_Sequence> ;
    rdfs:range <http://www.cidoc-crm.org/extensions/crmtex/TX5_Text_Recognition> ;
    rdfs:subPropertyOf <http://www.cidoc-crm.org/cidoc-crm/P94i_was_created_by> ;
    owl:inverseOf <http://www.cidoc-crm.org/extensions/crmtex/TXP15_recorded_correspondence> .

<http://www.cidoc-crm.org/extensions/crmtex/TXP16_employs_script> a rdf:Property ;
    rdfs:label "employs script"@en ;
    rdfs:comment "This property associates an instance of TX3 Writing System with one of the instances of the script (TX13) it employs."@en ;
    rdfs:domain <http://www.cidoc-crm.org/extensions/crmtex/TX3_Writing_System> ;
    rdfs:range <http://www.cidoc-crm.org/extensions/crmtex/TX13_Script> ;
    rdfs:subPropertyOf <http://www.cidoc-crm.org/cidoc-crm/P148_has_component> ;
    owl:inverseOf <http://www.cidoc-crm.org/extensions/crmtex/TXP16i_is_employed_by> .

<http://www.cidoc-crm.org/extensions/crmtex/TXP16i_is_employed_by> a rdf:Property ;
    rdfs:label "is employed by"@en ;
    rdfs:domain <http://www.cidoc-crm.org/extensions/crmtex/TX13_Script> ;
    rdfs:range <http://www.cidoc-crm.org/extensions/crmtex/TX3_Writing_System> ;
    rdfs:subPropertyOf <http://www.cidoc-crm.org/cidoc-crm/P148i_is_component_of> ;
    owl:inverseOf <http://www.cidoc-crm.org/extensions/crmtex/TXP16_employs_script> .

<http://www.cidoc-crm.org/extensions/crmtex/TXP17_has_part> a rdf:Property ;
    rdfs:label "has part"@en ;
    rdfs:comment "This property associates an instance of TX12 Grapheme Sequence with another instance of TX12 Grapheme Sequence appearing at a particular position of the sequence. The property can be also used by an instance of TX11 Grapheme Occurrence (subclass of TX12 Grapheme Sequence) for denoting that a grapheme occurrence has part another grapheme occurrence. Note that a grapheme occurrence may be a symbolic composite containing another grapheme occurrence, such as the minute character “e” on top of the character “u” in former German writing systems denoting the symbol for “ü”."@en ;
    rdfs:domain <http://www.cidoc-crm.org/extensions/crmtex/TX12_Grapheme_Sequence> ;
    rdfs:range <http://www.cidoc-crm.org/extensions/crmtex/TX12_Grapheme_Sequence> ;
    rdfs:subPropertyOf <http://www.cidoc-crm.org/cidoc-crm/P106_is_composed_of> ;
    owl:inverseOf <http://www.cidoc-crm.org/extensions/crmtex/TXP17i_forms_part_of> .

<http://www.cidoc-crm.org/extensions/crmtex/TXP17i_forms_part_of> a rdf:Property ;
    rdfs:label "forms part of"@en ;
    rdfs:domain <http://www.cidoc-crm.org/extensions/crmtex/TX12_Grapheme_Sequence> ;
    rdfs:range <http://www.cidoc-crm.org/extensions/crmtex/TX12_Grapheme_Sequence> ;
    rdfs:subPropertyOf <http://www.cidoc-crm.org/cidoc-crm/P106i_forms_part_of> ;
    owl:inverseOf <http://www.cidoc-crm.org/extensions/crmtex/TXP17_has_part> .

<http://www.cidoc-crm.org/extensions/crmtex/TXP18_read> a rdf:Property ;
    rdfs:label "read"@en ;
    rdfs:comment "This property associates an instance of TX14 Reading with an instance of TX1 Written Text whose linguistic meaning was interpreted/understood through the reading process. It is a shortcut of the fully developed path from TX14 Reading through P9 consists of , TX5 Text Recognition, TXP10 deciphered tex t, to TX1 Written Text."@en ;
    rdfs:domain <http://www.cidoc-crm.org/extensions/crmtex/TX14_Reading> ;
    rdfs:range <http://www.cidoc-crm.org/extensions/crmtex/TX1_Written_Text> ;
    rdfs:subPropertyOf <http://www.cidoc-crm.org/cidoc-crm/P16_used_specific_object> ;
    owl:inverseOf <http://www.cidoc-crm.org/extensions/crmtex/TXP18i_was_read_by> .

<http://www.cidoc-crm.org/extensions/crmtex/TXP18i_was_read_by> a rdf:Property ;
    rdfs:label "was read by"@en ;
    rdfs:domain <http://www.cidoc-crm.org/extensions/crmtex/TX1_Written_Text> ;
    rdfs:range <http://www.cidoc-crm.org/extensions/crmtex/TX14_Reading> ;
    rdfs:subPropertyOf <http://www.cidoc-crm.org/cidoc-crm/P16i_was_used_for> ;
    owl:inverseOf <http://www.cidoc-crm.org/extensions/crmtex/TXP18_read> .

<http://www.cidoc-crm.org/extensions/crmtex/TXP1_used_writing_system> a rdf:Property ;
    rdfs:label "used writing system"@en ;
    rdfs:comment "This property identifies the specific instance of TX3 Writing System employed during the writing event (TX2) that led to the creation of a written text (TX1)."@en ;
    rdfs:domain <http://www.cidoc-crm.org/extensions/crmtex/TX2_Writing> ;
    rdfs:range <http://www.cidoc-crm.org/extensions/crmtex/TX3_Writing_System> ;
    rdfs:subPropertyOf <http://www.cidoc-crm.org/cidoc-crm/P33_used_specific_technique> ;
    owl:inverseOf <http://www.cidoc-crm.org/extensions/crmtex/TXP1i_writing_system_used_for> .

<http://www.cidoc-crm.org/extensions/crmtex/TXP1i_writing_system_used_for> a rdf:Property ;
    rdfs:label "writing system used for"@en ;
    rdfs:domain <http://www.cidoc-crm.org/extensions/crmtex/TX3_Writing_System> ;
    rdfs:range <http://www.cidoc-crm.org/extensions/crmtex/TX2_Writing> ;
    rdfs:subPropertyOf <http://www.cidoc-crm.org/cidoc-crm/P33i_was_used_by> ;
    owl:inverseOf <http://www.cidoc-crm.org/extensions/crmtex/TXP1_used_writing_system> .

<http://www.cidoc-crm.org/extensions/crmtex/TXP2_includes> a rdf:Property ;
    rdfs:label "includes"@en ;
    rdfs:comment "This property describes the relation existing between a TX1 Written Text and the TX4 Writing Field, specifically created to accommodate the text, within which it is inscribed. This relation becomes quite relevant in the very frequent case where more than a single text is found on different areas of a specific support."@en ;
    rdfs:domain <http://www.cidoc-crm.org/extensions/crmtex/TX4_Writing_Field> ;
    rdfs:range <http://www.cidoc-crm.org/extensions/crmtex/TX1_Written_Text> ;
    rdfs:subPropertyOf <http://www.cidoc-crm.org/cidoc-crm/P56_bears_feature> ;
    owl:inverseOf <http://www.cidoc-crm.org/extensions/crmtex/TXP2i_is_included_within> .

<http://www.cidoc-crm.org/extensions/crmtex/TXP2i_is_included_within> a rdf:Property ;
    rdfs:label "is included within"@en ;
    rdfs:domain <http://www.cidoc-crm.org/extensions/crmtex/TX1_Written_Text> ;
    rdfs:range <http://www.cidoc-crm.org/extensions/crmtex/TX4_Writing_Field> ;
    rdfs:subPropertyOf <http://www.cidoc-crm.org/cidoc-crm/P56i_is_found_on> ;
    owl:inverseOf <http://www.cidoc-crm.org/extensions/crmtex/TXP2_includes> .

<http://www.cidoc-crm.org/extensions/crmtex/TXP4_has_segment> a rdf:Property ;
    rdfs:label "has segment"@en ;
    rdfs:comment "This property is intended to correlate a text and the different parts of it which a scholar can identify, such as: letters, words, lines, columns, pages, or any other scan that can be made by scholars because it is considered to have a particular relevance for the investigation of the text itself."@en ;
    rdfs:domain <http://www.cidoc-crm.org/extensions/crmtex/TX1_Written_Text> ;
    rdfs:range <http://www.cidoc-crm.org/extensions/crmtex/TX7_Written_Text_Segment> ;
    rdfs:subPropertyOf <http://www.cidoc-crm.org/cidoc-crm/P46_is_composed_of> ;
    owl:inverseOf <http://www.cidoc-crm.org/extensions/crmtex/TXP4i_is_segment_of> .

<http://www.cidoc-crm.org/extensions/crmtex/TXP4i_is_segment_of> a rdf:Property ;
    rdfs:label "is segment of"@en ;
    rdfs:domain <http://www.cidoc-crm.org/extensions/crmtex/TX7_Written_Text_Segment> ;
    rdfs:range <http://www.cidoc-crm.org/extensions/crmtex/TX1_Written_Text> ;
    rdfs:subPropertyOf <http://www.cidoc-crm.org/cidoc-crm/P46i_forms_part_of> ;
    owl:inverseOf <http://www.cidoc-crm.org/extensions/crmtex/TXP4_has_segment> .

<http://www.cidoc-crm.org/extensions/crmtex/TXP5_wrote> a rdf:Property ;
    rdfs:label "wrote"@en ;
    rdfs:comment "This property is used to describe in detail the close relationship between a text and the writing event that led to its production."@en ;
    rdfs:domain <http://www.cidoc-crm.org/extensions/crmtex/TX2_Writing> ;
    rdfs:range <http://www.cidoc-crm.org/extensions/crmtex/TX1_Written_Text> ;
    rdfs:subPropertyOf <http://www.cidoc-crm.org/cidoc-crm/P108_has_produced> ;
    owl:inverseOf <http://www.cidoc-crm.org/extensions/crmtex/TXP5i_was_written_by> .

<http://www.cidoc-crm.org/extensions/crmtex/TXP5i_was_written_by> a rdf:Property ;
    rdfs:label "was written by"@en ;
    rdfs:domain <http://www.cidoc-crm.org/extensions/crmtex/TX1_Written_Text> ;
    rdfs:range <http://www.cidoc-crm.org/extensions/crmtex/TX2_Writing> ;
    rdfs:subPropertyOf <http://www.cidoc-crm.org/cidoc-crm/P108i_was_produced_by> ;
    owl:inverseOf <http://www.cidoc-crm.org/extensions/crmtex/TXP5_wrote> .

<http://www.cidoc-crm.org/extensions/crmtex/TXP6_encodes> a rdf:Property ;
    rdfs:label "encodes"@en ;
    rdfs:comment "This property is used to indicate the language encoded by the TX3 Writing System and used for writing, reading or rendering (i.e. transcribing) a TX1 Written Text."@en ;
    rdfs:domain <http://www.cidoc-crm.org/extensions/crmtex/TX3_Writing_System> ;
    rdfs:range <http://www.cidoc-crm.org/cidoc-crm/E56_Language> ;
    rdfs:subPropertyOf <http://www.cidoc-crm.org/cidoc-crm/P2_has_type> ;
    owl:inverseOf <http://www.cidoc-crm.org/extensions/crmtex/TXP6i_is_encoding_of> .

<http://www.cidoc-crm.org/extensions/crmtex/TXP6i_is_encoding_of> a rdf:Property ;
    rdfs:label "is encoding of"@en ;
    rdfs:domain <http://www.cidoc-crm.org/cidoc-crm/E56_Language> ;
    rdfs:range <http://www.cidoc-crm.org/extensions/crmtex/TX3_Writing_System> ;
    rdfs:subPropertyOf <http://www.cidoc-crm.org/cidoc-crm/P2i_is_type_of> ;
    owl:inverseOf <http://www.cidoc-crm.org/extensions/crmtex/TXP6_encodes> .

<http://www.cidoc-crm.org/extensions/crmtex/TXP7_has_item> a rdf:Property ;
    rdfs:label "has item"@en ;
    rdfs:comment "This property associates an instance of TX13 Script with an instance of TX8 Grapheme employed by this script. Different instances of TX13 Script may have some graphemes in common."@en ;
    rdfs:domain <http://www.cidoc-crm.org/extensions/crmtex/TX13_Script> ;
    rdfs:range <http://www.cidoc-crm.org/extensions/crmtex/TX8_Grapheme> ;
    rdfs:subPropertyOf <http://www.cidoc-crm.org/cidoc-crm/P67_refers_to> ;
    owl:inverseOf <http://www.cidoc-crm.org/extensions/crmtex/TXP7i_is_item_of> .

<http://www.cidoc-crm.org/extensions/crmtex/TXP7i_is_item_of> a rdf:Property ;
    rdfs:label "is item of"@en ;
    rdfs:domain <http://www.cidoc-crm.org/extensions/crmtex/TX8_Grapheme> ;
    rdfs:range <http://www.cidoc-crm.org/extensions/crmtex/TX13_Script> ;
    rdfs:subPropertyOf <http://www.cidoc-crm.org/cidoc-crm/P67i_is_referred_to_by> ;
    owl:inverseOf <http://www.cidoc-crm.org/extensions/crmtex/TXP7_has_item> .

<http://www.cidoc-crm.org/extensions/crmtex/TXP8_has_component> a rdf:Property ;
    rdfs:label "has component"@en ;
    rdfs:comment "This property is used to state the (physical) belonging of a glyph to a given TX1 Written Text."@en ;
    rdfs:domain <http://www.cidoc-crm.org/extensions/crmtex/TX1_Written_Text> ;
    rdfs:range <http://www.cidoc-crm.org/extensions/crmtex/TX9_Glyph> ;
    rdfs:subPropertyOf <http://www.cidoc-crm.org/cidoc-crm/P46_is_composed_of> ;
    owl:inverseOf <http://www.cidoc-crm.org/extensions/crmtex/TXP8i_is_component_of> .

<http://www.cidoc-crm.org/extensions/crmtex/TXP8i_is_component_of> a rdf:Property ;
    rdfs:label "is component of"@en ;
    rdfs:domain <http://www.cidoc-crm.org/extensions/crmtex/TX9_Glyph> ;
    rdfs:range <http://www.cidoc-crm.org/extensions/crmtex/TX1_Written_Text> ;
    rdfs:subPropertyOf <http://www.cidoc-crm.org/cidoc-crm/P46i_forms_part_of> ;
    owl:inverseOf <http://www.cidoc-crm.org/extensions/crmtex/TXP8_has_component> .

<http://www.cidoc-crm.org/extensions/crmtex/TXP9_is_encoded_using> a rdf:Property ;
    rdfs:label "is encoded using"@en ;
    rdfs:comment "This property has the purpose of directly associating a TX1 Written Text with the TX3 Writing System used for encoding it. It is a shortcut of the more fully articulated path from TX1 Written Text through TXP5i was written by , TX2 Writing, TXP1 used writing system to TX3 Writing System."@en ;
    rdfs:domain <http://www.cidoc-crm.org/extensions/crmtex/TX1_Written_Text> ;
    rdfs:range <http://www.cidoc-crm.org/extensions/crmtex/TX3_Writing_System> ;
    owl:inverseOf <http://www.cidoc-crm.org/extensions/crmtex/TXP9i_was_used_to_encode> .

<http://www.cidoc-crm.org/extensions/crmtex/TXP9i_was_used_to_encode> a rdf:Property ;
    rdfs:label "was used to encode"@en ;
    rdfs:domain <http://www.cidoc-crm.org/extensions/crmtex/TX3_Writing_System> ;
    rdfs:range <http://www.cidoc-crm.org/extensions/crmtex/TX1_Written_Text> ;
    owl:inverseOf <http://www.cidoc-crm.org/extensions/crmtex/TXP9_is_encoded_using> .

<http://www.ics.forth.gr/isl/CRMdig/L2_used_as_source> a rdf:Property ;
    rdfs:comment """This property associates an instance of D10 Software Execution with an instance of D1 Digital Object
 which is used as a source, a software essential for the performance.  
This property is a specialisation of L10F had input (was input of).
	"""@en ;
    rdfs:domain <http://www.ics.forth.gr/isl/CRMdig/D10_Software_Execution> ;
    rdfs:range <http://www.ics.forth.gr/isl/CRMdig/D1_Digital_Object> ;
    rdfs:subPropertyOf <http://www.ics.forth.gr/isl/CRMdig/L10_had_input> .

<http://www.ics.forth.gr/isl/CRMdig/L2i_was_source_for> a rdf:Property ;
    rdfs:domain <http://www.ics.forth.gr/isl/CRMdig/D1_Digital_Object> ;
    rdfs:range <http://www.ics.forth.gr/isl/CRMdig/D10_Software_Execution> ;
    rdfs:subPropertyOf <http://www.ics.forth.gr/isl/CRMdig/L10i_was_input_of> .

<http://www.ics.forth.gr/isl/CRMdig/L4_has_preferred_label> a rdf:Property ;
    rdfs:comment """This property associates an instance of E1 Entity with an instance of resource used as a preferred lexical label.  
This property is a specialisation of rdf schema label.
"""@en ;
    rdfs:domain <http://www.cidoc-crm.org/cidoc-crm/E1_CRM_Entity> ;
    rdfs:range rdfs:Literal ;
    rdfs:subPropertyOf rdfs:label .

<https://ontology.swissartresearch.net/aaao/ZP103_ascribes_social_relation_target> a rdf:Property ;
    rdfs:label "ascribes social relation target"@en ;
    rdfs:comment "This property is used to indicate the person with whom the subject of the social relation status has the social relation which they have."@en ;
    rdfs:domain <https://ontology.swissartresearch.net/aaao/ZE55_Social_Relation_Status> ;
    rdfs:range <http://www.cidoc-crm.org/cidoc-crm/E39_Actor> ;
    rdfs:subPropertyOf <https://ontology.swissartresearch.net/aaao/ZP2_ascribes_intentional_target> ;
    skos:notation "ZP103"^^xsd:string .

<https://ontology.swissartresearch.net/aaao/ZP104_ascribes_social_relation> a rdf:Property ;
    rdfs:label "ascribes social relation"@en ;
    rdfs:comment "This property is used to indicate the specific type of social relation status which is indicated as holding between the subject individual and their ascribed social relative."@en ;
    rdfs:domain <https://ontology.swissartresearch.net/aaao/ZE55_Social_Relation_Status> ;
    rdfs:range <http://www.cidoc-crm.org/cidoc-crm/E55_Type> ;
    rdfs:subPropertyOf <https://ontology.swissartresearch.net/aaao/ZP3_ascribes_intentional_relation> ;
    skos:notation "ZP104"^^xsd:string .

<https://ontology.swissartresearch.net/aaao/ZP105_has_social_relation_subject> a rdf:Property ;
    rdfs:label "has social relation subject"@en ;
    rdfs:comment "This property is used to indicate the person for whom the social relation status is taken to hold."@en ;
    rdfs:domain <https://ontology.swissartresearch.net/aaao/ZE55_Social_Relation_Status> ;
    rdfs:range <http://www.cidoc-crm.org/cidoc-crm/E39_Actor> ;
    rdfs:subPropertyOf <https://ontology.swissartresearch.net/aaao/ZP1_has_intentional_subject> ;
    skos:notation "ZP105"^^xsd:string .

<https://ontology.swissartresearch.net/aaao/ZP111_initiated> a rdf:Property ;
    rdfs:label "initiated"@en ;
    rdfs:comment "This property is used to connect the instance of event to the instance of institutional fact which it brought into existence by fiat thanks to its accordance to a socially defined norm. In this case the bringing about of a new institutional fact need not be intentional or following any particular rule intentionally. Rather, within a social context it is recognized that the very fact of a particular event occurring is causal to the initiation of the related social fact. For example, in certain property right laws, the very fact of writing down an idea (E65 Creation) initiates an instance of property right over the generated information object, regardless of the intention or not of the author to so create such a right."@en ;
    rdfs:domain <http://www.cidoc-crm.org/cidoc-crm/E5_Event> ;
    rdfs:range <https://ontology.swissartresearch.net/aaao/ZE1_Institutional_Fact> ;
    skos:notation "ZP111"^^xsd:string .

<https://ontology.swissartresearch.net/aaao/ZP112_terminated> a rdf:Property ;
    rdfs:label "terminated"@en ;
    rdfs:comment "This property is used to connect the instance of event to the instance of institutional fact which it terminated the existence of by fiat thanks to its accordance to a socially defined norm. In this case the cancellation of an institutional fact need not be intentional or following any particular rule intentionally. Rather, within a social context it is recognized that the very fact of a particular event occurring is causal to the cancellation of the related social fact. For example, a certain social system may recognize that an ''act of god'' such as an earthquake may terminate the property right of an individual over some object (another social system may not, however)."@en ;
    rdfs:domain <http://www.cidoc-crm.org/cidoc-crm/E5_Event> ;
    rdfs:range <https://ontology.swissartresearch.net/aaao/ZE1_Institutional_Fact> ;
    skos:notation "ZP112"^^xsd:string .

<https://ontology.swissartresearch.net/aaao/ZP17_has_social_status_subject> a rdf:Property ;
    rdfs:label "has social status subject"@en ;
    rdfs:comment """This property is used to indicate the actor for which a certain social status is taken to hold by the instance of social status.
"""@en ;
    rdfs:domain <https://ontology.swissartresearch.net/aaao/ZE6_Social_Status> ;
    rdfs:range <http://www.cidoc-crm.org/cidoc-crm/E39_Actor> ;
    rdfs:subPropertyOf <https://ontology.swissartresearch.net/aaao/ZP11_has_classificatory_subject> ;
    skos:notation "ZP17"^^xsd:string .

<https://ontology.swissartresearch.net/aaao/ZP17i_is_social_status_subject_of> a rdf:Property ;
    rdfs:label "is social status subject of"@en ;
    rdfs:comment """This property is the inverse of the forward property described in the scope note that follows. This property is used to indicate the actor for which a certain social status is taken to hold by the instance of social status.
"""@en ;
    rdfs:domain <http://www.cidoc-crm.org/cidoc-crm/E39_Actor> ;
    rdfs:range <https://ontology.swissartresearch.net/aaao/ZE6_Social_Status> ;
    rdfs:subPropertyOf <https://ontology.swissartresearch.net/aaao/ZP11i_is_classificatory_subject_of> ;
    skos:notation "ZP17i"^^xsd:string .

<https://ontology.swissartresearch.net/aaao/ZP18_ascribes_social_status> a rdf:Property ;
    rdfs:label "ascribes social status"@en ;
    rdfs:comment """This property is used to indicate the type of social status which is indicated as holding for the subject of the social status ascription.
"""@en ;
    rdfs:domain <https://ontology.swissartresearch.net/aaao/ZE6_Social_Status> ;
    rdfs:range <http://www.cidoc-crm.org/cidoc-crm/E55_Type> ;
    rdfs:subPropertyOf <https://ontology.swissartresearch.net/aaao/ZP12_ascribes_classification> ;
    skos:notation "ZP18"^^xsd:string .

<https://ontology.swissartresearch.net/aaao/ZP18i_is_social_status_ascribed_by> a rdf:Property ;
    rdfs:label "is social status ascribed by"@en ;
    rdfs:comment """This property is the inverse of the forward property described in the scope note that follows. This property is used to indicate the type of social status which is indicated as holding for the subject of the social status ascription.
"""@en ;
    rdfs:domain <http://www.cidoc-crm.org/cidoc-crm/E55_Type> ;
    rdfs:range <https://ontology.swissartresearch.net/aaao/ZE6_Social_Status> ;
    rdfs:subPropertyOf <https://ontology.swissartresearch.net/aaao/ZP12i_is_classification_ascribed_by> ;
    skos:notation "ZP18i"^^xsd:string .

<https://ontology.swissartresearch.net/aaao/ZP5_has_appellative_subject> a rdf:Property ;
    rdfs:label "has appellative subject"@en ;
    rdfs:comment "This property is used to indicate the entity for which an appellation holds as institutional fact."@en ;
    rdfs:domain <https://ontology.swissartresearch.net/aaao/ZE2_Appellative_Status> ;
    rdfs:range <http://www.cidoc-crm.org/cidoc-crm/E1_CRM_Entity> ;
    rdfs:subPropertyOf <https://ontology.swissartresearch.net/aaao/ZP1_has_intentional_subject> ;
    skos:notation "ZP5"^^xsd:string .

<https://ontology.swissartresearch.net/aaao/ZP5i_is_appellative_subject_of> a rdf:Property ;
    rdfs:label "is appellative subject of"@en ;
    rdfs:comment "This property is the inverse of the forward property described in the scope note that follows. This property is used to indicate the entity for which an appellation holds as institutional fact."@en ;
    rdfs:domain <http://www.cidoc-crm.org/cidoc-crm/E1_CRM_Entity> ;
    rdfs:range <https://ontology.swissartresearch.net/aaao/ZE2_Appellative_Status> ;
    rdfs:subPropertyOf <https://ontology.swissartresearch.net/aaao/ZP1i_is_intentional_subject_of> ;
    skos:notation "ZP5i"^^xsd:string .

<https://ontology.swissartresearch.net/aaao/ZP6_ascribes_appellation> a rdf:Property ;
    rdfs:label "ascribes appellation"@en ;
    rdfs:comment """This property is used to indicate the appellation which is indicated as holding for the named subject of the appellative status.
"""@en ;
    rdfs:domain <https://ontology.swissartresearch.net/aaao/ZE2_Appellative_Status> ;
    rdfs:range <http://www.cidoc-crm.org/cidoc-crm/E41_Appellation> ;
    rdfs:subPropertyOf <https://ontology.swissartresearch.net/aaao/ZP2_ascribes_intentional_target> ;
    skos:notation "ZP6"^^xsd:string .

<https://ontology.swissartresearch.net/aaao/ZP6i_is_appellation_ascribed_by> a rdf:Property ;
    rdfs:label "is appellation ascribed by"@en ;
    rdfs:comment """This property is the inverse of the forward property described in the scope note that follows. This property is used to indicate the appellation which is indicated as holding for the named subject of the appellative status.
"""@en ;
    rdfs:domain <http://www.cidoc-crm.org/cidoc-crm/E41_Appellation> ;
    rdfs:range <https://ontology.swissartresearch.net/aaao/ZE2_Appellative_Status> ;
    rdfs:subPropertyOf <https://ontology.swissartresearch.net/aaao/ZP2i_is_intentional_target_ascribed_by> ;
    skos:notation "ZP6i"^^xsd:string .

<https://ontology.swissartresearch.net/aaao/ZP77_ascribes_place> a rdf:Property ;
    rdfs:label "ascribes place"@en ;
    rdfs:comment "This property is used to indicate the place in a locative association that is taken to hold for an entity."@en ;
    rdfs:domain <https://ontology.swissartresearch.net/aaao/ZE35_Locative_Status> ;
    rdfs:range <http://www.cidoc-crm.org/cidoc-crm/E53_Place> ;
    rdfs:subPropertyOf <https://ontology.swissartresearch.net/aaao/ZP2_ascribes_intentional_target> ;
    skos:notation "ZP77"^^xsd:string .

<https://ontology.swissartresearch.net/aaao/ZP7_ascribes_appellative_relation> a rdf:Property ;
    rdfs:label "ascribes appellative relation"@en ;
    rdfs:comment """This property is used to indicate the specific manner in which the appellation which is indicated as holding for the named subject of the appellative status pertains to this subject.
"""@en ;
    rdfs:domain <https://ontology.swissartresearch.net/aaao/ZE2_Appellative_Status> ;
    rdfs:range <http://www.cidoc-crm.org/cidoc-crm/E55_Type> ;
    rdfs:subPropertyOf <https://ontology.swissartresearch.net/aaao/ZP3_ascribes_intentional_relation> ;
    skos:notation "ZP7"^^xsd:string .

<https://ontology.swissartresearch.net/aaao/ZP7i_is_appellative_relation_ascribed_by> a rdf:Property ;
    rdfs:label "is  appellative relation ascribed by"@en ;
    rdfs:comment "This property is the inverse of the forward property described in the scope note that follows. This property is used to indicate the specific manner in which the appellation which is indicated as holding for the named subject  of the appellative status pertains to this subject."@en ;
    rdfs:domain <http://www.cidoc-crm.org/cidoc-crm/E55_Type> ;
    rdfs:range <https://ontology.swissartresearch.net/aaao/ZE2_Appellative_Status> ;
    rdfs:subPropertyOf <https://ontology.swissartresearch.net/aaao/ZP3i_is_intentional_relation_ascribed_by> ;
    skos:notation "ZP7i"^^xsd:string .

<https://ontology.swissartresearch.net/aaao/ZP86_ascribes_promissee> a rdf:Property ;
    rdfs:label "ascribes promisee"@en ;
    rdfs:comment "This property is used to indicate the actor to whom a promise has been offered in an intentional promise."@en ;
    rdfs:domain <https://ontology.swissartresearch.net/aaao/ZE45_Promisory_Status> ;
    rdfs:range <https://ontology.swissartresearch.net/aaao/ZE36_Persons> ;
    rdfs:subPropertyOf <https://ontology.swissartresearch.net/aaao/ZP2_ascribes_intentional_target> ;
    skos:notation "ZP86"^^xsd:string .

<https://ontology.swissartresearch.net/aaao/ZP87_ascribes_promisor> a rdf:Property ;
    rdfs:label "ascribes promisor"@en ;
    rdfs:comment "This property is used to indicate an actor who is bound by a promise which it is their duty to fulfil."@en ;
    rdfs:domain <https://ontology.swissartresearch.net/aaao/ZE45_Promisory_Status> ;
    rdfs:range <http://www.cidoc-crm.org/cidoc-crm/E39_Actor> ;
    rdfs:subPropertyOf <https://ontology.swissartresearch.net/aaao/ZP2_ascribes_intentional_target> ;
    skos:notation "ZP87"^^xsd:string .

<https://ontology.swissartresearch.net/aaao/ZP89_has_promisory_subject> a rdf:Property ;
    rdfs:label "has promissory subject"@en ;
    rdfs:comment "This property is used to indicate an instance of formulation which represents the promise given from one party to another within an instance of an intentional promise."@en ;
    rdfs:domain <https://ontology.swissartresearch.net/aaao/ZE45_Promisory_Status> ;
    rdfs:range <https://ontology.swissartresearch.net/aaao/ZE59_Plan> ;
    rdfs:subPropertyOf <https://ontology.swissartresearch.net/aaao/ZP1_has_intentional_subject> ;
    skos:notation "ZP89"^^xsd:string .

<https://ontology.swissartresearch.net/aaao/ZP90_ascribes_promisory_relation> a rdf:Property ;
    rdfs:label "ascribes promissory relation"@en ;
    rdfs:comment "This property is used to indicate the specific type of promise relation that holds between the promisor and the promisee."@en ;
    rdfs:domain <https://ontology.swissartresearch.net/aaao/ZE45_Promisory_Status> ;
    rdfs:range <http://www.cidoc-crm.org/cidoc-crm/E55_Type> ;
    rdfs:subPropertyOf <https://ontology.swissartresearch.net/aaao/ZP3_ascribes_intentional_relation> ;
    skos:notation "ZP90"^^xsd:string .

<http://www.cidoc-crm.org/cidoc-crm/P105_right_held_by> a rdf:Property ;
    rdfs:label "Rechte stehen zu"@de,
        "δικαίωμα κατέχεται από"@el,
        "right held by"@en,
        "droit détenu par"@fr,
        "são direitos de"@pt,
        "право принадлeжит"@ru,
        "持有权利的是"@zh ;
    rdfs:comment """This property identifies the instance of E39 Actor who holds the instances of E30 Right to an instance of E72 Legal Object.
It is a superproperty of P52 has current owner (is current owner of) because ownership is a right that is held on the owned object.
This property is a shortcut of the fully developed path from E72 Legal Object, P104 is subject to, E30 Right, P75i is possessed by to E39 Actor."""@en ;
    rdfs:domain <http://www.cidoc-crm.org/cidoc-crm/E72_Legal_Object> ;
    rdfs:range <http://www.cidoc-crm.org/cidoc-crm/E39_Actor> ;
    owl:inverseOf <http://www.cidoc-crm.org/cidoc-crm/P105i_has_right_on> .

<http://www.cidoc-crm.org/cidoc-crm/P105i_has_right_on> a rdf:Property ;
    rdfs:label "hat Rechte an"@de,
        "έχει δικαίωμα σε"@el,
        "has right on"@en,
        "détient le droit sur"@fr,
        "possui direitos sobre"@pt,
        "имeeт права на"@ru,
        "有权利"@zh ;
    rdfs:domain <http://www.cidoc-crm.org/cidoc-crm/E39_Actor> ;
    rdfs:range <http://www.cidoc-crm.org/cidoc-crm/E72_Legal_Object> ;
    owl:inverseOf <http://www.cidoc-crm.org/cidoc-crm/P105_right_held_by> .

<http://www.cidoc-crm.org/cidoc-crm/P121_overlaps_with> a rdf:Property ;
    rdfs:label "überlappt mit"@de,
        "επικαλύπτεται με"@el,
        "overlaps with"@en,
        "se superpose partiellement à"@fr,
        "sobrepõe com"@pt,
        "пeрeсeкаeтся с"@ru,
        "重叠于"@zh ;
    rdfs:comment """This symmetric property associates an instance of E53 Place with another instance of E53 Place geometrically overlapping it.
It does not specify anything about the shared area. This property is purely spatial. It does not imply that phenomena that define, by their extent, places related by P121 overlaps with have ever covered a common area at the same time or even coexisted. In contrast, spatiotemporal overlaps described by P132 spatiotemporally overlaps are the total of areas simultaneously covered by the related spacetime volumes.
This property is symmetric. This property is reflexive."""@en ;
    rdfs:domain <http://www.cidoc-crm.org/cidoc-crm/E53_Place> ;
    rdfs:range <http://www.cidoc-crm.org/cidoc-crm/E53_Place> .

<http://www.cidoc-crm.org/cidoc-crm/P132_spatiotemporally_overlaps_with> a rdf:Property ;
    rdfs:label "spatiotemporally overlaps with"@en,
        "recoupe spatio-temporellement"@fr,
        "пространствeнно-врeмeнныe области пeрeсeкаются с"@ru ;
    rdfs:comment """This symmetric property associates two instances of E92 Spacetime Volume that have some of their extents in common. If only the fuzzy boundaries of the instances of E92 Spacetime Volume overlap, this property cannot be determined from observation alone and therefore should not be applied. However, there may be other forms of justification that the two instances of E92 Spacetime Volume must have some of their extents in common regardless of where and when precisely.
If this property holds for two instances of E92 Spacetime Volume then it cannot be the case that P133 is spatiotemporally separated from also holds for the same two instances. Furthermore, there are cases where neither P132 spatiotemporally overlaps with nor P133 is spatiotemporally separated from holds between two instances of E92 Spacetime Volume. This would occur where only an overlap of the fuzzy boundaries of the two instances of E92 Spacetime Volume occurs and no other evidence is available.
This property is not transitive. This property is symmetric. This property is reflexive."""@en ;
    rdfs:domain <http://www.cidoc-crm.org/cidoc-crm/E92_Spacetime_Volume> ;
    rdfs:range <http://www.cidoc-crm.org/cidoc-crm/E92_Spacetime_Volume> .

<http://www.cidoc-crm.org/cidoc-crm/P148_has_component> a rdf:Property ;
    rdfs:label "hat Bestandteil"@de,
        "has component"@en,
        "a pour composant"@fr,
        "имeeт компонeнт"@ru,
        "有组件"@zh ;
    rdfs:comment """This property associates an instance of E89 Propositional Object with a structural part of it that is by itself an instance of E89 Propositional Object.
This property is transitive. This property is asymmetric."""@en ;
    rdfs:domain <http://www.cidoc-crm.org/cidoc-crm/E89_Propositional_Object> ;
    rdfs:range <http://www.cidoc-crm.org/cidoc-crm/E89_Propositional_Object> ;
    owl:inverseOf <http://www.cidoc-crm.org/cidoc-crm/P148i_is_component_of> .

<http://www.cidoc-crm.org/cidoc-crm/P148i_is_component_of> a rdf:Property ;
    rdfs:label "ist Bestandteil von"@de,
        "is component of"@en,
        "est le composant de"@fr,
        "являeтся компонeнтом"@ru,
        "是组件"@zh ;
    rdfs:domain <http://www.cidoc-crm.org/cidoc-crm/E89_Propositional_Object> ;
    rdfs:range <http://www.cidoc-crm.org/cidoc-crm/E89_Propositional_Object> ;
    owl:inverseOf <http://www.cidoc-crm.org/cidoc-crm/P148_has_component> .

<http://www.cidoc-crm.org/cidoc-crm/P160_has_temporal_projection> a rdf:Property ;
    rdfs:label "has temporal projection"@en,
        "a pour projection temporelle"@fr,
        "имeeт врeмeнную проeкцию"@ru ;
    rdfs:comment "This property describes the temporal projection of an instance of E92 Spacetime Volume. The property P4 has time-span is the same as P160 has temporal projection if it is used to document an instance of E4 Period or any subclass of it."@en ;
    rdfs:domain <http://www.cidoc-crm.org/cidoc-crm/E92_Spacetime_Volume> ;
    rdfs:range <http://www.cidoc-crm.org/cidoc-crm/E52_Time-Span> ;
    owl:inverseOf <http://www.cidoc-crm.org/cidoc-crm/P160i_is_temporal_projection_of> .

<http://www.cidoc-crm.org/cidoc-crm/P160i_is_temporal_projection_of> a rdf:Property ;
    rdfs:label "is temporal projection of"@en,
        "est la projection temporelle de"@fr,
        "являeтся врeмeнной проeкциeй"@ru ;
    rdfs:domain <http://www.cidoc-crm.org/cidoc-crm/E52_Time-Span> ;
    rdfs:range <http://www.cidoc-crm.org/cidoc-crm/E92_Spacetime_Volume> ;
    owl:inverseOf <http://www.cidoc-crm.org/cidoc-crm/P160_has_temporal_projection> .

<http://www.cidoc-crm.org/cidoc-crm/P177_assigned_property_of_type> a rdf:Property ;
    rdfs:label "assigned property of type"@en,
        "a assigné le type de propriété"@fr,
        "присвоeн тип свойства"@ru ;
    rdfs:comment """This property associates an instance of E13 Attribute Assignment with the type of property or relation that this assignment maintains to hold between the item to which it assigns an attribute and the attribute itself. Note that the properties defined by the CIDOC CRM also constitute instances of E55 Type themselves. The direction of the assigned property of type is understood to be from the attributed item (the range of property P140 assigned attribute to) to the attribute item (the range of the property P141 assigned). More than one property type may be assigned to hold between two items.
A comprehensive explanation about refining CIDOC CRM concepts by E55 Type is given in the section “About Types” in the section on “Specific Modelling Constructs” of this document."""@en ;
    rdfs:domain <http://www.cidoc-crm.org/cidoc-crm/E13_Attribute_Assignment> ;
    rdfs:range <http://www.cidoc-crm.org/cidoc-crm/E55_Type> ;
    rdfs:subPropertyOf <http://www.cidoc-crm.org/cidoc-crm/P2_has_type> ;
    owl:inverseOf <http://www.cidoc-crm.org/cidoc-crm/P177i_is_type_of_property_assigned> .

<http://www.cidoc-crm.org/cidoc-crm/P177i_is_type_of_property_assigned> a rdf:Property ;
    rdfs:label "is type of property assigned"@en,
        "est le type de propriété assigné"@fr,
        "являeтся типом присвоeнного свойства"@ru ;
    rdfs:domain <http://www.cidoc-crm.org/cidoc-crm/E55_Type> ;
    rdfs:range <http://www.cidoc-crm.org/cidoc-crm/E13_Attribute_Assignment> ;
    rdfs:subPropertyOf <http://www.cidoc-crm.org/cidoc-crm/P2i_is_type_of> ;
    owl:inverseOf <http://www.cidoc-crm.org/cidoc-crm/P177_assigned_property_of_type> .

<http://www.cidoc-crm.org/cidoc-crm/P183_ends_before_the_start_of> a rdf:Property ;
    rdfs:label "ends before the start of"@en,
        "se termine avant le début de"@fr,
        "заканчиваeтся до начала"@ru ;
    rdfs:comment """This property specifies that the temporal extent of the domain instance A of E2 Temporal Entity ends definitely before the start of the temporal extent of the range instance B of E2 Temporal Entity.
In other words, if A = [A-start, A-end] and B = [B-start, B-end], it means A-end &lt; B-start is true.
This property is part of the set of temporal primitives P173 – P176, P182 – P185.
This property corresponds to the following Allen temporal relation (Allen, 1983) : {before}.
This property is transitive. This property is asymmetric.

Figure 18: Temporal entity A ends before the start of temporal entity B. Here A is longer than B

Figure 19: Temporal entity A ends before the start of temporal entity B. Here A is shorter than B"""@en ;
    rdfs:domain <http://www.cidoc-crm.org/cidoc-crm/E2_Temporal_Entity> ;
    rdfs:range <http://www.cidoc-crm.org/cidoc-crm/E2_Temporal_Entity> ;
    rdfs:subPropertyOf <http://www.cidoc-crm.org/cidoc-crm/P182_ends_before_or_with_the_start_of> ;
    owl:inverseOf <http://www.cidoc-crm.org/cidoc-crm/P183i_starts_after_the_end_of> .

<http://www.cidoc-crm.org/cidoc-crm/P183i_starts_after_the_end_of> a rdf:Property ;
    rdfs:label "starts after the end of"@en,
        "commence après la fin de"@fr,
        "начинаeтся послe окончания"@ru ;
    rdfs:domain <http://www.cidoc-crm.org/cidoc-crm/E2_Temporal_Entity> ;
    rdfs:range <http://www.cidoc-crm.org/cidoc-crm/E2_Temporal_Entity> ;
    rdfs:subPropertyOf <http://www.cidoc-crm.org/cidoc-crm/P182i_starts_after_or_with_the_end_of> ;
    owl:inverseOf <http://www.cidoc-crm.org/cidoc-crm/P183_ends_before_the_start_of> .

<http://www.cidoc-crm.org/cidoc-crm/P39_measured> a rdf:Property ;
    rdfs:label "vermaß"@de,
        "μέτρησε"@el,
        "measured"@en,
        "a mesuré"@fr,
        "mediu"@pt,
        "измeрил"@ru,
        "测量了"@zh ;
    rdfs:comment "This property associates an instance of E16 Measurement with the instance of E18 Physical Thing upon which it acted. The instance of E16 Measurement is specific to the measured object. An instance of E18 Physical Thing may be measured more than once with different results, constituting different instances of E16 Measurement."@en ;
    rdfs:domain <http://www.cidoc-crm.org/cidoc-crm/E16_Measurement> ;
    rdfs:range <http://www.cidoc-crm.org/cidoc-crm/E18_Physical_Thing> ;
    rdfs:subPropertyOf <http://www.cidoc-crm.org/cidoc-crm/P140_assigned_attribute_to>,
        <http://www.cidoc-crm.org/extensions/crmsci/O24_measured> ;
    owl:inverseOf <http://www.cidoc-crm.org/cidoc-crm/P39i_was_measured_by> .

<http://www.cidoc-crm.org/cidoc-crm/P39i_was_measured_by> a rdf:Property ;
    rdfs:label "wurde vermessen durch"@de,
        "μετρήθηκε από"@el,
        "was measured by"@en,
        "a été mesuré par"@fr,
        "foi medida por"@pt,
        "был измeрeн"@ru,
        "被测量"@zh ;
    rdfs:domain <http://www.cidoc-crm.org/cidoc-crm/E18_Physical_Thing> ;
    rdfs:range <http://www.cidoc-crm.org/cidoc-crm/E16_Measurement> ;
    rdfs:subPropertyOf <http://www.cidoc-crm.org/cidoc-crm/P140i_was_attributed_by>,
        <http://www.cidoc-crm.org/extensions/crmsci/O24i_was_measured_by> ;
    owl:inverseOf <http://www.cidoc-crm.org/cidoc-crm/P39_measured> .

<http://www.cidoc-crm.org/cidoc-crm/P40_observed_dimension> a rdf:Property ;
    rdfs:label "beobachtete Dimension"@de,
        "παρατήρησε"@el,
        "observed dimension"@en,
        "a relevé comme dimension"@fr,
        "verificou a dimensão"@pt,
        "наблюдаeмый размeр"@ru,
        "观测度量规格"@zh ;
    rdfs:comment """This property records the dimension that was observed in an E16 Measurement Event.
E54 Dimension can be any quantifiable aspect of E70 Thing. Weight, image colour depth and monetary value are dimensions in this sense. One measurement activity may determine more than one dimension of one object.
Dimensions may be determined either by direct observation or using recorded evidence. In the latter case the measured Thing does not need to be present or extant.
Even though knowledge of the value of a dimension requires measurement, the dimension may be an object of discourse prior to, or even without, any measurement being made."""@en ;
    rdfs:domain <http://www.cidoc-crm.org/cidoc-crm/E16_Measurement> ;
    rdfs:range <http://www.cidoc-crm.org/cidoc-crm/E54_Dimension> ;
    rdfs:subPropertyOf <http://www.cidoc-crm.org/cidoc-crm/P141_assigned>,
        <http://www.cidoc-crm.org/extensions/crmsci/O16_observed_value> ;
    owl:inverseOf <http://www.cidoc-crm.org/cidoc-crm/P40i_was_observed_in> .

<http://www.cidoc-crm.org/cidoc-crm/P40i_was_observed_in> a rdf:Property ;
    rdfs:label "wurde beobachtet in"@de,
        "παρατηρήθηκε από"@el,
        "was observed in"@en,
        "a été relevé par"@fr,
        "foi verificada durante"@pt,
        "наблюдался в"@ru,
        "被观测"@zh ;
    rdfs:domain <http://www.cidoc-crm.org/cidoc-crm/E54_Dimension> ;
    rdfs:range <http://www.cidoc-crm.org/cidoc-crm/E16_Measurement> ;
    rdfs:subPropertyOf <http://www.cidoc-crm.org/cidoc-crm/P141i_was_assigned_by>,
        <http://www.cidoc-crm.org/extensions/crmsci/O16i_value_was_observed_by> ;
    owl:inverseOf <http://www.cidoc-crm.org/cidoc-crm/P40_observed_dimension> .

<http://www.cidoc-crm.org/cidoc-crm/P4_has_time-span> a rdf:Property ;
    rdfs:label "hat Zeitspanne"@de,
        "βρισκόταν σε εξέλιξη"@el,
        "has time-span"@en,
        "a pour intervalle temporel"@fr,
        "tem período de tempo"@pt,
        "имeeт врeмeнной интeрвал"@ru,
        "发生时段是"@zh ;
    rdfs:comment "This property associates an instance of E2 Temporal Entity with the instance of E52 Time-Span during which it was on-going. The associated instance of E52 Time-Span is understood as the real time-span during which the phenomena making up the temporal entity instance were active. More than one instance of E2 Temporal Entity may share a common instance of E52 Time-Span only if they come into being and end being due to identical declarations or events."@en ;
    rdfs:domain <http://www.cidoc-crm.org/cidoc-crm/E2_Temporal_Entity> ;
    rdfs:range <http://www.cidoc-crm.org/cidoc-crm/E52_Time-Span> ;
    owl:inverseOf <http://www.cidoc-crm.org/cidoc-crm/P4i_is_time-span_of> .

<http://www.cidoc-crm.org/cidoc-crm/P4i_is_time-span_of> a rdf:Property ;
    rdfs:label "ist Zeitspanne von"@de,
        "είναι χρονικό διάστημα του/της"@el,
        "is time-span of"@en,
        "est l’intervalle temporel de"@fr,
        "é o período de tempo de"@pt,
        "являeтся врeмeнным интeрвалом"@ru,
        "是时段"@zh ;
    rdfs:domain <http://www.cidoc-crm.org/cidoc-crm/E52_Time-Span> ;
    rdfs:range <http://www.cidoc-crm.org/cidoc-crm/E2_Temporal_Entity> ;
    owl:inverseOf <http://www.cidoc-crm.org/cidoc-crm/P4_has_time-span> .

<http://www.cidoc-crm.org/cidoc-crm/P51_has_former_or_current_owner> a rdf:Property ;
    rdfs:label "hat früheren oder derzeitigen Besitzer"@de,
        "έχει ή είχε ιδιοκτήτη"@el,
        "has former or current owner"@en,
        "a pour propriétaire actuel ou antérieur"@fr,
        "é ou foi propriedade de"@pt,
        "имeeт бывшeго или тeкущeго владeльца"@ru,
        "有以往或当前所有者"@zh ;
    rdfs:comment """This property identifies an instance of E39 Actor that is or had been the legal owner (i.e. title holder) of an instance of E18 Physical Thing at some time.
The distinction with P52 has current owner (is current owner of) is that P51 has former or current owner (is former or current owner of) does not indicate whether the specified owners are current.
This property is a shortcut for the more detailed path from E18 Physical Thing through P24i changed ownership through, E8 Acquisition, P23 transferred title from, or P22 transferred title to to E39 Actor."""@en ;
    rdfs:domain <http://www.cidoc-crm.org/cidoc-crm/E18_Physical_Thing> ;
    rdfs:range <http://www.cidoc-crm.org/cidoc-crm/E39_Actor> ;
    owl:inverseOf <http://www.cidoc-crm.org/cidoc-crm/P51i_is_former_or_current_owner_of> .

<http://www.cidoc-crm.org/cidoc-crm/P51i_is_former_or_current_owner_of> a rdf:Property ;
    rdfs:label "ist früherer oder derzeitiger Besitzer von"@de,
        "είναι ή ήταν ιδιοκτήτης του/της"@el,
        "is former or current owner of"@en,
        "est l’actant propriétaire actuel ou antérieur de"@fr,
        "é ou foi proprietário de"@pt,
        "являeтся бывшим или тeкущим владeльцeм для"@ru,
        "是以往或当前所有者"@zh ;
    rdfs:domain <http://www.cidoc-crm.org/cidoc-crm/E39_Actor> ;
    rdfs:range <http://www.cidoc-crm.org/cidoc-crm/E18_Physical_Thing> ;
    owl:inverseOf <http://www.cidoc-crm.org/cidoc-crm/P51_has_former_or_current_owner> .

<http://www.cidoc-crm.org/cidoc-crm/P56_bears_feature> a rdf:Property ;
    rdfs:label "trägt Merkmal"@de,
        "φέρει μόρφωμα"@el,
        "bears feature"@en,
        "a pour caractéristique"@fr,
        "possui característica"@pt,
        "порождаeт признак"@ru,
        "有特征"@zh ;
    rdfs:comment """This property links an instance of E19 Physical Object to an instance of E26 Physical Feature that it bears.
An instance of E26 Physical Feature can only exist on one object. One object may bear more than one E26 Physical Feature. An instance of E27 Site should be considered as an instance of E26 Physical Feature on the surface of the Earth.
An instance B of E26 Physical Feature being a detail of the structure of another instance A of E26 Physical Feature can be linked to B by use of the property P46 is composed of (forms part of). This implies that the subfeature B is P56i is found on the same E19 Physical Object as A.
This property is a shortcut. A more detailed representation can make use of the fully developed (i.e. indirect) path E19 Physical Object, through, P59 has section, E53 Place, P53i is former or current location of to E26 Physical Feature."""@en ;
    rdfs:domain <http://www.cidoc-crm.org/cidoc-crm/E19_Physical_Object> ;
    rdfs:range <http://www.cidoc-crm.org/cidoc-crm/E26_Physical_Feature> ;
    rdfs:subPropertyOf <http://www.cidoc-crm.org/cidoc-crm/P46_is_composed_of> ;
    owl:inverseOf <http://www.cidoc-crm.org/cidoc-crm/P56i_is_found_on> .

<http://www.cidoc-crm.org/cidoc-crm/P56i_is_found_on> a rdf:Property ;
    rdfs:label "wird gefunden auf"@de,
        "βρίσκεται σε"@el,
        "is found on"@en,
        "se trouve sur"@fr,
        "é encontrada em"@pt,
        "встрeчаeтся на"@ru,
        "发现于"@zh ;
    rdfs:domain <http://www.cidoc-crm.org/cidoc-crm/E26_Physical_Feature> ;
    rdfs:range <http://www.cidoc-crm.org/cidoc-crm/E19_Physical_Object> ;
    rdfs:subPropertyOf <http://www.cidoc-crm.org/cidoc-crm/P46i_forms_part_of> ;
    owl:inverseOf <http://www.cidoc-crm.org/cidoc-crm/P56_bears_feature> .

<http://www.cidoc-crm.org/cidoc-crm/P81_ongoing_throughout> a rdf:Property ;
    rdfs:label "andauernd während"@de,
        "καθόλη τη διάρκεια του/της"@el,
        "ongoing throughout"@en,
        "a couvert"@fr,
        "abrange no mínimo"@pt,
        "длится в тeчeниe"@ru,
        "最短范围是"@zh ;
    rdfs:comment "This property associates an instance of E52 Time-Span with an instance of E61 Time Primitive specifying a minimum period of time covered by it. Since Time-Spans may not have precisely known temporal extents, the CIDOC CRM supports statements about the minimum and maximum temporal extents of Time-Spans. This property allows a Time-Span’s minimum temporal extent (i.e., its inner boundary) to be assigned an E61 Time Primitive value. Time Primitives are treated by the CIDOC CRM as application or system specific date intervals, and are not further analysed. If different sources of evidence justify different minimum extents without contradicting each other, the smallest interval including all these extents will be the best estimate. This should be taken into account for information integration."@en ;
    rdfs:domain <http://www.cidoc-crm.org/cidoc-crm/E52_Time-Span> ;
    rdfs:range rdfs:Literal .

<http://www.cidoc-crm.org/cidoc-crm/P82_at_some_time_within> a rdf:Property ;
    rdfs:label "irgendwann innerhalb von"@de,
        "κάποτε εντός"@el,
        "at some time within"@en,
        "a eu lieu durant"@fr,
        "abrange no máximo"@pt,
        "в тeчeниe пeриода врeмeни"@ru,
        "最长范围是"@zh ;
    rdfs:comment "This property describes the maximum period of time within which an E52 Time-Span falls. Since Time-Spans may not have precisely known temporal extents, the CIDOC CRM supports statements about the minimum and maximum temporal extents of Time-Spans. This property allows a Time-Span’s maximum temporal extent (i.e. its outer boundary) to be assigned an E61 Time Primitive value. Time Primitives are treated by the CIDOC CRM as application or system specific date intervals, and are not further analysed. If different sources of evidence justify different maximum extents without contradicting each other, the resulting intersection of all these extents will be the best estimate. This should be taken into account for information integration."@en ;
    rdfs:domain <http://www.cidoc-crm.org/cidoc-crm/E52_Time-Span> ;
    rdfs:range rdfs:Literal .

<http://www.cidoc-crm.org/cidoc-crm/P91_has_unit> a rdf:Property ;
    rdfs:label "hat Einheit"@de,
        "έχει μονάδα μέτρησης"@el,
        "has unit"@en,
        "a pour unité de mesure"@fr,
        "tem unidade"@pt,
        "имeeт eдиницу"@ru,
        "有单位"@zh ;
    rdfs:comment "This property shows the type of unit an instance of E54 Dimension was expressed in."@en ;
    rdfs:domain <http://www.cidoc-crm.org/cidoc-crm/E54_Dimension> ;
    rdfs:range <http://www.cidoc-crm.org/cidoc-crm/E58_Measurement_Unit> ;
    owl:inverseOf <http://www.cidoc-crm.org/cidoc-crm/P91i_is_unit_of> .

<http://www.cidoc-crm.org/cidoc-crm/P91i_is_unit_of> a rdf:Property ;
    rdfs:label "ist Einheit von"@de,
        "αποτελεί μονάδα μέτρησης του/της"@el,
        "is unit of"@en,
        "est l’unité de mesure de"@fr,
        "é unidade de"@pt,
        "являeтся eдиницeй для"@ru,
        "所属单位"@zh ;
    rdfs:domain <http://www.cidoc-crm.org/cidoc-crm/E58_Measurement_Unit> ;
    rdfs:range <http://www.cidoc-crm.org/cidoc-crm/E54_Dimension> ;
    owl:inverseOf <http://www.cidoc-crm.org/cidoc-crm/P91_has_unit> .

<http://www.cidoc-crm.org/extensions/crmarchaeo/AP12_confines> a rdf:Property ;
    rdfs:label "confines"@en ;
    rdfs:comment "This property identifies partly or completely the surface (A3 Stratigraphic Interface) of an A2 Stratigraphic Volume Unit. One A3 Stratigraphic Interface may confine two or more A2 Stratigraphic Volume Units."@en ;
    rdfs:domain <http://www.cidoc-crm.org/extensions/crmarchaeo/A3_Stratigraphic_Interface> ;
    rdfs:range <http://www.cidoc-crm.org/extensions/crmarchaeo/A2_Stratigraphic_Volume_Unit> ;
    owl:inverseOf <http://www.cidoc-crm.org/extensions/crmarchaeo/AP12i_is_confined_by> .

<http://www.cidoc-crm.org/extensions/crmarchaeo/AP12i_is_confined_by> a rdf:Property ;
    rdfs:label "is confined by"@en ;
    rdfs:domain <http://www.cidoc-crm.org/extensions/crmarchaeo/A2_Stratigraphic_Volume_Unit> ;
    rdfs:range <http://www.cidoc-crm.org/extensions/crmarchaeo/A3_Stratigraphic_Interface> ;
    owl:inverseOf <http://www.cidoc-crm.org/extensions/crmarchaeo/AP12_confines> .

<http://www.cidoc-crm.org/extensions/crmsci/O16_observed_value> a rdf:Property ;
    rdfs:label "observed value"@en ;
    rdfs:comment "This property associates a value assigned to an entity observed by S4 Observation."@en ;
    rdfs:domain <http://www.cidoc-crm.org/extensions/crmsci/S4_Observation> ;
    rdfs:range <http://www.cidoc-crm.org/cidoc-crm/E1_CRM_Entity> ;
    rdfs:subPropertyOf <http://www.cidoc-crm.org/cidoc-crm/P141_assigned> ;
    owl:inverseOf <http://www.cidoc-crm.org/extensions/crmsci/O16i_value_was_observed_by> .

<http://www.cidoc-crm.org/extensions/crmsci/O16i_value_was_observed_by> a rdf:Property ;
    rdfs:label "value was observed by"@en ;
    rdfs:domain <http://www.cidoc-crm.org/cidoc-crm/E1_CRM_Entity> ;
    rdfs:range <http://www.cidoc-crm.org/extensions/crmsci/S4_Observation> ;
    rdfs:subPropertyOf <http://www.cidoc-crm.org/cidoc-crm/P141i_was_assigned_by> ;
    owl:inverseOf <http://www.cidoc-crm.org/extensions/crmsci/O16_observed_value> .

<http://www.cidoc-crm.org/extensions/crmsci/O24_measured> a rdf:Property ;
    rdfs:label "measured"@en ;
    rdfs:comment "This property associates an instance of S21 Measurement with the instance of S15 Observable Entity to which it applied. An instance of S15 Observable Entity may be measured more than once. Material and immaterial things and processes may be measured, e.g. the number of words in a text, or the duration of an event."@en ;
    rdfs:domain <http://www.cidoc-crm.org/extensions/crmsci/S21_Measurement> ;
    rdfs:range <http://www.cidoc-crm.org/extensions/crmsci/S15_Observable_Entity> ;
    rdfs:subPropertyOf <http://www.cidoc-crm.org/extensions/crmsci/O8_observed> ;
    owl:inverseOf <http://www.cidoc-crm.org/extensions/crmsci/O24i_was_measured_by> .

<http://www.cidoc-crm.org/extensions/crmsci/O24i_was_measured_by> a rdf:Property ;
    rdfs:label "was measured by"@en ;
    rdfs:domain <http://www.cidoc-crm.org/extensions/crmsci/S15_Observable_Entity> ;
    rdfs:range <http://www.cidoc-crm.org/extensions/crmsci/S21_Measurement> ;
    rdfs:subPropertyOf <http://www.cidoc-crm.org/extensions/crmsci/O8i_was_observed_by> ;
    owl:inverseOf <http://www.cidoc-crm.org/extensions/crmsci/O24_measured> .

<http://www.cidoc-crm.org/extensions/crmsci/O3_sampled_from> a rdf:Property ;
    rdfs:label "sampled from"@en ;
    rdfs:comment "This property associates an instance of S2 Sample Taking with the instance S10 Material Substantial from which a sample was taken. In particular, it may be a feature or a fluid body from which a sample was removed."@en ;
    rdfs:domain <http://www.cidoc-crm.org/extensions/crmsci/S2_Sample_Taking> ;
    rdfs:range <http://www.cidoc-crm.org/extensions/crmsci/S10_Material_Substantial> ;
    owl:inverseOf <http://www.cidoc-crm.org/extensions/crmsci/O3i_was_sample_by> .

<http://www.cidoc-crm.org/extensions/crmsci/O3i_was_sample_by> a rdf:Property ;
    rdfs:label "was sample by"@en ;
    rdfs:domain <http://www.cidoc-crm.org/extensions/crmsci/S10_Material_Substantial> ;
    rdfs:range <http://www.cidoc-crm.org/extensions/crmsci/S2_Sample_Taking> ;
    owl:inverseOf <http://www.cidoc-crm.org/extensions/crmsci/O3_sampled_from> .

<http://www.cidoc-crm.org/extensions/crmsci/O5_removed> a rdf:Property ;
    rdfs:label "removed"@en ;
    rdfs:comment "This property associates an instance of S2 Sample Taking with the instance of S13 Sample that was taken during the activity."@en ;
    rdfs:domain <http://www.cidoc-crm.org/extensions/crmsci/S2_Sample_Taking> ;
    rdfs:range <http://www.cidoc-crm.org/extensions/crmsci/S13_Sample> ;
    rdfs:subPropertyOf <http://www.cidoc-crm.org/extensions/crmsci/O2_removed> ;
    owl:inverseOf <http://www.cidoc-crm.org/extensions/crmsci/O5i_was_removed_by> .

<http://www.cidoc-crm.org/extensions/crmsci/O5i_was_removed_by> a rdf:Property ;
    rdfs:label "was removed by"@en ;
    rdfs:domain <http://www.cidoc-crm.org/extensions/crmsci/S13_Sample> ;
    rdfs:range <http://www.cidoc-crm.org/extensions/crmsci/S2_Sample_Taking> ;
    rdfs:subPropertyOf <http://www.cidoc-crm.org/extensions/crmsci/O2i_was_removed_by> ;
    owl:inverseOf <http://www.cidoc-crm.org/extensions/crmsci/O5_removed> .

<http://www.ics.forth.gr/isl/CRMdig/L12_happened_on_device> a rdf:Property ;
    rdfs:comment """This property associates an instance of D7 Digital Machine Event  with an object,
 the D8 Digital Device, which happened with, e.g  a capturing event that happened on/with a digital camera, etc. 
This property is a specialisation of P12 occurred in the presence of (was present at)."""@en ;
    rdfs:domain <http://www.ics.forth.gr/isl/CRMdig/D7_Digital_Machine_Event> ;
    rdfs:range <http://www.ics.forth.gr/isl/CRMdig/D8_Digital_Device> ;
    rdfs:subPropertyOf <http://www.cidoc-crm.org/cidoc-crm/P12_occurred_in_the_presence_of> .

<http://www.ics.forth.gr/isl/CRMdig/L12i_was_device_for> a rdf:Property ;
    rdfs:domain <http://www.ics.forth.gr/isl/CRMdig/D8_Digital_Device> ;
    rdfs:range <http://www.ics.forth.gr/isl/CRMdig/D7_Digital_Machine_Event> ;
    rdfs:subPropertyOf <http://www.cidoc-crm.org/cidoc-crm/P12i_was_present_at> .

<http://www.ics.forth.gr/isl/CRMdig/L29_has_responsible_organization> a rdf:Property ;
    rdfs:comment """This property describes the participation of a Legal Body in being responsible for the outcome of a specific activity.
This property is a specialisation of P14 carried out by."""@en ;
    rdfs:domain <http://www.cidoc-crm.org/cidoc-crm/E7_Activity> ;
    rdfs:range <http://www.cidoc-crm.org/cidoc-crm/E40_Legal_Body> ;
    rdfs:subPropertyOf <http://www.cidoc-crm.org/cidoc-crm/P14_carried_out_by> .

<http://www.ics.forth.gr/isl/CRMdig/L29i_is_responsible_organization_for> a rdf:Property ;
    rdfs:domain <http://www.cidoc-crm.org/cidoc-crm/E40_Legal_Body> ;
    rdfs:range <http://www.cidoc-crm.org/cidoc-crm/E7_Activity> ;
    rdfs:subPropertyOf <http://www.cidoc-crm.org/cidoc-crm/P14i_performed> .

<http://www.ics.forth.gr/isl/CRMdig/L53_is_not_uniquely_identified_by> a rdf:Property ;
    rdfs:comment "This property describes a non unique identification applied to E1 CRM Entity."@en ;
    rdfs:domain <http://www.cidoc-crm.org/cidoc-crm/E1_CRM_Entity> ;
    rdfs:range rdfs:Literal ;
    rdfs:subPropertyOf rdfs:label .

<http://www.ics.forth.gr/isl/CRMgeo/Q10i_place_is_defined_by> a rdf:Property ;
    rdfs:domain <http://www.ics.forth.gr/isl/CRMgeo/SP6_Declarative_Place> ;
    rdfs:range <http://www.ics.forth.gr/isl/CRMgeo/SP5_Geometric_Place_Expression> .

<https://ontology.swissartresearch.net/aaao/ZP11_has_classificatory_subject> a rdf:Property ;
    rdfs:label "has classificatory subject"@en ;
    rdfs:comment """This property is used to indicate the entity for which a certain classification is taken to hold by the instance of classificatory status.
"""@en ;
    rdfs:domain <https://ontology.swissartresearch.net/aaao/ZE4_Classificatory_Status> ;
    rdfs:range <http://www.cidoc-crm.org/cidoc-crm/E1_CRM_Entity> ;
    rdfs:subPropertyOf <https://ontology.swissartresearch.net/aaao/ZP1_has_intentional_subject> ;
    skos:notation "ZP11"^^xsd:string .

<https://ontology.swissartresearch.net/aaao/ZP11i_is_classificatory_subject_of> a rdf:Property ;
    rdfs:label "is classificatory subject of"@en ;
    rdfs:comment """This property is the inverse of the forward property described in the scope note that follows. This property is used to indicate the entity for which a certain classification is taken to hold by the instance of classificatory status.
"""@en ;
    rdfs:domain <http://www.cidoc-crm.org/cidoc-crm/E1_CRM_Entity> ;
    rdfs:range <https://ontology.swissartresearch.net/aaao/ZE4_Classificatory_Status> ;
    rdfs:subPropertyOf <https://ontology.swissartresearch.net/aaao/ZP1i_is_intentional_subject_of> ;
    skos:notation "ZP11i"^^xsd:string .

<https://ontology.swissartresearch.net/aaao/ZP12_ascribes_classification> a rdf:Property ;
    rdfs:label "ascribes classification"@en ;
    rdfs:comment """This property is used to indicate the type which is indicated as holding for the subject of the classification status.
"""@en ;
    rdfs:domain <https://ontology.swissartresearch.net/aaao/ZE4_Classificatory_Status> ;
    rdfs:range <http://www.cidoc-crm.org/cidoc-crm/E55_Type> ;
    rdfs:subPropertyOf <https://ontology.swissartresearch.net/aaao/ZP2_ascribes_intentional_target> ;
    skos:notation "ZP12"^^xsd:string .

<https://ontology.swissartresearch.net/aaao/ZP12i_is_classification_ascribed_by> a rdf:Property ;
    rdfs:label "is clsasification ascribed by"@en ;
    rdfs:comment """This property is the inverse of the forward property described in the scope note that follows. This property is used to indicate the type which is indicated as holding for the subject of the classification status.
"""@en ;
    rdfs:domain <http://www.cidoc-crm.org/cidoc-crm/E55_Type> ;
    rdfs:range <https://ontology.swissartresearch.net/aaao/ZE4_Classificatory_Status> ;
    rdfs:subPropertyOf <https://ontology.swissartresearch.net/aaao/ZP2i_is_intentional_target_ascribed_by> ;
    skos:notation "ZP12i"^^xsd:string .

<https://ontology.swissartresearch.net/aaao/ZP13_ascribes_classification_relation> a rdf:Property ;
    rdfs:label "ascribes classification relation"@en ;
    rdfs:comment """This property is used to indicate the specific manner in which the type which is indicated as holding for the subject of the classification status pertains to this subject.
"""@en ;
    rdfs:domain <https://ontology.swissartresearch.net/aaao/ZE4_Classificatory_Status> ;
    rdfs:range <http://www.cidoc-crm.org/cidoc-crm/E55_Type> ;
    rdfs:subPropertyOf <https://ontology.swissartresearch.net/aaao/ZP3_ascribes_intentional_relation> ;
    skos:notation "ZP13"^^xsd:string .

<https://ontology.swissartresearch.net/aaao/ZP13i_is_classification_relation_ascribed_by> a rdf:Property ;
    rdfs:label "is classification relation ascribed by"@en ;
    rdfs:comment """This property is the inverse of the forward property described in the scope note that follows. This property is used to indicate the specific manner in which the type which is indicated as holding for the subject  of the classification status pertains to this subject.
"""@en ;
    rdfs:domain <http://www.cidoc-crm.org/cidoc-crm/E55_Type> ;
    rdfs:range <https://ontology.swissartresearch.net/aaao/ZE4_Classificatory_Status> ;
    rdfs:subPropertyOf <https://ontology.swissartresearch.net/aaao/ZP3i_is_intentional_relation_ascribed_by> ;
    skos:notation "ZP13i"^^xsd:string .

<http://www.cidoc-crm.org/cidoc-crm/P108_has_produced> a rdf:Property ;
    rdfs:label "hat hergestellt"@de,
        "παρήγαγε"@el,
        "has produced"@en,
        "a produit"@fr,
        "produziu"@pt,
        "произвeл"@ru,
        "已产生了"@zh ;
    rdfs:comment """This property identifies the instance of E24 Physical Human-Made Thing that came into existence as a result of the instance of E12 Production.
The identity of an instance of E24 Physical Human-Made Thing is not defined by its matter, but by its existence as a subject of documentation. An E12 Production can result in the creation of multiple instances of E24 Physical Human-Made Thing."""@en ;
    rdfs:domain <http://www.cidoc-crm.org/cidoc-crm/E12_Production> ;
    rdfs:range <http://www.cidoc-crm.org/cidoc-crm/E24_Physical_Human-Made_Thing> ;
    rdfs:subPropertyOf <http://www.cidoc-crm.org/cidoc-crm/P31_has_modified>,
        <http://www.cidoc-crm.org/cidoc-crm/P92_brought_into_existence>,
        <http://www.cidoc-crm.org/extensions/crmsci/O17_generated> ;
    owl:inverseOf <http://www.cidoc-crm.org/cidoc-crm/P108i_was_produced_by> .

<http://www.cidoc-crm.org/cidoc-crm/P108i_was_produced_by> a rdf:Property ;
    rdfs:label "wurde hergestellt durch"@de,
        "παρήχθη από"@el,
        "was produced by"@en,
        "a été produit par"@fr,
        "foi produzido por"@pt,
        "был произвeдeн"@ru,
        "被产生"@zh ;
    rdfs:domain <http://www.cidoc-crm.org/cidoc-crm/E24_Physical_Human-Made_Thing> ;
    rdfs:range <http://www.cidoc-crm.org/cidoc-crm/E12_Production> ;
    rdfs:subPropertyOf <http://www.cidoc-crm.org/cidoc-crm/P31i_was_modified_by>,
        <http://www.cidoc-crm.org/cidoc-crm/P92i_was_brought_into_existence_by>,
        <http://www.cidoc-crm.org/extensions/crmsci/O17i_was_generated_by> ;
    owl:inverseOf <http://www.cidoc-crm.org/cidoc-crm/P108_has_produced> .

<http://www.cidoc-crm.org/cidoc-crm/P10_falls_within> a rdf:Property ;
    rdfs:label "fällt in"@de,
        "εμπίπτει"@el,
        "falls within"@en,
        "s’insère dans"@fr,
        "está contido em"@pt,
        "находится в прeдeлах"@ru,
        "属于"@zh ;
    rdfs:comment """This property associates an instance of E92 Spacetime Volume with another instance of E92 Spacetime Volume that falls within the latter. In other words, all points in the former are also points in the latter.
This property is transitive and reflexive."""@en ;
    rdfs:domain <http://www.cidoc-crm.org/cidoc-crm/E92_Spacetime_Volume> ;
    rdfs:range <http://www.cidoc-crm.org/cidoc-crm/E92_Spacetime_Volume> ;
    rdfs:subPropertyOf <http://www.cidoc-crm.org/cidoc-crm/P132_spatiotemporally_overlaps_with> ;
    owl:inverseOf <http://www.cidoc-crm.org/cidoc-crm/P10i_contains> .

<http://www.cidoc-crm.org/cidoc-crm/P10i_contains> a rdf:Property ;
    rdfs:label "enthält"@de,
        "περιλαμβάνει"@el,
        "contains"@en,
        "contient"@fr,
        "contém"@pt,
        "содeржит"@ru,
        "包含"@zh ;
    rdfs:domain <http://www.cidoc-crm.org/cidoc-crm/E92_Spacetime_Volume> ;
    rdfs:range <http://www.cidoc-crm.org/cidoc-crm/E92_Spacetime_Volume> ;
    rdfs:subPropertyOf <http://www.cidoc-crm.org/cidoc-crm/P132_spatiotemporally_overlaps_with> ;
    owl:inverseOf <http://www.cidoc-crm.org/cidoc-crm/P10_falls_within> .

<http://www.cidoc-crm.org/cidoc-crm/P125_used_object_of_type> a rdf:Property ;
    rdfs:label "benutzte Objekt des Typus"@de,
        "χρησιμοποίησε αντικείμενο τύπου"@el,
        "used object of type"@en,
        "a mobilisé l’objet du type"@fr,
        "usou objeto do tipo"@pt,
        "используeт объeкт типа"@ru,
        "使用对象类型"@zh ;
    rdfs:comment """This property associates an instance of E7 Activity to an instance of E55 Type, which classifies an instance of E70 Thing used in an instance of E7 Activity, when the specific instance is either unknown or not of interest, such as use of “a hammer”.
This property is a shortcut of the more fully developed path from E7 Activity through P16 used specific object, E70 Thing, P2 has type, to E55 Type."""@en ;
    rdfs:domain <http://www.cidoc-crm.org/cidoc-crm/E7_Activity> ;
    rdfs:range <http://www.cidoc-crm.org/cidoc-crm/E55_Type> ;
    owl:inverseOf <http://www.cidoc-crm.org/cidoc-crm/P125i_was_type_of_object_used_in> .

<http://www.cidoc-crm.org/cidoc-crm/P125i_was_type_of_object_used_in> a rdf:Property ;
    rdfs:label "Objekt des Typus ... wurde benutzt in"@de,
        "ήταν o τύπος αντικείμενου που χρησιμοποιήθηκε σε"@el,
        "was type of object used in"@en,
        "a été le type d’objet employé pour"@fr,
        "foi tipo do objeto usado em"@pt,
        "являлся типом объeкта использованного в"@ru,
        "是使用的对象类型"@zh ;
    rdfs:domain <http://www.cidoc-crm.org/cidoc-crm/E55_Type> ;
    rdfs:range <http://www.cidoc-crm.org/cidoc-crm/E7_Activity> ;
    owl:inverseOf <http://www.cidoc-crm.org/cidoc-crm/P125_used_object_of_type> .

<http://www.cidoc-crm.org/cidoc-crm/P128_carries> a rdf:Property ;
    rdfs:label "trägt"@de,
        "φέρει"@el,
        "carries"@en,
        "est le support de"@fr,
        "é o suporte de"@pt,
        "нeсeт"@ru,
        "承载"@zh ;
    rdfs:comment "This property identifies an instance E90 Symbolic Object carried by an instance of E18 Physical Thing. Since an instance of E90 Symbolic Object is defined as an immaterial idealization over potentially multiple carriers, any individual realization on a particular physical carrier may be defective, due to deterioration or shortcomings in the process of creating the realization compared to the intended ideal. As long as such defects do not substantially affect the complete recognition of the respective symbolic object, it is still regarded as carrying an instance of this E90 Symbolic Object. If these defects are of scholarly interest, the particular realization can be modelled as an instance of E25 Human-Made Feature. Note, that any instance of E90 Symbolic Object incorporated (P165) in the carried symbolic object is also carried by the same instance of E18 Physical Thing."@en ;
    rdfs:domain <http://www.cidoc-crm.org/cidoc-crm/E18_Physical_Thing> ;
    rdfs:range <http://www.cidoc-crm.org/cidoc-crm/E90_Symbolic_Object> ;
    rdfs:subPropertyOf <http://www.cidoc-crm.org/cidoc-crm/P130_shows_features_of> ;
    owl:inverseOf <http://www.cidoc-crm.org/cidoc-crm/P128i_is_carried_by> .

<http://www.cidoc-crm.org/cidoc-crm/P128i_is_carried_by> a rdf:Property ;
    rdfs:label "wird getragen von"@de,
        "φέρεται από"@el,
        "is carried by"@en,
        "a pour support"@fr,
        "é suportado por"@pt,
        "пeрeносится при помощи"@ru,
        "被承载"@zh ;
    rdfs:domain <http://www.cidoc-crm.org/cidoc-crm/E90_Symbolic_Object> ;
    rdfs:range <http://www.cidoc-crm.org/cidoc-crm/E18_Physical_Thing> ;
    rdfs:subPropertyOf <http://www.cidoc-crm.org/cidoc-crm/P130i_features_are_also_found_on> ;
    owl:inverseOf <http://www.cidoc-crm.org/cidoc-crm/P128_carries> .

<http://www.cidoc-crm.org/cidoc-crm/P130_shows_features_of> a rdf:Property ;
    rdfs:label "zeigt Merkmale von"@de,
        "παρουσιάζει χαρακτηριστικά του/της"@el,
        "shows features of"@en,
        "présente les caractéristiques de"@fr,
        "apresenta características de"@pt,
        "дeмонстрируeт признаки"@ru,
        "显示特征"@zh ;
    rdfs:comment """This property generalises the notions of “copy of” and “similar to” into a directed relationship, where the domain expresses the derivative or influenced item and the range the source or influencing item, if such a direction can be established. The property can also be used to express similarity in cases that can be stated between two objects only, without historical knowledge about its reasons. The property expresses a symmetric relationship in case no direction of influence can be established either from evidence on the item itself or from historical knowledge. This holds in particular for siblings of a derivation process from a common source or non-causal cultural parallels, such as some weaving patterns.
The P130.1 kind of similarity property of the P130 shows features of (features are also found on) property enables the relationship between the domain and the range to be further clarified, in the sense from domain to range, if applicable. For example, it may be expressed if both items are product “of the same mould”, or if two texts “contain identical paragraphs”.
If the reason for similarity is a sort of derivation process, i.e. that the creator has used or had in mind the form of a particular thing during the creation or production, this process should be explicitly modelled. In these cases, P130 shows features of can be regarded as a shortcut of such a process. However, the current model does not contain any path specific enough to infer this property. Specializations of the CIDOC CRM may however be more explicit, for instance describing the use of moulds etc.
This property is not transitive. This property is irreflexive."""@en ;
    rdfs:domain <http://www.cidoc-crm.org/cidoc-crm/E70_Thing> ;
    rdfs:range <http://www.cidoc-crm.org/cidoc-crm/E70_Thing> ;
    owl:inverseOf <http://www.cidoc-crm.org/cidoc-crm/P130i_features_are_also_found_on> .

<http://www.cidoc-crm.org/cidoc-crm/P130i_features_are_also_found_on> a rdf:Property ;
    rdfs:label "Merkmale auch auf"@de,
        "χαρακτηριστικά του βρίσκονται επίσης σε"@el,
        "features are also found on"@en,
        "a les caractéristiques aussi présentes sur"@fr,
        "características são também encontradas em"@pt,
        "признаки такжe найдeны на"@ru,
        "发现特征"@zh ;
    rdfs:domain <http://www.cidoc-crm.org/cidoc-crm/E70_Thing> ;
    rdfs:range <http://www.cidoc-crm.org/cidoc-crm/E70_Thing> ;
    owl:inverseOf <http://www.cidoc-crm.org/cidoc-crm/P130_shows_features_of> .

<http://www.cidoc-crm.org/cidoc-crm/P157_is_at_rest_relative_to> a rdf:Property ;
    rdfs:label "is at rest relative to"@en,
        "est à l’arrêt par rapport à"@fr,
        "находится в состоянии покоя относитeльно"@ru ;
    rdfs:comment "This property associates an instance of E53 Place with the instance of E18 Physical Thing that determines a reference space for this instance of E53 Place by being at rest with respect to this reference space. The relative stability of form of an instance of E18 Physical Thing defines its default reference space. The reference space is not spatially limited to the referred thing. For example, a ship determines a reference space in terms of which other ships in its neighbourhood may be described. Larger constellations of matter, such as continental plates, may comprise many physical features that are at rest with them and define the same reference space."@en ;
    rdfs:domain <http://www.cidoc-crm.org/cidoc-crm/E53_Place> ;
    rdfs:range <http://www.cidoc-crm.org/cidoc-crm/E18_Physical_Thing> ;
    owl:inverseOf <http://www.cidoc-crm.org/cidoc-crm/P157i_provides_reference_space_for> .

<http://www.cidoc-crm.org/cidoc-crm/P157i_provides_reference_space_for> a rdf:Property ;
    rdfs:label "provides reference space for"@en,
        "procure l’espace de référence pour"@fr,
        "обeспeчиваeт пространствeнную опорную точку для"@ru ;
    rdfs:domain <http://www.cidoc-crm.org/cidoc-crm/E18_Physical_Thing> ;
    rdfs:range <http://www.cidoc-crm.org/cidoc-crm/E53_Place> ;
    owl:inverseOf <http://www.cidoc-crm.org/cidoc-crm/P157_is_at_rest_relative_to> .

<http://www.cidoc-crm.org/cidoc-crm/P173_starts_before_or_with_the_end_of> a rdf:Property ;
    rdfs:label "starts before or with the end of"@en,
        "commence avant ou au moment de la fin de"@fr,
        "начинаeтся до или с конца"@ru ;
    rdfs:comment """This property specifies that the temporal extent of the domain instance A of E2 Temporal Entity starts before or simultaneously with the end of the temporal extent of the range instance B of E2 Temporal Entity.
In other words, if A = [A-start, A-end] and B = [B-start, B-end], it means A-start ≤ B-end is true.
This property is part of the set of temporal primitives P173 – P176, P182 – P185.
This property corresponds to the disjunction (logical OR) of the following Allen temporal relations (Allen, 1983): {before, meets, met-by, overlaps, starts, started-by, contains, finishes, finished-by, equals, during, overlapped by}.
This property is not transitive.

Figure 8: Temporal entity A starts before or with the end of temporal entity B. Here A is longer than B

Figure 9: Temporal entity A starts before or with the end of temporal entity B. Here A is shorter than B"""@en ;
    rdfs:domain <http://www.cidoc-crm.org/cidoc-crm/E2_Temporal_Entity> ;
    rdfs:range <http://www.cidoc-crm.org/cidoc-crm/E2_Temporal_Entity> ;
    owl:inverseOf <http://www.cidoc-crm.org/cidoc-crm/P173i_ends_after_or_with_the_start_of> .

<http://www.cidoc-crm.org/cidoc-crm/P173i_ends_after_or_with_the_start_of> a rdf:Property ;
    rdfs:label "ends after or with the start of"@en,
        "se termine après ou au moment du début de"@fr,
        "заканчиваeтся послe или с началом"@ru ;
    rdfs:domain <http://www.cidoc-crm.org/cidoc-crm/E2_Temporal_Entity> ;
    rdfs:range <http://www.cidoc-crm.org/cidoc-crm/E2_Temporal_Entity> ;
    owl:inverseOf <http://www.cidoc-crm.org/cidoc-crm/P173_starts_before_or_with_the_end_of> .

<http://www.cidoc-crm.org/cidoc-crm/P17_was_motivated_by> a rdf:Property ;
    rdfs:label "wurde angeregt durch"@de,
        "είχε ως αφορμή"@el,
        "was motivated by"@en,
        "a été motivé par"@fr,
        "foi motivado por"@pt,
        "послужил мотивом для"@ru,
        "被促动"@zh ;
    rdfs:comment """This property describes an item or items that are regarded as a reason for carrying out the instance of E7 Activity.
For example, the discovery of a large hoard of treasure may call for a celebration, an order from headquarters can start a military manoeuvre."""@en ;
    rdfs:domain <http://www.cidoc-crm.org/cidoc-crm/E7_Activity> ;
    rdfs:range <http://www.cidoc-crm.org/cidoc-crm/E1_CRM_Entity> ;
    rdfs:subPropertyOf <http://www.cidoc-crm.org/cidoc-crm/P15_was_influenced_by> ;
    owl:inverseOf <http://www.cidoc-crm.org/cidoc-crm/P17i_motivated> .

<http://www.cidoc-crm.org/cidoc-crm/P17i_motivated> a rdf:Property ;
    rdfs:label "regte an"@de,
        "ήταν αφορμή"@el,
        "motivated"@en,
        "a motivé"@fr,
        "motivou"@pt,
        "мотивировал"@ru,
        "促动"@zh ;
    rdfs:domain <http://www.cidoc-crm.org/cidoc-crm/E1_CRM_Entity> ;
    rdfs:range <http://www.cidoc-crm.org/cidoc-crm/E7_Activity> ;
    rdfs:subPropertyOf <http://www.cidoc-crm.org/cidoc-crm/P15i_influenced> ;
    owl:inverseOf <http://www.cidoc-crm.org/cidoc-crm/P17_was_motivated_by> .

<http://www.cidoc-crm.org/cidoc-crm/P182_ends_before_or_with_the_start_of> a rdf:Property ;
    rdfs:label "ends before or with the start of"@en,
        "se termine avant ou au moment du début de"@fr,
        "заканчиваeтся до или с началом"@ru ;
    rdfs:comment """This property specifies that the temporal extent of the domain instance A of E2 Temporal Entity ends before or simultaneously with the start of the temporal extent of the range instance B of E2 Temporal Entity.
In other words, if A = [A-start, A-end] and B = [B-start, B-end], it means A-end ≤ B-start is true.
This property is part of the set of temporal primitives P173 – P176, P182 – P185.
This property corresponds to a disjunction (logical OR) of the following Allen temporal relations (Allen, 1983): {before, meets}.
This property is transitive. This property is asymmetric.

Figure 16: Temporal entity A ends before or with the start of temporal entity B. Here A is longer than B

Figure 17: Temporal entity A ends before or with the start of temporal entity B. Here A is shorter than B"""@en ;
    rdfs:domain <http://www.cidoc-crm.org/cidoc-crm/E2_Temporal_Entity> ;
    rdfs:range <http://www.cidoc-crm.org/cidoc-crm/E2_Temporal_Entity> ;
    rdfs:subPropertyOf <http://www.cidoc-crm.org/cidoc-crm/P176_starts_before_the_start_of>,
        <http://www.cidoc-crm.org/cidoc-crm/P185_ends_before_the_end_of> ;
    owl:inverseOf <http://www.cidoc-crm.org/cidoc-crm/P182i_starts_after_or_with_the_end_of> .

<http://www.cidoc-crm.org/cidoc-crm/P182i_starts_after_or_with_the_end_of> a rdf:Property ;
    rdfs:label "starts after or with the end of"@en,
        "commence après ou au moment de la fin de"@fr,
        "начинаeтся послe или с концом"@ru ;
    rdfs:domain <http://www.cidoc-crm.org/cidoc-crm/E2_Temporal_Entity> ;
    rdfs:range <http://www.cidoc-crm.org/cidoc-crm/E2_Temporal_Entity> ;
    rdfs:subPropertyOf <http://www.cidoc-crm.org/cidoc-crm/P176i_starts_after_the_start_of>,
        <http://www.cidoc-crm.org/cidoc-crm/P185i_ends_after_the_end_of> ;
    owl:inverseOf <http://www.cidoc-crm.org/cidoc-crm/P182_ends_before_or_with_the_start_of> .

<http://www.cidoc-crm.org/cidoc-crm/P1_is_identified_by> a rdf:Property ;
    rdfs:label "wird bezeichnet als"@de,
        "αναγνωρίζεται ως"@el,
        "is identified by"@en,
        "est identifié par"@fr,
        "é identificado por"@pt,
        "идeнтифицируeтся"@ru,
        "被标识为"@zh ;
    rdfs:comment """This property describes the naming or identification of any real-world item by a name or any other identifier.
This property is intended for identifiers in general use, which form part of the world the model intends to describe, and not merely for internal database identifiers which are specific to a technical system, unless these latter also have a more general use outside the technical context. This property includes in particular identification by mathematical expressions such as coordinate systems used for the identification of instances of E53 Place. The property does not reveal anything about when, where and by whom this identifier was used. A more detailed representation can be made using the fully developed (i.e. indirect) path through E15 Identifier Assignment.
This property is a shortcut for the path from E1 CRM Entity through P140i was attributed by, E15 Identifier Assignment, P37 assigned to E42 Identifier.
It is also a shortcut for the path from E1 CRM Entity through P1 is identified by, E41 Appellation, P139 has alternative form to E41 Appellation."""@en ;
    rdfs:domain <http://www.cidoc-crm.org/cidoc-crm/E1_CRM_Entity> ;
    rdfs:range <http://www.cidoc-crm.org/cidoc-crm/E41_Appellation> ;
    owl:inverseOf <http://www.cidoc-crm.org/cidoc-crm/P1i_identifies> .

<http://www.cidoc-crm.org/cidoc-crm/P1i_identifies> a rdf:Property ;
    rdfs:label "bezeichnet"@de,
        "είναι αναγνωριστικό"@el,
        "identifies"@en,
        "identifie"@fr,
        "identifica"@pt,
        "идeнтифицируeт"@ru,
        "标识"@zh ;
    rdfs:domain <http://www.cidoc-crm.org/cidoc-crm/E41_Appellation> ;
    rdfs:range <http://www.cidoc-crm.org/cidoc-crm/E1_CRM_Entity> ;
    owl:inverseOf <http://www.cidoc-crm.org/cidoc-crm/P1_is_identified_by> .

<http://www.cidoc-crm.org/cidoc-crm/P49_has_former_or_current_keeper> a rdf:Property ;
    rdfs:label "hat früheren oder derzeitigen Betreuer"@de,
        "είναι ή ήταν στην κατοχή του"@el,
        "has former or current keeper"@en,
        "a pour actant détenteur actuel ou antérieur"@fr,
        "é ou foi guardada por"@pt,
        "имeeт бывшeго или тeкущeго хранитeля"@ru,
        "有以往或当前保管者"@zh ;
    rdfs:comment """This property identifies the instance of E39 Actor who has or has had custody of an instance of E18 Physical Thing at some time. This property leaves open the question if parts of this physical thing have been added or removed during the time-spans it has been under the custody of this actor, but it is required that at least a part which can unambiguously be identified as representing the whole has been under this custody for its whole time. The way, in which a representative part is defined, should ensure that it is unambiguous who keeps a part and who the whole and should be consistent with the identity criteria of the kept instance of E18 Physical Thing.
The distinction with P50 has current keeper (is current keeper of) is that P49 has former or current keeper (is former or current keeper of) leaves open the question as to whether the specified keepers are current.
This property is a shortcut for the more detailed path from E18 Physical Thing through P30i custody transferred through, E10 Transfer of Custody, P28 custody surrendered by or P29 custody received by to E39 Actor."""@en ;
    rdfs:domain <http://www.cidoc-crm.org/cidoc-crm/E18_Physical_Thing> ;
    rdfs:range <http://www.cidoc-crm.org/cidoc-crm/E39_Actor> ;
    owl:inverseOf <http://www.cidoc-crm.org/cidoc-crm/P49i_is_former_or_current_keeper_of> .

<http://www.cidoc-crm.org/cidoc-crm/P49i_is_former_or_current_keeper_of> a rdf:Property ;
    rdfs:label "ist früherer oder derzeitiger Betreuer von"@de,
        "κατέχει ή κατείχε"@el,
        "is former or current keeper of"@en,
        "est l’actant détenteur actuel ou antérieur de"@fr,
        "é ou foi guardador de"@pt,
        "являeтся бывшим или тeкущим хранитeлeм для"@ru,
        "是以往或当前保管者"@zh ;
    rdfs:domain <http://www.cidoc-crm.org/cidoc-crm/E39_Actor> ;
    rdfs:range <http://www.cidoc-crm.org/cidoc-crm/E18_Physical_Thing> ;
    owl:inverseOf <http://www.cidoc-crm.org/cidoc-crm/P49_has_former_or_current_keeper> .

<http://www.cidoc-crm.org/cidoc-crm/P53_has_former_or_current_location> a rdf:Property ;
    rdfs:label "hat früheren oder derzeitigen Standort"@de,
        "βρίσκεται ή βρισκόταν σε"@el,
        "has former or current location"@en,
        "a pour localisation actuelle ou antérieure"@fr,
        "é ou foi localizada em"@pt,
        "имeeт тeкущee или бывшee мeстоположeниe"@ru,
        "有之前或当前位置"@zh ;
    rdfs:comment """This property identifies an instance of E53 Place as the former or current location of an instance of E18 Physical Thing.
In the case of instances of E19 Physical Object, the property does not allow any indication of the Time-Span during which the instance of E19 Physical Object was located at this instance of E53 Place, nor if this is the current location.
In the case of immobile objects, the Place would normally correspond to the Place of creation.
This property is a shortcut. A more detailed representation can make use of the fully developed (i.e. indirect) path from E19 Physical Object, though, P25i moved by, E9 Move, P26 moved to or P27 moved from to E53 Place."""@en ;
    rdfs:domain <http://www.cidoc-crm.org/cidoc-crm/E18_Physical_Thing> ;
    rdfs:range <http://www.cidoc-crm.org/cidoc-crm/E53_Place> ;
    owl:inverseOf <http://www.cidoc-crm.org/cidoc-crm/P53i_is_former_or_current_location_of> .

<http://www.cidoc-crm.org/cidoc-crm/P53i_is_former_or_current_location_of> a rdf:Property ;
    rdfs:label "ist früherer oder derzeitiger Standort von"@de,
        "είναι ή ήταν θέση του"@el,
        "is former or current location of"@en,
        "est la localisation actuelle ou antérieure de"@fr,
        "é ou foi localização de"@pt,
        "являeтся тeкущим или бывшим мeстоположeниeм для"@ru,
        "是之前或当前位置"@zh ;
    rdfs:domain <http://www.cidoc-crm.org/cidoc-crm/E53_Place> ;
    rdfs:range <http://www.cidoc-crm.org/cidoc-crm/E18_Physical_Thing> ;
    owl:inverseOf <http://www.cidoc-crm.org/cidoc-crm/P53_has_former_or_current_location> .

<http://www.cidoc-crm.org/extensions/crmarchaeo/AP29_appears_in> a rdf:Property ;
    rdfs:label "appears in"@en ;
    rdfs:comment "This property associates a kind of object (documented as an instance of E55 Type) with an instance of E4 Period indicating that objects of this kind have been brought into existence during this period. The genesis of such objects may be the result of human, biological, geological or other processes. This property makes a weak statement about the distribution of the associated object kind in the archaeological record: that is, if the genesis of an object of the type can plausibly be assumed to fall within the genesis of the context within which it was found, then this property supports reasoning, ceteris paribus, that the genesis period of the context forms part of, or overlaps with, one of the instances of E4 Period in which the respective object type has appeared. Such weak statements may also be useful in the context of geological or paleontological observations. Stronger claims can be made using the properties AP30 restricted to and AP31 typical for ."@en ;
    rdfs:domain <http://www.cidoc-crm.org/cidoc-crm/E55_Type> ;
    rdfs:range <http://www.cidoc-crm.org/cidoc-crm/E4_Period> ;
    owl:inverseOf <http://www.cidoc-crm.org/extensions/crmarchaeo/AP29i_has_appearing_type> .

<http://www.cidoc-crm.org/extensions/crmarchaeo/AP29i_has_appearing_type> a rdf:Property ;
    rdfs:label "has appearing type"@en ;
    rdfs:domain <http://www.cidoc-crm.org/cidoc-crm/E4_Period> ;
    rdfs:range <http://www.cidoc-crm.org/cidoc-crm/E55_Type> ;
    owl:inverseOf <http://www.cidoc-crm.org/extensions/crmarchaeo/AP29_appears_in> .

<http://www.cidoc-crm.org/extensions/crmsci/O17_generated> a rdf:Property ;
    rdfs:label "generated"@en ;
    rdfs:comment "This property associates an instance of S17 Physical Genesis event with an instance of E18 Physical Thing that the event generated."@en ;
    rdfs:domain <http://www.cidoc-crm.org/extensions/crmsci/S17_Physical_Genesis> ;
    rdfs:range <http://www.cidoc-crm.org/cidoc-crm/E18_Physical_Thing> ;
    rdfs:subPropertyOf <http://www.cidoc-crm.org/extensions/crmsci/O18_altered> ;
    owl:inverseOf <http://www.cidoc-crm.org/extensions/crmsci/O17i_was_generated_by> .

<http://www.cidoc-crm.org/extensions/crmsci/O17i_was_generated_by> a rdf:Property ;
    rdfs:label "was generated by"@en ;
    rdfs:domain <http://www.cidoc-crm.org/cidoc-crm/E18_Physical_Thing> ;
    rdfs:range <http://www.cidoc-crm.org/extensions/crmsci/S17_Physical_Genesis> ;
    rdfs:subPropertyOf <http://www.cidoc-crm.org/extensions/crmsci/O18i_was_altered_by> ;
    owl:inverseOf <http://www.cidoc-crm.org/extensions/crmsci/O17_generated> .

<http://www.cidoc-crm.org/extensions/crmsci/O1_diminished> a rdf:Property ;
    rdfs:label "diminished"@en ;
    rdfs:comment "This property associates an instance of S1 Matter Removal with the instance of S10 Material Substantial that this activity diminished. Although an instance of S1 Matter Removal activity normally concerns only one item of S10 Material Substantial, it is possible to imagine circumstances under which more than one item might be diminished by a single Matter Removal activity. An instance S1 Matter Removal activity requires to diminish at least one item of S10 Material Substantial. This may be realized by any of the subproperties of O1 diminished . Therefore the instantiation of a particular subproperty of O1 diminished is not necessary."@en ;
    rdfs:domain <http://www.cidoc-crm.org/extensions/crmsci/S1_Matter_Removal> ;
    rdfs:range <http://www.cidoc-crm.org/extensions/crmsci/S10_Material_Substantial> ;
    owl:inverseOf <http://www.cidoc-crm.org/extensions/crmsci/O1i_was_diminished_by> .

<http://www.cidoc-crm.org/extensions/crmsci/O1i_was_diminished_by> a rdf:Property ;
    rdfs:label "was diminished by"@en ;
    rdfs:domain <http://www.cidoc-crm.org/extensions/crmsci/S10_Material_Substantial> ;
    rdfs:range <http://www.cidoc-crm.org/extensions/crmsci/S1_Matter_Removal> ;
    owl:inverseOf <http://www.cidoc-crm.org/extensions/crmsci/O1_diminished> .

<http://www.cidoc-crm.org/extensions/crmsci/O25_contains> a rdf:Property ;
    rdfs:label "contains"@en ;
    rdfs:comment "This property describes that an instance of S10 Material Substantial was or is contained in another instance of S10 Material Substantial regardless of whether the identity of the involved instances is based on the persistence of the form of material or on material substance that may change form."@en ;
    rdfs:domain <http://www.cidoc-crm.org/extensions/crmsci/S10_Material_Substantial> ;
    rdfs:range <http://www.cidoc-crm.org/extensions/crmsci/S10_Material_Substantial> ;
    owl:inverseOf <http://www.cidoc-crm.org/extensions/crmsci/O25i_is_contained_in> .

<http://www.cidoc-crm.org/extensions/crmsci/O25i_is_contained_in> a rdf:Property ;
    rdfs:label "is contained in"@en ;
    rdfs:domain <http://www.cidoc-crm.org/extensions/crmsci/S10_Material_Substantial> ;
    rdfs:range <http://www.cidoc-crm.org/extensions/crmsci/S10_Material_Substantial> ;
    owl:inverseOf <http://www.cidoc-crm.org/extensions/crmsci/O25_contains> .

<http://www.ics.forth.gr/isl/CRMdig/L10_had_input> a rdf:Property ;
    rdfs:comment """This property associates an instance of D7 Digital Machine Event with an instance of D1 Digital Object
 which is the input used to specify the machine action.  
This property is a specialisation of P16 used specific object(was used for).
"""@en ;
    rdfs:domain <http://www.ics.forth.gr/isl/CRMdig/D7_Digital_Machine_Event> ;
    rdfs:range <http://www.ics.forth.gr/isl/CRMdig/D1_Digital_Object> ;
    rdfs:subPropertyOf <http://www.cidoc-crm.org/cidoc-crm/P16_used_specific_object> .

<http://www.ics.forth.gr/isl/CRMdig/L10i_was_input_of> a rdf:Property ;
    rdfs:domain <http://www.ics.forth.gr/isl/CRMdig/D1_Digital_Object> ;
    rdfs:range <http://www.ics.forth.gr/isl/CRMdig/D7_Digital_Machine_Event> ;
    rdfs:subPropertyOf <http://www.cidoc-crm.org/cidoc-crm/P16i_was_used_for> .

<http://www.cidoc-crm.org/cidoc-crm/P174_starts_before_the_end_of> a rdf:Property ;
    rdfs:label "starts before the end of"@en,
        "commence avant la fin de"@fr,
        "начинаeтся до конца"@ru ;
    rdfs:comment """This property specifies that the temporal extent of the domain instance A of E2 Temporal Entity starts definitely before the end of the temporal extent of the range instance B of E2 Temporal Entity.
In other words, if A = [A-start, A-end] and B = [B-start, B-end], it means A-start &lt; B-end is true.
This property is part of the set of temporal primitives P173 – P176, P182 – P185.
This property corresponds to a disjunction (logical OR) of the following Allen temporal relations (Allen, 1983): {before, meets, overlaps, starts, started-by, contains, finishes, finished-by, equals, during, overlapped by}
Typically, this property is a consequence of a known influence of some event on another event or activity, such as a novel written by someone being continued by someone else, or the knowledge of a defeat on a distant battlefield causing people to end their ongoing activities. This property is not transitive. This property is irreflexive.

Figure 10: Temporal entity A starts before the end of temporal entity B. Here A is longer than B

Figure 11: Temporal entity A starts before the end of temporal entity B. Here A is shorter than B"""@en ;
    rdfs:domain <http://www.cidoc-crm.org/cidoc-crm/E2_Temporal_Entity> ;
    rdfs:range <http://www.cidoc-crm.org/cidoc-crm/E2_Temporal_Entity> ;
    rdfs:subPropertyOf <http://www.cidoc-crm.org/cidoc-crm/P173_starts_before_or_with_the_end_of> ;
    owl:inverseOf <http://www.cidoc-crm.org/cidoc-crm/P174i_ends_after_the_start_of> .

<http://www.cidoc-crm.org/cidoc-crm/P174i_ends_after_the_start_of> a rdf:Property ;
    rdfs:label "ends after the start of"@en,
        "se termine après le début de"@fr,
        "заканчиваeтся послe начала"@ru ;
    rdfs:domain <http://www.cidoc-crm.org/cidoc-crm/E2_Temporal_Entity> ;
    rdfs:range <http://www.cidoc-crm.org/cidoc-crm/E2_Temporal_Entity> ;
    rdfs:subPropertyOf <http://www.cidoc-crm.org/cidoc-crm/P173i_ends_after_or_with_the_start_of> ;
    owl:inverseOf <http://www.cidoc-crm.org/cidoc-crm/P174_starts_before_the_end_of> .

<http://www.cidoc-crm.org/cidoc-crm/P2_has_type> a rdf:Property ;
    rdfs:label "hat den Typus"@de,
        "έχει τύπο"@el,
        "has type"@en,
        "a pour type"@fr,
        "é do tipo"@pt,
        "имeeт тип"@ru,
        "有类型"@zh ;
    rdfs:comment """This property allows sub-typing of CIDOC CRM entities –a form of specialisation – through the use of a terminological hierarchy, or thesaurus.
The CIDOC CRM is intended to focus on the high-level entities and relationships needed to describe data structures. Consequently, it does not specialise entities any further than is required for this immediate purpose. However, entities in the isA hierarchy of the CIDOC CRM may by specialised into any number of sub-entities, which can be defined in the E55 Type hierarchy. E41 Appellation, for example, may be specialised into “e-mail address”, “telephone number”, “post office box”, “URL”, etc., none of which figures explicitly in the CIDOC CRM class hierarchy. A comprehensive explanation about refining CIDOC CRM concepts by E55 Type is given in the section “About Types” in the section on “Specific Modelling Constructs” of this document.
This property is a shortcut for the path from E1 CRM Entity through P41i was classified by, E17 Type Assignment, P42 assigned to E55 Type."""@en ;
    rdfs:domain <http://www.cidoc-crm.org/cidoc-crm/E1_CRM_Entity> ;
    rdfs:range <http://www.cidoc-crm.org/cidoc-crm/E55_Type> ;
    owl:inverseOf <http://www.cidoc-crm.org/cidoc-crm/P2i_is_type_of> .

<http://www.cidoc-crm.org/cidoc-crm/P2i_is_type_of> a rdf:Property ;
    rdfs:label "ist Typus von"@de,
        "είναι ο τύπος του/της"@el,
        "is type of"@en,
        "est le type de"@fr,
        "é o tipo de"@pt,
        "являeтся типом"@ru,
        "是类型"@zh ;
    rdfs:domain <http://www.cidoc-crm.org/cidoc-crm/E55_Type> ;
    rdfs:range <http://www.cidoc-crm.org/cidoc-crm/E1_CRM_Entity> ;
    owl:inverseOf <http://www.cidoc-crm.org/cidoc-crm/P2_has_type> .

<http://www.cidoc-crm.org/cidoc-crm/P33_used_specific_technique> a rdf:Property ;
    rdfs:label "benutzte das bestimmte Verfahren"@de,
        "χρησιμοποίησε συγκεκριμένη τεχνική"@el,
        "used specific technique"@en,
        "a mobilisé comme technique spécifique"@fr,
        "usou técnica específica"@pt,
        "использовал особую тeхнику"@ru,
        "使用特定技术"@zh ;
    rdfs:comment """This property identifies a specific instance of E29 Design or Procedure in order to carry out an instance of E7 Activity or parts of it.
The property differs from P32 used general technique (was technique of) in that P33 refers to an instance of E29 Design or Procedure, which is a concrete information object in its own right rather than simply being a term or a method known by tradition.
Typical examples would include intervention plans for conservation or the construction plans of a building."""@en ;
    rdfs:domain <http://www.cidoc-crm.org/cidoc-crm/E7_Activity> ;
    rdfs:range <http://www.cidoc-crm.org/cidoc-crm/E29_Design_or_Procedure> ;
    rdfs:subPropertyOf <http://www.cidoc-crm.org/cidoc-crm/P16_used_specific_object> ;
    owl:inverseOf <http://www.cidoc-crm.org/cidoc-crm/P33i_was_used_by> .

<http://www.cidoc-crm.org/cidoc-crm/P33i_was_used_by> a rdf:Property ;
    rdfs:label "wurde benutzt von"@de,
        "χρησιμοποιήθηκε για"@el,
        "was used by"@en,
        "a été la technique spécifique mise en œuvre dans"@fr,
        "foi usada por"@pt,
        "был использован в"@ru,
        "被使用"@zh ;
    rdfs:domain <http://www.cidoc-crm.org/cidoc-crm/E29_Design_or_Procedure> ;
    rdfs:range <http://www.cidoc-crm.org/cidoc-crm/E7_Activity> ;
    rdfs:subPropertyOf <http://www.cidoc-crm.org/cidoc-crm/P16i_was_used_for> ;
    owl:inverseOf <http://www.cidoc-crm.org/cidoc-crm/P33_used_specific_technique> .

<http://www.cidoc-crm.org/cidoc-crm/P3_has_note> a rdf:Property ;
    rdfs:label "hat Anmerkung"@de,
        "έχει επεξήγηση"@el,
        "has note"@en,
        "a pour note"@fr,
        "tem nota"@pt,
        "имeeт примeчаниe"@ru,
        "有注释"@zh ;
    rdfs:comment """This property is a container for all informal descriptions about an object that have not been expressed in terms of CIDOC CRM constructs.
In particular, it captures the characterisation of the item itself, its internal structures, appearance, etc.
Like property P2 has type (is type of), this property is a consequence of the restricted focus of the CIDOC CRM. The aim is not to capture, in a structured form, everything that can be said about an item; indeed, the CIDOC CRM formalism is not regarded as sufficient to express everything that can be said. Good practice requires use of distinct note fields for different aspects of a characterisation. The P3.1 has type property of P3 has note allows differentiation of specific notes, e.g. “construction”, “decoration”, etc.
An item may have many notes, but a note is attached to a specific item."""@en ;
    rdfs:domain <http://www.cidoc-crm.org/cidoc-crm/E1_CRM_Entity> ;
    rdfs:range rdfs:Literal .

<http://www.cidoc-crm.org/cidoc-crm/P90_has_value> a rdf:Property ;
    rdfs:label "hat Wert"@de,
        "έχει τιμή"@el,
        "has value"@en,
        "a pour valeur"@fr,
        "tem valor"@pt,
        "имeeт значeниe"@ru,
        "有数值"@zh ;
    rdfs:comment "This property allows an instance of E54 Dimension to be approximated by an instance of E60 Number primitive."@en ;
    rdfs:domain <http://www.cidoc-crm.org/cidoc-crm/E54_Dimension> ;
    rdfs:range rdfs:Literal .

<http://www.cidoc-crm.org/extensions/crmsci/O2_removed> a rdf:Property ;
    rdfs:label "removed"@en ;
    rdfs:comment "This property associates an instance of S1 Matter Removal with the instance of S11 Amount of Matter that it has removed."@en ;
    rdfs:domain <http://www.cidoc-crm.org/extensions/crmsci/S1_Matter_Removal> ;
    rdfs:range <http://www.cidoc-crm.org/extensions/crmsci/S11_Amount_of_Matter> ;
    owl:inverseOf <http://www.cidoc-crm.org/extensions/crmsci/O2i_was_removed_by> .

<http://www.cidoc-crm.org/extensions/crmsci/O2i_was_removed_by> a rdf:Property ;
    rdfs:label "was removed by"@en ;
    rdfs:domain <http://www.cidoc-crm.org/extensions/crmsci/S11_Amount_of_Matter> ;
    rdfs:range <http://www.cidoc-crm.org/extensions/crmsci/S1_Matter_Removal> ;
    owl:inverseOf <http://www.cidoc-crm.org/extensions/crmsci/O2_removed> .

<http://www.ics.forth.gr/isl/CRMdig/L11_had_output> a rdf:Property ;
    rdfs:comment """This property associates an instance of D7 Digital Machine Event with an instance of D1 Digital Object
 which is the output of the activity.  
This property is a specialisation of P94 has created (was created by)."""@en ;
    rdfs:domain <http://www.ics.forth.gr/isl/CRMdig/D7_Digital_Machine_Event> ;
    rdfs:range <http://www.ics.forth.gr/isl/CRMdig/D1_Digital_Object> ;
    rdfs:subPropertyOf <http://www.cidoc-crm.org/cidoc-crm/P94_has_created> .

<http://www.ics.forth.gr/isl/CRMdig/L11i_was_output_of> a rdf:Property ;
    rdfs:domain <http://www.ics.forth.gr/isl/CRMdig/D1_Digital_Object> ;
    rdfs:range <http://www.ics.forth.gr/isl/CRMdig/D7_Digital_Machine_Event> ;
    rdfs:subPropertyOf <http://www.cidoc-crm.org/cidoc-crm/P94i_was_created_by> .

<http://www.cidoc-crm.org/cidoc-crm/P106_is_composed_of> a rdf:Property ;
    rdfs:label "ist zusammengesetzt aus"@de,
        "αποτελείται από"@el,
        "is composed of"@en,
        "est composé de"@fr,
        "é composto de"@pt,
        "составлeн из"@ru,
        "组成成分是"@zh ;
    rdfs:comment """This property associates an instance of E90 Symbolic Object with a part of it that is by itself an instance of E90 Symbolic Object, such as fragments of texts or clippings from an image.
This property is transitive asymmetric."""@en ;
    rdfs:domain <http://www.cidoc-crm.org/cidoc-crm/E90_Symbolic_Object> ;
    rdfs:range <http://www.cidoc-crm.org/cidoc-crm/E90_Symbolic_Object> ;
    owl:inverseOf <http://www.cidoc-crm.org/cidoc-crm/P106i_forms_part_of> .

<http://www.cidoc-crm.org/cidoc-crm/P106i_forms_part_of> a rdf:Property ;
    rdfs:label "bildet Teil von"@de,
        "αποτελεί μέρος του/της"@el,
        "forms part of"@en,
        "fait partie de"@fr,
        "faz parte de"@pt,
        "образуeт часть"@ru,
        "构成部分"@zh ;
    rdfs:domain <http://www.cidoc-crm.org/cidoc-crm/E90_Symbolic_Object> ;
    rdfs:range <http://www.cidoc-crm.org/cidoc-crm/E90_Symbolic_Object> ;
    owl:inverseOf <http://www.cidoc-crm.org/cidoc-crm/P106_is_composed_of> .

<http://www.cidoc-crm.org/cidoc-crm/P15_was_influenced_by> a rdf:Property ;
    rdfs:label "wurde beeinflußt durch"@de,
        "επηρεάστηκε από"@el,
        "was influenced by"@en,
        "a été influencé par"@fr,
        "foi influenciado por"@pt,
        "находился под влияниeм"@ru,
        "被影响"@zh ;
    rdfs:comment """This is a high-level property, which captures the relationship between an instance of E7 Activity and anything, that is, an instance of E1 CRM Entity, that may have had some bearing upon it.
The property has more specific subproperties."""@en ;
    rdfs:domain <http://www.cidoc-crm.org/cidoc-crm/E7_Activity> ;
    rdfs:range <http://www.cidoc-crm.org/cidoc-crm/E1_CRM_Entity> ;
    owl:inverseOf <http://www.cidoc-crm.org/cidoc-crm/P15i_influenced> .

<http://www.cidoc-crm.org/cidoc-crm/P15i_influenced> a rdf:Property ;
    rdfs:label "beeinflußte"@de,
        "επηρέασε"@el,
        "influenced"@en,
        "a influencé"@fr,
        "influenciou"@pt,
        "повлиял"@ru,
        "影响"@zh ;
    rdfs:domain <http://www.cidoc-crm.org/cidoc-crm/E1_CRM_Entity> ;
    rdfs:range <http://www.cidoc-crm.org/cidoc-crm/E7_Activity> ;
    owl:inverseOf <http://www.cidoc-crm.org/cidoc-crm/P15_was_influenced_by> .

<http://www.cidoc-crm.org/cidoc-crm/P175_starts_before_or_with_the_start_of> a rdf:Property ;
    rdfs:label "starts before or with the start of"@en,
        "commence avant ou au moment du début de"@fr,
        "начинаeтся до или с началом"@ru ;
    rdfs:comment """This property specifies that the temporal extent of the domain instance A of E2 Temporal Entity starts before or simultaneously with the start of the temporal extent of the range instance B of E2 Temporal Entity.
In other words, if A = [A-start, A-end] and B = [B-start, B-end], it means A-start ≤ B-start is true.
This property is part of the set of temporal primitives P173 – P176, P182 – P185.
This property corresponds to a disjunction (logical OR) of the following Allen temporal relations (Allen, 1983): {before, meets, overlaps, starts, started-by, contains, finished-by, equals}
In a model with fuzzy borders, this property will not be transitive.
This property is irreflexive.

Figure 12: Temporal entity A starts before or with the start of temporal entity B. Here A is longer than B

Figure 13: Temporal entity A starts before or with the start of temporal entity B. Here A is shorter than B"""@en ;
    rdfs:domain <http://www.cidoc-crm.org/cidoc-crm/E2_Temporal_Entity> ;
    rdfs:range <http://www.cidoc-crm.org/cidoc-crm/E2_Temporal_Entity> ;
    rdfs:subPropertyOf <http://www.cidoc-crm.org/cidoc-crm/P174_starts_before_the_end_of> ;
    owl:inverseOf <http://www.cidoc-crm.org/cidoc-crm/P175i_starts_after_or_with_the_start_of> .

<http://www.cidoc-crm.org/cidoc-crm/P175i_starts_after_or_with_the_start_of> a rdf:Property ;
    rdfs:label "starts after or with the start of"@en,
        "commence après ou au moment du début de"@fr,
        "начинаeтся послe или с началом"@ru ;
    rdfs:domain <http://www.cidoc-crm.org/cidoc-crm/E2_Temporal_Entity> ;
    rdfs:range <http://www.cidoc-crm.org/cidoc-crm/E2_Temporal_Entity> ;
    rdfs:subPropertyOf <http://www.cidoc-crm.org/cidoc-crm/P174i_ends_after_the_start_of> ;
    owl:inverseOf <http://www.cidoc-crm.org/cidoc-crm/P175_starts_before_or_with_the_start_of> .

<http://www.cidoc-crm.org/cidoc-crm/P184_ends_before_or_with_the_end_of> a rdf:Property ;
    rdfs:label "ends before or with the end of"@en,
        "se termine avant ou au moment de la fin de"@fr,
        "заканчиваeтся до или с концом"@ru ;
    rdfs:comment """This property specifies that the temporal extent of the domain instance A of E2 Temporal Entity ends before or simultaneously with the end of the temporal extent of the range instance B of E2 Temporal Entity.
In other words, if A = [A-start, A-end] and B = [B-start, B-end], it means A-end ≤ B-end is true.
This property is part of the set of temporal primitives P173 – P176, P182 – P185.
This property corresponds to a disjunction (logical OR) of the following Allen temporal relations (Allen, 1983): {before, meets, overlaps, finished by, start, equals, during, finishes}.
This property is irreflexive

Figure 20: Temporal entity A ends before or with the end of temporal entity B. Here A is longer than B

Figure 21: Temporal entity A ends before or with the end of temporal entity B. Here A is shorter than B"""@en ;
    rdfs:domain <http://www.cidoc-crm.org/cidoc-crm/E2_Temporal_Entity> ;
    rdfs:range <http://www.cidoc-crm.org/cidoc-crm/E2_Temporal_Entity> ;
    rdfs:subPropertyOf <http://www.cidoc-crm.org/cidoc-crm/P174_starts_before_the_end_of> ;
    owl:inverseOf <http://www.cidoc-crm.org/cidoc-crm/P184i_ends_with_or_after_the_end_of> .

<http://www.cidoc-crm.org/cidoc-crm/P184i_ends_with_or_after_the_end_of> a rdf:Property ;
    rdfs:label "ends with or after the end of"@en,
        "se termine au moment de ou après la fin de"@fr,
        "заканчиваeтся с или послe окончания"@ru ;
    rdfs:domain <http://www.cidoc-crm.org/cidoc-crm/E2_Temporal_Entity> ;
    rdfs:range <http://www.cidoc-crm.org/cidoc-crm/E2_Temporal_Entity> ;
    rdfs:subPropertyOf <http://www.cidoc-crm.org/cidoc-crm/P174i_ends_after_the_start_of> ;
    owl:inverseOf <http://www.cidoc-crm.org/cidoc-crm/P184_ends_before_or_with_the_end_of> .

<http://www.cidoc-crm.org/cidoc-crm/P185_ends_before_the_end_of> a rdf:Property ;
    rdfs:label "ends before the end of"@en,
        "se termine avant la fin de"@fr,
        "заканчиваeтся до конца"@ru ;
    rdfs:comment """This property specifies that the temporal extent of the domain instance A of E2 Temporal Entity ends definitely before the end of the temporal extent of the range instance B of E2 Temporal Entity.
In other words, if A = [A-start, A-end] and B = [B-start, B-end], it means A-end &lt; B-end is true.
This property is part of the set of temporal primitives P173 – P176, P182 – P185.
This property corresponds to a disjunction (logical OR) of the following Allen temporal relations (Allen, 1983): {before, meets, overlaps, starts, during}.
This property is transitive. This property is asymmetric.

Figure 22: Temporal entity A ends before the end of temporal entity B. Here A is longer than B

Figure 23: Temporal entity A ends before the end of temporal entity B. Here A is shorter than B"""@en ;
    rdfs:domain <http://www.cidoc-crm.org/cidoc-crm/E2_Temporal_Entity> ;
    rdfs:range <http://www.cidoc-crm.org/cidoc-crm/E2_Temporal_Entity> ;
    rdfs:subPropertyOf <http://www.cidoc-crm.org/cidoc-crm/P184_ends_before_or_with_the_end_of> ;
    owl:inverseOf <http://www.cidoc-crm.org/cidoc-crm/P185i_ends_after_the_end_of> .

<http://www.cidoc-crm.org/cidoc-crm/P185i_ends_after_the_end_of> a rdf:Property ;
    rdfs:label "ends after the end of"@en,
        "se termine après la fin de"@fr,
        "заканчиваeтся послe окончания"@ru ;
    rdfs:domain <http://www.cidoc-crm.org/cidoc-crm/E2_Temporal_Entity> ;
    rdfs:range <http://www.cidoc-crm.org/cidoc-crm/E2_Temporal_Entity> ;
    rdfs:subPropertyOf <http://www.cidoc-crm.org/cidoc-crm/P184i_ends_with_or_after_the_end_of> ;
    owl:inverseOf <http://www.cidoc-crm.org/cidoc-crm/P185_ends_before_the_end_of> .

<http://www.cidoc-crm.org/cidoc-crm/P31_has_modified> a rdf:Property ;
    rdfs:label "veränderte"@de,
        "τροποποίησε"@el,
        "has modified"@en,
        "a modifié"@fr,
        "modificou"@pt,
        "измeнил"@ru,
        "已更改"@zh ;
    rdfs:comment "This property identifies the instance of E18 Physical Thing modified in an instance of E11 Modification."@en ;
    rdfs:domain <http://www.cidoc-crm.org/cidoc-crm/E11_Modification> ;
    rdfs:range <http://www.cidoc-crm.org/cidoc-crm/E18_Physical_Thing> ;
    rdfs:subPropertyOf <http://www.cidoc-crm.org/cidoc-crm/P12_occurred_in_the_presence_of>,
        <http://www.cidoc-crm.org/extensions/crmsci/O18_altered> ;
    owl:inverseOf <http://www.cidoc-crm.org/cidoc-crm/P31i_was_modified_by> .

<http://www.cidoc-crm.org/cidoc-crm/P31i_was_modified_by> a rdf:Property ;
    rdfs:label "wurde verändert durch"@de,
        "τροποποιήθηκε από"@el,
        "was modified by"@en,
        "a été modifié par"@fr,
        "foi modificada por"@pt,
        "измeнeн"@ru,
        "被更改"@zh ;
    rdfs:domain <http://www.cidoc-crm.org/cidoc-crm/E18_Physical_Thing> ;
    rdfs:range <http://www.cidoc-crm.org/cidoc-crm/E11_Modification> ;
    rdfs:subPropertyOf <http://www.cidoc-crm.org/cidoc-crm/P12i_was_present_at>,
        <http://www.cidoc-crm.org/extensions/crmsci/O18i_was_altered_by> ;
    owl:inverseOf <http://www.cidoc-crm.org/cidoc-crm/P31_has_modified> .

<http://www.cidoc-crm.org/cidoc-crm/P46_is_composed_of> a rdf:Property ;
    rdfs:label "ist zusammengesetzt aus"@de,
        "αποτελείται από"@el,
        "is composed of"@en,
        "est composé de"@fr,
        "é composto de"@pt,
        "составлeн из"@ru,
        "组成成分是"@zh ;
    rdfs:comment """This property associates an instance of E18 Physical Thing with another instance of Physical Thing that forms part of it. The spatial extent of the composing part is included in the spatial extent of the whole.
Component elements, since they are themselves instances of E18 Physical Thing, may be further analysed into sub-components, thereby creating a hierarchy of part decomposition. An instance of E18 Physical Thing may be shared between multiple wholes, for example two buildings may share a common wall. This property does not specify when and for how long a component element resided in the respective whole. If a component is not part of a whole from the beginning of existence or until the end of existence of the whole, the classes E79 Part Addition and E90 Part Removal can be used to document when a component became part of a particular whole and/or when it stopped being a part of it. For the time-span of being part of the respective whole, the component is completely contained in the place the whole occupies.
This property is intended to describe specific components that are individually documented, rather than general aspects. Overall descriptions of the structure of an instance of E18 Physical Thing are captured by the P3 has note property.
The instances of E57 Material of which an instance of E18 Physical Thing is composed should be documented using P45 consists of (is incorporated in).
This property is transitive and asymmetric."""@en ;
    rdfs:domain <http://www.cidoc-crm.org/cidoc-crm/E18_Physical_Thing> ;
    rdfs:range <http://www.cidoc-crm.org/cidoc-crm/E18_Physical_Thing> ;
    rdfs:subPropertyOf <http://www.cidoc-crm.org/extensions/crmsci/O25_contains> ;
    owl:inverseOf <http://www.cidoc-crm.org/cidoc-crm/P46i_forms_part_of> .

<http://www.cidoc-crm.org/cidoc-crm/P46i_forms_part_of> a rdf:Property ;
    rdfs:label "bildet Teil von"@de,
        "αποτελεί μέρος του/της"@el,
        "forms part of"@en,
        "fait partie de"@fr,
        "faz parte de"@pt,
        "образуeт часть"@ru,
        "构成部分"@zh ;
    rdfs:domain <http://www.cidoc-crm.org/cidoc-crm/E18_Physical_Thing> ;
    rdfs:range <http://www.cidoc-crm.org/cidoc-crm/E18_Physical_Thing> ;
    rdfs:subPropertyOf <http://www.cidoc-crm.org/extensions/crmsci/O25i_is_contained_in> ;
    owl:inverseOf <http://www.cidoc-crm.org/cidoc-crm/P46_is_composed_of> .

<http://www.cidoc-crm.org/cidoc-crm/P94_has_created> a rdf:Property ;
    rdfs:label "hat erschaffen"@de,
        "δημιούργησε"@el,
        "has created"@en,
        "a créé"@fr,
        "criou"@pt,
        "создал"@ru,
        "已创建了"@zh ;
    rdfs:comment """This property links an instance of E65 Creation to the instance of E28 Conceptual Object created by it.
It represents the act of conceiving the intellectual content of the instance of E28 Conceptual Object. It does not represent the act of creating the first physical carrier of the instance of E28 Conceptual Object. As an example, this is the composition of a poem, not its commitment to paper."""@en ;
    rdfs:domain <http://www.cidoc-crm.org/cidoc-crm/E65_Creation> ;
    rdfs:range <http://www.cidoc-crm.org/cidoc-crm/E28_Conceptual_Object> ;
    rdfs:subPropertyOf <http://www.cidoc-crm.org/cidoc-crm/P92_brought_into_existence> ;
    owl:inverseOf <http://www.cidoc-crm.org/cidoc-crm/P94i_was_created_by> .

<http://www.cidoc-crm.org/cidoc-crm/P94i_was_created_by> a rdf:Property ;
    rdfs:label "wurde erschaffen durch"@de,
        "δημιουργήθηκε από"@el,
        "was created by"@en,
        "a été créé par"@fr,
        "foi criado por"@pt,
        "был создан"@ru,
        "被创建"@zh ;
    rdfs:domain <http://www.cidoc-crm.org/cidoc-crm/E28_Conceptual_Object> ;
    rdfs:range <http://www.cidoc-crm.org/cidoc-crm/E65_Creation> ;
    rdfs:subPropertyOf <http://www.cidoc-crm.org/cidoc-crm/P92i_was_brought_into_existence_by> ;
    owl:inverseOf <http://www.cidoc-crm.org/cidoc-crm/P94_has_created> .

<http://www.cidoc-crm.org/extensions/crmsci/O18_altered> a rdf:Property ;
    rdfs:label "altered"@en ;
    rdfs:comment "This property associates an instance of S18 Alteration process with an instance of E18 Physical Thing which was altered by this activity."@en ;
    rdfs:domain <http://www.cidoc-crm.org/extensions/crmsci/S18_Alteration> ;
    rdfs:range <http://www.cidoc-crm.org/cidoc-crm/E18_Physical_Thing> ;
    owl:inverseOf <http://www.cidoc-crm.org/extensions/crmsci/O18i_was_altered_by> .

<http://www.cidoc-crm.org/extensions/crmsci/O18i_was_altered_by> a rdf:Property ;
    rdfs:label "was altered by"@en ;
    rdfs:domain <http://www.cidoc-crm.org/cidoc-crm/E18_Physical_Thing> ;
    rdfs:range <http://www.cidoc-crm.org/extensions/crmsci/S18_Alteration> ;
    owl:inverseOf <http://www.cidoc-crm.org/extensions/crmsci/O18_altered> .

<http://www.cidoc-crm.org/cidoc-crm/P176_starts_before_the_start_of> a rdf:Property ;
    rdfs:label "starts before the start of"@en,
        "commence avant le début de"@fr,
        "начинаeтся до начала"@ru ;
    rdfs:comment """This property specifies that the temporal extent of the domain instance A of E2 Temporal Entity starts definitely before the start of the temporal extent of the range instance B of E2 Temporal Entity.
In other words, if A = [A-start, A-end] and B = [B-start, B-end], it means A-start &lt; B-start is true.
This property is part of the set of temporal primitives P173 – P176, P182 – P185.
This property corresponds to a disjunction (logical OR) of the following Allen temporal relations (Allen, 1983): {before, meets, overlaps, contains, finished-by}. This property is transitive. This property is asymmetric.

Figure 14: Temporal entity A starts before the start of temporal entity B. Here A is longer than B

Figure 15: Temporal entity A starts before the start of temporal entity B. Here A is shorter than B"""@en ;
    rdfs:domain <http://www.cidoc-crm.org/cidoc-crm/E2_Temporal_Entity> ;
    rdfs:range <http://www.cidoc-crm.org/cidoc-crm/E2_Temporal_Entity> ;
    rdfs:subPropertyOf <http://www.cidoc-crm.org/cidoc-crm/P175_starts_before_or_with_the_start_of> ;
    owl:inverseOf <http://www.cidoc-crm.org/cidoc-crm/P176i_starts_after_the_start_of> .

<http://www.cidoc-crm.org/cidoc-crm/P176i_starts_after_the_start_of> a rdf:Property ;
    rdfs:label "starts after the start of"@en,
        "commence après le début de"@fr,
        "начинаeтся послe начала"@ru ;
    rdfs:domain <http://www.cidoc-crm.org/cidoc-crm/E2_Temporal_Entity> ;
    rdfs:range <http://www.cidoc-crm.org/cidoc-crm/E2_Temporal_Entity> ;
    rdfs:subPropertyOf <http://www.cidoc-crm.org/cidoc-crm/P175i_starts_after_or_with_the_start_of> ;
    owl:inverseOf <http://www.cidoc-crm.org/cidoc-crm/P176_starts_before_the_start_of> .

<http://www.cidoc-crm.org/cidoc-crm/P92_brought_into_existence> a rdf:Property ;
    rdfs:label "brachte in Existenz"@de,
        "γέννησε"@el,
        "brought into existence"@en,
        "a fait exister"@fr,
        "trouxe à existência"@pt,
        "запустил в дeйствиe"@ru,
        "导致存在的是"@zh ;
    rdfs:comment """This property links an instance of E63 Beginning of Existence to the instance of E77 Persistent Item brought into existence by it.
It allows a “start” to be attached to any instance of E77 Persistent Item being documented, i.e., as instances of E70 Thing, E72 Legal Object, E39 Actor, E41 Appellation and E55 Type."""@en ;
    rdfs:domain <http://www.cidoc-crm.org/cidoc-crm/E63_Beginning_of_Existence> ;
    rdfs:range <http://www.cidoc-crm.org/cidoc-crm/E77_Persistent_Item> ;
    rdfs:subPropertyOf <http://www.cidoc-crm.org/cidoc-crm/P12_occurred_in_the_presence_of> ;
    owl:inverseOf <http://www.cidoc-crm.org/cidoc-crm/P92i_was_brought_into_existence_by> .

<http://www.cidoc-crm.org/cidoc-crm/P92i_was_brought_into_existence_by> a rdf:Property ;
    rdfs:label "wurde in Existenz gebracht durch"@de,
        "γεννήθηκε από"@el,
        "was brought into existence by"@en,
        "a commencé à exister par"@fr,
        "passou a existir por"@pt,
        "был пущeн в дeйствиe"@ru,
        "使导致存在"@zh ;
    rdfs:domain <http://www.cidoc-crm.org/cidoc-crm/E77_Persistent_Item> ;
    rdfs:range <http://www.cidoc-crm.org/cidoc-crm/E63_Beginning_of_Existence> ;
    rdfs:subPropertyOf <http://www.cidoc-crm.org/cidoc-crm/P12i_was_present_at> ;
    owl:inverseOf <http://www.cidoc-crm.org/cidoc-crm/P92_brought_into_existence> .

<http://www.cidoc-crm.org/cidoc-crm/P93_took_out_of_existence> a rdf:Property ;
    rdfs:label "beendete die Existenz von"@de,
        "αναίρεσε"@el,
        "took out of existence"@en,
        "a mis fin à l’existence de"@fr,
        "cessou a existência de"@pt,
        "положил конeц сущeствованию"@ru,
        "结束存在的是"@zh ;
    rdfs:comment """This property links an instance of E64 End of Existence to the instance of E77 Persistent Item taken out of existence by it.
In the case of immaterial things, the instance of E64 End of Existence is considered to take place with the destruction of the last physical carrier.
This allows an “end” to be attached to any instance of E77 Persistent Item being documented i.e. instances of E70 Thing, E72 Legal Object, E39 Actor, E41 Appellation, and E55 Type. For many instances of E77 Persistent Item we know the maximum life-span and can infer that they must have ended to exist. We assume in that case an instance of E64 End of Existence, which may be as unnoticeable as forgetting the secret knowledge by the last representative of some indigenous nation."""@en ;
    rdfs:domain <http://www.cidoc-crm.org/cidoc-crm/E64_End_of_Existence> ;
    rdfs:range <http://www.cidoc-crm.org/cidoc-crm/E77_Persistent_Item> ;
    rdfs:subPropertyOf <http://www.cidoc-crm.org/cidoc-crm/P12_occurred_in_the_presence_of> ;
    owl:inverseOf <http://www.cidoc-crm.org/cidoc-crm/P93i_was_taken_out_of_existence_by> .

<http://www.cidoc-crm.org/cidoc-crm/P93i_was_taken_out_of_existence_by> a rdf:Property ;
    rdfs:label "wurde seiner Existenz beraubt durch"@de,
        "αναιρέθηκε από"@el,
        "was taken out of existence by"@en,
        "a cessé d’exister par"@fr,
        "deixou de existir"@pt,
        "сущeствованиe было прeкращeно"@ru,
        "被结束存在"@zh ;
    rdfs:domain <http://www.cidoc-crm.org/cidoc-crm/E77_Persistent_Item> ;
    rdfs:range <http://www.cidoc-crm.org/cidoc-crm/E64_End_of_Existence> ;
    rdfs:subPropertyOf <http://www.cidoc-crm.org/cidoc-crm/P12i_was_present_at> ;
    owl:inverseOf <http://www.cidoc-crm.org/cidoc-crm/P93_took_out_of_existence> .

<http://www.cidoc-crm.org/cidoc-crm/P140_assigned_attribute_to> a rdf:Property ;
    rdfs:label "wies Merkmal zu"@de,
        "απέδωσε ιδιότητα σε"@el,
        "assigned attribute to"@en,
        "a assigné l’attribut à"@fr,
        "atribuiu atributo para"@pt,
        "получeн атрибут посрeдством"@ru,
        "分配属性于"@zh ;
    rdfs:comment """This property associates an instance of E13 Attribute Assignment with the instance of E1 CRM Entity about which it made an attribution. The instance of E1 CRM Entity plays the role of the domain of the attribution.
The kind of attribution made should be documented using P177 assigned property of type (is type of property assigned)."""@en ;
    rdfs:domain <http://www.cidoc-crm.org/cidoc-crm/E13_Attribute_Assignment> ;
    rdfs:range <http://www.cidoc-crm.org/cidoc-crm/E1_CRM_Entity> ;
    owl:inverseOf <http://www.cidoc-crm.org/cidoc-crm/P140i_was_attributed_by> .

<http://www.cidoc-crm.org/cidoc-crm/P140i_was_attributed_by> a rdf:Property ;
    rdfs:label "bekam Merkmal zugewiesen durch"@de,
        "χαρακτηρίστηκε από"@el,
        "was attributed by"@en,
        "a reçu l’attribut par"@fr,
        "foi atribuído por"@pt,
        "присвоeн атрибут"@ru,
        "接受属性"@zh ;
    rdfs:domain <http://www.cidoc-crm.org/cidoc-crm/E1_CRM_Entity> ;
    rdfs:range <http://www.cidoc-crm.org/cidoc-crm/E13_Attribute_Assignment> ;
    owl:inverseOf <http://www.cidoc-crm.org/cidoc-crm/P140_assigned_attribute_to> .

<http://www.cidoc-crm.org/cidoc-crm/P67_refers_to> a rdf:Property ;
    rdfs:label "verweist auf"@de,
        "αναφέρεται σε"@el,
        "refers to"@en,
        "renvoie à"@fr,
        "referencia"@pt,
        "ссылаeтся на"@ru,
        "涉及"@zh ;
    rdfs:comment "This property documents that an instance of E89 Propositional Object makes a statement about an instance of E1 CRM Entity. P67 refers to (is referred to by) has the P67.1 has type link to an instance of E55 Type. This is intended to allow a more detailed description of the type of reference. This differs from P129 is about (is subject of), which describes the primary subject or subjects of the instance of E89 Propositional Object."@en ;
    rdfs:domain <http://www.cidoc-crm.org/cidoc-crm/E89_Propositional_Object> ;
    rdfs:range <http://www.cidoc-crm.org/cidoc-crm/E1_CRM_Entity> ;
    owl:inverseOf <http://www.cidoc-crm.org/cidoc-crm/P67i_is_referred_to_by> .

<http://www.cidoc-crm.org/cidoc-crm/P67i_is_referred_to_by> a rdf:Property ;
    rdfs:label "wird angeführt von"@de,
        "αναφέρεται από"@el,
        "is referred to by"@en,
        "fait l'objet d'un renvoi par"@fr,
        "é referenciado por"@pt,
        "на который ссылаeтся"@ru,
        "被涉及"@zh ;
    rdfs:domain <http://www.cidoc-crm.org/cidoc-crm/E1_CRM_Entity> ;
    rdfs:range <http://www.cidoc-crm.org/cidoc-crm/E89_Propositional_Object> ;
    owl:inverseOf <http://www.cidoc-crm.org/cidoc-crm/P67_refers_to> .

<http://www.cidoc-crm.org/extensions/crmsci/O8_observed> a rdf:Property ;
    rdfs:label "observed"@en ;
    rdfs:comment "This property associates an instance of S4 Observation with an instance of S15 Observable Entity that was observed. Specifically it describes that a thing, a feature, a phenomenon or its reaction is observed by an activity of Observation."@en ;
    rdfs:domain <http://www.cidoc-crm.org/extensions/crmsci/S4_Observation> ;
    rdfs:range <http://www.cidoc-crm.org/extensions/crmsci/S15_Observable_Entity> ;
    rdfs:subPropertyOf <http://www.cidoc-crm.org/cidoc-crm/P140_assigned_attribute_to> ;
    owl:inverseOf <http://www.cidoc-crm.org/extensions/crmsci/O8i_was_observed_by> .

<http://www.cidoc-crm.org/extensions/crmsci/O8i_was_observed_by> a rdf:Property ;
    rdfs:label "was observed by"@en ;
    rdfs:domain <http://www.cidoc-crm.org/extensions/crmsci/S15_Observable_Entity> ;
    rdfs:range <http://www.cidoc-crm.org/extensions/crmsci/S4_Observation> ;
    rdfs:subPropertyOf <http://www.cidoc-crm.org/cidoc-crm/P140i_was_attributed_by> ;
    owl:inverseOf <http://www.cidoc-crm.org/extensions/crmsci/O8_observed> .

<http://www.cidoc-crm.org/cidoc-crm/P141_assigned> a rdf:Property ;
    rdfs:label "wies zu"@de,
        "απέδωσε"@el,
        "assigned"@en,
        "a attribué"@fr,
        "atribuiu"@pt,
        "назначил"@ru,
        "分配"@zh ;
    rdfs:comment """This property associates an instance of E13 Attribute Assignment with the instance of E1 CRM Entity used in the attribution. The instance of E1 CRM Entity here plays the role of the range of the attribution.
The kind of attribution made should be documented using P177 assigned property of type (is type of property assigned)."""@en ;
    rdfs:domain <http://www.cidoc-crm.org/cidoc-crm/E13_Attribute_Assignment> ;
    rdfs:range <http://www.cidoc-crm.org/cidoc-crm/E1_CRM_Entity> ;
    owl:inverseOf <http://www.cidoc-crm.org/cidoc-crm/P141i_was_assigned_by> .

<http://www.cidoc-crm.org/cidoc-crm/P141i_was_assigned_by> a rdf:Property ;
    rdfs:label "wurde zugewiesen durch"@de,
        "αποδόθηκε από"@el,
        "was assigned by"@en,
        "a été attribué par"@fr,
        "foi atribuído por"@pt,
        "назначeн посрeдством"@ru,
        "被分配"@zh ;
    rdfs:domain <http://www.cidoc-crm.org/cidoc-crm/E1_CRM_Entity> ;
    rdfs:range <http://www.cidoc-crm.org/cidoc-crm/E13_Attribute_Assignment> ;
    owl:inverseOf <http://www.cidoc-crm.org/cidoc-crm/P141_assigned> .

<http://www.cidoc-crm.org/cidoc-crm/P12_occurred_in_the_presence_of> a rdf:Property ;
    rdfs:label "fand statt im Beisein von"@de,
        "συνέβη παρουσία του/της"@el,
        "occurred in the presence of"@en,
        "a eu lieu en présence de"@fr,
        "ocorreu na presença de"@pt,
        "появился в присутствии"@ru,
        "已出现"@zh ;
    rdfs:comment """This property describes the active or passive presence of an E77 Persistent Item in an instance of E5 Event without implying any specific role.
It documents known events in which an instance of E77 Persistent Item was present during the course of its life or history. For example, an object may be the desk, now in a museum, on which a treaty was signed. The instance of E53 Place and the instance of E52 Time-Span where and when these events happened provide constraints about the presence of the related instance E77 Persistent Item in the past. Instances of E90 Symbolic Object, in particular information objects, are physically present in events via at least one of the instances of E18 Physical Thing carrying them. Note, that the human mind can be such a carrier. A precondition for a transfer of information to a person or another new physical carrier is the presence of the respective information object and this person or physical thing in one event."""@en ;
    rdfs:domain <http://www.cidoc-crm.org/cidoc-crm/E5_Event> ;
    rdfs:range <http://www.cidoc-crm.org/cidoc-crm/E77_Persistent_Item> ;
    owl:inverseOf <http://www.cidoc-crm.org/cidoc-crm/P12i_was_present_at> .

<http://www.cidoc-crm.org/cidoc-crm/P12i_was_present_at> a rdf:Property ;
    rdfs:label "war anwesend bei"@de,
        "ήταν παρών/παρούσα/παρόν σε"@el,
        "was present at"@en,
        "a été présent à"@fr,
        "estava presente no"@pt,
        "присутствовал при"@ru,
        "出现在"@zh ;
    rdfs:domain <http://www.cidoc-crm.org/cidoc-crm/E77_Persistent_Item> ;
    rdfs:range <http://www.cidoc-crm.org/cidoc-crm/E5_Event> ;
    owl:inverseOf <http://www.cidoc-crm.org/cidoc-crm/P12_occurred_in_the_presence_of> .

<http://www.cidoc-crm.org/cidoc-crm/P11_had_participant> a rdf:Property ;
    rdfs:label "hatte Teilnehmer"@de,
        "είχε συμμέτοχο"@el,
        "had participant"@en,
        "a eu pour actant participant"@fr,
        "tem participante"@pt,
        "имeл участника"@ru,
        "有参与者"@zh ;
    rdfs:comment """This property describes the active or passive participation of instances of E39 Actors in an instance of E5 Event.
It documents known events in which an instance of E39 Actor has participated during the course of that actor’s life or history. The instances of E53 Place and E52 Time-Span where and when these events happened provide constraints about the presence of the related instances of E39 Actor in the past. Collective actors, i.e. instances of E74 Group, may physically participate in events via their representing instances of E21 Persons only. The participation of multiple actors in an event is most likely an indication of their acquaintance and interaction.
The property implies that the actor was involved in the event but does not imply any causal relationship. For instance, someone having been portrayed can be said to have participated in the creation of the portrait."""@en ;
    rdfs:domain <http://www.cidoc-crm.org/cidoc-crm/E5_Event> ;
    rdfs:range <http://www.cidoc-crm.org/cidoc-crm/E39_Actor> ;
    rdfs:subPropertyOf <http://www.cidoc-crm.org/cidoc-crm/P12_occurred_in_the_presence_of> ;
    owl:inverseOf <http://www.cidoc-crm.org/cidoc-crm/P11i_participated_in> .

<http://www.cidoc-crm.org/cidoc-crm/P11i_participated_in> a rdf:Property ;
    rdfs:label "nahm Teil an"@de,
        "συμμετείχε σε"@el,
        "participated in"@en,
        "a participé à"@fr,
        "participa em"@pt,
        "участвовал в"@ru,
        "参与"@zh ;
    rdfs:domain <http://www.cidoc-crm.org/cidoc-crm/E39_Actor> ;
    rdfs:range <http://www.cidoc-crm.org/cidoc-crm/E5_Event> ;
    rdfs:subPropertyOf <http://www.cidoc-crm.org/cidoc-crm/P12i_was_present_at> ;
    owl:inverseOf <http://www.cidoc-crm.org/cidoc-crm/P11_had_participant> .

<http://www.cidoc-crm.org/cidoc-crm/P14i_performed> a rdf:Property ;
    rdfs:label "führte aus"@de,
        "πραγματοποίησε"@el,
        "performed"@en,
        "a effectué"@fr,
        "executou"@pt,
        "выполнял"@ru,
        "执行"@zh ;
    rdfs:domain <http://www.cidoc-crm.org/cidoc-crm/E39_Actor> ;
    rdfs:range <http://www.cidoc-crm.org/cidoc-crm/E7_Activity> ;
    rdfs:subPropertyOf <http://www.cidoc-crm.org/cidoc-crm/P11i_participated_in> ;
    owl:inverseOf <http://www.cidoc-crm.org/cidoc-crm/P14_carried_out_by> .

<http://www.cidoc-crm.org/cidoc-crm/P14_carried_out_by> a rdf:Property ;
    rdfs:label "wurde ausgeführt von"@de,
        "πραγματοποιήθηκε από"@el,
        "carried out by"@en,
        "a été effectué par"@fr,
        "realizada por"@pt,
        "выполнялся"@ru,
        "执行者是"@zh ;
    rdfs:comment """This property describes the active participation of an instance of E39 Actor in an instance of E7 Activity.
It implies causal or legal responsibility. The P14.1 in the role of property of the property specifies the nature of an Actor’s participation."""@en ;
    rdfs:domain <http://www.cidoc-crm.org/cidoc-crm/E7_Activity> ;
    rdfs:range <http://www.cidoc-crm.org/cidoc-crm/E39_Actor> ;
    rdfs:subPropertyOf <http://www.cidoc-crm.org/cidoc-crm/P11_had_participant> ;
    owl:inverseOf <http://www.cidoc-crm.org/cidoc-crm/P14i_performed> .

<http://www.cidoc-crm.org/cidoc-crm/P16_used_specific_object> a rdf:Property ;
    rdfs:label "benutzte das bestimmte Objekt"@de,
        "χρησιμοποίησε αντικείμενο"@el,
        "used specific object"@en,
        "a mobilisé l’objet spécifique"@fr,
        "usou objeto específico"@pt,
        "пользовался"@ru,
        "使用特定对象"@zh ;
    rdfs:comment """This property describes the use of material or immaterial things in a way essential to the performance or the outcome of an instance of E7 Activity.
This property typically applies to tools, instruments, moulds, raw materials and items embedded in a product. It implies that the presence of the object in question was a necessary condition for the action. For example, the activity of writing this text required the use of a computer. An immaterial thing can be used if at least one of its carriers is present. For example, the software tools on a computer.
Another example is the use of a particular name by a particular group of people over some span to identify a thing, such as a settlement. In this case, the physical carriers of this name are at least the people understanding its use."""@en ;
    rdfs:domain <http://www.cidoc-crm.org/cidoc-crm/E7_Activity> ;
    rdfs:range <http://www.cidoc-crm.org/cidoc-crm/E70_Thing> ;
    rdfs:subPropertyOf <http://www.cidoc-crm.org/cidoc-crm/P12_occurred_in_the_presence_of>,
        <http://www.cidoc-crm.org/cidoc-crm/P15_was_influenced_by> ;
    owl:inverseOf <http://www.cidoc-crm.org/cidoc-crm/P16i_was_used_for> .

<http://www.cidoc-crm.org/cidoc-crm/P16i_was_used_for> a rdf:Property ;
    rdfs:label "wurde benutzt für"@de,
        "χρησιμοποιήθηκε για"@el,
        "was used for"@en,
        "a été mobilisé pour"@fr,
        "foi usado por"@pt,
        "был использован"@ru,
        "用于"@zh ;
    rdfs:domain <http://www.cidoc-crm.org/cidoc-crm/E70_Thing> ;
    rdfs:range <http://www.cidoc-crm.org/cidoc-crm/E7_Activity> ;
    rdfs:subPropertyOf <http://www.cidoc-crm.org/cidoc-crm/P12i_was_present_at>,
        <http://www.cidoc-crm.org/cidoc-crm/P15i_influenced> ;
    owl:inverseOf <http://www.cidoc-crm.org/cidoc-crm/P16_used_specific_object> .

<https://ontology.swissartresearch.net/aaao/ZP2_ascribes_intentional_target> a rdf:Property ;
    rdfs:label "ascribes intentional target"@en ;
    rdfs:comment "This property is used to indicate the entity which an instance of institutional fact ascribes to its subject. The intentional target indicated by this property is the object which the institutional fact establishes as holding of its subject for the group committed to this institutional reality. The manner of its holding is indicated by the intentional relation."@en ;
    rdfs:domain <https://ontology.swissartresearch.net/aaao/ZE1_Institutional_Fact> ;
    rdfs:range <http://www.cidoc-crm.org/cidoc-crm/E1_CRM_Entity> ;
    skos:notation "ZP2"^^xsd:string .

<https://ontology.swissartresearch.net/aaao/ZP1_has_intentional_subject> a rdf:Property ;
    rdfs:label "has intentional subject"@en ;
    rdfs:comment "This property is used to connect an instance of institutional fact to an entity with which it is concerned. The intentional subject indicated by this property is the object about which the institutional fact holds for the group committed to this institutional reality."@en ;
    rdfs:domain <https://ontology.swissartresearch.net/aaao/ZE1_Institutional_Fact> ;
    rdfs:range <http://www.cidoc-crm.org/cidoc-crm/E1_CRM_Entity> ;
    skos:notation "ZP1"^^xsd:string .

<https://ontology.swissartresearch.net/aaao/ZP3_ascribes_intentional_relation> a rdf:Property ;
    rdfs:label "ascribes intentional relation"@en ;
    rdfs:comment "This property is used to indicate the relationship which an instance of institutional fact takes to hold between its subject and its object. The intentional relation indicated by this property is the kind of relationship which the institutional fact establishes as holding between them for the group committed to this institutional reality."@en ;
    rdfs:domain <https://ontology.swissartresearch.net/aaao/ZE1_Institutional_Fact> ;
    rdfs:range <http://www.cidoc-crm.org/cidoc-crm/E55_Type> ;
    skos:notation "ZP3"^^xsd:string .

<https://ontology.swissartresearch.net/aaao/ZP1i_is_intentional_subject_of> a rdf:Property ;
    rdfs:label "is intentional subject of"@en ;
    rdfs:comment "This property is the inverse of the forward property described in the scope note that follows. This property is used to connect an instance of institutional fact to an entity with which it is concerned. The intentional subject indicated by this property is the object about which the institutional fact holds for the group committed to this institutional reality."@en ;
    rdfs:domain <http://www.cidoc-crm.org/cidoc-crm/E1_CRM_Entity> ;
    rdfs:range <https://ontology.swissartresearch.net/aaao/ZE1_Institutional_Fact> ;
    skos:notation "ZP1i"^^xsd:string .

<https://ontology.swissartresearch.net/aaao/ZP2i_is_intentional_target_ascribed_by> a rdf:Property ;
    rdfs:label "is intentional target ascribed  by"@en ;
    rdfs:comment "This property is the inverse of the forward property described in the scope note that follows. This property is used to indicate the entity which an instance of institutional fact ascribes to its subject. The intentional target indicated by this property is the object which the institutional fact establishes as holding of its subject for the group committed to this institutional reality. The manner of its holding is indicated by the intentional relation."@en ;
    rdfs:domain <http://www.cidoc-crm.org/cidoc-crm/E1_CRM_Entity> ;
    rdfs:range <https://ontology.swissartresearch.net/aaao/ZE1_Institutional_Fact> ;
    skos:notation "ZP2i"^^xsd:string .

<https://ontology.swissartresearch.net/aaao/ZP3i_is_intentional_relation_ascribed_by> a rdf:Property ;
    rdfs:label "is intentional relation ascribed by"@en ;
    rdfs:comment "This property is the inverse of the forward property described in the scope note that follows. This property is used to indicate the relationship which an instance of institutional fact takes to hold between its subject and its object. The intentional relation indicated by this property is the kind of relationship which the institutional fact establishes as holding between them  for the group committed to this institutional reality."@en ;
    rdfs:domain <http://www.cidoc-crm.org/cidoc-crm/E55_Type> ;
    rdfs:range <https://ontology.swissartresearch.net/aaao/ZE1_Institutional_Fact> ;
    skos:notation "ZP3i"^^xsd:string .

